@prefix crm: <http://www.cidoc-crm.org/cidoc-crm/> .
@prefix crmeh: <http://purl.org/crmeh#> .
@prefix data: <http://www.w3.org/ns/formats/data/> .
@prefix dc: <http://purl.org/dc/elements/1.1/> .
@prefix dcam: <http://purl.org/dc/dcam/> .
@prefix dcat: <http://www.w3.org/ns/dcat#> .
@prefix dcterms: <http://purl.org/dc/terms/> .
@prefix dctypes: <http://purl.org/dc/dcmitype/> .
@prefix eu: <http://ec.europa.eu/> .
@prefix foaf: <http://xmlns.com/foaf/0.1/> .
@prefix geosparql: <http://www.opengis.net/ont/geosparql#> .
@prefix gn: <http://www.geonames.org/ontology#> .
@prefix history: <http://dublincore.org/usage/terms/history/#> .
@prefix jrc: <https://ec.europa.eu/jrc/> .
@prefix licence: <https://joinup.ec.europa.eu/category/licence/> .
@prefix locn: <http://www.w3.org/ns/locn#> .
@prefix ns: <http://creativecommons.org/ns#> .
@prefix ns1: <http://www.w3.org/ns/adms#> .
@prefix ns2: <http://www.w3.org/2001/02pd/rec54#> .
@prefix ns3: <http://www.w3.org/2003/g/data-view#> .
@prefix ns4: <http://id.loc.gov/vocabulary/relators/> .
@prefix org: <http://schema.org/> .
@prefix owl: <http://www.w3.org/2002/07/owl#> .
@prefix owl2-rdf-based-semantics: <http://www.w3.org/TR/owl2-rdf-based-semantics/#> .
@prefix person: <http://data.semanticweb.org/person/> .
@prefix powder-s: <http://www.w3.org/2007/05/powder-s#> .
@prefix rdf: <http://www.w3.org/1999/02/22-rdf-syntax-ns#> .
@prefix rdf11-concepts: <http://www.w3.org/TR/rdf11-concepts/#> .
@prefix rdfs: <http://www.w3.org/2000/01/rdf-schema#> .
@prefix resource: <http://dbpedia.org/resource/> .
@prefix skos: <http://www.w3.org/2004/02/skos/core#> .
@prefix swvocab: <http://www.w3.org/2003/06/sw-vocab-status/ns#> .
@prefix vann: <http://purl.org/vocab/vann/> .
@prefix voaf: <http://purl.org/vocommons/voaf#> .
@prefix wgs84: <http://www.w3.org/2003/01/geo/wgs84_pos#> .
@prefix wot: <http://xmlns.com/wot/0.1/> .
@prefix xml: <http://www.w3.org/XML/1998/namespace> .
@prefix xsd: <http://www.w3.org/2001/XMLSchema#> .

dcterms:Agent a dcterms:AgentClass,
        rdfs:Class ;
    rdfs:label "Agent"@en ;
    dcterms:description "Examples of Agent include person, organization, and software agent."@en ;
    dcterms:hasVersion history:Agent-001 ;
    dcterms:issued "2008-01-14"^^xsd:date ;
    rdfs:comment "A resource that acts or has the power to act."@en ;
    rdfs:isDefinedBy dcterms: .

dcterms:AgentClass a rdfs:Class ;
    rdfs:label "Agent Class"@en ;
    dcterms:description "Examples of Agent Class include groups seen as classes, such as students, women, charities, lecturers."@en ;
    dcterms:hasVersion history:AgentClass-003 ;
    dcterms:issued "2008-01-14"^^xsd:date ;
    dcterms:modified "2012-06-14"^^xsd:date ;
    rdfs:comment "A group of agents."@en ;
    rdfs:isDefinedBy dcterms: ;
    rdfs:subClassOf rdfs:Class .

dcterms:BibliographicResource a rdfs:Class ;
    rdfs:label "Bibliographic Resource"@en ;
    dcterms:hasVersion history:BibliographicResource-001 ;
    dcterms:issued "2008-01-14"^^xsd:date ;
    rdfs:comment "A book, article, or other documentary resource."@en ;
    rdfs:isDefinedBy dcterms: .

dcterms:FileFormat a rdfs:Class ;
    rdfs:label "File Format"@en ;
    dcterms:description "Examples include the formats defined by the list of Internet Media Types."@en ;
    dcterms:hasVersion history:FileFormat-001 ;
    dcterms:issued "2008-01-14"^^xsd:date ;
    rdfs:comment "A digital resource format."@en ;
    rdfs:isDefinedBy dcterms: ;
    rdfs:subClassOf dcterms:MediaType .

dcterms:Frequency a rdfs:Class ;
    rdfs:label "Frequency"@en ;
    dcterms:hasVersion history:Frequency-001 ;
    dcterms:issued "2008-01-14"^^xsd:date ;
    rdfs:comment "A rate at which something recurs."@en ;
    rdfs:isDefinedBy dcterms: .

dcterms:Jurisdiction a rdfs:Class ;
    rdfs:label "Jurisdiction"@en ;
    dcterms:hasVersion history:Jurisdiction-001 ;
    dcterms:issued "2008-01-14"^^xsd:date ;
    rdfs:comment "The extent or range of judicial, law enforcement, or other authority."@en ;
    rdfs:isDefinedBy dcterms: ;
    rdfs:subClassOf dcterms:LocationPeriodOrJurisdiction .

dcterms:LicenseDocument a rdfs:Class ;
    rdfs:label "License Document"@en ;
    dcterms:hasVersion history:LicenseDocument-001 ;
    dcterms:issued "2008-01-14"^^xsd:date ;
    rdfs:comment "A legal document giving official permission to do something with a Resource."@en ;
    rdfs:isDefinedBy dcterms: ;
    rdfs:subClassOf dcterms:RightsStatement .

dcterms:LinguisticSystem a rdfs:Class ;
    rdfs:label "Linguistic System"@en ;
    dcterms:description "Examples include written, spoken, sign, and computer languages."@en ;
    dcterms:hasVersion history:LinguisticSystem-001 ;
    dcterms:issued "2008-01-14"^^xsd:date ;
    rdfs:comment "A system of signs, symbols, sounds, gestures, or rules used in communication."@en ;
    rdfs:isDefinedBy dcterms: .

dcterms:Location a rdfs:Class ;
    rdfs:label "Location"@en ;
    dcterms:hasVersion history:Location-001 ;
    dcterms:identifier "dcterms:Location" ;
    dcterms:issued "2008-01-14"^^xsd:date ;
    vann:usageNote "This is the key class for the ISA Programme Location Core Vocabulary and represents any location, irrespective of size or other restriction."@en ;
    rdfs:comment "A spatial region or named place."@en,
        "dcterms:Location class fully represents the ISA Programme Location Core Vocabulary class of Location."@en ;
    rdfs:isDefinedBy dcterms: ;
    rdfs:subClassOf dcterms:LocationPeriodOrJurisdiction ;
    swvocab:term_status "testing"@en .

dcterms:LocationPeriodOrJurisdiction a rdfs:Class ;
    rdfs:label "Location, Period, or Jurisdiction"@en ;
    dcterms:hasVersion history:LocationPeriodOrJurisdiction-001 ;
    dcterms:issued "2008-01-14"^^xsd:date ;
    rdfs:comment "A location, period of time, or jurisdiction."@en ;
    rdfs:isDefinedBy dcterms: .

dcterms:MediaType a rdfs:Class ;
    rdfs:label "Media Type"@en ;
    dcterms:hasVersion history:MediaType-001 ;
    dcterms:issued "2008-01-14"^^xsd:date ;
    rdfs:comment "A file format or physical medium."@en ;
    rdfs:isDefinedBy dcterms: ;
    rdfs:subClassOf dcterms:MediaTypeOrExtent .

dcterms:MediaTypeOrExtent a rdfs:Class ;
    rdfs:label "Media Type or Extent"@en ;
    dcterms:hasVersion history:MediaTypeOrExtent-001 ;
    dcterms:issued "2008-01-14"^^xsd:date ;
    rdfs:comment "A media type or extent."@en ;
    rdfs:isDefinedBy dcterms: .

dcterms:MethodOfAccrual a rdfs:Class ;
    rdfs:label "Method of Accrual"@en ;
    dcterms:hasVersion history:MethodOfAccrual-001 ;
    dcterms:issued "2008-01-14"^^xsd:date ;
    rdfs:comment "A method by which resources are added to a collection."@en ;
    rdfs:isDefinedBy dcterms: .

dcterms:MethodOfInstruction a rdfs:Class ;
    rdfs:label "Method of Instruction"@en ;
    dcterms:hasVersion history:MethodOfInstruction-001 ;
    dcterms:issued "2008-01-14"^^xsd:date ;
    rdfs:comment "A process that is used to engender knowledge, attitudes, and skills."@en ;
    rdfs:isDefinedBy dcterms: .

dcterms:PeriodOfTime a rdfs:Class ;
    rdfs:label "Period of Time"@en ;
    dcterms:hasVersion history:PeriodOfTime-001 ;
    dcterms:issued "2008-01-14"^^xsd:date ;
    rdfs:comment "An interval of time that is named or defined by its start and end dates."@en ;
    rdfs:isDefinedBy dcterms: ;
    rdfs:subClassOf dcterms:LocationPeriodOrJurisdiction .

dcterms:PhysicalMedium a rdfs:Class ;
    rdfs:label "Physical Medium"@en ;
    dcterms:description "Examples include paper, canvas, or DVD."@en ;
    dcterms:hasVersion history:PhysicalMedium-001 ;
    dcterms:issued "2008-01-14"^^xsd:date ;
    rdfs:comment "A physical material or carrier."@en ;
    rdfs:isDefinedBy dcterms: ;
    rdfs:subClassOf dcterms:MediaType .

dcterms:PhysicalResource a rdfs:Class ;
    rdfs:label "Physical Resource"@en ;
    dcterms:hasVersion history:PhysicalResource-001 ;
    dcterms:issued "2008-01-14"^^xsd:date ;
    rdfs:comment "A material thing."@en ;
    rdfs:isDefinedBy dcterms: .

dcterms:Policy a rdfs:Class ;
    rdfs:label "Policy"@en ;
    dcterms:hasVersion history:Policy-001 ;
    dcterms:issued "2008-01-14"^^xsd:date ;
    rdfs:comment "A plan or course of action by an authority, intended to influence and determine decisions, actions, and other matters."@en ;
    rdfs:isDefinedBy dcterms: .

dcterms:ProvenanceStatement a rdfs:Class ;
    rdfs:label "Provenance Statement"@en ;
    dcterms:hasVersion history:ProvenanceStatement-001 ;
    dcterms:issued "2008-01-14"^^xsd:date ;
    rdfs:comment "A statement of any changes in ownership and custody of a resource since its creation that are significant for its authenticity, integrity, and interpretation."@en ;
    rdfs:isDefinedBy dcterms: .

dcterms:RightsStatement a rdfs:Class ;
    rdfs:label "Rights Statement"@en ;
    dcterms:hasVersion history:RightsStatement-001 ;
    dcterms:issued "2008-01-14"^^xsd:date ;
    rdfs:comment "A statement about the intellectual property rights (IPR) held in or over a Resource, a legal document giving official permission to do something with a resource, or a statement about access rights."@en ;
    rdfs:isDefinedBy dcterms: .

dcterms:SizeOrDuration a rdfs:Class ;
    rdfs:label "Size or Duration"@en ;
    dcterms:description "Examples include a number of pages, a specification of length, width, and breadth, or a period in hours, minutes, and seconds."@en ;
    dcterms:hasVersion history:SizeOrDuration-001 ;
    dcterms:issued "2008-01-14"^^xsd:date ;
    rdfs:comment "A dimension or extent, or a time taken to play or execute."@en ;
    rdfs:isDefinedBy dcterms: ;
    rdfs:subClassOf dcterms:MediaTypeOrExtent .

dcterms:Standard a rdfs:Class ;
    rdfs:label "Standard"@en ;
    dcterms:hasVersion history:Standard-001 ;
    dcterms:issued "2008-01-14"^^xsd:date ;
    rdfs:comment "A basis for comparison; a reference point against which other things can be evaluated."@en ;
    rdfs:isDefinedBy dcterms: .

crm:E10_Transfer_of_Custody a rdfs:Class ;
    rdfs:label "Übertragung des Gewahrsams"@de,
        "Μεταβίβαση  Κατοχής"@el,
        "Transfer of Custody"@en,
        "Changement de détenteur"@fr,
        "Transferência de Custódia"@pt,
        "Передача Опеки"@ru ;
    rdfs:comment """This class comprises transfers of physical custody of objects between instances of E39 Actor. 
The recording of the donor and/or recipient is optional. It is possible that in an instance of E10 Transfer of Custody there is either no donor or no recipient. Depending on the circumstances it may describe:
1.	the beginning of custody 
2.	the end of custody 
3.	the transfer of custody 
4.	the receipt of custody from an unknown source
5.	the declared loss of an object
The distinction between the legal responsibility for custody and the actual physical possession of the object should be expressed using the property P2 has type (is type of). A specific case of transfer of custody is theft.
The interpretation of the museum notion of "accession" differs between institutions. The CRM therefore models legal ownership and physical custody separately. Institutions will then model their specific notions of accession and deaccession as combinations of these."""@en ;
    rdfs:subClassOf crm:E7_Activity .

crm:E11_Modification a rdfs:Class ;
    rdfs:label "Bearbeitung"@de,
        "Τροποποίηση"@el,
        "Modification"@en,
        "Modification"@fr,
        "Modificação"@pt,
        "Событие Изменения"@ru ;
    rdfs:comment """This class comprises all instances of E7 Activity that create, alter or change E24 Physical Man-Made Thing. 
This class includes the production of an item from raw materials, and other so far undocumented objects, and the preventive treatment or restoration of an object for conservation. 
Since the distinction between modification and production is not always clear, modification is regarded as the more generally applicable concept. This implies that some items may be consumed or destroyed in a Modification, and that others may be produced as a result of it. An event should also be documented using E81 Transformation if it results in the destruction of one or more objects and the simultaneous production of others using parts or material from the originals. In this case, the new items have separate identities. 
If the instance of the E29 Design or Procedure utilized for the modification prescribes the use of specific materials, they should be documented using property P68 foresees use of (use foreseen by): E57 Material of E29 Design or Procedure, rather than via P126 employed (was employed in): E57 Material."""@en ;
    rdfs:subClassOf crm:E7_Activity .

crm:E12_Production a rdfs:Class ;
    rdfs:label "Herstellung"@de,
        "Παραγωγή"@el,
        "Production"@en,
        "Production"@fr,
        "Produção"@pt,
        "Событие Производства"@ru ;
    rdfs:comment """This class comprises activities that are designed to, and succeed in, creating one or more new items. 
It specializes the notion of modification into production. The decision as to whether or not an object is regarded as new is context sensitive. Normally, items are considered “new” if there is no obvious overall similarity between them and the consumed items and material used in their production. In other cases, an item is considered “new” because it becomes relevant to documentation by a modification. For example, the scribbling of a name on a potsherd may make it a voting token. The original potsherd may not be worth documenting, in contrast to the inscribed one. 
This entity can be collective: the printing of a thousand books, for example, would normally be considered a single event. 
An event should also be documented using E81 Transformation if it results in the destruction of one or more objects and the simultaneous production of others using parts or material from the originals. In this case, the new items have separate identities and matter is preserved, but identity is not."""@en ;
    rdfs:subClassOf crm:E11_Modification,
        crm:E63_Beginning_of_Existence .

crm:E13_Attribute_Assignment a rdfs:Class ;
    rdfs:label "Merkmalszuweisung"@de,
        "Απόδοση Ιδιοτήτων"@el,
        "Attribute Assignment"@en,
        "Affectation d'attribut"@fr,
        "Atribuição de Característica"@pt,
        "Присвоение Атрибута"@ru ;
    rdfs:comment """This class comprises the actions of making assertions about properties of an object or any relation between two items or concepts. 
This class allows the documentation of how the respective assignment came about, and whose opinion it was. All the attributes or properties assigned in such an action can also be seen as directly attached to the respective item or concept, possibly as a collection of contradictory values. All cases of properties in this model that are also described indirectly through an action are characterised as "short cuts" of this action. This redundant modelling of two alternative views is preferred because many implementations may have good reasons to model either the action or the short cut, and the relation between both alternatives can be captured by simple rules. 
In particular, the class describes the actions of people making propositions and statements during certain museum procedures, e.g. the person and date when a condition statement was made, an identifier was assigned, the museum object was measured, etc. Which kinds of such assignments and statements need to be documented explicitly in structures of a schema rather than free text, depends on if this information should be accessible by structured queries. """@en ;
    rdfs:subClassOf crm:E7_Activity .

crm:E14_Condition_Assessment a rdfs:Class ;
    rdfs:label "Zustandsfeststellung"@de,
        "Εκτίμηση Κατάστασης"@el,
        "Condition Assessment"@en,
        "Expertise de l'état matériel"@fr,
        "Avaliação do Estado Material"@pt,
        "Оценка Состояния"@ru ;
    rdfs:comment """This class describes the act of assessing the state of preservation of an object during a particular period. 
The condition assessment may be carried out by inspection, measurement or through historical research. This class is used to document circumstances of the respective assessment that may be relevant to interpret its quality at a later stage, or to continue research on related documents. """@en ;
    rdfs:subClassOf crm:E13_Attribute_Assignment .

crm:E15_Identifier_Assignment a rdfs:Class ;
    rdfs:label "Kennzeichenzuweisung"@de,
        "Απόδοση Αναγνωριστικού"@el,
        "Identifier Assignment"@en,
        "Attribution d’identificateur"@fr,
        "Atribuição de Identificador"@pt,
        "Назначение Идентификатора"@ru ;
    rdfs:comment """This class comprises activities that result in the allocation of an identifier to an instance of E1 CRM Entity. An E15 Identifier Assignment may include the creation of the identifier from multiple constituents, which themselves may be instances of E41 Appellation. The syntax and kinds of constituents to be used may be declared in a rule constituting an instance of E29 Design or Procedure.
Examples of such identifiers include Find Numbers, Inventory Numbers, uniform titles in the sense of librarianship and Digital Object Identifiers (DOI). Documenting the act of identifier assignment and deassignment is especially useful when objects change custody or the identification system of an organization is changed. In order to keep track of the identity of things in such cases, it is important to document by whom, when and for what purpose an identifier is assigned to an item.
The fact that an identifier is a preferred one for an organisation can be expressed by using the property E1 CRM Entity. P48 has preferred identifier (is preferred identifier of): E42 Identifier. It can better be expressed in a context independent form by assigning a suitable E55 Type, such as “preferred identifier assignment”, to the respective instance of E15 Identifier Assignment via the P2 has type property."""@en ;
    rdfs:subClassOf crm:E13_Attribute_Assignment .

crm:E16_Measurement a rdfs:Class ;
    rdfs:label "Messung"@de,
        "Μέτρηση"@el,
        "Measurement"@en,
        "Mesurage"@fr,
        "Medição"@pt,
        "Событие Измерения"@ru ;
    rdfs:comment """This class comprises actions measuring physical properties and other values that can be determined by a systematic procedure. 
Examples include measuring the monetary value of a collection of coins or the running time of a specific video cassette. 
The E16 Measurement may use simple counting or tools, such as yardsticks or radiation detection devices. The interest is in the method and care applied, so that the reliability of the result may be judged at a later stage, or research continued on the associated documents. The date of the event is important for dimensions, which may change value over time, such as the length of an object subject to shrinkage. Details of methods and devices are best handled as free text, whereas basic techniques such as "carbon 14 dating" should be encoded using P2 has type (is type of:) E55 Type."""@en ;
    rdfs:subClassOf crm:E13_Attribute_Assignment .

crm:E17_Type_Assignment a rdfs:Class ;
    rdfs:label "Typuszuweisung"@de,
        "Απόδοση Τύπου"@el,
        "Type Assignment"@en,
        "Attribution de type"@fr,
        "Atribuição de Tipo"@pt,
        "Присвоение Типа"@ru ;
    rdfs:comment """This class comprises the actions of classifying items of whatever kind. Such items include objects, specimens, people, actions and concepts. 
This class allows for the documentation of the context of classification acts in cases where the value of the classification depends on the personal opinion of the classifier, and the date that the classification was made. This class also encompasses the notion of "determination," i.e. the systematic and molecular identification of a specimen in biology. """@en ;
    rdfs:subClassOf crm:E13_Attribute_Assignment .

crm:E18_Physical_Thing a rdfs:Class ;
    rdfs:label "Materielles"@de,
        "Υλικό Πράγμα"@el,
        "Physical Thing"@en,
        "Chose matérielle"@fr,
        "Coisa Material"@pt,
        "Физическая Вещь"@ru ;
    rdfs:comment """This class comprises all persistent physical items with a relatively stable form, man-made or natural. 
Depending on the existence of natural boundaries of such things, the CRM distinguishes the instances of E19 Physical Object from instances of E26 Physical Feature, such as holes, rivers, pieces of land etc. Most instances of E19 Physical Object can be moved (if not too heavy), whereas features are integral to the surrounding matter. 
The CRM is generally not concerned with amounts of matter in fluid or gaseous states. """@en ;
    rdfs:subClassOf crm:E72_Legal_Object .

crm:E19_Physical_Object a rdfs:Class ;
    rdfs:label "Materieller Gegenstand"@de,
        "Υλικό Αντικείμενο"@el,
        "Physical Object"@en,
        "Objet matériel"@fr,
        "Objeto Material"@pt,
        "Физический Объект"@ru ;
    rdfs:comment """This class comprises items of a material nature that are units for documentation and have physical boundaries that separate them completely in an objective way from other objects. 
The class also includes all aggregates of objects made for functional purposes of whatever kind, independent of physical coherence, such as a set of chessmen. Typically, instances of E19 Physical Object can be moved (if not too heavy).
In some contexts, such objects, except for aggregates, are also called “bona fide objects” (Smith & Varzi, 2000, pp.401-420), i.e. naturally defined objects. 
The decision as to what is documented as a complete item, rather than by its parts or components, may be a purely administrative decision or may be a result of the order in which the item was acquired."""@en ;
    rdfs:subClassOf crm:E18_Physical_Thing .

crm:E1_CRM_Entity a rdfs:Class ;
    rdfs:label "CRM Entität"@de,
        "Οντότητα CIDOC CRM"@el,
        "CRM Entity"@en,
        "Entité CRM"@fr,
        "Entidade CRM"@pt,
        "CRM Сущность"@ru ;
    rdfs:comment """This class comprises all things in the universe of discourse of the CIDOC Conceptual Reference Model. 
It is an abstract concept providing for three general properties:
1.	Identification by name or appellation, and in particular by a preferred identifier
2.	Classification by type, allowing further refinement of the specific subclass an instance belongs to 
3.	Attachment of free text for the expression of anything not captured by formal properties
With the exception of E59 Primitive Value, all other classes within the CRM are directly or indirectly specialisations of E1 CRM Entity. """@en .

crm:E20_Biological_Object a rdfs:Class ;
    rdfs:label "Biologischer Gegenstand"@de,
        "Βιολογικό Ακτικείμενο"@el,
        "Biological Object"@en,
        "Objet biologique"@fr,
        "Objeto Biológico"@pt,
        "Биологический Объект"@ru ;
    rdfs:comment """This class comprises individual items of a material nature, which live, have lived or are natural products of or from living organisms. 
Artificial objects that incorporate biological elements, such as Victorian butterfly frames, can be documented as both instances of E20 Biological Object and E22 Man-Made Object. """@en ;
    rdfs:subClassOf crm:E19_Physical_Object .

crm:E21_Person a rdfs:Class ;
    rdfs:label "Person"@de,
        "Πρόσωπο"@el,
        "Person"@en,
        "Personne"@fr,
        "Pessoa"@pt,
        "Личность"@ru ;
    rdfs:comment """This class comprises real persons who live or are assumed to have lived. 
Legendary figures that may have existed, such as Ulysses and King Arthur, fall into this class if the documentation refers to them as historical figures. In cases where doubt exists as to whether several persons are in fact identical, multiple instances can be created and linked to indicate their relationship. The CRM does not propose a specific form to support reasoning about possible identity."""@en ;
    rdfs:subClassOf crm:E20_Biological_Object,
        crm:E39_Actor .

crm:E22_Man-Made_Object a rdfs:Class ;
    rdfs:label "Künstlicher Gegenstand"@de,
        "Ανθρωπογενές Αντικείμενο"@el,
        "Man-Made Object"@en,
        "Objet fabriqué"@fr,
        "Objeto Fabricado"@pt,
        "Рукотворный Объект"@ru ;
    rdfs:comment """This class comprises physical objects purposely created by human activity.
No assumptions are made as to the extent of modification required to justify regarding an object as man-made. For example, an inscribed piece of rock or a preserved butterfly are both regarded as instances of E22 Man-Made Object."""@en ;
    rdfs:subClassOf crm:E19_Physical_Object,
        crm:E24_Physical_Man-Made_Thing .

crm:E24_Physical_Man-Made_Thing a rdfs:Class ;
    rdfs:label "Hergestelltes"@de,
        "Ανθρωπογενές Υλικό Πράγμα"@el,
        "Physical Man-Made Thing"@en,
        "Chose matérielle fabriquée"@fr,
        "Coisa Material Fabricada"@pt,
        "Физическая Рукотворная Вещь"@ru ;
    rdfs:comment """This class comprises all persistent physical items that are purposely created by human activity.
This class comprises man-made objects, such as a swords, and man-made features, such as rock art. No assumptions are made as to the extent of modification required to justify regarding an object as man-made. For example, a “cup and ring” carving on bedrock is regarded as instance of E24 Physical Man-Made Thing. """@en ;
    rdfs:subClassOf crm:E18_Physical_Thing,
        crm:E71_Man-Made_Thing .

crm:E25_Man-Made_Feature a rdfs:Class ;
    rdfs:label "Hergestelltes Merkmal"@de,
        "Ανθρωπογενές Μόρφωμα"@el,
        "Man-Made Feature"@en,
        "Caractéristique fabriquée"@fr,
        "Característica Fabricada"@pt,
        "Искусственный Признак"@ru ;
    rdfs:comment """This class comprises physical features that are purposely created by human activity, such as scratches, artificial caves, artificial water channels, etc. 
No assumptions are made as to the extent of modification required to justify regarding a feature as man-made. For example, rock art or even “cup and ring” carvings on bedrock a regarded as types of E25 Man-Made Feature."""@en ;
    rdfs:subClassOf crm:E24_Physical_Man-Made_Thing,
        crm:E26_Physical_Feature .

crm:E26_Physical_Feature a rdfs:Class ;
    rdfs:label "Materielles Merkmal"@de,
        "Υλικό Μόρφωμα"@el,
        "Physical Feature"@en,
        "Caractéristique matérielle"@fr,
        "Característica Material"@pt,
        "Физический Признак"@ru ;
    rdfs:comment """This class comprises identifiable features that are physically attached in an integral way to particular physical objects. 
Instances of E26 Physical Feature share many of the attributes of instances of E19 Physical Object. They may have a one-, two- or three-dimensional geometric extent, but there are no natural borders that separate them completely in an objective way from the carrier objects. For example, a doorway is a feature but the door itself, being attached by hinges, is not. 
Instances of E26 Physical Feature can be features in a narrower sense, such as scratches, holes, reliefs, surface colours, reflection zones in an opal crystal or a density change in a piece of wood. In the wider sense, they are portions of particular objects with partially imaginary borders, such as the core of the Earth, an area of property on the surface of the Earth, a landscape or the head of a contiguous marble statue. They can be measured and dated, and it is sometimes possible to state who or what is or was responsible for them. They cannot be separated from the carrier object, but a segment of the carrier object may be identified (or sometimes removed) carrying the complete feature. 
This definition coincides with the definition of "fiat objects" (Smith & Varzi, 2000, pp.401-420), with the exception of aggregates of “bona fide objects”. """@en ;
    rdfs:subClassOf crm:E18_Physical_Thing .

crm:E27_Site a rdfs:Class ;
    rdfs:label "Gelände"@de,
        "Φυσικός Χώρος"@el,
        "Site"@en,
        "Site"@fr,
        "Lugar"@pt,
        "Участок"@ru ;
    rdfs:comment """This class comprises pieces of land or sea floor. 
In contrast to the purely geometric notion of E53 Place, this class describes constellations of matter on the surface of the Earth or other celestial body, which can be represented by photographs, paintings and maps.
 Instances of E27 Site are composed of relatively immobile material items and features in a particular configuration at a particular location"""@en ;
    rdfs:subClassOf crm:E26_Physical_Feature .

crm:E28_Conceptual_Object a rdfs:Class ;
    rdfs:label "Begrifflicher Gegenstand"@de,
        "Νοητικό Αντικείμενο"@el,
        "Conceptual Object"@en,
        "Objet conceptuel"@fr,
        "Objeto Conceitual"@pt,
        "Концептуальный Объект"@ru ;
    rdfs:comment """This class comprises non-material products of our minds and other human produced data that 		have become objects of a discourse about their identity, circumstances of creation or historical 		implication. The production of such information may have been supported by the use of    		technical devices such as cameras or computers.
Characteristically, instances of this class are created, invented or thought by someone, and then may be documented or communicated between persons. Instances of E28 Conceptual Object have the ability to exist on more than one particular carrier at the same time, such as paper, electronic signals, marks, audio media, paintings, photos, human memories, etc.
They cannot be destroyed. They exist as long as they can be found on at least one carrier or in at least one human memory. Their existence ends when the last carrier and the last memory are lost. """@en ;
    rdfs:subClassOf crm:E71_Man-Made_Thing .

crm:E29_Design_or_Procedure a rdfs:Class ;
    rdfs:label "Entwurf oder Verfahren"@de,
        "Σχέδιο"@el,
        "Design or Procedure"@en,
        "Conception ou procédure"@fr,
        "Projeto ou Procedimento"@pt,
        "Проект или Процедура"@ru ;
    rdfs:comment """This class comprises documented plans for the execution of actions in order to achieve a result of a specific quality, form or contents. In particular it comprises plans for deliberate human activities that may result in the modification or production of instances of E24 Physical Thing. 
Instances of E29 Design or Procedure can be structured in parts and sequences or depend on others. This is modelled using P69 is associated with. 
Designs or procedures can be seen as one of the following:
1.	A schema for the activities it describes
2.	A schema of the products that result from their application. 
3.	An independent intellectual product that may have never been applied, such as Leonardo da Vinci’s famous plans for flying machines.
Because designs or procedures may never be applied or only partially executed, the CRM models a loose relationship between the plan and the respective product."""@en ;
    rdfs:subClassOf crm:E73_Information_Object .

crm:E2_Temporal_Entity a rdfs:Class ;
    rdfs:label "Geschehendes"@de,
        "Έγχρονη  Οντότητα"@el,
        "Temporal Entity"@en,
        "Entité temporelle"@fr,
        "Entidade Temporal"@pt,
        "Временная Сущность"@ru ;
    rdfs:comment """This class comprises all phenomena, such as the instances of E4 Periods, E5 Events and states, which happen over a limited extent in time. 
	In some contexts, these are also called perdurants. This class is disjoint from E77 Persistent Item. This is an abstract class and has no direct instances. E2 Temporal Entity is specialized into E4 Period, which applies to a particular geographic area (defined with a greater or lesser degree of precision), and E3 Condition State, which applies to instances of E18 Physical Thing."""@en ;
    rdfs:subClassOf crm:E1_CRM_Entity .

crm:E30_Right a rdfs:Class ;
    rdfs:label "Recht"@de,
        "Δικαίωμα"@el,
        "Right"@en,
        "Droit"@fr,
        "Direitos"@pt,
        "Право"@ru ;
    rdfs:comment """This class comprises legal privileges concerning material and immaterial things or their derivatives. 
These include reproduction and property rights"""@en ;
    rdfs:subClassOf crm:E89_Propositional_Object .

crm:E31_Document a rdfs:Class ;
    rdfs:label "Dokument"@de,
        "Τεκμήριο"@el,
        "Document"@en,
        "Document"@fr,
        "Documento"@pt,
        "Документ"@ru ;
    rdfs:comment """This class comprises identifiable immaterial items that make propositions about reality.
These propositions may be expressed in text, graphics, images, audiograms, videograms or by other similar means. Documentation databases are regarded as a special case of E31 Document. This class should not be confused with the term “document” in Information Technology, which is compatible with E73 Information Object."""@en ;
    rdfs:subClassOf crm:E73_Information_Object .

crm:E32_Authority_Document a rdfs:Class ;
    rdfs:label "Referenzdokument"@de,
        "Πηγή Καθιερωμένων Όρων"@el,
        "Authority Document"@en,
        "Document de référence"@fr,
        "Documento de Referência"@pt,
        "Официальный Документ"@ru ;
    rdfs:comment "This class comprises encyclopaedia, thesauri, authority lists and other documents that define terminology or conceptual systems for consistent use."@en ;
    rdfs:subClassOf crm:E31_Document .

crm:E33_Linguistic_Object a rdfs:Class ;
    rdfs:label "Sprachlicher Gegenstand"@de,
        "Γλωσσικό Αντικείμενο"@el,
        "Linguistic Object"@en,
        "Objet linguistique"@fr,
        "Objeto Lingüístico"@pt,
        "Линвистический Объект"@ru ;
    rdfs:comment """This class comprises identifiable expressions in natural language or languages. 
Instances of E33 Linguistic Object can be expressed in many ways: e.g. as written texts, recorded speech or sign language. However, the CRM treats instances of E33 Linguistic Object independently from the medium or method by which they are expressed. Expressions in formal languages, such as computer code or mathematical formulae, are not treated as instances of E33 Linguistic Object by the CRM. These should be modelled as instances of E73 Information Object.
The text of an instance of E33 Linguistic Object can be documented in a note by P3 has note: E62 String"""@en ;
    rdfs:subClassOf crm:E73_Information_Object .

crm:E34_Inscription a rdfs:Class ;
    rdfs:label "Inschrift"@de,
        "Επιγραφή"@el,
        "Inscription"@en,
        "Inscription"@fr,
        "Inscrição"@pt,
        "Надпись"@ru ;
    rdfs:comment """This class comprises recognisable, short texts attached to instances of E24 Physical Man-Made Thing. 
The transcription of the text can be documented in a note by P3 has note: E62 String. The alphabet used can be documented by P2 has type: E55 Type. This class does not intend to describe the idiosyncratic characteristics of an individual physical embodiment of an inscription, but the underlying prototype. The physical embodiment is modelled in the CRM as E24 Physical Man-Made Thing.
The relationship of a physical copy of a book to the text it contains is modelled using E84 Information Carrier. P128 carries (is carried by): E33 Linguistic Object. """@en ;
    rdfs:subClassOf crm:E33_Linguistic_Object,
        crm:E37_Mark .

crm:E35_Title a rdfs:Class ;
    rdfs:label "Titel"@de,
        " Τίτλος"@el,
        "Title"@en,
        "Titre"@fr,
        "Título"@pt,
        "Заголовок"@ru ;
    rdfs:comment """This class comprises the names assigned to works, such as texts, artworks or pieces of music. 
Titles are proper noun phrases or verbal phrases, and should not be confused with generic object names such as “chair”, “painting” or “book” (the latter are common nouns that stand for instances of E55 Type). Titles may be assigned by the creator of the work itself, or by a social group. 
This class also comprises the translations of titles that are used as surrogates for the original titles in different social contexts."""@en ;
    rdfs:subClassOf crm:E33_Linguistic_Object,
        crm:E41_Appellation .

crm:E36_Visual_Item a rdfs:Class ;
    rdfs:label "Bildliches"@de,
        "Οπτικό Στοιχείο"@el,
        "Visual Item"@en,
        "Item visuel"@fr,
        "Item Visual"@pt,
        "Визуальный Предмет"@ru ;
    rdfs:comment """This class comprises the intellectual or conceptual aspects of recognisable marks and images.
This class does not intend to describe the idiosyncratic characteristics of an individual physical embodiment of a visual item, but the underlying prototype. For example, a mark such as the ICOM logo is generally considered to be the same logo when used on any number of publications. The size, orientation and colour may change, but the logo remains uniquely identifiable. The same is true of images that are reproduced many times. This means that visual items are independent of their physical support. 
The class E36 Visual Item provides a means of identifying and linking together instances of E24 Physical Man-Made Thing that carry the same visual symbols, marks or images etc. The property P62 depicts (is depicted by) between E24 Physical Man-Made Thing and depicted subjects (E1 CRM Entity) can be regarded as a short-cut of the more fully developed path from E24 Physical Man-Made Thing through P65 shows visual item (is shown by), E36 Visual Item, P138 represents (has representation) to E1CRM Entity, which in addition captures the optical features of the depiction.  """@en ;
    rdfs:subClassOf crm:E73_Information_Object .

crm:E37_Mark a rdfs:Class ;
    rdfs:label "Marke"@de,
        "Σήμανση"@el,
        "Mark"@en,
        "Marque"@fr,
        "Marca"@pt,
        "Пометка"@ru ;
    rdfs:comment """This class comprises symbols, signs, signatures or short texts applied to instances of E24 Physical Man-Made Thing by arbitrary techniques in order to indicate the creator, owner, dedications, purpose, etc. 
This class specifically excludes features that have no semantic significance, such as scratches or tool marks. These should be documented as instances of E25 Man-Made Feature. """@en ;
    rdfs:subClassOf crm:E36_Visual_Item .

crm:E38_Image a rdfs:Class ;
    rdfs:label "Bild"@de,
        "Εικόνα"@el,
        "Image"@en,
        "Image"@fr,
        "Imagem"@pt,
        "Изображение"@ru ;
    rdfs:comment """This class comprises distributions of form, tone and colour that may be found on surfaces such as photos, paintings, prints and sculptures or directly on electronic media. 
The degree to which variations in the distribution of form and colour affect the identity of an instance of E38 Image depends on a given purpose. The original painting of the Mona Lisa in the Louvre may be said to bear the same instance of E38 Image as reproductions in the form of transparencies, postcards, posters or T-shirts, even though they may differ in size and carrier and may vary in tone and colour. The images in a “spot the difference” competition are not the same with respect to their context, however similar they may at first appear."""@en ;
    rdfs:subClassOf crm:E36_Visual_Item .

crm:E39_Actor a rdfs:Class ;
    rdfs:label "Akteur"@de,
        "Δράστης"@el,
        "Actor"@en,
        "Agent"@fr,
        "Agente"@pt,
        "Агент"@ru ;
    rdfs:comment """This class comprises people, either individually or in groups, who have the potential to perform intentional actions for which they can be held responsible. 
The CRM does not attempt to model the inadvertent actions of such actors. Individual people should be documented as instances of E21 Person, whereas groups should be documented as instances of either E74 Group or its subclass E40 Legal Body."""@en ;
    rdfs:subClassOf crm:E77_Persistent_Item .

crm:E3_Condition_State a rdfs:Class ;
    rdfs:label "Zustandsphase"@de,
        "Κατάσταση"@el,
        "Condition State"@en,
        "État matériel"@fr,
        "Estado Material"@pt,
        "Состояние"@ru ;
    rdfs:comment """This class comprises the states of objects characterised by a certain condition over a time-span. 
An instance of this class describes the prevailing physical condition of any material object or feature during a specific E52 Time Span. In general, the time-span for which a certain condition can be asserted may be shorter than the real time-span, for which this condition held.
 The nature of that condition can be described using P2 has type. For example, the E3 Condition State “condition of the SS Great Britain between 22 September 1846 and 27 August 1847” can be characterized as E55 Type “wrecked”. """@en ;
    rdfs:subClassOf crm:E2_Temporal_Entity .

crm:E40_Legal_Body a rdfs:Class ;
    rdfs:label "Juristische Person"@de,
        "Νομικό Πρόσωπο"@el,
        "Legal Body"@en,
        "Collectivité"@fr,
        "Pessoa Jurídica"@pt,
        "Юридическое Лицо"@ru ;
    rdfs:comment """This class comprises institutions or groups of people that have obtained a legal recognition as a group and can act collectively as agents.  
This means that they can perform actions, own property, create or destroy things and can be held collectively responsible for their actions like individual people. The term 'personne morale' is often used for this in French. """@en ;
    rdfs:subClassOf crm:E74_Group .

crm:E41_Appellation a rdfs:Class ;
    rdfs:label "Benennung"@de,
        "Ονομασία"@el,
        "Appellation"@en,
        "Appellation"@fr,
        "Designação"@pt,
        "Обозначение"@ru ;
    rdfs:comment """This class comprises all sequences of signs of any nature, either meaningful or not, that are used or can be used to refer to and identify a specific instance of some class within a certain context.
Instances of E41 Appellation do not identify things by their meaning, even if they happen to have one, but by convention, tradition, or agreement. Instances of E41 Appellation are cultural constructs; as such, they have a context, a history, and a use in time and space by some group of users. A given instance of E41 Appellation can have alternative forms, i.e., other instances of E41 Appellation that are always regarded as equivalent independent from the thing it denotes. 
Specific subclasses of E41 Appellation should be used when instances of E41 Appellation of a characteristic form are used for particular objects. Instances of E49 Time Appellation, for example, which take the form of instances of E50 Date, can be easily recognised.
E41 Appellation should not be confused with the act of naming something. Cf. E15 Identifier Assignment"""@en ;
    rdfs:subClassOf crm:E90_Symbolic_Object .

crm:E42_Identifier a rdfs:Class ;
    rdfs:label "Kennung"@de,
        "Κωδικός Αναγνώρισης"@el,
        "Identifier"@en,
        "Identificateur d'objet"@fr,
        "Identificador de Objeto"@pt,
        "Идентификатор Объекта"@ru ;
    rdfs:comment "This class comprises strings or codes assigned to instances of E1 CRM Entity in order to identify them uniquely and permanently within the context of one or more organisations. Such codes are often known as inventory numbers, registration codes, etc. and are typically composed of alphanumeric sequences. The class E42 Identifier is not normally used for machine-generated identifiers used for automated processing unless these are also used by human agents."@en ;
    rdfs:subClassOf crm:E41_Appellation .

crm:E44_Place_Appellation a rdfs:Class ;
    rdfs:label "Ortsbenennung"@de,
        "Ονομασία Τόπου"@el,
        "Place Appellation"@en,
        "Appellation de lieu"@fr,
        "Designação de Local"@pt,
        "Обозначение Места"@ru ;
    rdfs:comment """This class comprises any sort of identifier characteristically used to refer to an E53 Place. 
Instances of E44 Place Appellation may vary in their degree of precision and their meaning may vary over time - the same instance of E44 Place Appellation may be used to refer to several places, either because of cultural shifts, or because objects used as reference points have moved around. Instances of E44 Place Appellation can be extremely varied in form: postal addresses, instances of E47 Spatial Coordinate, and parts of buildings can all be considered as instances of E44 Place Appellation."""@en ;
    rdfs:subClassOf crm:E41_Appellation .

crm:E45_Address a rdfs:Class ;
    rdfs:label "Adresse"@de,
        "Διεύθυνση"@el,
        "Address"@en,
        "Adresse"@fr,
        "Endereço"@pt,
        "Адрес"@ru ;
    rdfs:comment """This class comprises identifiers expressed in coding systems for places, such as postal addresses used for mailing.
An E45 Address can be considered both as the name of an E53 Place and as an E51 Contact Point for an E39 Actor. This dual aspect is reflected in the multiple inheritance. However, some forms of mailing addresses, such as a postal box, are only instances of E51 Contact Point, since they do not identify any particular Place. These should not be documented as instances of E45 Address."""@en ;
    rdfs:subClassOf crm:E44_Place_Appellation,
        crm:E51_Contact_Point .

crm:E46_Section_Definition a rdfs:Class ;
    rdfs:label "Abschnittsdefinition"@de,
        "Ονομασία Τμήματος"@el,
        "Section Definition"@en,
        "Désignation de section"@fr,
        "Designação de Seção"@pt,
        "Определение Района"@ru ;
    rdfs:comment """This class comprises areas of objects referred to in terms specific to the general geometry or structure of its kind. 
The 'prow' of the boat, the 'frame' of the picture, the 'front' of the building are all instances of E46 Section Definition. The class highlights the fact that parts of objects can be treated as locations. This holds in particular for features without natural boundaries, such as the “head” of a marble statue made out of one block (cf. E53 Place). In answer to the question 'where is the signature?' one might reply 'on the lower left corner'. (Section Definition is closely related to the term “segment” in Gerstl, P.& Pribbenow, S, 1996 “ A conceptual theory of part – whole relations and its applications”, Data & Knowledge 	Engineering 20 305-322, North Holland- Elsevier )."""@en ;
    rdfs:subClassOf crm:E44_Place_Appellation .

crm:E47_Spatial_Coordinates a rdfs:Class ;
    rdfs:label "Raumkoordinaten"@de,
        "Χωρικές Συντεταγμένες"@el,
        "Spatial Coordinates"@en,
        "Coordonnées spatiales"@fr,
        "Coordenadas Espaciais"@pt,
        "Пространственные Координаты"@ru ;
    rdfs:comment """This class comprises the textual or numeric information required to locate specific instances of E53 Place within schemes of spatial identification. 

Coordinates are a specific form of E44 Place Appellation, that is, a means of referring to a particular E53 Place. Coordinates are not restricted to longitude, latitude and altitude. Any regular system of reference that maps onto an E19 Physical Object can be used to generate coordinates."""@en ;
    rdfs:subClassOf crm:E44_Place_Appellation .

crm:E48_Place_Name a rdfs:Class ;
    rdfs:label "Orts- oder Flurname"@de,
        "Τοπωνύμιο"@el,
        "Place Name"@en,
        "Toponyme"@fr,
        "Nome de Local"@pt,
        "Название Места"@ru ;
    rdfs:comment """This class comprises particular and common forms of E44 Place Appellation. 
Place Names may change their application over time: the name of an E53 Place may change, and a name may be reused for a different E53 Place. Instances of E48 Place Name are typically subject to place name gazetteers."""@en ;
    rdfs:subClassOf crm:E44_Place_Appellation .

crm:E49_Time_Appellation a rdfs:Class ;
    rdfs:label "Zeitbenennung"@de,
        "Ονομασία Χρόνου"@el,
        "Time Appellation"@en,
        "Appellation temporelle"@fr,
        "Designação de Tempo"@pt,
        "Обозначение Времени"@ru ;
    rdfs:comment """This class comprises all forms of names or codes, such as historical periods, and dates, which are characteristically used to refer to a specific E52 Time-Span. 
The instances of E49 Time Appellation may vary in their degree of precision, and they may be relative to other time frames, “Before Christ” for example. Instances of E52 Time-Span are often defined by reference to a cultural period or an event e.g. ‘the duration of the Ming Dynasty’."""@en ;
    rdfs:subClassOf crm:E41_Appellation .

crm:E4_Period a rdfs:Class ;
    rdfs:label "Phase"@de,
        "Περίοδος"@el,
        "Period"@en,
        "Période"@fr,
        "Período"@pt,
        "Период"@ru ;
    rdfs:comment """	This class comprises sets of coherent phenomena or cultural manifestations bounded in time and space. 
It is the social or physical coherence of these phenomena that identify an E4 Period and not the associated spatio-temporal bounds. These bounds are a mere approximation of the actual process of growth, spread and retreat. Consequently, different periods can overlap and coexist in time and space, such as when a nomadic culture exists in the same area as a sedentary culture. 
Typically this class is used to describe prehistoric or historic periods such as the “Neolithic Period”, the “Ming Dynasty” or the “McCarthy Era”. There are however no assumptions about the scale of the associated phenomena. In particular all events are seen as synthetic processes consisting of coherent phenomena. Therefore E4 Period is a superclass of E5 Event. For example, a modern clinical E67 Birth can be seen as both an atomic E5 Event and as an E4 Period that consists of multiple activities performed by multiple instances of E39 Actor. 
There are two different conceptualisations of ‘artistic style’, defined either by physical features or by historical context. For example, “Impressionism” can be viewed as a period lasting from approximately 1870 to 1905 during which paintings with particular characteristics were produced by a group of artists that included (among others) Monet, Renoir, Pissarro, Sisley and Degas. Alternatively, it can be regarded as a style applicable to all paintings sharing the characteristics of the works produced by the Impressionist painters, regardless of historical context. The first interpretation is an E4 Period, and the second defines morphological object types that fall under E55 Type.
Another specific case of an E4 Period is the set of activities and phenomena associated with a settlement, such as the populated period of Nineveh."""@en ;
    rdfs:subClassOf crm:E2_Temporal_Entity .

crm:E50_Date a rdfs:Class ;
    rdfs:label "Datum"@de,
        "Ημερομηνία"@el,
        "Date"@en,
        "Date"@fr,
        "Data"@pt,
        "Дата"@ru ;
    rdfs:comment "This class comprises specific forms of E49 Time Appellation."@en ;
    rdfs:subClassOf crm:E49_Time_Appellation .

crm:E51_Contact_Point a rdfs:Class ;
    rdfs:label "Kontaktpunkt"@de,
        "Στοιχείο Επικοινωνίας"@el,
        "Contact Point"@en,
        "Coordonnées individuelles"@fr,
        "Ponto de Contato"@pt,
        "Контакт"@ru ;
    rdfs:comment """This class comprises identifiers employed, or understood, by communication services to direct communications to an instance of E39 Actor. These include E-mail addresses, telephone numbers, post office boxes, Fax numbers, URLs etc. Most postal addresses can be considered both as instances of E44 Place Appellation and E51 Contact Point. In such cases the subclass E45 Address should be used. 
URLs are addresses used by machines to access another machine through an http request. Since the accessed machine acts on behalf of the E39 Actor providing the machine, URLs are considered as instances of E51 Contact Point to that E39 Actor."""@en ;
    rdfs:subClassOf crm:E41_Appellation .

crm:E52_Time-Span a rdfs:Class ;
    rdfs:label "Zeitspanne"@de,
        "Χρονικό Διάστημα"@el,
        "Time-Span"@en,
        "Durée"@fr,
        "Período de Tempo"@pt,
        "Интервал Времени"@ru ;
    rdfs:comment """This class comprises abstract temporal extents, in the sense of Galilean physics, having a beginning, an end and a duration. 
Time Span has no other semantic connotations. Time-Spans are used to define the temporal extent of instances of E4 Period, E5 Event and any other phenomena valid for a certain time. An E52 Time-Span may be identified by one or more instances of E49 Time Appellation. 
Since our knowledge of history is imperfect, instances of E52 Time-Span can best be considered as approximations of the actual Time-Spans of temporal entities. The properties of E52 Time-Span are intended to allow these approximations to be expressed precisely.  An extreme case of approximation, might, for example, define an E52 Time-Span having unknown beginning, end and duration. Used as a common E52 Time-Span for two events, it would nevertheless define them as being simultaneous, even if nothing else was known. 
	Automatic processing and querying of instances of E52 Time-Span is facilitated if data can be parsed into an E61 Time Primitive."""@en ;
    rdfs:subClassOf crm:E1_CRM_Entity .

crm:E53_Place a rdfs:Class ;
    rdfs:label "Ort"@de,
        "Τόπος"@el,
        "Place"@en,
        "Lieu"@fr,
        "Local"@pt,
        "Место"@ru ;
    rdfs:comment """This class comprises extents in space, in particular on the surface of the earth, in the pure sense of physics: independent from temporal phenomena and matter. 
The instances of E53 Place are usually determined by reference to the position of “immobile” objects such as buildings, cities, mountains, rivers, or dedicated geodetic marks. A Place can be determined by combining a frame of reference and a location with respect to this frame. It may be identified by one or more instances of E44 Place Appellation.
 It is sometimes argued that instances of E53 Place are best identified by global coordinates or absolute reference systems. However, relative references are often more relevant in the context of cultural documentation and tend to be more precise. In particular, we are often interested in position in relation to large, mobile objects, such as ships. For example, the Place at which Nelson died is known with reference to a large mobile object – H.M.S Victory. A resolution of this Place in terms of absolute coordinates would require knowledge of the movements of the vessel and the precise time of death, either of which may be revised, and the result would lack historical and cultural relevance.
Any object can serve as a frame of reference for E53 Place determination. The model foresees the notion of a "section" of an E19 Physical Object as a valid E53 Place determination."""@en ;
    rdfs:subClassOf crm:E1_CRM_Entity .

crm:E54_Dimension a rdfs:Class ;
    rdfs:label "Maß"@de,
        "Μέγεθος"@el,
        "Dimension"@en,
        "Dimensions"@fr,
        "Dimensão"@pt,
        "Величина"@ru ;
    rdfs:comment """This class comprises quantifiable properties that can be measured by some calibrated means and can be approximated by values, i.e. points or regions in a mathematical or conceptual space, such as natural or real numbers, RGB values etc.
An instance of E54 Dimension represents the true quantity, independent from its numerical approximation, e.g. in inches or in cm. The properties of the class E54 Dimension allow for expressing the numerical approximation of the values of an instance of E54 Dimension. If the true values belong to a non-discrete space, such as spatial distances, it is recommended to record them as approximations by intervals or regions of indeterminacy enclosing the assumed true values. For instance, a length of 5 cm may be recorded as 4.5-5.5 cm, according to the precision of the respective observation. Note, that interoperability of values described in different units depends critically on the representation as value regions.
Numerical approximations in archaic instances of E58 Measurement Unit used in historical records should be preserved. Equivalents corresponding to current knowledge should be recorded as additional instances of E54 Dimension as appropriate."""@en ;
    rdfs:subClassOf crm:E1_CRM_Entity .

crm:E55_Type a rdfs:Class ;
    rdfs:label "Typus"@de,
        "Τύπος"@el,
        "Type"@en,
        "Type"@fr,
        "Tipo"@pt,
        "Тип"@ru ;
    rdfs:comment """This class comprises concepts denoted by terms from thesauri and controlled vocabularies used to characterize and classify instances of CRM classes. Instances of E55 Type represent concepts  in contrast to instances of E41 Appellation which are used to name instances of CRM classes. 
E55 Type is the CRM’s interface to domain specific ontologies and thesauri. These can be represented in the CRM as subclasses of E55 Type, forming hierarchies of terms, i.e. instances of E55 Type linked via P127 has broader  term (has narrower term). Such hierarchies may be extended with additional properties. """@en ;
    rdfs:subClassOf crm:E28_Conceptual_Object .

crm:E56_Language a rdfs:Class ;
    rdfs:label "Sprache"@de,
        "Γλώσσα"@el,
        "Language"@en,
        "Langue"@fr,
        "Língua"@pt,
        "Язык"@ru ;
    rdfs:comment """This class is a specialization of E55 Type and comprises the natural languages in the sense of concepts. 
This type is used categorically in the model without reference to instances of it, i.e. the Model does not foresee the description of instances of instances of E56 Language, e.g.: “instances of  Mandarin Chinese”.
It is recommended that internationally or nationally agreed codes and terminology are used to denote instances of E56 Language, such as those defined in ISO 639:1988. """@en ;
    rdfs:subClassOf crm:E55_Type .

crm:E57_Material a rdfs:Class ;
    rdfs:label "Material"@de,
        "Υλικό"@el,
        "Material"@en,
        "Matériau"@fr,
        "Material"@pt,
        "Материал"@ru ;
    rdfs:comment """This class is a specialization of E55 Type and comprises the concepts of materials. 
Instances of E57 Material may denote properties of matter before its use, during its use, and as incorporated in an object, such as ultramarine powder, tempera paste, reinforced concrete. Discrete pieces of raw-materials kept in museums, such as bricks, sheets of fabric, pieces of metal, should be modelled individually in the same way as other objects. Discrete used or processed pieces, such as the stones from Nefer Titi's temple, should be modelled as parts (cf. P46 is composed of).
This type is used categorically in the model without reference to instances of it, i.e. the Model does not foresee the description of instances of instances of E57 Material, e.g.: “instances of  gold”.
It is recommended that internationally or nationally agreed codes and terminology are used."""@en ;
    rdfs:subClassOf crm:E55_Type .

crm:E58_Measurement_Unit a rdfs:Class ;
    rdfs:label "Maßeinheit"@de,
        "Μονάδα Μέτρησης"@el,
        "Measurement Unit"@en,
        "Unité de mesure"@fr,
        "Unidade de Medida"@pt,
        "Единица Измерения"@ru ;
    rdfs:comment """This class is a specialization of E55 Type and comprises the types of measurement units: feet, inches, centimetres, litres, lumens, etc. 
This type is used categorically in the model without reference to instances of it, i.e. the Model does not foresee the description of instances of instances of E58 Measurement Unit, e.g.: “instances of cm”.
Syst?me International (SI) units or internationally recognized non-SI terms should be used whenever possible. (ISO 1000:1992). Archaic Measurement Units used in historical records should be preserved."""@en ;
    rdfs:subClassOf crm:E55_Type .

crm:E5_Event a rdfs:Class ;
    rdfs:label "Ereignis"@de,
        "Συμβάν"@el,
        "Event"@en,
        "Événement"@fr,
        "Evento"@pt,
        "Событие"@ru ;
    rdfs:comment """This class comprises changes of states in cultural, social or physical systems, regardless of scale, brought about by a series or group of coherent physical, cultural, technological or legal phenomena. Such changes of state will affect instances of E77 Persistent Item or its subclasses.
The distinction between an E5 Event and an E4 Period is partly a question of the scale of observation. Viewed at a coarse level of detail, an E5 Event is an ‘instantaneous’ change of state. At a fine level, the E5 Event can be analysed into its component phenomena within a space and time frame, and as such can be seen as an E4 Period. The reverse is not necessarily the case: not all instances of E4 Period give rise to a noteworthy change of state."""@en ;
    rdfs:subClassOf crm:E4_Period .

crm:E63_Beginning_of_Existence a rdfs:Class ;
    rdfs:label "Daseinsbeginn"@de,
        "Αρχή Ύπαρξης"@el,
        "Beginning of Existence"@en,
        "Début d'existence"@fr,
        "Início da Existência"@pt,
        "Начало Существования"@ru ;
    rdfs:comment """This class comprises events that bring into existence any E77 Persistent Item. 
It may be used for temporal reasoning about things (intellectual products, physical items, groups of people, living beings) beginning to exist; it serves as a hook for determination of a terminus post quem and ante quem. """@en ;
    rdfs:subClassOf crm:E5_Event .

crm:E64_End_of_Existence a rdfs:Class ;
    rdfs:label "Daseinsende"@de,
        "Τέλος Ύπαρξης"@el,
        "End of Existence"@en,
        "Fin d'existence"@fr,
        "Fim da Existência"@pt,
        "Конец Существования"@ru ;
    rdfs:comment """This class comprises events that end the existence of any E77 Persistent Item. 
It may be used for temporal reasoning about things (physical items, groups of people, living beings) ceasing to exist; it serves as a hook for determination of a terminus postquem and antequem. In cases where substance from a Persistent Item continues to exist in a new form, the process would be documented by E81 Transformation."""@en ;
    rdfs:subClassOf crm:E5_Event .

crm:E65_Creation a rdfs:Class ;
    rdfs:label "Begriffliche Schöpfung"@de,
        "Δημιουργία"@el,
        "Creation"@en,
        "Création"@fr,
        "Criação"@pt,
        "Событие Творения"@ru ;
    rdfs:comment "This class comprises events that result in the creation of conceptual items or immaterial products, such as legends, poems, texts, music, images, movies, laws, types etc."@en ;
    rdfs:subClassOf crm:E63_Beginning_of_Existence,
        crm:E7_Activity .

crm:E66_Formation a rdfs:Class ;
    rdfs:label "Gruppenbildung"@de,
        "Συγκρότηση Ομάδας"@el,
        "Formation"@en,
        "Formation"@fr,
        "Formação"@pt,
        "Событие Формирования"@ru ;
    rdfs:comment """This class comprises events that result in the formation of a formal or informal E74 Group of people, such as a club, society, association, corporation or nation. 
E66 Formation does not include the arbitrary aggregation of people who do not act as a collective.
The formation of an instance of E74 Group does not mean that the group is populated with members at the time of formation. In order to express the joining of members at the time of formation, the respective activity should be simultaneously an instance of both E66 Formation and E85 Joining. """@en ;
    rdfs:subClassOf crm:E63_Beginning_of_Existence,
        crm:E7_Activity .

crm:E67_Birth a rdfs:Class ;
    rdfs:label "Geburt"@de,
        "Γέννηση"@el,
        "Birth"@en,
        "Naissance"@fr,
        "Nascimento"@pt,
        "Рождение"@ru ;
    rdfs:comment """This class comprises the births of human beings. E67 Birth is a biological event focussing on the context of people coming into life. (E63 Beginning of Existence comprises the coming into life of any living beings). 
Twins, triplets etc. are brought into life by the same E67 Birth event. The introduction of the E67 Birth event as a documentation element allows the description of a range of family relationships in a simple model. Suitable extensions may describe more details and the complexity of motherhood with the intervention of modern medicine. In this model, the biological father is not seen as a necessary participant in the E67 Birth event."""@en ;
    rdfs:subClassOf crm:E63_Beginning_of_Existence .

crm:E68_Dissolution a rdfs:Class ;
    rdfs:label "Gruppenauflösung"@de,
        "Διάλυση Ομάδας"@el,
        "Dissolution"@en,
        "Dissolution"@fr,
        "Dissolução"@pt,
        "Роспуск"@ru ;
    rdfs:comment """This class comprises the events that result in the formal or informal termination of an E74 Group of people. 
If the dissolution was deliberate, the Dissolution event should also be instantiated as an E7 Activity."""@en ;
    rdfs:subClassOf crm:E64_End_of_Existence .

crm:E69_Death a rdfs:Class ;
    rdfs:label "Tod"@de,
        "Θάνατος"@el,
        "Death"@en,
        "Mort"@fr,
        "Morte"@pt,
        "Смерть"@ru ;
    rdfs:comment """This class comprises the deaths of human beings. 
If a person is killed, their death should be instantiated as E69 Death and as E7 Activity. The death or perishing of other living beings should be documented using E64 End of Existence."""@en ;
    rdfs:subClassOf crm:E64_End_of_Existence .

crm:E6_Destruction a rdfs:Class ;
    rdfs:label "Zerstörung"@de,
        "Καταστροφή"@el,
        "Destruction"@en,
        "Destruction"@fr,
        "Destruição"@pt,
        "Разрушение"@ru ;
    rdfs:comment """This class comprises events that destroy one or more instances of E18 Physical Thing such that they lose their identity as the subjects of documentation.  
Some destruction events are intentional, while others are independent of human activity. Intentional destruction may be documented by classifying the event as both an E6 Destruction and E7 Activity. 
The decision to document an object as destroyed, transformed or modified is context sensitive: 
1.  If the matter remaining from the destruction is not documented, the event is modelled solely as E6 Destruction. 
2. An event should also be documented using E81 Transformation if it results in the destruction of one or more objects and the simultaneous production of others using parts or material from the original. In this case, the new items have separate identities. Matter is preserved, but identity is not.
3. When the initial identity of the changed instance of E18 Physical Thing is preserved, the event should be documented as E11 Modification. """@en ;
    rdfs:subClassOf crm:E64_End_of_Existence .

crm:E70_Thing a rdfs:Class ;
    rdfs:label "Sache"@de,
        "Πράγμα"@el,
        "Thing"@en,
        "Chose"@fr,
        "Coisa"@pt,
        ""@ru ;
    rdfs:comment """This general class comprises usable discrete, identifiable, instances of E77 Persistent Item that are documented as single units. 

They can be either intellectual products or physical things, and are characterized by relative stability. They may for instance either have a solid physical form, an electronic encoding, or they may be logical concept or structure. """@en ;
    rdfs:subClassOf crm:E77_Persistent_Item .

crm:E71_Man-Made_Thing a rdfs:Class ;
    rdfs:label "Künstliches"@de,
        "Ανθρώπινο Δημιούργημα"@el,
        "Man-Made Thing"@en,
        "Chose fabriquée"@fr,
        "Coisa Fabricada"@pt,
        "Рукотворная Вещь"@ru ;
    rdfs:comment """This class comprises discrete, identifiable man-made items that are documented as single units. 
These items are either intellectual products or man-made physical things, and are characterized by relative stability. They may for instance have a solid physical form, an electronic encoding, or they may be logical concepts or structures."""@en ;
    rdfs:subClassOf crm:E70_Thing .

crm:E72_Legal_Object a rdfs:Class ;
    rdfs:label "Rechtsobjekt"@de,
        "Νομικό Αντικείμενο"@el,
        "Legal Object"@en,
        "Objet juridique"@fr,
        "Objeto Jurídico"@pt,
        "Объект Права"@ru ;
    rdfs:comment """This class comprises those material or immaterial items to which instances of E30 Right, such as the right of ownership or use, can be applied. 
This is true for all E18 Physical Thing. In the case of instances of E28 Conceptual Object, however, the identity of the E28 Conceptual Object or the method of its use may be too ambiguous to reliably establish instances of E30 Right, as in the case of taxa and inspirations. Ownership of corporations is currently regarded as out of scope of the CRM. """@en ;
    rdfs:subClassOf crm:E70_Thing .

crm:E73_Information_Object a rdfs:Class ;
    rdfs:label "Informationsgegenstand"@de,
        "Πληροφοριακό Αντικείμενο"@el,
        "Information Object"@en,
        "Objet d'information"@fr,
        "Objeto de Informação"@pt,
        "Информационный Объект"@ru ;
    rdfs:comment """This class comprises identifiable immaterial items, such as a poems, jokes, data sets, images, texts, multimedia objects, procedural prescriptions, computer program code, algorithm or mathematical formulae, that have an objectively recognizable structure and are documented as single units. 
An E73 Information Object does not depend on a specific physical carrier, which can include human memory, and it can exist on one or more carriers simultaneously.
Instances of E73 Information Object of a linguistic nature should be declared as instances of the E33 Linguistic Object subclass. Instances of E73 Information Object of a documentary nature should be declared as instances of the E31 Document subclass. Conceptual items such as types and classes are not instances of E73 Information Object, nor are ideas without a reproducible expression. """@en ;
    rdfs:subClassOf crm:E89_Propositional_Object,
        crm:E90_Symbolic_Object .

crm:E74_Group a rdfs:Class ;
    rdfs:label "Menschliche Gruppe"@de,
        "Ομάδα"@el,
        "Group"@en,
        "Groupe"@fr,
        "Grupo"@pt,
        "Группа"@ru ;
    rdfs:comment """This class comprises any gatherings or organizations of two or more people that act collectively or in a similar way due to any form of unifying relationship. In the wider sense this class also comprises official positions which used to be regarded in certain contexts as one actor, independent of the current holder of the office, such as the president of a country. 
A gathering of people becomes an E74 Group when it exhibits organizational characteristics usually typified by a set of ideas or beliefs held in common, or actions performed together. These might be communication, creating some common artifact, a common purpose such as study, worship, business, sports, etc. Nationality can be modeled as membership in an E74 Group (cf. HumanML markup). Married couples and other concepts of family are regarded as particular examples of E74 Group."""@en ;
    rdfs:subClassOf crm:E39_Actor .

crm:E75_Conceptual_Object_Appellation a rdfs:Class ;
    rdfs:label "Begriff- oder Konzeptbenennung "@de,
        "Ονομασία Νοητικού Αντικειμένου"@el,
        "Conceptual Object Appellation"@en,
        "Appellation d'objet conceptuel"@fr,
        "Designação de Objeto Conceitual"@pt,
        "Обозначение Концептуального Объекта"@ru ;
    rdfs:comment "This class comprises all appellations specific to intellectual products or standardized patterns."@en ;
    rdfs:subClassOf crm:E41_Appellation .

crm:E77_Persistent_Item a rdfs:Class ;
    rdfs:label "Seiendes"@de,
        "Ον"@el,
        "Persistent Item"@en,
        "Entité persistante"@fr,
        "Entidade Persistente"@pt,
        "Постоянная Сущность"@ru ;
    rdfs:comment """This class comprises items that have a persistent identity, sometimes known as “endurants” in philosophy. 
They can be repeatedly recognized within the duration of their existence by identity criteria rather than by continuity or observation. Persistent Items can be either physical entities, such as people, animals or things, or conceptual entities such as ideas, concepts, products of the imagination or common names.
The criteria that determine the identity of an item are often difficult to establish -; the decision depends largely on the judgement of the observer. For example, a building is regarded as no longer existing if it is dismantled and the materials reused in a different configuration. On the other hand, human beings go through radical and profound changes during their life-span, affecting both material composition and form, yet preserve their identity by other criteria. Similarly, inanimate objects may be subject to exchange of parts and matter. The class E77 Persistent Item does not take any position about the nature of the applicable identity criteria and if actual knowledge about identity of an instance of this class exists. There may be cases, where the identity of an E77 Persistent Item is not decidable by a certain state of knowledge.
The main classes of objects that fall outside the scope the E77 Persistent Item class are temporal objects such as periods, events and acts, and descriptive properties. """@en ;
    rdfs:subClassOf crm:E1_CRM_Entity .

crm:E78_Collection a rdfs:Class ;
    rdfs:label "Sammlung"@de,
        "Συλλογή"@el,
        "Collection"@en,
        "Collection"@fr,
        "Coleção"@pt,
        "Коллекция"@ru ;
    rdfs:comment """This class comprises aggregations of instances of E18 Physical Thing that are assembled and maintained (“curated” and “preserved,” in museological terminology) by one or more instances of E39 Actor over time for a specific purpose and audience, and according to a particular collection development plan.  
Items may be added or removed from an E78 Collection in pursuit of this plan. This class should not be confused with the E39 Actor maintaining the E78 Collection often referred to with the name of the E78 Collection (e.g. “The Wallace Collection decided…”).
Collective objects in the general sense, like a tomb full of gifts, a folder with stamps or a set of chessmen, should be documented as instances of E19 Physical Object, and not as instances of E78 Collection. This is because they form wholes either because they are physically bound together or because they are kept together for their functionality."""@en ;
    rdfs:subClassOf crm:E24_Physical_Man-Made_Thing .

crm:E79_Part_Addition a rdfs:Class ;
    rdfs:label "Teilhinzufügung"@de,
        "Προσθήκη Μερών"@el,
        "Part Addition"@en,
        "Addition d'élément"@fr,
        "Adição de Parte"@pt,
        "Добавление Части"@ru ;
    rdfs:comment """This class comprises activities that result in an instance of E24 Physical Man-Made Thing being increased, enlarged or augmented by the addition of a part. 
Typical scenarios include the attachment of an accessory, the integration of a component, the addition of an element to an aggregate object, or the accessioning of an object into a curated E78 Collection. Objects to which parts are added are, by definition, man-made, since the addition of a part implies a human activity. Following the addition of parts, the resulting man-made assemblages are treated objectively as single identifiable wholes, made up of constituent or component parts bound together either physically (for example the engine becoming a part of the car), or by sharing a common purpose (such as the 32 chess pieces that make up a chess set). This class of activities forms a basis for reasoning about the history and continuity of identity of objects that are integrated into other objects over time, such as precious gemstones being repeatedly incorporated into different items of jewellery, or cultural artifacts being added to different museum instances of E78 Collection over their lifespan."""@en ;
    rdfs:subClassOf crm:E11_Modification .

crm:E7_Activity a rdfs:Class ;
    rdfs:label "Handlung"@de,
        "Δράση"@el,
        "Activity"@en,
        "Activité"@fr,
        "Atividade"@pt,
        "Деятельность"@ru ;
    rdfs:comment """This class comprises actions intentionally carried out by instances of E39 Actor that result in changes of state in the cultural, social, or physical systems documented. 
This notion includes complex, composite and long-lasting actions such as the building of a settlement or a war, as well as simple, short-lived actions such as the opening of a door."""@en ;
    rdfs:subClassOf crm:E5_Event .

crm:E80_Part_Removal a rdfs:Class ;
    rdfs:label "Teilentfernung"@de,
        "Αφαίρεση Μερών"@el,
        "Part Removal"@en,
        "Soustraction d'élément"@fr,
        "Remoção de Parte"@pt,
        "Удаление Части"@ru ;
    rdfs:comment """This class comprises the activities that result in an instance of E18 Physical Thing being decreased by the removal of a part.
Typical scenarios include the detachment of an accessory, the removal of a component or part of a composite object, or the deaccessioning of an object from a curated E78 Collection. If the E80 Part Removal results in the total decomposition of the original object into pieces, such that the whole ceases to exist, the activity should instead be modelled as an E81 Transformation, i.e. a simultaneous destruction and production. In cases where the part removed has no discernible identity prior to its removal but does have an identity subsequent to its removal, the activity should be regarded as both E80 Part Removal and E12 Production. This class of activities forms a basis for reasoning about the history, and continuity of identity over time, of objects that are removed from other objects, such as precious gemstones being extracted from different items of jewelry, or cultural artifacts being deaccessioned from different museum collections over their lifespan."""@en ;
    rdfs:subClassOf crm:E11_Modification .

crm:E81_Transformation a rdfs:Class ;
    rdfs:label "Umwandlung"@de,
        "Μετατροπή"@el,
        "Transformation"@en,
        "Transformation"@fr,
        "Transformação"@pt,
        "Трансформация"@ru ;
    rdfs:comment """This class comprises the events that result in the simultaneous destruction of one or more than one E77 Persistent Item and the creation of one or more than one E77 Persistent Item that preserves recognizable substance from the first one(s) but has fundamentally different nature and identity. 
Although the old and the new instances of E77 Persistent Item are treated as discrete entities having separate, unique identities, they are causally connected through the E81 Transformation; the destruction of the old E77 Persistent Item(s) directly causes the creation of the new one(s) using or preserving some relevant substance. Instances of E81 Transformation are therefore distinct from re-classifications (documented using E17 Type Assignment) or modifications (documented using E11 Modification) of objects that do not fundamentally change their nature or identity. Characteristic cases are reconstructions and repurposing of historical buildings or ruins, fires leaving buildings in ruins, taxidermy of specimen in natural history and the reorganization of a corporate body into a new one."""@en ;
    rdfs:subClassOf crm:E63_Beginning_of_Existence,
        crm:E64_End_of_Existence .

crm:E82_Actor_Appellation a rdfs:Class ;
    rdfs:label "Akteurbenennung"@de,
        "Ονομασία Δράστη"@el,
        "Actor Appellation"@en,
        "Appellation d'agent"@fr,
        "Designação de Agente"@pt,
        "Обозначение Агента"@ru ;
    rdfs:comment """This class comprises any sort of name, number, code or symbol characteristically used to identify an E39 Actor. 
An E39 Actor will typically have more than one E82 Actor Appellation, and instances of E82 Actor Appellation in turn may have alternative representations. The distinction between corporate and personal names, which is particularly important in library applications, should be made by explicitly linking the E82 Actor Appellation to an instance of either E21 Person or E74 Group/E40 Legal Body. If this is not possible, the distinction can be made through the use of the P2 has type mechanism. """@en ;
    rdfs:subClassOf crm:E41_Appellation .

crm:E83_Type_Creation a rdfs:Class ;
    rdfs:label "Typuserfindung"@de,
        "Δημιουργία Τύπου"@el,
        "Type Creation"@en,
        "Création de type"@fr,
        "Criação de Tipo"@pt,
        "Создание Типа"@ru ;
    rdfs:comment """This class comprises activities formally defining new types of items. 
It is typically a rigorous scholarly or scientific process that ensures a type is exhaustively described and appropriately named. In some cases, particularly in archaeology and the life sciences, E83 Type Creation requires the identification of an exemplary specimen and the publication of the type definition in an appropriate scholarly forum. The activity of E83 Type Creation is central to research in the life sciences, where a type would be referred to as a “taxon,” the type description as a “protologue,” and the exemplary specimens as “orgininal element” or “holotype”."""@en ;
    rdfs:subClassOf crm:E65_Creation .

crm:E84_Information_Carrier a rdfs:Class ;
    rdfs:label "Informationsträger"@de,
        "Φορέας Πληροφορίας"@el,
        "Information Carrier"@en,
        "Support d'information"@fr,
        "Suporte de Informação"@pt,
        "Носитель Информации"@ru ;
    rdfs:comment """This class comprises all instances of E22 Man-Made Object that are explicitly designed to act as persistent physical carriers for instances of E73 Information Object. 
This allows a relationship to be asserted between an E19 Physical Object and its immaterial information contents. An E84 Information Carrier may or may not contain information, e.g., a diskette. Note that any E18 Physical Thing may carry information, such as an E34 Inscription. However, unless it was specifically designed for this purpose, it is not an Information Carrier. Therefore the property P128 carries (is carried by) applies to E18 Physical Thing in general."""@en ;
    rdfs:subClassOf crm:E22_Man-Made_Object .

crm:E85_Joining a rdfs:Class ;
    rdfs:label "Beitritt"@de,
        "Joining"@en ;
    rdfs:comment """This class comprises the activities that result in an instance of E39 Actor becoming a member of an instance of E74 Group. This class does not imply initiative by either party.
Typical scenarios include becoming a member of a social organisation, becoming employee of a company, marriage, the adoption of a child by a family and the inauguration of somebody into an official position. """@en ;
    rdfs:subClassOf crm:E7_Activity .

crm:E86_Leaving a rdfs:Class ;
    rdfs:label "Austritt"@de,
        "Leaving"@en ;
    rdfs:comment """This class comprises the activities that result in an instance of E39 Actor to be disassociated from an instance of E74 Group. This class does not imply initiative by either party. 
Typical scenarios include the termination of membership in a social organisation, ending the employment at a company, divorce, and the end of tenure of somebody in an official position."""@en ;
    rdfs:subClassOf crm:E7_Activity .

crm:E87_Curation_Activity a rdfs:Class ;
    rdfs:label "Kuratorische Tätigkeit"@de,
        "Curation Activity"@en ;
    rdfs:comment """This class comprises the activities that result in the continuity of management and the preservation and evolution of instances of E78 Collection, following an implicit or explicit curation plan. 
It specializes the notion of activity into the curation of a collection and allows the history of curation to be recorded.
Items are accumulated and organized following criteria like subject, chronological period, material type, style of art etc. and can be added or removed from an E78 Collection for a specific purpose and/or audience. The initial aggregation of items of a collection is regarded as an instance of E12 Production Event while the activity of evolving, preserving and promoting a collection is regarded as an instance of E87 Curation Activity."""@en ;
    rdfs:subClassOf crm:E7_Activity .

crm:E89_Propositional_Object a rdfs:Class ;
    rdfs:label "Aussagenobjekt"@de,
        "Propositional Object"@en ;
    rdfs:comment """This class comprises immaterial items, including but not limited to stories, plots, procedural prescriptions, algorithms, laws of physics or images that are, or represent in some sense, sets of propositions about real or imaginary things and that are documented as single units or serve as topics of discourse. 
	
This class also comprises items that are “about” something in the sense of a subject. In the wider sense, this class includes expressions of psychological value such as non-figural art and musical themes. However, conceptual items such as types and classes are not instances of E89 Propositional Object. This should not be confused with the definition of a type, which is indeed an instance of E89 Propositional Object."""@en ;
    rdfs:subClassOf crm:E28_Conceptual_Object .

crm:E8_Acquisition a rdfs:Class ;
    rdfs:label "Erwerb"@de,
        "Απόκτηση"@el,
        "Acquisition"@en,
        "Acquisition"@fr,
        "Aquisição"@pt,
        "Событие Приобретения"@ru ;
    rdfs:comment """This class comprises transfers of legal ownership from one or more instances of E39 Actor to one or more other instances of E39 Actor. 
The class also applies to the establishment or loss of ownership of instances of E18 Physical Thing. It does not, however, imply changes of any other kinds of right. The recording of the donor and/or recipient is optional. It is possible that in an instance of E8 Acquisition there is either no donor or no recipient. Depending on the circumstances, it may describe:
1.	the beginning of ownership
2.	the end of ownership
3.	the transfer of ownership
4.	the acquisition from an unknown source 
5.	the loss of title due to destruction of the item
It may also describe events where a collector appropriates legal title, for example by annexation or field collection. The interpretation of the museum notion of "accession" differs between institutions. The CRM therefore models legal ownership (E8 Acquisition) and physical custody (E10 Transfer of Custody) separately. Institutions will then model their specific notions of accession and deaccession as combinations of these."""@en ;
    rdfs:subClassOf crm:E7_Activity .

crm:E90_Symbolic_Object a rdfs:Class ;
    rdfs:label "Symbolisches Objekt"@de,
        "Symbolic Object"@en ;
    rdfs:comment """This class comprises identifiable symbols and any aggregation of symbols, such as characters, identifiers, traffic signs, emblems, texts, data sets, images, musical scores, multimedia objects, computer program code or mathematical formulae that have an objectively recognizable structure and that are documented as single units.
It includes sets of signs of any nature, which may serve to designate something, or to communicate some propositional content. 
An instance of E90 Symbolic Object does not depend on a specific physical carrier, which can include human memory, and it can exist on one or more carriers simultaneously. An instance of E90 Symbolic Object may or may not have a specific meaning, for example an arbitrary character string."""@en ;
    rdfs:subClassOf crm:E28_Conceptual_Object,
        crm:E72_Legal_Object .

crm:E9_Move a rdfs:Class ;
    rdfs:label "Objektbewegung"@de,
        "Μετακίνηση"@el,
        "Move"@en,
        "Déplacement"@fr,
        "Locomoção"@pt,
        "Перемещение"@ru ;
    rdfs:comment """This class comprises changes of the physical location of the instances of E19 Physical Object. 
Note, that the class E9 Move inherits the property P7 took place at (witnessed): E53 Place. This property should be used to describe the trajectory or a larger area within which a move takes place, whereas the properties P26 moved to (was destination of), P27 moved from (was origin of) describe the start and end points only. Moves may also be documented to consist of other moves (via P9 consists of (forms part of)), in order to describe intermediate stages on a trajectory. In that case, start and end points of the partial moves should match appropriately between each other and with the overall event."""@en ;
    rdfs:subClassOf crm:E7_Activity .

rdf:Alt a rdfs:Class ;
    rdfs:label "Alt" ;
    rdfs:comment "The class of containers of alternatives." ;
    rdfs:isDefinedBy rdf: ;
    rdfs:subClassOf rdfs:Container .

rdf:Bag a rdfs:Class ;
    rdfs:label "Bag" ;
    rdfs:comment "The class of unordered containers." ;
    rdfs:isDefinedBy rdf: ;
    rdfs:subClassOf rdfs:Container .

rdf:List a rdfs:Class ;
    rdfs:label "List" ;
    rdfs:comment "The class of RDF Lists." ;
    rdfs:isDefinedBy rdf: ;
    rdfs:subClassOf rdfs:Resource .

rdf:Property a rdfs:Class ;
    rdfs:label "Property" ;
    rdfs:comment "The class of RDF properties." ;
    rdfs:isDefinedBy rdf: ;
    rdfs:subClassOf rdfs:Resource .

rdf:Seq a rdfs:Class ;
    rdfs:label "Seq" ;
    rdfs:comment "The class of ordered containers." ;
    rdfs:isDefinedBy rdf: ;
    rdfs:subClassOf rdfs:Container .

rdf:Statement a rdfs:Class ;
    rdfs:label "Statement" ;
    rdfs:comment "The class of RDF statements." ;
    rdfs:isDefinedBy rdf: ;
    rdfs:subClassOf rdfs:Resource .

rdfs:Class a rdfs:Class,
        owl:Class ;
    rdfs:label "Class" ;
    rdfs:comment "The class of classes." ;
    rdfs:isDefinedBy rdfs: ;
    rdfs:subClassOf rdfs:Resource .

rdfs:Container a rdfs:Class ;
    rdfs:label "Container" ;
    rdfs:comment "The class of RDF containers." ;
    rdfs:isDefinedBy rdfs: ;
    rdfs:subClassOf rdfs:Resource .

rdfs:ContainerMembershipProperty a rdfs:Class ;
    rdfs:label "ContainerMembershipProperty" ;
    rdfs:comment """The class of container membership properties, rdf:_1, rdf:_2, ...,
                    all of which are sub-properties of 'member'.""" ;
    rdfs:isDefinedBy rdfs: ;
    rdfs:subClassOf rdf:Property .

rdfs:Datatype a rdfs:Class ;
    rdfs:label "Datatype" ;
    rdfs:comment "The class of RDF datatypes." ;
    rdfs:isDefinedBy rdfs: ;
    rdfs:subClassOf rdfs:Class .

rdfs:Literal a rdfs:Class ;
    rdfs:label "Literal" ;
    rdfs:comment "The class of literal values, eg. textual strings and integers." ;
    rdfs:isDefinedBy rdfs: ;
    rdfs:subClassOf rdfs:Resource .

rdfs:Resource a rdfs:Class ;
    rdfs:label "Resource" ;
    rdfs:comment "The class resource, everything." ;
    rdfs:isDefinedBy rdfs: .

owl:AllDifferent a rdfs:Class ;
    rdfs:label "AllDifferent" ;
    rdfs:comment "The class of collections of pairwise different individuals." ;
    rdfs:isDefinedBy owl: ;
    rdfs:subClassOf rdfs:Resource .

owl:AllDisjointClasses a rdfs:Class ;
    rdfs:label "AllDisjointClasses" ;
    rdfs:comment "The class of collections of pairwise disjoint classes." ;
    rdfs:isDefinedBy owl: ;
    rdfs:subClassOf rdfs:Resource .

owl:AllDisjointProperties a rdfs:Class ;
    rdfs:label "AllDisjointProperties" ;
    rdfs:comment "The class of collections of pairwise disjoint properties." ;
    rdfs:isDefinedBy owl: ;
    rdfs:subClassOf rdfs:Resource .

owl:Annotation a rdfs:Class ;
    rdfs:label "Annotation" ;
    rdfs:comment "The class of annotated annotations for which the RDF serialization consists of an annotated subject, predicate and object." ;
    rdfs:isDefinedBy owl: ;
    rdfs:subClassOf rdfs:Resource .

owl:AnnotationProperty a rdfs:Class ;
    rdfs:label "AnnotationProperty" ;
    rdfs:comment "The class of annotation properties." ;
    rdfs:isDefinedBy owl: ;
    rdfs:subClassOf rdf:Property .

owl:AsymmetricProperty a rdfs:Class ;
    rdfs:label "AsymmetricProperty" ;
    rdfs:comment "The class of asymmetric properties." ;
    rdfs:isDefinedBy owl: ;
    rdfs:subClassOf owl:ObjectProperty .

owl:Axiom a rdfs:Class ;
    rdfs:label "Axiom" ;
    rdfs:comment "The class of annotated axioms for which the RDF serialization consists of an annotated subject, predicate and object." ;
    rdfs:isDefinedBy owl: ;
    rdfs:subClassOf rdfs:Resource .

owl:Class a rdfs:Class ;
    rdfs:label "Class" ;
    rdfs:comment "The class of OWL classes." ;
    rdfs:isDefinedBy owl: ;
    rdfs:subClassOf rdfs:Class .

owl:DataRange a rdfs:Class ;
    rdfs:label "DataRange" ;
    rdfs:comment "The class of OWL data ranges, which are special kinds of datatypes. Note: The use of the IRI owl:DataRange has been deprecated as of OWL 2. The IRI rdfs:Datatype SHOULD be used instead." ;
    rdfs:isDefinedBy owl: ;
    rdfs:subClassOf rdfs:Datatype .

owl:DatatypeProperty a rdfs:Class ;
    rdfs:label "DatatypeProperty" ;
    rdfs:comment "The class of data properties." ;
    rdfs:isDefinedBy owl: ;
    rdfs:subClassOf rdf:Property .

owl:DeprecatedClass a rdfs:Class ;
    rdfs:label "DeprecatedClass" ;
    rdfs:comment "The class of deprecated classes." ;
    rdfs:isDefinedBy owl: ;
    rdfs:subClassOf rdfs:Class .

owl:DeprecatedProperty a rdfs:Class ;
    rdfs:label "DeprecatedProperty" ;
    rdfs:comment "The class of deprecated properties." ;
    rdfs:isDefinedBy owl: ;
    rdfs:subClassOf rdf:Property .

owl:FunctionalProperty a rdfs:Class ;
    rdfs:label "FunctionalProperty" ;
    rdfs:comment "The class of functional properties." ;
    rdfs:isDefinedBy owl: ;
    rdfs:subClassOf rdf:Property .

owl:InverseFunctionalProperty a rdfs:Class ;
    rdfs:label "InverseFunctionalProperty" ;
    rdfs:comment "The class of inverse-functional properties." ;
    rdfs:isDefinedBy owl: ;
    rdfs:subClassOf owl:ObjectProperty .

owl:IrreflexiveProperty a rdfs:Class ;
    rdfs:label "IrreflexiveProperty" ;
    rdfs:comment "The class of irreflexive properties." ;
    rdfs:isDefinedBy owl: ;
    rdfs:subClassOf owl:ObjectProperty .

owl:NamedIndividual a rdfs:Class ;
    rdfs:label "NamedIndividual" ;
    rdfs:comment "The class of named individuals." ;
    rdfs:isDefinedBy owl: ;
    rdfs:subClassOf owl:Thing .

owl:NegativePropertyAssertion a rdfs:Class ;
    rdfs:label "NegativePropertyAssertion" ;
    rdfs:comment "The class of negative property assertions." ;
    rdfs:isDefinedBy owl: ;
    rdfs:subClassOf rdfs:Resource .

owl:ObjectProperty a rdfs:Class ;
    rdfs:label "ObjectProperty" ;
    rdfs:comment "The class of object properties." ;
    rdfs:isDefinedBy owl: ;
    rdfs:subClassOf rdf:Property .

owl:Ontology a rdfs:Class ;
    rdfs:label "Ontology" ;
    rdfs:comment "The class of ontologies." ;
    rdfs:isDefinedBy owl: ;
    rdfs:subClassOf rdfs:Resource .

owl:OntologyProperty a rdfs:Class ;
    rdfs:label "OntologyProperty" ;
    rdfs:comment "The class of ontology properties." ;
    rdfs:isDefinedBy owl: ;
    rdfs:subClassOf rdf:Property .

owl:ReflexiveProperty a rdfs:Class ;
    rdfs:label "ReflexiveProperty" ;
    rdfs:comment "The class of reflexive properties." ;
    rdfs:isDefinedBy owl: ;
    rdfs:subClassOf owl:ObjectProperty .

owl:Restriction a rdfs:Class ;
    rdfs:label "Restriction" ;
    rdfs:comment "The class of property restrictions." ;
    rdfs:isDefinedBy owl: ;
    rdfs:subClassOf owl:Class .

owl:SymmetricProperty a rdfs:Class ;
    rdfs:label "SymmetricProperty" ;
    rdfs:comment "The class of symmetric properties." ;
    rdfs:isDefinedBy owl: ;
    rdfs:subClassOf owl:ObjectProperty .

owl:TransitiveProperty a rdfs:Class ;
    rdfs:label "TransitiveProperty" ;
    rdfs:comment "The class of transitive properties." ;
    rdfs:isDefinedBy owl: ;
    rdfs:subClassOf owl:ObjectProperty .

wgs84:Point a rdfs:Class ;
    rdfs:label "point" ;
    rdfs:comment """ 
Uniquely identified by lat/long/alt. i.e.

spaciallyIntersects(P1, P2) :- lat(P1, LAT), long(P1, LONG), alt(P1, ALT),
  lat(P2, LAT), long(P2, LONG), alt(P2, ALT).

sameThing(P1, P2) :- type(P1, Point), type(P2, Point), spaciallyIntersects(P1, P2).
  """,
        """A point, typically described using a coordinate system relative to Earth, such as WGS84.
  """ ;
    rdfs:subClassOf wgs84:SpatialThing .

wgs84:SpatialThing a rdfs:Class,
        owl:Class ;
    rdfs:label "Spatial Thing",
        "SpatialThing" ;
    rdfs:comment """Anything with spatial extent, i.e. size, shape, or position.
 e.g. people, places, bowling balls, as well as abstract areas like cubes.""" .

locn:Address a rdfs:Class ;
    rdfs:label "Address"@en ;
    dcterms:identifier "locn:Address" ;
    rdfs:comment "An \"address representation\" as conceptually defined by the INSPIRE Address Representation data type. The locn:addressId property may be used to link this locn:Address to other representations."@en ;
    rdfs:isDefinedBy <http://www.w3.org/ns/locn> ;
    swvocab:term_status "testing"@en ;
    powder-s:describedby <https://joinup.ec.europa.eu/node/55858> .

locn:Geometry a rdfs:Class ;
    rdfs:label "Geometry"@en ;
    dcterms:identifier "locn:Geometry" ;
    vann:usageNote "This class defines the notion of \"geometry\" at the conceptual level, and it shall be encoded by using different formats (see usage note of the locn:geometry property)."@en ;
    rdfs:comment "The locn:Geometry class provides the means to identify a location as a point, line, polygon, etc. expressed using coordinates in some coordinate reference system."@en ;
    rdfs:isDefinedBy <http://www.w3.org/ns/locn> ;
    swvocab:term_status "unstable"@en .

foaf:Agent a rdfs:Class,
        owl:Class ;
    rdfs:label "Agent" ;
    rdfs:comment "An agent (eg. person, group, software or physical artifact)." ;
    owl:equivalentClass dcterms:Agent ;
    swvocab:term_status "stable" .

foaf:Document a rdfs:Class,
        owl:Class ;
    rdfs:label "Document" ;
    rdfs:comment "A document." ;
    rdfs:isDefinedBy foaf: ;
    owl:disjointWith foaf:Organization,
        foaf:Project ;
    owl:equivalentClass org:CreativeWork ;
    swvocab:term_status "stable" .

foaf:Group a rdfs:Class,
        owl:Class ;
    rdfs:label "Group" ;
    rdfs:comment "A class of Agents." ;
    rdfs:subClassOf foaf:Agent ;
    swvocab:term_status "stable" .

foaf:Image a rdfs:Class,
        owl:Class ;
    rdfs:label "Image" ;
    rdfs:comment "An image." ;
    rdfs:isDefinedBy foaf: ;
    rdfs:subClassOf foaf:Document ;
    owl:equivalentClass org:ImageObject ;
    swvocab:term_status "stable" .

foaf:LabelProperty a rdfs:Class,
        owl:Class ;
    rdfs:label "Label Property" ;
    rdfs:comment "A foaf:LabelProperty is any RDF property with texual values that serve as labels." ;
    rdfs:isDefinedBy foaf: ;
    swvocab:term_status "unstable" .

foaf:OnlineAccount a rdfs:Class,
        owl:Class ;
    rdfs:label "Online Account" ;
    rdfs:comment "An online account." ;
    rdfs:isDefinedBy foaf: ;
    rdfs:subClassOf owl:Thing ;
    swvocab:term_status "testing" .

foaf:OnlineChatAccount a rdfs:Class,
        owl:Class ;
    rdfs:label "Online Chat Account" ;
    rdfs:comment "An online chat account." ;
    rdfs:isDefinedBy foaf: ;
    rdfs:subClassOf foaf:OnlineAccount ;
    swvocab:term_status "unstable" .

foaf:OnlineEcommerceAccount a rdfs:Class,
        owl:Class ;
    rdfs:label "Online E-commerce Account" ;
    rdfs:comment "An online e-commerce account." ;
    rdfs:isDefinedBy foaf: ;
    rdfs:subClassOf foaf:OnlineAccount ;
    swvocab:term_status "unstable" .

foaf:OnlineGamingAccount a rdfs:Class,
        owl:Class ;
    rdfs:label "Online Gaming Account" ;
    rdfs:comment "An online gaming account." ;
    rdfs:isDefinedBy foaf: ;
    rdfs:subClassOf foaf:OnlineAccount ;
    swvocab:term_status "unstable" .

foaf:Organization a rdfs:Class,
        owl:Class ;
    rdfs:label "Organization" ;
    rdfs:comment "An organization." ;
    rdfs:isDefinedBy foaf: ;
    rdfs:subClassOf foaf:Agent ;
    owl:disjointWith foaf:Document,
        foaf:Person ;
    swvocab:term_status "stable" .

foaf:Person a rdfs:Class,
        owl:Class ;
    rdfs:label "Person" ;
    rdfs:comment "A person." ;
    rdfs:isDefinedBy foaf: ;
    rdfs:subClassOf wgs84:SpatialThing,
        foaf:Agent ;
    owl:disjointWith foaf:Organization,
        foaf:Project ;
    owl:equivalentClass org:Person,
        <http://www.w3.org/2000/10/swap/pim/contact#Person> ;
    swvocab:term_status "stable" .

foaf:PersonalProfileDocument a rdfs:Class,
        owl:Class ;
    rdfs:label "PersonalProfileDocument" ;
    rdfs:comment "A personal profile RDF document." ;
    rdfs:subClassOf foaf:Document ;
    swvocab:term_status "testing" .

foaf:Project a rdfs:Class,
        owl:Class ;
    rdfs:label "Project" ;
    rdfs:comment "A project (a collective endeavour of some kind)." ;
    rdfs:isDefinedBy foaf: ;
    owl:disjointWith foaf:Document,
        foaf:Person ;
    swvocab:term_status "testing" .

crmeh:EHE0001_EHProject a owl:Class ;
    rdfs:label "EH Project"@en ;
    rdfs:comment "A project can be modelled as a Period, but as it results in a \"change of state in the cultural, social or physical systems documented,\" the specialisation Event can be used. As it is intentionally carried out by people, the specialization Activity should be used"@en ;
    rdfs:isDefinedBy crmeh:CRMEH ;
    rdfs:subClassOf crm:E7_Activity ;
    owl:sameAs crmeh:EHE0001 ;
    skos:notation "EHE0001" .

crmeh:EHE0002_ArchaeologicalSite a owl:Class ;
    rdfs:label "Archaeological Site"@en ;
    rdfs:comment "The notion of an archaeological site as a material feature on the earth irrespective of spatial bounds e.g. Stonehenge. Provides a means to relate projects carried out at a particular site, even where the interventions or survey work have not been at the same spatial location. For example, excavations at one end of the West Kennet Avenue can be seen to be related to excavations at the other, even though they are some distance apart and may not be within the defined extent of the avenue as recorded in the SMR"@en ;
    rdfs:isDefinedBy crmeh:CRMEH ;
    rdfs:subClassOf crm:E27_Site ;
    owl:sameAs crmeh:EHE0002 ;
    skos:notation "EHE0002" .

crmeh:EHE0003_AreaOfInvestigation a owl:Class ;
    rdfs:label "Area of Investigation"@en ;
    rdfs:comment "Effectively, the extent of the archaeological site as defined by the current project. The word Site is not used here to avoid confusion with the CRM concept of Site. In this case, we are meaning the area under investigation as opposed to an instance of E27 Site or a site as defined in the SMR or NMR or other data source. The CRM concept of Site denotes the material constellations and may be subject to change due to excavation activity and physical phenomena. It should not be confused with the mere geographic extent of the site that does not change.  This entity is not present in the recording system, but is necessary so we can reason about the place, the actual patch of land, being investigated"@en ;
    rdfs:isDefinedBy crmeh:CRMEH ;
    rdfs:subClassOf crm:E53_Place ;
    owl:sameAs crmeh:EHE0003 ;
    skos:notation "EHE0003" .

crmeh:EHE0004_SiteSubDivision a owl:Class ;
    rdfs:label "Site Sub-Division"@en ;
    rdfs:comment "These represent the extents of particular regions within the area of investigation"@en ;
    rdfs:isDefinedBy crmeh:CRMEH ;
    rdfs:subClassOf crm:E53_Place ;
    owl:sameAs crmeh:EHE0004 ;
    skos:notation "EHE0004" .

crmeh:EHE0005_Group a owl:Class ;
    rdfs:label "Group"@en ;
    rdfs:comment "The process of grouping draws together the various places that represent contexts into interpretive spatial entities. The extent of the group will contain the extents of individual contexts but may extend beyond them"@en ;
    rdfs:isDefinedBy crmeh:CRMEH ;
    rdfs:subClassOf crm:E53_Place ;
    owl:sameAs crmeh:EHE0005 ;
    skos:notation "EHE0005" .

crmeh:EHE0010_BulkFind a owl:Class ;
    rdfs:label "Bulk Find"@en ;
    rdfs:comment "A specialisation of Finds in general describing a collection of finds from an excavation that are grouped according to the type of material e.g. flint, pottery, glass etc. This should not be confused with categorical (\"meta\")descriptions, that fall under specializations of E55 Type"@en ;
    rdfs:isDefinedBy crmeh:CRMEH ;
    rdfs:subClassOf crmeh:EHE0009_ContextFind ;
    owl:sameAs crmeh:EHE0010 ;
    skos:notation "EHE0010" .

crmeh:EHE0011_GroupEventRecord a owl:Class ;
    rdfs:label "Group Event Record"@en ;
    rdfs:comment "The idea of documenting events allows us to make assertions regarding the quality of the documentation. For example, it allows us to talk about uncertainty regarding time-spans of events when in reality an event time-span is fixed and absolute although it may not be known"@en ;
    rdfs:isDefinedBy crmeh:CRMEH ;
    rdfs:subClassOf crm:E73_Information_Object ;
    owl:sameAs crmeh:EHE0011 ;
    skos:notation "EHE0011" .

crmeh:EHE0012_ContextEventRecord a owl:Class ;
    rdfs:label "Context Event Record"@en ;
    rdfs:comment "The idea of documenting events allows us to make assertions regarding the quality of the documentation. For example, it allows us to talk about uncertainty regarding time-spans of events when in reality an event time-span is fixed and absolute although it may not be known"@en ;
    rdfs:isDefinedBy crmeh:CRMEH ;
    rdfs:subClassOf crm:E73_Information_Object ;
    owl:sameAs crmeh:EHE0012 ;
    skos:notation "EHE0012" .

crmeh:EHE0013_ContextSheet a owl:Class ;
    rdfs:label "Context Sheet"@en ;
    rdfs:comment "As with other information objects, there is the need to carry them. It is this entity that provides a mechanism for managing the physical manifestation of contextual information i.e. the actual sheets on which it is written"@en ;
    rdfs:isDefinedBy crmeh:CRMEH ;
    rdfs:subClassOf crm:E84_Information_Carrier ;
    owl:sameAs crmeh:EHE0013 ;
    skos:notation "EHE0013" .

crmeh:EHE0014_ContextFindProductionEventRecord a owl:Class ;
    rdfs:label "Context Find Production Event Record"@en ;
    rdfs:comment "The idea of documenting events allows us to make assertions regarding the quality of the documentation. For example, it allows us to talk about uncertainty regarding time-spans of events when in reality an event time-span is fixed and absolute although it may not be known"@en ;
    rdfs:isDefinedBy crmeh:CRMEH ;
    rdfs:subClassOf crm:E31_Document ;
    owl:sameAs crmeh:EHE0014 ;
    skos:notation "EHE0014" .

crmeh:EHE0015_ContextFindUseEventRecord a owl:Class ;
    rdfs:label "Context Find Use Event Record"@en ;
    rdfs:comment "The idea of documenting events allows us to make assertions regarding the quality of the documentation. For example, it allows us to talk about uncertainty regarding time-spans of events when in reality an event time-span is fixed and absolute although it may not be known. "@en ;
    rdfs:isDefinedBy crmeh:CRMEH ;
    rdfs:subClassOf crm:E31_Document ;
    owl:sameAs crmeh:EHE0015 ;
    skos:notation "EHE0015" .

crmeh:EHE0016_RecordDrawing a owl:Class ;
    rdfs:label "Record Drawing"@en ;
    rdfs:comment "Plans and sections as drawn by the excavator which show archaeological features relative to each other and to a local co-ordinate system. Photographs provide a similar record but are generally not taken relative to any co-ordinate system: Potentially model photographs and drawings as subclasses of a generic information object, with only drawings having a relationship to a co-ordinate system?"@en ;
    rdfs:isDefinedBy crmeh:CRMEH ;
    rdfs:subClassOf crm:E36_Visual_Item ;
    owl:sameAs crmeh:EHE0016 ;
    skos:notation "EHE0016" .

crmeh:EHE0017_RecordPhotograph a owl:Class ;
    rdfs:label "Record Photograph"@en ;
    rdfs:comment "Record shots of context detail (relative position, colour, inclusions, finds in situ, etc). The photograph is here defined by its contents (be it ideal or a digital one). If the physical film material is to be traced, it should be documented as \"carrier\""@en ;
    rdfs:isDefinedBy crmeh:CRMEH ;
    rdfs:subClassOf crm:E38_Image ;
    owl:sameAs crmeh:EHE0017 ;
    skos:notation "EHE0017" .

crmeh:EHE0019_AreaOfInvestigationDepiction a owl:Class ;
    rdfs:label "Area of Investigation Depiction"@en ;
    rdfs:comment "The Spatial co-ordinates of the Area of Investigation, defining the actual spatial extent of the area under investigation"@en ;
    rdfs:isDefinedBy crmeh:CRMEH ;
    rdfs:subClassOf crm:E47_Spatial_Coordinates ;
    owl:sameAs crmeh:EHE0019 ;
    skos:notation "EHE0019" .

crmeh:EHE0020_BulkFindComponentCount a rdfs:Datatype,
        owl:Class ;
    rdfs:label "Bulk Find Component Count"@en ;
    rdfs:comment "The actual number of individual items that were collected in a bulk find from a context. E.g. The number of pieces of pottery in a bulk finds pot bag"@en ;
    rdfs:isDefinedBy crmeh:CRMEH ;
    rdfs:subClassOf xsd:nonNegativeInteger ;
    owl:sameAs crmeh:EHE0020 ;
    skos:notation "EHE0020" .

crmeh:EHE0021_EHProjectTimespan a owl:Class ;
    rdfs:label "EH Project Timespan"@en ;
    rdfs:comment "The time from when a project first begins to when the project is officially closed"@en ;
    rdfs:isDefinedBy crmeh:CRMEH ;
    rdfs:subClassOf crm:E52_Time-Span ;
    owl:sameAs crmeh:EHE0021 ;
    skos:notation "EHE0021" .

crmeh:EHE0022_ContextDepiction a owl:Class ;
    rdfs:label "Context Depiction"@en ;
    rdfs:comment "The Spatial co-ordinates of a Context, defining the actual spatial extent of the context. Usually recorded at the time of excavation or other investigative work"@en ;
    rdfs:isDefinedBy crmeh:CRMEH ;
    rdfs:subClassOf crm:E47_Spatial_Coordinates ;
    owl:sameAs crmeh:EHE0022 ;
    skos:notation "EHE0022" .

crmeh:EHE0023_ContextEventRecordNote a rdfs:Datatype,
        owl:Class ;
    rdfs:label "Context Event Record Note"@en ;
    rdfs:comment "Notes made about recording a Context, such as date recorded, weather conditions, and name of recorder, either contained in a log book or on a recording form. This might include the notes made on a context recording sheet, but it is not the same as the actual concept of a Context Record as defined by all the information held on a  Context recording form (either paper or digital) which is an information object in its own right"@en ;
    rdfs:isDefinedBy crmeh:CRMEH ;
    rdfs:subClassOf rdfs:Literal ;
    owl:sameAs crmeh:EHE0023 ;
    skos:notation "EHE0023" .

crmeh:EHE0024_ContextEventRecordNoteType a owl:Class ;
    rdfs:label "Context Event Record Note Type"@en ;
    rdfs:comment "A controlled list of the different types of notes made about recording a Context, such as date recorded, weather conditions, etc. The list of types might be equivalent to a list of the field names for a recording system"@en ;
    rdfs:isDefinedBy crmeh:CRMEH ;
    rdfs:subClassOf crm:E55_Type ;
    owl:sameAs crmeh:EHE0024 ;
    skos:notation "EHE0024" .

crmeh:EHE0025_ContextEventTimespan a owl:Class ;
    rdfs:label "Context Event Timespan"@en ;
    rdfs:comment "The length of time that a context took to form. Else the time span of any  transformation it undertook to reach its state when excavated. We can reason about when in time these formation/transformation events took place. We do not need to have absolute dates for this, we are simply building a relative sequence of events from the observed stratigraphy and other evidence"@en ;
    rdfs:isDefinedBy crmeh:CRMEH ;
    rdfs:subClassOf crm:E52_Time-Span ;
    owl:sameAs crmeh:EHE0025 ;
    skos:notation "EHE0025" .

crmeh:EHE0026_ContextEventTimespanAppellation a owl:Class ;
    rdfs:label "Context Event Timespan Appellation"@en ;
    rdfs:comment "The name given to a particular time-span for a context formation. E.g. ditch silting up event, pit back-filling, time of abandonment of building prior to demolition"@en ;
    rdfs:isDefinedBy crmeh:CRMEH ;
    rdfs:subClassOf crm:E49_Time_Appellation ;
    owl:sameAs crmeh:EHE0026 ;
    skos:notation "EHE0026" .

crmeh:EHE0027_ContextFindConditionAssessmentEventTimespan a owl:Class ;
    rdfs:label "Context Find Condition Assessment Event Timespan"@en ;
    rdfs:comment "How long the condition assessment of a find will take. Recorded as part of the conservation process"@en ;
    rdfs:isDefinedBy crmeh:CRMEH ;
    rdfs:subClassOf crm:E52_Time-Span ;
    owl:sameAs crmeh:EHE0027 ;
    skos:notation "EHE0027" .

crmeh:EHE0028_ContextFindConditionAssessmentEventType a owl:Class ;
    rdfs:label "Context Find Condition Assessment Event Type"@en ;
    rdfs:comment "Condition assessment types might include: Visual inspection, Cleaning, "@en ;
    rdfs:isDefinedBy crmeh:CRMEH ;
    rdfs:subClassOf crm:E55_Type ;
    owl:sameAs crmeh:EHE0028 ;
    skos:notation "EHE0028" .

crmeh:EHE0029_ContextFindConditionState a owl:Class ;
    rdfs:label "Context Find Condition State"@en ;
    rdfs:comment "Condition of an object as identified at the time of excavation e.g. Waterlogged, burnt, damaged"@en ;
    rdfs:isDefinedBy crmeh:CRMEH ;
    rdfs:subClassOf crm:E3_Condition_State ;
    owl:sameAs crmeh:EHE0029 ;
    skos:notation "EHE0029" .

crmeh:EHE0030_ContextFindMaterial a owl:Class ;
    rdfs:label "Context Find Material"@en ;
    rdfs:comment "For EH a glossary controlled list is used for finds recording eg Animal bone, Ceramic building material, fired clay, flint, glass, human bone etc. and a thesaurus has been developed by Environmental sciences that hierarchically classifies these further"@en ;
    rdfs:isDefinedBy crmeh:CRMEH ;
    rdfs:subClassOf crm:E57_Material ;
    owl:sameAs crmeh:EHE0030 ;
    skos:notation "EHE0030" .

crmeh:EHE0031_ContextFindMeasurement a owl:Class ;
    rdfs:label "Context Find Measurement"@en ;
    rdfs:comment "Many different measurements are recorded about artefacts and ecofacts, both during excavation and in later analysis. Examples include, length, width, diameter, weight, etc"@en ;
    rdfs:isDefinedBy crmeh:CRMEH ;
    rdfs:subClassOf crm:E54_Dimension ;
    owl:sameAs crmeh:EHE0031 ;
    skos:notation "EHE0031" .

crmeh:EHE0032_ContextFindMeasurementEventTimespan a owl:Class ;
    rdfs:label "Context Find Measurement Event Timespan"@en ;
    rdfs:comment "The time taken for measuring is most likely to be recorded for more complex finds measurements such as processing an item sent for detailed analysis e.g. SEM or X-Ray of objects"@en ;
    rdfs:isDefinedBy crmeh:CRMEH ;
    rdfs:subClassOf crm:E52_Time-Span ;
    owl:sameAs crmeh:EHE0032 ;
    skos:notation "EHE0032" .

crmeh:EHE0033_ContextFindMeasurementEventType a owl:Class ;
    rdfs:label "Context Find Measurement Event Type"@en ;
    rdfs:comment "Different types of measurement events could include: Initial investigation, Lab analysis, conservation recording"@en ;
    rdfs:isDefinedBy crmeh:CRMEH ;
    rdfs:subClassOf crm:E55_Type ;
    owl:sameAs crmeh:EHE0033 ;
    skos:notation "EHE0033" .

crmeh:EHE0034_ContextFindMeasurementUnit a owl:Class ;
    rdfs:label "Context Find Measurement Unit"@en ;
    rdfs:comment "The unit of measurement used to record information about a finds object e.g. metres, seconds, kilogrammes, etc"@en ;
    rdfs:isDefinedBy crmeh:CRMEH ;
    rdfs:subClassOf crm:E58_Measurement_Unit ;
    owl:sameAs crmeh:EHE0034 ;
    skos:notation "EHE0034" .

crmeh:EHE0035_ContextFindMeasurementValue a rdfs:Datatype,
        owl:Class ;
    rdfs:label "Context Find Measurement Value"@en ;
    rdfs:comment "The actual value recorded for a measurement"@en ;
    rdfs:isDefinedBy crmeh:CRMEH ;
    rdfs:subClassOf xsd:float ;
    owl:sameAs crmeh:EHE0035 ;
    skos:notation "EHE0035" .

crmeh:EHE0036_ContextFindProductionEventRecordNote a rdfs:Datatype,
        owl:Class ;
    rdfs:label "Context Find Production Event Record Note"@en ;
    rdfs:comment "Notes regarding record compilation and dating process. Notes made during the archaeological process about the original production, manufacture or creation of a find object"@en ;
    rdfs:isDefinedBy crmeh:CRMEH ;
    rdfs:subClassOf rdfs:Literal ;
    owl:sameAs crmeh:EHE0036 ;
    skos:notation "EHE0036" .

crmeh:EHE0037_ContextFindProductionEventRecordNoteType a owl:Class ;
    rdfs:label "Context Find Production Event Record Note Type"@en ;
    rdfs:comment "Type used to structure notes eg certainty"@en ;
    rdfs:isDefinedBy crmeh:CRMEH ;
    rdfs:subClassOf crm:E55_Type ;
    owl:sameAs crmeh:EHE0037 ;
    skos:notation "EHE0037" .

crmeh:EHE0038_ContextFindProductionEventTimespan a owl:Class ;
    rdfs:label "Context Find Production Event Timespan"@en ;
    rdfs:comment "We can reason about when in time these production events took place"@en ;
    rdfs:isDefinedBy crmeh:CRMEH ;
    rdfs:subClassOf crm:E52_Time-Span ;
    owl:sameAs crmeh:EHE0038 ;
    skos:notation "EHE0038" .

crmeh:EHE0039_ContextFindProductionEventTimespanAppellation a owl:Class ;
    rdfs:label "Context Find Production Event Timespan Appellation"@en ;
    rdfs:comment "It is this entity that provides the labelling of basic spot-dating evidence for contexts (i.e. the date of context finds). We may know very little about the actual production event in the past, but the concept of such a production event enables us to discuss modes of production, place of manufacture, etc. "@en ;
    rdfs:isDefinedBy crmeh:CRMEH ;
    rdfs:subClassOf crm:E49_Time_Appellation ;
    owl:sameAs crmeh:EHE0039 ;
    skos:notation "EHE0039" .

crmeh:EHE0040_ContextFindTreatmentLocation a owl:Class ;
    rdfs:label "Context Find Treatment Location"@en ;
    rdfs:comment "The place where finds treatment takes place may be recorded so others can locate the finds, particularly if treatment needs to take a considerable amount of time (e.g. the Mary Rose) "@en ;
    rdfs:isDefinedBy crmeh:CRMEH ;
    rdfs:subClassOf crm:E53_Place ;
    owl:sameAs crmeh:EHE0040 ;
    skos:notation "EHE0040" .

crmeh:EHE0041_ContextFindTreatmentProcedure a owl:Class ;
    rdfs:label "Context Find Treatment Procedure"@en ;
    rdfs:comment "Treatment will follow a particular procedure depending upon the diagnosis of finds staff"@en ;
    rdfs:isDefinedBy crmeh:CRMEH ;
    rdfs:subClassOf crm:E29_Design_or_Procedure ;
    owl:sameAs crmeh:EHE0041 ;
    skos:notation "EHE0041" .

crmeh:EHE0042_ContextFindTreatmentType a owl:Class ;
    rdfs:label "Context Find Treatment Type"@en ;
    rdfs:comment "Although finds may be given some interim treatment on site such as \"kept damp\" most treatments will take place off site as part of a conservation process. Treatments might include, PVA impregnation, cleaning, etc"@en ;
    rdfs:isDefinedBy crmeh:CRMEH ;
    rdfs:subClassOf crm:E55_Type ;
    owl:sameAs crmeh:EHE0042 ;
    skos:notation "EHE0042" .

crmeh:EHE0043_ContextFindUID a owl:Class ;
    rdfs:label "Context Find UID"@en ;
    rdfs:comment "The unique identifier allocated to a finds object as part of recording procedures. In most cases only special or small finds are given individual finds numbers. For small finds generally one number is allocated to each item, even if several objects are found together. In some cases one Small Find number is given to a group of pieces from one context, e.g. nails, window and vessel glass, but this is only done with prior agreement. General Bulk finds (e.g. pottery and animal bone), which tend to be processed and analysed in groups, are bagged and labelled with the context number that they come from, but not given individual UID finds numbers"@en ;
    rdfs:isDefinedBy crmeh:CRMEH ;
    rdfs:subClassOf crm:E42_Identifier ;
    owl:sameAs crmeh:EHE0043 ;
    skos:notation "EHE0043" .

crmeh:EHE0044_ContextFindUseEventRecordNote a rdfs:Datatype,
        owl:Class ;
    rdfs:label "Context Find Use Event Record Note"@en ;
    rdfs:comment "This is the actual notes of the proposed use that the find had. The note is made in the document that records information about how the find was used, or possibly re-used, in different ways. The idea of documenting events allows us to make assertions regarding the quality of the documentation. For example, it allows us to talk about uncertainty regarding different possible usage events when in reality the actual use (or uses) has happened and is therefore finite although it may not be known"@en ;
    rdfs:isDefinedBy crmeh:CRMEH ;
    rdfs:subClassOf rdfs:Literal ;
    owl:sameAs crmeh:EHE0044 ;
    skos:notation "EHE0044" .

crmeh:EHE0045_ContextFindUseEventRecordNoteType a owl:Class ;
    rdfs:label "Context Find Use Event Record Note Type"@en ;
    rdfs:comment "Type used to structure notes e.g. certainty"@en ;
    rdfs:isDefinedBy crmeh:CRMEH ;
    rdfs:subClassOf crm:E55_Type ;
    owl:sameAs crmeh:EHE0045 ;
    skos:notation "EHE0045" .

crmeh:EHE0046_ContextNote a rdfs:Datatype,
        owl:Class ;
    rdfs:label "Context Note"@en ;
    rdfs:comment "Notes on context and other attributes not needing further structure. Notes are further specified by type"@en ;
    rdfs:isDefinedBy crmeh:CRMEH ;
    rdfs:subClassOf rdfs:Literal ;
    owl:sameAs crmeh:EHE0046 ;
    skos:notation "EHE0046" .

crmeh:EHE0047_ContextNoteType a owl:Class ;
    rdfs:label "Context Note Type"@en ;
    rdfs:comment "Types of notes made on context record forms e.g. Method of Excavation, Weather, Comments, Interpretation"@en ;
    rdfs:isDefinedBy crmeh:CRMEH ;
    rdfs:subClassOf crm:E55_Type ;
    owl:sameAs crmeh:EHE0047 ;
    skos:notation "EHE0047" .

crmeh:EHE0048_ContextRecord a owl:Class ;
    rdfs:label "Context Record"@en ;
    rdfs:comment "The actual recording form used to record information about each individually numbered context. In practice there are a range of forms for various contexts, Deposit/Cuts, Timbers, Skeletons, Masonry, etc"@en ;
    rdfs:isDefinedBy crmeh:CRMEH ;
    rdfs:subClassOf crm:E73_Information_Object ;
    owl:sameAs crmeh:EHE0048 ;
    skos:notation "EHE0048" .

crmeh:EHE0049_ContextSampleMeasurement a owl:Class ;
    rdfs:label "Context Sample Measurement"@en ;
    rdfs:comment "Measurements taken during the processing of a sample"@en ;
    rdfs:isDefinedBy crmeh:CRMEH ;
    rdfs:subClassOf crm:E54_Dimension ;
    owl:sameAs crmeh:EHE0049 ;
    skos:notation "EHE0049" .

crmeh:EHE0050_ContextSampleMeasurementType a owl:Class ;
    rdfs:label "Context Sample Measurement Type"@en ;
    rdfs:comment "Type of measurement taken on a sample"@en ;
    rdfs:isDefinedBy crmeh:CRMEH ;
    rdfs:subClassOf crm:E55_Type ;
    owl:sameAs crmeh:EHE0050 ;
    skos:notation "EHE0050" .

crmeh:EHE0051_ContextSampleMeasurementUnit a owl:Class ;
    rdfs:label "Context Sample Measurement Unit"@en ;
    rdfs:comment "The unit of measurement used to record information about a sample e.g. metres,  kilogrammes, etc"@en ;
    rdfs:isDefinedBy crmeh:CRMEH ;
    rdfs:subClassOf crm:E58_Measurement_Unit ;
    owl:sameAs crmeh:EHE0051 ;
    skos:notation "EHE0051" .

crmeh:EHE0052_ContextSampleMeasurementValue a rdfs:Datatype,
        owl:Class ;
    rdfs:label "Context Sample Measurement Value"@en ;
    rdfs:comment "The actual value recorded for a measurement taken of a sample"@en ;
    rdfs:isDefinedBy crmeh:CRMEH ;
    rdfs:subClassOf xsd:float ;
    owl:sameAs crmeh:EHE0052 ;
    skos:notation "EHE0052" .

crmeh:EHE0053_ContextSampleType a owl:Class ;
    rdfs:label "Context Sample Type"@en ;
    rdfs:comment "Samples may be taken for a variety of analyses, e.g. to identify insect or faunal remains and the type of sample usually indicates how it will be processed. Sample types might include dendrochronology, radio-carbon dating, flotation, or soil column"@en ;
    rdfs:isDefinedBy crmeh:CRMEH ;
    rdfs:subClassOf crm:E55_Type ;
    owl:sameAs crmeh:EHE0053 ;
    skos:notation "EHE0053" .

crmeh:EHE0054_ContextStuffMeasurement a owl:Class ;
    rdfs:label "Context Stuff Measurement"@en ;
    rdfs:comment "Measurements of length, width, depth, diameter, orientation, etc, of a context"@en ;
    rdfs:isDefinedBy crmeh:CRMEH ;
    rdfs:subClassOf crm:E54_Dimension ;
    owl:sameAs crmeh:EHE0054 ;
    skos:notation "EHE0054" .

crmeh:EHE0055_ContextStuffMeasurementEventTimespan a owl:Class ;
    rdfs:label "Context Stuff Measurement Event Timespan"@en ;
    rdfs:comment "The timespan of the event of recording the physical attributes of a context"@en ;
    rdfs:isDefinedBy crmeh:CRMEH ;
    rdfs:subClassOf crm:E52_Time-Span ;
    owl:sameAs crmeh:EHE0055 ;
    skos:notation "EHE0055" .

crmeh:EHE0056_ContextStuffMeasurementEventType a owl:Class ;
    rdfs:label "Context Stuff Measurement Event Type"@en ;
    rdfs:isDefinedBy crmeh:CRMEH ;
    rdfs:subClassOf crm:E55_Type ;
    owl:sameAs crmeh:EHE0056 ;
    skos:notation "EHE0056" .

crmeh:EHE0057_ContextStuffMeasurementUnit a owl:Class ;
    rdfs:label "Context Stuff Measurement Unit"@en ;
    rdfs:isDefinedBy crmeh:CRMEH ;
    rdfs:subClassOf crm:E58_Measurement_Unit ;
    owl:sameAs crmeh:EHE0057 ;
    skos:notation "EHE0057" .

crmeh:EHE0058_ContextStuffMeasurementValue a rdfs:Datatype,
        owl:Class ;
    rdfs:label "Context Stuff Measurement Value"@en ;
    rdfs:isDefinedBy crmeh:CRMEH ;
    rdfs:subClassOf xsd:float ;
    owl:sameAs crmeh:EHE0058 ;
    skos:notation "EHE0058" .

crmeh:EHE0059_ContextStuffNote a rdfs:Datatype,
        owl:Class ;
    rdfs:label "Context Stuff Note"@en ;
    rdfs:comment "The notes made in context records about physical attributes of the context such as inclusions, compaction, colour, texture, contamination"@en ;
    rdfs:isDefinedBy crmeh:CRMEH ;
    rdfs:subClassOf rdfs:Literal ;
    owl:sameAs crmeh:EHE0059 ;
    skos:notation "EHE0059" .

crmeh:EHE0060_ContextStuffNoteType a owl:Class ;
    rdfs:label "Context Stuff Note Type"@en ;
    rdfs:comment "Types of context notes would be: compaction, colour, texture, inclusions, contamination, and more general comments fields"@en ;
    rdfs:isDefinedBy crmeh:CRMEH ;
    rdfs:subClassOf crm:E55_Type ;
    owl:sameAs crmeh:EHE0060 ;
    skos:notation "EHE0060" .

crmeh:EHE0061_ContextUID a owl:Class ;
    rdfs:label "Context UID"@en ;
    rdfs:comment "The number of the individual stratigraphic unit. All context numbers, be they stone or timber structures, deposits, cuts, or any other stratigraphic unit, must be part of a sequence recorded in project registers"@en ;
    rdfs:isDefinedBy crmeh:CRMEH ;
    rdfs:subClassOf crm:E48_Place_Name ;
    owl:sameAs crmeh:EHE0061 ;
    skos:notation "EHE0061" .

crmeh:EHE0062_FlotationSample a owl:Class ;
    rdfs:label "Flotation Sample"@en ;
    rdfs:comment "Some samples are known as flotation samples because of the way in which they are processed, using a flotation machine. The flotation process is a method of separating charred plant remains and charcoal from the rest of the sample. It uses the fact that charred plant remains are less dense than bone, gravel, and pottery, etc, and thus have a tendency to float or be held in suspension when a soil sample is added to water"@en ;
    rdfs:isDefinedBy crmeh:CRMEH ;
    rdfs:subClassOf crmeh:EHE0018_ContextSample ;
    owl:sameAs crmeh:EHE0062 ;
    skos:notation "EHE0062" .

crmeh:EHE0063_FlotationSampleResidue a owl:Class ;
    rdfs:label "Flotation Sample Residue"@en ;
    rdfs:comment "The residue is the material that does not float during flotation whereas the material that floats is called flot. Residues of different sizes get sorted and dealt with differently after flotation"@en ;
    rdfs:isDefinedBy crmeh:CRMEH ;
    rdfs:subClassOf crm:E18_Physical_Thing ;
    owl:sameAs crmeh:EHE0063 ;
    skos:notation "EHE0063" .

crmeh:EHE0064_FlotationSampleResidueMeasurement a owl:Class ;
    rdfs:label "Flotation Sample Residue Measurement"@en ;
    rdfs:comment "Measurements made on residues would include weight"@en ;
    rdfs:isDefinedBy crmeh:CRMEH ;
    rdfs:subClassOf crm:E54_Dimension ;
    owl:sameAs crmeh:EHE0064 ;
    skos:notation "EHE0064" .

crmeh:EHE0065_FlotationSampleResidueMeasurementUnit a owl:Class ;
    rdfs:label "Flotation Sample Residue Measurement Unit"@en ;
    rdfs:comment "Units of weight, e.g. Kg"@en ;
    rdfs:isDefinedBy crmeh:CRMEH ;
    rdfs:subClassOf crm:E58_Measurement_Unit ;
    owl:sameAs crmeh:EHE0065 ;
    skos:notation "EHE0065" .

crmeh:EHE0066_FlotationSampleResidueMeasurementValue a rdfs:Datatype,
        owl:Class ;
    rdfs:label "Flotation Sample Residue Measurement Value"@en ;
    rdfs:comment "The actual value of the measurement taken"@en ;
    rdfs:isDefinedBy crmeh:CRMEH ;
    rdfs:subClassOf xsd:float ;
    owl:sameAs crmeh:EHE0066 ;
    skos:notation "EHE0066" .

crmeh:EHE0067_FlotationSampleResidueType a owl:Class ;
    rdfs:label "Flotation Sample Residue Type"@en ;
    rdfs:comment "Different residues are usually distinguished according to the types and sizes of sieving used to process them"@en ;
    rdfs:isDefinedBy crmeh:CRMEH ;
    rdfs:subClassOf crm:E55_Type ;
    owl:sameAs crmeh:EHE0067 ;
    skos:notation "EHE0067" .

crmeh:EHE0068_GroupEventRecordNote a rdfs:Datatype,
        owl:Class ;
    rdfs:label "Group Event Record Note"@en ;
    rdfs:comment "Interpretive and descriptive notes about possible events in archaeological time, derived from analysis of a grouping of contexts. These notes would be made during the grouping and phasing process to build up the interpreted archaeological sequence and inter-relationships of contexts"@en ;
    rdfs:isDefinedBy crmeh:CRMEH ;
    rdfs:subClassOf rdfs:Literal ;
    owl:sameAs crmeh:EHE0068 ;
    skos:notation "EHE0068" .

crmeh:EHE0069_GroupEventRecordNoteType a owl:Class ;
    rdfs:label "Group Event Record Note Type"@en ;
    rdfs:comment "Group records may include aspects such as certainty, interim dating, description, interpretation"@en ;
    rdfs:isDefinedBy crmeh:CRMEH ;
    rdfs:subClassOf crm:E55_Type ;
    owl:sameAs crmeh:EHE0069 ;
    skos:notation "EHE0069" .

crmeh:EHE0070_GroupEventTimespan a owl:Class ;
    rdfs:label "Group Event Timespan"@en ;
    rdfs:comment "The time span of events such as the occupation of a building or how long a particular group of ditches were in use"@en ;
    rdfs:isDefinedBy crmeh:CRMEH ;
    rdfs:subClassOf crm:E52_Time-Span ;
    owl:sameAs crmeh:EHE0070 ;
    skos:notation "EHE0070" .

crmeh:EHE0071_GroupEventTimespanAppellation a owl:Class ;
    rdfs:label "Group Event Timespan Appellation"@en ;
    rdfs:comment "For the purposes of publication and dissemination, groups or phases will be distinguished by the period during which they were interpreted as being in use. Typical appellations might be e.g. late iron age, Early Romano-British, 2nd century, Mid-Roman, Late Roman, etc"@en ;
    rdfs:isDefinedBy crmeh:CRMEH ;
    rdfs:subClassOf crm:E49_Time_Appellation ;
    owl:sameAs crmeh:EHE0071 ;
    skos:notation "EHE0071" .

crmeh:EHE0072_GroupEventType a owl:Class ;
    rdfs:label "Group Event Type"@en ;
    rdfs:comment "Values drawn from controlled vocabulary of acceptable Group or Phase definitions e.g. construction, use, disuse"@en ;
    rdfs:isDefinedBy crmeh:CRMEH ;
    rdfs:subClassOf crm:E55_Type ;
    owl:sameAs crmeh:EHE0072 ;
    skos:notation "EHE0072" .

crmeh:EHE0073_GroupingPhasingProcedure a owl:Class ;
    rdfs:label "Grouping Phasing Procedure"@en ;
    rdfs:comment "The actual process of Grouping and Phasing. The process adopted may vary according to the organisation or individuals concerned, for example some use Land-use classifications"@en ;
    rdfs:isDefinedBy crmeh:CRMEH ;
    rdfs:subClassOf crm:E29_Design_or_Procedure ;
    owl:sameAs crmeh:EHE0073 ;
    skos:notation "EHE0073" .

crmeh:EHE0074_IdentifiedFeature a owl:Class ;
    rdfs:label "Identified Feature"@en ;
    rdfs:comment "Any physical feature identified for recording during investigation. This could range from a plan of all features pre-excavation to a feature identified through interpretation of a geophysical survey"@en ;
    rdfs:isDefinedBy crmeh:CRMEH ;
    rdfs:subClassOf crm:E53_Place ;
    owl:sameAs crmeh:EHE0074 ;
    skos:notation "EHE0074" .

crmeh:EHE0075_IdentifiedFeatureDepiction a owl:Class ;
    rdfs:label "Identified Feature Depiction"@en ;
    rdfs:comment "The actual spatial co-ordinates representing the physical location of any feature depicted by the drawn record"@en ;
    rdfs:isDefinedBy crmeh:CRMEH ;
    rdfs:subClassOf crm:E47_Spatial_Coordinates ;
    owl:sameAs crmeh:EHE0075 ;
    skos:notation "EHE0075" .

crmeh:EHE0076_ProjectDesign a owl:Class ;
    rdfs:label "Project Design"@en ;
    rdfs:comment "A project design is the document that contains details of how a project is to be carried out, who is involved and what resources are required. The project design should specify the research Aims and Objectives according to which the project data is being collected"@en ;
    rdfs:isDefinedBy crmeh:CRMEH ;
    rdfs:subClassOf crm:E29_Design_or_Procedure ;
    owl:sameAs crmeh:EHE0076 ;
    skos:notation "EHE0076" .

crmeh:EHE0077_ProjectTeamMember a owl:Class ;
    rdfs:label "Project Team Member"@en ;
    rdfs:comment "A variety of tasks and roles are fulfilled by people working on a project. Along with general project management, these would include excavating and recording contexts, measurement, classification and assessment of finds, Grouping and Phasing"@en ;
    rdfs:isDefinedBy crmeh:CRMEH ;
    rdfs:subClassOf crm:E39_Actor ;
    owl:sameAs crmeh:EHE0077 ;
    skos:notation "EHE0077" .

crmeh:EHE0078_ProjectTeamMemberRole a owl:Class ;
    rdfs:label "Project Team Member Role"@en ;
    rdfs:comment "It is important to identify the specific role(s) undertaken by a project team member so that their responsibilities and what is required of them is understood. Roles might include Project Manager, Supervisor, Finds manager, Environmental specialist, etc. It is possible for someone to have more than one role in a project team as long as this is clear to them and other members of the team"@en ;
    rdfs:isDefinedBy crmeh:CRMEH ;
    rdfs:subClassOf crm:E55_Type ;
    owl:sameAs crmeh:EHE0078 ;
    skos:notation "EHE0078" .

crmeh:EHE0079_RecordDrawingNote a rdfs:Datatype,
        owl:Class ;
    rdfs:label "Record Drawing Note"@en ;
    rdfs:comment "Notes made about drawn plans or sections. Might include location information about which area of the site the plan or section covers, and details of who did the drawing and what it depicts"@en ;
    rdfs:isDefinedBy crmeh:CRMEH ;
    rdfs:subClassOf rdfs:Literal ;
    owl:sameAs crmeh:EHE0079 ;
    skos:notation "EHE0079" .

crmeh:EHE0080_RecordDrawingNoteType a owl:Class ;
    rdfs:label "Record Drawing Note Type"@en ;
    rdfs:comment "Types of notes might include: Scale; Coordinates, Description of the context numbers shown; the area of the site depicted; drawn by and date. For survey and more interpretive drawings might include Certainty"@en ;
    rdfs:isDefinedBy crmeh:CRMEH ;
    rdfs:subClassOf crm:E55_Type ;
    owl:sameAs crmeh:EHE0080 ;
    skos:notation "EHE0080" .

crmeh:EHE0081_RecordDrawingReferenceType a owl:Class ;
    rdfs:label "Record Drawing Reference Type"@en ;
    rdfs:comment "The types will usually be \"Plan drawing of\" or Section drawing of\" and possibly \"profile drawing of\" or \"sketch drawing of\""@en ;
    rdfs:isDefinedBy crmeh:CRMEH ;
    rdfs:subClassOf crm:E55_Type ;
    owl:sameAs crmeh:EHE0081 ;
    skos:notation "EHE0081" .

crmeh:EHE0082_RecordDrawingSheet a owl:Class ;
    rdfs:label "Record Drawing Sheet"@en ;
    rdfs:comment "The actual drawing media for plans or sections either on paper, permatrace or as digital objects. This is primarily needed as a record of where, and how, the drawings are managed and stored, e.g. Section 5 is on Record Sheet 3"@en ;
    rdfs:isDefinedBy crmeh:CRMEH ;
    rdfs:subClassOf crm:E84_Information_Carrier ;
    owl:sameAs crmeh:EHE0082 ;
    skos:notation "EHE0082" .

crmeh:EHE0083_RecordPhotographNote a rdfs:Datatype,
        owl:Class ;
    rdfs:label "Record Photograph Note"@en ;
    rdfs:comment "Notes might include direction of shot, scales used, a description of the shot and the main contexts or other features recorded"@en ;
    rdfs:isDefinedBy crmeh:CRMEH ;
    rdfs:subClassOf rdfs:Literal ;
    owl:sameAs crmeh:EHE0083 ;
    skos:notation "EHE0083" .

crmeh:EHE0084_RecordPhotographNoteType a owl:Class ;
    rdfs:label "Record Photograph Note Type"@en ;
    rdfs:comment "Types include, colour, B/W, digital, shot number, film numbers, comments, scale"@en ;
    rdfs:isDefinedBy crmeh:CRMEH ;
    rdfs:subClassOf crm:E55_Type ;
    owl:sameAs crmeh:EHE0084 ;
    skos:notation "EHE0084" .

crmeh:EHE0085_RecordPhotographReferenceType a owl:Class ;
    rdfs:label "Record Photograph Reference Type"@en ;
    rdfs:comment "Will be \"Colour photo of\" or \"Black and White (B/W) photo of\" or \"Digital photo of\""@en ;
    rdfs:isDefinedBy crmeh:CRMEH ;
    rdfs:subClassOf crm:E55_Type ;
    owl:sameAs crmeh:EHE0085 ;
    skos:notation "EHE0085" .

crmeh:EHE0086_ResponsibleAgent a owl:Class ;
    rdfs:label "Responsible Agent"@en ;
    rdfs:comment "This is used to record the person or organisation that takes responsibility for records and finds when an archive is transferred."@en ;
    rdfs:isDefinedBy crmeh:CRMEH ;
    rdfs:subClassOf crm:E39_Actor ;
    owl:sameAs crmeh:EHE0086 ;
    skos:notation "EHE0086" .

crmeh:EHE0087_SiteSubDivisionAppellation a owl:Class ;
    rdfs:label "Site Sub-Division Appellation"@en ;
    rdfs:comment "Name given to demarcate different sub-divisions of a site e.g. Trench 1, Area C, etc"@en ;
    rdfs:isDefinedBy crmeh:CRMEH ;
    rdfs:subClassOf crm:E48_Place_Name ;
    owl:sameAs crmeh:EHE0087 ;
    skos:notation "EHE0087" .

crmeh:EHE0088_SiteSubDivisionDepiction a owl:Class ;
    rdfs:label "Site Sub-Division Depiction"@en ;
    rdfs:comment "Spatial coordinates depicting the extent of a site sub division such as in a plan of a trench"@en ;
    rdfs:isDefinedBy crmeh:CRMEH ;
    rdfs:subClassOf crm:E47_Spatial_Coordinates ;
    owl:sameAs crmeh:EHE0088 ;
    skos:notation "EHE0088" .

crmeh:EHE0089_StorageLocation a owl:Class ;
    rdfs:label "Storage Location"@en ;
    rdfs:comment "This entity could be used to record either the current location or the new location of a record or an object"@en ;
    rdfs:isDefinedBy crmeh:CRMEH ;
    rdfs:subClassOf crm:E53_Place ;
    owl:sameAs crmeh:EHE0089 ;
    skos:notation "EHE0089" .

crmeh:EHE0090_SurveyDataset a owl:Class ;
    rdfs:label "Survey Dataset"@en ;
    rdfs:comment "This distinguishes data derived by non-intrusive survey recording from excavation data. This dataset could be from a topographic, geophysical, GPS or other survey activity"@en ;
    rdfs:isDefinedBy crmeh:CRMEH ;
    rdfs:subClassOf crm:E73_Information_Object ;
    owl:sameAs crmeh:EHE0090 ;
    skos:notation "EHE0090" .

crmeh:EHE0091_Timestamp a rdfs:Datatype,
        owl:Class ;
    rdfs:label "Timestamp"@en ;
    rdfs:comment "Used to record start and end dates for the time span of events and activities"@en ;
    rdfs:isDefinedBy crmeh:CRMEH ;
    rdfs:subClassOf rdfs:Literal ;
    owl:sameAs crmeh:EHE0091 ;
    skos:notation "EHE0091" .

crmeh:EHE0092_GroupUID a owl:Class ;
    rdfs:label "Group UID"@en ;
    rdfs:comment "The unique identifier given to a grouped collection of contexts so that the group can be treated as an integrated entity for analysis."@en ;
    rdfs:isDefinedBy crmeh:CRMEH ;
    rdfs:subClassOf crm:E48_Place_Name ;
    owl:sameAs crmeh:EHE0092 ;
    skos:notation "EHE0092" .

crmeh:EHE0093_GroupDepiction a owl:Class ;
    rdfs:label "Group Depiction"@en ;
    rdfs:comment "For spatial analysis a group will need a plan. This will usually be derived by combination of the individual plans for the associated group of individual contexts"@en ;
    rdfs:isDefinedBy crmeh:CRMEH ;
    rdfs:subClassOf crm:E47_Spatial_Coordinates ;
    owl:sameAs crmeh:EHE0093 ;
    skos:notation "EHE0093" .

crmeh:EHE0094_FlotationSampleResidueMeasurementType a owl:Class ;
    rdfs:label "Flotation Sample Residue Measurement Type"@en ;
    rdfs:comment "Most often weight, and then counts of different items such as bone and other finds"@en ;
    rdfs:isDefinedBy crmeh:CRMEH ;
    rdfs:subClassOf crm:E55_Type ;
    owl:sameAs crmeh:EHE0094 ;
    skos:notation "EHE0094" .

crmeh:EHE0095_ContextFindProductionEventLocation a owl:Class ;
    rdfs:label "Context Find Production Event Location"@en ;
    rdfs:comment "For refinement of the dating of finds based upon finds typologies and regional or local variations in manufacturing and production techniques. Also analysis of interactions with other localities and associated  trading patterns"@en ;
    rdfs:isDefinedBy crmeh:CRMEH ;
    rdfs:subClassOf crm:E53_Place ;
    owl:sameAs crmeh:EHE0095 ;
    skos:notation "EHE0095" .

crmeh:EHE0096_ContextFindGeneralUse a owl:Class ;
    rdfs:label "Context Find General Use"@en ;
    rdfs:comment "In general a finds data set should provide evidence of the usage of a find up to the point where it was deposited in the context in which it was found. The general use may refer to how something was reused in the context it was discovered. Thus a timber might have had a general use when it was excavated as part of a waterside revetment, even though it also showed evidence of previously being intended as a boat timber (see ContextFindIntendedUse EHE0097)"@en ;
    rdfs:isDefinedBy crmeh:CRMEH ;
    rdfs:subClassOf crm:E55_Type ;
    owl:sameAs crmeh:EHE0096 ;
    skos:notation "EHE0096" .

crmeh:EHE0097_ContextFindIntendedUse a owl:Class ;
    rdfs:label "Context Find Intended Use"@en ;
    rdfs:comment "As noted (EHE0097), some finds do not end up being used in the way that their makers might have intended. It is sometimes necessary therefore to distinguish the original intended use for which something was made, from the general use that it ended up having. (e.g. quite often pieces of sculpture get reused as building material in later walls, once the significance of them as art or religious works goes out of fashion)"@en ;
    rdfs:isDefinedBy crmeh:CRMEH ;
    rdfs:subClassOf crm:E55_Type ;
    owl:sameAs crmeh:EHE0097 ;
    skos:notation "EHE0097" .

crmeh:EHE0098_ContextExcavationEventTimespan a owl:Class ;
    rdfs:label "Context Excavation Event Timespan"@en ;
    rdfs:comment "This could be the time taken for excavating an individual context or the time taken for the whole excavation event"@en ;
    rdfs:isDefinedBy crmeh:CRMEH ;
    rdfs:subClassOf crm:E52_Time-Span ;
    owl:sameAs crmeh:EHE0098 ;
    skos:notation "EHE0098" .

crmeh:EHE0099_ContextFindUseEventTimespan a owl:Class ;
    rdfs:label "Context Find Use Event Timespan"@en ;
    rdfs:comment "Time duration of event associated with the proposed use of a find. E.g. time span that a pot was in use. Allows us to make statements about the likely length of time finds were being used before they ended up being deposited and this may effect judgements about the relative grouping and phasing of contexts"@en ;
    rdfs:isDefinedBy crmeh:CRMEH ;
    rdfs:subClassOf crm:E52_Time-Span ;
    owl:sameAs crmeh:EHE0099 ;
    skos:notation "EHE0099" .

crmeh:EHE0100_ContextSamplingEventType a owl:Class ;
    rdfs:label "Context Sampling Event Type"@en ;
    rdfs:comment "When sampling archaeological remains, different types of sampling method can be used"@en ;
    rdfs:isDefinedBy crmeh:CRMEH ;
    rdfs:subClassOf crm:E55_Type ;
    owl:sameAs crmeh:EHE0100 ;
    skos:notation "EHE0100" .

crmeh:EHE1001_ContextEvent a owl:Class ;
    rdfs:label "Context Event"@en ;
    rdfs:comment "By modelling context formation as an event in CRM terms, it is a spatio-temporal phenomenon. We can reason about the sequence in which context formation events took place and build a stratigraphic understanding of the site. We are interested in the formation of the context as it is observed when excavated and the condition it is in (i.e. the effect of any natural modification events such as waterlogging or chemical leaching)"@en ;
    rdfs:isDefinedBy crmeh:CRMEH ;
    rdfs:subClassOf crm:E63_Beginning_of_Existence ;
    owl:sameAs crmeh:EHE1001 ;
    skos:notation "EHE1001" .

crmeh:EHE1002_ContextFindProductionEvent a owl:Class ;
    rdfs:label "Context Find Production Event"@en ;
    rdfs:comment "Events which took place in the past and resulted in the production of artefacts which later came to be deposited and eventually excavated. We may know very little about such events, but this entity is necessary in order to discuss modes of production, place of manufacture, etc. It is this entity that provides basic spot-dating evidence for contexts (i.e. the date of context finds)"@en ;
    rdfs:isDefinedBy crmeh:CRMEH ;
    rdfs:subClassOf crm:E12_Production ;
    owl:sameAs crmeh:EHE1002 ;
    skos:notation "EHE1002" .

crmeh:EHE1003_GroupEvent a owl:Class ;
    rdfs:label "Group Event"@en ;
    rdfs:comment "The construction of a sequence of development is effectively the process of phasing. Based upon the sequence of context formation (i.e. stratigraphic sequence), any finds (i.e. spot dating) and any other pertinent information, sub-groups and groups (and further levels of group as required) are used to develop a sequence of landscape events for the excavation. This sequence of landscape events is effectively the phased chronology for the site based on available evidence "@en ;
    rdfs:isDefinedBy crmeh:CRMEH ;
    rdfs:subClassOf crm:E5_Event ;
    owl:sameAs crmeh:EHE1003 ;
    skos:notation "EHE1003" .

crmeh:EHE1004_ContextFindDepositionEvent a owl:Class ;
    rdfs:label "Context Find Deposition Event"@en ;
    rdfs:comment "The construction of a sequence of development is effectively the process of phasing. Based upon the sequence of context formation (i.e. stratigraphic sequence), any finds (i.e. spot dating) and any other pertinent information, sub-groups and groups (and further levels of group as required) are used to develop a sequence of landscape events for the excavation. This sequence of landscape events is effectively the phased chronology for the site based on available evidence"@en ;
    rdfs:isDefinedBy crmeh:CRMEH ;
    rdfs:subClassOf crm:E9_Move ;
    owl:sameAs crmeh:EHE1004 ;
    skos:notation "EHE1004" .

crmeh:EHE1005_ContextFindUseEvent a owl:Class ;
    rdfs:label "Context Find Use Event"@en ;
    rdfs:isDefinedBy crmeh:CRMEH ;
    rdfs:subClassOf crm:E7_Activity ;
    owl:sameAs crmeh:EHE1005 ;
    skos:notation "EHE1005" .

crmeh:EHE2001_ContextExcavationEvent a owl:Class ;
    rdfs:label "Context Excavation Event"@en ;
    rdfs:comment "The process of excavation results in the destruction of the physical stuff at a particular place, i.e. a context. It also results in the production of knowledge regarding said place"@en ;
    rdfs:isDefinedBy crmeh:CRMEH ;
    rdfs:subClassOf crm:E65_Creation,
        crm:E6_Destruction ;
    owl:sameAs crmeh:EHE2001 ;
    skos:notation "EHE2001" .

crmeh:EHE2002_ContextFindClassificationEvent a owl:Class ;
    rdfs:label "Context Find Classification Event"@en ;
    rdfs:comment "The classification of finds according to some typology or other"@en ;
    rdfs:isDefinedBy crmeh:CRMEH ;
    rdfs:subClassOf crm:E17_Type_Assignment ;
    owl:sameAs crmeh:EHE2002 ;
    skos:notation "EHE2002" .

crmeh:EHE2003_ContextFindTreatmentEvent a owl:Class ;
    rdfs:label "Context Find Treatment Event"@en ;
    rdfs:comment "The various processes applied to objects by finds specialists and conservators"@en ;
    rdfs:isDefinedBy crmeh:CRMEH ;
    rdfs:subClassOf crm:E11_Modification ;
    owl:sameAs crmeh:EHE2003 ;
    skos:notation "EHE2003" .

crmeh:EHE2004_GroupingPhasingEvent a owl:Class ;
    rdfs:label "Grouping Phasing Event"@en ;
    rdfs:comment "This creation event produces the phasing record which we can then make assertions about. As with context formation, the events which make up the sequence of phases have unknown but fixed time-spans; it is our understanding of this time-span which we can reason about. This allows multiple interpretations of the same underlying chronological sequence of which we may only have partial information"@en ;
    rdfs:isDefinedBy crmeh:CRMEH ;
    rdfs:subClassOf crm:E65_Creation ;
    owl:sameAs crmeh:EHE2004 ;
    skos:notation "EHE2004" .

crmeh:EHE2005_ContextFindDatingEvent a owl:Class ;
    rdfs:label "Context Find Dating Event"@en ;
    rdfs:comment "The process of assigning dates to finds. In terms of the CRM, the date of a find is the date of creation of the find. As with phasing and excavation, it is the documented time-span associated with a find not the actual time-span we make assertions about (the actual time-span being potentially unknown)"@en ;
    rdfs:isDefinedBy crmeh:CRMEH ;
    rdfs:subClassOf crm:E65_Creation ;
    owl:sameAs crmeh:EHE2005 ;
    skos:notation "EHE2005" .

crmeh:EHE2006_ContextSamplingEvent a owl:Class ;
    rdfs:label "Context Sampling Event"@en ;
    rdfs:comment "The process of sampling can be seen as a part removal of some matter to be further studied. There is a problem here regarding part removal from natural, non-man-made objects (i.e. the CRM does not allow this) which needs to be resolved"@en ;
    rdfs:isDefinedBy crmeh:CRMEH ;
    rdfs:subClassOf crm:E80_Part_Removal ;
    owl:sameAs crmeh:EHE2006 ;
    skos:notation "EHE2006" .

crmeh:EHE2007_SurveyEvent a owl:Class ;
    rdfs:label "Survey Event"@en ;
    rdfs:comment "The concept of survey is here used to describe activities which involve going to a location and gathering some data. This includes geochemical surveys as well as auger surveys, topographic surveys, geophysical surveys and the like; they can all be characterised by the site-based nature of the data gathering activity and the resultant (often spatial) dataset"@en ;
    rdfs:isDefinedBy crmeh:CRMEH ;
    rdfs:subClassOf crm:E65_Creation ;
    owl:sameAs crmeh:EHE2007 ;
    skos:notation "EHE2007" .

crmeh:EHE2008_ProcessSurveyDatasetEvent a owl:Class ;
    rdfs:label "Process Survey Dataset Event"@en ;
    rdfs:comment "This is the process of taking a raw survey dataset and processing/interpreting it. This will generally result in some kind of plot, trace or plan of the survey results e.g. an interpolated surface showing geochemical trends"@en ;
    rdfs:isDefinedBy crmeh:CRMEH ;
    rdfs:subClassOf crm:E65_Creation ;
    owl:sameAs crmeh:EHE2008 ;
    skos:notation "EHE2008" .

crmeh:EHE2009_TransferObjectEvent a owl:Class ;
    rdfs:label "Transfer Object Event"@en ;
    rdfs:comment "This entity allows us to track the movements of objects, including paper/digital copies of information objects such as drawings, photos and context sheets"@en ;
    rdfs:isDefinedBy crmeh:CRMEH ;
    rdfs:subClassOf crm:E10_Transfer_of_Custody,
        crm:E9_Move ;
    owl:sameAs crmeh:EHE2009 ;
    skos:notation "EHE2009" .

crmeh:EHE2011_BulkFindItemRemovalEvent a owl:Class ;
    rdfs:label "Bulk Find Item Removal Event"@en ;
    rdfs:comment "Sometimes items that have been collected as part of a bulk finds group, may be identified during further processing as worthy of individual analysis. Such items will be extracted from the bulk finds. E.g. a piece of pottery collected as a bulk find which is found after washing and processing to have graffiti on it requiring specialist identification work"@en ;
    rdfs:isDefinedBy crmeh:CRMEH ;
    rdfs:subClassOf crm:E80_Part_Removal ;
    owl:sameAs crmeh:EHE2011 ;
    skos:notation "EHE2011" .

crmeh:EHE2012_ContextFindConditionAssessmentEvent a owl:Class ;
    rdfs:label "Context Find Condition Assessment Event"@en ;
    rdfs:comment "Assessment of the condition of a small find to decide any conservation needs"@en ;
    rdfs:isDefinedBy crmeh:CRMEH ;
    rdfs:subClassOf crm:E14_Condition_Assessment ;
    owl:sameAs crmeh:EHE2012 ;
    skos:notation "EHE2012" .

crmeh:EHE2013_ContextFindIdentifierAssignmentEvent a owl:Class ;
    rdfs:label "Context Find Identifier Assignment Event"@en ;
    rdfs:comment "Finds which are extracted from bulk samples will need a small finds number UID"@en ;
    rdfs:isDefinedBy crmeh:CRMEH ;
    rdfs:subClassOf crm:E15_Identifier_Assignment ;
    owl:sameAs crmeh:EHE2013 ;
    skos:notation "EHE2013" .

crmeh:EHE2014_ContextFindUseAssessmentEvent a owl:Class ;
    rdfs:label "Context Find Use Assessment Event"@en ;
    rdfs:comment "This describes the process of assessing the functional aspect of an object; the kinds of use that an object was designed for, uses to which it was actually put and even specific relationships to particular events"@en ;
    rdfs:isDefinedBy crmeh:CRMEH ;
    rdfs:subClassOf crm:E17_Type_Assignment,
        crm:E65_Creation ;
    owl:sameAs crmeh:EHE2014 ;
    skos:notation "EHE2014" .

crmeh:EHE2015_ContextSampleProcessingEvent a owl:Class ;
    rdfs:label "Context Sample Processing Event"@en ;
    rdfs:comment "Sample quantification, classification and measurement. Might include Radio-carbon analysis, dendrochronological analysis, floatation"@en ;
    rdfs:isDefinedBy crmeh:CRMEH ;
    rdfs:subClassOf crm:E16_Measurement,
        crm:E17_Type_Assignment ;
    owl:sameAs crmeh:EHE2015 ;
    skos:notation "EHE2015" .

crmeh:EHE2016_ContextStuffMeasurementEvent a owl:Class ;
    rdfs:label "Context Stuff Measurement Event"@en ;
    rdfs:comment "Measurements taken on the physical aspects of a context, such as the length, width, or orientation of a feature or deposit"@en ;
    rdfs:isDefinedBy crmeh:CRMEH ;
    rdfs:subClassOf crm:E16_Measurement ;
    owl:sameAs crmeh:EHE2016 ;
    skos:notation "EHE2016" .

crmeh:EHE2017_FlotationSampleProcessingEvent a owl:Class ;
    rdfs:label "Flotation Sample Processing Event"@en ;
    rdfs:comment "The particular process of floatation of an environmental sample, that involves applying water to soil samples and collecting the outputs. This processing event in effect transforms a soil sample from a solid sample into a number of different products such as flotation samples (flot) which float and heavier residues that are collected in various sieves, along with any finds or other objects extracted for further analysis"@en ;
    rdfs:isDefinedBy crmeh:CRMEH ;
    rdfs:subClassOf crm:E81_Transformation ;
    owl:sameAs crmeh:EHE2017 ;
    skos:notation "EHE2017" .

crmeh:EHE2018_FlotationSampleResidueProcessingEvent a owl:Class ;
    rdfs:label "Flotation Sample Residue Processing Event"@en ;
    rdfs:comment "The process of flotation results in residues which are collected in various types of sieve. The residues are assigned types according to the size of sieving mesh in which they are collected, and the residue is measured (usually weighed) and analysed for the presence of small objects"@en ;
    rdfs:isDefinedBy crmeh:CRMEH ;
    rdfs:subClassOf crm:E16_Measurement,
        crm:E17_Type_Assignment ;
    owl:sameAs crmeh:EHE2018 ;
    skos:notation "EHE2018" .

crmeh:EHE2019_SimpleNameAssignmentEvent a owl:Class ;
    rdfs:label "Simple Name Assignment Event"@en ;
    rdfs:comment "This is the name, derived from a glossary list of types, which the recorder assigns to a context they are recording. Common examples might include: layer, pit, ditch, wall, etc"@en ;
    rdfs:isDefinedBy crmeh:CRMEH ;
    rdfs:subClassOf crm:E17_Type_Assignment ;
    owl:sameAs crmeh:EHE2019 ;
    skos:notation "EHE2019" .

crmeh:EHE2020_ContextFindMeasurementEvent a owl:Class ;
    rdfs:label "Context Find Measurement Event"@en ;
    rdfs:comment "The process of taking measurements of finds objects such as length, width, diameter, weight, etc. There are a number of different types of measurement event which are documented as part of the procedures for recording and analysing finds"@en ;
    rdfs:isDefinedBy crmeh:CRMEH ;
    rdfs:subClassOf crm:E16_Measurement ;
    owl:sameAs crmeh:EHE2020 ;
    skos:notation "EHE2020" .

crmeh:EHE2021_BulkFindAssessment a owl:Class ;
    rdfs:label "Bulk Find Assessment"@en ;
    rdfs:comment "An assessment of the items in the bulk find"@en ;
    rdfs:isDefinedBy crmeh:CRMEH ;
    rdfs:subClassOf crm:E13_Attribute_Assignment ;
    owl:sameAs crmeh:EHE2021 ;
    skos:notation "EHE2021" .

crmeh:EHP1_is_trace_of a owl:ObjectProperty ;
    rdfs:label "is trace of"@en ;
    rdfs:comment "This link is a shortcut of the full path describing that part of the Context Stuff is result of a transformation process of something of archaeological interest. In this way, we can talk about e.g. a group of post-holes representing a post-built structure, the group being used to represent the (creation of the) building. It is then reasonable to describe events happening at the building"@en ;
    rdfs:domain crmeh:EHE0008_ContextStuff ;
    rdfs:isDefinedBy crmeh:CRMEH ;
    rdfs:range crmeh:EHE0006_GroupStuff ;
    owl:sameAs crmeh:EHP1 ;
    skos:notation "EHP1" .

crmeh:EHP2_is_trace_of_type a owl:ObjectProperty ;
    rdfs:label "is trace of type"@en ;
    rdfs:comment "This link is a shortcut of the full path describing that part of the Context Stuff is result of a transformation process of types of things"@en ;
    rdfs:domain crmeh:EHE0008_ContextStuff ;
    rdfs:isDefinedBy crmeh:CRMEH ;
    rdfs:range crm:E55_Type ;
    rdfs:subPropertyOf crm:P2_has_type ;
    owl:sameAs crmeh:EHP2 ;
    skos:notation "EHP2" .

crmeh:EXP1 a owl:DataTypeProperty ;
    rdfs:label "timespan start"@en ;
    rdfs:comment "start year for timespan"@en ;
    rdfs:domain crm:E52_Time-Span ;
    rdfs:isDefinedBy crmeh:CRMEH ;
    rdfs:range xsd:gYear ;
    rdfs:subPropertyOf rdf:value .

crmeh:EXP10_is_represented_by a owl:ObjectProperty ;
    rdfs:label "is represented by"@en ;
    rdfs:comment "Relationship between E55 type and SKOS concept. Extension property to link E55.Type to skos:Concept without saying they are the SAME resource"@en ;
    rdfs:domain crm:E55_Type ;
    rdfs:isDefinedBy crmeh:CRMEH ;
    rdfs:range skos:Concept .

crmeh:EXP2 a owl:DataTypeProperty ;
    rdfs:label "timespan end"@en ;
    rdfs:comment "end year for timespan"@en ;
    rdfs:domain crm:E52_Time-Span ;
    rdfs:isDefinedBy crmeh:CRMEH ;
    rdfs:range xsd:gYear ;
    rdfs:subPropertyOf rdf:value .

crmeh:EXP3 a owl:DataTypeProperty ;
    rdfs:label "spatial x coordinate"@en ;
    rdfs:comment "extension property to hold the 'x' part of a spatial coordinate (longitude)"@en ;
    rdfs:domain crm:E47_Spatial_Coordinates ;
    rdfs:isDefinedBy crmeh:CRMEH ;
    rdfs:range xsd:float ;
    rdfs:subPropertyOf rdf:value .

crmeh:EXP4 a owl:DataTypeProperty ;
    rdfs:label "spatial y coordinate"@en ;
    rdfs:comment "extension property to hold the 'y' part of a spatial coordinate (latitude)"@en ;
    rdfs:domain crm:E47_Spatial_Coordinates ;
    rdfs:isDefinedBy crmeh:CRMEH ;
    rdfs:range xsd:float ;
    rdfs:subPropertyOf rdf:value .

crmeh:EXP5 a owl:DataTypeProperty ;
    rdfs:label "spatial z coordinate"@en ;
    rdfs:comment "extension property to hold the 'z' part of a spatial coordinate (altitude)"@en ;
    rdfs:domain crm:E47_Spatial_Coordinates ;
    rdfs:isDefinedBy crmeh:CRMEH ;
    rdfs:range xsd:float ;
    rdfs:subPropertyOf rdf:value .

dcterms:Box a rdfs:Datatype ;
    rdfs:label "DCMI Box"@en ;
    dcterms:hasVersion history:Box-003 ;
    dcterms:issued "2000-07-11"^^xsd:date ;
    dcterms:modified "2008-01-14"^^xsd:date ;
    rdfs:comment "The set of regions in space defined by their geographic coordinates according to the DCMI Box Encoding Scheme."@en ;
    rdfs:isDefinedBy dcterms: ;
    rdfs:seeAlso <http://dublincore.org/documents/dcmi-box/> .

dcterms:DCMIType a dcam:VocabularyEncodingScheme ;
    rdfs:label "DCMI Type Vocabulary"@en ;
    dcterms:hasVersion history:DCMIType-005 ;
    dcterms:issued "2000-07-11"^^xsd:date ;
    dcterms:modified "2012-06-14"^^xsd:date ;
    rdfs:comment "The set of classes specified by the DCMI Type Vocabulary, used to categorize the nature or genre of the resource."@en ;
    rdfs:isDefinedBy dcterms: ;
    rdfs:seeAlso dctypes: .

dcterms:DDC a dcam:VocabularyEncodingScheme ;
    rdfs:label "DDC"@en ;
    dcterms:hasVersion history:DDC-003 ;
    dcterms:issued "2000-07-11"^^xsd:date ;
    dcterms:modified "2008-01-14"^^xsd:date ;
    rdfs:comment "The set of conceptual resources specified by the Dewey Decimal Classification."@en ;
    rdfs:isDefinedBy dcterms: ;
    rdfs:seeAlso <http://www.oclc.org/dewey/> .

dcterms:IMT a dcam:VocabularyEncodingScheme ;
    rdfs:label "IMT"@en ;
    dcterms:hasVersion history:IMT-004 ;
    dcterms:issued "2000-07-11"^^xsd:date ;
    dcterms:modified "2008-01-14"^^xsd:date ;
    rdfs:comment "The set of media types specified by the Internet Assigned Numbers Authority."@en ;
    rdfs:isDefinedBy dcterms: ;
    rdfs:seeAlso <http://www.iana.org/assignments/media-types/> .

dcterms:ISO3166 a rdfs:Datatype ;
    rdfs:label "ISO 3166"@en ;
    dcterms:hasVersion history:ISO3166-004 ;
    dcterms:issued "2000-07-11"^^xsd:date ;
    dcterms:modified "2008-01-14"^^xsd:date ;
    rdfs:comment "The set of codes listed in ISO 3166-1 for the representation of names of countries."@en ;
    rdfs:isDefinedBy dcterms: ;
    rdfs:seeAlso <http://www.iso.org/iso/en/prods-services/iso3166ma/02iso-3166-code-lists/list-en1.html> .

dcterms:ISO639-2 a rdfs:Datatype ;
    rdfs:label "ISO 639-2"@en ;
    dcterms:hasVersion history:ISO639-2-003 ;
    dcterms:issued "2000-07-11"^^xsd:date ;
    dcterms:modified "2008-01-14"^^xsd:date ;
    rdfs:comment "The three-letter alphabetic codes listed in ISO639-2 for the representation of names of languages."@en ;
    rdfs:isDefinedBy dcterms: ;
    rdfs:seeAlso <http://lcweb.loc.gov/standards/iso639-2/langhome.html> .

dcterms:ISO639-3 a rdfs:Datatype ;
    rdfs:label "ISO 639-3"@en ;
    dcterms:hasVersion history:ISO639-3-001 ;
    dcterms:issued "2008-01-14"^^xsd:date ;
    rdfs:comment "The set of three-letter codes listed in ISO 639-3 for the representation of names of languages."@en ;
    rdfs:isDefinedBy dcterms: ;
    rdfs:seeAlso <http://www.sil.org/iso639-3/> .

dcterms:LCC a dcam:VocabularyEncodingScheme ;
    rdfs:label "LCC"@en ;
    dcterms:hasVersion history:LCC-003 ;
    dcterms:issued "2000-07-11"^^xsd:date ;
    dcterms:modified "2008-01-14"^^xsd:date ;
    rdfs:comment "The set of conceptual resources specified by the Library of Congress Classification."@en ;
    rdfs:isDefinedBy dcterms: ;
    rdfs:seeAlso <http://lcweb.loc.gov/catdir/cpso/lcco/lcco.html> .

dcterms:LCSH a dcam:VocabularyEncodingScheme ;
    rdfs:label "LCSH"@en ;
    dcterms:hasVersion history:LCSH-003 ;
    dcterms:issued "2000-07-11"^^xsd:date ;
    dcterms:modified "2008-01-14"^^xsd:date ;
    rdfs:comment "The set of labeled concepts specified by the Library of Congress Subject Headings."@en ;
    rdfs:isDefinedBy dcterms: .

dcterms:MESH a dcam:VocabularyEncodingScheme ;
    rdfs:label "MeSH"@en ;
    dcterms:hasVersion history:MESH-003 ;
    dcterms:issued "2000-07-11"^^xsd:date ;
    dcterms:modified "2008-01-14"^^xsd:date ;
    rdfs:comment "The set of labeled concepts specified by the Medical Subject Headings."@en ;
    rdfs:isDefinedBy dcterms: ;
    rdfs:seeAlso <http://www.nlm.nih.gov/mesh/meshhome.html> .

dcterms:NLM a dcam:VocabularyEncodingScheme ;
    rdfs:label "NLM"@en ;
    dcterms:hasVersion history:NLM-002 ;
    dcterms:issued "2005-06-13"^^xsd:date ;
    dcterms:modified "2008-01-14"^^xsd:date ;
    rdfs:comment "The set of conceptual resources specified by the National Library of Medicine Classification."@en ;
    rdfs:isDefinedBy dcterms: ;
    rdfs:seeAlso <http://wwwcf.nlm.nih.gov/class/> .

dcterms:Period a rdfs:Datatype ;
    rdfs:label "DCMI Period"@en ;
    dcterms:hasVersion history:Period-003 ;
    dcterms:issued "2000-07-11"^^xsd:date ;
    dcterms:modified "2008-01-14"^^xsd:date ;
    rdfs:comment "The set of time intervals defined by their limits according to the DCMI Period Encoding Scheme."@en ;
    rdfs:isDefinedBy dcterms: ;
    rdfs:seeAlso <http://dublincore.org/documents/dcmi-period/> .

dcterms:Point a rdfs:Datatype ;
    rdfs:label "DCMI Point"@en ;
    dcterms:hasVersion history:Point-003 ;
    dcterms:issued "2000-07-11"^^xsd:date ;
    dcterms:modified "2008-01-14"^^xsd:date ;
    rdfs:comment "The set of points in space defined by their geographic coordinates according to the DCMI Point Encoding Scheme."@en ;
    rdfs:isDefinedBy dcterms: ;
    rdfs:seeAlso <http://dublincore.org/documents/dcmi-point/> .

dcterms:RFC1766 a rdfs:Datatype ;
    rdfs:label "RFC 1766"@en ;
    dcterms:hasVersion history:RFC1766-003 ;
    dcterms:issued "2000-07-11"^^xsd:date ;
    dcterms:modified "2008-01-14"^^xsd:date ;
    rdfs:comment "The set of tags, constructed according to RFC 1766, for the identification of languages."@en ;
    rdfs:isDefinedBy dcterms: ;
    rdfs:seeAlso <http://www.ietf.org/rfc/rfc1766.txt> .

dcterms:RFC3066 a rdfs:Datatype ;
    rdfs:label "RFC 3066"@en ;
    dcterms:description "RFC 3066 has been obsoleted by RFC 4646."@en ;
    dcterms:hasVersion history:RFC3066-002 ;
    dcterms:issued "2002-07-13"^^xsd:date ;
    dcterms:modified "2008-01-14"^^xsd:date ;
    rdfs:comment "The set of tags constructed according to RFC 3066 for the identification of languages."@en ;
    rdfs:isDefinedBy dcterms: ;
    rdfs:seeAlso <http://www.ietf.org/rfc/rfc3066.txt> .

dcterms:RFC4646 a rdfs:Datatype ;
    rdfs:label "RFC 4646"@en ;
    dcterms:description "RFC 4646 obsoletes RFC 3066."@en ;
    dcterms:hasVersion history:RFC4646-001 ;
    dcterms:issued "2008-01-14"^^xsd:date ;
    rdfs:comment "The set of tags constructed according to RFC 4646 for the identification of languages."@en ;
    rdfs:isDefinedBy dcterms: ;
    rdfs:seeAlso <http://www.ietf.org/rfc/rfc4646.txt> .

dcterms:RFC5646 a rdfs:Datatype ;
    rdfs:label "RFC 5646"@en ;
    dcterms:description "RFC 5646 obsoletes RFC 4646."@en ;
    dcterms:hasVersion history:RFC5646-001 ;
    dcterms:issued "2010-10-11"^^xsd:date ;
    rdfs:comment "The set of tags constructed according to RFC 5646 for the identification of languages."@en ;
    rdfs:isDefinedBy dcterms: ;
    rdfs:seeAlso <http://www.ietf.org/rfc/rfc5646.txt> .

dcterms:TGN a dcam:VocabularyEncodingScheme ;
    rdfs:label "TGN"@en ;
    dcterms:hasVersion history:TGN-003 ;
    dcterms:issued "2000-07-11"^^xsd:date ;
    dcterms:modified "2008-01-14"^^xsd:date ;
    rdfs:comment "The set of places specified by the Getty Thesaurus of Geographic Names."@en ;
    rdfs:isDefinedBy dcterms: ;
    rdfs:seeAlso <http://www.getty.edu/research/tools/vocabulary/tgn/index.html> .

dcterms:UDC a dcam:VocabularyEncodingScheme ;
    rdfs:label "UDC"@en ;
    dcterms:hasVersion history:UDC-003 ;
    dcterms:issued "2000-07-11"^^xsd:date ;
    dcterms:modified "2008-01-14"^^xsd:date ;
    rdfs:comment "The set of conceptual resources specified by the Universal Decimal Classification."@en ;
    rdfs:isDefinedBy dcterms: ;
    rdfs:seeAlso <http://www.udcc.org/> .

dcterms:URI a rdfs:Datatype ;
    rdfs:label "URI"@en ;
    dcterms:hasVersion history:URI-003 ;
    dcterms:issued "2000-07-11"^^xsd:date ;
    dcterms:modified "2008-01-14"^^xsd:date ;
    rdfs:comment "The set of identifiers constructed according to the generic syntax for Uniform Resource Identifiers as specified by the Internet Engineering Task Force."@en ;
    rdfs:isDefinedBy dcterms: ;
    rdfs:seeAlso <http://www.ietf.org/rfc/rfc3986.txt> .

dcterms:W3CDTF a rdfs:Datatype ;
    rdfs:label "W3C-DTF"@en ;
    dcterms:hasVersion history:W3CDTF-003 ;
    dcterms:issued "2000-07-11"^^xsd:date ;
    dcterms:modified "2008-01-14"^^xsd:date ;
    rdfs:comment "The set of dates and times constructed according to the W3C Date and Time Formats Specification."@en ;
    rdfs:isDefinedBy dcterms: ;
    rdfs:seeAlso <http://www.w3.org/TR/NOTE-datetime> .

dcterms:abstract a rdf:Property ;
    rdfs:label "Abstract"@en ;
    dcterms:hasVersion history:abstract-003 ;
    dcterms:issued "2000-07-11"^^xsd:date ;
    dcterms:modified "2008-01-14"^^xsd:date ;
    rdfs:comment "A summary of the resource."@en ;
    rdfs:isDefinedBy dcterms: ;
    rdfs:subPropertyOf dc:description,
        dcterms:description .

dcterms:accessRights a rdf:Property ;
    rdfs:label "Access Rights"@en ;
    dcterms:description "Access Rights may include information regarding access or restrictions based on privacy, security, or other policies."@en ;
    dcterms:hasVersion history:accessRights-002 ;
    dcterms:issued "2003-02-15"^^xsd:date ;
    dcterms:modified "2008-01-14"^^xsd:date ;
    rdfs:comment "Information about who can access the resource or an indication of its security status."@en ;
    rdfs:isDefinedBy dcterms: ;
    rdfs:range dcterms:RightsStatement ;
    rdfs:subPropertyOf dc:rights,
        dcterms:rights .

dcterms:accrualMethod a rdf:Property ;
    rdfs:label "Accrual Method"@en ;
    dcterms:hasVersion history:accrualMethod-003 ;
    dcterms:issued "2005-06-13"^^xsd:date ;
    dcterms:modified "2010-10-11"^^xsd:date ;
    rdfs:comment "The method by which items are added to a collection."@en ;
    rdfs:domain dctypes:Collection ;
    rdfs:isDefinedBy dcterms: ;
    rdfs:range dcterms:MethodOfAccrual .

dcterms:accrualPeriodicity a rdf:Property ;
    rdfs:label "Accrual Periodicity"@en ;
    dcterms:hasVersion history:accrualPeriodicity-003 ;
    dcterms:issued "2005-06-13"^^xsd:date ;
    dcterms:modified "2010-10-11"^^xsd:date ;
    rdfs:comment "The frequency with which items are added to a collection."@en ;
    rdfs:domain dctypes:Collection ;
    rdfs:isDefinedBy dcterms: ;
    rdfs:range dcterms:Frequency .

dcterms:accrualPolicy a rdf:Property ;
    rdfs:label "Accrual Policy"@en ;
    dcterms:hasVersion history:accrualPolicy-003 ;
    dcterms:issued "2005-06-13"^^xsd:date ;
    dcterms:modified "2010-10-11"^^xsd:date ;
    rdfs:comment "The policy governing the addition of items to a collection."@en ;
    rdfs:domain dctypes:Collection ;
    rdfs:isDefinedBy dcterms: ;
    rdfs:range dcterms:Policy .

dcterms:alternative a rdf:Property ;
    rdfs:label "Alternative Title"@en ;
    dcterms:description "The distinction between titles and alternative titles is application-specific."@en ;
    dcterms:hasVersion history:alternative-003 ;
    dcterms:issued "2000-07-11"^^xsd:date ;
    dcterms:modified "2010-10-11"^^xsd:date ;
    rdfs:comment "An alternative name for the resource."@en ;
    rdfs:isDefinedBy dcterms: ;
    rdfs:range rdfs:Literal ;
    rdfs:subPropertyOf dc:title,
        dcterms:title .

dcterms:available a rdf:Property ;
    rdfs:label "Date Available"@en ;
    dcterms:hasVersion history:available-003 ;
    dcterms:issued "2000-07-11"^^xsd:date ;
    dcterms:modified "2008-01-14"^^xsd:date ;
    rdfs:comment "Date (often a range) that the resource became or will become available."@en ;
    rdfs:isDefinedBy dcterms: ;
    rdfs:range rdfs:Literal ;
    rdfs:subPropertyOf dc:date,
        dcterms:date .

dcterms:bibliographicCitation a rdf:Property ;
    rdfs:label "Bibliographic Citation"@en ;
    dcterms:description "Recommended practice is to include sufficient bibliographic detail to identify the resource as unambiguously as possible."@en ;
    dcterms:hasVersion history:bibliographicCitation-002 ;
    dcterms:issued "2003-02-15"^^xsd:date ;
    dcterms:modified "2008-01-14"^^xsd:date ;
    rdfs:comment "A bibliographic reference for the resource."@en ;
    rdfs:domain dcterms:BibliographicResource ;
    rdfs:isDefinedBy dcterms: ;
    rdfs:range rdfs:Literal ;
    rdfs:subPropertyOf dc:identifier,
        dcterms:identifier .

dcterms:conformsTo a rdf:Property ;
    rdfs:label "Conforms To"@en ;
    dcterms:hasVersion history:conformsTo-003 ;
    dcterms:issued "2001-05-21"^^xsd:date ;
    dcterms:modified "2008-01-14"^^xsd:date ;
    rdfs:comment "An established standard to which the described resource conforms."@en ;
    rdfs:isDefinedBy dcterms: ;
    rdfs:range dcterms:Standard ;
    rdfs:subPropertyOf dc:relation,
        dcterms:relation .

dcterms:created a rdf:Property ;
    rdfs:label "Date Created"@en ;
    dcterms:hasVersion history:created-003 ;
    dcterms:issued "2000-07-11"^^xsd:date ;
    dcterms:modified "2008-01-14"^^xsd:date ;
    rdfs:comment "Date of creation of the resource."@en ;
    rdfs:isDefinedBy dcterms: ;
    rdfs:range rdfs:Literal ;
    rdfs:subPropertyOf dc:date,
        dcterms:date .

dcterms:dateAccepted a rdf:Property ;
    rdfs:label "Date Accepted"@en ;
    dcterms:description "Examples of resources to which a Date Accepted may be relevant are a thesis (accepted by a university department) or an article (accepted by a journal)."@en ;
    dcterms:hasVersion history:dateAccepted-002 ;
    dcterms:issued "2002-07-13"^^xsd:date ;
    dcterms:modified "2008-01-14"^^xsd:date ;
    rdfs:comment "Date of acceptance of the resource."@en ;
    rdfs:isDefinedBy dcterms: ;
    rdfs:range rdfs:Literal ;
    rdfs:subPropertyOf dc:date,
        dcterms:date .

dcterms:dateCopyrighted a rdf:Property ;
    rdfs:label "Date Copyrighted"@en ;
    dcterms:hasVersion history:dateCopyrighted-002 ;
    dcterms:issued "2002-07-13"^^xsd:date ;
    dcterms:modified "2008-01-14"^^xsd:date ;
    rdfs:comment "Date of copyright."@en ;
    rdfs:isDefinedBy dcterms: ;
    rdfs:range rdfs:Literal ;
    rdfs:subPropertyOf dc:date,
        dcterms:date .

dcterms:dateSubmitted a rdf:Property ;
    rdfs:label "Date Submitted"@en ;
    dcterms:description "Examples of resources to which a Date Submitted may be relevant are a thesis (submitted to a university department) or an article (submitted to a journal)."@en ;
    dcterms:hasVersion history:dateSubmitted-002 ;
    dcterms:issued "2002-07-13"^^xsd:date ;
    dcterms:modified "2008-01-14"^^xsd:date ;
    rdfs:comment "Date of submission of the resource."@en ;
    rdfs:isDefinedBy dcterms: ;
    rdfs:range rdfs:Literal ;
    rdfs:subPropertyOf dc:date,
        dcterms:date .

dcterms:educationLevel a rdf:Property ;
    rdfs:label "Audience Education Level"@en ;
    dcterms:hasVersion history:educationLevel-002 ;
    dcterms:issued "2002-07-13"^^xsd:date ;
    dcterms:modified "2008-01-14"^^xsd:date ;
    rdfs:comment "A class of entity, defined in terms of progression through an educational or training context, for which the described resource is intended."@en ;
    rdfs:isDefinedBy dcterms: ;
    rdfs:range dcterms:AgentClass ;
    rdfs:subPropertyOf dcterms:audience .

dcterms:extent a rdf:Property ;
    rdfs:label "Extent"@en ;
    dcterms:hasVersion history:extent-003 ;
    dcterms:issued "2000-07-11"^^xsd:date ;
    dcterms:modified "2008-01-14"^^xsd:date ;
    rdfs:comment "The size or duration of the resource."@en ;
    rdfs:isDefinedBy dcterms: ;
    rdfs:range dcterms:SizeOrDuration ;
    rdfs:subPropertyOf dc:format,
        dcterms:format .

dcterms:hasFormat a rdf:Property ;
    rdfs:label "Has Format"@en ;
    dcterms:hasVersion history:hasFormat-003 ;
    dcterms:issued "2000-07-11"^^xsd:date ;
    dcterms:modified "2008-01-14"^^xsd:date ;
    rdfs:comment "A related resource that is substantially the same as the pre-existing described resource, but in another format."@en ;
    rdfs:isDefinedBy dcterms: ;
    rdfs:subPropertyOf dc:relation,
        dcterms:relation ;
    skos:note "This term is intended to be used with non-literal values as defined in the DCMI Abstract Model (http://dublincore.org/documents/abstract-model/).  As of December 2007, the DCMI Usage Board is seeking a way to express this intention with a formal range declaration."@en .

dcterms:hasPart a rdf:Property ;
    rdfs:label "Has Part"@en ;
    dcterms:hasVersion history:hasPart-003 ;
    dcterms:issued "2000-07-11"^^xsd:date ;
    dcterms:modified "2008-01-14"^^xsd:date ;
    rdfs:comment "A related resource that is included either physically or logically in the described resource."@en ;
    rdfs:isDefinedBy dcterms: ;
    rdfs:subPropertyOf dc:relation,
        dcterms:relation ;
    skos:note "This term is intended to be used with non-literal values as defined in the DCMI Abstract Model (http://dublincore.org/documents/abstract-model/).  As of December 2007, the DCMI Usage Board is seeking a way to express this intention with a formal range declaration."@en .

dcterms:hasVersion a rdf:Property ;
    rdfs:label "Has Version"@en ;
    dcterms:hasVersion history:hasVersion-003 ;
    dcterms:issued "2000-07-11"^^xsd:date ;
    dcterms:modified "2008-01-14"^^xsd:date ;
    rdfs:comment "A related resource that is a version, edition, or adaptation of the described resource."@en ;
    rdfs:isDefinedBy dcterms: ;
    rdfs:subPropertyOf dc:relation,
        dcterms:relation ;
    skos:note "This term is intended to be used with non-literal values as defined in the DCMI Abstract Model (http://dublincore.org/documents/abstract-model/).  As of December 2007, the DCMI Usage Board is seeking a way to express this intention with a formal range declaration."@en .

dcterms:instructionalMethod a rdf:Property ;
    rdfs:label "Instructional Method"@en ;
    dcterms:description "Instructional Method will typically include ways of presenting instructional materials or conducting instructional activities, patterns of learner-to-learner and learner-to-instructor interactions, and mechanisms by which group and individual levels of learning are measured.  Instructional methods include all aspects of the instruction and learning processes from planning and implementation through evaluation and feedback."@en ;
    dcterms:hasVersion history:instructionalMethod-002 ;
    dcterms:issued "2005-06-13"^^xsd:date ;
    dcterms:modified "2008-01-14"^^xsd:date ;
    rdfs:comment "A process, used to engender knowledge, attitudes and skills, that the described resource is designed to support."@en ;
    rdfs:isDefinedBy dcterms: ;
    rdfs:range dcterms:MethodOfInstruction .

dcterms:isFormatOf a rdf:Property ;
    rdfs:label "Is Format Of"@en ;
    dcterms:hasVersion history:isFormatOf-003 ;
    dcterms:issued "2000-07-11"^^xsd:date ;
    dcterms:modified "2008-01-14"^^xsd:date ;
    rdfs:comment "A related resource that is substantially the same as the described resource, but in another format."@en ;
    rdfs:isDefinedBy dcterms: ;
    rdfs:subPropertyOf dc:relation,
        dcterms:relation ;
    skos:note "This term is intended to be used with non-literal values as defined in the DCMI Abstract Model (http://dublincore.org/documents/abstract-model/).  As of December 2007, the DCMI Usage Board is seeking a way to express this intention with a formal range declaration."@en .

dcterms:isPartOf a rdf:Property ;
    rdfs:label "Is Part Of"@en ;
    dcterms:hasVersion history:isPartOf-003 ;
    dcterms:issued "2000-07-11"^^xsd:date ;
    dcterms:modified "2008-01-14"^^xsd:date ;
    rdfs:comment "A related resource in which the described resource is physically or logically included."@en ;
    rdfs:isDefinedBy dcterms: ;
    rdfs:subPropertyOf dc:relation,
        dcterms:relation ;
    skos:note "This term is intended to be used with non-literal values as defined in the DCMI Abstract Model (http://dublincore.org/documents/abstract-model/).  As of December 2007, the DCMI Usage Board is seeking a way to express this intention with a formal range declaration."@en .

dcterms:isReferencedBy a rdf:Property ;
    rdfs:label "Is Referenced By"@en ;
    dcterms:hasVersion history:isReferencedBy-003 ;
    dcterms:issued "2000-07-11"^^xsd:date ;
    dcterms:modified "2008-01-14"^^xsd:date ;
    rdfs:comment "A related resource that references, cites, or otherwise points to the described resource."@en ;
    rdfs:isDefinedBy dcterms: ;
    rdfs:subPropertyOf dc:relation,
        dcterms:relation ;
    skos:note "This term is intended to be used with non-literal values as defined in the DCMI Abstract Model (http://dublincore.org/documents/abstract-model/).  As of December 2007, the DCMI Usage Board is seeking a way to express this intention with a formal range declaration."@en .

dcterms:isReplacedBy a rdf:Property ;
    rdfs:label "Is Replaced By"@en ;
    dcterms:hasVersion history:isReplacedBy-003 ;
    dcterms:issued "2000-07-11"^^xsd:date ;
    dcterms:modified "2008-01-14"^^xsd:date ;
    rdfs:comment "A related resource that supplants, displaces, or supersedes the described resource."@en ;
    rdfs:isDefinedBy dcterms: ;
    rdfs:subPropertyOf dc:relation,
        dcterms:relation ;
    skos:note "This term is intended to be used with non-literal values as defined in the DCMI Abstract Model (http://dublincore.org/documents/abstract-model/).  As of December 2007, the DCMI Usage Board is seeking a way to express this intention with a formal range declaration."@en .

dcterms:isRequiredBy a rdf:Property ;
    rdfs:label "Is Required By"@en ;
    dcterms:hasVersion history:isRequiredBy-003 ;
    dcterms:issued "2000-07-11"^^xsd:date ;
    dcterms:modified "2008-01-14"^^xsd:date ;
    rdfs:comment "A related resource that requires the described resource to support its function, delivery, or coherence."@en ;
    rdfs:isDefinedBy dcterms: ;
    rdfs:subPropertyOf dc:relation,
        dcterms:relation ;
    skos:note "This term is intended to be used with non-literal values as defined in the DCMI Abstract Model (http://dublincore.org/documents/abstract-model/).  As of December 2007, the DCMI Usage Board is seeking a way to express this intention with a formal range declaration."@en .

dcterms:isVersionOf a rdf:Property ;
    rdfs:label "Is Version Of"@en ;
    dcterms:description "Changes in version imply substantive changes in content rather than differences in format."@en ;
    dcterms:hasVersion history:isVersionOf-003 ;
    dcterms:issued "2000-07-11"^^xsd:date ;
    dcterms:modified "2008-01-14"^^xsd:date ;
    rdfs:comment "A related resource of which the described resource is a version, edition, or adaptation."@en ;
    rdfs:isDefinedBy dcterms: ;
    rdfs:subPropertyOf dc:relation,
        dcterms:relation ;
    skos:note "This term is intended to be used with non-literal values as defined in the DCMI Abstract Model (http://dublincore.org/documents/abstract-model/).  As of December 2007, the DCMI Usage Board is seeking a way to express this intention with a formal range declaration."@en .

dcterms:issued a rdf:Property ;
    rdfs:label "Date Issued"@en ;
    dcterms:hasVersion history:issued-003 ;
    dcterms:issued "2000-07-11"^^xsd:date ;
    dcterms:modified "2008-01-14"^^xsd:date ;
    rdfs:comment "Date of formal issuance (e.g., publication) of the resource."@en ;
    rdfs:isDefinedBy dcterms: ;
    rdfs:range rdfs:Literal ;
    rdfs:subPropertyOf dc:date,
        dcterms:date .

dcterms:language a rdf:Property ;
    rdfs:label "Language"@en ;
    dcterms:description "Recommended best practice is to use a controlled vocabulary such as RFC 4646 [RFC4646]."@en ;
    dcterms:hasVersion history:languageT-001 ;
    dcterms:issued "2008-01-14"^^xsd:date ;
    dcterms:modified "2008-01-14"^^xsd:date ;
    rdfs:comment "A language of the resource."@en ;
    rdfs:isDefinedBy dcterms: ;
    rdfs:range dcterms:LinguisticSystem ;
    rdfs:subPropertyOf dc:language .

dcterms:license a rdf:Property ;
    rdfs:label "License"@en ;
    dcterms:hasVersion history:license-002 ;
    dcterms:issued "2004-06-14"^^xsd:date ;
    dcterms:modified "2008-01-14"^^xsd:date ;
    rdfs:comment "A legal document giving official permission to do something with the resource."@en ;
    rdfs:isDefinedBy dcterms: ;
    rdfs:range dcterms:LicenseDocument ;
    rdfs:subPropertyOf dc:rights,
        dcterms:rights .

dcterms:mediator a rdf:Property ;
    rdfs:label "Mediator"@en ;
    dcterms:description "In an educational context, a mediator might be a parent, teacher, teaching assistant, or care-giver."@en ;
    dcterms:hasVersion history:mediator-003 ;
    dcterms:issued "2001-05-21"^^xsd:date ;
    dcterms:modified "2008-01-14"^^xsd:date ;
    rdfs:comment "An entity that mediates access to the resource and for whom the resource is intended or useful."@en ;
    rdfs:isDefinedBy dcterms: ;
    rdfs:range dcterms:AgentClass ;
    rdfs:subPropertyOf dcterms:audience .

dcterms:medium a rdf:Property ;
    rdfs:label "Medium"@en ;
    dcterms:hasVersion history:medium-003 ;
    dcterms:issued "2000-07-11"^^xsd:date ;
    dcterms:modified "2008-01-14"^^xsd:date ;
    rdfs:comment "The material or physical carrier of the resource."@en ;
    rdfs:domain dcterms:PhysicalResource ;
    rdfs:isDefinedBy dcterms: ;
    rdfs:range dcterms:PhysicalMedium ;
    rdfs:subPropertyOf dc:format,
        dcterms:format .

dcterms:modified a rdf:Property ;
    rdfs:label "Date Modified"@en ;
    dcterms:hasVersion history:modified-003 ;
    dcterms:issued "2000-07-11"^^xsd:date ;
    dcterms:modified "2008-01-14"^^xsd:date ;
    rdfs:comment "Date on which the resource was changed."@en ;
    rdfs:isDefinedBy dcterms: ;
    rdfs:range rdfs:Literal ;
    rdfs:subPropertyOf dc:date,
        dcterms:date .

dcterms:provenance a rdf:Property ;
    rdfs:label "Provenance"@en ;
    dcterms:description "The statement may include a description of any changes successive custodians made to the resource."@en ;
    dcterms:hasVersion history:provenance-002 ;
    dcterms:issued "2004-09-20"^^xsd:date ;
    dcterms:modified "2008-01-14"^^xsd:date ;
    rdfs:comment "A statement of any changes in ownership and custody of the resource since its creation that are significant for its authenticity, integrity, and interpretation."@en ;
    rdfs:isDefinedBy dcterms: ;
    rdfs:range dcterms:ProvenanceStatement .

dcterms:publisher a rdf:Property ;
    rdfs:label "Publisher"@en ;
    dcterms:description "Examples of a Publisher include a person, an organization, or a service."@en ;
    dcterms:hasVersion history:publisherT-001 ;
    dcterms:issued "2008-01-14"^^xsd:date ;
    dcterms:modified "2010-10-11"^^xsd:date ;
    rdfs:comment "An entity responsible for making the resource available."@en ;
    rdfs:isDefinedBy dcterms: ;
    rdfs:range dcterms:Agent ;
    rdfs:subPropertyOf dc:publisher .

dcterms:references a rdf:Property ;
    rdfs:label "References"@en ;
    dcterms:hasVersion history:references-003 ;
    dcterms:issued "2000-07-11"^^xsd:date ;
    dcterms:modified "2008-01-14"^^xsd:date ;
    rdfs:comment "A related resource that is referenced, cited, or otherwise pointed to by the described resource."@en ;
    rdfs:isDefinedBy dcterms: ;
    rdfs:subPropertyOf dc:relation,
        dcterms:relation ;
    skos:note "This term is intended to be used with non-literal values as defined in the DCMI Abstract Model (http://dublincore.org/documents/abstract-model/).  As of December 2007, the DCMI Usage Board is seeking a way to express this intention with a formal range declaration."@en .

dcterms:replaces a rdf:Property ;
    rdfs:label "Replaces"@en ;
    dcterms:hasVersion history:replaces-003 ;
    dcterms:issued "2000-07-11"^^xsd:date ;
    dcterms:modified "2008-01-14"^^xsd:date ;
    rdfs:comment "A related resource that is supplanted, displaced, or superseded by the described resource."@en ;
    rdfs:isDefinedBy dcterms: ;
    rdfs:subPropertyOf dc:relation,
        dcterms:relation ;
    skos:note "This term is intended to be used with non-literal values as defined in the DCMI Abstract Model (http://dublincore.org/documents/abstract-model/).  As of December 2007, the DCMI Usage Board is seeking a way to express this intention with a formal range declaration."@en .

dcterms:requires a rdf:Property ;
    rdfs:label "Requires"@en ;
    dcterms:hasVersion history:requires-003 ;
    dcterms:issued "2000-07-11"^^xsd:date ;
    dcterms:modified "2008-01-14"^^xsd:date ;
    rdfs:comment "A related resource that is required by the described resource to support its function, delivery, or coherence."@en ;
    rdfs:isDefinedBy dcterms: ;
    rdfs:subPropertyOf dc:relation,
        dcterms:relation ;
    skos:note "This term is intended to be used with non-literal values as defined in the DCMI Abstract Model (http://dublincore.org/documents/abstract-model/).  As of December 2007, the DCMI Usage Board is seeking a way to express this intention with a formal range declaration."@en .

dcterms:rightsHolder a rdf:Property ;
    rdfs:label "Rights Holder"@en ;
    dcterms:hasVersion history:rightsHolder-002 ;
    dcterms:issued "2004-06-14"^^xsd:date ;
    dcterms:modified "2008-01-14"^^xsd:date ;
    rdfs:comment "A person or organization owning or managing rights over the resource."@en ;
    rdfs:isDefinedBy dcterms: ;
    rdfs:range dcterms:Agent .

dcterms:source a rdf:Property ;
    rdfs:label "Source"@en ;
    dcterms:description "The described resource may be derived from the related resource in whole or in part. Recommended best practice is to identify the related resource by means of a string conforming to a formal identification system."@en ;
    dcterms:hasVersion history:sourceT-001 ;
    dcterms:issued "2008-01-14"^^xsd:date ;
    dcterms:modified "2008-01-14"^^xsd:date ;
    rdfs:comment "A related resource from which the described resource is derived."@en ;
    rdfs:isDefinedBy dcterms: ;
    rdfs:subPropertyOf dc:source,
        dcterms:relation ;
    skos:note "This term is intended to be used with non-literal values as defined in the DCMI Abstract Model (http://dublincore.org/documents/abstract-model/).  As of December 2007, the DCMI Usage Board is seeking a way to express this intention with a formal range declaration."@en .

dcterms:spatial a rdf:Property ;
    rdfs:label "Spatial Coverage"@en ;
    dcterms:hasVersion history:spatial-003 ;
    dcterms:issued "2000-07-11"^^xsd:date ;
    dcterms:modified "2008-01-14"^^xsd:date ;
    rdfs:comment "Spatial characteristics of the resource."@en ;
    rdfs:isDefinedBy dcterms: ;
    rdfs:range dcterms:Location ;
    rdfs:subPropertyOf dc:coverage,
        dcterms:coverage .

dcterms:subject a rdf:Property ;
    rdfs:label "Subject"@en ;
    dcterms:description "Typically, the subject will be represented using keywords, key phrases, or classification codes. Recommended best practice is to use a controlled vocabulary."@en ;
    dcterms:hasVersion history:subjectT-002 ;
    dcterms:issued "2008-01-14"^^xsd:date ;
    dcterms:modified "2012-06-14"^^xsd:date ;
    rdfs:comment "The topic of the resource."@en ;
    rdfs:isDefinedBy dcterms: ;
    rdfs:subPropertyOf dc:subject ;
    skos:note "This term is intended to be used with non-literal values as defined in the DCMI Abstract Model (http://dublincore.org/documents/abstract-model/).  As of December 2007, the DCMI Usage Board is seeking a way to express this intention with a formal range declaration."@en .

dcterms:tableOfContents a rdf:Property ;
    rdfs:label "Table Of Contents"@en ;
    dcterms:hasVersion history:tableOfContents-003 ;
    dcterms:issued "2000-07-11"^^xsd:date ;
    dcterms:modified "2008-01-14"^^xsd:date ;
    rdfs:comment "A list of subunits of the resource."@en ;
    rdfs:isDefinedBy dcterms: ;
    rdfs:subPropertyOf dc:description,
        dcterms:description .

dcterms:temporal a rdf:Property ;
    rdfs:label "Temporal Coverage"@en ;
    dcterms:hasVersion history:temporal-003 ;
    dcterms:issued "2000-07-11"^^xsd:date ;
    dcterms:modified "2008-01-14"^^xsd:date ;
    rdfs:comment "Temporal characteristics of the resource."@en ;
    rdfs:isDefinedBy dcterms: ;
    rdfs:range dcterms:PeriodOfTime ;
    rdfs:subPropertyOf dc:coverage,
        dcterms:coverage .

dcterms:valid a rdf:Property ;
    rdfs:label "Date Valid"@en ;
    dcterms:hasVersion history:valid-003 ;
    dcterms:issued "2000-07-11"^^xsd:date ;
    dcterms:modified "2008-01-14"^^xsd:date ;
    rdfs:comment "Date (often a range) of validity of a resource."@en ;
    rdfs:isDefinedBy dcterms: ;
    rdfs:range rdfs:Literal ;
    rdfs:subPropertyOf dc:date,
        dcterms:date .

crm:P100_was_death_of a rdf:Property ;
    rdfs:label "Tod von"@de,
        "ήταν θάνατος του/της"@el,
        "was death of"@en,
        "a été la mort de"@fr,
        "foi a morte para "@pt,
        "был смертью для"@ru ;
    rdfs:comment "This property property links an E69 Death event to the E21 Person that died."@en ;
    rdfs:domain crm:E69_Death ;
    rdfs:range crm:E21_Person ;
    rdfs:subPropertyOf crm:P93_took_out_of_existence .

crm:P100i_died_in a rdf:Property ;
    rdfs:domain crm:E21_Person ;
    rdfs:range crm:E69_Death ;
    rdfs:subPropertyOf crm:P93i_was_taken_out_of_existence_by .

crm:P101_had_as_general_use a rdf:Property ;
    rdfs:label "hatte die allgemeine Verwendung"@de,
        "είχε ως γενική χρήση"@el,
        "had as general use"@en,
        "avait comme utilisation générale"@fr,
        "tem como uso geral"@pt,
        "имел основное применение"@ru ;
    rdfs:comment """This property links an instance of E70 Thing to an E55 Type of usage.
It allows the relationship between particular things, both physical and immaterial, and general methods and techniques of use to be documented. Thus it can be asserted that a baseball bat had a general use for sport and a specific use for threatening people during the Great Train Robbery."""@en ;
    rdfs:domain crm:E70_Thing ;
    rdfs:range crm:E55_Type .

crm:P101i_was_use_of a rdf:Property ;
    rdfs:label "war die Verwendung von"@de,
        "ήταν χρήση του/της"@el,
        "was use of"@en,
        "était l’utilisation de"@fr,
        "foi uso de"@pt,
        "был применением для"@ru ;
    rdfs:domain crm:E55_Type ;
    rdfs:range crm:E70_Thing .

crm:P102_has_title a rdf:Property ;
    rdfs:label "trägt den Titel"@de,
        "έχει τίτλο"@el,
        "has title"@en,
        "a pour titre"@fr,
        "tem título"@pt,
        "имеет заголовок"@ru ;
    rdfs:comment """This property describes the E35 Title applied to an instance of E71 Man-Made Thing. The E55 Type of Title is assigned in a sub property.
The P102.1 has type property of the P102 has title (is title of) property enables the relationship between the Title and the thing to be further clarified, for example, if the Title was a given Title, a supplied Title etc.
It allows any man-made material or immaterial thing to be given a Title. It is possible to imagine a Title being created without a specific object in mind."""@en ;
    rdfs:domain crm:E71_Man-Made_Thing ;
    rdfs:range crm:E35_Title ;
    rdfs:subPropertyOf crm:P1_is_identified_by .

crm:P102i_is_title_of a rdf:Property ;
    rdfs:label "ist der Titel von"@de,
        "είναι τίτλος του/της"@el,
        "is title of"@en,
        "est le titre de"@fr,
        "é título de"@pt,
        "является заголовком для"@ru ;
    rdfs:domain crm:E35_Title ;
    rdfs:range crm:E71_Man-Made_Thing ;
    rdfs:subPropertyOf crm:P1i_identifies .

crm:P103_was_intended_for a rdf:Property ;
    rdfs:label "bestimmt für"@de,
        "προοριζόταν για"@el,
        "was intended for"@en,
        "était destiné à"@fr,
        "era destinado à"@pt,
        "был задуман для"@ru ;
    rdfs:comment """This property links an instance of E71 Man-Made Thing to an E55 Type of usage. 
It creates a property between specific man-made things, both physical and immaterial, to Types of intended methods and techniques of use. Note: A link between specific man-made things and a specific use activity should be expressed using P19 was intended use of (was made for)."""@en ;
    rdfs:domain crm:E71_Man-Made_Thing ;
    rdfs:range crm:E55_Type .

crm:P103i_was_intention_of a rdf:Property ;
    rdfs:label "war Bestimmung von"@de,
        "ήταν προορισμός του"@el,
        "was intention of"@en,
        "était la raison d'être de"@fr,
        "era a destinação de"@pt,
        "был интенцией для"@ru ;
    rdfs:domain crm:E55_Type ;
    rdfs:range crm:E71_Man-Made_Thing .

crm:P104_is_subject_to a rdf:Property ;
    rdfs:label "Gegenstand von"@de,
        "υπόκειται σε"@el,
        "is subject to"@en,
        "est sujet à"@fr,
        "está sujeito à"@pt,
        "является объектом для"@ru ;
    rdfs:comment """This property links a particular E72 Legal Object to the instances of E30 Right to which it is subject.
The Right is held by an E39 Actor as described by P75 possesses (is possessed by)."""@en ;
    rdfs:domain crm:E72_Legal_Object ;
    rdfs:range crm:E30_Right .

crm:P104i_applies_to a rdf:Property ;
    rdfs:label "findet Anwendung auf"@de,
        "ισχύει για"@el,
        "applies to"@en,
        "s’applique à"@fr,
        "se aplicam à"@pt,
        "применяется к"@ru ;
    rdfs:domain crm:E30_Right ;
    rdfs:range crm:E72_Legal_Object .

crm:P106_is_composed_of a rdf:Property ;
    rdfs:label " ist zusammengesetzt aus"@de,
        "αποτελείται από"@el,
        "is composed of"@en,
        "est composé de"@fr,
        "é composto de"@pt,
        "составлен из"@ru ;
    rdfs:comment "This property associates an instance of E90 Symbolic Object with a part of it that is by itself an instance of E90 Symbolic Object, such as fragments of texts or clippings from an image."@en ;
    rdfs:domain crm:E90_Symbolic_Object ;
    rdfs:range crm:E90_Symbolic_Object .

crm:P106i_forms_part_of a rdf:Property ;
    rdfs:label "bildet Teil von"@de,
        "αποτελεί μέρος του/της"@el,
        "forms part of"@en,
        "fait partie de"@fr,
        "faz parte de"@pt,
        "формирует часть"@ru ;
    rdfs:domain crm:E90_Symbolic_Object ;
    rdfs:range crm:E90_Symbolic_Object .

crm:P107_has_current_or_former_member a rdf:Property ;
    rdfs:label "hat derzeitiges oder früheres Mitglied"@de,
        "έχει ή είχε μέλος"@el,
        "has current or former member"@en,
        "a pour membre actuel ou ancien"@fr,
        "tem ou teve membro"@pt,
        "имеет действующего или бывшего члена"@ru ;
    rdfs:comment """This property relates an E39 Actor to the E74 Group of which that E39 Actor is a member.
Groups, Legal Bodies and Persons, may all be members of Groups. A Group necessarily consists of more than one member.
This property is a shortcut of the more fully developed path from E74 Group through P144 joined with (gained member by), E85 Joining, P143 joined (was joined by) to E39 Actor
The property P107.1 kind of member can be used to specify the type of membership or the role the member has in the group. """@en ;
    rdfs:domain crm:E74_Group ;
    rdfs:range crm:E39_Actor .

crm:P107i_is_current_or_former_member_of a rdf:Property ;
    rdfs:label "ist derzeitiges oder früheres Mitglied von"@de,
        "είναι ή ήταν μέλος του/της"@el,
        "is current or former member of"@en,
        "est actuel ou ancien membre de"@fr,
        "é ou foi membro de"@pt,
        "является действующим или бывшим членом"@ru ;
    rdfs:domain crm:E39_Actor ;
    rdfs:range crm:E74_Group .

crm:P108_has_produced a rdf:Property ;
    rdfs:label "hat hergestellt"@de,
        "παρήγαγε"@el,
        "has produced"@en,
        "a produit"@fr,
        "produziu"@pt,
        "произвел"@ru ;
    rdfs:comment """This property identifies the E24 Physical Man-Made Thing that came into existence as a result of an E12 Production.
The identity of an instance of E24 Physical Man-Made Thing is not defined by its matter, but by its existence as a subject of documentation. An E12 Production can result in the creation of multiple instances of E24 Physical Man-Made Thing."""@en ;
    rdfs:domain crm:E12_Production ;
    rdfs:range crm:E24_Physical_Man-Made_Thing ;
    rdfs:subPropertyOf crm:P31_has_modified,
        crm:P92_brought_into_existence .

crm:P108i_was_produced_by a rdf:Property ;
    rdfs:label "wurde hergestellt durch"@de,
        "παρήχθη από"@el,
        "was produced by"@en,
        "a été produit par"@fr,
        "foi produzido por"@pt,
        "был произведен посредством"@ru ;
    rdfs:domain crm:E24_Physical_Man-Made_Thing ;
    rdfs:range crm:E12_Production ;
    rdfs:subPropertyOf crm:P31i_was_modified_by,
        crm:P92i_was_brought_into_existence_by .

crm:P109_has_current_or_former_curator a rdf:Property ;
    rdfs:label "hat derzeitigen oder früheren Kurator"@de,
        "έχει ή είχε επιμελητή"@el,
        "has current or former curator"@en,
        "a pour conservateur actuel ou ancien"@fr,
        "tem ou teve curador"@pt,
        "имеет действующего или бывшего хранителя"@ru ;
    rdfs:comment """This property identifies the E39 Actor or Actors who assume or have assumed overall curatorial responsibility for an E78 Collection.
This property is effectively a short-cut. It does not allow a history of curation to be recorded. This would require use of an Event assigning responsibility for a Collection to a curator."""@en ;
    rdfs:domain crm:E78_Collection ;
    rdfs:range crm:E39_Actor ;
    rdfs:subPropertyOf crm:P49_has_former_or_current_keeper .

crm:P109i_is_current_or_former_curator_of a rdf:Property ;
    rdfs:label "ist derzeitiger oder früherer Kurator von"@de,
        "είναι ή ήταν επιμελητής του/της"@el,
        "is current or former curator of"@en,
        "est ou a été le conservateur de"@fr,
        "é ou foi curador de"@pt,
        "является действующим или бывшим хранителем"@ru ;
    rdfs:domain crm:E39_Actor ;
    rdfs:range crm:E78_Collection ;
    rdfs:subPropertyOf crm:P49i_is_former_or_current_keeper_of .

crm:P10_falls_within a rdf:Property ;
    rdfs:label "fällt in"@de,
        "εμπίπτει"@el,
        "falls within"@en,
        "s’insère dans le cours de"@fr,
        "está contido em"@pt,
        "находится в пределах"@ru ;
    rdfs:comment """This property describes an instance of E4 Period, which falls within the E53 Place and E52 Time-Span of another. 
The difference with P9 consists of (forms part of) is subtle. Unlike P9 consists of (forms part of), P10 falls within (contains) does not imply any logical connection between the two periods and it may refer to a period of a completely different type."""@en ;
    rdfs:domain crm:E4_Period ;
    rdfs:range crm:E4_Period .

crm:P10i_contains a rdf:Property ;
    rdfs:label "enthält"@de,
        "περιλαμβάνει"@el,
        "contains"@en,
        "contient"@fr,
        "contém"@pt,
        "содержит"@ru ;
    rdfs:domain crm:E4_Period ;
    rdfs:range crm:E4_Period .

crm:P110_augmented a rdf:Property ;
    rdfs:label "erweiterte"@de,
        "επαύξησε"@el,
        "augmented"@en,
        "a augmenté"@fr,
        "aumentou"@pt,
        "увеличил"@ru ;
    rdfs:comment """This property identifies the E24 Physical Man-Made Thing that is added to (augmented) in an E79 Part Addition.
Although a Part Addition event normally concerns only one item of Physical Man-Made Thing, it is possible to imagine circumstances under which more than one item might be added to (augmented). For example, the artist Jackson Pollock trailing paint onto multiple canvasses."""@en ;
    rdfs:domain crm:E79_Part_Addition ;
    rdfs:range crm:E24_Physical_Man-Made_Thing ;
    rdfs:subPropertyOf crm:P31_has_modified .

crm:P110i_was_augmented_by a rdf:Property ;
    rdfs:label "wurde erweitert durch"@de,
        "επαυξήθηκε από"@el,
        "was augmented by"@en,
        "a été augmenté par"@fr,
        "foi aumentada por"@pt,
        "был увеличен посредством"@ru ;
    rdfs:domain crm:E24_Physical_Man-Made_Thing ;
    rdfs:range crm:E79_Part_Addition ;
    rdfs:subPropertyOf crm:P31i_was_modified_by .

crm:P111_added a rdf:Property ;
    rdfs:label "fügte hinzu"@de,
        "προσέθεσε"@el,
        "added"@en,
        "a ajouté"@fr,
        "adicionou"@pt,
        "добавил"@ru ;
    rdfs:comment "This property identifies the E18 Physical Thing that is added during an E79 Part Addition activity"@en ;
    rdfs:domain crm:E79_Part_Addition ;
    rdfs:range crm:E18_Physical_Thing ;
    rdfs:subPropertyOf crm:P12_occurred_in_the_presence_of,
        crm:P16_used_specific_object .

crm:P111i_was_added_by a rdf:Property ;
    rdfs:label "wurde hinzugefügt durch"@de,
        "προστέθηκε από"@el,
        "was added by"@en,
        "a été ajouté par"@fr,
        "foi adicionado por"@pt,
        "был добавлен посредством"@ru ;
    rdfs:domain crm:E18_Physical_Thing ;
    rdfs:range crm:E79_Part_Addition ;
    rdfs:subPropertyOf crm:P12i_was_present_at,
        crm:P16i_was_used_for .

crm:P112_diminished a rdf:Property ;
    rdfs:label "verminderte"@de,
        "εξάλειψε"@el,
        "diminished"@en,
        "a diminué"@fr,
        "diminuiu"@pt,
        "уменьшил"@ru ;
    rdfs:comment """This property identifies the E24 Physical Man-Made Thing that was diminished by E80 Part Removal.
Although a Part removal activity normally concerns only one item of Physical Man-Made Thing, it is possible to imagine circumstances under which more than one item might be diminished by a single Part Removal activity. """@en ;
    rdfs:domain crm:E80_Part_Removal ;
    rdfs:range crm:E24_Physical_Man-Made_Thing ;
    rdfs:subPropertyOf crm:P31_has_modified .

crm:P112i_was_diminished_by a rdf:Property ;
    rdfs:label "wurde vermindert durch"@de,
        "εξαλείφθηκε από"@el,
        "was diminished by"@en,
        "a été diminué par"@fr,
        "foi diminuído por"@pt,
        "был уменьшен посредством"@ru ;
    rdfs:domain crm:E24_Physical_Man-Made_Thing ;
    rdfs:range crm:E80_Part_Removal ;
    rdfs:subPropertyOf crm:P31i_was_modified_by .

crm:P113_removed a rdf:Property ;
    rdfs:label "entfernte"@de,
        "αφαίρεσε"@el,
        "removed"@en,
        "a enlevé"@fr,
        "removeu"@pt,
        "удален"@ru ;
    rdfs:comment "This property identifies the E18 Physical Thing that is removed during an E80 Part Removal activity."@en ;
    rdfs:domain crm:E80_Part_Removal ;
    rdfs:range crm:E18_Physical_Thing ;
    rdfs:subPropertyOf crm:P12_occurred_in_the_presence_of .

crm:P113i_was_removed_by a rdf:Property ;
    rdfs:label "wurde entfernt durch"@de,
        "αφαιρέθηκε από"@el,
        "was removed by"@en,
        "a été enlevée par"@fr,
        "foi removido por"@pt,
        "был удален посредством"@ru ;
    rdfs:domain crm:E18_Physical_Thing ;
    rdfs:range crm:E80_Part_Removal ;
    rdfs:subPropertyOf crm:P12i_was_present_at .

crm:P114_is_equal_in_time_to a rdf:Property ;
    rdfs:label "zeitgleich zu"@de,
        "συμπίπτει χρονικά με"@el,
        "is equal in time to"@en,
        "est temporellement égale à"@fr,
        "é temporalmente igual a"@pt,
        "равен по времени"@ru ;
    rdfs:comment """This symmetric property allows the instances of E2 Temporal Entity with the same E52 Time-Span to be equated. 
This property is only necessary if the time span is unknown (otherwise the equivalence can be calculated).
This property is the same as the "equal" relationship of Allen’s temporal logic (Allen, 1983, pp. 832-843)."""@en ;
    rdfs:domain crm:E2_Temporal_Entity ;
    rdfs:range crm:E2_Temporal_Entity .

crm:P115_finishes a rdf:Property ;
    rdfs:label "beendet"@de,
        "περατώνει"@el,
        "finishes"@en,
        "termine"@fr,
        "finaliza"@pt,
        "заканчивает"@ru ;
    rdfs:comment """This property allows the ending point for a E2 Temporal Entity to be situated by reference to the ending point of another temporal entity of longer duration.  
This property is only necessary if the time span is unknown (otherwise the relationship can be calculated). This property is the same as the "finishes / finished-by" relationships of Allen’s temporal logic (Allen, 1983, pp. 832-843)."""@en ;
    rdfs:domain crm:E2_Temporal_Entity ;
    rdfs:range crm:E2_Temporal_Entity .

crm:P115i_is_finished_by a rdf:Property ;
    rdfs:label "wurde beendet mit"@de,
        "περατώνεται με"@el,
        "is finished by"@en,
        "est terminée par"@fr,
        "é finalizada por"@pt,
        "заканчивается"@ru ;
    rdfs:domain crm:E2_Temporal_Entity ;
    rdfs:range crm:E2_Temporal_Entity .

crm:P116_starts a rdf:Property ;
    rdfs:label "beginnt"@de,
        "αρχίζει"@el,
        "starts"@en,
        "commence"@fr,
        "inicia"@pt,
        "начинает"@ru ;
    rdfs:comment """This property allows the starting point for a E2 Temporal Entity to be situated by reference to the starting point of another temporal entity of longer duration.  
This property is only necessary if the time span is unknown (otherwise the relationship can be calculated). This property is the same as the "starts / started-by" relationships of Allen’s temporal logic (Allen, 1983, pp. 832-843)."""@en ;
    rdfs:domain crm:E2_Temporal_Entity ;
    rdfs:range crm:E2_Temporal_Entity .

crm:P116i_is_started_by a rdf:Property ;
    rdfs:label "wurde begonnen mit"@de,
        "αρχίζει με"@el,
        "is started by"@en,
        "est commencée par"@fr,
        "é iniciada por"@pt,
        "начинается"@ru ;
    rdfs:domain crm:E2_Temporal_Entity ;
    rdfs:range crm:E2_Temporal_Entity .

crm:P117_occurs_during a rdf:Property ;
    rdfs:label "fällt in"@de,
        "εμφανίζεται κατά τη διάρκεια"@el,
        "occurs during"@en,
        "a lieu pendant"@fr,
        "ocorre durante"@pt,
        "появляется во течение"@ru ;
    rdfs:comment """This property allows the entire E52 Time-Span of an E2 Temporal Entity to be situated within the Time-Span of another temporal entity that starts before and ends after the included temporal entity.   
This property is only necessary if the time span is unknown (otherwise the relationship can be calculated). This property is the same as the "during / includes" relationships of Allen’s temporal logic (Allen, 1983, pp. 832-843)."""@en ;
    rdfs:domain crm:E2_Temporal_Entity ;
    rdfs:range crm:E2_Temporal_Entity .

crm:P117i_includes a rdf:Property ;
    rdfs:label "beinhaltet"@de,
        "περιλαμβάνει"@el,
        "includes"@en,
        "comporte"@fr,
        "inclui"@pt,
        "включает"@ru ;
    rdfs:domain crm:E2_Temporal_Entity ;
    rdfs:range crm:E2_Temporal_Entity .

crm:P118_overlaps_in_time_with a rdf:Property ;
    rdfs:label "überlappt zeitlich mit"@de,
        "προηγείται μερικώς επικαλύπτοντας"@el,
        "overlaps in time with"@en,
        "est partiellement recouverte dans le temps par"@fr,
        "sobrepõe temporalmente"@pt,
        "перекрывает во времени"@ru ;
    rdfs:comment """This property identifies an overlap between the instances of E52 Time-Span of two instances of E2 Temporal Entity. 
It implies a temporal order between the two entities: if A overlaps in time B, then A must start before B, and B must end after A. This property is only necessary if the relevant time spans are unknown (otherwise the relationship can be calculated).
This property is the same as the "overlaps / overlapped-by" relationships of Allen’s temporal logic (Allen, 1983, pp. 832-843)."""@en ;
    rdfs:domain crm:E2_Temporal_Entity ;
    rdfs:range crm:E2_Temporal_Entity .

crm:P118i_is_overlapped_in_time_by a rdf:Property ;
    rdfs:label "wird zeitlich überlappt von"@de,
        "έπεται μερικώς επικαλυπτόμενο"@el,
        "is overlapped in time by"@en,
        "recouvre partiellement dans le temps"@fr,
        "é sobreposto temporalmente por"@pt,
        "перекрывается во времени"@ru ;
    rdfs:domain crm:E2_Temporal_Entity ;
    rdfs:range crm:E2_Temporal_Entity .

crm:P119_meets_in_time_with a rdf:Property ;
    rdfs:label "trifft zeitlich auf"@de,
        "προηγείται"@el,
        "meets in time with"@en,
        "est temporellement contiguë avec"@fr,
        "é temporalmente contíguo com"@pt,
        "следует во времени за"@ru ;
    rdfs:comment """This property indicates that one E2 Temporal Entity immediately follows another. 
It implies a particular order between the two entities: if A meets in time with B, then A must precede B. This property is only necessary if the relevant time spans are unknown (otherwise the relationship can be calculated). 
This property is the same as the "meets / met-by" relationships of Allen’s temporal logic (Allen, 1983, pp. 832-843)."""@en ;
    rdfs:domain crm:E2_Temporal_Entity ;
    rdfs:range crm:E2_Temporal_Entity .

crm:P119i_is_met_in_time_by a rdf:Property ;
    rdfs:label "wird zeitlich getroffen von"@de,
        "έπεται"@el,
        "is met in time by"@en,
        "est immédiatement précédé par"@fr,
        "é imediatamente precedido por"@pt,
        "предшествует во времени"@ru ;
    rdfs:domain crm:E2_Temporal_Entity ;
    rdfs:range crm:E2_Temporal_Entity .

crm:P120_occurs_before a rdf:Property ;
    rdfs:label "kommt vor"@de,
        "εμφανίζεται πριν"@el,
        "occurs before"@en,
        "a lieu avant"@fr,
        "ocorre antes"@pt,
        "появляется до"@ru ;
    rdfs:comment """This property identifies the relative chronological sequence of two temporal entities. 
It implies that a temporal gap exists between the end of A and the start of B. This property is only necessary if the relevant time spans are unknown (otherwise the relationship can be calculated).
This property is the same as the "before / after" relationships of Allen’s temporal logic (Allen, 1983, pp. 832-843)."""@en ;
    rdfs:domain crm:E2_Temporal_Entity ;
    rdfs:range crm:E2_Temporal_Entity .

crm:P120i_occurs_after a rdf:Property ;
    rdfs:label "kommt nach"@de,
        "εμφανίζεται μετά"@el,
        "occurs after"@en,
        "a lieu après"@fr,
        "ocorre depois"@pt,
        "появляется после"@ru ;
    rdfs:domain crm:E2_Temporal_Entity ;
    rdfs:range crm:E2_Temporal_Entity .

crm:P121_overlaps_with a rdf:Property ;
    rdfs:label "überlappt mit"@de,
        "επικαλύπτεται με"@el,
        "overlaps with"@en,
        "chevauche"@fr,
        "sobrepõe com"@pt,
        "пересекается с"@ru ;
    rdfs:comment """This symmetric property allows the instances of E53 Place with overlapping geometric extents to be associated with each other. 
It does not specify anything about the shared area. This property is purely spatial, in contrast to Allen operators, which are purely temporal."""@en ;
    rdfs:domain crm:E53_Place ;
    rdfs:range crm:E53_Place .

crm:P122_borders_with a rdf:Property ;
    rdfs:label "grenzt an"@de,
        "συνορεύει με"@el,
        "borders with"@en,
        "jouxte"@fr,
        "fronteira com"@pt,
        "граничит с"@ru ;
    rdfs:comment """This symmetric property allows the instances of E53 Place which share common borders to be related as such. 
This property is purely spatial, in contrast to Allen operators, which are purely temporal."""@en ;
    rdfs:domain crm:E53_Place ;
    rdfs:range crm:E53_Place .

crm:P123_resulted_in a rdf:Property ;
    rdfs:label "ergab"@de,
        "είχε ως αποτέλεσμα"@el,
        "resulted in"@en,
        "a eu pour résultat"@fr,
        "resultou em"@pt,
        "повлек появление"@ru ;
    rdfs:comment """This property identifies the E77 Persistent Item or items that are the result of an E81 Transformation. 
New items replace the transformed item or items, which cease to exist as units of documentation. The physical continuity between the old and the new is expressed by the link to the common Transformation."""@en ;
    rdfs:domain crm:E81_Transformation ;
    rdfs:range crm:E77_Persistent_Item ;
    rdfs:subPropertyOf crm:P92_brought_into_existence .

crm:P123i_resulted_from a rdf:Property ;
    rdfs:label "ergab sich aus"@de,
        "προέκυψε από"@el,
        "resulted from"@en,
        "est le résultat de"@fr,
        "resultado de"@pt,
        "был результатом"@ru ;
    rdfs:domain crm:E77_Persistent_Item ;
    rdfs:range crm:E81_Transformation ;
    rdfs:subPropertyOf crm:P92i_was_brought_into_existence_by .

crm:P124_transformed a rdf:Property ;
    rdfs:label "wandelte um"@de,
        "μετέτρεψε"@el,
        "transformed"@en,
        "a transformé"@fr,
        "transformou"@pt,
        "трансформировал"@ru ;
    rdfs:comment """This property identifies the E77 Persistent Item or items that cease to exist due to a E81 Transformation. 
It is replaced by the result of the Transformation, which becomes a new unit of documentation. The continuity between both items, the new and the old, is expressed by the link to the common Transformation."""@en ;
    rdfs:domain crm:E81_Transformation ;
    rdfs:range crm:E77_Persistent_Item ;
    rdfs:subPropertyOf crm:P93_took_out_of_existence .

crm:P124i_was_transformed_by a rdf:Property ;
    rdfs:label "wurde umgewandelt durch"@de,
        "μετατράπηκε από"@el,
        "was transformed by"@en,
        "a été transformé par"@fr,
        "foi transformado por"@pt,
        "был трансформирован посредством"@ru ;
    rdfs:domain crm:E77_Persistent_Item ;
    rdfs:range crm:E81_Transformation ;
    rdfs:subPropertyOf crm:P93i_was_taken_out_of_existence_by .

crm:P126_employed a rdf:Property ;
    rdfs:label "verwendete"@de,
        "χρησιμοποίησε"@el,
        "employed"@en,
        "a employé"@fr,
        "empregou"@pt,
        "использовал"@ru ;
    rdfs:comment """This property identifies E57 Material employed in an E11 Modification.
The E57 Material used during the E11 Modification does not necessarily become incorporated into the E24 Physical Man-Made Thing that forms the subject of the E11 Modification."""@en ;
    rdfs:domain crm:E11_Modification ;
    rdfs:range crm:E57_Material .

crm:P126i_was_employed_in a rdf:Property ;
    rdfs:label "wurde verwendet bei"@de,
        "χρησιμοποιήθηκε σε"@el,
        "was employed in"@en,
        "a été employé dans"@fr,
        "foi empregado em"@pt,
        "использовался в"@ru ;
    rdfs:domain crm:E57_Material ;
    rdfs:range crm:E11_Modification .

crm:P127_has_broader_term a rdf:Property ;
    rdfs:label "hat den Oberbegriff"@de,
        "έχει ευρύτερο όρο"@el,
        "has broader term"@en,
        "a pour terme générique"@fr,
        "tem termo genérico"@pt,
        "имеет вышестоящий термин"@ru ;
    rdfs:comment """This property identifies a super-Type to which an E55 Type is related. 
		It allows Types to be organised into hierarchies. This is the sense of "broader term generic  		(BTG)" as defined in ISO 2788"""@en ;
    rdfs:domain crm:E55_Type ;
    rdfs:range crm:E55_Type .

crm:P127i_has_narrower_term a rdf:Property ;
    rdfs:label "hat den Unterbegriff"@de,
        "έχει στενότερο όρο"@el,
        "has narrower term"@en,
        "a pour terme spécifique"@fr,
        "tem termo específico"@pt ;
    rdfs:domain crm:E55_Type ;
    rdfs:range crm:E55_Type .

crm:P129_is_about a rdf:Property ;
    rdfs:label "handelt über"@de,
        "έχει ως θέμα"@el,
        "is about"@en,
        "est au sujet de"@fr,
        "é sobre"@pt,
        "касается"@ru ;
    rdfs:comment "This property documents that an E89 Propositional Object has as subject an instance of E1 CRM Entity. "@en ;
    rdfs:domain crm:E89_Propositional_Object ;
    rdfs:range crm:E1_CRM_Entity ;
    rdfs:subPropertyOf crm:P67_refers_to .

crm:P129i_is_subject_of a rdf:Property ;
    rdfs:label "wird behandelt in"@de,
        "είναι θέμα  του/της"@el,
        "is subject of"@en,
        "est le sujet de"@fr,
        "é assunto de"@pt,
        "является предметом для"@ru ;
    rdfs:domain crm:E1_CRM_Entity ;
    rdfs:range crm:E89_Propositional_Object ;
    rdfs:subPropertyOf crm:P67i_is_referred_to_by .

crm:P131_is_identified_by a rdf:Property ;
    rdfs:label "wird identifziert durch"@de,
        "αναγνωρίζεται ως"@el,
        "is identified by"@en,
        "est identifié par"@fr,
        "é identificado por"@pt,
        "идентифицируется посредством"@ru ;
    rdfs:comment """This property identifies a name used specifically to identify an E39 Actor. 
This property is a specialisation of P1 is identified by (identifies) is identified by."""@en ;
    rdfs:domain crm:E39_Actor ;
    rdfs:range crm:E82_Actor_Appellation ;
    rdfs:subPropertyOf crm:P1_is_identified_by .

crm:P131i_identifies a rdf:Property ;
    rdfs:label "identifiziert"@de,
        "είναι αναγνωριστικό"@el,
        "identifies"@en,
        "identifie"@fr,
        "identifica"@pt,
        "идентифицирует"@ru ;
    rdfs:domain crm:E82_Actor_Appellation ;
    rdfs:range crm:E39_Actor ;
    rdfs:subPropertyOf crm:P1i_identifies .

crm:P132_overlaps_with a rdf:Property ;
    rdfs:label "überlappt mit"@de,
        "επικαλύπτεται με"@el,
        "overlaps with"@en,
        "chevauche"@fr,
        "sobrepõe"@pt,
        "пересекается с"@ru ;
    rdfs:comment """This symmetric property allows instances of E4 Period that overlap both temporally and spatially to be related, i,e. they share some spatio-temporal extent.
This property does not imply any ordering or sequence between the two periods, either spatial or temporal."""@en ;
    rdfs:domain crm:E4_Period ;
    rdfs:range crm:E4_Period .

crm:P133_is_separated_from a rdf:Property ;
    rdfs:label "getrennt von"@de,
        "διαχωρίζεται από"@el,
        "is separated from"@en,
        "est séparée de"@fr,
        "é separado de"@pt,
        "отделен от"@ru ;
    rdfs:comment """This symmetric property allows instances of E4 Period that do not overlap both temporally and spatially, to be related i,e. they do not share any spatio-temporal extent.
This property does not imply any ordering or sequence between the two periods either spatial or temporal."""@en ;
    rdfs:domain crm:E4_Period ;
    rdfs:range crm:E4_Period .

crm:P134_continued a rdf:Property ;
    rdfs:label "setzte sich fort in"@de,
        "συνέχισε"@el,
        "continued"@en,
        "est la suite de"@fr,
        "continuou"@pt,
        "продолжил"@ru ;
    rdfs:comment """This property allows two activities to be related where the domain is considered as an intentional continuation of the range.
Used multiple times, this allows a chain of related activities to be created which follow each other in sequence."""@en ;
    rdfs:domain crm:E7_Activity ;
    rdfs:range crm:E7_Activity ;
    rdfs:subPropertyOf crm:P15_was_influenced_by .

crm:P134i_was_continued_by a rdf:Property ;
    rdfs:label "wurde fortgesetzt durch"@de,
        "συνεχίστηκε από"@el,
        "was continued by"@en,
        "a été continuée par"@fr,
        "foi continuada por"@pt,
        "был продолжен"@ru ;
    rdfs:domain crm:E7_Activity ;
    rdfs:range crm:E7_Activity ;
    rdfs:subPropertyOf crm:P15i_influenced .

crm:P135_created_type a rdf:Property ;
    rdfs:label "erschuf Typus"@de,
        "δημιούργησε τύπο"@el,
        "created type"@en,
        "a créé le type"@fr,
        "criou tipo"@pt,
        "создал тип"@ru ;
    rdfs:comment "This property identifies the E55 Type, which is created in an E83Type Creation activity."@en ;
    rdfs:domain crm:E83_Type_Creation ;
    rdfs:range crm:E55_Type ;
    rdfs:subPropertyOf crm:P94_has_created .

crm:P135i_was_created_by a rdf:Property ;
    rdfs:label "wurde geschaffen durch"@de,
        "δημιουργήθηκε από"@el,
        "was created by"@en,
        "a été créé par"@fr,
        "foi criado por"@pt,
        "был создан посредством"@ru ;
    rdfs:domain crm:E55_Type ;
    rdfs:range crm:E83_Type_Creation ;
    rdfs:subPropertyOf crm:P94i_was_created_by .

crm:P136_was_based_on a rdf:Property ;
    rdfs:label "stützte sich auf"@de,
        "βασίστηκε σε"@el,
        "was based on"@en,
        "s’est fondée sur"@fr,
        "foi baseado em"@pt,
        "был основан на"@ru ;
    rdfs:comment """This property identifies one or more items that were used as evidence to declare a new E55 Type.
The examination of these items is often the only objective way to understand the precise characteristics of a new Type. Such items should be deposited in a museum or similar institution for that reason. The taxonomic role renders the specific relationship of each item to the Type, such as "holotype" or "original element"."""@en ;
    rdfs:domain crm:E83_Type_Creation ;
    rdfs:range crm:E1_CRM_Entity ;
    rdfs:subPropertyOf crm:P15_was_influenced_by .

crm:P136i_supported_type_creation a rdf:Property ;
    rdfs:label "belegte"@de,
        "υποστήριξε τη δημιουργία τύπου"@el,
        "supported type creation"@en,
        "a justifié la création de type"@fr,
        "suportou a criação de tipo"@pt,
        "поддержал создание типа"@ru ;
    rdfs:domain crm:E1_CRM_Entity ;
    rdfs:range crm:E83_Type_Creation ;
    rdfs:subPropertyOf crm:P15i_influenced .

crm:P137_exemplifies a rdf:Property ;
    rdfs:label "erläutert"@de,
        "δειγματίζει"@el,
        "exemplifies"@en,
        "exemplifie"@fr,
        "é exemplificado por"@pt,
        "поясняет"@ru ;
    rdfs:comment """This property allows an item to be declared as a particular example of an E55 Type or taxon
	The P137.1 in the taxonomic role property of P137 exemplifies (is exemplified by) allows differentiation of taxonomic roles. The taxonomic role renders the specific relationship of this example to the Type, such as "prototypical", "archetypical", "lectotype", etc. The taxonomic role "lectotype" is not associated with the Type Creation (E83) itself, but selected in a later phase."""@en ;
    rdfs:domain crm:E1_CRM_Entity ;
    rdfs:range crm:E55_Type ;
    rdfs:subPropertyOf crm:P2_has_type .

crm:P137i_is_exemplified_by a rdf:Property ;
    rdfs:label "erläutert durch Beispiel"@de,
        "δειγματίζεται από"@el,
        "is exemplified by"@en,
        "est exemplifié par"@fr,
        "exemplifica"@pt,
        "поясняется посредством"@ru ;
    rdfs:domain crm:E55_Type ;
    rdfs:range crm:E1_CRM_Entity ;
    rdfs:subPropertyOf crm:P2i_is_type_of .

crm:P138_represents a rdf:Property ;
    rdfs:label "stellt dar"@de,
        "παριστάνει"@el,
        "represents"@en,
        "représente"@fr,
        "representa"@pt,
        "представляет"@ru ;
    rdfs:comment """This property establishes the relationship between an E36 Visual Item and the entity that it visually represents.
Any entity may be represented visually. This property is part of the fully developed path from E24 Physical Man-Made Thing through P65 shows visual item (is shown by), E36 Visual Item, P138 represents (has representation) to E1 CRM Entity, which is shortcut by P62depicts (is depicted by). P138.1 mode of representation allows the nature of the representation to be refined."""@en ;
    rdfs:domain crm:E36_Visual_Item ;
    rdfs:range crm:E1_CRM_Entity ;
    rdfs:subPropertyOf crm:P67_refers_to .

crm:P138i_has_representation a rdf:Property ;
    rdfs:label "wird dargestellt durch"@de,
        "παριστάνεται από"@el,
        "has representation"@en,
        "est représentée par"@fr,
        "tem representação"@pt,
        "имеет представление"@ru ;
    rdfs:domain crm:E1_CRM_Entity ;
    rdfs:range crm:E36_Visual_Item ;
    rdfs:subPropertyOf crm:P67i_is_referred_to_by .

crm:P139_has_alternative_form a rdf:Property ;
    rdfs:label "hat alternative Form"@de,
        "έχει εναλλακτική μορφή"@el,
        "has alternative form"@en,
        "a pour autre forme"@fr,
        "tem forma alternativa"@pt,
        "имеет альтернативную форму"@ru ;
    rdfs:comment """This property establishes a relationship of equivalence between two instances of E41 Appellation independent from any item identified by them. It is a dynamic asymmetric relationship, where the range expresses the derivative, if such a direction can be established. Otherwise, the relationship is symmetric. The relationship is not transitive.
The equivalence applies to all cases of use of an instance of E41 Appellation. Multiple names assigned to an object, which are not equivalent for all things identified with a specific instance of E41 Appellation, should be modelled as repeated values of P1 is identified by (identifies). 
P139.1 has type allows the type of derivation, such as “transliteration from Latin 1 to ASCII” be refined.."""@en ;
    rdfs:domain crm:E41_Appellation ;
    rdfs:range crm:E41_Appellation .

crm:P13_destroyed a rdf:Property ;
    rdfs:label "zerstörte"@de,
        "κατέστρεψε"@el,
        "destroyed"@en,
        "a détruit"@fr,
        "destruiu"@pt,
        "уничтожил"@ru ;
    rdfs:comment """This property allows specific instances of E18 Physical Thing that have been destroyed to be related to a destruction event. 
Destruction implies the end of an item’s life as a subject of cultural documentation – the physical matter of which the item was composed may in fact continue to exist. A destruction event may be contiguous with a Production that brings into existence a derived object composed partly of matter from the destroyed object."""@en ;
    rdfs:domain crm:E6_Destruction ;
    rdfs:range crm:E18_Physical_Thing ;
    rdfs:subPropertyOf crm:P93_took_out_of_existence .

crm:P13i_was_destroyed_by a rdf:Property ;
    rdfs:label "wurde zerstört durch"@de,
        "καταστράφηκε από"@el,
        "was destroyed by"@en,
        "a été détruite par"@fr,
        "foi destruído por"@pt,
        "был уничтожен посредством"@ru ;
    rdfs:domain crm:E18_Physical_Thing ;
    rdfs:range crm:E6_Destruction ;
    rdfs:subPropertyOf crm:P93i_was_taken_out_of_existence_by .

crm:P142_used_constituent a rdf:Property ;
    rdfs:label "benutzte Bestandteil"@de,
        "used constituent"@en ;
    rdfs:comment "This property associates the event of assigning an instance of E42 Identifier to an entity, with  the instances of E41 Appellation that were used as elements of the identifier."@en ;
    rdfs:domain crm:E15_Identifier_Assignment ;
    rdfs:range crm:E41_Appellation ;
    rdfs:subPropertyOf crm:P16_used_specific_object .

crm:P142i_was_used_in a rdf:Property ;
    rdfs:label "wurde benutzt in"@de,
        "was used in"@en ;
    rdfs:domain crm:E41_Appellation ;
    rdfs:range crm:E15_Identifier_Assignment ;
    rdfs:subPropertyOf crm:P16i_was_used_for .

crm:P143_joined a rdf:Property ;
    rdfs:label "verband"@de,
        "joined"@en ;
    rdfs:comment """This property identifies the instance of E39 Actor that becomes member of a E74 Group in an E85 Joining.
 	Joining events allow for describing people becoming members of a group with a more detailed path from E74 Group through P144 joined with (gained member by), E85 Joining, P143 joined (was joined by) to E39 Actor, compared to the shortcut offered by P107 has current or former member (is current or former member of)."""@en ;
    rdfs:domain crm:E85_Joining ;
    rdfs:range crm:E39_Actor ;
    rdfs:subPropertyOf crm:P11_had_participant .

crm:P143i_was_joined_by a rdf:Property ;
    rdfs:label "wurde verbunden durch"@de,
        "was joined by"@en ;
    rdfs:domain crm:E39_Actor ;
    rdfs:range crm:E85_Joining ;
    rdfs:subPropertyOf crm:P11i_participated_in .

crm:P144_joined_with a rdf:Property ;
    rdfs:label "verband mit"@de,
        "joined with"@en ;
    rdfs:comment """This property identifies the instance of E74 Group of which an instance of E39 Actor becomes a member through an instance of E85 Joining.
Although a Joining activity normally concerns only one instance of E74 Group, it is possible to imagine circumstances under which becoming member of one Group implies becoming member of another Group as well. 
Joining events allow for describing people becoming members of a group with a more detailed path from E74 Group through P144 joined with (gained member by), E85 Joining, P143 joined (was joined by) to E39 Actor, compared to the shortcut offered by P107 has current or former member (is current or former member of).
The property P144.1 kind of member can be used to specify the type of membership or the role the member has in the group. """@en ;
    rdfs:domain crm:E85_Joining ;
    rdfs:range crm:E74_Group ;
    rdfs:subPropertyOf crm:P11_had_participant .

crm:P144i_gained_member_by a rdf:Property ;
    rdfs:label "erwarb Mitglied durch"@de,
        "gained member by"@en ;
    rdfs:domain crm:E74_Group ;
    rdfs:range crm:E85_Joining ;
    rdfs:subPropertyOf crm:P11i_participated_in .

crm:P145_separated a rdf:Property ;
    rdfs:label "entließ"@de,
        "separated"@en ;
    rdfs:comment "This property identifies the instance of E39 Actor that leaves an instance of E74 Group through an instance of E86 Leaving."@en ;
    rdfs:domain crm:E86_Leaving ;
    rdfs:range crm:E39_Actor ;
    rdfs:subPropertyOf crm:P11_had_participant .

crm:P145i_left_by a rdf:Property ;
    rdfs:label "wurde entlassen durch"@de,
        "left by"@en ;
    rdfs:domain crm:E39_Actor ;
    rdfs:range crm:E86_Leaving ;
    rdfs:subPropertyOf crm:P11i_participated_in .

crm:P146_separated_from a rdf:Property ;
    rdfs:label "entließ von"@de,
        "separated from"@en ;
    rdfs:comment """This property identifies the instance of E74 Group an instance of E39 Actor leaves through an instance of E86 Leaving.
Although a Leaving activity normally concerns only one instance of E74 Group, it is possible to imagine circumstances under which leaving one E74 Group implies leaving another E74 Group as well."""@en ;
    rdfs:domain crm:E86_Leaving ;
    rdfs:range crm:E74_Group ;
    rdfs:subPropertyOf crm:P11_had_participant .

crm:P146i_lost_member_by a rdf:Property ;
    rdfs:label "verlor Mitglied durch"@de,
        "lost member by"@en ;
    rdfs:domain crm:E74_Group ;
    rdfs:range crm:E86_Leaving ;
    rdfs:subPropertyOf crm:P11i_participated_in .

crm:P147_curated a rdf:Property ;
    rdfs:label "betreute kuratorisch"@de,
        "curated"@en ;
    rdfs:comment "This property associates an instance of E78 Collection or collections with  subject of a curation activity following some implicit or explicit curation plan."@en ;
    rdfs:domain crm:E87_Curation_Activity ;
    rdfs:range crm:E78_Collection .

crm:P147i_was_curated_by a rdf:Property ;
    rdfs:label "wurde kuratorisch betreut durch"@de,
        "was curated by"@en ;
    rdfs:domain crm:E78_Collection ;
    rdfs:range crm:E87_Curation_Activity .

crm:P148_has_component a rdf:Property ;
    rdfs:label "hat Bestandteil"@de,
        "has component"@en ;
    rdfs:comment "This property associates an instance of E89 Propositional Object with a structural part of it that is by itself an instance of E89 Propositional Object."@en ;
    rdfs:domain crm:E89_Propositional_Object ;
    rdfs:range crm:E89_Propositional_Object .

crm:P148i_is_component_of a rdf:Property ;
    rdfs:label "ist Bestandteil von"@de,
        "is component of"@en ;
    rdfs:domain crm:E89_Propositional_Object ;
    rdfs:range crm:E89_Propositional_Object .

crm:P149_is_identified_by a rdf:Property ;
    rdfs:label "is identified by"@en ;
    rdfs:comment "This property identifies an instance of E28 Conceptual Object using an instance of E75 Conceptual Object Appellation."@en ;
    rdfs:domain crm:E28_Conceptual_Object ;
    rdfs:range crm:E75_Conceptual_Object_Appellation ;
    rdfs:subPropertyOf crm:P1_is_identified_by .

crm:P149i_identifies a rdf:Property ;
    rdfs:label "identifies"@en ;
    rdfs:domain crm:E75_Conceptual_Object_Appellation ;
    rdfs:range crm:E28_Conceptual_Object ;
    rdfs:subPropertyOf crm:P1i_identifies .

crm:P17_was_motivated_by a rdf:Property ;
    rdfs:label "wurde angeregt durch"@de,
        "είχε ως αφορμή"@el,
        "was motivated by"@en,
        "a été motivée par"@fr,
        "foi motivado por"@pt,
        "был обусловлен посредством"@ru ;
    rdfs:comment """This property describes an item or items that are regarded as a reason for carrying out the E7 Activity. 
For example, the discovery of a large hoard of treasure may call for a celebration, an order from head quarters can start a military manoeuvre. """@en ;
    rdfs:domain crm:E7_Activity ;
    rdfs:range crm:E1_CRM_Entity ;
    rdfs:subPropertyOf crm:P15_was_influenced_by .

crm:P17i_motivated a rdf:Property ;
    rdfs:label "regte an"@de,
        "ήταν αφορμή"@el,
        "motivated"@en,
        "a motivé"@fr,
        "motivou"@pt,
        "обусловил"@ru ;
    rdfs:domain crm:E1_CRM_Entity ;
    rdfs:range crm:E7_Activity ;
    rdfs:subPropertyOf crm:P15i_influenced .

crm:P19_was_intended_use_of a rdf:Property ;
    rdfs:label "war beabsichtigteter Gebrauch von "@de,
        "ήταν προορισμένη χρήση του"@el,
        "was intended use of"@en,
        "était l'utilisation prévue de"@fr,
        "era prevista a utilização de"@pt,
        "был предполагаемым использованием для"@ru ;
    rdfs:comment """This property relates an E7 Activity with objects created specifically for use in the activity. 
This is distinct from the intended use of an item in some general type of activity such as the book of common prayer which was intended for use in Church of England services (see P101 had as general use (was use of))."""@en ;
    rdfs:domain crm:E7_Activity ;
    rdfs:range crm:E71_Man-Made_Thing .

crm:P19i_was_made_for a rdf:Property ;
    rdfs:label "wurde hergestellt für"@de,
        "έγινε για"@el,
        "was made for"@en,
        "a été fabriquée pour"@fr,
        "foi feito para"@pt,
        "был создан для"@ru ;
    rdfs:domain crm:E71_Man-Made_Thing ;
    rdfs:range crm:E7_Activity .

crm:P20_had_specific_purpose a rdf:Property ;
    rdfs:label "hatte den bestimmten Zweck"@de,
        "είχε συγκεκριμένο σκοπό"@el,
        "had specific purpose"@en,
        "avait pour but spécifique"@fr,
        "tinha propósito específico"@pt,
        "имел конкретную цель"@ru ;
    rdfs:comment """This property identifies the relationship between a preparatory activity and the event it is intended to be preparation for.
This includes activities, orders and other organisational actions, taken in preparation for other activities or events. 
P20 had specific purpose (was purpose of) implies that an activity succeeded in achieving its aim. If it does not succeed, such as the setting of a trap that did not catch anything, one may document the unrealized intention using P21 had general purpose (was purpose of):E55 Type and/or  P33 used specific technique (was used by): E29 Design or Procedure."""@en ;
    rdfs:domain crm:E7_Activity ;
    rdfs:range crm:E5_Event .

crm:P20i_was_purpose_of a rdf:Property ;
    rdfs:label "war Zweck von"@de,
        "ήταν σκοπός του/της"@el,
        "was purpose of"@en,
        "était le but de"@fr,
        "era o propósito de"@pt,
        "был целью для"@ru ;
    rdfs:domain crm:E5_Event ;
    rdfs:range crm:E7_Activity .

crm:P21_had_general_purpose a rdf:Property ;
    rdfs:label "hatte den allgemeinen Zweck"@de,
        "είχε γενικό σκοπό"@el,
        "had general purpose"@en,
        "avait pour but général"@fr,
        "tinha propósito geral"@pt,
        "имел общую цель"@ru ;
    rdfs:comment """This property describes an intentional relationship between an E7 Activity and some general goal or purpose. 
This may involve activities intended as preparation for some type of activity or event. P21had general purpose (was purpose of) differs from P20 had specific purpose (was purpose of) in that no occurrence of an event is implied as the purpose. """@en ;
    rdfs:domain crm:E7_Activity ;
    rdfs:range crm:E55_Type .

crm:P21i_was_purpose_of a rdf:Property ;
    rdfs:label "war Zweck von"@de,
        "ήταν σκοπός του/της"@el,
        "was purpose of"@en,
        "était le but de"@fr,
        "era o propósito de"@pt,
        "был целью для"@ru ;
    rdfs:domain crm:E55_Type ;
    rdfs:range crm:E7_Activity .

crm:P22_transferred_title_to a rdf:Property ;
    rdfs:label "übertrug Besitztitel auf"@de,
        "μετεβίβασε τον τίτλο σε"@el,
        "transferred title to"@en,
        "a fait passer le droit de propriété à"@fr,
        "transferiu os direitos de propriedade para"@pt,
        "передал право собственности"@ru ;
    rdfs:comment """This property identifies the E39 Actor that acquires the legal ownership of an object as a result of an E8 Acquisition. 
The property will typically describe an Actor purchasing or otherwise acquiring an object from another Actor. However, title may also be acquired, without any corresponding loss of title by another Actor, through legal fieldwork such as hunting, shooting or fishing.
In reality the title is either transferred to or from someone, or both."""@en ;
    rdfs:domain crm:E8_Acquisition ;
    rdfs:range crm:E39_Actor ;
    rdfs:subPropertyOf crm:P14_carried_out_by .

crm:P22i_acquired_title_through a rdf:Property ;
    rdfs:label "erwarb Besitztitel durch"@de,
        "απέκτησε τον τίτλο μέσω"@el,
        "acquired title through"@en,
        "a acquis le droit de propriété du fait de"@fr,
        "adquiriu os direitos de propriedade por meio da"@pt,
        "получил право собственности через"@ru ;
    rdfs:domain crm:E39_Actor ;
    rdfs:range crm:E8_Acquisition ;
    rdfs:subPropertyOf crm:P14i_performed .

crm:P23_transferred_title_from a rdf:Property ;
    rdfs:label "übertrug Besitztitel von"@de,
        "μετεβίβασε τον τίτλο από"@el,
        "transferred title from"@en,
        "a fait passer le droit de propriété de"@fr,
        "transferiu os direitos de propriedade de"@pt,
        "передал право собственности от"@ru ;
    rdfs:comment """This property identifies the E39 Actor or Actors who relinquish legal ownership as the result of an E8 Acquisition.
The property will typically be used to describe a person donating or selling an object to a museum. In reality title is either transferred to or from someone, or both."""@en ;
    rdfs:domain crm:E8_Acquisition ;
    rdfs:range crm:E39_Actor ;
    rdfs:subPropertyOf crm:P14_carried_out_by .

crm:P23i_surrendered_title_through a rdf:Property ;
    rdfs:label "trat Besitztitel ab in"@de,
        "παρέδωσε τον τίτλο μέσω"@el,
        "surrendered title through"@en,
        "a perdu le droit de propriété du fait de"@fr,
        "perdeu os direitos de propriedade por meio da"@pt,
        "право собственности отдано через"@ru ;
    rdfs:domain crm:E39_Actor ;
    rdfs:range crm:E8_Acquisition ;
    rdfs:subPropertyOf crm:P14i_performed .

crm:P24_transferred_title_of a rdf:Property ;
    rdfs:label "übertrug Besitz über"@de,
        "μετεβίβασε τον τίτλο του/της"@el,
        "transferred title of"@en,
        "a fait passer le droit de propriété sur"@fr,
        "transferiu os direitos de propriedade sobre o"@pt,
        "передал право собственности на"@ru ;
    rdfs:comment """This property identifies the E18 Physical Thing or things involved in an E8 Acquisition. 
In reality, an acquisition must refer to at least one transferred item."""@en ;
    rdfs:domain crm:E8_Acquisition ;
    rdfs:range crm:E18_Physical_Thing .

crm:P24i_changed_ownership_through a rdf:Property ;
    rdfs:label "ging über in Besitz durch"@de,
        "άλλαξε ιδιοκτησία μέσω"@el,
        "changed ownership through"@en,
        "a changé de mains du fait de"@fr,
        "mudou de proprietário por meio de"@pt,
        "сменил владельца через"@ru ;
    rdfs:domain crm:E18_Physical_Thing ;
    rdfs:range crm:E8_Acquisition .

crm:P25_moved a rdf:Property ;
    rdfs:label "bewegte"@de,
        "μετεκίνησε"@el,
        "moved"@en,
        "a déplacé"@fr,
        "locomoveu"@pt,
        "переместил"@ru ;
    rdfs:comment """This property identifies the E19 Physical Object that is moved during a move event. 
The property implies the object’s passive participation. For example, Monet’s painting “Impression sunrise” was moved for the first Impressionist exhibition in 1874. 
In reality, a move must concern at least one object."""@en ;
    rdfs:domain crm:E9_Move ;
    rdfs:range crm:E19_Physical_Object ;
    rdfs:subPropertyOf crm:P12_occurred_in_the_presence_of .

crm:P25i_moved_by a rdf:Property ;
    rdfs:label "wurde bewegt durch"@de,
        "μετακινήθηκε από"@el,
        "moved by"@en,
        "a été déplacé par"@fr,
        "foi locomovido por"@pt,
        "перемещен посредством"@ru ;
    rdfs:domain crm:E19_Physical_Object ;
    rdfs:range crm:E9_Move ;
    rdfs:subPropertyOf crm:P12i_was_present_at .

crm:P26_moved_to a rdf:Property ;
    rdfs:label "bewegte bis zu"@de,
        "μετακινήθηκε προς"@el,
        "moved to"@en,
        "a déplacé vers"@fr,
        "locomoveu para"@pt,
        "перемещен в"@ru ;
    rdfs:comment """This property identifies the destination of a E9 Move. 
A move will be linked to a destination, such as the move of an artefact from storage to display. A move may be linked to many terminal instances of E53 Places. In this case the move describes a distribution of a set of objects. The area of the move includes the origin, route and destination."""@en ;
    rdfs:domain crm:E9_Move ;
    rdfs:range crm:E53_Place ;
    rdfs:subPropertyOf crm:P7_took_place_at .

crm:P26i_was_destination_of a rdf:Property ;
    rdfs:label "war Zielort von"@de,
        "ήταν προορισμός του/της"@el,
        "was destination of"@en,
        "a été la destination de"@fr,
        "era destinação de"@pt,
        "был пунктом назначения для"@ru ;
    rdfs:domain crm:E53_Place ;
    rdfs:range crm:E9_Move ;
    rdfs:subPropertyOf crm:P7i_witnessed .

crm:P27_moved_from a rdf:Property ;
    rdfs:label "bewegte weg von"@de,
        "μετακινήθηκε από"@el,
        "moved from"@en,
        "a retiré de"@fr,
        "locomoveu de"@pt,
        "перемещен из"@ru ;
    rdfs:comment """This property identifies the starting E53 Place of an E9 Move.
A move will be linked to an origin, such as the move of an artefact from storage to display. A move may be linked to many origins. In this case the move describes the picking up of a set of objects. The area of the move includes the origin, route and destination."""@en ;
    rdfs:domain crm:E9_Move ;
    rdfs:range crm:E53_Place ;
    rdfs:subPropertyOf crm:P7_took_place_at .

crm:P27i_was_origin_of a rdf:Property ;
    rdfs:label "war Ausgangsort von"@de,
        "ήταν αφετηρία του/της"@el,
        "was origin of"@en,
        "a été l'origine de"@fr,
        "era origem de"@pt,
        "был исходной точкой для"@ru ;
    rdfs:domain crm:E53_Place ;
    rdfs:range crm:E9_Move ;
    rdfs:subPropertyOf crm:P7i_witnessed .

crm:P28_custody_surrendered_by a rdf:Property ;
    rdfs:label "übergab Gewahrsam an"@de,
        "μετεβίβασε κατοχή από"@el,
        "custody surrendered by"@en,
        "changement de détenteur au détriment de"@fr,
        "custódia concedida por"@pt,
        "опека отдана"@ru ;
    rdfs:comment """This property identifies the E39 Actor or Actors who surrender custody of an instance of E18 Physical Thing in an E10 Transfer of Custody activity. 
The property will typically describe an Actor surrendering custody of an object when it is handed over to someone else’s care. On occasion, physical custody may be surrendered involuntarily – through accident, loss or theft.
In reality, custody is either transferred to someone or from someone, or both."""@en ;
    rdfs:domain crm:E10_Transfer_of_Custody ;
    rdfs:range crm:E39_Actor ;
    rdfs:subPropertyOf crm:P14_carried_out_by .

crm:P28i_surrendered_custody_through a rdf:Property ;
    rdfs:label "wurde Gewahrsam übergeben durch"@de,
        "παρέδωσε κατοχή μέσω"@el,
        "surrendered custody through"@en,
        "a cessé d’être détenteur à cause de"@fr,
        "final da custódia por meio de"@pt,
        "опека отдана через"@ru ;
    rdfs:domain crm:E39_Actor ;
    rdfs:range crm:E10_Transfer_of_Custody ;
    rdfs:subPropertyOf crm:P14i_performed .

crm:P29_custody_received_by a rdf:Property ;
    rdfs:label "übertrug Gewahrsam auf"@de,
        "μετεβίβασε κατοχή σε"@el,
        "custody received by"@en,
        "changement de détenteur au profit de"@fr,
        "custódia recebida por"@pt,
        "опека получена"@ru ;
    rdfs:comment """This property identifies the E39 Actor or Actors who receive custody of an instance of E18 Physical Thing in an E10 Transfer of Custody activity. 
The property will typically describe Actors receiving custody of an object when it is handed over from another Actor’s care. On occasion, physical custody may be received involuntarily or illegally – through accident, unsolicited donation, or theft.
In reality, custody is either transferred to someone or from someone, or both."""@en ;
    rdfs:domain crm:E10_Transfer_of_Custody ;
    rdfs:range crm:E39_Actor ;
    rdfs:subPropertyOf crm:P14_carried_out_by .

crm:P29i_received_custody_through a rdf:Property ;
    rdfs:label "erhielt Gewahrsam durch"@de,
        "παρέλαβε κατοχή μέσω"@el,
        "received custody through"@en,
        "est devenu détenteur grâce à"@fr,
        "início da custódia por meio de"@pt,
        "получил опеку через"@ru ;
    rdfs:domain crm:E39_Actor ;
    rdfs:range crm:E10_Transfer_of_Custody ;
    rdfs:subPropertyOf crm:P14i_performed .

crm:P30_transferred_custody_of a rdf:Property ;
    rdfs:label "übertrug Gewahrsam über"@de,
        "μετεβίβασε κατοχή του/της/των"@el,
        "transferred custody of"@en,
        "changement de détenteur concernant"@fr,
        "transferida custódia de"@pt,
        "передало опеку на"@ru ;
    rdfs:comment """This property identifies an item or items of E18 Physical Thing concerned in an E10 Transfer of Custody activity. 
The property will typically describe the object that is handed over by an E39 Actor to another Actor’s custody. On occasion, physical custody may be transferred involuntarily or illegally – through accident, unsolicited donation, or theft."""@en ;
    rdfs:domain crm:E10_Transfer_of_Custody ;
    rdfs:range crm:E18_Physical_Thing .

crm:P30i_custody_transferred_through a rdf:Property ;
    rdfs:label "wechselte Gewahrsam durch"@de,
        "άλλαξε κατοχή μέσω"@el,
        "custody transferred through"@en,
        "a changé de détenteur du fait de"@fr,
        "custódia transferida por meio de"@pt,
        "опека передана через"@ru ;
    rdfs:domain crm:E18_Physical_Thing ;
    rdfs:range crm:E10_Transfer_of_Custody .

crm:P32_used_general_technique a rdf:Property ;
    rdfs:label "benutzte das allgemeine Verfahren"@de,
        "χρησιμοποίησε γενική τεχνική"@el,
        "used general technique"@en,
        "a employé comme technique générique"@fr,
        "usou técnica geral"@pt,
        "использовал общую технику"@ru ;
    rdfs:comment """This property identifies the technique that was employed in an act of modification. 
These techniques should be drawn from an external E55 Type hierarchy of consistent terminology of general techniques such as embroidery, oil-painting, etc. Specific techniques may be further described as instances of E29 Design or Procedure."""@en ;
    rdfs:domain crm:E7_Activity ;
    rdfs:range crm:E55_Type ;
    rdfs:subPropertyOf crm:P125_used_object_of_type .

crm:P32i_was_technique_of a rdf:Property ;
    rdfs:label "war Verfahren von"@de,
        "ήταν τεχνική του/της"@el,
        "was technique of"@en,
        "a été la technique mise en œuvre dans"@fr,
        "foi técnica da"@pt,
        "был техникой для"@ru ;
    rdfs:domain crm:E55_Type ;
    rdfs:range crm:E7_Activity ;
    rdfs:subPropertyOf crm:P125i_was_type_of_object_used_in .

crm:P33_used_specific_technique a rdf:Property ;
    rdfs:label "benutzte das bestimmte Verfahren"@de,
        "χρησιμοποίησε συγκεκριμένη τεχνική"@el,
        "used specific technique"@en,
        "a employé comme technique spécifique"@fr,
        "usou técnica específica"@pt,
        "использовал особую технику"@ru ;
    rdfs:comment """This property identifies a specific instance of E29 Design or Procedure in order to carry out an instance of E7 Activity or parts of it. 
The property differs from P32 used general technique (was technique of) in that P33 refers to an instance of E29 Design or Procedure, which is a concrete information object in its own right rather than simply being a term or a method known by tradition. 
Typical examples would include intervention plans for conservation or the construction plans of a building."""@en ;
    rdfs:domain crm:E7_Activity ;
    rdfs:range crm:E29_Design_or_Procedure ;
    rdfs:subPropertyOf crm:P16_used_specific_object .

crm:P33i_was_used_by a rdf:Property ;
    rdfs:label "wurde benutzt von"@de,
        "χρησιμοποιήθηκε για"@el,
        "was used by"@en,
        "a été employée par"@fr,
        "foi usada por"@pt,
        "был использован посредством"@ru ;
    rdfs:domain crm:E29_Design_or_Procedure ;
    rdfs:range crm:E7_Activity ;
    rdfs:subPropertyOf crm:P16i_was_used_for .

crm:P34_concerned a rdf:Property ;
    rdfs:label "betraf"@de,
        "αφορούσε σε"@el,
        "concerned"@en,
        "a concerné"@fr,
        "interessada"@pt,
        "имел дело с"@ru ;
    rdfs:comment """This property identifies the E18 Physical Thing that was assessed during an E14 Condition Assessment activity. 
Conditions may be assessed either by direct observation or using recorded evidence. In the latter case the E18 Physical Thing does not need to be present or extant."""@en ;
    rdfs:domain crm:E14_Condition_Assessment ;
    rdfs:range crm:E18_Physical_Thing ;
    rdfs:subPropertyOf crm:P140_assigned_attribute_to .

crm:P34i_was_assessed_by a rdf:Property ;
    rdfs:label "wurde beurteilt durch"@de,
        "εκτιμήθηκε από"@el,
        "was assessed by"@en,
        "expertisé par le biais de"@fr,
        "foi avaliada por"@pt,
        "был оценен посредством"@ru ;
    rdfs:domain crm:E18_Physical_Thing ;
    rdfs:range crm:E14_Condition_Assessment ;
    rdfs:subPropertyOf crm:P140i_was_attributed_by .

crm:P35_has_identified a rdf:Property ;
    rdfs:label "hat identifiziert"@de,
        "έχει διαπιστώσει"@el,
        "has identified"@en,
        "a identifié"@fr,
        "identificou"@pt,
        "идентифицировал"@ru ;
    rdfs:comment "This property identifies the E3 Condition State that was observed in an E14 Condition Assessment activity."@en ;
    rdfs:domain crm:E14_Condition_Assessment ;
    rdfs:range crm:E3_Condition_State ;
    rdfs:subPropertyOf crm:P141_assigned .

crm:P35i_was_identified_by a rdf:Property ;
    rdfs:label "wurde identifiziert durch"@de,
        "έχει διαπιστωθεί από"@el,
        "was identified by"@en,
        "est identifié par"@fr,
        "foi identificado por"@pt,
        "идентифицирован посредством"@ru ;
    rdfs:domain crm:E3_Condition_State ;
    rdfs:range crm:E14_Condition_Assessment ;
    rdfs:subPropertyOf crm:P141i_was_assigned_by .

crm:P37_assigned a rdf:Property ;
    rdfs:label "wies zu"@de,
        "απέδωσε"@el,
        "assigned"@en,
        "a attribué"@fr,
        "atribuiu"@pt,
        "назначил"@ru ;
    rdfs:comment """This property records the identifier that was assigned to an item in an Identifier Assignment activity.
The same identifier may be assigned on more than one occasion.
An Identifier might be created prior to an assignment."""@en ;
    rdfs:domain crm:E15_Identifier_Assignment ;
    rdfs:range crm:E42_Identifier ;
    rdfs:subPropertyOf crm:P141_assigned .

crm:P37i_was_assigned_by a rdf:Property ;
    rdfs:label "wurde zugewiesen durch"@de,
        "αποδόθηκε ως ιδιότητα από"@el,
        "was assigned by"@en,
        "a été attribuée par"@fr,
        "foi atribuído por"@pt,
        "был присвоен посредством"@ru ;
    rdfs:domain crm:E42_Identifier ;
    rdfs:range crm:E15_Identifier_Assignment ;
    rdfs:subPropertyOf crm:P141i_was_assigned_by .

crm:P38_deassigned a rdf:Property ;
    rdfs:label " hob Zuweisung auf von"@de,
        "ακύρωσε"@el,
        "deassigned"@en,
        "a désattribué"@fr,
        "retirou a atribuição do"@pt,
        "отменил назначение"@ru ;
    rdfs:comment """This property records the identifier that was deassigned from an instance of E1 CRM Entity.
Deassignment of an identifier may be necessary when an item is taken out of an inventory, a new numbering system is introduced or items are merged or split up. 
The same identifier may be deassigned on more than one occasion."""@en ;
    rdfs:domain crm:E15_Identifier_Assignment ;
    rdfs:range crm:E42_Identifier ;
    rdfs:subPropertyOf crm:P141_assigned .

crm:P38i_was_deassigned_by a rdf:Property ;
    rdfs:label "wurde aufgehoben durch"@de,
        "ακυρώθηκε από"@el,
        "was deassigned by"@en,
        "a été désattribué par"@fr,
        "foi retirada a atribuição por"@pt,
        "был отменен посредством"@ru ;
    rdfs:domain crm:E42_Identifier ;
    rdfs:range crm:E15_Identifier_Assignment ;
    rdfs:subPropertyOf crm:P141i_was_assigned_by .

crm:P39_measured a rdf:Property ;
    rdfs:label "vermaß"@de,
        "μέτρησε"@el,
        "measured"@en,
        "a mesuré"@fr,
        "mediu"@pt,
        "измерил"@ru ;
    rdfs:comment "This property associates an instance of E16 Measurement with the instance of E1 CRM Entity to which it applied. An instance of E1 CRM Entity may be measured more than once. Material and immaterial things and processes may be measured, e.g. the number of words in a text, or the duration of an event."@en ;
    rdfs:domain crm:E16_Measurement ;
    rdfs:range crm:E1_CRM_Entity ;
    rdfs:subPropertyOf crm:P140_assigned_attribute_to .

crm:P39i_was_measured_by a rdf:Property ;
    rdfs:label "wurde vermessen durch"@de,
        "μετρήθηκε από"@el,
        "was measured by"@en,
        "a été mesuré par"@fr,
        "foi medida por"@pt,
        "был измерен посредством"@ru ;
    rdfs:domain crm:E1_CRM_Entity ;
    rdfs:range crm:E16_Measurement ;
    rdfs:subPropertyOf crm:P140i_was_attributed_by .

crm:P40_observed_dimension a rdf:Property ;
    rdfs:label "beobachtete Dimension"@de,
        "παρατήρησε"@el,
        "observed dimension"@en,
        "a relevé comme dimension"@fr,
        "verificou a dimensão"@pt,
        "определил величину"@ru ;
    rdfs:comment """This property records the dimension that was observed in an E16 Measurement Event.
E54 Dimension can be any quantifiable aspect of E70 Thing. Weight, image colour depth and monetary value are dimensions in this sense. One measurement activity may determine more than one dimension of one object.
Dimensions may be determined either by direct observation or using recorded evidence. In the latter case the measured Thing does not need to be present or extant.
Even though knowledge of the value of a dimension requires measurement, the dimension may be an object of discourse prior to, or even without, any measurement being made."""@en ;
    rdfs:domain crm:E16_Measurement ;
    rdfs:range crm:E54_Dimension ;
    rdfs:subPropertyOf crm:P141_assigned .

crm:P40i_was_observed_in a rdf:Property ;
    rdfs:label "wurde beobachtet in"@de,
        "παρατηρήθηκε από"@el,
        "was observed in"@en,
        "a été relevée au cours de"@fr,
        "foi verificada durante"@pt,
        "наблюдался в"@ru ;
    rdfs:domain crm:E54_Dimension ;
    rdfs:range crm:E16_Measurement ;
    rdfs:subPropertyOf crm:P141i_was_assigned_by .

crm:P41_classified a rdf:Property ;
    rdfs:label "klassifizierte"@de,
        "χαρακτήρισε"@el,
        "classified"@en,
        "a classifié"@fr,
        "classificou"@pt,
        "классифицировал"@ru ;
    rdfs:comment """This property records the item to which a type was assigned in an E17 Type Assignment activity.
Any instance of a CRM entity may be assigned a type through type assignment. Type assignment events allow a more detailed path from E1 CRM Entity through P41 classified (was classified), E17 Type Assignment, P42 assigned (was assigned by) to E55 Type for assigning types to objects compared to the shortcut offered by P2 has type (is type of)."""@en ;
    rdfs:domain crm:E17_Type_Assignment ;
    rdfs:range crm:E1_CRM_Entity ;
    rdfs:subPropertyOf crm:P140_assigned_attribute_to .

crm:P41i_was_classified_by a rdf:Property ;
    rdfs:label "wurde klassifiziert durch"@de,
        "χαρακτηρίσθηκε από"@el,
        "was classified by"@en,
        "a été classifiée par le biais de"@fr,
        "foi classificada por"@pt,
        "был классифицирован посредством"@ru ;
    rdfs:domain crm:E1_CRM_Entity ;
    rdfs:range crm:E17_Type_Assignment ;
    rdfs:subPropertyOf crm:P140i_was_attributed_by .

crm:P42_assigned a rdf:Property ;
    rdfs:label "wies zu"@de,
        "απέδωσε ως ιδιότητα"@el,
        "assigned"@en,
        "a attribué"@fr,
        "atribuiu"@pt,
        "назначил"@ru ;
    rdfs:comment """This property records the type that was assigned to an entity by an E17 Type Assignment activity. 
Type assignment events allow a more detailed path from E1 CRM Entity through P41 classified (was classified by), E17 Type Assignment, P42 assigned (was assigned by) to E55 Type for assigning types to objects compared to the shortcut offered by P2 has type (is type of).
For example, a fragment of an antique vessel could be assigned the type “attic red figured belly handled amphora” by expert A. The same fragment could be assigned the type “shoulder handled amphora” by expert B.
A Type may be intellectually constructed independent from assigning an instance of it."""@en ;
    rdfs:domain crm:E17_Type_Assignment ;
    rdfs:range crm:E55_Type ;
    rdfs:subPropertyOf crm:P141_assigned .

crm:P42i_was_assigned_by a rdf:Property ;
    rdfs:label "wurde zugewiesen durch"@de,
        "αποδόθηκε από"@el,
        "was assigned by"@en,
        "a été attribué par"@fr,
        "foi atribuído por"@pt,
        "был присвоен посредством"@ru ;
    rdfs:domain crm:E55_Type ;
    rdfs:range crm:E17_Type_Assignment ;
    rdfs:subPropertyOf crm:P141i_was_assigned_by .

crm:P43_has_dimension a rdf:Property ;
    rdfs:label "hat Dimension"@de,
        "έχει μέγεθος"@el,
        "has dimension"@en,
        "a pour dimension"@fr,
        "tem dimensão"@pt,
        "имеет величину"@ru ;
    rdfs:comment """This property records a E54 Dimension of some E70 Thing.
It is a shortcut of the more fully developed path from E70 Thing through P39 measured (was measured by), E16 Measurement P40 observed dimension (was observed in) to E54 Dimension. It offers no information about how and when an E54 Dimension was established, nor by whom.
An instance of E54 Dimension is specific to an instance of E70 Thing."""@en ;
    rdfs:domain crm:E70_Thing ;
    rdfs:range crm:E54_Dimension .

crm:P43i_is_dimension_of a rdf:Property ;
    rdfs:label "ist Dimension von"@de,
        "είναι μέγεθος του"@el,
        "is dimension of"@en,
        "est dimension de"@fr,
        "é dimensão de"@pt,
        "является величиной для"@ru ;
    rdfs:domain crm:E54_Dimension ;
    rdfs:range crm:E70_Thing .

crm:P44_has_condition a rdf:Property ;
    rdfs:label "hat Zustand"@de,
        "έχει κατάσταση"@el,
        "has condition"@en,
        "a pour état matériel"@fr,
        "tem estado material "@pt,
        "имеет условие"@ru ;
    rdfs:comment """This property records an E3 Condition State for some E18 Physical Thing.
It is a shortcut of the more fully developed path from E18 Physical Thing through P34 concerned (was assessed by), E14 Condition Assessment P35 has identified (was identified by) to E3 Condition State. It offers no information about how and when the E3 Condition State was established, nor by whom. 
An instance of Condition State is specific to an instance of Physical Thing."""@en ;
    rdfs:domain crm:E18_Physical_Thing ;
    rdfs:range crm:E3_Condition_State .

crm:P44i_is_condition_of a rdf:Property ;
    rdfs:label "ist Zustand von"@de,
        "είναι κατάσταση του"@el,
        "is condition of"@en,
        "état matériel de"@fr,
        "estado material de"@pt,
        "является условием для"@ru ;
    rdfs:domain crm:E3_Condition_State ;
    rdfs:range crm:E18_Physical_Thing .

crm:P45_consists_of a rdf:Property ;
    rdfs:label "besteht aus"@de,
        "αποτελείται από"@el,
        "consists of"@en,
        "consiste en"@fr,
        "consiste de"@pt,
        "составлен из"@ru ;
    rdfs:comment """This property identifies the instances of E57 Materials of which an instance of E18 Physical Thing is composed.
All physical things consist of physical materials. P45 consists of (is incorporated in) allows the different Materials to be recorded. P45 consists of (is incorporated in) refers here to observed Material as opposed to the consumed raw material.
A Material, such as a theoretical alloy, may not have any physical instances"""@en ;
    rdfs:domain crm:E18_Physical_Thing ;
    rdfs:range crm:E57_Material .

crm:P45i_is_incorporated_in a rdf:Property ;
    rdfs:label "ist enthalten in"@de,
        "είναι ενσωματωμένος/η/ο σε"@el,
        "is incorporated in"@en,
        "est présent dans"@fr,
        "está presente em"@pt,
        "входит в состав"@ru ;
    rdfs:domain crm:E57_Material ;
    rdfs:range crm:E18_Physical_Thing .

crm:P48_has_preferred_identifier a rdf:Property ;
    rdfs:label "hat bevorzugtes Kennzeichen"@de,
        "έχει προτιμώμενο αναγνωριστικό"@el,
        "has preferred identifier"@en,
        "a pour identificateur retenu"@fr,
        "tem identificador preferido"@pt,
        "имеет предпочтительный идентификатор"@ru ;
    rdfs:comment """This property records the preferred E42 Identifier that was used to identify an instance of E1 CRM Entity at the time this property was recorded.
More than one preferred identifier may have been assigned to an item over time.
Use of this property requires an external mechanism for assigning temporal validity to the respective CRM instance.
P48 has preferred identifier (is preferred identifier of), is a shortcut for the path from E1 CRM Entity through P140 assigned attribute to (was attributed by), E15 Identifier Assignment, P37 assigned (was assigned by) to E42 Identifier. The fact that an identifier is a preferred one for an organisation can be better expressed in a context independent form by assigning a suitable E55 Type to the respective instance of E15 Identifier Assignment using the P2 has type property."""@en ;
    rdfs:domain crm:E1_CRM_Entity ;
    rdfs:range crm:E42_Identifier ;
    rdfs:subPropertyOf crm:P1_is_identified_by .

crm:P48i_is_preferred_identifier_of a rdf:Property ;
    rdfs:label "ist bevorzugtes Kennzeichen für"@de,
        "είναι προτιμώμενο αναγνωριστικό"@el,
        "is preferred identifier of"@en,
        "est l’identificateur retenu de"@fr,
        "é o identificador preferido de"@pt,
        "является предпочтительным идентификатором для"@ru ;
    rdfs:domain crm:E42_Identifier ;
    rdfs:range crm:E1_CRM_Entity ;
    rdfs:subPropertyOf crm:P1i_identifies .

crm:P4_has_time-span a rdf:Property ;
    rdfs:label "hat Zeitspanne"@de,
        "βρισκόταν σε εξέλιξη"@el,
        "has time-span"@en,
        "a pour durée"@fr,
        "tem período de tempo"@pt,
        "имеет временной отрезок"@ru ;
    rdfs:comment """This property describes the temporal confinement of an instance of an E2 Temporal Entity.
The related E52 Time-Span is understood as the real Time-Span during which the phenomena were active, which make up the temporal entity instance. It does not convey any other meaning than a positioning on the “time-line” of chronology. The Time-Span in turn is approximated by a set of dates (E61 Time Primitive). A temporal entity can have in reality only one Time-Span, but there may exist alternative opinions about it, which we would express by assigning multiple Time-Spans. Related temporal entities may share a Time-Span. Time-Spans may have completely unknown dates but other descriptions by which we can infer knowledge."""@en ;
    rdfs:domain crm:E2_Temporal_Entity ;
    rdfs:range crm:E52_Time-Span .

crm:P4i_is_time-span_of a rdf:Property ;
    rdfs:label "ist Zeitspanne von"@de,
        "είναι χρονικό διάστημα του/της"@el,
        "is time-span of"@en,
        "est la durée de"@fr,
        "é o período de tempo de"@pt,
        "является временным отрезком для"@ru ;
    rdfs:domain crm:E52_Time-Span ;
    rdfs:range crm:E2_Temporal_Entity .

crm:P50_has_current_keeper a rdf:Property ;
    rdfs:label "hat derzeitigen Betreuer"@de,
        "είναι στην κατοχή του"@el,
        "has current keeper"@en,
        "est actuellement détenu par"@fr,
        "é guardada por"@pt,
        "имеет текущего смотрителя"@ru ;
    rdfs:comment """This property identifies the E39 Actor or Actors who had custody of an instance of E18 Physical Thing at the time this property was recorded.
P50 has current keeper (is current keeper of) is a shortcut for the more detailed path from E18 Physical Thing through P30 transferred custody of (custody transferred through), E10 Transfer of Custody, P29 custody received by (received custody through) to E39 Actor."""@en ;
    rdfs:domain crm:E18_Physical_Thing ;
    rdfs:range crm:E39_Actor ;
    rdfs:subPropertyOf crm:P49_has_former_or_current_keeper .

crm:P50i_is_current_keeper_of a rdf:Property ;
    rdfs:label "ist derzeitiger Betreuer von"@de,
        "κατέχει"@el,
        "is current keeper of"@en,
        "est actuel détenteur de"@fr,
        "é guardador de"@pt,
        "является текущим смотрителем для"@ru ;
    rdfs:domain crm:E39_Actor ;
    rdfs:range crm:E18_Physical_Thing ;
    rdfs:subPropertyOf crm:P49i_is_former_or_current_keeper_of .

crm:P52_has_current_owner a rdf:Property ;
    rdfs:label "hat derzeitigen Besitzer"@de,
        "έχει ιδιοκτήτη"@el,
        "has current owner"@en,
        "est actuellement possédée par"@fr,
        "é propriedade de"@pt,
        "имеет текущего владельца"@ru ;
    rdfs:comment """This property identifies the E21 Person, E74 Group or E40 Legal Body that was the owner of an instance of E18 Physical Thing at the time this property was recorded.
P52 has current owner (is current owner of) is a shortcut for the more detailed path from E18 Physical Thing through P24 transferred title of (changed ownership through), E8 Acquisition, P22 transferred title to (acquired title through) to E39 Actor, if and only if this acquisition event is the most recent."""@en ;
    rdfs:domain crm:E18_Physical_Thing ;
    rdfs:range crm:E39_Actor ;
    rdfs:subPropertyOf crm:P105_right_held_by,
        crm:P51_has_former_or_current_owner .

crm:P52i_is_current_owner_of a rdf:Property ;
    rdfs:label "ist derzeitiger Besitzer von"@de,
        "είναι ιδιοκτήτης του"@el,
        "is current owner of"@en,
        "est le propriétaire actuel de"@fr,
        "é proprietário de"@pt,
        "является текущим владельцем для"@ru ;
    rdfs:domain crm:E39_Actor ;
    rdfs:range crm:E18_Physical_Thing ;
    rdfs:subPropertyOf crm:P105i_has_right_on,
        crm:P51i_is_former_or_current_owner_of .

crm:P54_has_current_permanent_location a rdf:Property ;
    rdfs:label "hat derzeitigen permanenten Standort"@de,
        "έχει μόνιμη θέση"@el,
        "has current permanent location"@en,
        "a actuellement pour localisation à demeure"@fr,
        "é localizado permanentemente em"@pt,
        "имеет текущее постоянное местоположение"@ru ;
    rdfs:comment """This property records the foreseen permanent location of an instance of E19 Physical Object at the time this property was recorded.
P54 has current permanent location (is current permanent location of) is similar to P55 has current location (currently holds). However, it indicates the E53 Place currently reserved for an object, such as the permanent storage location or a permanent exhibit location. The object may be temporarily removed from the permanent location, for example when used in temporary exhibitions or loaned to another institution. The object may never actually be located at its permanent location."""@en ;
    rdfs:domain crm:E19_Physical_Object ;
    rdfs:range crm:E53_Place .

crm:P54i_is_current_permanent_location_of a rdf:Property ;
    rdfs:label "ist derzeitiger permanenter Standort von"@de,
        "είναι μόνιμη θέση του/της"@el,
        "is current permanent location of"@en,
        "est actuellement localisation à demeure de"@fr,
        "é localização permanente de"@pt,
        "является текущим постоянным местоположением для"@ru ;
    rdfs:domain crm:E53_Place ;
    rdfs:range crm:E19_Physical_Object .

crm:P55_has_current_location a rdf:Property ;
    rdfs:label "hat derzeitigen Standort"@de,
        "βρίσκεται σε"@el,
        "has current location"@en,
        "a pour localisation actuelle"@fr,
        "é localizado em"@pt,
        "в данный момент находится в"@ru ;
    rdfs:comment """This property records the location of an E19 Physical Object at the time the property was recorded.
This property is a specialisation of P53 has former or current location (is former or current location of). It indicates that the E53 Place associated with the E19 Physical Object is the current location of the object. The property does not allow any indication of how long the Object has been at the current location. 
P55 has current location (currently holds) is a shortcut. A more detailed representation can make use of the fully developed (i.e. indirect) path from E19 Physical Object through P25 moved (moved by), E9 Move P26 moved to (was destination of) to E53 Place if and only if this Move is the most recent."""@en ;
    rdfs:domain crm:E19_Physical_Object ;
    rdfs:range crm:E53_Place ;
    rdfs:subPropertyOf crm:P53_has_former_or_current_location .

crm:P55i_currently_holds a rdf:Property ;
    rdfs:label "hält derzeitig"@de,
        "είναι θέση του"@el,
        "currently holds"@en,
        "est localisation actuelle de"@fr,
        "é localização atual de"@pt,
        "в данный момент содержит"@ru ;
    rdfs:domain crm:E53_Place ;
    rdfs:range crm:E19_Physical_Object ;
    rdfs:subPropertyOf crm:P53i_is_former_or_current_location_of .

crm:P56_bears_feature a rdf:Property ;
    rdfs:label "trägt Merkmal"@de,
        "φέρει μόρφωμα"@el,
        "bears feature"@en,
        "présente pour caractéristique"@fr,
        "possui característica"@pt,
        "несет признак"@ru ;
    rdfs:comment """This property describes a E26 Physical Feature found on a E19 Physical Object It does not specify the location of the feature on the object.
P56 bears feature (is found on) is a shortcut. A more detailed representation can make use of the fully developed (i.e. indirect) path from E19 Physical Object through P59 has section (is located on or within), E53 Place, P53 has former or current location (is former or current location of) to E26 Physical Feature.
A Physical Feature can only exist on one object. One object may bear more than one Physical Feature. An E27 Site should be considered as an E26 Physical Feature on the surface of the Earth."""@en ;
    rdfs:domain crm:E19_Physical_Object ;
    rdfs:range crm:E26_Physical_Feature ;
    rdfs:subPropertyOf crm:P46_is_composed_of .

crm:P56i_is_found_on a rdf:Property ;
    rdfs:label "wird gefunden auf"@de,
        "βρίσκεται σε"@el,
        "is found on"@en,
        "se trouve sur"@fr,
        "é encontrada em"@pt,
        "найден на"@ru ;
    rdfs:domain crm:E26_Physical_Feature ;
    rdfs:range crm:E19_Physical_Object ;
    rdfs:subPropertyOf crm:P46i_forms_part_of .

crm:P57_has_number_of_parts a rdf:Property ;
    rdfs:label "hat Anzahl Teile"@de,
        "έχει αριθμό μερών"@el,
        "has number of parts"@en,
        "a pour nombre de parties"@fr,
        "tem número de partes"@pt,
        "имеет число частей"@ru ;
    rdfs:comment """This property documents the E60 Number of parts of which an instance of E19 Physical Object is composed.
This may be used as a method of checking inventory counts with regard to aggregate or collective objects. What constitutes a part or component depends on the context and requirements of the documentation. Normally, the parts documented in this way would not be considered as worthy of individual attention.
For a more complete description, objects may be decomposed into their components and constituents using P46 is composed of (forms parts of) and P45 consists of (is incorporated in). This allows each element to be described individually."""@en ;
    rdfs:domain crm:E19_Physical_Object ;
    rdfs:range rdfs:Literal .

crm:P58_has_section_definition a rdf:Property ;
    rdfs:label "hat Abschittsdefinition"@de,
        "έχει ορισμό τμήματος"@el,
        "has section definition"@en,
        "a pour désignation de section"@fr,
        "tem designação de seção"@pt,
        "имеет определение района"@ru ;
    rdfs:comment """This property links an area (section) named by a E46 Section Definition to the instance of E18 Physical Thing upon which it is found.
The CRM handles sections as locations (instances of E53 Place) within or on E18 Physical Thing that are identified by E46 Section Definitions. Sections need not be discrete and separable components or parts of an object.
This is part of a more developed path from E18 Physical Thing through P58, E46 Section Definition, P87 is identified by (identifies) that allows a more precise definition of a location found on an object than the shortcut P59 has section (is located on or within).
A particular instance of a Section Definition only applies to one instance of Physical Thing."""@en ;
    rdfs:domain crm:E18_Physical_Thing ;
    rdfs:range crm:E46_Section_Definition .

crm:P58i_defines_section a rdf:Property ;
    rdfs:label "definiert Abschitt auf oder von"@de,
        "ορίζει τμήμα σε"@el,
        "defines section"@en,
        "définit une section de"@fr,
        "define uma seção de"@pt,
        "определяет район"@ru ;
    rdfs:domain crm:E46_Section_Definition ;
    rdfs:range crm:E18_Physical_Thing .

crm:P59_has_section a rdf:Property ;
    rdfs:label "hat Bereich"@de,
        "έχει τομέα"@el,
        "has section"@en,
        "a pour section"@fr,
        "tem seção"@pt,
        "имеет район"@ru ;
    rdfs:comment """This property links an area to the instance of E18 Physical Thing upon which it is found.
It is typically used when a named E46 Section Definition is not appropriate.
E18 Physical Thing may be subdivided into arbitrary regions. 
P59 has section (is located on or within) is a shortcut. If the E53 Place is identified by a Section Definition, a more detailed representation can make use of the fully developed (i.e. indirect) path from E18 Physical Thing through P58 has section definition (defines section), E46 Section Definition, P87 is identified by (identifies) to E53 Place. A Place can only be located on or within one Physical Object."""@en ;
    rdfs:domain crm:E18_Physical_Thing ;
    rdfs:range crm:E53_Place .

crm:P59i_is_located_on_or_within a rdf:Property ;
    rdfs:label "befindet sich auf oder in"@de,
        "βρίσκεται σε ή εντός"@el,
        "is located on or within"@en,
        "se situe sur ou dans"@fr,
        "está localizada sobre ou dentro de"@pt,
        "находится на или внутри"@ru ;
    rdfs:domain crm:E53_Place ;
    rdfs:range crm:E18_Physical_Thing .

crm:P5_consists_of a rdf:Property ;
    rdfs:label "besteht aus"@de,
        "αποτελείται από"@el,
        "consists of"@en,
        "consiste en"@fr,
        "consiste de"@pt,
        "состоит из"@ru ;
    rdfs:comment """This property describes the decomposition of an E3 Condition State into discrete, subsidiary states. 
It is assumed that the sub-states into which the condition state is analysed form a logical whole - although the entire story may not be completely known – and that the sub-states are in fact constitutive of the general condition state. For example, a general condition state of “in ruins” may be decomposed into the individual stages of decay"""@en ;
    rdfs:domain crm:E3_Condition_State ;
    rdfs:range crm:E3_Condition_State .

crm:P5i_forms_part_of a rdf:Property ;
    rdfs:label "bildet Teil von"@de,
        "αποτελεί μέρος του/της"@el,
        "forms part of"@en,
        "fait partie de"@fr,
        "faz parte de"@pt,
        "формирует часть"@ru ;
    rdfs:domain crm:E3_Condition_State ;
    rdfs:range crm:E3_Condition_State .

crm:P65_shows_visual_item a rdf:Property ;
    rdfs:label "zeigt Bildliches"@de,
        "εμφανίζει οπτικό στοιχείο"@el,
        "shows visual item"@en,
        "présente l'item visuel"@fr,
        "apresenta item visual"@pt,
        "показывает визуальный предмет"@ru ;
    rdfs:comment """This property documents an E36 Visual Item shown by an instance of E24 Physical Man-Made Thing.
This property is similar to P62 depicts (is depicted by) in that it associates an item of E24 Physical Man-Made Thing with a visual representation. However, P65 shows visual item (is shown by) differs from the P62 depicts (is depicted by) property in that it makes no claims about what the E36 Visual Item is deemed to represent. E36 Visual Item identifies a recognisable image or visual symbol, regardless of what this image may or may not represent.
For example, all recent British coins bear a portrait of Queen Elizabeth II, a fact that is correctly documented using P62 depicts (is depicted by). Different portraits have been used at different periods, however. P65 shows visual item (is shown by) can be used to refer to a particular portrait.
P65 shows visual item (is shown by) may also be used for Visual Items such as signs, marks and symbols, for example the 'Maltese Cross' or the 'copyright symbol’ that have no particular representational content. 
This property is part of the fully developed path from E24 Physical Man-Made Thing through P65 shows visual item (is shown by), E36 Visual Item, P138 represents (has representation) to E1 CRM Entity which is shortcut by, P62 depicts (is depicted by)."""@en ;
    rdfs:domain crm:E24_Physical_Man-Made_Thing ;
    rdfs:range crm:E36_Visual_Item ;
    rdfs:subPropertyOf crm:P128_carries .

crm:P65i_is_shown_by a rdf:Property ;
    rdfs:label "wird gezeigt durch"@de,
        "εμφανίζεται σε"@el,
        "is shown by"@en,
        "est présenté par"@fr,
        "é apresentado por"@pt,
        "показан посредством"@ru ;
    rdfs:domain crm:E36_Visual_Item ;
    rdfs:range crm:E24_Physical_Man-Made_Thing ;
    rdfs:subPropertyOf crm:P128i_is_carried_by .

crm:P68_foresees_use_of a rdf:Property ;
    rdfs:label " sieht den Gebrauch vor von"@de,
        "συνήθως χρησιμοποιεί"@el,
        "foresees use of"@en,
        "utilise habituellement"@fr,
        "normalmente emprega"@pt,
        "обычно применяет"@ru ;
    rdfs:comment """This property identifies an E57 Material foreseeen to be used by an E29 Design or Procedure. 
E29 Designs and procedures commonly foresee the use of particular E57 Materials. The fabrication of adobe bricks, for example, requires straw, clay and water. This property enables this to be documented.
This property is not intended for the documentation of E57 Materials that were used on a particular occasion when an instance of E29 Design or Procedure was executed."""@en ;
    rdfs:domain crm:E29_Design_or_Procedure ;
    rdfs:range crm:E57_Material ;
    rdfs:subPropertyOf crm:P67_refers_to .

crm:P68i_use_foreseen_by a rdf:Property ;
    rdfs:label "vorgesehen für Gebrauch durch defined"@de,
        "συνήθως χρησιμοποιείται από"@el,
        "use foreseen by"@en,
        "est habituellement utilisé par"@fr,
        "é empregado por"@pt,
        "обычно используется посредством"@ru ;
    rdfs:domain crm:E57_Material ;
    rdfs:range crm:E29_Design_or_Procedure ;
    rdfs:subPropertyOf crm:P67i_is_referred_to_by .

crm:P69_is_associated_with a rdf:Property ;
    rdfs:label "ist verbunden mit"@de,
        "σχετίζεται με"@el,
        "is associated with"@en,
        "est associée à"@fr,
        "é associado com"@pt,
        "ассоциирован с"@ru ;
    rdfs:comment """This symmetric property describes the association of an E29 Design or Procedure with other Designs or Procedures.
Any instance of E29 Design or Procedure may be associated with other designs or procedures. The P69.1 has type property of P69 is associated with allows the nature of the association to be specified; examples of types of association between instances of E29 Design or Procedure include: whole-part, sequence, prerequisite, etc."""@en ;
    rdfs:domain crm:E29_Design_or_Procedure ;
    rdfs:range crm:E29_Design_or_Procedure .

crm:P70_documents a rdf:Property ;
    rdfs:label "belegt"@de,
        "τεκμηριώνει"@el,
        "documents"@en,
        "mentionne"@fr,
        "documenta"@pt,
        "документирует"@ru ;
    rdfs:comment """This property describes the CRM Entities documented by instances of E31 Document.
Documents may describe any conceivable entity, hence the link to the highest-level entity in the CRM hierarchy. This property is intended for cases where a reference is regarded as being of a documentary character, in the scholarly or scientific sense."""@en ;
    rdfs:domain crm:E31_Document ;
    rdfs:range crm:E1_CRM_Entity ;
    rdfs:subPropertyOf crm:P67_refers_to .

crm:P70i_is_documented_in a rdf:Property ;
    rdfs:label "wird belegt in"@de,
        "τεκμηριώνεται σε"@el,
        "is documented in"@en,
        "est mentionnée dans"@fr,
        "é documentado em"@pt,
        "документирован в"@ru ;
    rdfs:domain crm:E1_CRM_Entity ;
    rdfs:range crm:E31_Document ;
    rdfs:subPropertyOf crm:P67i_is_referred_to_by .

crm:P71_lists a rdf:Property ;
    rdfs:label "listet"@de,
        "περιλαμβάνει"@el,
        "lists"@en,
        "définit"@fr,
        "define"@pt,
        "перечисляет"@ru ;
    rdfs:comment "This property documents a source E32 Authority Document for an instance of an E1 CRM Entity."@en ;
    rdfs:domain crm:E32_Authority_Document ;
    rdfs:range crm:E1_CRM_Entity ;
    rdfs:subPropertyOf crm:P67_refers_to .

crm:P71i_is_listed_in a rdf:Property ;
    rdfs:label "wird aufgelistet in"@de,
        "περιλαμβάνεται σε"@el,
        "is listed in"@en,
        "est défini par"@fr,
        "é definido por"@pt,
        "перечислен в"@ru ;
    rdfs:domain crm:E1_CRM_Entity ;
    rdfs:range crm:E32_Authority_Document ;
    rdfs:subPropertyOf crm:P67i_is_referred_to_by .

crm:P72_has_language a rdf:Property ;
    rdfs:label "hat Sprache"@de,
        "έχει γλώσσα"@el,
        "has language"@en,
        "est en langue"@fr,
        "é da língua "@pt,
        "имеет язык"@ru ;
    rdfs:comment """This property describes the E56 Language of an E33 Linguistic Object. 
Linguistic Objects are composed in one or more human Languages. This property allows these languages to be documented."""@en ;
    rdfs:domain crm:E33_Linguistic_Object ;
    rdfs:range crm:E56_Language .

crm:P72i_is_language_of a rdf:Property ;
    rdfs:label "ist Sprache von"@de,
        "είναι γλώσσα του/της"@el,
        "is language of"@en,
        "est la langue de"@fr,
        "é a língua de"@pt,
        "является языком для"@ru ;
    rdfs:domain crm:E56_Language ;
    rdfs:range crm:E33_Linguistic_Object .

crm:P73_has_translation a rdf:Property ;
    rdfs:label "hat Übersetzung"@de,
        "έχει μετάφραση"@el,
        "has translation"@en,
        "a pour traduction"@fr,
        "tem tradução"@pt,
        "имеет перевод"@ru ;
    rdfs:comment """This property describes the source and target of instances of E33Linguistic Object involved in a translation.
When a Linguistic Object is translated into a new language it becomes a new Linguistic Object, despite being conceptually similar to the source object."""@en ;
    rdfs:domain crm:E33_Linguistic_Object ;
    rdfs:range crm:E33_Linguistic_Object ;
    rdfs:subPropertyOf crm:P130_shows_features_of .

crm:P73i_is_translation_of a rdf:Property ;
    rdfs:label "ist Übersetzung von"@de,
        "είναι μετάφραση του/της"@el,
        "is translation of"@en,
        "est la traduction de"@fr,
        "é tradução de"@pt,
        "является переводом"@ru ;
    rdfs:domain crm:E33_Linguistic_Object ;
    rdfs:range crm:E33_Linguistic_Object ;
    rdfs:subPropertyOf crm:P130i_features_are_also_found_on .

crm:P74_has_current_or_former_residence a rdf:Property ;
    rdfs:label "hat derzeitigen oder früheren Sitz"@de,
        "έχει ή είχε κατοικία"@el,
        "has current or former residence"@en,
        "réside ou a résidé à"@fr,
        "reside ou residiu em"@pt,
        "имеет текущее или бывшее местожительства"@ru ;
    rdfs:comment """This property describes the current or former E53 Place of residence of an E39 Actor. 
The residence may be either the Place where the Actor resides, or a legally registered address of any kind."""@en ;
    rdfs:domain crm:E39_Actor ;
    rdfs:range crm:E53_Place .

crm:P74i_is_current_or_former_residence_of a rdf:Property ;
    rdfs:label "ist derzeitiger oder früherer Sitz von"@de,
        "είναι ή ήταν κατοικία του/της"@el,
        "is current or former residence of"@en,
        "est ou a été la résidence de"@fr,
        "é ou foi residência de"@pt,
        "является текущим или бывшим местом жительства для"@ru ;
    rdfs:domain crm:E53_Place ;
    rdfs:range crm:E39_Actor .

crm:P75_possesses a rdf:Property ;
    rdfs:label "besitzt"@de,
        "κατέχει"@el,
        "possesses"@en,
        "est détenteur de"@fr,
        "é detentor de"@pt,
        "владеет"@ru ;
    rdfs:comment "This property identifies former or current instances of E30 Rights held by an E39 Actor."@en ;
    rdfs:domain crm:E39_Actor ;
    rdfs:range crm:E30_Right .

crm:P75i_is_possessed_by a rdf:Property ;
    rdfs:label "sind im Besitz von"@de,
        "κατέχεται από"@el,
        "is possessed by"@en,
        "est détenu par"@fr,
        "são detidos por"@pt,
        "принадлежит"@ru ;
    rdfs:domain crm:E30_Right ;
    rdfs:range crm:E39_Actor .

crm:P76_has_contact_point a rdf:Property ;
    rdfs:label "hat Kontaktpunkt"@de,
        "έχει σημείο επικοινωνίας"@el,
        "has contact point"@en,
        "a pour coordonnées individuelles"@fr,
        "possui ponto de contato"@pt,
        "имеет контакт"@ru ;
    rdfs:comment "This property identifies an E51 Contact Point of any type that provides access to an E39 Actor by any communication method, such as e-mail or fax."@en ;
    rdfs:domain crm:E39_Actor ;
    rdfs:range crm:E51_Contact_Point .

crm:P76i_provides_access_to a rdf:Property ;
    rdfs:label "bietet Zugang zu"@de,
        "παρέχει πρόσβαση σε"@el,
        "provides access to"@en,
        "permettent de contacter"@fr,
        "é ponto de contado de"@pt,
        "предоставляет доступ к"@ru ;
    rdfs:domain crm:E51_Contact_Point ;
    rdfs:range crm:E39_Actor .

crm:P78_is_identified_by a rdf:Property ;
    rdfs:label "wird bezeichnet als"@de,
        "αναγνωρίζεται ως"@el,
        "is identified by"@en,
        "est identifiée par"@fr,
        "é identificado por "@pt,
        "идентифицируется посредством"@ru ;
    rdfs:comment "This property identifies an E52 Time-Span using an E49Time Appellation."@en ;
    rdfs:domain crm:E52_Time-Span ;
    rdfs:range crm:E49_Time_Appellation ;
    rdfs:subPropertyOf crm:P1_is_identified_by .

crm:P78i_identifies a rdf:Property ;
    rdfs:label "bezeichnet"@de,
        "είναι αναγνωριστικό"@el,
        "identifies"@en,
        "identifie"@fr,
        "identifica"@pt,
        "идентифицирует"@ru ;
    rdfs:domain crm:E49_Time_Appellation ;
    rdfs:range crm:E52_Time-Span ;
    rdfs:subPropertyOf crm:P1i_identifies .

crm:P79_beginning_is_qualified_by a rdf:Property ;
    rdfs:label "hat Anfangsbegründung"@de,
        "αρχή προσδιορίζεται από"@el,
        "beginning is qualified by"@en,
        "début est qualifié par"@fr,
        "início é qualificado por"@pt,
        "начало ограничено"@ru ;
    rdfs:comment """This property qualifies the beginning of an E52 Time-Span in some way. 
The nature of the qualification may be certainty, precision, source etc."""@en ;
    rdfs:domain crm:E52_Time-Span ;
    rdfs:range rdfs:Literal ;
    rdfs:subPropertyOf crm:P3_has_note .

crm:P80_end_is_qualified_by a rdf:Property ;
    rdfs:label "hat Begründung des Endes"@de,
        "τέλος προσδιορίζεται από"@el,
        "end is qualified by"@en,
        "fin est qualifiée par"@fr,
        "final é qualificado por"@pt,
        "конец ограничен"@ru ;
    rdfs:comment """This property qualifies the end of an E52 Time-Span in some way. 
The nature of the qualification may be certainty, precision, source etc."""@en ;
    rdfs:domain crm:E52_Time-Span ;
    rdfs:range rdfs:Literal ;
    rdfs:subPropertyOf crm:P3_has_note .

crm:P81_ongoing_throughout a rdf:Property ;
    rdfs:label "andauernd während"@de,
        "καθόλη τη διάρκεια του/της"@el,
        "ongoing throughout"@en,
        "couvre au moins"@fr,
        "abrange no mínimo"@pt,
        "длится в течение"@ru ;
    rdfs:comment """This property describes the minimum period of time covered by an E52 Time-Span.
Since Time-Spans may not have precisely known temporal extents, the CRM supports statements about the minimum and maximum temporal extents of Time-Spans. This property allows a Time-Span’s minimum temporal extent (i.e. its inner boundary) to be assigned an E61 Time Primitive value. Time Primitives are treated by the CRM as application or system specific date intervals, and are not further analysed."""@en ;
    rdfs:domain crm:E52_Time-Span ;
    rdfs:range rdfs:Literal .

crm:P82_at_some_time_within a rdf:Property ;
    rdfs:label "irgendwann innerhalb von"@de,
        "κάποτε εντός"@el,
        "at some time within"@en,
        "couvre au plus"@fr,
        "abrange no máximo"@pt,
        "некоторое время в течение"@ru ;
    rdfs:comment """This property describes the maximum period of time within which an E52 Time-Span falls.
Since Time-Spans may not have precisely known temporal extents, the CRM supports statements about the minimum and maximum temporal extents of Time-Spans. This property allows a Time-Span’s maximum temporal extent (i.e. its outer boundary) to be assigned an E61 Time Primitive value. Time Primitives are treated by the CRM as application or system specific date intervals, and are not further analysed."""@en ;
    rdfs:domain crm:E52_Time-Span ;
    rdfs:range rdfs:Literal .

crm:P83_had_at_least_duration a rdf:Property ;
    rdfs:label "hatte Mindestdauer"@de,
        "είχε ελάχιστη διάρκεια"@el,
        "had at least duration"@en,
        "a duré au moins"@fr,
        "durou no mínimo"@pt,
        "имеет длительность по крайней мере больше чем"@ru ;
    rdfs:comment """This property describes the minimum length of time covered by an E52 Time-Span. 
It allows an E52 Time-Span to be associated with an E54 Dimension representing it’s minimum duration (i.e. it’s inner boundary) independent from the actual beginning and end."""@en ;
    rdfs:domain crm:E52_Time-Span ;
    rdfs:range crm:E54_Dimension .

crm:P83i_was_minimum_duration_of a rdf:Property ;
    rdfs:label "war Mindestdauer von"@de,
        "είναι ελάχιστη διάρκεια του/της"@el,
        "was minimum duration of"@en,
        "a été la durée minimum de"@fr,
        "foi a duração mínima de"@pt,
        "был минимальной длительностью для"@ru ;
    rdfs:domain crm:E54_Dimension ;
    rdfs:range crm:E52_Time-Span .

crm:P84_had_at_most_duration a rdf:Property ;
    rdfs:label "hatte Höchstdauer"@de,
        "είχε μέγιστη διάρκεια"@el,
        "had at most duration"@en,
        "a duré au plus"@fr,
        "durou no máximo"@pt,
        "имеет длительность меньше чем"@ru ;
    rdfs:comment """This property describes the maximum length of time covered by an E52 Time-Span. 
It allows an E52 Time-Span to be associated with an E54 Dimension representing it’s maximum duration (i.e. it’s outer boundary) independent from the actual beginning and end."""@en ;
    rdfs:domain crm:E52_Time-Span ;
    rdfs:range crm:E54_Dimension .

crm:P84i_was_maximum_duration_of a rdf:Property ;
    rdfs:label "war längste Dauer von"@de,
        "είναι μέγιστη διάρκεια του/της"@el,
        "was maximum duration of"@en,
        "a été la durée maximum de"@fr,
        "foi a duração máxima de"@pt,
        "был максимальной длительностью для"@ru ;
    rdfs:domain crm:E54_Dimension ;
    rdfs:range crm:E52_Time-Span .

crm:P86_falls_within a rdf:Property ;
    rdfs:label "fällt in"@de,
        "περιέχεται σε"@el,
        "falls within"@en,
        "s’insère dans"@fr,
        "está contido em"@pt,
        "содержится в"@ru ;
    rdfs:comment """This property describes the inclusion relationship between two instances of E52 Time-Span.
This property supports the notion that a Time-Span’s temporal extent falls within the temporal extent of another Time-Span. It addresses temporal containment only, and no contextual link between the two instances of Time-Span is implied."""@en ;
    rdfs:domain crm:E52_Time-Span ;
    rdfs:range crm:E52_Time-Span .

crm:P86i_contains a rdf:Property ;
    rdfs:label "enthält"@de,
        "περιέχει"@el,
        "contains"@en,
        "inclut"@fr,
        "contém"@pt,
        "содержит"@ru ;
    rdfs:domain crm:E52_Time-Span ;
    rdfs:range crm:E52_Time-Span .

crm:P87_is_identified_by a rdf:Property ;
    rdfs:label "wird bezeichnet als"@de,
        "αναγνωρίζεται ως"@el,
        "is identified by"@en,
        "est identifié par"@fr,
        "é identificado por"@pt,
        "идентифицируется посредством"@ru ;
    rdfs:comment """This property identifies an E53 Place using an E44 Place Appellation. 
Examples of Place Appellations used to identify Places include instances of E48 Place Name, addresses, E47 Spatial Coordinates etc."""@en ;
    rdfs:domain crm:E53_Place ;
    rdfs:range crm:E44_Place_Appellation ;
    rdfs:subPropertyOf crm:P1_is_identified_by .

crm:P87i_identifies a rdf:Property ;
    rdfs:label "bezeichnet"@de,
        "είναι αναγνωριστικό"@el,
        "identifies"@en,
        "identifie"@fr,
        "identifica"@pt,
        "идентифицирует"@ru ;
    rdfs:domain crm:E44_Place_Appellation ;
    rdfs:range crm:E53_Place ;
    rdfs:subPropertyOf crm:P1i_identifies .

crm:P88_consists_of a rdf:Property ;
    rdfs:label "besteht aus"@de,
        "αποτελείται από"@el,
        "consists of"@en,
        "est en"@fr,
        "consiste de"@pt,
        "сделан из"@ru ;
    rdfs:comment """This property identifies an E53 Place that forms part of another Place.
It supports the notion that a Place can be subdivided into one or more constituent parts. It implies both spatial and contextual containment relationships between the two Places."""@en ;
    rdfs:domain crm:E53_Place ;
    rdfs:range crm:E53_Place .

crm:P88i_forms_part_of a rdf:Property ;
    rdfs:label "bildet Teil von"@de,
        "είναι τμήμα του"@el,
        "forms part of"@en,
        "fait partie de"@fr,
        "faz parte de"@pt,
        "формирует часть"@ru ;
    rdfs:domain crm:E53_Place ;
    rdfs:range crm:E53_Place .

crm:P89_falls_within a rdf:Property ;
    rdfs:label "fällt in"@de,
        "περιέχεται σε"@el,
        "falls within"@en,
        "s’insère dans"@fr,
        "está contido em"@pt,
        "содержится в"@ru ;
    rdfs:comment """This property identifies the instances of E53 Places that fall within the area covered by another Place.
It addresses spatial containment only, and no ‘whole-part’ relationship between the two places is implied."""@en ;
    rdfs:domain crm:E53_Place ;
    rdfs:range crm:E53_Place .

crm:P89i_contains a rdf:Property ;
    rdfs:label "enthält"@de,
        "περιέχει"@el,
        "contains"@en,
        "inclut"@fr,
        "contém"@pt,
        "содержит"@ru ;
    rdfs:domain crm:E53_Place ;
    rdfs:range crm:E53_Place .

crm:P8_took_place_on_or_within a rdf:Property ;
    rdfs:label "fand statt auf oder innerhalb von "@de,
        "έλαβε χώρα σε ή εντός"@el,
        "took place on or within"@en,
        "a eu lieu sur ou dans"@fr,
        "ocorreu em ou dentro"@pt,
        "имел место на или в"@ru ;
    rdfs:comment """This property describes the location of an instance of E4 Period with respect to an E19 Physical Object.
P8 took place on or within (witnessed) is a short-cut of a path defining a E53 Place with respect to the geometry of an object. cf. E46 Section Definition.
This property is in effect a special case of P7 took place at. It describes a period that can be located with respect to the space defined by an E19 Physical Object such as a ship or a building. The precise geographical location of the object during the period in question may be unknown or unimportant. 
For example, the French and German armistice of 22 June 1940 was signed in the same railway carriage as the armistice of 11 November 1918."""@en ;
    rdfs:domain crm:E4_Period ;
    rdfs:range crm:E19_Physical_Object .

crm:P8i_witnessed a rdf:Property ;
    rdfs:label "bezeugte"@de,
        "υπήρξε τόπος του"@el,
        "witnessed"@en,
        "a été témoin de"@fr,
        "testemunhou"@pt,
        "являлся местом для"@ru ;
    rdfs:domain crm:E19_Physical_Object ;
    rdfs:range crm:E4_Period .

crm:P90_has_value a rdf:Property ;
    rdfs:label "hat Wert"@de,
        "έχει τιμή"@el,
        "has value"@en,
        "a la valeur"@fr,
        "tem valor"@pt,
        "имеет значение"@ru ;
    rdfs:comment "This property allows an E54 Dimension to be approximated by an E60 Number primitive."@en ;
    rdfs:domain crm:E54_Dimension ;
    rdfs:range rdfs:Literal .

crm:P91_has_unit a rdf:Property ;
    rdfs:label "hat Einheit"@de,
        "έχει μονάδα μέτρησης"@el,
        "has unit"@en,
        "a pour unité"@fr,
        "tem unidade"@pt,
        "имеет единицу"@ru ;
    rdfs:comment "This property shows the type of unit an E54 Dimension was expressed in."@en ;
    rdfs:domain crm:E54_Dimension ;
    rdfs:range crm:E58_Measurement_Unit .

crm:P91i_is_unit_of a rdf:Property ;
    rdfs:label "ist Einheit von"@de,
        "αποτελεί μονάδα μέτρησης του/της"@el,
        "is unit of"@en,
        "est l'unité de"@fr,
        "é unidade de"@pt,
        "является единицей для"@ru ;
    rdfs:domain crm:E58_Measurement_Unit ;
    rdfs:range crm:E54_Dimension .

crm:P95_has_formed a rdf:Property ;
    rdfs:label "hat gebildet"@de,
        "σχημάτισε"@el,
        "has formed"@en,
        "a fondé"@fr,
        "formou"@pt,
        "сформировал"@ru ;
    rdfs:comment "This property links the founding or E66 Formation for an E74 Group with the Group itself."@en ;
    rdfs:domain crm:E66_Formation ;
    rdfs:range crm:E74_Group ;
    rdfs:subPropertyOf crm:P92_brought_into_existence .

crm:P95i_was_formed_by a rdf:Property ;
    rdfs:label "wurde gebildet von"@de,
        "σχηματίστηκε από"@el,
        "was formed by"@en,
        "a été fondé par"@fr,
        "foi formado por"@pt,
        "была сформирована посредством"@ru ;
    rdfs:domain crm:E74_Group ;
    rdfs:range crm:E66_Formation ;
    rdfs:subPropertyOf crm:P92i_was_brought_into_existence_by .

crm:P96_by_mother a rdf:Property ;
    rdfs:label "durch Mutter"@de,
        "είχε μητέρα"@el,
        "by mother"@en,
        "de mère"@fr,
        "pela mãe"@pt,
        "посредством матери"@ru ;
    rdfs:comment """This property links an E67 Birth event to an E21 Person as a participant in the role of birth-giving mother.

Note that biological fathers are not necessarily participants in the Birth (see P97 from father (was father for)). The Person being born is linked to the Birth with the property P98 brought into life (was born). This is not intended for use with general natural history material, only people. There is no explicit method for modelling conception and gestation except by using extensions. This is a sub-property of P11 had participant (participated in)."""@en ;
    rdfs:domain crm:E67_Birth ;
    rdfs:range crm:E21_Person ;
    rdfs:subPropertyOf crm:P11_had_participant .

crm:P96i_gave_birth a rdf:Property ;
    rdfs:label "gebar"@de,
        "ήταν μητέρα του/της"@el,
        "gave birth"@en,
        "a donné naissance à"@fr,
        "deu nascimento"@pt,
        "дал рождение"@ru ;
    rdfs:domain crm:E21_Person ;
    rdfs:range crm:E67_Birth ;
    rdfs:subPropertyOf crm:P11i_participated_in .

crm:P97_from_father a rdf:Property ;
    rdfs:label "gab Vaterschaft"@de,
        "είχε πατέρα"@el,
        "from father"@en,
        "de père"@fr,
        "pelo pai"@pt,
        "от отца"@ru ;
    rdfs:comment """This property links an E67 Birth event to an E21 Person in the role of biological father.
Note that biological fathers are not seen as necessary participants in the Birth, whereas birth-giving mothers are (see P96 by mother (gave birth)). The Person being born is linked to the Birth with the property P98 brought into life (was born).
This is not intended for use with general natural history material, only people. There is no explicit method for modelling conception and gestation except by using extensions. 
A Birth event is normally (but not always) associated with one biological father."""@en ;
    rdfs:domain crm:E67_Birth ;
    rdfs:range crm:E21_Person .

crm:P97i_was_father_for a rdf:Property ;
    rdfs:label "war Vater für"@de,
        "ήταν πατέρας του/της"@el,
        "was father for"@en,
        "a été père dans"@fr,
        "foi pai para"@pt,
        "был отцом для"@ru ;
    rdfs:domain crm:E21_Person ;
    rdfs:range crm:E67_Birth .

crm:P98_brought_into_life a rdf:Property ;
    rdfs:label "brachte zur Welt"@de,
        "έφερε στη ζωή"@el,
        "brought into life"@en,
        "a donné vie à"@fr,
        "trouxe à vida"@pt,
        "породил"@ru ;
    rdfs:comment """This property links an E67Birth event to an E21 Person in the role of offspring.
Twins, triplets etc. are brought into life by the same Birth event. This is not intended for use with general Natural History material, only people. There is no explicit method for modelling conception and gestation except by using extensions."""@en ;
    rdfs:domain crm:E67_Birth ;
    rdfs:range crm:E21_Person ;
    rdfs:subPropertyOf crm:P92_brought_into_existence .

crm:P98i_was_born a rdf:Property ;
    rdfs:label "wurde geboren durch"@de,
        "γεννήθηκε"@el,
        "was born"@en,
        "est né"@fr,
        "veio à vida pelo"@pt,
        "был рожден"@ru ;
    rdfs:domain crm:E21_Person ;
    rdfs:range crm:E67_Birth ;
    rdfs:subPropertyOf crm:P92i_was_brought_into_existence_by .

crm:P99_dissolved a rdf:Property ;
    rdfs:label "löste auf"@de,
        "διέλυσε"@el,
        "dissolved"@en,
        "a dissous"@fr,
        "dissolveu"@pt,
        "распустил"@ru ;
    rdfs:comment "This property links the disbanding or E68 Dissolution of an E74 Group to the Group itself."@en ;
    rdfs:domain crm:E68_Dissolution ;
    rdfs:range crm:E74_Group ;
    rdfs:subPropertyOf crm:P11_had_participant,
        crm:P93_took_out_of_existence .

crm:P99i_was_dissolved_by a rdf:Property ;
    rdfs:label "wurde aufgelöst durch"@de,
        "διαλύθηκε από"@el,
        "was dissolved by"@en,
        "a été dissous par"@fr,
        "foi dissolvido por"@pt,
        "был распущен посредством"@ru ;
    rdfs:domain crm:E74_Group ;
    rdfs:range crm:E68_Dissolution ;
    rdfs:subPropertyOf crm:P11i_participated_in,
        crm:P93i_was_taken_out_of_existence_by .

crm:P9_consists_of a rdf:Property ;
    rdfs:label "setzt sich zusammen aus"@de,
        "αποτελείται από"@el,
        "consists of"@en,
        "consiste en"@fr,
        "consiste de"@pt,
        "состоит из"@ru ;
    rdfs:comment """This property describes the decomposition of an instance of E4 Period into discrete, subsidiary periods.
The sub-periods into which the period is decomposed form a logical whole - although the entire picture may not be completely known - and the sub-periods are constitutive of the general period."""@en ;
    rdfs:domain crm:E4_Period ;
    rdfs:range crm:E4_Period .

crm:P9i_forms_part_of a rdf:Property ;
    rdfs:label "bildet Teil von"@de,
        "αποτελεί μέρος του/της"@el,
        "forms part of"@en,
        "fait partie de"@fr,
        "faz parte de"@pt,
        "формирует часть"@ru ;
    rdfs:domain crm:E4_Period ;
    rdfs:range crm:E4_Period .

<http://www.geonames.org/ontology> a owl:Ontology ;
    ns:license <http://creativecommons.org/licenses/by/3.0/> ;
    dcterms:contributor "Erik Bolstad (norwegian and swedish translations)",
        "Roman Rachkov (bulgarian translation)",
        "Valery Hronusov (russian translation)" ;
    dcterms:creator person:bernard-vatant ;
    dcterms:description "The Geonames ontologies provides elements of description for geographical features, in particular those defined in the geonames.org data base"@en ;
    dcterms:issued "2006-10-14" ;
    dcterms:modified "2012-10-29" ;
    dcterms:publisher resource:GeoNames ;
    dcterms:title "The Geonames ontology"@en ;
    vann:preferredNamespacePrefix "gn" ;
    vann:preferredNamespaceUri "http://www.geonames.org/ontology#" ;
    rdfs:comment """Modifications from version 3.01 :
            Added : gn:GeonamesFeature, subclass of gn:Feature.
            Added : explicit property gn:geonamesID, mandatory and unique for each gn:GeonamesFeature instance.
            Deleted : owl:FunctionalProperty declarations for properties attached to gn:Feature, replaced by local cardinality restrictions on gn:GeonamesFeature
            The gn:Feature class and attached properties can therefore be used in the open world for features not necessarily identified in the Geonames data base, or with partial descriptions.
            Modified : Equivalent classes and superclasses of geonames:Feature in other vocabularies.
            Added : new feature codes for historical features.
            Improved metadata.
      """@en ;
    rdfs:isDefinedBy <http://www.geonames.org/ontology_v3.1.rdf> ;
    owl:priorVersion <http://www.geonames.org/ontology_v3.0.1.rdf> ;
    owl:versionInfo "Version 3.1 - 2012-10-29"@en ;
    ns1:relatedDocumentation <http://www.geonames.org/documentation.html> ;
    foaf:homepage <http://www.geonames.org/documentation.html> .

gn:A.ADM1H a gn:Code ;
    skos:historyNote "Added in v3.1"@en ;
    skos:inScheme gn:A ;
    skos:notation "A.ADM1H" ;
    skos:prefLabel "historical first-order administrative division"@en .

gn:A.ADM2H a gn:Code ;
    skos:historyNote "Added in v3.1"@en ;
    skos:inScheme gn:A ;
    skos:notation "A.ADM2H" ;
    skos:prefLabel "historical second-order administrative division"@en .

gn:A.ADM3H a gn:Code ;
    skos:historyNote "Added in v3.1"@en ;
    skos:inScheme gn:A ;
    skos:notation "A.ADM3H" ;
    skos:prefLabel "historical third-order administrative division"@en .

gn:A.ADM4H a gn:Code ;
    skos:historyNote "Added in v3.1"@en ;
    skos:inScheme gn:A ;
    skos:notation "A.ADM4H" ;
    skos:prefLabel "historical fourth-order administrative division"@en .

gn:A.ADM5 a gn:Code ;
    skos:definition "a subdivision of a fourth-order administrative division"@en ;
    skos:notation "A.ADM5" ;
    skos:prefLabel "fifth-order administrative division"@en .

gn:A.ADMD a gn:Code ;
    skos:definition "an administrative division of a country, undifferentiated as to administrative level"@en,
        "деление страны на административные единицы"@ru ;
    skos:inScheme gn:A ;
    skos:notation "A.ADMD" ;
    skos:prefLabel "административно делене"@bg,
        "administrative division"@en,
        "administrativ inndeling"@no,
        "политико-административное  деление"@ru,
        "administrativ avdelning"@sv .

gn:A.ADMH a gn:Code ;
    skos:historyNote "Added in v3.1"@en ;
    skos:inScheme gn:A ;
    skos:notation "A.ADMH" ;
    skos:prefLabel "historical administrative division"@en .

gn:A.LTER a gn:Code ;
    skos:definition "a tract of land leased to another country, usually for military installations"@en,
        "арендованный правительством Великобритании у властей Китая участок земли, часть Гонконга"@ru ;
    skos:inScheme gn:A ;
    skos:notation "A.LTER" ;
    skos:prefLabel "територия под аренда"@bg,
        "leased area"@en,
        "leid landområde"@no,
        "арендованный район/территория"@ru,
        "uthyrt område"@sv .

gn:A.PCL a gn:Code ;
    skos:inScheme gn:A ;
    skos:notation "A.PCL" ;
    skos:prefLabel "политическо тяло"@bg,
        "political entity"@en,
        "politisk enhet"@no,
        "политическое образование"@ru,
        "politisk enhet"@sv .

gn:A.PCLD a gn:Code ;
    skos:inScheme gn:A ;
    skos:notation "A.PCLD" ;
    skos:prefLabel "зависимо политическо тяло"@bg,
        "dependent political entity"@en,
        "avhengig politisk enhet"@no,
        "зависимое политическое образование"@ru,
        "beroende politisk enhet"@sv .

gn:A.PCLF a gn:Code ;
    skos:inScheme gn:A ;
    skos:notation "A.PCLF" ;
    skos:prefLabel "свободно асоциирана държава"@bg,
        "freely associated state"@en,
        "fritt tilknyttet stat"@no,
        "свободно присоединившееся государство (свободное ассоциированное государство)"@ru,
        "fritt associerad stat"@sv .

gn:A.PCLH a gn:Code ;
    skos:historyNote "Added in v3.1"@en ;
    skos:inScheme gn:A ;
    skos:notation "A.PCLH" ;
    skos:prefLabel "historical political entity"@en .

gn:A.PCLIX a gn:Code ;
    skos:inScheme gn:A ;
    skos:notation "A.PCLIX" ;
    skos:prefLabel "част от независимо политическо образувание"@bg,
        "section of independent political entity"@en,
        "del av uavhengig politisk enhet"@no,
        "участок независимого политического образования"@ru,
        "del av oberoende politisk enhet"@sv .

gn:A.PCLS a gn:Code ;
    skos:inScheme gn:A ;
    skos:notation "A.PCLS" ;
    skos:prefLabel "полу-независимо политическо образувание"@bg,
        "semi-independent political entity"@en,
        "delvis uavhengig politisk enhet"@no,
        "наполовину зависимое политическое образование"@ru,
        "delvis oberoende politisk enhet"@sv .

gn:A.PPCLH a gn:Code ;
    skos:historyNote "Added in v3.1"@en ;
    skos:inScheme gn:P ;
    skos:notation "A.PPCLH" ;
    skos:prefLabel "historical capital of a political entity"@en .

gn:A.PPLH a gn:Code ;
    skos:historyNote "Added in v3.1"@en ;
    skos:inScheme gn:P ;
    skos:notation "A.PPLH" ;
    skos:prefLabel "historical populated place"@en .

gn:A.PRSH a gn:Code ;
    skos:definition "an ecclesiastical district"@en,
        "низший церковный округ в христианской церкви, центром которого является храм"@ru ;
    skos:inScheme gn:A ;
    skos:notation "A.PRSH" ;
    skos:prefLabel "енория"@bg,
        "parish"@en,
        "sogn"@no,
        "церковный приход"@ru,
        "kommun"@sv .

gn:A.TERR a gn:Code ;
    skos:inScheme gn:A ;
    skos:notation "A.TERR" ;
    skos:prefLabel "територия"@bg,
        "territory"@en,
        "territorium"@no,
        "территория (административная единица в США, Канаде и Австралии, не имеющая прав штата или провинции)"@ru,
        "territorium"@sv .

gn:A.ZN a gn:Code ;
    skos:inScheme gn:A ;
    skos:notation "A.ZN" ;
    skos:prefLabel "зона"@bg,
        "zone"@en,
        "sone"@no,
        "зона"@ru,
        "zon"@sv .

gn:A.ZNB a gn:Code ;
    skos:definition "a zone recognized as a buffer between two nations in which military presence is minimal or absent"@en,
        "область, официально признанная в качестве буфера между двумя нациями; военное присутствие минимально или вовсе отсутствует"@ru ;
    skos:inScheme gn:A ;
    skos:notation "A.ZNB" ;
    skos:prefLabel "буферна зона"@bg,
        "buffer zone"@en,
        "buffersone"@no,
        "буферная зона"@ru,
        "bufferzon"@sv .

gn:GeonamesFeature a owl:Class ;
    rdfs:label "Geonames Feature"@en ;
    rdfs:comment "A feature described in geonames database, uniquely defined by its geonames identifier"@en ;
    rdfs:subClassOf [ a owl:Restriction ;
            owl:cardinality "1"^^xsd:nonNegativeInteger ;
            owl:onProperty gn:geonamesID ],
        [ a owl:Restriction ;
            owl:maxCardinality "1"^^xsd:nonNegativeInteger ;
            owl:onProperty gn:parentADM3 ],
        [ a owl:Restriction ;
            owl:maxCardinality "1"^^xsd:nonNegativeInteger ;
            owl:onProperty gn:parentADM4 ],
        [ a owl:Restriction ;
            owl:maxCardinality "1"^^xsd:nonNegativeInteger ;
            owl:onProperty gn:population ],
        [ a owl:Restriction ;
            owl:cardinality "1"^^xsd:nonNegativeInteger ;
            owl:onProperty gn:name ],
        [ a owl:Restriction ;
            owl:cardinality "1"^^xsd:nonNegativeInteger ;
            owl:onProperty wgs84:lat ],
        [ a owl:Restriction ;
            owl:cardinality "1"^^xsd:nonNegativeInteger ;
            owl:onProperty wgs84:long ],
        [ a owl:Restriction ;
            owl:cardinality "1"^^xsd:nonNegativeInteger ;
            owl:onProperty gn:featureClass ],
        [ a owl:Restriction ;
            owl:maxCardinality "1"^^xsd:nonNegativeInteger ;
            owl:onProperty gn:featureCode ],
        [ a owl:Restriction ;
            owl:maxCardinality "1"^^xsd:nonNegativeInteger ;
            owl:onProperty gn:countryCode ],
        [ a owl:Restriction ;
            owl:maxCardinality "1"^^xsd:nonNegativeInteger ;
            owl:onProperty gn:parentADM1 ],
        [ a owl:Restriction ;
            owl:maxCardinality "1"^^xsd:nonNegativeInteger ;
            owl:onProperty gn:parentADM2 ],
        gn:Feature ;
    skos:historyNote "Added in version 3.1"@en .

gn:H.AIRS a gn:Code ;
    skos:definition "a place on a waterbody where floatplanes land and take off"@en,
        "место на воде для взлета и посадки гидросамолета"@ru ;
    skos:inScheme gn:H ;
    skos:notation "H.AIRS" ;
    skos:prefLabel "летище за хидроплани"@bg,
        "seaplane landing area"@en,
        "landingsområde for sjøfly"@no,
        "посадочная полоса для гидросамолета"@ru,
        "landningsplats för sjöflygplan"@sv .

gn:H.ANCH a gn:Code ;
    skos:definition "an area where vessels may anchor"@en,
        "место, где судна бросают якорь"@ru ;
    skos:inScheme gn:H ;
    skos:notation "H.ANCH" ;
    skos:prefLabel "пристанище"@bg,
        "anchorage"@en,
        "ankerplass"@no,
        "якорная стоянка"@ru,
        "ankarplats"@sv .

gn:H.BAY a gn:Code ;
    skos:definition "a coastal indentation between two capes or headlands, larger than a cove but smaller than a gulf"@en,
        "изгиб берега  между двумя мысами, больше чем открытая гавань, но меньше чем залив"@ru ;
    skos:inScheme gn:H ;
    skos:notation "H.BAY" ;
    skos:prefLabel "залив"@bg,
        "bay"@en,
        "bukt"@no,
        "бухта"@ru,
        "vik, bukt"@sv .

gn:H.BAYS a gn:Code ;
    skos:definition "coastal indentations between two capes or headlands, larger than a cove but smaller than a gulf"@en,
        "изгибы берега  между двумя мысами, больше чем открытая гавань, но меньше чем залив"@ru ;
    skos:inScheme gn:H ;
    skos:notation "H.BAYS" ;
    skos:prefLabel "заливи"@bg,
        "bays"@en,
        "bukter"@no,
        "бухты"@ru,
        "vikar, bukter"@sv .

gn:H.BGHT a gn:Code ;
    skos:definition "an open body of water forming a slight recession in a coastline"@en,
        "открытый участок воды; там, где происходит отступание береговой черты"@ru ;
    skos:inScheme gn:H ;
    skos:notation "H.BGHT" ;
    skos:prefLabel "ивица(и)"@bg,
        "bight(s)"@en,
        "vik"@no,
        "излучина (реки)"@ru,
        "bukt(er)"@sv .

gn:H.BNK a gn:Code ;
    skos:definition "an elevation, typically located on a shelf, over which the depth of water is relatively shallow but sufficient for most surface navigation"@en,
        "возвышенность, которая обычно располагается на мелководье; однако количества воды достаточно для надводного судоходства"@ru ;
    skos:inScheme gn:H ;
    skos:notation "H.BNK" ;
    skos:prefLabel "бряг(ове)"@bg,
        "bank(s)"@en,
        "banker"@no,
        "нанос"@ru,
        "strandssluttning, strandvall"@sv .

gn:H.BNKR a gn:Code ;
    skos:definition "a sloping margin of a stream channel which normally confines the stream to its channel on land"@en,
        "косой берег реки, который удерживает поток воды в своих границах"@ru ;
    skos:inScheme gn:H ;
    skos:notation "H.BNKR" ;
    skos:prefLabel "бряг изложен на течение"@bg,
        "stream bank"@en,
        "elvebredd"@no,
        "речной берег"@ru,
        "flodstrand"@sv .

gn:H.BNKX a gn:Code ;
    skos:inScheme gn:H ;
    skos:notation "H.BNKX" ;
    skos:prefLabel "част от бряг"@bg,
        "section of bank"@en,
        "del av bredd"@no,
        "участок берега"@ru,
        "del av flodstrand"@sv .

gn:H.BOG a gn:Code ;
    skos:definition "a wetland characterized by peat forming sphagnum moss, sedge, and other acid-water plants"@en,
        "заболоченная территория, которая является благоприятной почвой для торфяного мха, осоки и других болотных растений"@ru ;
    skos:inScheme gn:H ;
    skos:notation "H.BOG" ;
    skos:prefLabel "блато(а)"@bg,
        "bog(s)"@en,
        "myr"@no,
        "болото"@ru,
        "kärr, träsk"@sv .

gn:H.CAPG a gn:Code ;
    skos:definition "a dome-shaped mass of glacial ice covering an area of  mountain summits or other high lands; smaller than an ice sheet"@en,
        "куполообразная масса ледникового льда, покрывающая гонные вершины; по размеру меньше ледникового щита"@ru ;
    skos:inScheme gn:H ;
    skos:notation "H.CAPG" ;
    skos:prefLabel "ледена покривка"@bg,
        "icecap"@en,
        "iskappe"@no,
        "шапка полярного льда"@ru,
        "iskalott"@sv .

gn:H.CHN a gn:Code ;
    skos:definition "the deepest part of a stream, bay, lagoon, or strait, through which the main current flows"@en,
        "самый глубоки участок реки, пролива, залива, лагуны; через него проходит основной поток воды"@ru ;
    skos:inScheme gn:H ;
    skos:notation "H.CHN" ;
    skos:prefLabel "канал"@bg,
        "channel"@en,
        "kanal"@no,
        "русло"@ru,
        "kanal"@sv .

gn:H.CHNL a gn:Code ;
    skos:definition "that part of a lake having water deep enough for navigation between islands, shoals, etc."@en,
        "наиболее глубокое место в озере; здесь могут проходить суда"@ru ;
    skos:inScheme gn:H ;
    skos:notation "H.CHNL" ;
    skos:prefLabel "езерен канал(и)"@bg,
        "lake channel(s)"@en,
        "seilingskanal i innsjø"@no,
        "омут"@ru,
        "sjökanal(er)"@sv .

gn:H.CHNM a gn:Code ;
    skos:definition "that part of a body of water deep enough for navigation through an area otherwise not suitable"@en,
        "канал, предназначенный для судоходной связи между морями"@ru ;
    skos:inScheme gn:H ;
    skos:notation "H.CHNM" ;
    skos:prefLabel "морски канал"@bg,
        "marine channel"@en,
        "skipsled på sjøen"@no,
        "морской канал"@ru,
        "marinkanal"@sv .

gn:H.CHNN a gn:Code ;
    skos:definition "a buoyed channel of sufficient depth for the safe navigation of vessels"@en,
        "огражденный буями пролив, достаточно глубокий для безопасного судоходства"@ru ;
    skos:inScheme gn:H ;
    skos:notation "H.CHNN" ;
    skos:prefLabel "навигационен канал"@bg,
        "navigation channel"@en,
        "merket skipsled"@no,
        "судоходное русло"@ru,
        "navigeringskanal"@sv .

gn:H.CNFL a gn:Code ;
    skos:definition "a place where two or more streams or intermittent streams flow together"@en,
        "место, где две (или больше) реки соединяются в одну"@ru ;
    skos:inScheme gn:H ;
    skos:notation "H.CNFL" ;
    skos:prefLabel "устие"@bg,
        "confluence"@en,
        "sammenløp"@no,
        "место слияние (рек)"@ru,
        "sammanflöde"@sv .

gn:H.CNL a gn:Code ;
    skos:definition "an artificial watercourse"@en,
        "искусственная река"@ru ;
    skos:inScheme gn:H ;
    skos:notation "H.CNL" ;
    skos:prefLabel "канал"@bg,
        "canal"@en,
        "kanal"@no,
        "канал"@ru,
        "kanal"@sv .

gn:H.CNLA a gn:Code ;
    skos:definition "a conduit used to carry water"@en,
        "трубопровод, используемый для передачи воды"@ru ;
    skos:inScheme gn:H ;
    skos:notation "H.CNLA" ;
    skos:prefLabel "аквадукт"@bg,
        "aqueduct"@en,
        "akvedukt"@no,
        "акведук/водопровод"@ru,
        "akvedukt"@sv .

gn:H.CNLB a gn:Code ;
    skos:definition "a conspicuously curved or bent section of a canal"@en,
        "изогнутый участок канала"@ru ;
    skos:inScheme gn:H ;
    skos:notation "H.CNLB" ;
    skos:prefLabel "канална връзка"@bg,
        "canal bend"@en,
        "kanalsving"@no,
        "излучина канала"@ru,
        "kanalkrök"@sv .

gn:H.CNLD a gn:Code ;
    skos:definition "an artificial waterway carrying water away from a wetland or from drainage ditches"@en,
        "искусственный судоходный канал, забирает лишнюю воду  либо в заболоченной местности, либо из дренажного канала"@ru ;
    skos:inScheme gn:H ;
    skos:notation "H.CNLD" ;
    skos:prefLabel "отводнителен канал"@bg,
        "drainage canal"@en,
        "dreneringskanal"@no,
        "водоотводный канал"@ru,
        "dräneringskanal"@sv .

gn:H.CNLI a gn:Code ;
    skos:definition "a canal which serves as a main conduit for irrigation water"@en,
        "канал, который служит главным средством передачи воды для орошения"@ru ;
    skos:inScheme gn:H ;
    skos:notation "H.CNLI" ;
    skos:prefLabel "напоителен канал"@bg,
        "irrigation canal"@en,
        "vanningskanal"@no,
        "оросительный канал"@ru,
        "bevattningskanal"@sv .

gn:H.CNLN a gn:Code ;
    skos:definition "a watercourse constructed for navigation of vessels"@en,
        "канал, предназначенный для судоходства"@ru ;
    skos:inScheme gn:H ;
    skos:notation "H.CNLN" ;
    skos:prefLabel "навигационен канал(и)"@bg,
        "navigation canal(s)"@en,
        "seilingskanal"@no,
        "судоходный канал"@ru,
        "navigeringskanaler"@sv .

gn:H.CNLQ a gn:Code ;
    skos:inScheme gn:H ;
    skos:notation "H.CNLQ" ;
    skos:prefLabel "изоставен канал"@bg,
        "abandoned canal"@en,
        "nedlagt kanal"@no,
        "заброшенный канал"@ru,
        "övergiven kanal"@sv .

gn:H.CNLSB a gn:Code ;
    skos:definition "a gently inclined underground tunnel bringing water for irrigation from aquifers"@en,
        "подземный туннель, по которому течет вода, используемая  для орошения; вода берется из водоносного слоя почвы"@ru ;
    skos:inScheme gn:H ;
    skos:notation "H.CNLSB" ;
    skos:prefLabel "подземна напоителна система"@bg,
        "underground irrigation canal(s)"@en,
        "underjordisk vanningskanal"@no,
        "подземный оросительный канал"@ru,
        "underjordisk bevattningskanal(er)"@sv .

gn:H.CNLX a gn:Code ;
    skos:inScheme gn:H ;
    skos:notation "H.CNLX" ;
    skos:prefLabel "част от канал"@bg,
        "section of canal"@en,
        "del av kanal"@no,
        "сечение канала"@ru,
        "del av kanal"@sv .

gn:H.COVE a gn:Code ;
    skos:definition "a small coastal indentation, smaller than a bay"@en,
        "защищённое, закрытое место в скалах на морском берегу"@ru ;
    skos:inScheme gn:H ;
    skos:notation "H.COVE" ;
    skos:prefLabel "заливче"@bg,
        "cove(s)"@en,
        "kil"@no,
        "прибойная пещера"@ru,
        "liten vik"@sv .

gn:H.CRKT a gn:Code ;
    skos:definition "a meandering channel in a coastal wetland subject to bi-directional tidal currents"@en,
        "извилистый канал на прибрежной заболоченной территории, по которому идет двустороннее приливное течение"@ru ;
    skos:inScheme gn:H ;
    skos:notation "H.CRKT" ;
    skos:prefLabel "приливно заливче"@bg,
        "tidal creek(s)"@en,
        "tidevannselv"@no,
        "небольшой временный водоток (связанный с приливами и отливами)"@ru,
        "tidvattensvik(ar)"@sv .

gn:H.CRNT a gn:Code ;
    skos:definition "a horizontal flow of water in a given direction with uniform velocity"@en,
        "горизонтальный поток воды в заданном направлении с одинаковой скоростью"@ru ;
    skos:inScheme gn:H ;
    skos:notation "H.CRNT" ;
    skos:prefLabel "течение"@bg,
        "current"@en,
        "strøm"@no,
        "течение"@ru,
        "ström, strömning"@sv .

gn:H.CUTF a gn:Code ;
    skos:definition "a channel formed as a result of a stream cutting through a meander neck"@en,
        "канал, образованный в результате потока воды, идущей  через шейку меандра"@ru ;
    skos:inScheme gn:H ;
    skos:notation "H.CUTF" ;
    skos:prefLabel "скъсяване"@bg,
        "cutoff"@en,
        "avskåret"@no,
        "обводной канал"@ru,
        "cutoff"@sv .

gn:H.DCK a gn:Code ;
    skos:definition "a waterway between two piers, or cut into the land for the berthing of ships"@en,
        "портовое сооружение для ремонта и постройки судов."@ru ;
    skos:inScheme gn:H ;
    skos:notation "H.DCK" ;
    skos:prefLabel "пристанище(а)"@bg,
        "dock(s)"@en,
        "dokk"@no,
        "док"@ru,
        "skeppsdocka"@sv .

gn:H.DCKB a gn:Code ;
    skos:definition "a part of a harbor where ships dock"@en,
        "часть гавани, предназначенная для стоянки судов"@ru ;
    skos:inScheme gn:H ;
    skos:notation "H.DCKB" ;
    skos:prefLabel "басейнов док"@bg,
        "docking basin"@en,
        "havnebasseng"@no,
        "портовый бассейн"@ru,
        "fartygsdocka"@sv .

gn:H.DOMG a gn:Code ;
    skos:definition "a comparatively elevated area on an icecap"@en,
        "небольшая возвышенность на поверхности ледника"@ru ;
    skos:inScheme gn:H ;
    skos:notation "H.DOMG" ;
    skos:prefLabel "ледено покритие"@bg,
        "icecap dome"@en,
        "iskuppel"@no,
        "ледниковый купол"@ru,
        "välvd iskalott"@sv .

gn:H.DPRG a gn:Code ;
    skos:definition "a comparatively depressed area on an icecap"@en,
        "небольшое углубление на поверхности ледника"@ru ;
    skos:inScheme gn:H ;
    skos:notation "H.DPRG" ;
    skos:prefLabel "заледена падина"@bg,
        "icecap depression"@en,
        "fordypning i iskappen"@no,
        "ледниковая впадина"@ru,
        "sänka i iskalott"@sv .

gn:H.DTCH a gn:Code ;
    skos:definition "a small artificial watercourse dug for draining or irrigating the land"@en,
        "небольшой искусственный водоем, используемый для осушения и орошения территории"@ru ;
    skos:inScheme gn:H ;
    skos:notation "H.DTCH" ;
    skos:prefLabel "канавка"@bg,
        "ditch"@en,
        "grøft"@no,
        "канава"@ru,
        "dike"@sv .

gn:H.DTCHD a gn:Code ;
    skos:definition "a ditch which serves to drain the land"@en,
        "канава, используемая для осушения территории"@ru ;
    skos:inScheme gn:H ;
    skos:notation "H.DTCHD" ;
    skos:prefLabel "отводнителна канавка"@bg,
        "drainage ditch"@en,
        "dreneringsgrøft"@no,
        "водоотводная канава"@ru,
        "dräneringsdike"@sv .

gn:H.DTCHI a gn:Code ;
    skos:definition "a ditch which serves to distribute irrigation water"@en,
        "канава, используемая для орошения почвы"@ru ;
    skos:inScheme gn:H ;
    skos:notation "H.DTCHI" ;
    skos:prefLabel "напоителна канавка"@bg,
        "irrigation ditch"@en,
        "vanningsgrøft"@no,
        "оросительная канава"@ru,
        "bevattningsdike"@sv .

gn:H.DTCHM a gn:Code ;
    skos:definition "an area where a drainage ditch enters a lagoon, lake or bay"@en,
        "место, где осушительный канал впадает в лагуну, озеро или залив"@ru ;
    skos:inScheme gn:H ;
    skos:notation "H.DTCHM" ;
    skos:prefLabel "заустване на канавка"@bg,
        "ditch mouth(s)"@en,
        "grøfteutløp"@no,
        "устье канала"@ru,
        "dikesmynning"@sv .

gn:H.ESTY a gn:Code ;
    skos:definition "a funnel-shaped stream mouth or embayment where fresh water mixes with sea water under tidal influences"@en,
        "однорукавное, воронкообразное устье реки, расширяющееся в сторону моря"@ru ;
    skos:inScheme gn:H ;
    skos:notation "H.ESTY" ;
    skos:prefLabel "заливно устие"@bg,
        "estuary"@en,
        "elvemunning"@no,
        "эстуарий"@ru,
        "flodmynning"@sv .

gn:H.FISH a gn:Code ;
    skos:definition "a fishing ground, bank or area where fishermen go to catch fish"@en,
        "место ловли рыбы"@ru ;
    skos:inScheme gn:H ;
    skos:notation "H.FISH" ;
    skos:prefLabel "риболовен район"@bg,
        "fishing area"@en,
        "fiskeområde"@no,
        "рыболовная зона"@ru,
        "fiskeområde"@sv .

gn:H.FJD a gn:Code ;
    skos:definition "a long, narrow, steep-walled, deep-water arm of the sea at high latitudes, usually along mountainous coasts"@en,
        "узкий, длинный, глубоководный морской залив с крутыми берегами; берега фьорда  в большинстве случаев образованы высокими скалами"@ru ;
    skos:inScheme gn:H ;
    skos:notation "H.FJD" ;
    skos:prefLabel "фиорд"@bg,
        "fjord"@en,
        "fjord"@no,
        "фьорд"@ru,
        "fjord"@sv .

gn:H.FJDS a gn:Code ;
    skos:definition "long, narrow, steep-walled, deep-water arms of the sea at high latitudes, usually along mountainous coasts"@en,
        "узкие, длинные, глубоководные морские заливы с крутыми берегами"@ru ;
    skos:inScheme gn:H ;
    skos:notation "H.FJDS" ;
    skos:prefLabel "фиорди"@bg,
        "fjords"@en,
        "fjorder"@no,
        "фьорды"@ru,
        "fjordar"@sv .

gn:H.FLLS a gn:Code ;
    skos:definition "a perpendicular or very steep descent of the water of a stream"@en,
        "падение воды в реке с уступа, пересекающего речное русло"@ru ;
    skos:inScheme gn:H ;
    skos:notation "H.FLLS" ;
    skos:prefLabel "водопад(и)"@bg,
        "waterfall(s)"@en,
        "foss"@no,
        "водопад"@ru,
        "vattenfall"@sv .

gn:H.FLLSX a gn:Code ;
    skos:inScheme gn:H ;
    skos:notation "H.FLLSX" ;
    skos:prefLabel "част от водопад(и)"@bg,
        "section of waterfall(s)"@en,
        "del av foss"@no,
        "участок водопада"@ru,
        "del av vattenfall"@sv .

gn:H.FLTM a gn:Code ;
    skos:definition "a relatively level area of mud either between high and low tide lines, or subject to flooding"@en,
        "средних размеров площадь илистого грунта, занимает промежуточное место между высокой и низкой границами прилива, подвергается затоплению"@ru ;
    skos:inScheme gn:H ;
    skos:notation "H.FLTM" ;
    skos:prefLabel "тинесто мочурище(а)"@bg,
        "mud flat(s)"@en,
        "slamområde"@no,
        "топь"@ru,
        "mud flat(s)"@sv .

gn:H.FLTT a gn:Code ;
    skos:definition "a large flat area of mud or sand attached to the shore and alternately covered and uncovered by the tide"@en,
        "береговая полоса, покрываемая водой при приливе"@ru ;
    skos:inScheme gn:H ;
    skos:notation "H.FLTT" ;
    skos:prefLabel "заливно мочурище(а)"@bg,
        "tidal flat(s)"@en,
        "tidevannsområde"@no,
        "приливно-отливная отмель"@ru,
        "tidal flat(s)"@sv .

gn:H.GLCR a gn:Code ;
    skos:definition "a mass of ice, usually at high latitudes or high elevations, with sufficient thickness to flow away from the source area in lobes, tongues, or masses"@en,
        "масса льда преимущественно атмосферного происхождения, испытывающая вязкопластическое течение под действием силы тяжести и принявшая форму потока, системы потоков, купола (щита) или плавучей плиты"@ru ;
    skos:inScheme gn:H ;
    skos:notation "H.GLCR" ;
    skos:prefLabel "ледник"@bg,
        "glacier(s)"@en,
        "isbre"@no,
        "ледник"@ru,
        "glaciär(er)"@sv .

gn:H.GULF a gn:Code ;
    skos:definition "a large recess in the coastline, larger than a bay"@en,
        "вдавшаяся в сушу часть моря"@ru ;
    skos:inScheme gn:H ;
    skos:notation "H.GULF" ;
    skos:prefLabel "залив"@bg,
        "gulf"@en,
        "golf"@no,
        "морской залив"@ru,
        "golf, bukt"@sv .

gn:H.GYSR a gn:Code ;
    skos:definition "a type of hot spring with intermittent eruptions of jets of hot water and steam"@en,
        "источник вулканического происхождения, выбрасывающий через определённые промежутки времени фонтаны горячей воды и пара"@ru ;
    skos:inScheme gn:H ;
    skos:notation "H.GYSR" ;
    skos:prefLabel "гейзер"@bg,
        "geyser"@en,
        "geysir"@no,
        "гейзер"@ru,
        "geyser"@sv .

gn:H.HBR a gn:Code ;
    skos:definition "a haven or space of deep water so sheltered by the adjacent land as to afford a safe anchorage for ships"@en,
        "естественная или искусственная защищенная от ветра и волн прибрежная часть водного пространства, служащая местом стоянки, причала и ремонта судов"@ru ;
    skos:inScheme gn:H ;
    skos:notation "H.HBR" ;
    skos:prefLabel "пристанище(а)"@bg,
        "harbor(s)"@en,
        "havn"@no,
        "гавань"@ru,
        "hamn(ar)"@sv .

gn:H.HBRX a gn:Code ;
    skos:inScheme gn:H ;
    skos:notation "H.HBRX" ;
    skos:prefLabel "част от пристанище"@bg,
        "section of harbor"@en,
        "del av havn"@no,
        "участок гавани"@ru,
        "del av hamn"@sv .

gn:H.INLT a gn:Code ;
    skos:definition "a narrow waterway extending into the land, or connecting a bay or lagoon with a larger body of water"@en,
        "узкий водный путь, простирающийся до суши; или связывающий бухту или лагуну с большим водным образованием"@ru ;
    skos:inScheme gn:H ;
    skos:notation "H.INLT" ;
    skos:prefLabel "проток"@bg,
        "inlet"@en,
        "innløp"@no,
        "узкий пролив"@ru,
        "vik, sund"@sv .

gn:H.INLTQ a gn:Code ;
    skos:definition "an inlet which has been filled in, or blocked by deposits"@en,
        "узкий пролив, который ранее был пригоден для судоходства, в настоящее время пролив засыпан"@ru ;
    skos:inScheme gn:H ;
    skos:notation "H.INLTQ" ;
    skos:prefLabel "бивш проток"@bg,
        "former inlet"@en,
        "tidligere innløp"@no,
        "засыпанный узкий пролив"@ru,
        "tidigare vik"@sv .

gn:H.LBED a gn:Code ;
    skos:definition "a dried up or drained area of a former lake"@en,
        "место, которое осталось после высохшего или специально осушенного озера"@ru ;
    skos:inScheme gn:H ;
    skos:notation "H.LBED" ;
    skos:prefLabel "легло на езеро(а)"@bg,
        "lake bed(s)"@en,
        "gammel innsjøbunn"@no,
        "озерная котловина"@ru,
        "sjöbotten"@sv .

gn:H.LGN a gn:Code ;
    skos:definition "a shallow coastal waterbody, completely or partly separated from a larger body of water by a barrier island, coral reef or other depositional feature"@en,
        "мелководный залив или озеро, отделившиеся от моря вследствие образования песчаной полосы"@ru ;
    skos:inScheme gn:H ;
    skos:notation "H.LGN" ;
    skos:prefLabel "лагуна"@bg,
        "lagoon"@en,
        "lagune"@no,
        "лагуна"@ru,
        "lagun"@sv .

gn:H.LGNS a gn:Code ;
    skos:definition "shallow coastal waterbodies, completely or partly separated from a larger body of water by a barrier island, coral reef or other depositional feature"@en,
        "мелководные заливы или озеро, отделившиеся от моря вследствие образования песчаной полосы"@ru ;
    skos:inScheme gn:H ;
    skos:notation "H.LGNS" ;
    skos:prefLabel "лагуни"@bg,
        "lagoons"@en,
        "laguner"@no,
        "лагуны"@ru,
        "laguner"@sv .

gn:H.LGNX a gn:Code ;
    skos:inScheme gn:H ;
    skos:notation "H.LGNX" ;
    skos:prefLabel "част от кагуна"@bg,
        "section of lagoon"@en,
        "del av lagune"@no,
        "участок лагуны"@ru,
        "del av lagun"@sv .

gn:H.LK a gn:Code ;
    skos:definition "a large inland body of standing water"@en,
        "замкнутый естественный водоём в углублении суши, котловине"@ru ;
    skos:inScheme gn:H ;
    skos:notation "H.LK" ;
    skos:prefLabel "езеро"@bg,
        "lake"@en,
        "innsjø"@no,
        "озеро"@ru,
        "sjö"@sv .

gn:H.LKC a gn:Code ;
    skos:definition "a lake in a crater or caldera"@en,
        "озеро в кратере или кальдере (круглое или овальное углубление в жерле вулкана)"@ru ;
    skos:inScheme gn:H ;
    skos:notation "H.LKC" ;
    skos:prefLabel "вулканично езеро"@bg,
        "crater lake"@en,
        "kratersjø"@no,
        "кратерное озеро"@ru,
        "kratersjö"@sv .

gn:H.LKI a gn:Code ;
    skos:inScheme gn:H ;
    skos:notation "H.LKI" ;
    skos:prefLabel "пресъхващо езеро"@bg,
        "intermittent lake"@en,
        "tilbakevendende innsjø"@no,
        "временно исчезающее озеро"@ru,
        "periodisk sjö"@sv .

gn:H.LKN a gn:Code ;
    skos:definition "an inland body of salt water with no outlet"@en,
        "озеро, вода которого сильно минерализована; содержит большое количество солей"@ru ;
    skos:inScheme gn:H ;
    skos:notation "H.LKN" ;
    skos:prefLabel "солено езеро"@bg,
        "salt lake"@en,
        "saltsjø"@no,
        "соленое озеро"@ru,
        "saltsjö"@sv .

gn:H.LKNI a gn:Code ;
    skos:inScheme gn:H ;
    skos:notation "H.LKNI" ;
    skos:prefLabel "пресъхващо солено езеро"@bg,
        "intermittent salt lake"@en,
        "tilbakevendende saltsjø"@no,
        "временно исчезающее соленое озеро"@ru,
        "periodisk saltsjö"@sv .

gn:H.LKO a gn:Code ;
    skos:definition "a crescent-shaped lake commonly found adjacent to meandering streams"@en,
        "серповидное озеро, прилегающее  к извилистым рекам"@ru ;
    skos:inScheme gn:H ;
    skos:notation "H.LKO" ;
    skos:prefLabel "корекция"@bg,
        "oxbow lake"@en,
        "kroksjø"@no,
        "пойменное озеро"@ru,
        "uformad sjö"@sv .

gn:H.LKOI a gn:Code ;
    skos:inScheme gn:H ;
    skos:notation "H.LKOI" ;
    skos:prefLabel "пресъхващи корекции"@bg,
        "intermittent oxbow lake"@en,
        "tilbakevendende kroksjø"@no,
        "временно исчезающее пойменное озеро"@ru,
        "peridodisk uformad sjö"@sv .

gn:H.LKS a gn:Code ;
    skos:definition "large inland bodies of standing water"@en,
        "замкнутые естественные водоёмы в углублении суши, котловине"@ru ;
    skos:inScheme gn:H ;
    skos:notation "H.LKS" ;
    skos:prefLabel "езера"@bg,
        "lakes"@en,
        "innsjøer"@no,
        "озера"@ru,
        "sjöar"@sv .

gn:H.LKSB a gn:Code ;
    skos:definition "a standing body of water in a cave"@en,
        "озеро в карстовых пещерах, питающееся подземными водами"@ru ;
    skos:inScheme gn:H ;
    skos:notation "H.LKSB" ;
    skos:prefLabel "подземни езера"@bg,
        "underground lake"@en,
        "underjordisk innsjø"@no,
        "подземное озеро"@ru,
        "underjordisk sjö"@sv .

gn:H.LKSC a gn:Code ;
    skos:definition "lakes in a crater or caldera"@en,
        "озера в кратере или кальдере (круглое или овальное углубление в жерле вулкана)"@ru ;
    skos:inScheme gn:H ;
    skos:notation "H.LKSC" ;
    skos:prefLabel "вулканични езера"@bg,
        "crater lakes"@en,
        "kratersjøer"@no,
        "кратерные озера"@ru,
        "kratersjöar"@sv .

gn:H.LKSI a gn:Code ;
    skos:inScheme gn:H ;
    skos:notation "H.LKSI" ;
    skos:prefLabel "пресъхващи езера"@bg,
        "intermittent lakes"@en,
        "tilbakevendende innsjøer"@no,
        "исчезающие озера"@ru,
        "periodiska sjöar"@sv .

gn:H.LKSN a gn:Code ;
    skos:definition "inland bodies of salt water with no outlet"@en,
        "озера, вода которых сильно минерализована; содержит большое количество солей"@ru ;
    skos:inScheme gn:H ;
    skos:notation "H.LKSN" ;
    skos:prefLabel "солени езера"@bg,
        "salt lakes"@en,
        "saltsjøer"@no,
        "соленые озера"@ru,
        "saltsjöar"@sv .

gn:H.LKSNI a gn:Code ;
    skos:inScheme gn:H ;
    skos:notation "H.LKSNI" ;
    skos:prefLabel "пресъхващи солени езера"@bg,
        "intermittent salt lakes"@en,
        "tilbakevendende saltsjøer"@no,
        "исчезающие соленые озера"@ru,
        "periodiska saltsjöar"@sv .

gn:H.LKX a gn:Code ;
    skos:inScheme gn:H ;
    skos:notation "H.LKX" ;
    skos:prefLabel "част от езеро"@bg,
        "section of lake"@en,
        "del av innsjø"@no,
        "участок озера"@ru,
        "del av sjö"@sv .

gn:H.MFGN a gn:Code ;
    skos:definition "diked salt ponds used in the production of solar evaporated salt"@en,
        "обвалованный соленые пруды, используемые в производстве  выварочной соли"@ru ;
    skos:inScheme gn:H ;
    skos:notation "H.MFGN" ;
    skos:prefLabel "солено испаряващо се езерце"@bg,
        "salt evaporation ponds"@en,
        "saltutvinningsbasseng"@no,
        "соленый испарительный пруд"@ru,
        "saltdammar"@sv .

gn:H.MGV a gn:Code ;
    skos:definition "a tropical tidal mud flat characterized by mangrove vegetation"@en,
        "связанная с приливами и отливами, тропическая, илистая, равнинная местность, на которой произрастают мангровые растения"@ru ;
    skos:inScheme gn:H ;
    skos:notation "H.MGV" ;
    skos:prefLabel "мангрови блата"@bg,
        "mangrove swamp"@en,
        "mangrovesump"@no,
        "мангровое болото"@ru,
        "mangroveträsk"@sv .

gn:H.MOOR a gn:Code ;
    skos:definition "an area of open ground overlaid with wet peaty soils"@en,
        "залежи торфа, торфяное болото"@ru ;
    skos:inScheme gn:H ;
    skos:notation "H.MOOR" ;
    skos:prefLabel "тресавище(а)"@bg,
        "moor(s)"@en,
        "mo"@no,
        "торфяник"@ru,
        "hed(ar)"@sv .

gn:H.MRSH a gn:Code ;
    skos:definition "a wetland dominated by grass-like vegetation"@en,
        "заболоченная территория, заросшая травой"@ru ;
    skos:inScheme gn:H ;
    skos:notation "H.MRSH" ;
    skos:prefLabel "мочурище(а)"@bg,
        "marsh(es)"@en,
        "myr"@no,
        "травяное болото"@ru,
        "moras, sumpmark"@sv .

gn:H.MRSHN a gn:Code ;
    skos:definition "a flat area, subject to periodic salt water inundation, dominated by grassy salt-tolerant plants"@en,
        "равнинная местность, подверженная затоплению соленой водой; здесь произрастают преимущественно травянистые солеустойчивые растения"@ru ;
    skos:inScheme gn:H ;
    skos:notation "H.MRSHN" ;
    skos:prefLabel "солени мочурища"@bg,
        "salt marsh"@en,
        "marskland"@no,
        "соленое травяное болото"@ru,
        "salt sumpmark"@sv .

gn:H.NRWS a gn:Code ;
    skos:definition "a navigable narrow part of a bay, strait, river, etc."@en,
        "район водной поверхности, доступный для плавания по ширине и по глубинам, но стесняющий свободное маневрирование из-за близости берегов, рифов, отмелей и кос"@ru ;
    skos:inScheme gn:H ;
    skos:notation "H.NRWS" ;
    skos:prefLabel "тясна част на протоци"@bg,
        "narrows"@en,
        "smale sund"@no,
        "узкости"@ru,
        "trångt sund"@sv .

gn:H.OCN a gn:Code ;
    skos:definition "one of the major divisions of the vast expanse of salt water covering part of the earth"@en,
        "непрерывная водная оболочка Земли, окружающая материки и острова и обладающая общностью солевого состава"@ru ;
    skos:inScheme gn:H ;
    skos:notation "H.OCN" ;
    skos:prefLabel "океан"@bg,
        "ocean"@en,
        "hav"@no,
        "океан"@ru,
        "hav"@sv .

gn:H.OVF a gn:Code ;
    skos:definition "an area of breaking waves caused by the meeting of currents or by waves moving against the current"@en,
        "круговращательное движение воды, происходящее от столкновения встречных течений"@ru ;
    skos:inScheme gn:H ;
    skos:notation "H.OVF" ;
    skos:prefLabel "бързеи"@bg,
        "overfalls"@en,
        "brenninger"@no,
        "водоворот"@ru,
        "vattenfall"@sv .

gn:H.PND a gn:Code ;
    skos:definition "a small standing waterbody"@en,
        "небольшой водоем со стоячей водой"@ru ;
    skos:inScheme gn:H ;
    skos:notation "H.PND" ;
    skos:prefLabel "поток"@bg,
        "pond"@en,
        "tjern"@no,
        "пруд"@ru,
        "damm"@sv .

gn:H.PNDI a gn:Code ;
    skos:inScheme gn:H ;
    skos:notation "H.PNDI" ;
    skos:prefLabel "пресъхващ поток"@bg,
        "intermittent pond"@en,
        "tilbakevendende tjern"@no,
        "временно исчезающий пруд"@ru,
        "periodisk damm"@sv .

gn:H.PNDN a gn:Code ;
    skos:definition "a small standing body of salt water often in a marsh or swamp, usually along a seacoast"@en,
        "небольшой водоем с соленой водой, обычно в болотистой местности, или вдоль морского побережья"@ru ;
    skos:inScheme gn:H ;
    skos:notation "H.PNDN" ;
    skos:prefLabel "солено езерце"@bg,
        "salt pond"@en,
        "saltvannsdam"@no,
        "соленый пруд"@ru,
        "saltdamm"@sv .

gn:H.PNDNI a gn:Code ;
    skos:inScheme gn:H ;
    skos:notation "H.PNDNI" ;
    skos:prefLabel "пресъхващо солено езерце(а)"@bg,
        "intermittent salt pond(s)"@en,
        "tilbakevendende saltvannsdam"@no,
        "временно исчезающий соленый пруд"@ru,
        "periodiska saltdammar"@sv .

gn:H.PNDS a gn:Code ;
    skos:definition "small standing waterbodies"@en,
        "небольшие водоемы со стоячей водой"@ru ;
    skos:inScheme gn:H ;
    skos:notation "H.PNDS" ;
    skos:prefLabel "езерца"@bg,
        "ponds"@en,
        "dammer"@no,
        "пруды"@ru,
        "dammar"@sv .

gn:H.PNDSF a gn:Code ;
    skos:definition "ponds or enclosures in which fish are kept or raised"@en,
        "специальный искусственный водоем, в котором разводят рыб"@ru ;
    skos:inScheme gn:H ;
    skos:notation "H.PNDSF" ;
    skos:prefLabel "рибарник"@bg,
        "fishponds"@en,
        "fiskedammer"@no,
        "пруд для разведения рыб"@ru,
        "fiskdammar"@sv .

gn:H.PNDSI a gn:Code ;
    skos:inScheme gn:H ;
    skos:notation "H.PNDSI" ;
    skos:prefLabel "пресъхващи езерца"@bg,
        "intermittent ponds"@en,
        "tilbakevendende dammer"@no,
        "временно исчезающие пруды"@ru,
        "periodiska dammar"@sv .

gn:H.PNDSN a gn:Code ;
    skos:definition "small standing bodies of salt water often in a marsh or swamp, usually along a seacoast"@en,
        "небольшие водоемы с соленой водой, обычно в болотистой местности, или вдоль морского побережья"@ru ;
    skos:inScheme gn:H ;
    skos:notation "H.PNDSN" ;
    skos:prefLabel "солени езерца"@bg,
        "salt ponds"@en,
        "saltvannsdammer"@no,
        "соленые пруды"@ru,
        "saltdammar"@sv .

gn:H.POOL a gn:Code ;
    skos:definition "a small and comparatively still, deep part of a larger body of water such as a stream or harbor; or a small body of standing water"@en,
        "водоем со стоячей водой"@ru ;
    skos:inScheme gn:H ;
    skos:notation "H.POOL" ;
    skos:prefLabel "вир(ове)"@bg,
        "pool(s)"@en,
        "kulp"@no,
        "бассейн"@ru,
        "pöl, damm, pool"@sv .

gn:H.POOLI a gn:Code ;
    skos:inScheme gn:H ;
    skos:notation "H.POOLI" ;
    skos:prefLabel "пресъхващи вирове"@bg,
        "intermittent pool"@en,
        "tilbakevendende kulp"@no,
        "временно исчезающий водоем"@ru,
        "peridodisk pool"@sv .

gn:H.RCH a gn:Code ;
    skos:definition "a straight section of a navigable stream or channel between two bends"@en,
        "участок реки между изгибами, перекатами с широким, спокойным течением и большей, чем на перекатах, глубиной"@ru ;
    skos:inScheme gn:H ;
    skos:notation "H.RCH" ;
    skos:prefLabel "част на река между два завоя/на канал между два шлюза"@bg,
        "reach"@en,
        "rett elve- eller kanalstrekning"@no,
        "плёс"@ru,
        "utvidgning"@sv .

gn:H.RDGG a gn:Code ;
    skos:definition "a linear elevation on an icecap"@en,
        "узкая и длинная возвышенность на ледниковой поверхности"@ru ;
    skos:inScheme gn:H ;
    skos:notation "H.RDGG" ;
    skos:prefLabel "заледена част на река между два завоя/на канал между два шлюза"@bg,
        "icecap ridge"@en,
        "iskapperygg"@no,
        "шапка полярного льда"@ru,
        "iskalottsfåra"@sv .

gn:H.RDST a gn:Code ;
    skos:definition "an open anchorage affording less protection than a harbor"@en,
        "часть акватории порта, предназначенная для якорной стоянки судов и перегрузки грузов"@ru ;
    skos:inScheme gn:H ;
    skos:notation "H.RDST" ;
    skos:prefLabel "пристанище далеч от брега"@bg,
        "roadstead"@en,
        "åpen ankerplass"@no,
        "рейд"@ru,
        "redd"@sv .

gn:H.RF a gn:Code ;
    skos:definition "a surface-navigation hazard composed of consolidated material"@en,
        "резкое надводное или подводное возвышение морского дна на мелководьях, препятствующее судоходству"@ru ;
    skos:inScheme gn:H ;
    skos:notation "H.RF" ;
    skos:prefLabel "риф(ове)"@bg,
        "reef(s)"@en,
        "rev"@no,
        "риф(ы)"@ru,
        "rev"@sv .

gn:H.RFC a gn:Code ;
    skos:definition "a surface-navigation hazard composed of coral"@en,
        "подводные геологические образования из органогенных известняков, представляющие собой препятствия (опасности) для навигации"@ru ;
    skos:inScheme gn:H ;
    skos:notation "H.RFC" ;
    skos:prefLabel "коралов риф(ове)"@bg,
        "coral reef(s)"@en,
        "korallrev"@no,
        "коралловые рифы"@ru,
        "korallrev"@sv .

gn:H.RFX a gn:Code ;
    skos:inScheme gn:H ;
    skos:notation "H.RFX" ;
    skos:prefLabel "част от риф"@bg,
        "section of reef"@en,
        "del av rev"@no,
        "участок риф"@ru,
        "del av rev"@sv .

gn:H.RPDS a gn:Code ;
    skos:definition "a turbulent section of a stream associated with a steep, irregular stream bed"@en,
        "мелководный каменистый или скалистый участок в русле реки с относительно большим падением уровня воды и повышенной скоростью течения"@ru ;
    skos:inScheme gn:H ;
    skos:notation "H.RPDS" ;
    skos:prefLabel "бързеи"@bg,
        "rapids"@en,
        "stryk"@no,
        "пороги реки"@ru,
        "forsar"@sv .

gn:H.RSV a gn:Code ;
    skos:definition "an artificial pond or lake"@en,
        "искусственный водоём, образованный, как правило, в долине реки водоподпорными сооружениями для накопления и хранения воды в целях её использования в народном хозяйстве"@ru ;
    skos:inScheme gn:H ;
    skos:notation "H.RSV" ;
    skos:prefLabel "водохранилище(а)"@bg,
        "reservoir(s)"@en,
        "reservoar"@no,
        "водохранилище"@ru,
        "reservoar"@sv .

gn:H.RSVI a gn:Code ;
    skos:inScheme gn:H ;
    skos:notation "H.RSVI" ;
    skos:prefLabel "пресъхващи водохранилища"@bg,
        "intermittent reservoir"@en,
        "tilbakevendende reservoar"@no,
        "периодически пересыхающее водохранилище"@ru,
        "periodisk reservoar"@sv .

gn:H.RSVT a gn:Code ;
    skos:definition "a contained pool or tank of water at, below, or above ground level"@en,
        "наполненный водой бак или резервуар, находящийся на, выше или ниже уровня земли"@ru ;
    skos:inScheme gn:H ;
    skos:notation "H.RSVT" ;
    skos:prefLabel "воден ресервуар"@bg,
        "water tank"@en,
        "vanntank"@no,
        "водяной бак"@ru,
        "vattentank"@sv .

gn:H.RVN a gn:Code ;
    skos:definition "a small, narrow, deep, steep-sided stream channel, smaller than a gorge"@en,
        "глубокая длинная впадина на поверхности земли, образовавшаяся от действия дождевых и талых вод"@ru ;
    skos:inScheme gn:H ;
    skos:notation "H.RVN" ;
    skos:prefLabel "клисура(и)"@bg,
        "ravine(s)"@en,
        "ravine"@no,
        "овраг"@ru,
        "ravin(er)"@sv .

gn:H.SBKH a gn:Code ;
    skos:definition "a salt flat or salt encrusted plain subject to periodic inundation from flooding or high tides"@en,
        "замкнутое бессточное понижение рельефа с плоским глинистым днищем, занятым солончаками"@ru ;
    skos:inScheme gn:H ;
    skos:notation "H.SBKH" ;
    skos:prefLabel "сухо легло на солено езеро(а)"@bg,
        "sabkha(s)"@en,
        "sabkha (oversvømt område)"@no,
        "себха"@ru,
        "sabkha"@sv .

gn:H.SD a gn:Code ;
    skos:definition "a long arm of the sea forming a channel between the mainland and an island or islands; or connecting two larger bodies of water"@en,
        "длинный морской рукав, образующий пролив между материком и островом, или островами"@ru ;
    skos:inScheme gn:H ;
    skos:notation "H.SD" ;
    skos:prefLabel "морски ръкав"@bg,
        "sound"@en,
        "sund"@no,
        "широкая лагуна"@ru,
        "sund"@sv .

gn:H.SEA a gn:Code ;
    skos:definition "a large body of salt water more or less confined by continuous land or chains of islands forming a subdivision of an ocean"@en,
        "большое водное пространство, ограниченное с одной или нескольких сторон сушей и отделяемое от самого океана островами или возвышенностями подводного рельефа"@ru ;
    skos:inScheme gn:H ;
    skos:notation "H.SEA" ;
    skos:prefLabel "море"@bg,
        "sea"@en,
        "sjø"@no,
        "море"@ru,
        "hav"@sv .

gn:H.SHOL a gn:Code ;
    skos:definition "a surface-navigation hazard composed of unconsolidated material"@en,
        "участок (обычно прибрежный) реки, озера и т.п. с небольшой глубиной"@ru ;
    skos:inScheme gn:H ;
    skos:notation "H.SHOL" ;
    skos:prefLabel "плитчина(и)"@bg,
        "shoal(s)"@en,
        "sandgrunne"@no,
        "мелководье"@ru,
        "grund, rev"@sv .

gn:H.SILL a gn:Code ;
    skos:definition "the low part of an underwater gap or saddle separating basins, including a similar feature at the mouth of a fjord"@en,
        "вытянутое горное поднятие на дне океанов и морей. Часто подводные хребты выступают над поверхностью воды в виде островов или целых архипелагов"@ru ;
    skos:inScheme gn:H ;
    skos:notation "H.SILL" ;
    skos:prefLabel "врата на шлюз"@bg,
        "sill"@en,
        "terskel"@no,
        "подводный хребет"@ru,
        "tröskel"@sv .

gn:H.SPNG a gn:Code ;
    skos:definition "a place where ground water flows naturally out of the ground"@en,
        "водный источник, бьющий, текущий из глубины земли; ключ"@ru ;
    skos:inScheme gn:H ;
    skos:notation "H.SPNG" ;
    skos:prefLabel "извор(и)"@bg,
        "spring(s)"@en,
        "kilde"@no,
        "родник"@ru,
        "källa(or)"@sv .

gn:H.SPNS a gn:Code ;
    skos:definition "a place where sulphur ground water flows naturally out of the ground"@en,
        "источник воды, насыщенной сероводородом"@ru ;
    skos:inScheme gn:H ;
    skos:notation "H.SPNS" ;
    skos:prefLabel "серен извор(и)"@bg,
        "sulphur spring(s)"@en,
        "svovelkilde"@no,
        "серный источник"@ru,
        "svavelkälla(or)"@sv .

gn:H.SPNT a gn:Code ;
    skos:definition "a place where hot ground water flows naturally out of the ground"@en,
        "источник термальных вод, температура которых выше 20°C"@ru ;
    skos:inScheme gn:H ;
    skos:notation "H.SPNT" ;
    skos:prefLabel "горещ извор(и)"@bg,
        "hot spring(s)"@en,
        "varm kilde"@no,
        "термальный источник"@ru,
        "varmkälla (or)"@sv .

gn:H.STM a gn:Code ;
    skos:definition "a body of running water moving to a lower level in a channel on land"@en,
        "небольшой мелкий водоток с постоянным или временным течением"@ru ;
    skos:inScheme gn:H ;
    skos:notation "H.STM" ;
    skos:prefLabel "поток"@bg,
        "stream"@en,
        "bekk"@no,
        "ручей"@ru,
        "å, bäck, ström"@sv .

gn:H.STMA a gn:Code ;
    skos:definition "a diverging branch flowing out of a main stream and rejoining it downstream"@en,
        "водоток, отходящий от реки и впадающий в неё ниже по течению;"@ru ;
    skos:inScheme gn:H ;
    skos:notation "H.STMA" ;
    skos:prefLabel "речен скален остров"@bg,
        "anabranch"@en,
        "elvearm som vender tilbake til hovedløpet"@no,
        "протока"@ru,
        "bifurkation"@sv .

gn:H.STMB a gn:Code ;
    skos:definition "a conspicuously curved or bent segment of a stream"@en,
        "крутой поворот, изгиб ручья"@ru ;
    skos:inScheme gn:H ;
    skos:notation "H.STMB" ;
    skos:prefLabel "завой на поток"@bg,
        "stream bend"@en,
        "elvesving"@no,
        "излучина ручья"@ru,
        "åkrök"@sv .

gn:H.STMC a gn:Code ;
    skos:definition "a stream that has been substantially ditched, diked, or straightened"@en,
        "естественный или искусственный водный поток канала"@ru ;
    skos:inScheme gn:H ;
    skos:notation "H.STMC" ;
    skos:prefLabel "канализиран поток"@bg,
        "canalized stream"@en,
        "kanalisert bekk"@no,
        "водоток канала"@ru,
        "kanaliserat vattendrag"@sv .

gn:H.STMD a gn:Code ;
    skos:definition "a branch which flows away from the main stream, as in a delta or irrigation canal"@en,
        "ответвление, отходящее от главного русла реки"@ru ;
    skos:inScheme gn:H ;
    skos:notation "H.STMD" ;
    skos:prefLabel "речен ръкав(и)"@bg,
        "distributary(-ies)"@en,
        "flodarm som ikke vender tilbake til hovedløpet"@no,
        "рукав реки"@ru,
        "biflod(er)"@sv .

gn:H.STMH a gn:Code ;
    skos:definition "the source and upper part of a stream, including the upper drainage basin"@en,
        "часть реки, близкая к её истокам; прилегающая к ней местность"@ru ;
    skos:inScheme gn:H ;
    skos:notation "H.STMH" ;
    skos:prefLabel "горен бйеф"@bg,
        "headwaters"@en,
        "utspring"@no,
        "верховье"@ru,
        "källfloder"@sv .

gn:H.STMI a gn:Code ;
    skos:inScheme gn:H ;
    skos:notation "H.STMI" ;
    skos:prefLabel "пресъхващ поток"@bg,
        "intermittent stream"@en,
        "tilbakevendende bekk"@no,
        "река с периодическим водотоком"@ru,
        "periodiskt vattendrag"@sv .

gn:H.STMIX a gn:Code ;
    skos:inScheme gn:H ;
    skos:notation "H.STMIX" ;
    skos:prefLabel "част от пресъхващ пото"@bg,
        "section of intermittent stream"@en,
        "del av tilbakevendende bekk"@no,
        "участок реки с периодическим водотоком"@ru,
        "del av periodiskt vattendrag"@sv .

gn:H.STMM a gn:Code ;
    skos:definition "a place where a stream discharges into a lagoon, lake, or the sea"@en,
        "место впадения реки (в море, озеро и т.п.), конечный участок нижнего течения реки"@ru ;
    skos:inScheme gn:H ;
    skos:notation "H.STMM" ;
    skos:prefLabel "планински поток(и)"@bg,
        "stream mouth(s)"@en,
        "bekkeutløp"@no,
        "устье реки"@ru,
        "åmynning(ar)"@sv .

gn:H.STMQ a gn:Code ;
    skos:definition "a former stream or distributary no longer carrying flowing water, but still evident due to lakes, wetland, topographic or vegetation patterns"@en,
        "водоем, в котором больше нет воды, но который еще заметный благодаря его топографическим или растительным особенностям"@ru ;
    skos:inScheme gn:H ;
    skos:notation "H.STMQ" ;
    skos:prefLabel "пресъхнали реки"@bg,
        "abandoned watercourse"@en,
        "inntørket elveleie"@no,
        "высохший водоем"@ru,
        "övergivet vattendrag"@sv .

gn:H.STMS a gn:Code ;
    skos:definition "bodies of running water moving to a lower level in a channel on land"@en,
        "небольшие мелкие водотоки с постоянным или временным течением"@ru ;
    skos:inScheme gn:H ;
    skos:notation "H.STMS" ;
    skos:prefLabel "потоци"@bg,
        "streams"@en,
        "bekker"@no,
        "ручьи"@ru,
        "vattendrag"@sv .

gn:H.STMSB a gn:Code ;
    skos:definition "a surface stream that disappears into an underground channel, or dries up in an arid area"@en,
        "река,  полностью высохшая или превратившаяся в подземный канал"@ru ;
    skos:inScheme gn:H ;
    skos:notation "H.STMSB" ;
    skos:prefLabel "изгубващи се реки"@bg,
        "lost river"@en,
        "elv uten utløp"@no,
        "высохшая река"@ru,
        "lost river"@sv .

gn:H.STMX a gn:Code ;
    skos:inScheme gn:H ;
    skos:notation "H.STMX" ;
    skos:prefLabel "част от поток"@bg,
        "section of stream"@en,
        "del av bekk"@no,
        "участок ручья"@ru,
        "del av vattendrag"@sv .

gn:H.STRT a gn:Code ;
    skos:definition "a relatively narrow waterway, usually narrower and less extensive than a sound, connecting two larger bodies of water"@en,
        "узкое водное пространство, разъединяющее участки суши и соединяющее водоёмы (моря, озёра и т.п.) или их части"@ru ;
    skos:inScheme gn:H ;
    skos:notation "H.STRT" ;
    skos:prefLabel "пролив"@bg,
        "strait"@en,
        "sund"@no,
        "пролив"@ru,
        "sund"@sv .

gn:H.SWMP a gn:Code ;
    skos:definition "a wetland dominated by tree vegetation"@en,
        "заболоченная территория, на которой преобладает древесная растительность"@ru ;
    skos:inScheme gn:H ;
    skos:notation "H.SWMP" ;
    skos:prefLabel "язовир"@bg,
        "swamp"@en,
        "sump"@no,
        "лесное болото"@ru,
        "träsk, sumpmark, kärr"@sv .

gn:H.SYSI a gn:Code ;
    skos:definition "a network of ditches and one or more of the following elements: water supply, reservoir, canal, pump, well, drain, etc."@en,
        "земельная территория вместе с сетью каналов и др. гидротехнических и эксплуатационных сооружений, обеспечивающих её орошение"@ru ;
    skos:inScheme gn:H ;
    skos:notation "H.SYSI" ;
    skos:prefLabel "напоителен язовир"@bg,
        "irrigation system"@en,
        "vanningssystem"@no,
        "оросительная система"@ru,
        "bevattningssystem"@sv .

gn:H.TNLC a gn:Code ;
    skos:definition "a tunnel through which a canal passes"@en,
        "тоннель, сооружаемый при пересечении судоходным каналом возвышенности, горного хребта и т. п."@ru ;
    skos:inScheme gn:H ;
    skos:notation "H.TNLC" ;
    skos:prefLabel "канален тунел"@bg,
        "canal tunnel"@en,
        "kanaltunnel"@no,
        "судоходный тоннель"@ru,
        "canal tunnel"@sv .

gn:H.WAD a gn:Code ;
    skos:definition "a valley or ravine, bounded by relatively steep banks, which in the rainy season becomes a watercourse; found primarily in North Africa and the Middle East"@en,
        "русло или долина пересыхающего водотока; в Азии, в Африке"@ru ;
    skos:inScheme gn:H ;
    skos:notation "H.WAD" ;
    skos:prefLabel "сухи речни корита (вади)"@bg,
        "wadi"@en,
        "wadi"@no,
        "вади"@ru,
        "flod"@sv .

gn:H.WADB a gn:Code ;
    skos:definition "a conspicuously curved or bent segment of a wadi"@en,
        "изогнутый участок вади"@ru ;
    skos:inScheme gn:H ;
    skos:notation "H.WADB" ;
    skos:prefLabel "извивка на вади"@bg,
        "wadi bend"@en,
        "wadi-sving"@no,
        "излучина вади"@ru,
        "flodkrök"@sv .

gn:H.WADJ a gn:Code ;
    skos:definition "a place where two or more wadies join"@en ;
    skos:inScheme gn:H ;
    skos:notation "H.WADJ" ;
    skos:prefLabel "възел на вади"@bg,
        "wadi junction"@en,
        "wadi-sammenløp"@no,
        "место слияния двух или более вади"@ru,
        "flodförbindning"@sv .

gn:H.WADM a gn:Code ;
    skos:definition "the lower terminus of a wadi where it widens into an adjoining floodplain, depression, or waterbody"@en,
        "место впадения вади (в море, озеро и т.п.), конечный участок нижнего течения вади"@ru ;
    skos:inScheme gn:H ;
    skos:notation "H.WADM" ;
    skos:prefLabel "гърло на вади"@bg,
        "wadi mouth"@en,
        "wadi-utløp"@no,
        "устье вади"@ru,
        "flodmynning"@sv .

gn:H.WADS a gn:Code ;
    skos:definition "valleys or ravines, bounded by relatively steep banks, which in the rainy season become watercourses; found primarily in North Africa and the Middle East"@en,
        "русла или долины пересыхающих водотоков; в Азии, в Африке"@ru ;
    skos:inScheme gn:H ;
    skos:notation "H.WADS" ;
    skos:prefLabel "множество вади"@bg,
        "wadies"@en,
        "wadier"@no,
        "множество вади"@ru,
        "floder"@sv .

gn:H.WADX a gn:Code ;
    skos:inScheme gn:H ;
    skos:notation "H.WADX" ;
    skos:prefLabel "част от вади"@bg,
        "section of wadi"@en,
        "del av wadi"@no,
        "участок вади"@ru,
        "del av flod"@sv .

gn:H.WHRL a gn:Code ;
    skos:definition "a turbulent, rotating movement of water in a stream"@en,
        "вращательное движение воды в реках, морях и т.п.; место, где происходит такое движение"@ru ;
    skos:inScheme gn:H ;
    skos:notation "H.WHRL" ;
    skos:prefLabel "водовъртеж"@bg,
        "whirlpool"@en,
        "strømvirvel"@no,
        "водоворот"@ru,
        "virvel"@sv .

gn:H.WLL a gn:Code ;
    skos:definition "a cylindrical hole, pit, or tunnel drilled or dug down to a depth from which water, oil, or gas can be pumped or brought to the surface"@en,
        "глубокая яма с отвесными стенками, обычно защищённая от обвалов срубом, служащая для добывания воды из водоносных слоёв земли"@ru ;
    skos:inScheme gn:H ;
    skos:notation "H.WLL" ;
    skos:prefLabel "кладенец"@bg,
        "well"@en,
        "brønn"@no,
        "колодец"@ru,
        "brunn, källa"@sv .

gn:H.WLLQ a gn:Code ;
    skos:inScheme gn:H ;
    skos:notation "H.WLLQ" ;
    skos:prefLabel "изоставен кладенец"@bg,
        "abandoned well"@en,
        "forlatt brønn"@no,
        "заброшенный колодец"@ru,
        "övergiven källa"@sv .

gn:H.WLLS a gn:Code ;
    skos:definition "cylindrical holes, pits, or tunnels drilled or dug down to a depth from which water, oil, or gas can be pumped or brought to the surface"@en,
        "глубокие ямы с отвесными стенками, обычно защищённые от обвалов срубом, служащие для добывания воды из водоносных слоёв земли"@ru ;
    skos:inScheme gn:H ;
    skos:notation "H.WLLS" ;
    skos:prefLabel "кладенци"@bg,
        "wells"@en,
        "brønner"@no,
        "колодцы"@ru,
        "källor"@sv .

gn:H.WTLD a gn:Code ;
    skos:definition "an area subject to inundation, usually characterized by bog, marsh, or swamp vegetation"@en,
        "территория, подвергающаяся частым наводнениям; здесь часто образуются болота, на которых растет характерная для них болотная растительность"@ru ;
    skos:inScheme gn:H ;
    skos:notation "H.WTLD" ;
    skos:prefLabel "влажни зони"@bg,
        "wetland"@en,
        "våtmark"@no,
        "заболоченная местность"@ru,
        "våtmark"@sv .

gn:H.WTLDI a gn:Code ;
    skos:inScheme gn:H ;
    skos:notation "H.WTLDI" ;
    skos:prefLabel "пресъхващи влажни зони"@bg,
        "intermittent wetland"@en,
        "tilbakevendende våtmark"@no,
        "периодически затопляемая территория"@ru,
        "periodisk våtmark"@sv .

gn:H.WTRC a gn:Code ;
    skos:definition "a natural, well-defined channel produced by flowing water, or an artificial channel designed to carry flowing water"@en,
        "стремительно текущая река или ручей"@ru ;
    skos:inScheme gn:H ;
    skos:notation "H.WTRC" ;
    skos:prefLabel "речно корито"@bg,
        "watercourse"@en,
        "vannløp"@no,
        "поток"@ru,
        "vattendrag"@sv .

gn:H.WTRH a gn:Code ;
    skos:definition "a natural hole, hollow, or small depression that contains water, used by man and animals, especially in arid areas"@en,
        "естественное углубление, в котором собирается вода"@ru ;
    skos:inScheme gn:H ;
    skos:notation "H.WTRH" ;
    skos:prefLabel "гьол(ове)"@bg,
        "waterhole(s)"@en,
        "vannhull"@no,
        "водяная яма"@ru,
        "vattenhål"@sv .

gn:L.AGRC a gn:Code ;
    skos:definition "a tract of land set aside for agricultural settlement"@en,
        "участок земли, отведенный для сельскохозяйственных поселений"@ru ;
    skos:inScheme gn:L ;
    skos:notation "L.AGRC" ;
    skos:prefLabel "селскостопанска колония"@bg,
        "agricultural colony"@en,
        "landbrukskoloni"@no,
        "сельскохозяйственная колония"@ru,
        "jordbrukskoloni"@sv .

gn:L.AMUS a gn:Code ;
    skos:definition "Amusement Park are theme parks, adventure parks offering entertainment, similar to funfairs but with a fix location"@en,
        "парк развлечений, то же, что и ярмарка, только с постоянным месторасположением"@ru ;
    skos:inScheme gn:L ;
    skos:notation "L.AMUS" ;
    skos:prefLabel "amusement park"@bg,
        "amusement park"@en,
        "amusement park"@no,
        "Парк аттракционов  (ПКиО)"@ru,
        "nöjespark"@sv .

gn:L.AREA a gn:Code ;
    skos:definition "a tract of land without homogeneous character or boundaries"@en,
        "местность, земля, край; часть какой-либо территории (страны, государства, материка, земной суши и т.п.), выделяемая при районировании по определённому существенному признаку"@ru ;
    skos:inScheme gn:L ;
    skos:notation "L.AREA" ;
    skos:prefLabel "регион"@bg,
        "area"@en,
        "område"@no,
        "Область"@ru,
        "area, område"@sv .

gn:L.BSND a gn:Code ;
    skos:definition "an area drained by a stream"@en,
        "поверхность, с которой речная система, море или озеро собирают воды"@ru ;
    skos:inScheme gn:L ;
    skos:notation "L.BSND" ;
    skos:prefLabel "доден басейн"@bg,
        "drainage basin"@en,
        "dreneringsbasseng"@no,
        "Водосборный бассейн"@ru,
        "vattenuppsamlingsområde"@sv .

gn:L.BSNP a gn:Code ;
    skos:definition "an area underlain by an oil-rich structural basin"@en,
        "область с богатой нефтью структурной впадиной"@ru ;
    skos:inScheme gn:L ;
    skos:notation "L.BSNP" ;
    skos:prefLabel "нефтен басейн"@bg,
        "petroleum basin"@en,
        "petroleumsbasseng"@no,
        "нефтегазовый бассейн"@ru,
        "råoljebassäng"@sv .

gn:L.BTL a gn:Code ;
    skos:definition "a site of a land battle of historical importance"@en,
        "район боевых действий; имеет важное историческое значение"@ru ;
    skos:inScheme gn:L ;
    skos:notation "L.BTL" ;
    skos:prefLabel "полесражение"@bg,
        "battlefield"@en,
        "slagmark"@no,
        "поле боя"@ru,
        "slagfält"@sv .

gn:L.CLG a gn:Code ;
    skos:definition "an area in a forest with trees removed"@en,
        "открытое пространство в парке или в лесу"@ru ;
    skos:inScheme gn:L ;
    skos:notation "L.CLG" ;
    skos:prefLabel "сечище"@bg,
        "clearing"@en,
        "lysning"@no,
        "поляна"@ru,
        "uthuggning, röjt område"@sv .

gn:L.CMN a gn:Code ;
    skos:definition "a park or pasture for community use"@en,
        "земли (выгоны, сенокосы, леса), которые  находятся в общем пользовании"@ru ;
    skos:inScheme gn:L ;
    skos:notation "L.CMN" ;
    skos:prefLabel "обществена собственост"@bg,
        "common"@en,
        "allmenning"@no,
        "общинные земли"@ru,
        "allmänt område"@sv .

gn:L.CNS a gn:Code ;
    skos:definition "a lease of land by a government for economic development, e.g., mining, forestry"@en,
        "арендуемая государством земля, пользование которой необходимо для экономического развития, например, шахты, лесные массивы"@ru ;
    skos:inScheme gn:L ;
    skos:notation "L.CNS" ;
    skos:prefLabel "концесионен район"@bg,
        "concession area"@en,
        "konsesjonsområde"@no,
        "лицензионная территория"@ru,
        "koncessionsområde"@sv .

gn:L.COLF a gn:Code ;
    skos:definition "a region in which coal deposits of possible economic value occur"@en,
        "площадь непрерывного или островного распространения угленосных формаций, значительная по размерам или запасам угля"@ru ;
    skos:inScheme gn:L ;
    skos:notation "L.COLF" ;
    skos:prefLabel "въглищно находище"@bg,
        "coalfield"@en,
        "kullfelt"@no,
        "угольный бассейн"@ru,
        "kolfält"@sv .

gn:L.CONT a gn:Code ;
    skos:definition "continent : Europe, Africa, Asia, North America, South America, Oceania,Antarctica"@en,
        "континент: Евразия, Африка, Северная Америка, Южная Америка, Антарктида, Австралия, Океания"@ru ;
    skos:inScheme gn:L ;
    skos:notation "L.CONT" ;
    skos:prefLabel "континент"@bg,
        "continent"@en,
        "kontinent"@no,
        "континент"@ru,
        "kontinent"@sv .

gn:L.CST a gn:Code ;
    skos:definition "a zone of variable width straddling the shoreline"@en,
        "полоса суши, примыкающая к водной поверхности моря или океана и взаимодействующая с ним"@ru ;
    skos:inScheme gn:L ;
    skos:notation "L.CST" ;
    skos:prefLabel "крайбрежие"@bg,
        "coast"@en,
        "kyst"@no,
        "морской берег"@ru,
        "kust"@sv .

gn:L.CTRB a gn:Code ;
    skos:definition "a place where a number of businesses are located"@en,
        "деловая часть города"@ru ;
    skos:inScheme gn:L ;
    skos:notation "L.CTRB" ;
    skos:prefLabel "бизнес център"@bg,
        "business center"@en,
        "forretningssenter"@no,
        "бизнес центр"@ru,
        "affärscenter"@sv .

gn:L.DEVH a gn:Code ;
    skos:definition "a tract of land on which many houses of similar design are built according to a development plan"@en,
        "часть застроенной территории населенного пункта, предполагающая целостность архитектурного замысла"@ru ;
    skos:inScheme gn:L ;
    skos:notation "L.DEVH" ;
    skos:prefLabel "жилищна зона"@bg,
        "housing development"@en,
        "boligområde"@no,
        "квартал"@ru,
        "housing development"@sv .

gn:L.FLD a gn:Code ;
    skos:definition "an open as opposed to wooded area"@en,
        "безлесная равнина, ровное (в отличие от селения, леса) обширное пространство"@ru ;
    skos:inScheme gn:L ;
    skos:notation "L.FLD" ;
    skos:prefLabel "поле(та)"@bg,
        "field(s)"@en,
        "åker"@no,
        "поле"@ru,
        "fält"@sv .

gn:L.FLDI a gn:Code ;
    skos:definition "a tract of level or terraced land which is irrigated"@en,
        "участки земли, подготовленные для естественной биологической очистки сточных вод и выращивания с.-х. растений"@ru ;
    skos:inScheme gn:L ;
    skos:notation "L.FLDI" ;
    skos:prefLabel "напоявани полета"@bg,
        "irrigated field(s)"@en,
        "overrislet åker"@no,
        "ирригационные поля"@ru,
        "(konst)bevattnade fält"@sv .

gn:L.GASF a gn:Code ;
    skos:definition "an area containing a subterranean store of natural gas of economic value"@en,
        "совокупность залежей природного газа на определенной территории"@ru ;
    skos:inScheme gn:L ;
    skos:notation "L.GASF" ;
    skos:prefLabel "залежи от гас"@bg,
        "gasfield"@en,
        "gassfelt"@no,
        "месторождение газа"@ru,
        "gasfält"@sv .

gn:L.GRAZ a gn:Code ;
    skos:definition "an area of grasses and shrubs used for grazing"@en,
        "участок травянистой растительности, используемый и поддерживаемый для выпаса домашних животных"@ru ;
    skos:inScheme gn:L ;
    skos:notation "L.GRAZ" ;
    skos:prefLabel "тревиста зона"@bg,
        "grazing area"@en,
        "beiteområde"@no,
        "пастбище"@ru,
        "betesområde"@sv .

gn:L.GVL a gn:Code ;
    skos:definition "an area covered with gravel"@en,
        "покрытая гравием территория"@ru ;
    skos:inScheme gn:L ;
    skos:notation "L.GVL" ;
    skos:prefLabel "едрозърнест пясък"@bg,
        "gravel area"@en,
        "grusområde"@no,
        "покрытие из гравия"@ru,
        "grusområde"@sv .

gn:L.INDS a gn:Code ;
    skos:definition "an area characterized by industrial activity"@en,
        "территория с ярко выраженной индустриально-производственной специализацией"@ru ;
    skos:inScheme gn:L ;
    skos:notation "L.INDS" ;
    skos:prefLabel "индустриална зона"@bg,
        "industrial area"@en,
        "industriområde"@no,
        "промышленный район"@ru,
        "industriområde"@sv .

gn:L.LAND a gn:Code ;
    skos:definition "a tract of land in the Arctic"@en,
        "участок земли в Арктике"@ru ;
    skos:inScheme gn:L ;
    skos:notation "L.LAND" ;
    skos:prefLabel "арктически територии"@bg,
        "arctic land"@en,
        "arktisk landskap"@no,
        "арктические земли"@ru,
        "arktiskt land"@sv .

gn:L.LCTY a gn:Code ;
    skos:definition "a minor area or place of unspecified or mixed character and indefinite boundaries"@en,
        "название низовой административно-территориальной единицы"@ru ;
    skos:inScheme gn:L ;
    skos:notation "L.LCTY" ;
    skos:prefLabel "местност"@bg,
        "locality"@en,
        "trakt"@no,
        "район"@ru,
        "locality"@sv .

gn:L.MILB a gn:Code ;
    skos:definition "a place used by an army or other armed service for storing arms and supplies, and for accommodating and training troops, a base from which operations can be initiated"@en,
        "территория (важный в стратегическом или политическом отношении пункт, район) и размещенные на ней войска с запасами оружия, боеприпасов, продовольствия и других материальных средств, необходимых для боевой и повседневной деятельности"@ru ;
    skos:inScheme gn:L ;
    skos:notation "L.MILB" ;
    skos:prefLabel "военна база"@bg,
        "military base"@en,
        "militærbase"@no,
        "военная база"@ru,
        "militärbas"@sv .

gn:L.MNA a gn:Code ;
    skos:definition "an area of mine sites where minerals and ores are extracted"@en,
        "район добычи полезных ископаемых"@ru ;
    skos:inScheme gn:L ;
    skos:notation "L.MNA" ;
    skos:prefLabel "полезни ископаеми"@bg,
        "mining area"@en,
        "gruveområde"@no,
        "район разработки"@ru,
        "gruvområde"@sv .

gn:L.MVA a gn:Code ;
    skos:definition "a tract of land where military field exercises are carried out"@en,
        "участок суши или моря, предназначенный для испытаний различных видов оружия, боевых средств и техники, а также для боевой подготовки войск"@ru ;
    skos:inScheme gn:L ;
    skos:notation "L.MVA" ;
    skos:prefLabel "военен полигон"@bg,
        "maneuver area"@en,
        "militært treningsområde"@no,
        "полигон"@ru,
        "maneuver area"@sv .

gn:L.NVB a gn:Code ;
    skos:definition "an area used to store supplies, provide barracks for troops and naval personnel, a port for naval vessels, and from which operations are initiated"@en,
        "оборудованный и обороняемый район (зона) побережья и прилегающего участка моря обычно с несколькими пунктами базирования кораблей, с силами и средствами, предназначенными для обороны"@ru ;
    skos:inScheme gn:L ;
    skos:notation "L.NVB" ;
    skos:prefLabel "военоворска база"@bg,
        "naval base"@en,
        "marinebase"@no,
        "военно-морская база"@ru,
        "marinbas"@sv .

gn:L.OAS a gn:Code ;
    skos:definition "an area in a desert made productive by the availability of water"@en,
        "участок пустыни или полупустыни с обильным естественным или искусственным увлажнением, обусловленным близостью рек и грунтовых вод, и с богатой растительностью"@ru ;
    skos:inScheme gn:L ;
    skos:notation "L.OAS" ;
    skos:prefLabel "оазис(и)"@bg,
        "oasis(-es)"@en,
        "oase"@no,
        "оазис"@ru,
        "oas(er)"@sv .

gn:L.OILF a gn:Code ;
    skos:definition "an area containing a subterranean store of petroleum of economic value"@en,
        "место под землей, где залегают запасы нефти"@ru ;
    skos:inScheme gn:L ;
    skos:notation "L.OILF" ;
    skos:prefLabel "петролно находище"@bg,
        "oilfield"@en,
        "oljefelt"@no,
        "нефтяное месторождение"@ru,
        "oljefält"@sv .

gn:L.PEAT a gn:Code ;
    skos:definition "an area where peat is harvested"@en,
        "место, где добывают торф"@ru ;
    skos:inScheme gn:L ;
    skos:notation "L.PEAT" ;
    skos:prefLabel "торфено находище"@bg,
        "peat cutting area"@en,
        "torvskjæringsområde"@no,
        "торфяное месторождение"@ru,
        "torvfält"@sv .

gn:L.PRK a gn:Code ;
    skos:definition "an area, often of forested land, maintained as a place of beauty, or for recreation"@en,
        "обширная озелененная территория, благоустроенная и художественно оформленная для отдыха под открытым небом"@ru ;
    skos:inScheme gn:L ;
    skos:notation "L.PRK" ;
    skos:prefLabel "парк"@bg,
        "park"@en,
        "park"@no,
        "парк"@ru,
        "park"@sv .

gn:L.PRT a gn:Code ;
    skos:definition "a place provided with terminal and transfer facilities for loading and discharging waterborne cargo or passengers, usually located in a harbor"@en,
        "место с закрытым водным пространством, специально оборудованное для стоянки, погрузки и разгрузки судов, гавань"@ru ;
    skos:inScheme gn:L ;
    skos:notation "L.PRT" ;
    skos:prefLabel "пристанище"@bg,
        "port"@en,
        "havn"@no,
        "порт"@ru,
        "hamn"@sv .

gn:L.QCKS a gn:Code ;
    skos:definition "an area where loose sand with water moving through it may become unstable when heavy objects are placed at the surface, causing them to sink"@en,
        "пески, перенасыщенные водой восходящих источников и способные вследствие этого засасывать попадающие на них предметы, животных и человека"@ru ;
    skos:inScheme gn:L ;
    skos:notation "L.QCKS" ;
    skos:prefLabel "плаващ пясък"@bg,
        "quicksand"@en,
        "kvikksand"@no,
        "зыбучие пески"@ru,
        "kvicksand"@sv .

gn:L.REP a gn:Code ;
    owl:deprecated true ;
    skos:inScheme gn:L ;
    skos:notation "L.REP" ;
    skos:prefLabel "republic"@en .

gn:L.RES a gn:Code ;
    skos:definition "a tract of public land reserved for future use or restricted as to use"@en,
        "особо охраняемая территория, полностью исключенная из любой хозяйственной деятельности в целях сохранения в нетронутом виде природных комплексов"@ru ;
    skos:inScheme gn:L ;
    skos:notation "L.RES" ;
    skos:prefLabel "резерват"@bg,
        "reserve"@en,
        "regulert område"@no,
        "заповедник"@ru,
        "reservat"@sv .

gn:L.RESA a gn:Code ;
    skos:definition "a tract of land reserved for agricultural reclamation and/or development"@en,
        "участок земли, предназначенный для агромелиорации"@ru ;
    skos:inScheme gn:L ;
    skos:notation "L.RESA" ;
    skos:prefLabel "аграрен резерват"@bg,
        "agricultural reserve"@en,
        "område regulert til landbruk"@no,
        "агрозаповедник"@ru,
        "jordbruksreservat"@sv .

gn:L.RESF a gn:Code ;
    skos:definition "a forested area set aside for preservation or controlled use"@en,
        "особо охраняемый участок леса, использование которого контролируется"@ru ;
    skos:inScheme gn:L ;
    skos:notation "L.RESF" ;
    skos:prefLabel "горски резерват"@bg,
        "forest reserve"@en,
        "vernet skog"@no,
        "лесной заповедник"@ru,
        "skogsreservat"@sv .

gn:L.RESH a gn:Code ;
    skos:definition "a tract of land used primarily for hunting"@en,
        "участок территории, выделенный для интенсивного воспроизводства дичи и проведения строго регулируемых охот"@ru ;
    skos:inScheme gn:L ;
    skos:notation "L.RESH" ;
    skos:prefLabel "ловен резерват"@bg,
        "hunting reserve"@en,
        "jaktområde"@no,
        "заповедно-охотничье хозяйство"@ru,
        "jaktreservat"@sv .

gn:L.RESN a gn:Code ;
    skos:definition "an area reserved for the maintenance of a natural habitat"@en,
        "особо охраняемые участки земли, водной поверхности и воздушного пространства над ними, где располагаются природные комплексы и объекты, которые имеют свое научное, культурное, эстетическое и оздоровительное значение, которые изъяты решениями органов государственной власти полностью или частично из хозяйственного использования"@ru ;
    skos:inScheme gn:L ;
    skos:notation "L.RESN" ;
    skos:prefLabel "природен резерват"@bg,
        "nature reserve"@en,
        "naturreservat"@no,
        "особо охраняемая природная  территория"@ru,
        "naturreservat"@sv .

gn:L.RESP a gn:Code ;
    skos:definition "an area of palm trees where use is controlled"@en,
        "место, где растут пальмы, использование которых контролируется"@ru ;
    skos:inScheme gn:L ;
    skos:notation "L.RESP" ;
    skos:prefLabel "резерват от палмови дървета"@bg,
        "palm tree reserve"@en,
        "palmereservat"@no,
        "пальмовый заповедник"@ru,
        "palmträdsreservat"@sv .

gn:L.RESV a gn:Code ;
    skos:definition "a tract of land set aside for aboriginal, tribal, or native populations"@en,
        "территории, отведенные для поселения коренного населения страны"@ru ;
    skos:inScheme gn:L ;
    skos:notation "L.RESV" ;
    skos:prefLabel "резерват"@bg,
        "reservation"@en,
        "reservat"@no,
        "резервация"@ru,
        "reservat"@sv .

gn:L.RESW a gn:Code ;
    skos:definition "a tract of public land reserved for the preservation of wildlife"@en,
        "заповедник, территория, где природные богатства (животные и растения) находятся под особой охраной правительства"@ru ;
    skos:inScheme gn:L ;
    skos:notation "L.RESW" ;
    skos:prefLabel "резерват дива природа"@bg,
        "wildlife reserve"@en,
        "viltreservat"@no,
        "резерват"@ru,
        "viltreservat"@sv .

gn:L.RGN a gn:Code ;
    skos:definition "an area distinguished by one or more observable physical or cultural characteristics"@en,
        "область, район, территория, часть страны, отличающиеся совокупностью естественных или исторически сложившихся экономико-географических условий и национального состава населения"@ru ;
    skos:inScheme gn:L ;
    skos:notation "L.RGN" ;
    skos:prefLabel "регион"@bg,
        "region"@en,
        "region"@no,
        "регион"@ru,
        "region"@sv .

gn:L.RGNE a gn:Code ;
    skos:definition "a region of a country established for economic development or for statistical purposes"@en,
        "регион страны, характеризующийся своеобразием природных и экономических условий; деление страны на эк. регионы используется для получения статистических данных"@ru ;
    skos:inScheme gn:L ;
    skos:notation "L.RGNE" ;
    skos:prefLabel "икономически регион"@bg,
        "economic region"@en,
        "økonomisk region"@no,
        "экономический регион"@ru,
        "ekonomisk region"@sv .

gn:L.RGNH a gn:Code ;
    skos:historyNote "Added in v3.1"@en ;
    skos:inScheme gn:L ;
    skos:notation "L.RGNH" ;
    skos:prefLabel "historical region"@en .

gn:L.RGNL a gn:Code ;
    skos:definition "a tract of land distinguished by numerous lakes"@en,
        "место скопления большого количества озер"@ru ;
    skos:inScheme gn:L ;
    skos:notation "L.RGNL" ;
    skos:prefLabel "езерен регион"@bg,
        "lake region"@en,
        "innsjøområde"@no,
        "озерный край"@ru,
        "sjöregion"@sv .

gn:L.RNGA a gn:Code ;
    skos:definition "a tract of land used for artillery firing practice"@en,
        "участок земли, где проходят военные артиллерийские учения"@ru ;
    skos:inScheme gn:L ;
    skos:notation "L.RNGA" ;
    skos:prefLabel "артилерийски полигон"@bg,
        "artillery range"@en,
        "militært skytefelt"@no,
        "артиллерийский полигон"@ru,
        "skjutfält"@sv .

gn:L.SALT a gn:Code ;
    skos:definition "a shallow basin or flat where salt accumulates after periodic inundation"@en,
        "мелководье или равнинная местность, где после периодических наводнений собирается соль"@ru ;
    skos:inScheme gn:L ;
    skos:notation "L.SALT" ;
    skos:prefLabel "засолени територии"@bg,
        "salt area"@en,
        "saltområde"@no,
        "солевой бассейн"@ru,
        "saltområde"@sv .

gn:L.SNOW a gn:Code ;
    skos:definition "an area of permanent snow and ice forming the accumulation area of a glacier"@en,
        "место скопления многолетнего снега и льда"@ru ;
    skos:inScheme gn:L ;
    skos:notation "L.SNOW" ;
    skos:prefLabel "перманентна снежна покривка"@bg,
        "snowfield"@en,
        "snødekt område"@no,
        "ледник"@ru,
        "snöfält"@sv .

gn:L.TRB a gn:Code ;
    skos:definition "a tract of land used by nomadic or other tribes"@en,
        "участок земли, являющийся в течение некоторого времени местом жительства для кочующих племен"@ru ;
    skos:inScheme gn:L ;
    skos:notation "L.TRB" ;
    skos:prefLabel "племенна територия"@bg,
        "tribal area"@en,
        "stammeområde"@no,
        "территория племени"@ru,
        "stamområde"@sv .

gn:L.ZZZZZ a gn:Code ;
    owl:deprecated true ;
    skos:inScheme gn:L ;
    skos:notation "L.ZZZZZ" ;
    skos:prefLabel "master source holdings list"@en .

gn:P.PPL a gn:Code ;
    skos:definition "a city, town, village, or other agglomeration of buildings where people live and work"@en,
        "место, где живут люди (город, село, поселок и т. п.)"@ru ;
    skos:inScheme gn:P ;
    skos:notation "P.PPL" ;
    skos:prefLabel "населено място"@bg,
        "populated place"@en,
        "befolket sted"@no,
        "населенный пункт"@ru,
        "befolkad plats"@sv .

gn:P.PPLA a gn:Code ;
    skos:definition "seat of a first-order administrative division (PPLC takes precedence over PPLA)"@en,
        "центр административного деления первого порядка (столица политического образования предшествует центру АТД первого порядка)"@ru ;
    skos:inScheme gn:P ;
    skos:notation "P.PPLA" ;
    skos:prefLabel "център на първостепенна административна единица"@bg,
        """seat of a first-order administrative
            division"""@en,
        "sete for primær administrativ inndeling"@no,
        "центр административного деления первого порядка"@ru,
        "säte för en första ordningens administrativ enhet"@sv .

gn:P.PPLA2 a gn:Code ;
    skos:inScheme gn:P ;
    skos:notation "P.PPLA2" ;
    skos:prefLabel "seat of a second-order administrative division"@en,
        "центр административного деления второго порядка"@ru .

gn:P.PPLA3 a gn:Code ;
    skos:inScheme gn:P ;
    skos:notation "P.PPLA3" ;
    skos:prefLabel "seat of a third-order administrative division"@en,
        "центр административного деления третьего порядка"@ru .

gn:P.PPLA4 a gn:Code ;
    skos:inScheme gn:P ;
    skos:notation "P.PPLA4" ;
    skos:prefLabel "seat of a fourth-order administrative division"@en,
        "центр административного деления четвертого порядка"@ru .

gn:P.PPLC a gn:Code ;
    skos:inScheme gn:P ;
    skos:notation "P.PPLC" ;
    skos:prefLabel "столица на политическо образувание"@bg,
        "capital of a political entity"@en,
        "Hovedstad"@no,
        "столица политического образования"@ru,
        "huvudstad i politisk enhet"@sv .

gn:P.PPLF a gn:Code ;
    skos:definition "a populated place where the population is largely engaged in agricultural activities"@en,
        "населенный пункт, где большая часть населения занята в сельским хозяйством"@ru ;
    skos:inScheme gn:P ;
    skos:notation "P.PPLF" ;
    skos:prefLabel "farm village"@en,
        "деревня"@ru .

gn:P.PPLG a gn:Code ;
    skos:inScheme gn:P ;
    skos:notation "P.PPLG" ;
    skos:prefLabel "столица на правителство на политическо образувание"@bg,
        "seat of government of a political entity"@en,
        "regjeringssete i en politisk enhet"@no,
        "здание правительства политического образования"@ru,
        "säte av ledningen för en politisk enhet"@sv .

gn:P.PPLL a gn:Code ;
    skos:definition "an area similar to a locality but with a small group of dwellings or other buildings"@en,
        "первичная единица расселения людей в пределах одного застроенного земельного участка: город, поселок городского типа, село. Обязательным признаком населенного пункта является постоянство его использования как места обитания"@ru ;
    skos:inScheme gn:P ;
    skos:notation "P.PPLL" ;
    skos:prefLabel "населено място"@bg,
        "populated locality"@en,
        "befolket trakt"@no,
        "населенный пункт"@ru,
        "befolkad ort"@sv .

gn:P.PPLQ a gn:Code ;
    skos:inScheme gn:P ;
    skos:notation "P.PPLQ" ;
    skos:prefLabel "изоставено населено място"@bg,
        "abandoned populated place"@en,
        "avfolket sted"@no,
        "покинутый населенный пункт"@ru,
        "tidigare befolkad plats"@sv .

gn:P.PPLR a gn:Code ;
    skos:definition "a populated place whose population is largely engaged in religious occupations"@en,
        "населенный пункт, где большую часть населения составляют люди, объединенные одной верой. Например, монастырь"@ru ;
    skos:inScheme gn:P ;
    skos:notation "P.PPLR" ;
    skos:prefLabel "религиозен център"@bg,
        "religious populated place"@en,
        "religiøst befolket sted"@no,
        "религиозная община"@ru,
        "religiös befolkad plats"@sv .

gn:P.PPLS a gn:Code ;
    skos:definition "cities, towns, villages, or other agglomerations of buildings where people live and work"@en,
        "первичные единицы расселения людей в пределах одного застроенного земельного участка: город, поселок городского типа, село. Обязательным признаком населенных пункт является постоянство его использования как места обитания."@ru ;
    skos:inScheme gn:P ;
    skos:notation "P.PPLS" ;
    skos:prefLabel "населени места"@bg,
        "populated places"@en,
        "befolkede steder"@no,
        "населенные пункты"@ru,
        "befolkade platser"@sv .

gn:P.PPLW a gn:Code ;
    skos:definition "a village, town or city destroyed by a natural disaster, or by war"@en,
        "населенный пункт (деревня, город), пострадавший в результате природной катастрофы или войны"@ru ;
    skos:inScheme gn:P ;
    skos:notation "P.PPLW" ;
    skos:prefLabel "разрушено населено място"@bg,
        "destroyed populated place"@en,
        "ødelagt befolket sted"@no,
        "разрушенный населенный пункт"@ru,
        "förstörd befolkad plats"@sv .

gn:P.PPLX a gn:Code ;
    skos:inScheme gn:P ;
    skos:notation "P.PPLX" ;
    skos:prefLabel "част от населено място"@bg,
        "section of populated place"@en,
        "del av befolket sted"@no,
        "участок населенного пункта"@ru,
        "del av befolkad plats"@sv .

gn:P.STLMT a gn:Code ;
    skos:inScheme gn:P ;
    skos:notation "P.STLMT" ;
    skos:prefLabel "израелски поселения"@bg,
        "israeli settlement"@en,
        "israelsk bosetning"@no,
        "еврейские поселения"@ru,
        "israelisk bosättning"@sv .

gn:R.CSWY a gn:Code ;
    skos:definition "a raised roadway across wet ground or shallow water"@en,
        "насыпная дорога для проезда, прохода через топкое место"@ru ;
    skos:inScheme gn:R ;
    skos:notation "R.CSWY" ;
    skos:prefLabel "път в блато"@bg,
        "causeway"@en,
        "veifylling"@no,
        "гать"@ru,
        "broväg, höjd gångbana"@sv .

gn:R.CSWYQ a gn:Code ;
    owl:deprecated true ;
    skos:definition "a causeway no longer used for transportation"@en ;
    skos:inScheme gn:R ;
    skos:notation "R.CSWYQ" ;
    skos:prefLabel "former causeway"@en .

gn:R.OILP a gn:Code ;
    skos:definition "a pipeline used for transporting oil"@en,
        "трубопровод для перекачки нефти и нефтепродуктов"@ru ;
    skos:inScheme gn:R ;
    skos:notation "R.OILP" ;
    skos:prefLabel "нефтопровод"@bg,
        "oil pipeline"@en,
        "oljeledning"@no,
        "нефтепровод"@ru,
        "oljepipeline"@sv .

gn:R.PRMN a gn:Code ;
    skos:definition "a place for public walking, usually along a beach front"@en,
        "место для прогулки, особ. набережная, проспект, бульвар, аллея, палуба корабля"@ru ;
    skos:inScheme gn:R ;
    skos:notation "R.PRMN" ;
    skos:prefLabel "стъргало"@bg,
        "promenade"@en,
        "promenade"@no,
        "променад"@ru,
        "promenad"@sv .

gn:R.PTGE a gn:Code ;
    skos:definition "a place where boats, goods, etc., are carried overland between navigable waters"@en,
        "перевал в верховьях рек различных бассейнов"@ru ;
    skos:inScheme gn:R ;
    skos:notation "R.PTGE" ;
    skos:prefLabel "място за пренос на лодки"@bg,
        "portage"@en,
        "eid"@no,
        "волок"@ru,
        "portage"@sv .

gn:R.RD a gn:Code ;
    skos:definition "an open way with improved surface for transportation of animals, people and vehicles"@en,
        "полоса земли, служащая для езды и ходьбы"@ru ;
    skos:inScheme gn:R ;
    skos:notation "R.RD" ;
    skos:prefLabel "път"@bg,
        "road"@en,
        "vei"@no,
        "дорога"@ru,
        "väg"@sv .

gn:R.RDA a gn:Code ;
    skos:definition "the remains of a road used by ancient cultures"@en,
        "развалины, на месте которых была дорога во времена античности"@ru ;
    skos:inScheme gn:R ;
    skos:notation "R.RDA" ;
    skos:prefLabel "античен път"@bg,
        "ancient road"@en,
        "gammel vei"@no,
        "старая дорога"@ru,
        "historisk väg"@sv .

gn:R.RDB a gn:Code ;
    skos:definition "a conspicuously curved or bent section of a road"@en,
        "изогнутый участок дороги"@ru ;
    skos:inScheme gn:R ;
    skos:notation "R.RDB" ;
    skos:prefLabel "завой на път"@bg,
        "road bend"@en,
        "veikurve"@no,
        "поворот дороги"@ru,
        "vägkrök"@sv .

gn:R.RDCUT a gn:Code ;
    skos:definition "an excavation cut through a hill or ridge for a road"@en,
        "вырытый в горном хребте туннель, через который будет проведена дорога"@ru ;
    skos:inScheme gn:R ;
    skos:notation "R.RDCUT" ;
    skos:prefLabel "прекъсване на път"@bg,
        "road cut"@en,
        "veiskjæring"@no,
        "выемка грунта под дорогу"@ru,
        "road cut"@sv .

gn:R.RDJCT a gn:Code ;
    skos:definition "a place where two or more roads join"@en,
        "место пересечения двух или более дорог"@ru ;
    skos:inScheme gn:R ;
    skos:notation "R.RDJCT" ;
    skos:prefLabel "кръстопът"@bg,
        "road junction"@en,
        "veikryss"@no,
        "перекресток"@ru,
        "vägknytpunkt"@sv .

gn:R.RJCT a gn:Code ;
    skos:definition "a place where two or more railroad tracks join"@en,
        "пункт на пересечении нескольких ж.-д. линий, представляющий собой сложный комплекс разнообразных технических сооружений и устройств"@ru ;
    skos:inScheme gn:R ;
    skos:notation "R.RJCT" ;
    skos:prefLabel "жп кръстопът"@bg,
        "railroad junction"@en,
        "jernbanekryss"@no,
        "железнодорожный узел"@ru,
        "järnvägsknytpunkt"@sv .

gn:R.RR a gn:Code ;
    skos:definition "a permanent twin steel-rail track on which freight and passenger cars move long distances"@en,
        "рельсовый путь, предназначенный для движения поездов"@ru ;
    skos:inScheme gn:R ;
    skos:notation "R.RR" ;
    skos:prefLabel "жп линия"@bg,
        "railroad"@en,
        "jernbane"@no,
        "железная дорога"@ru,
        "järnväg"@sv .

gn:R.RRQ a gn:Code ;
    skos:inScheme gn:R ;
    skos:notation "R.RRQ" ;
    skos:prefLabel "изоставена жп линия"@bg,
        "abandoned railroad"@en,
        "nedlagt jernbane"@no,
        "заброшенная железная дорога"@ru,
        "övergiven järnväg"@sv .

gn:R.RTE a gn:Code ;
    skos:definition "the route taken by caravans"@en,
        "маршрут следования караванов"@ru ;
    skos:inScheme gn:R ;
    skos:notation "R.RTE" ;
    skos:prefLabel "Керванен път"@bg,
        "caravan route"@en,
        "karavanerute"@no,
        "караванный путь"@ru,
        "karavanväg"@sv .

gn:R.RYD a gn:Code ;
    skos:definition "a system of tracks used for the making up of trains, and switching and storing freight cars"@en,
        "техническая железнодорожная станция для расформирования и формирования различных категорий поездов, выполнение техническое обслуживание и коммерческий осмотр составов поездов и устранение выявленных неисправностей вагонов, смена локомотивов и локомотивных бригад"@ru ;
    skos:inScheme gn:R ;
    skos:notation "R.RYD" ;
    skos:prefLabel "жп парк"@bg,
        "railroad yard"@en,
        "jernbaneområde"@no,
        "сортировочная станция"@ru,
        "railroad yard"@sv .

gn:R.ST a gn:Code ;
    skos:definition "a paved urban thoroughfare"@en,
        "пространство между двумя рядами домов в населенных пунктах для проезда и прохода"@ru ;
    skos:inScheme gn:R ;
    skos:notation "R.ST" ;
    skos:prefLabel "улица"@bg,
        "street"@en,
        "gate"@no,
        "улица"@ru,
        "väg"@sv .

gn:R.STKR a gn:Code ;
    skos:definition "a route taken by livestock herds"@en,
        "маршрут перегона крупного рогатого домашнего скота"@ru ;
    skos:inScheme gn:R ;
    skos:notation "R.STKR" ;
    skos:prefLabel "път на стада"@bg,
        "stock route"@en,
        "rute for krøtterdrift"@no,
        "скотопрогон"@ru,
        "boskapsled"@sv .

gn:R.TNL a gn:Code ;
    skos:definition "a subterranean passageway for transportation"@en,
        "подземное сооружение, служащее для транспортных целей"@ru ;
    skos:inScheme gn:R ;
    skos:notation "R.TNL" ;
    skos:prefLabel "тунел"@bg,
        "tunnel"@en,
        "tunnel"@no,
        "туннель"@ru,
        "tunnel"@sv .

gn:R.TNLN a gn:Code ;
    skos:definition "a cave that is open at both ends"@en,
        "пещера, открытая с двух концов"@ru ;
    skos:inScheme gn:R ;
    skos:notation "R.TNLN" ;
    skos:prefLabel "естествен тунел"@bg,
        "natural tunnel"@en,
        "naturlig tunnel"@no,
        "природный туннель"@ru,
        "naturlig tunnel"@sv .

gn:R.TNLRD a gn:Code ;
    skos:definition "a tunnel through which a road passes"@en,
        "тоннель, через который проходит дорога"@ru ;
    skos:inScheme gn:R ;
    skos:notation "R.TNLRD" ;
    skos:prefLabel "пътен тунел"@bg,
        "road tunnel"@en,
        "veitunnel"@no,
        "автодорожный туннель"@ru,
        "vägtunnel"@sv .

gn:R.TNLRR a gn:Code ;
    skos:definition "a tunnel through which a railroad passes"@en,
        "тоннель, по которому проходит ж/д дорога"@ru ;
    skos:inScheme gn:R ;
    skos:notation "R.TNLRR" ;
    skos:prefLabel "жп тунел"@bg,
        "railroad tunnel"@en,
        "jernbanetunnel"@no,
        "железнодорожный туннель"@ru,
        "järnvägstunnel"@sv .

gn:R.TNLS a gn:Code ;
    skos:definition "subterranean passageways for transportation"@en,
        "подземные  сооружение, служащие для транспортных целей"@ru ;
    skos:inScheme gn:R ;
    skos:notation "R.TNLS" ;
    skos:prefLabel "тунели"@bg,
        "tunnels"@en,
        "tunneler"@no,
        "туннели"@ru,
        "tunnlar"@sv .

gn:R.TRL a gn:Code ;
    skos:definition "a path, track, or route used by pedestrians, animals, or off-road vehicles"@en,
        "узкая пешеходная дорожка, протоптанная людьми или животными в лесу, в поле, по снегу и т. п."@ru ;
    skos:inScheme gn:R ;
    skos:notation "R.TRL" ;
    skos:prefLabel "пътека"@bg,
        "trail"@en,
        "sti"@no,
        "тропинка"@ru,
        "spår, stig"@sv .

gn:S.ADMF a gn:Code ;
    skos:definition "a government building"@en,
        "Исполнительные и распорядительные органы управления, власти в государстве."@ru ;
    skos:inScheme gn:S ;
    skos:notation "S.ADMF" ;
    skos:prefLabel "административна сграда"@bg,
        "administrative facility"@en,
        "administrasjonsanlegg"@no,
        "администрация"@ru,
        "administrativ inrättning"@sv .

gn:S.AGRF a gn:Code ;
    skos:definition "a building and/or tract of land used for improving agriculture"@en,
        "здание или участок земли, используемый для повышения качества сельскохозяйственной продукции"@ru ;
    skos:inScheme gn:S ;
    skos:notation "S.AGRF" ;
    skos:prefLabel "селскостопанска сграда"@bg,
        "agricultural facility"@en,
        "jordbruksanlegg"@no,
        "агробаза"@ru,
        "jordbruksinrättning"@sv .

gn:S.AIRB a gn:Code ;
    skos:definition "an area used to store supplies, provide barracks for air force personnel, hangars and runways for aircraft, and from which operations are initiated"@en,
        "земельный (водный) участок, предназначенный для базирования самолётов стратегической, тактической и транспортной авиации, вертолётов, частей обеспечения, ремонта, запасов материальных и технических средств обеспечения боевых действий"@ru ;
    skos:inScheme gn:S ;
    skos:notation "S.AIRB" ;
    skos:prefLabel "авиобаза"@bg,
        "airbase"@en,
        "flybase"@no,
        "авиабаза"@ru,
        "flygbas"@sv .

gn:S.AIRF a gn:Code ;
    skos:definition "a place on land where aircraft land and take off; no facilities provided for the commercial handling of passengers and cargo"@en,
        "комплекс сооружений, оборудования и земельный участок с воздушным пространством, предназначенный для взлёта, посадки, размещения и обслуживания самолётов"@ru ;
    skos:inScheme gn:S ;
    skos:notation "S.AIRF" ;
    skos:prefLabel "самолетна писта"@bg,
        "airfield"@en,
        "flyplass"@no,
        "аэродром"@ru,
        "flygfält"@sv .

gn:S.AIRH a gn:Code ;
    skos:definition "a place where helicopters land and take off"@en,
        "земельный участок, площадка на здании, судне и т.п., оборудованные для взлёта, посадки и обслуживания вертолётов"@ru ;
    skos:inScheme gn:S ;
    skos:notation "S.AIRH" ;
    skos:prefLabel "летище за хеикоптери"@bg,
        "heliport"@en,
        "heliport"@no,
        "вертолетная площадка"@ru,
        "landningsplats för helikopter"@sv .

gn:S.AIRP a gn:Code ;
    skos:definition "a place where aircraft regularly land and take off, with runways, navigational aids, and major facilities for the commercial handling of passengers and cargo"@en,
        "комплекс сооружений (с аэродромом и аэровокзалом) для осуществления регулярных полётов транспортной авиации и обслуживания пассажиров"@ru ;
    skos:inScheme gn:S ;
    skos:notation "S.AIRP" ;
    skos:prefLabel "летище"@bg,
        "airport"@en,
        "lufthavn"@no,
        "аэропорт"@ru,
        "flygplats"@sv .

gn:S.AIRQ a gn:Code ;
    skos:inScheme gn:S ;
    skos:notation "S.AIRQ" ;
    skos:prefLabel "изоставено летище"@bg,
        "abandoned airfield"@en,
        "forlatt lufthavn"@no,
        "заброшенный аэродром"@ru,
        "övergivet flygfält"@sv .

gn:S.AMTH a gn:Code ;
    skos:definition "an oval or circular structure with rising tiers of seats about a stage or open space"@en,
        "декоративное сооружение в форме эллипса со ступенчато расположенными рядами сидений, предназначенное для зрелищных мероприятий"@ru ;
    skos:inScheme gn:S ;
    skos:notation "S.AMTH" ;
    skos:prefLabel "амфитеатър"@bg,
        "amphitheater"@en,
        "amfiteater"@no,
        "амфитеатр"@ru,
        "amfiteater"@sv .

gn:S.ANS a gn:Code ;
    skos:definition "a place where archeological remains, old structures, or cultural artifacts are located"@en,
        "остатки древнего укрепленного поселения или города"@ru ;
    skos:inScheme gn:S ;
    skos:notation "S.ANS" ;
    skos:prefLabel "антични останки"@bg,
        "ancient site"@en,
        "historisk sted"@no,
        "городище"@ru,
        "forntida lämning"@sv .

gn:S.AQC a gn:Code ;
    skos:definition "facility or area for the cultivation of aquatic animals and plants, especially fish, shellfish, and seaweed, in natural or controlled marine or freshwater environments; underwater agriculture"@en ;
    skos:historyNote "Added in v3.0"@en ;
    skos:inScheme gn:S ;
    skos:notation "S.AQC" ;
    skos:prefLabel "aquaculture facility"@en .

gn:S.ARCH a gn:Code ;
    skos:definition "a natural or man-made structure in the form of an arch"@en,
        "декоративное сооружение в виде больших ворот со сводом"@ru ;
    skos:inScheme gn:S ;
    skos:notation "S.ARCH" ;
    skos:prefLabel "арка"@bg,
        "arch"@en,
        "bue"@no,
        "арка"@ru,
        "båge, valv"@sv .

gn:S.ASTR a gn:Code ;
    skos:definition "a point on the earth whose position has been determined by observations of celestial bodies"@en,
        "научное учреждение, ведущее астрономические и геофизические наблюдения и исследования; здание, специально оборудованное для таких наблюдений"@ru ;
    skos:inScheme gn:S ;
    skos:notation "S.ASTR" ;
    skos:prefLabel "астрономическа станция"@bg,
        "astronomical station"@en,
        "astronomisk stasjon"@no,
        "обсерватория"@ru,
        "astronomisk station"@sv .

gn:S.ASYL a gn:Code ;
    skos:definition "a facility where the insane are cared for and protected"@en,
        "место, где можно укрыться, скрыться от чего-н."@ru ;
    skos:inScheme gn:S ;
    skos:notation "S.ASYL" ;
    skos:prefLabel "лудница"@bg,
        "asylum"@en,
        "asyl"@no,
        "убежище"@ru,
        "mentalsjukhus"@sv .

gn:S.ATHF a gn:Code ;
    skos:definition "a tract of land used for playing team sports, and athletic track and field events"@en,
        "комплексное спортивное сооружение со специально оборудованными площадками для состязаний, тренировок, вспомогательными помещениями и трибунами для зрителей"@ru ;
    skos:inScheme gn:S ;
    skos:notation "S.ATHF" ;
    skos:prefLabel "спортно игрище"@bg,
        "athletic field"@en,
        "idrettsbane"@no,
        "стадион"@ru,
        "idrottsfält"@sv .

gn:S.ATM a gn:Code ;
    skos:definition "An unattended electronic machine in a public place, connected to a data system and related equipment and activated by a bank customer to obtain cash withdrawals and other banking services."@en,
        "автоматическое устройство, предназначенное для получения наличных денег по кредитной карточке."@ru ;
    skos:inScheme gn:S ;
    skos:notation "S.ATM" ;
    skos:prefLabel "automatic teller machine"@bg,
        "automatic teller machine"@en,
        "automatic teller machine"@no,
        "банкомат"@ru,
        "bankomat"@sv .

gn:S.BANK a gn:Code ;
    skos:definition "A business establishment in which money is kept for saving or commercial purposes or is invested, supplied for loans, or exchanged."@en,
        "особые экономические институты, осуществляющие: аккумуляцию денежных средств и накоплений, предоставление кредита, проведение денежных расчётов, выпуск в обращение определённых видов денег"@ru ;
    skos:inScheme gn:S ;
    skos:notation "S.BANK" ;
    skos:prefLabel "bank"@en .

gn:S.BCN a gn:Code ;
    skos:definition "a fixed artificial navigation mark"@en,
        "устройство, оборудованное звуковой, световой или радиотехнической сигнализацией для навигационного ориентирования судов, самолетов и т.п."@ru ;
    skos:inScheme gn:S ;
    skos:notation "S.BCN" ;
    skos:prefLabel "фар"@bg,
        "beacon"@en,
        "signalstasjon"@no,
        "маяк"@ru,
        "båk, fyrtorn"@sv .

gn:S.BDG a gn:Code ;
    skos:definition "a structure erected across an obstacle such as a stream, road, etc., in order to carry roads, railroads, and pedestrians across"@en,
        "сооружение для перехода, переезда через реку, овраг, железнодорожный путь и т.п."@ru ;
    skos:inScheme gn:S ;
    skos:notation "S.BDG" ;
    skos:prefLabel "мост"@bg,
        "bridge"@en,
        "bro"@no,
        "мост"@ru,
        "bro"@sv .

gn:S.BDGQ a gn:Code ;
    skos:definition "a destroyed or decayed bridge which is no longer functional"@en,
        "мост, который больше не функционирует"@ru ;
    skos:inScheme gn:S ;
    skos:notation "S.BDGQ" ;
    skos:prefLabel "останки от мост"@bg,
        "ruined bridge"@en,
        "ødelagt bro"@no,
        "разрушенный мост"@ru,
        "raserad bro"@sv .

gn:S.BLDG a gn:Code ;
    skos:definition "a structure built for permanent use, as a house, factory, etc."@en,
        "архитектурное сооружение, постройка (обычно больших размеров), например, дом, завод и т.п."@ru ;
    skos:inScheme gn:S ;
    skos:notation "S.BLDG" ;
    skos:prefLabel "сграда(и)"@bg,
        "building(s)"@en,
        "bygning"@no,
        "здание"@ru,
        "byggnad"@sv .

gn:S.BLDO a gn:Code ;
    skos:definition "commercial building where business and/or services are conducted"@en ;
    skos:historyNote "Added in v3.0"@en ;
    skos:inScheme gn:S ;
    skos:notation "S.BLDO" ;
    skos:prefLabel "office building"@en .

gn:S.BP a gn:Code ;
    skos:definition "a fixture marking a point along a boundary"@en,
        "ограничительный знак, используемый для обозначения границ"@ru ;
    skos:inScheme gn:S ;
    skos:notation "S.BP" ;
    skos:prefLabel "граничен пазар"@bg,
        "boundary marker"@en,
        "grensemarkør"@no,
        "межевой знак"@ru,
        "gränsmärke"@sv .

gn:S.BRKS a gn:Code ;
    skos:definition "a building for lodging military personnel"@en,
        "шалаши, временные, легкие строения для размещения войск или рабочих"@ru ;
    skos:inScheme gn:S ;
    skos:notation "S.BRKS" ;
    skos:prefLabel "бараки"@bg,
        "barracks"@en,
        "brakker"@no,
        "бараки"@ru,
        "kaserner"@sv .

gn:S.BRKW a gn:Code ;
    skos:definition "a structure erected to break the force of waves at the entrance to a harbor or port"@en,
        "гидротехническое сооружение для защиты места стоянки судов или берега от разрушительного действия волн"@ru ;
    skos:inScheme gn:S ;
    skos:notation "S.BRKW" ;
    skos:prefLabel "вълнолом"@bg,
        "breakwater"@en,
        "bølgebryter"@no,
        "волнорез"@ru,
        "vågbrytare"@sv .

gn:S.BSTN a gn:Code ;
    skos:definition "a facility for baling agricultural products"@en,
        "место, где прессуют сено в тюки"@ru ;
    skos:inScheme gn:S ;
    skos:notation "S.BSTN" ;
    skos:prefLabel "товарна станция"@bg,
        "baling station"@en,
        "ballestasjon"@no,
        "прессовальная станция"@ru,
        "baling station"@sv .

gn:S.BTYD a gn:Code ;
    skos:definition "a waterside facility for servicing, repairing, and building small vessels"@en,
        "расположенное на берегу моря, реки и т.п.  сооружение, которое занимается обслуживанием, ремонтом и изготовлением лодок"@ru ;
    skos:inScheme gn:S ;
    skos:notation "S.BTYD" ;
    skos:prefLabel "лодкостоянка"@bg,
        "boatyard"@en,
        "verft"@no,
        "лодочная мастерская"@ru,
        "skeppsvarv"@sv .

gn:S.BUR a gn:Code ;
    skos:definition "a cave used for human burials"@en,
        "яма для погребения умершего"@ru ;
    skos:inScheme gn:S ;
    skos:notation "S.BUR" ;
    skos:prefLabel "пгребална пещера(и)"@bg,
        "burial cave(s)"@en,
        "gravhule"@no,
        "могила"@ru,
        "begravningsgrotta(or)"@sv .

gn:S.BUSTN a gn:Code ;
    skos:definition "a facility comprising ticket office, platforms, etc. for loading and unloading passengers"@en,
        "транспортное предприятие для обслуживания пассажиров междугородных и пригородных автобусных сообщений"@ru ;
    skos:inScheme gn:S ;
    skos:notation "S.BUSTN" ;
    skos:prefLabel "bus station"@en,
        "автостанция"@ru .

gn:S.BUSTP a gn:Code ;
    skos:definition "a place lacking station facilities"@en,
        "пункт, место, установленные для посадки и высадки пассажиров"@ru ;
    skos:inScheme gn:S ;
    skos:notation "S.BUSTP" ;
    skos:prefLabel "bus stop"@en,
        "автобусная остановка"@ru,
        "Busshållplats"@sv .

gn:S.CARN a gn:Code ;
    skos:definition "a heap of stones erected as a landmark or for other purposes"@en,
        "груда камней, служащая условным знаком, надгробным памятником и т.п."@ru ;
    skos:inScheme gn:S ;
    skos:notation "S.CARN" ;
    skos:prefLabel "грамада"@bg,
        "cairn"@en,
        "varde"@no,
        "пирамида из камней"@ru,
        "stenkummel"@sv .

gn:S.CAVE a gn:Code ;
    skos:definition "an underground passageway or chamber, or cavity on the side of a cliff"@en,
        "углубление, полое пространство, образовавшееся в земной коре, горных массивах естественным путём или созданные человеком, с выходом наружу"@ru ;
    skos:inScheme gn:S ;
    skos:notation "S.CAVE" ;
    skos:prefLabel "пещера(и)"@bg,
        "cave(s)"@en,
        "grotte"@no,
        "пещера"@ru,
        "grotta(or)"@sv .

gn:S.CCL a gn:Code ;
    owl:deprecated true ;
    skos:definition "Centres for Continuous Learning"@en ;
    skos:inScheme gn:S ;
    skos:notation "S.CCL" ;
    skos:prefLabel "Centre Continuous Learning"@en .

gn:S.CH a gn:Code ;
    skos:definition "a building for public Christian worship"@en,
        "здание, в котором происходит христианское богослужение"@ru ;
    skos:inScheme gn:S ;
    skos:notation "S.CH" ;
    skos:prefLabel "църква"@bg,
        "church"@en,
        "kirke"@no,
        "церковь"@ru,
        "kyrka"@sv .

gn:S.CMP a gn:Code ;
    skos:definition "a site occupied by tents, huts, or other shelters for temporary use"@en,
        "временное поселение, стоянка"@ru ;
    skos:inScheme gn:S ;
    skos:notation "S.CMP" ;
    skos:prefLabel "лагер(и)"@bg,
        "camp(s)"@en,
        "leir"@no,
        "лагерь"@ru,
        "läger"@sv .

gn:S.CMPL a gn:Code ;
    skos:definition "a camp used by loggers"@en,
        "временное поселение лесозаготовителей"@ru ;
    skos:inScheme gn:S ;
    skos:notation "S.CMPL" ;
    skos:prefLabel "лагер на дървосекачи"@bg,
        "logging camp"@en,
        "tømmerkoie"@no,
        "лесной поселок"@ru,
        "logging camp"@sv .

gn:S.CMPLA a gn:Code ;
    skos:definition "a camp used by migrant or temporary laborers"@en,
        "лагерь, в котором живут трудовые мигранты, приезжающие на заработки"@ru ;
    skos:inScheme gn:S ;
    skos:notation "S.CMPLA" ;
    skos:prefLabel "трудов лагер"@bg,
        "labor camp"@en,
        "arbeidsleir"@no,
        "лагерь сезонных рабочих"@ru,
        "arbetsläger"@sv .

gn:S.CMPMN a gn:Code ;
    skos:definition "a camp used by miners"@en,
        "временное поселение горняков"@ru ;
    skos:inScheme gn:S ;
    skos:notation "S.CMPMN" ;
    skos:prefLabel "миньорски лагер"@bg,
        "mining camp"@en,
        "gruveleir"@no,
        "рудничный поселок"@ru,
        "gruvläger"@sv .

gn:S.CMPO a gn:Code ;
    skos:definition "a camp used by oilfield workers"@en,
        "поселок, в котором живут работники нефтяной промышленности"@ru ;
    skos:inScheme gn:S ;
    skos:notation "S.CMPO" ;
    skos:prefLabel "лагер на нефторъботници"@bg,
        "oil camp"@en,
        "oljeleir"@no,
        "поселок нефтяников"@ru,
        "oljeläger"@sv .

gn:S.CMPQ a gn:Code ;
    skos:inScheme gn:S ;
    skos:notation "S.CMPQ" ;
    skos:prefLabel "изоставен лагер"@bg,
        "abandoned camp"@en,
        "forlatt leir"@no,
        "покинутый лагерь/поселок"@ru,
        "övergivet läger"@sv .

gn:S.CMPRF a gn:Code ;
    skos:definition "a camp used by refugees"@en,
        "лагерь, в котором живут беженцы (люди, покинувшие место своего жительства, спасаясь от бедствия (землетрясения, войны, голода и т.п.)"@ru ;
    skos:inScheme gn:S ;
    skos:notation "S.CMPRF" ;
    skos:prefLabel "бежански лагер"@bg,
        "refugee camp"@en,
        "flyktningleir"@no,
        "лагерь беженцев"@ru,
        "flyktingläger"@sv .

gn:S.CMTY a gn:Code ;
    skos:definition "a burial place or ground"@en,
        "место, предназначенное для погребения умерших"@ru ;
    skos:inScheme gn:S ;
    skos:notation "S.CMTY" ;
    skos:prefLabel "гробище"@bg,
        "cemetery"@en,
        "gravlund"@no,
        "кладбище"@ru,
        "kyrkogård"@sv .

gn:S.COMC a gn:Code ;
    skos:definition "a facility, including buildings, antennae, towers and electronic equipment for receiving and transmitting information"@en,
        "совокупность технических средств оператора связи, обеспечивающих оказание услуг связи и присоединение к сети общего пользования"@ru ;
    skos:inScheme gn:S ;
    skos:notation "S.COMC" ;
    skos:prefLabel "комуникационен център"@bg,
        "communication center"@en,
        "узел связи"@ru .

gn:S.CRRL a gn:Code ;
    skos:definition "a pen or enclosure for confining or capturing animals"@en,
        "загон для скота"@ru ;
    skos:inScheme gn:S ;
    skos:notation "S.CRRL" ;
    skos:prefLabel "заграждение(я) за добитък"@bg,
        "corral(s)"@en,
        "innhegning"@no,
        "корраль"@ru,
        "fålla, inhägnad"@sv .

gn:S.CSNO a gn:Code ;
    skos:definition "a building used for entertainment, especially gambling"@en,
        "игорный дом, в котором осуществляется проведение азартных игр"@ru ;
    skos:inScheme gn:S ;
    skos:notation "S.CSNO" ;
    skos:prefLabel "казино"@bg,
        "casino"@en,
        "kasino"@no,
        "казино"@ru,
        "kasino"@sv .

gn:S.CSTL a gn:Code ;
    skos:definition "a large fortified building or set of buildings"@en,
        "здание (или комплекс зданий), сочетающие в себе жилые и оборонительно функции"@ru ;
    skos:inScheme gn:S ;
    skos:notation "S.CSTL" ;
    skos:prefLabel "замък"@bg,
        "castle"@en,
        "slott"@no,
        "замок"@ru,
        "slott"@sv .

gn:S.CSTM a gn:Code ;
    skos:definition "a building in a port where customs and duties are paid, and where vessels are entered and cleared"@en,
        "помещение, где размещается учреждение, ведающее контролем провоза через границу грузов, багажа, почты и собирающее пошлину за такой провоз"@ru ;
    skos:inScheme gn:S ;
    skos:notation "S.CSTM" ;
    skos:prefLabel "митница"@bg,
        "customs house"@en,
        "tollbod"@no,
        "таможня"@ru,
        "tullhus"@sv .

gn:S.CTHSE a gn:Code ;
    skos:definition "a building in which courts of law are held"@en,
        "здание, в котором проходят заседания суда"@ru ;
    skos:inScheme gn:S ;
    skos:notation "S.CTHSE" ;
    skos:prefLabel "съдебна сграда"@bg,
        "courthouse"@en,
        "rettsbygning"@no,
        "здание суда"@ru,
        "domstolsbyggnad"@sv .

gn:S.CTRA a gn:Code ;
    skos:definition "a facility where atomic research is carried out"@en,
        "научный центр, в котором проводятся атомные исследования"@ru ;
    skos:inScheme gn:S ;
    skos:notation "S.CTRA" ;
    skos:prefLabel "атомен център"@bg,
        "atomic center"@en,
        "atomsenter"@no,
        "центр атомных исследований"@ru,
        "atomcentrum"@sv .

gn:S.CTRCM a gn:Code ;
    skos:definition "a facility for community recreation and other activities"@en,
        "помещение для проведения культурных и общественных мероприятий"@ru ;
    skos:inScheme gn:S ;
    skos:notation "S.CTRCM" ;
    skos:prefLabel "обществен център"@bg,
        "community center"@en,
        "kommunesenter"@no,
        "дом культуры"@ru,
        "kulturcentrum"@sv .

gn:S.CTRF a gn:Code ;
    skos:definition "a place where more than one facility is situated"@en,
        "центр, предоставляющий не одну, а сразу несколько услуг одновременно"@ru ;
    skos:inScheme gn:S ;
    skos:notation "S.CTRF" ;
    skos:prefLabel "паркинг"@bg,
        "facility center"@en,
        "tjenestesenter"@no,
        "центр обслуживания"@ru,
        "tjänstecentrum"@sv .

gn:S.CTRM a gn:Code ;
    skos:definition "a complex of health care buildings including two or more of the following: hospital, medical school, clinic, pharmacy, doctor's offices, etc."@en,
        "комплекс лечебных учреждений; включает в себя: больницу, поликлинику, аптеку, медицинский институт"@ru ;
    skos:inScheme gn:S ;
    skos:notation "S.CTRM" ;
    skos:prefLabel "медицински център"@bg,
        "medical center"@en,
        "legesenter"@no,
        "медицинский центр"@ru,
        "medicinskt center"@sv .

gn:S.CTRR a gn:Code ;
    skos:definition "a facility where more than one religious activity is carried out, e.g., retreat, school, monastery, worship"@en,
        "комплекс нескольких религиозных учреждений (монашеская обитель, школа для священнослужителей, церковь)"@ru ;
    skos:inScheme gn:S ;
    skos:notation "S.CTRR" ;
    skos:prefLabel "религиозен център"@bg,
        "religious center"@en,
        "religiøst senter"@no,
        "религиозный центр"@ru,
        "religiöst center"@sv .

gn:S.CTRS a gn:Code ;
    skos:definition "a facility for launching, tracking, or controlling satellites and space vehicles"@en,
        "центр, который осуществляет запуск и наблюдение за полетом искусственных спутников земли и космических кораблей"@ru ;
    skos:inScheme gn:S ;
    skos:notation "S.CTRS" ;
    skos:prefLabel "космически център"@bg,
        "space center"@en,
        "romsenter"@no,
        "космический центр"@ru,
        "rymdcenter"@sv .

gn:S.CVNT a gn:Code ;
    skos:definition "a building where a community of nuns lives in seclusion"@en,
        "обитель, общежитие монахинь"@ru ;
    skos:inScheme gn:S ;
    skos:notation "S.CVNT" ;
    skos:prefLabel "женски манастир"@bg,
        "convent"@en,
        "kloster"@no,
        "женский монастырь"@ru,
        "kloster"@sv .

gn:S.DAM a gn:Code ;
    skos:definition "a barrier constructed across a stream to impound water"@en,
        "гидротехническое сооружение, искусственная насыпь для предохранения местности от затопления, для ограждения водохранилищ и т.п."@ru ;
    skos:inScheme gn:S ;
    skos:notation "S.DAM" ;
    skos:prefLabel "язовирна стена"@bg,
        "dam"@en,
        "demning"@no,
        "дамба"@ru,
        "damm"@sv .

gn:S.DAMQ a gn:Code ;
    skos:definition "a destroyed or decayed dam which is no longer functional"@en,
        "дамба, которая больше не функционирует"@ru ;
    skos:inScheme gn:S ;
    skos:notation "S.DAMQ" ;
    skos:prefLabel "разрушена язовирна стена"@bg,
        "ruined dam"@en,
        "ødelagt demning"@no,
        "разрушенная дамба"@ru,
        "förstörd damm"@sv .

gn:S.DAMSB a gn:Code ;
    skos:definition "a dam put down to bedrock in a sand river"@en,
        "дамба, возведенная на  песчаном дне реки"@ru ;
    skos:inScheme gn:S ;
    skos:notation "S.DAMSB" ;
    skos:prefLabel "нископовърхностна стена"@bg,
        "sub-surface dam"@en,
        "demning gravd ned til grunnfjellet"@no,
        "грунтовая дамба"@ru,
        "underjordisk damm"@sv .

gn:S.DARY a gn:Code ;
    skos:definition "a facility for the processing, sale and distribution of milk or milk products"@en,
        "предприятие по производству молочных продуктов"@ru ;
    skos:inScheme gn:S ;
    skos:notation "S.DARY" ;
    skos:prefLabel "мандра"@bg,
        "dairy"@en,
        "meieri"@no,
        "молочный комбинат"@ru,
        "mejeri"@sv .

gn:S.DCKD a gn:Code ;
    skos:definition "a dock providing support for a vessel, and means for removing the water so that the bottom of the vessel can be exposed"@en,
        "портовое сооружение для ремонта и постройки судов; сухой док сооружается на защищённой от волнения акватории и представляет собой отделяемую от неё с торца затвором водонепроницаемую камеру"@ru ;
    skos:inScheme gn:S ;
    skos:notation "S.DCKD" ;
    skos:prefLabel "сух док"@bg,
        "dry dock"@en,
        "demning gravd ned til grunnfjellet"@no,
        "сухой док"@ru,
        "torrdocka"@sv .

gn:S.DCKY a gn:Code ;
    skos:definition "a facility for servicing, building, or repairing ships"@en,
        "предприятие для постройки и ремонта судов"@ru ;
    skos:inScheme gn:S ;
    skos:notation "S.DCKY" ;
    skos:prefLabel "корабостроителница"@bg,
        "dockyard"@en,
        "skipsverft"@no,
        "верфь"@ru,
        "skeppsvarv"@sv .

gn:S.DIKE a gn:Code ;
    skos:definition "an earth or stone embankment usually constructed for flood or stream control"@en,
        "неглубокий и неширокий ров, обычно служащий для спуска или отвода воды"@ru ;
    skos:inScheme gn:S ;
    skos:notation "S.DIKE" ;
    skos:prefLabel "дига"@bg,
        "dike"@en,
        "dike"@no,
        "канава"@ru,
        "damm, fördämning, bank"@sv .

gn:S.DIP a gn:Code ;
    skos:definition "office, residence, or facility of a foreign government, which may include an embassy, consulate, chancery, office of charge d?affaires, or other diplomatic, economic, military, or cultural mission"@en,
        "office, residence, or facility of a foreign government, which may include an embassy, consulate, chancery, office of charge d?affaires, or other diplomatic, economic, military, or cultural mission"@ru ;
    skos:historyNote "Added in v3.0"@en ;
    skos:inScheme gn:S ;
    skos:notation "S.DIP" ;
    skos:prefLabel "diplomatic facility"@en .

gn:S.DPOF a gn:Code ;
    skos:definition "an area where fuel is stored"@en,
        "специальное помещение, предназначенное для хранения горючего"@ru ;
    skos:inScheme gn:S ;
    skos:notation "S.DPOF" ;
    skos:prefLabel "горивно депо"@bg,
        "fuel depot"@en,
        "brennstofflager"@no,
        "склад горючего"@ru,
        "bränsledepå"@sv .

gn:S.EST a gn:Code ;
    skos:definition "a large commercialized agricultural landholding with associated buildings and other facilities"@en,
        "крупное земельное владение, обычно с усадьбой"@ru ;
    skos:inScheme gn:S ;
    skos:notation "S.EST" ;
    skos:prefLabel "имение(я)"@bg,
        "estate(s)"@en,
        "gods"@no,
        "поместье"@ru,
        "egendom(ar)"@sv .

gn:S.ESTB a gn:Code ;
    owl:deprecated true ;
    skos:definition "an estate that specializes in the growing of bananas"@en ;
    skos:inScheme gn:S ;
    skos:notation "S.ESTB" ;
    skos:prefLabel "banana plantation"@en .

gn:S.ESTC a gn:Code ;
    owl:deprecated true ;
    skos:definition "an estate specializing in the cultivation of cotton"@en ;
    skos:inScheme gn:S ;
    skos:notation "S.ESTC" ;
    skos:prefLabel "cotton plantation"@en .

gn:S.ESTO a gn:Code ;
    skos:definition "an estate specializing in the cultivation of oil palm trees"@en,
        "большая земельная площадь, на которой выращивают масличные пальмы"@ru ;
    skos:inScheme gn:S ;
    skos:notation "S.ESTO" ;
    skos:prefLabel "плантация за маслена палма"@bg,
        "oil palm plantation"@en,
        "oljepalmeplantasje"@no,
        "плантация масличных пальм"@ru,
        "oljepalmsplantage"@sv .

gn:S.ESTR a gn:Code ;
    skos:definition "an estate which specializes in growing and tapping rubber trees"@en,
        "большая земельная площадь, на которой выращивают каучуковые деревья"@ru ;
    skos:inScheme gn:S ;
    skos:notation "S.ESTR" ;
    skos:prefLabel "каучукова плантация"@bg,
        "rubber plantation"@en,
        "gummiplantasje"@no,
        "каучуковая плантация"@ru,
        "gummiplantage"@sv .

gn:S.ESTSG a gn:Code ;
    skos:definition "an estate that specializes in growing sugar cane"@en,
        "большая земельная площадь, на которой выращивают сахарный тростник"@ru ;
    skos:inScheme gn:S ;
    skos:notation "S.ESTSG" ;
    skos:prefLabel "захарна плантация"@bg,
        "sugar plantation"@en,
        "sukkerplantasje"@no,
        "сахарная плантация"@ru,
        "sockerplantage"@sv .

gn:S.ESTSL a gn:Code ;
    owl:deprecated true ;
    skos:definition "an estate that specializes in growing sisal"@en ;
    skos:inScheme gn:S ;
    skos:notation "S.ESTSL" ;
    skos:prefLabel "sisal plantation"@en .

gn:S.ESTT a gn:Code ;
    skos:definition "an estate which specializes in growing tea bushes"@en,
        "большая земельная площадь, на которой выращивают чай"@ru ;
    skos:inScheme gn:S ;
    skos:notation "S.ESTT" ;
    skos:prefLabel "чайна плантация"@bg,
        "tea plantation"@en,
        "teplantasje"@no,
        "чайная плантация"@ru,
        "teplantage"@sv .

gn:S.ESTX a gn:Code ;
    skos:inScheme gn:S ;
    skos:notation "S.ESTX" ;
    skos:prefLabel "част от имение"@bg,
        "section of estate"@en,
        "del av gods"@no,
        "участок плантации"@ru,
        "del av egendom"@sv .

gn:S.FCL a gn:Code ;
    skos:definition "a building or buildings housing a center, institute, foundation, hospital, prison, mission, courthouse, etc."@en,
        "организация, образуемая для осуществления определённого рода деятельности (Государственное у. Общественные учреждения. Научные учреждения. Торговое, лечебно-профилактическое, административное у.)"@ru ;
    skos:inScheme gn:S ;
    skos:notation "S.FCL" ;
    skos:prefLabel "съоръжение"@bg,
        "facility"@en,
        "anlegg"@no,
        "учреждение"@ru,
        "inrättning"@sv .

gn:S.FNDY a gn:Code ;
    skos:definition "a building or works where metal casting is carried out"@en,
        "мастерская, в которой происходит обработка металла путем плавления и заливки в литейные формы"@ru ;
    skos:inScheme gn:S ;
    skos:notation "S.FNDY" ;
    skos:prefLabel "леярна"@bg,
        "foundry"@en,
        "støperi"@no,
        "литейный цех"@ru,
        "gjuteri"@sv .

gn:S.FRM a gn:Code ;
    skos:definition "a tract of land with associated buildings devoted to agriculture"@en,
        "частное сельскохозяйственное предприятие, принадлежащее фермеру и ведущееся им на собственной или арендованной земле"@ru ;
    skos:inScheme gn:S ;
    skos:notation "S.FRM" ;
    skos:prefLabel "ферма"@bg,
        "farm"@en,
        "gård"@no,
        "ферма"@ru,
        "farm"@sv .

gn:S.FRMQ a gn:Code ;
    skos:inScheme gn:S ;
    skos:notation "S.FRMQ" ;
    skos:prefLabel "изоставена ферма"@bg,
        "abandoned farm"@en,
        "forlatt gård"@no,
        "покинутая (заброшенная) ферма"@ru,
        "övergiven farm"@sv .

gn:S.FRMS a gn:Code ;
    skos:definition "tracts of land with associated buildings devoted to agriculture"@en,
        "частные сельскохозяйственные предприятия, принадлежащие фермеру и ведущиеся им на собственной или арендованной земле"@ru ;
    skos:inScheme gn:S ;
    skos:notation "S.FRMS" ;
    skos:prefLabel "ферми"@bg,
        "farms"@en,
        "gårder"@no,
        "фермы"@ru,
        "farmer"@sv .

gn:S.FRMT a gn:Code ;
    skos:definition "the buildings and adjacent service areas of a farm"@en,
        "жилой дом с примыкающими надворными постройками и угодьями (сад, огород и т.п.), представляющий собой отдельное хозяйство (преимущественно в сельской местности)"@ru ;
    skos:inScheme gn:S ;
    skos:notation "S.FRMT" ;
    skos:prefLabel "чифлик"@bg,
        "farmstead"@en,
        "gårdsbruk"@no,
        "усадьба"@ru,
        "bondgård"@sv .

gn:S.FT a gn:Code ;
    skos:definition "a defensive structure or earthworks"@en,
        "защитное сооружение или земляное укрепление"@ru ;
    skos:inScheme gn:S ;
    skos:notation "S.FT" ;
    skos:prefLabel "форт"@bg,
        "fort"@en,
        "fort"@no,
        "крепость"@ru,
        "fort"@sv .

gn:S.FY a gn:Code ;
    skos:definition "a boat or other floating conveyance and terminal facilities regularly used to transport people and vehicles across a waterbody"@en,
        "плоскодонное судно, плот для переправы людей, транспорта, грузов через реку, озеро или пролив"@ru ;
    skos:inScheme gn:S ;
    skos:notation "S.FY" ;
    skos:prefLabel "ферибот"@bg,
        "ferry"@en,
        "ferge"@no,
        "паром"@ru,
        "färja"@sv .

gn:S.GATE a gn:Code ;
    skos:definition "a controlled access entrance or exit"@en,
        "конструкция для регулирования входа и выхода"@ru ;
    skos:inScheme gn:S ;
    skos:notation "S.GATE" ;
    skos:prefLabel "бариера"@bg,
        "gate"@en,
        "grind"@no,
        "ворота"@ru,
        "grind,port"@sv .

gn:S.GDN a gn:Code ;
    skos:definition "an enclosure for displaying selected plant or animal life"@en,
        "участок земли для выращивания садовых растений"@ru ;
    skos:inScheme gn:S ;
    skos:notation "S.GDN" ;
    skos:prefLabel "градина(и)"@bg,
        "garden(s)"@en,
        "hage"@no,
        "сад"@ru,
        "trädgård(ar)"@sv .

gn:S.GHAT a gn:Code ;
    skos:definition "a set of steps leading to a river, which are of religious significance, and at their base is usually a platform for bathing"@en,
        "a set of steps leading to a river, which are of religious significance, and at their base is usually a platform for bathing"@ru ;
    skos:historyNote "Added in v3.0"@en ;
    skos:inScheme gn:S ;
    skos:notation "S.GHAT" ;
    skos:prefLabel "ghat"@en .

gn:S.GHSE a gn:Code ;
    skos:definition "a house used to provide lodging for paying guests"@en,
        "дом с меблированными комнатами («номерами») для временного проживания путешественников"@ru ;
    skos:inScheme gn:S ;
    skos:notation "S.GHSE" ;
    skos:prefLabel "къща за гости"@bg,
        "guest house"@en,
        "gjestehus"@no,
        "гостиница"@ru,
        "gästhus"@sv .

gn:S.GOSP a gn:Code ;
    skos:definition "a facility for separating gas from oil"@en,
        "аппарат для отделения газа от нефти"@ru ;
    skos:inScheme gn:S ;
    skos:notation "S.GOSP" ;
    skos:prefLabel "сепаратор на нефт-гас"@bg,
        "gas-oil separator plant"@en,
        "separasjonsanlegg for gass og olje"@no,
        "нефтегазовый сепаратор"@ru,
        "gas och olje separator"@sv .

gn:S.GOVL a gn:Code ;
    skos:definition "a facility housing local governmental offices, usually a city, town, or village hall"@en ;
    skos:historyNote "Added in v3.0"@en ;
    skos:inScheme gn:S ;
    skos:notation "S.GOVL" ;
    skos:prefLabel "local government office"@en .

gn:S.GRVE a gn:Code ;
    skos:definition "a burial site"@en,
        "место захоронения"@ru ;
    skos:inScheme gn:S ;
    skos:notation "S.GRVE" ;
    skos:prefLabel "гроб"@bg,
        "grave"@en,
        "grav"@no,
        "могила"@ru,
        "grav"@sv .

gn:S.HERM a gn:Code ;
    skos:definition "a secluded residence, usually for religious sects"@en,
        "жилище монахов-отшельников"@ru ;
    skos:inScheme gn:S ;
    skos:notation "S.HERM" ;
    skos:prefLabel "отшелническа килия"@bg,
        "hermitage"@en,
        "eneboerhytte"@no,
        "скит"@ru,
        "eremitage"@sv .

gn:S.HLT a gn:Code ;
    skos:definition "a place where caravans stop for rest"@en,
        "место, где караваны останавливаются, чтобы передохнуть"@ru ;
    skos:inScheme gn:S ;
    skos:notation "S.HLT" ;
    skos:prefLabel "отбивка за почивка"@bg,
        "halting place"@en,
        "stoppested"@no,
        "место привала"@ru,
        "halting place"@sv .

gn:S.HMSD a gn:Code ;
    skos:definition "a residence, owner's or manager's, on a sheep or cattle station, woolshed, outcamp, or Aboriginal outstation, specific to Australia and New Zealand" ;
    skos:historyNote "Added in v3.1"@en ;
    skos:inScheme gn:S ;
    skos:notation "S.HMSD" ;
    skos:prefLabel "homestead"@en .

gn:S.HSE a gn:Code ;
    skos:definition "a building used as a human habitation"@en,
        "жилое здание, строение"@ru ;
    skos:inScheme gn:S ;
    skos:notation "S.HSE" ;
    skos:prefLabel "къща(и)"@bg,
        "house(s)"@en,
        "hus"@no,
        "дом"@ru,
        "hus"@sv .

gn:S.HSEC a gn:Code ;
    skos:definition "a large house, mansion, or chateau, on a large estate"@en,
        "дом, находящийся за городом, вне города, вблизи от него"@ru ;
    skos:inScheme gn:S ;
    skos:notation "S.HSEC" ;
    skos:prefLabel "селска къща"@bg,
        "country house"@en,
        "landsted"@no,
        "загородный дом"@ru,
        "lantgods"@sv .

gn:S.HSP a gn:Code ;
    skos:definition "a building in which sick or injured, especially those confined to bed, are medically treated"@en,
        "лечебное учреждение, больница"@ru ;
    skos:inScheme gn:S ;
    skos:notation "S.HSP" ;
    skos:prefLabel "болница"@bg,
        "hospital"@en,
        "sykehus"@no,
        "госпиталь"@ru,
        "sjukhus"@sv .

gn:S.HSPC a gn:Code ;
    skos:definition "a medical facility associated with a hospital for outpatients"@en,
        "медицинское учреждение, осуществляющее внебольничное лечебно-профилактическое обслуживание населения"@ru ;
    skos:inScheme gn:S ;
    skos:notation "S.HSPC" ;
    skos:prefLabel "клиника"@bg,
        "clinic"@en,
        "klinikk"@no,
        "поликлиника"@ru,
        "klinik"@sv .

gn:S.HSPD a gn:Code ;
    skos:definition "a building where medical or dental aid is dispensed"@en,
        "медицинское учреждение, занимающееся лечением и предупреждением болезней путём систематического врачебного наблюдения"@ru ;
    skos:inScheme gn:S ;
    skos:notation "S.HSPD" ;
    skos:prefLabel "диспансер"@bg,
        "dispensary"@en,
        "apotek"@no,
        "диспансер"@ru,
        "klinik"@sv .

gn:S.HSPL a gn:Code ;
    skos:definition "an asylum or hospital for lepers"@en,
        "приют для прокаженных"@ru ;
    skos:inScheme gn:S ;
    skos:notation "S.HSPL" ;
    skos:prefLabel "общежитие за прокажени"@bg,
        "leprosarium"@en,
        "leprasykehus"@no,
        "лепрозорий"@ru,
        "leprosarium"@sv .

gn:S.HSTS a gn:Code ;
    skos:definition "a place of historical importance"@en,
        "здания, сооружения, памятные места и предметы, связанные с важнейшими историческими событиями, жизнью исторических деятелей и т.п."@ru ;
    skos:inScheme gn:S ;
    skos:notation "S.HSTS" ;
    skos:prefLabel "историческо място"@bg,
        "historical site"@en,
        "historisk sted"@no,
        "исторический памятник"@ru,
        "historisk plats"@sv .

gn:S.HTL a gn:Code ;
    skos:definition "a building providing lodging and/or meals for the public"@en,
        "то же, что и гостиница; дом для временного проживания туристов"@ru ;
    skos:inScheme gn:S ;
    skos:notation "S.HTL" ;
    skos:prefLabel "хотел"@bg,
        "hotel"@en,
        "hotell"@no,
        "отель"@ru,
        "hotell"@sv .

gn:S.HUT a gn:Code ;
    skos:definition "a small primitive house"@en,
        "небольшой примитивный домик"@ru ;
    skos:inScheme gn:S ;
    skos:notation "S.HUT" ;
    skos:prefLabel "хижа"@bg,
        "hut"@en,
        "hytte"@no,
        "хижина"@ru,
        "hydda"@sv .

gn:S.HUTS a gn:Code ;
    skos:definition "small primitive houses"@en,
        "небольшие примитивные домики"@ru ;
    skos:inScheme gn:S ;
    skos:notation "S.HUTS" ;
    skos:prefLabel "хижи"@bg,
        "huts"@en,
        "hytter"@no,
        "хижины"@ru,
        "hyddor"@sv .

gn:S.INSM a gn:Code ;
    skos:definition "a facility for use of and control by armed forces"@en,
        "территория (важный в стратегическом или политическом отношении пункт, район) и размещенные на ней войска с запасами оружия, боеприпасов, продовольствия и других материальных средств, необходимых для боевой и повседневной деятельности"@ru ;
    skos:inScheme gn:S ;
    skos:notation "S.INSM" ;
    skos:prefLabel "военна инсталация"@bg,
        "military installation"@en,
        "militæranlegg"@no,
        "военная база"@ru,
        "militär installation"@sv .

gn:S.ITTR a gn:Code ;
    skos:definition "a facility where research is carried out"@en,
        "учреждение, занимающееся исследованиями"@ru ;
    skos:inScheme gn:S ;
    skos:notation "S.ITTR" ;
    skos:prefLabel "иследователски институт"@bg,
        "research institute"@en,
        "forskningsinstitutt"@no,
        "научно-исследовательский институт"@ru,
        "forskningsinstitut"@sv .

gn:S.JTY a gn:Code ;
    skos:definition "a structure built out into the water at a river mouth or harbor entrance to regulate currents and silting"@en,
        "гидротехническое сооружение, перегораживающее реку (или др. водоток) для подъёма уровня воды перед ним, сосредоточения напора в месте расположения сооружения и создания водохранилища"@ru ;
    skos:inScheme gn:S ;
    skos:notation "S.JTY" ;
    skos:prefLabel "вълнолом"@bg,
        "jetty"@en,
        "molo"@no,
        "плотина"@ru,
        "pir,brygga"@sv .

gn:S.LDNG a gn:Code ;
    skos:definition "a place where boats receive or discharge passengers and freight, but lacking most port facilities"@en,
        "совокупность сооружений и устройств для стоянки и обслуживания судов, посадки и высадки пассажиров, грузовых операций и т.п."@ru ;
    skos:inScheme gn:S ;
    skos:notation "S.LDNG" ;
    skos:prefLabel "стоварище"@bg,
        "landing"@en,
        "kai"@no,
        "причал"@ru,
        "landstigning"@sv .

gn:S.LEPC a gn:Code ;
    skos:definition "a settled area inhabited by lepers in relative isolation"@en,
        "лечебное учреждение для больных проказой; место проживания и лечения таких больных"@ru ;
    skos:inScheme gn:S ;
    skos:notation "S.LEPC" ;
    skos:prefLabel "колония на прокажени"@bg,
        "leper colony"@en,
        "leprakoloni"@no,
        "приют для прокаженных"@ru,
        "spetälskekoloni"@sv .

gn:S.LIBR a gn:Code ;
    skos:definition "A place in which information resources such as books are kept for reading, reference, or lending."@en,
        "учреждение или отдел какого-л. учреждения, собирающие и хранящие книги, периодику, памятники письменности и т.п. для общественного пользования"@ru ;
    skos:inScheme gn:S ;
    skos:notation "S.LIBR" ;
    skos:prefLabel "library"@bg,
        "library"@en,
        "library"@no,
        "библиотека"@ru,
        "bibliotek"@sv .

gn:S.LNDF a gn:Code ;
    skos:definition "a place for trash and garbage disposal in which the waste is buried between layers of earth to build up low-lying land"@en,
        "место, куда свозят, выбрасывают мусор, нечистоты, негодные вещи"@ru ;
    skos:inScheme gn:S ;
    skos:notation "S.LNDF" ;
    skos:prefLabel "landfill"@bg,
        "landfill"@en,
        "landfill"@no,
        "свалка"@ru,
        "landfill"@sv .

gn:S.LOCK a gn:Code ;
    skos:definition "a basin in a waterway with gates at each end by means of which vessels are passed from one water level to another"@en,
        "гидротехническое сооружение между водоёмами с различными уровнями воды, позволяющее переводить суда из одного водоёма в другой"@ru ;
    skos:inScheme gn:S ;
    skos:notation "S.LOCK" ;
    skos:prefLabel "шлюз(ове)"@bg,
        "lock(s)"@en,
        "sluse"@no,
        "шлюз"@ru,
        "sluss(ar)"@sv .

gn:S.LTHSE a gn:Code ;
    skos:definition "a distinctive structure exhibiting a major navigation light"@en,
        "сооружение башенного типа, служащее ориентиром для опознавания берегов, определения места судна и предупреждения о навигационной опасности"@ru ;
    skos:inScheme gn:S ;
    skos:notation "S.LTHSE" ;
    skos:prefLabel "фар"@bg,
        "lighthouse"@en,
        "fyrtårn"@no,
        "световой маяк"@ru,
        "fyr"@sv .

gn:S.MALL a gn:Code ;
    skos:definition "A large, often enclosed shopping complex containing various stores, businesses, and restaurants usually accessible by common passageways."@en,
        "группа разнородных торговых предприятий, сосредоточенных в одном месте, функционирующих и управляемых как единый, целостный объект"@ru ;
    skos:inScheme gn:S ;
    skos:notation "S.MALL" ;
    skos:prefLabel "мол"@bg,
        "mall"@en,
        "kjøpesenter"@no,
        "торговый центр"@ru,
        "köpcentrum"@sv .

gn:S.MAR a gn:Code ;
    skos:definition "a harbor facility for small boats, yachts, etc."@en,
        "специально оборудованное место, сооружение для причаливания и стоянки лодок, яхт и т.д."@ru ;
    skos:inScheme gn:S ;
    skos:notation "S.MAR" ;
    skos:prefLabel "яхтостроителница"@bg,
        "marina"@en,
        "småbåthavn"@no,
        "пристань"@ru,
        "marina"@sv .

gn:S.MFG a gn:Code ;
    skos:definition "one or more buildings where goods are manufactured, processed or fabricated"@en,
        "промышленное или крупное промысловое предприятие, или комплекс предприятий"@ru ;
    skos:inScheme gn:S ;
    skos:notation "S.MFG" ;
    skos:prefLabel "фабрика"@bg,
        "factory"@en,
        "fabrikk"@no,
        "завод"@ru,
        "fabrik"@sv .

gn:S.MFGB a gn:Code ;
    skos:definition "one or more buildings where beer is brewed"@en,
        "предприятие по производству пива"@ru ;
    skos:inScheme gn:S ;
    skos:notation "S.MFGB" ;
    skos:prefLabel "пивоварна"@bg,
        "brewery"@en,
        "bryggeri"@no,
        "пивоварня"@ru,
        "bryggeri"@sv .

gn:S.MFGC a gn:Code ;
    skos:definition "a building where food items are canned"@en,
        "предприятие по производству консерв"@ru ;
    skos:inScheme gn:S ;
    skos:notation "S.MFGC" ;
    skos:prefLabel "консервна фабрика"@bg,
        "cannery"@en,
        "hermetikkfabrikk"@no,
        "консервный завод"@ru,
        "konservfabrik"@sv .

gn:S.MFGCU a gn:Code ;
    skos:definition "a facility for processing copper ore"@en,
        "предприятие по переработке медной руды"@ru ;
    skos:inScheme gn:S ;
    skos:notation "S.MFGCU" ;
    skos:prefLabel "медна фабрика"@bg,
        "copper works"@en,
        "kopperverk"@no,
        "медеплавильный завод"@ru,
        "kopparbruk"@sv .

gn:S.MFGLM a gn:Code ;
    skos:definition "a furnace in which limestone is reduced to lime"@en,
        "печь для обжига извести"@ru ;
    skos:inScheme gn:S ;
    skos:notation "S.MFGLM" ;
    skos:prefLabel "варница"@bg,
        "limekiln"@en,
        "kalkbrenneri"@no,
        "известеобжигательная печь"@ru,
        "kalkugn"@sv .

gn:S.MFGM a gn:Code ;
    skos:definition "a factory where ammunition is made"@en,
        "предприятие по производству оружия"@ru ;
    skos:inScheme gn:S ;
    skos:notation "S.MFGM" ;
    skos:prefLabel "фабрка за амуниции"@bg,
        "munitions plant"@en,
        "ammunisjonsfabrikk"@no,
        "оружейный завод"@ru,
        "ammunitionsfabrik"@sv .

gn:S.MFGPH a gn:Code ;
    skos:definition "a facility for producing fertilizer"@en,
        "предприятие по производству удобрений"@ru ;
    skos:inScheme gn:S ;
    skos:notation "S.MFGPH" ;
    skos:prefLabel "фосфатна фабрика"@bg,
        "phosphate works"@en,
        "fosfatanlegg"@no,
        "фосфатный завод"@ru,
        "fosfatfabrik"@sv .

gn:S.MFGQ a gn:Code ;
    skos:inScheme gn:S ;
    skos:notation "S.MFGQ" ;
    skos:prefLabel "изоставена фабрика"@bg,
        "abandoned factory"@en,
        "nedlagt fabrikk"@no,
        "покинутый завод"@ru,
        "övergiven fabrik"@sv .

gn:S.MFGSG a gn:Code ;
    skos:definition "a facility for converting raw sugar into refined sugar"@en,
        "завод по переработки сахарного тростника в рафинад"@ru ;
    skos:inScheme gn:S ;
    skos:notation "S.MFGSG" ;
    skos:prefLabel "захарна рафинерия"@bg,
        "sugar refinery"@en,
        "sukkerraffineri"@no,
        "рафинадный завод"@ru,
        "sockerbruk, sockerraffinaderi"@sv .

gn:S.MKT a gn:Code ;
    skos:definition "a place where goods are bought and sold at regular intervals"@en,
        "место торговли, на котором встречаются продавцы и покупатели"@ru ;
    skos:inScheme gn:S ;
    skos:notation "S.MKT" ;
    skos:prefLabel "пазар"@bg,
        "market"@en,
        "marked"@no,
        "рынок"@ru,
        "marknad"@sv .

gn:S.ML a gn:Code ;
    skos:definition "a building housing machines for transforming, shaping, finishing, grinding, or extracting products"@en,
        "промышленное предприятие, обрабатывающее сырье машинным способом"@ru ;
    skos:inScheme gn:S ;
    skos:notation "S.ML" ;
    skos:prefLabel "мелница(и)"@bg,
        "mill(s)"@en,
        "mølle"@no,
        "фабрика"@ru,
        "kvarn"@sv .

gn:S.MLM a gn:Code ;
    skos:definition "a facility for improving the metal content of ore by concentration"@en,
        "предприятие, которое занимается отделением друг от друга входящих в состав руды металлов"@ru ;
    skos:inScheme gn:S ;
    skos:notation "S.MLM" ;
    skos:prefLabel "миннообогатително предприятие"@bg,
        "ore treatment plant"@en,
        "malmbehandlingsanlegg"@no,
        "завод по переработке руды"@ru,
        "malmförädling"@sv .

gn:S.MLO a gn:Code ;
    skos:definition "a mill where oil is extracted from olives"@en,
        "предприятие, которое занимается переработкой оливок и получением из них оливкового масла."@ru ;
    skos:inScheme gn:S ;
    skos:notation "S.MLO" ;
    skos:prefLabel "фабрика за зехтин"@bg,
        "olive oil mill"@en,
        "olivenoljemølle"@no,
        "завод по производству оливкового масла"@ru,
        "olivoljebruk"@sv .

gn:S.MLSG a gn:Code ;
    skos:definition "a facility where sugar cane is processed into raw sugar"@en,
        "предприятие, которое занимается переработкой сахарного тростника в нерафинированный сахар"@ru ;
    skos:inScheme gn:S ;
    skos:notation "S.MLSG" ;
    skos:prefLabel "захарна фабрика"@bg,
        "sugar mill"@en,
        "sukkermølle"@no,
        "сахарный завод"@ru,
        "sockerbruk, sockerraffinaderi"@sv .

gn:S.MLSGQ a gn:Code ;
    skos:definition "a sugar mill no longer used as a sugar mill"@en,
        "сахарный завод, прекративший свою работу"@ru ;
    skos:inScheme gn:S ;
    skos:notation "S.MLSGQ" ;
    skos:prefLabel "бивша захарна фабрика"@bg,
        "former sugar mill"@en,
        "tidligere sukkermølle"@no,
        "бывший сахарный завод"@ru,
        "tidigare sockerbruk"@sv .

gn:S.MLSW a gn:Code ;
    skos:definition "a mill where logs or lumber are sawn to specified shapes and sizes"@en,
        "изготовление пиломатериалов (брусьев и досок) из брёвен"@ru ;
    skos:inScheme gn:S ;
    skos:notation "S.MLSW" ;
    skos:prefLabel "дъскорезница"@bg,
        "sawmill"@en,
        "sagbruk"@no,
        "лесопильный завод"@ru,
        "sågverk"@sv .

gn:S.MLWND a gn:Code ;
    skos:definition "a mill or water pump powered by wind"@en,
        "аэродинамический механизм, который выполняет механическую работу за счет энергии ветра, улавливаемой крыльями мельницы. Наиболее известным применением ветряных мельниц является их использование для помола муки"@ru ;
    skos:inScheme gn:S ;
    skos:notation "S.MLWND" ;
    skos:prefLabel "вятърна мелница"@bg,
        "windmill"@en,
        "vindmølle"@no,
        "ветряная мельница"@ru,
        "väderkvarn"@sv .

gn:S.MLWTR a gn:Code ;
    skos:definition "a mill powered by running water"@en,
        "гидротехнические сооружение, использующее гидроэнергию, получаемую с водяного колеса, движение которого выполняет полезную работу посредством зубчатой передачи"@ru ;
    skos:inScheme gn:S ;
    skos:notation "S.MLWTR" ;
    skos:prefLabel "водна мелница"@bg,
        "water mill"@en,
        "kvernhus"@no,
        "водяная мельница"@ru,
        "vattenkvarn"@sv .

gn:S.MN a gn:Code ;
    skos:definition "a site where mineral ores are extracted from the ground by excavating surface pits and subterranean passages"@en,
        "горнопромышленное предприятие, ведущее добычу полезных ископаемых подземным способом; место проведения подземных работ"@ru ;
    skos:inScheme gn:S ;
    skos:notation "S.MN" ;
    skos:prefLabel "мина(и)"@bg,
        "mine(s)"@en,
        "gruve"@no,
        "шахта"@ru,
        "gruva(or)"@sv .

gn:S.MNAU a gn:Code ;
    skos:definition "a mine where gold ore, or alluvial gold is extracted"@en,
        "предприятие, осуществляющее добычу золота или золотой руды"@ru ;
    skos:inScheme gn:S ;
    skos:notation "S.MNAU" ;
    skos:prefLabel "златна мина(и)"@bg,
        "gold mine(s)"@en,
        "gullgruve"@no,
        "золотопромышленный рудник"@ru,
        "guldgruva(or)"@sv .

gn:S.MNC a gn:Code ;
    skos:definition "a mine where coal is extracted"@en,
        "горнопромышленное предприятие, ведущее добычу угля подземным способом"@ru ;
    skos:inScheme gn:S ;
    skos:notation "S.MNC" ;
    skos:prefLabel "въглищна мина(и)"@bg,
        "coal mine(s)"@en,
        "kullgruve"@no,
        "угольная шахта"@ru,
        "kolgruva(or)"@sv .

gn:S.MNCR a gn:Code ;
    skos:definition "a mine where chrome ore is extracted"@en,
        "горнопромышленное предприятие, ведущее добычу хрома подземным способом"@ru ;
    skos:inScheme gn:S ;
    skos:notation "S.MNCR" ;
    skos:prefLabel "хромна мина(и)"@bg,
        "chrome mine(s)"@en,
        "kromgruve"@no,
        "шахта по добыче хрома"@ru,
        "kromgruva(or)"@sv .

gn:S.MNCU a gn:Code ;
    skos:definition "a mine where copper ore is extracted"@en,
        "горнопромышленное предприятие, осуществляющее добычу меди"@ru ;
    skos:inScheme gn:S ;
    skos:notation "S.MNCU" ;
    skos:prefLabel "медна мина(и)"@bg,
        "copper mine(s)"@en,
        "koppergruve"@no,
        "медный рудник"@ru,
        "koppargruva(or)"@sv .

gn:S.MNDT a gn:Code ;
    owl:deprecated true ;
    skos:definition "a place where diatomaceous earth is extracted"@en ;
    skos:inScheme gn:S ;
    skos:notation "S.MNDT" ;
    skos:prefLabel "diatomite mine(s)"@en .

gn:S.MNFE a gn:Code ;
    skos:definition "a mine where iron ore is extracted"@en,
        "горнопромышленное предприятие, осуществляющее добычу железа"@ru ;
    skos:inScheme gn:S ;
    skos:notation "S.MNFE" ;
    skos:prefLabel "желязна мина(и)"@bg,
        "iron mine(s)"@en,
        "jerngruve"@no,
        "железный рудник"@ru,
        "järngruva(or)"@sv .

gn:S.MNMT a gn:Code ;
    skos:definition "a commemorative structure or statue"@en,
        "архитектурное или скульптурное сооружение в память какого-л. лица, события"@ru ;
    skos:inScheme gn:S ;
    skos:notation "S.MNMT" ;
    skos:prefLabel "монумент"@bg,
        "monument"@en,
        "monument"@no,
        "памятник"@ru,
        "monument"@sv .

gn:S.MNN a gn:Code ;
    skos:definition "a mine from which salt is extracted"@en,
        "горнопромышленное предприятие, осуществляющее добычу солей"@ru ;
    skos:inScheme gn:S ;
    skos:notation "S.MNN" ;
    skos:prefLabel "солна мина(и)"@bg,
        "salt mine(s)"@en,
        "saltgruve"@no,
        "соляная шахта"@ru,
        "saltgruva(or)"@sv .

gn:S.MNNI a gn:Code ;
    owl:deprecated true ;
    skos:definition "a mine where nickel ore is extracted"@en ;
    skos:inScheme gn:S ;
    skos:notation "S.MNNI" ;
    skos:prefLabel "nickel mine(s)"@en .

gn:S.MNPB a gn:Code ;
    owl:deprecated true ;
    skos:definition "a mine where lead ore is extracted"@en ;
    skos:inScheme gn:S ;
    skos:notation "S.MNPB" ;
    skos:prefLabel "lead mine(s)"@en .

gn:S.MNPL a gn:Code ;
    owl:deprecated true ;
    skos:definition "a place where heavy metals are concentrated and running water is used to extract them from unconsolidated sediments"@en ;
    skos:inScheme gn:S ;
    skos:notation "S.MNPL" ;
    skos:prefLabel "placer mine(s)"@en .

gn:S.MNQ a gn:Code ;
    skos:inScheme gn:S ;
    skos:notation "S.MNQ" ;
    skos:prefLabel "изоставена мина"@bg,
        "abandoned mine"@en,
        "nedlagt gruve"@no,
        "заброшенная шахта"@ru,
        "övergiven gruva"@sv .

gn:S.MNQR a gn:Code ;
    skos:definition "a surface mine where building stone or gravel and sand, etc. are extracted"@en,
        "место открытой разработки неглубоко залегающих полезных ископаемых (угля, песка, глины и т.п.)"@ru ;
    skos:inScheme gn:S ;
    skos:notation "S.MNQR" ;
    skos:prefLabel "каменоломна(и)"@bg,
        "quarry(-ies)"@en,
        "steinbrudd"@no,
        "карьер"@ru,
        "stenbrott"@sv .

gn:S.MNSN a gn:Code ;
    owl:deprecated true ;
    skos:definition "a mine where tin ore is extracted"@en ;
    skos:inScheme gn:S ;
    skos:notation "S.MNSN" ;
    skos:prefLabel "tin mine(s)"@en .

gn:S.MOLE a gn:Code ;
    skos:definition "a massive structure of masonry or large stones serving as a pier or breakwater"@en,
        "гидротехническое сооружение для защиты места стоянки судов или берега от разрушительного действия волн"@ru ;
    skos:inScheme gn:S ;
    skos:notation "S.MOLE" ;
    skos:prefLabel "дига"@bg,
        "mole"@en,
        "molo"@no,
        "волнолом"@ru,
        "pir, vågbrytare"@sv .

gn:S.MSQE a gn:Code ;
    skos:definition "a building for public Islamic worship"@en,
        "у мусульман: молитвенный дом"@ru ;
    skos:inScheme gn:S ;
    skos:notation "S.MSQE" ;
    skos:prefLabel "джамия"@bg,
        "mosque"@en,
        "moské"@no,
        "мечеть"@ru,
        "moské"@sv .

gn:S.MSSN a gn:Code ;
    skos:definition "a place characterized by dwellings, school, church, hospital and other facilities operated by a religious group for the purpose of providing charitable services and to propagate religion"@en,
        "жилые дома, больница, школа, принадлежащие религиозной организации, которая занимается благотворительностью и распространением собственной религии среди инаковерующих"@ru ;
    skos:inScheme gn:S ;
    skos:notation "S.MSSN" ;
    skos:prefLabel "мисия"@bg,
        "mission"@en,
        "misjonsstasjon"@no,
        "резиденция миссионеров"@ru,
        "beskickning"@sv .

gn:S.MSSNQ a gn:Code ;
    skos:inScheme gn:S ;
    skos:notation "S.MSSNQ" ;
    skos:prefLabel "изоставена мисия"@bg,
        "abandoned mission"@en,
        "nedlagt misjonsstasjon"@no,
        "заброшенная резиденция миссионеров"@ru,
        "övergiven beskickning"@sv .

gn:S.MSTY a gn:Code ;
    skos:definition "a building and grounds where a community of monks lives in seclusion"@en,
        "религиозная община монахов, представляющая собой церковно-хозяйственную организацию, владеющую землями и капиталами"@ru ;
    skos:inScheme gn:S ;
    skos:notation "S.MSTY" ;
    skos:prefLabel "манастир"@bg,
        "monastery"@en,
        "kloster"@no,
        "мужской монастырь"@ru,
        "munkkloster"@sv .

gn:S.MTRO a gn:Code ;
    skos:definition "metro station (Underground, Tube, or Métro)"@en,
        "пункт остановки электропоездов в  метрополитене"@ru ;
    skos:inScheme gn:S ;
    skos:notation "S.MTRO" ;
    skos:prefLabel "metro station"@bg,
        "metro station"@en,
        "metro station"@no,
        "станция метро"@ru,
        "tunnelbanestation"@sv .

gn:S.MUS a gn:Code ;
    skos:definition "a building where objects of permanent interest in one or more of the arts and sciences are preserved and exhibited"@en,
        "учреждение, собирающее, хранящее и выставляющее на обозрение памятники истории, искусства, культуры, науки, техники и других областей, сфер деятельности общества; помещение такого учреждения"@ru ;
    skos:inScheme gn:S ;
    skos:notation "S.MUS" ;
    skos:prefLabel "музей"@bg,
        "museum"@en,
        "museum"@no,
        "музей"@ru,
        "museum"@sv .

gn:S.NOV a gn:Code ;
    skos:definition "a religious house or school where novices are trained"@en,
        "религиозный дом, где учатся послушники, готовящиеся стать монахами"@ru ;
    skos:inScheme gn:S ;
    skos:notation "S.NOV" ;
    skos:prefLabel "семинария"@bg,
        "novitiate"@en,
        "novisiat"@no,
        "дом послушничества"@ru,
        "novitiat"@sv .

gn:S.NSY a gn:Code ;
    skos:definition "a place where plants are propagated for transplanting or grafting"@en,
        "тёплое с покрытием из прозрачного материала помещение для выращивания ранних овощей, цветов, теплолюбивых растений; оранжерея"@ru ;
    skos:inScheme gn:S ;
    skos:notation "S.NSY" ;
    skos:prefLabel "парник(-ци)"@bg,
        "nursery(-ies)"@en,
        "barnehage"@no,
        "теплица"@ru,
        "plantskola"@sv .

gn:S.OBPT a gn:Code ;
    skos:definition "a wildlife or scenic observation point"@en,
        "специально оборудованное место, с которого ведётся наблюдение за действиями противника и своих войск"@ru ;
    skos:inScheme gn:S ;
    skos:notation "S.OBPT" ;
    skos:prefLabel "наблюдателна точка"@bg,
        "observation point"@en,
        "observasjonssted"@no,
        "наблюдательный пункт"@ru,
        "observationspunkt"@sv .

gn:S.OBS a gn:Code ;
    skos:definition "a facility equipped for observation of atmospheric or space phenomena"@en,
        "научное учреждение, ведущее астрономические и геофизические наблюдения и исследования; здание, специально оборудованное для таких наблюдений"@ru ;
    skos:inScheme gn:S ;
    skos:notation "S.OBS" ;
    skos:prefLabel "обсерватория"@bg,
        "observatory"@en,
        "observatorium"@no,
        "обсерватория"@ru,
        "observatorium"@sv .

gn:S.OBSR a gn:Code ;
    skos:definition "a facility equipped with an array of antennae for receiving radio waves from space"@en,
        "учреждение, оборудованное антеннами для приема радиоволн из Космоса"@ru ;
    skos:inScheme gn:S ;
    skos:notation "S.OBSR" ;
    skos:prefLabel "радио обсерватория"@bg,
        "radio observatory"@en,
        "radioobservatorium"@no,
        "радиообсерватория"@ru,
        "radioobservatorium"@sv .

gn:S.OILJ a gn:Code ;
    skos:definition "a section of an oil pipeline where two or more pipes join together"@en,
        "участок нефтепровода, на котором происходит соединение двух или более трубопроводов"@ru ;
    skos:inScheme gn:S ;
    skos:notation "S.OILJ" ;
    skos:prefLabel "връзка на нефтопровод"@bg,
        "oil pipeline junction"@en,
        "oljeledningsknutepunkt"@no,
        "место соединение нескольких нефтепроводов"@ru,
        "knutpunkt för oljepipeline"@sv .

gn:S.OILQ a gn:Code ;
    skos:inScheme gn:S ;
    skos:notation "S.OILQ" ;
    skos:prefLabel "изоставен петролен кладенец"@bg,
        "abandoned oil well"@en,
        "forlatt oljebrønn"@no,
        "заброшенная нефтяная скважина"@ru,
        "övergiven oljekälla"@sv .

gn:S.OILR a gn:Code ;
    skos:definition "a facility for converting crude oil into refined petroleum products"@en,
        "предприятие, которое занимается переработкой нефти в бензин, авиационный керосин, мазут, дизельное топливо, смазочные масла, смазки, битумы, нефтяной кокс сырьё для нефтехимии"@ru ;
    skos:inScheme gn:S ;
    skos:notation "S.OILR" ;
    skos:prefLabel "петролна рафинерия"@bg,
        "oil refinery"@en,
        "oljeraffineri"@no,
        "нефтеперерабатывающий завод"@ru,
        "oljeraffinaderi"@sv .

gn:S.OILT a gn:Code ;
    skos:definition "a tract of land occupied by large, cylindrical, metal tanks in which oil or liquid petrochemicals are stored"@en,
        "промышленный объект для хранения нефти или нефтепродуктов"@ru ;
    skos:inScheme gn:S ;
    skos:notation "S.OILT" ;
    skos:prefLabel "петролна база"@bg,
        "tank farm"@en,
        "petrokjemisk anlegg"@no,
        "нефтехранилище"@ru,
        "depå"@sv .

gn:S.OILW a gn:Code ;
    skos:definition "a well from which oil may be pumped"@en,
        "вертикальная горная выработка круглого сечения, предназначенная для разведки либо добычи нефти и попутного газа"@ru ;
    skos:inScheme gn:S ;
    skos:notation "S.OILW" ;
    skos:prefLabel "петролен кладенец"@bg,
        "oil well"@en,
        "oljebrønn"@no,
        "нефтяная скважина"@ru,
        "oljekälla"@sv .

gn:S.OPRA a gn:Code ;
    skos:definition "A theater designed chiefly for the performance of operas."@en,
        "театр; оперная труппа театра"@ru ;
    skos:inScheme gn:S ;
    skos:notation "S.OPRA" ;
    skos:prefLabel "опера"@bg,
        "opera house"@en,
        "operahus"@no,
        "оперный дом"@ru,
        "operahus"@sv .

gn:S.PAL a gn:Code ;
    skos:definition "a large stately house, often a royal or presidential residence"@en,
        "здание, являющееся жилищем, постоянным местопребыванием царствующей особы, главы государства, а также членов царствующей семьи"@ru ;
    skos:inScheme gn:S ;
    skos:notation "S.PAL" ;
    skos:prefLabel "дворец"@bg,
        "palace"@en,
        "palass"@no,
        "дворец"@ru,
        "palats"@sv .

gn:S.PGDA a gn:Code ;
    skos:definition "a tower-like storied structure, usually a Buddhist shrine"@en,
        "в Китае, Японии и некоторых других странах: культовое мемориальное буддийское сооружение"@ru ;
    skos:inScheme gn:S ;
    skos:notation "S.PGDA" ;
    skos:prefLabel "пагода"@bg,
        "pagoda"@en,
        "pagode"@no,
        "пагода"@ru,
        "pagod"@sv .

gn:S.PIER a gn:Code ;
    skos:definition "a structure built out into navigable water on piles providing berthing for ships and recreation"@en,
        "двусторонний причал, выдающийся в акваторию порта и предназначенный для швартовки судов с двух сторон"@ru ;
    skos:inScheme gn:S ;
    skos:notation "S.PIER" ;
    skos:prefLabel "пристан"@bg,
        "pier"@en,
        "pir"@no,
        "пирс"@ru,
        "pir, kaj, vågbrytare"@sv .

gn:S.PKLT a gn:Code ;
    skos:definition "an area used for parking vehicles"@en,
        "место для парковки автотранспорта"@ru ;
    skos:inScheme gn:S ;
    skos:notation "S.PKLT" ;
    skos:prefLabel "място за паркиране"@bg,
        "parking lot"@en,
        "parkeringsplass"@no,
        "автостоянка"@ru,
        "parkerginsplats"@sv .

gn:S.PMPO a gn:Code ;
    skos:definition "a facility for pumping oil through a pipeline"@en,
        "станция, предназначенная для перекачки нефти через трубопроводы"@ru ;
    skos:inScheme gn:S ;
    skos:notation "S.PMPO" ;
    skos:prefLabel "нефтена помпена станция"@bg,
        "oil pumping station"@en,
        "oljepumpestasjon"@no,
        "нефтеперекачивающая станция"@ru,
        "pumpstation för olja"@sv .

gn:S.PMPW a gn:Code ;
    skos:definition "a facility for pumping water from a major well or through a pipeline"@en,
        "специальное здание для насосов, перекачивающих воду из водоёма к местам её использования"@ru ;
    skos:inScheme gn:S ;
    skos:notation "S.PMPW" ;
    skos:prefLabel "водна помпена станция"@bg,
        "water pumping station"@en,
        "vannpumpestasjon"@no,
        "водокачка"@ru,
        "pumpstation för vatten"@sv .

gn:S.PO a gn:Code ;
    skos:definition "a public building in which mail is received, sorted and distributed"@en,
        "учреждение связи, ведающее пересылкой писем, периодических изданий, посылок, денег и т.п.; здание, помещение, где находится это учреждение"@ru ;
    skos:inScheme gn:S ;
    skos:notation "S.PO" ;
    skos:prefLabel "пощенска станция"@bg,
        "post office"@en,
        "postkontor"@no,
        "почта"@ru,
        "postkontor"@sv .

gn:S.PP a gn:Code ;
    skos:definition "a building in which police are stationed"@en,
        "здание, в котором располагается пост милиции"@ru ;
    skos:inScheme gn:S ;
    skos:notation "S.PP" ;
    skos:prefLabel "полицейски пост"@bg,
        "police post"@en,
        "politiforlegning"@no,
        "милицейский пост"@ru,
        "polispostering"@sv .

gn:S.PPQ a gn:Code ;
    skos:inScheme gn:S ;
    skos:notation "S.PPQ" ;
    skos:prefLabel "изоставен полицейски пост"@bg,
        "abandoned police post"@en,
        "nedlagt politiforlegning"@no,
        "заброшенный полицейский пост"@ru,
        "övergiven polispostering"@sv .

gn:S.PRKGT a gn:Code ;
    skos:definition "a controlled access to a park"@en,
        "вход в парк, запираемый створами"@ru ;
    skos:inScheme gn:S ;
    skos:notation "S.PRKGT" ;
    skos:prefLabel "паркова бариера"@bg,
        "park gate"@en,
        "inngang til militæranlegg"@no,
        "ворота парка"@ru,
        "parkingång"@sv .

gn:S.PRKHQ a gn:Code ;
    skos:definition "a park administrative facility"@en,
        "здание, в котором располагается администрация парка"@ru ;
    skos:inScheme gn:S ;
    skos:notation "S.PRKHQ" ;
    skos:prefLabel "администрация на парк"@bg,
        "park headquarters"@en,
        "hovedkvarter på militæranlegg"@no,
        "администрация парка"@ru,
        "park huvudkontor"@sv .

gn:S.PRN a gn:Code ;
    skos:definition "a facility for confining prisoners"@en,
        "место заключения, здание, где содержатся лица, приговорённые судом к лишению свободы; лица, находящиеся под следствием"@ru ;
    skos:inScheme gn:S ;
    skos:notation "S.PRN" ;
    skos:prefLabel "зътвор"@bg,
        "prison"@en,
        "fengsel"@no,
        "тюрьма"@ru,
        "fängelse"@sv .

gn:S.PRNJ a gn:Code ;
    skos:definition "a facility for confining, training, and reforming young law offenders"@en,
        "исправительно-трудовое учреждение, в котором отбывают наказание лица до 18 лет, осуждённые к лишению свободы"@ru ;
    skos:inScheme gn:S ;
    skos:notation "S.PRNJ" ;
    skos:prefLabel "исправително училище"@bg,
        "reformatory"@en,
        "forbedringsanstalt"@no,
        "колония для несовершеннолетних"@ru,
        "uppfostringsanstalt"@sv .

gn:S.PRNQ a gn:Code ;
    skos:inScheme gn:S ;
    skos:notation "S.PRNQ" ;
    skos:prefLabel "изоставен затвор"@bg,
        "abandoned prison"@en,
        "nedlagt fengsel"@no,
        "заброшенная тюрьма"@ru,
        "övergivet fängelse"@sv .

gn:S.PS a gn:Code ;
    skos:definition "a facility for generating electric power"@en,
        "предприятие, где производится электроэнергия из других видов энергии"@ru ;
    skos:inScheme gn:S ;
    skos:notation "S.PS" ;
    skos:prefLabel "влектростанция"@bg,
        "power station"@en,
        "kraftstasjon"@no,
        "электростанция"@ru,
        "kraftstation"@sv .

gn:S.PSH a gn:Code ;
    skos:definition "a building where electricity is generated from water power"@en,
        "электростанция, преобразующая энергию падающей воды в электроэнергию (сокращённо ГЭС)"@ru ;
    skos:inScheme gn:S ;
    skos:notation "S.PSH" ;
    skos:prefLabel "ВЕЦ"@bg,
        "hydroelectric power station"@en,
        "vannkraftverk"@no,
        "гидроэлектростанция"@ru,
        "vattenkraftstation"@sv .

gn:S.PSTB a gn:Code ;
    skos:definition "a post or station at an international boundary for the regulation of movement of people and goods"@en,
        "пост, ведающий контролем  передвижения через международную границу людей и товаров"@ru ;
    skos:inScheme gn:S ;
    skos:notation "S.PSTB" ;
    skos:prefLabel "граничен пост"@bg,
        "border post"@en,
        "grensestasjon"@no,
        "пограничный пост"@ru,
        "gränspostering"@sv .

gn:S.PSTC a gn:Code ;
    skos:definition "a building at an international boundary where customs and duties are paid on goods"@en,
        "пост, ведающий контролем провоза через границу грузов, багажа, почты и собирающее пошлину за такой провоз"@ru ;
    skos:inScheme gn:S ;
    skos:notation "S.PSTC" ;
    skos:prefLabel "митнически пост"@bg,
        "customs post"@en,
        "tollstasjon"@no,
        "таможенный пост"@ru,
        "tullpostering"@sv .

gn:S.PSTP a gn:Code ;
    skos:definition "a post from which patrols are sent out"@en,
        "вид наряда, который используется для несения патрульно-постовой службы"@ru ;
    skos:inScheme gn:S ;
    skos:notation "S.PSTP" ;
    skos:prefLabel "патрулен пост"@bg,
        "patrol post"@en,
        "patruljepost"@no,
        "патрульный пост"@ru,
        "patrullpostering"@sv .

gn:S.PYR a gn:Code ;
    skos:definition "an ancient massive structure of square ground plan with four triangular faces meeting at a point and used for enclosing tombs"@en,
        "В Древнем Египте: массивное сооружение из каменных блоков с четырёхугольным основанием и сходящимися к вершине боковыми гранями, служившее гробницей фараона"@ru ;
    skos:inScheme gn:S ;
    skos:notation "S.PYR" ;
    skos:prefLabel "пирамида"@bg,
        "pyramid"@en,
        "pyramide"@no,
        "пирамида"@ru,
        "pyramid"@sv .

gn:S.PYRS a gn:Code ;
    skos:definition "ancient massive structures of square ground plan with four triangular faces meeting at a point and used for enclosing tombs"@en,
        "В Древнем Египте: массивные сооружения из каменных блоков с четырёхугольным основанием и сходящимися к вершине боковыми гранями, служившие гробницей фараона"@ru ;
    skos:inScheme gn:S ;
    skos:notation "S.PYRS" ;
    skos:prefLabel "пирамиди"@bg,
        "pyramids"@en,
        "pyramider"@no,
        "пирамиды"@ru,
        "pyramider"@sv .

gn:S.QUAY a gn:Code ;
    skos:definition "a structure of solid construction along a shore or bank which provides berthing for ships and which generally provides cargo handling facilities"@en,
        "стоянка для судов; специальное сооружение, к которому причаливают суда"@ru ;
    skos:inScheme gn:S ;
    skos:notation "S.QUAY" ;
    skos:prefLabel "кей"@bg,
        "quay"@en,
        "brygge"@no,
        "причал"@ru,
        "kaj"@sv .

gn:S.RDCR a gn:Code ;
    skos:definition "a road junction formed around a central circle about which traffic moves in one direction only"@en ;
    skos:historyNote "Added in v3.0"@en ;
    skos:inScheme gn:S ;
    skos:notation "S.RDCR" ;
    skos:prefLabel "traffic circle"@en .

gn:S.RECG a gn:Code ;
    skos:definition "a recreation field where golf is played"@en,
        "место для отдыха, где находится поле, предназначенное для игры в гольф"@ru ;
    skos:inScheme gn:S ;
    skos:notation "S.RECG" ;
    skos:prefLabel "голф игрище"@bg,
        "golf course"@en,
        "golfbane"@no,
        "поле для гольфа"@ru,
        "golfbana"@sv .

gn:S.RECR a gn:Code ;
    skos:definition "a track where races are held"@en,
        "специально оборудованный участок для конных бегов, скачек и состязаний, представляющий собой площадь овальной формы с амфитеатром для зрителей"@ru ;
    skos:inScheme gn:S ;
    skos:notation "S.RECR" ;
    skos:prefLabel "хиподрум"@bg,
        "racetrack"@en,
        "veddeløpsbane"@no,
        "ипподром"@ru,
        "kapplöpningsbana"@sv .

gn:S.REST a gn:Code ;
    skos:definition "A place where meals are served to the public"@en,
        "торговое заведение, где можно вкусно поесть и приятно провести время (иногда с музыкой, танцами и т.п.)"@ru ;
    skos:inScheme gn:S ;
    skos:notation "S.REST" ;
    skos:prefLabel "ресторант"@bg,
        "restaurant"@en,
        "restaurant"@no,
        "ресторан"@ru,
        "restaurang"@sv .

gn:S.RET a gn:Code ;
    skos:definition "a building where goods and/or services are offered for sale"@en ;
    skos:historyNote "Added in v3.0"@en ;
    skos:inScheme gn:S ;
    skos:notation "S.RET" ;
    skos:prefLabel "store"@en .

gn:S.RHSE a gn:Code ;
    skos:definition "a structure maintained for the rest and shelter of travelers"@en,
        "лечебно-профилактическое учреждение для лечения и отдыха"@ru ;
    skos:inScheme gn:S ;
    skos:notation "S.RHSE" ;
    skos:prefLabel "страноприемница"@bg,
        "resthouse"@en,
        "hvilehjem"@no,
        "дом отдыха"@ru,
        "härbärge, vilohem"@sv .

gn:S.RKRY a gn:Code ;
    skos:definition "a breeding place of a colony of birds or seals"@en,
        "место, где лежат стадами некоторые морские животные"@ru ;
    skos:inScheme gn:S ;
    skos:notation "S.RKRY" ;
    skos:prefLabel "птича колония"@bg,
        "rookery"@en,
        "fuglekoloni"@no,
        "лежбище"@ru,
        "djurkoloni"@sv .

gn:S.RLG a gn:Code ;
    skos:definition "an ancient site of significant religious importance"@en,
        "место религиозного поклонения"@ru ;
    skos:inScheme gn:S ;
    skos:notation "S.RLG" ;
    skos:prefLabel "религиозно място"@bg,
        "religious site"@en,
        "religiøst sted"@no,
        "религиозная святыня"@ru,
        "religiös plats"@sv .

gn:S.RLGR a gn:Code ;
    skos:definition "a place of temporary seclusion, especially for religious groups"@en,
        "жилище, где кто-л. чувствует себя безопасно, уютно и спокойно; пристанище, прибежище для бездомных или одиноких, нуждающихся людей"@ru ;
    skos:inScheme gn:S ;
    skos:notation "S.RLGR" ;
    skos:prefLabel "приют"@bg,
        "retreat"@en,
        "tilfluktssted"@no,
        "приют"@ru,
        "fristad, tillflyktsort"@sv .

gn:S.RNCH a gn:Code ;
    skos:definition "a large farm specializing in extensive grazing of livestock"@en,
        "крупная ферма, основной специализацией которой является разведение крупного рогатого скота"@ru ;
    skos:inScheme gn:S ;
    skos:notation "S.RNCH" ;
    skos:prefLabel "ранчо(а)"@bg,
        "ranch(es)"@en,
        "ranch"@no,
        "ранчо"@ru,
        "ranch(er)"@sv .

gn:S.RSD a gn:Code ;
    skos:definition "a short track parallel to and joining the main track"@en,
        "короткая железная дорога, параллельная и примыкающая к главной железной дороге"@ru ;
    skos:inScheme gn:S ;
    skos:notation "S.RSD" ;
    skos:prefLabel "коловоз"@bg,
        "railroad siding"@en,
        "jernbanesidespor"@no,
        "запасный железнодорожный путь"@ru,
        "järnvägsstickspår"@sv .

gn:S.RSGNL a gn:Code ;
    skos:definition "a signal at the entrance of a particular section of track governing the movement of trains"@en,
        "сигнал для передачи приказов и указаний, обеспечивающих безопасность движения поездов, маневровых работ"@ru ;
    skos:inScheme gn:S ;
    skos:notation "S.RSGNL" ;
    skos:prefLabel "жп сигнализация"@bg,
        "railroad signal"@en,
        "jernbanesignal"@no,
        "железнодорожный сигнал"@ru,
        "järnvägssignal"@sv .

gn:S.RSRT a gn:Code ;
    skos:definition "a specialized facility for vacation, health, or participation sports activities"@en,
        "местность с целебными природными свойствами, используемая для лечебных целей и для отдыха"@ru ;
    skos:inScheme gn:S ;
    skos:notation "S.RSRT" ;
    skos:prefLabel "курорт"@bg,
        "resort"@en,
        "feriested"@no,
        "курорт"@ru,
        "semesterort"@sv .

gn:S.RSTN a gn:Code ;
    skos:definition "a facility comprising ticket office, platforms, etc. for loading and unloading train passengers and freight"@en,
        "здание или комплекс зданий для обслуживания пассажиров и размещения служб на железнодорожных станциях"@ru ;
    skos:inScheme gn:S ;
    skos:notation "S.RSTN" ;
    skos:prefLabel "жп гара"@bg,
        "railroad station"@en,
        "jernbanestasjon"@no,
        "ж/д вокзал"@ru,
        "järnvägsstation"@sv .

gn:S.RSTNQ a gn:Code ;
    skos:inScheme gn:S ;
    skos:notation "S.RSTNQ" ;
    skos:prefLabel "изоставена жп гара"@bg,
        "abandoned railroad station"@en,
        "nedlagt jernbanestasjon"@no,
        "заброшенный вокзал"@ru,
        "övergiven järnvägsstation"@sv .

gn:S.RSTP a gn:Code ;
    skos:definition "a place lacking station facilities where trains stop to pick up and unload passengers and freight"@en,
        "пункт, место, установленные для посадки и высадки пассажиров электропоезда"@ru ;
    skos:inScheme gn:S ;
    skos:notation "S.RSTP" ;
    skos:prefLabel "жп спирка"@bg,
        "railroad stop"@en,
        "jernbanestoppested"@no,
        "остановка поезда"@ru,
        "järnvägsstopp"@sv .

gn:S.RSTPQ a gn:Code ;
    skos:inScheme gn:S ;
    skos:notation "S.RSTPQ" ;
    skos:prefLabel "изоставена жп спирка"@bg,
        "abandoned railroad stop"@en,
        "nedlagt jernbanestoppested"@no,
        "заброшенная остановка"@ru,
        "övergivet järnvägsstopp"@sv .

gn:S.RUIN a gn:Code ;
    skos:definition "a destroyed or decayed structure which is no longer functional"@en,
        "развалины какого-л. строения, сооружения"@ru ;
    skos:inScheme gn:S ;
    skos:notation "S.RUIN" ;
    skos:prefLabel "руина(и)"@bg,
        "ruin(s)"@en,
        "ruin"@no,
        "руины"@ru,
        "ruin(er)"@sv .

gn:S.SCH a gn:Code ;
    skos:definition "building(s) where instruction in one or more branches of knowledge takes place"@en,
        "учебное заведение, которое осуществляет общее образование и воспитание молодого поколения; здание, в котором помещается это заведение"@ru ;
    skos:inScheme gn:S ;
    skos:notation "S.SCH" ;
    skos:prefLabel "училище"@bg,
        "school"@en,
        "skole"@no,
        "школа"@ru,
        "skola"@sv .

gn:S.SCHA a gn:Code ;
    skos:definition "a school with a curriculum focused on agriculture"@en,
        "школа, в учебном плане которой сделан акцент на изучение сельскохозяйственных наук"@ru ;
    skos:inScheme gn:S ;
    skos:notation "S.SCHA" ;
    skos:prefLabel "земеделско училище"@bg,
        "agricultural school"@en,
        "landbruksskole"@no,
        "сельскохозяйственная школа"@ru,
        "jordbruksskola"@sv .

gn:S.SCHC a gn:Code ;
    skos:definition "the grounds and buildings of an institution of higher learning"@en,
        "в Англии, США и некоторых других странах: высшее или среднее учебное заведение"@ru ;
    skos:inScheme gn:S ;
    skos:notation "S.SCHC" ;
    skos:prefLabel "колеж"@bg,
        "college"@en,
        "høyskole"@no,
        "колледж"@ru,
        "universitet"@sv .

gn:S.SCHD a gn:Code ;
    owl:deprecated true ;
    skos:definition "Driving School"@en ;
    skos:inScheme gn:S ;
    skos:notation "S.SCHD" ;
    skos:prefLabel "Driving School"@en .

gn:S.SCHL a gn:Code ;
    skos:definition "Language Schools & Institutions"@en,
        "языковые учебные заведения"@ru ;
    skos:inScheme gn:S ;
    skos:notation "S.SCHL" ;
    skos:prefLabel "language school"@bg,
        "Language School"@en,
        "language school"@en,
        "language school"@no,
        "языковая школа"@ru,
        "Språkskola"@sv .

gn:S.SCHM a gn:Code ;
    skos:definition "a school at which military science forms the core of the curriculum"@en,
        "военное образовательное учреждение высшего и среднего профессионального образования"@ru ;
    skos:inScheme gn:S ;
    skos:notation "S.SCHM" ;
    skos:prefLabel "военен колеж"@bg,
        "military school"@en,
        "militærskole"@no,
        "военное училище"@ru,
        "militärskola"@sv .

gn:S.SCHN a gn:Code ;
    skos:definition "a school at which maritime sciences form the core of the curriculum"@en,
        "военно-учебное заведение для подготовки офицеров военно-морского флота (ВМФ)"@ru ;
    skos:inScheme gn:S ;
    skos:notation "S.SCHN" ;
    skos:prefLabel "морско училище"@bg,
        "maritime school"@en,
        "sjøfartsskole"@no,
        "военно-морское училище"@ru,
        "sjöfartsskola"@sv .

gn:S.SCHT a gn:Code ;
    skos:definition "post-secondary school with a specifically technical or vocational curriculum"@en,
        "школа, предоставляющая профессионально-техническое образование"@ru ;
    skos:inScheme gn:S ;
    skos:notation "S.SCHT" ;
    skos:prefLabel "technical school"@en,
        "техническое училище"@ru .

gn:S.SECP a gn:Code ;
    skos:definition "state exam preparation centres"@en,
        "центры по подготовке к сдаче государственного экзамена"@ru ;
    skos:inScheme gn:S ;
    skos:notation "S.SECP" ;
    skos:prefLabel "State Exam Prep Centre"@bg,
        "State Exam Prep Centre"@en,
        "State Exam Prep Centre"@no,
        "центр подготовки к государственному экзамену"@ru,
        "State Exam Prep Centre"@sv .

gn:S.SHPF a gn:Code ;
    skos:definition "a fence or wall enclosure for sheep and other small herd animals"@en,
        "хлев, загон для овец"@ru ;
    skos:inScheme gn:S ;
    skos:notation "S.SHPF" ;
    skos:prefLabel "кошара за овце"@bg,
        "sheepfold"@en,
        "sauekve"@no,
        "овчарня"@ru,
        "fårfälla"@sv .

gn:S.SHRN a gn:Code ;
    skos:definition "a structure or place memorializing a person or religious concept"@en,
        "в христианской церкви: большой ларец (в виде гробницы или саркофага), в котором хранятся мощи святого"@ru ;
    skos:inScheme gn:S ;
    skos:notation "S.SHRN" ;
    skos:prefLabel "светилище"@bg,
        "shrine"@en,
        "helligdom"@no,
        "рака"@ru,
        "helgedom"@sv .

gn:S.SHSE a gn:Code ;
    skos:definition "a building for storing goods, especially provisions"@en,
        "специальное помещение для хранения товаров, сырья, оборудования и т.п."@ru ;
    skos:inScheme gn:S ;
    skos:notation "S.SHSE" ;
    skos:prefLabel "хамбар"@bg,
        "storehouse"@en,
        "lagerbygning"@no,
        "склад"@ru,
        "magasin"@sv .

gn:S.SLCE a gn:Code ;
    skos:definition "a conduit or passage for carrying off surplus water from a waterbody, usually regulated by means of a sluice gate"@en,
        "гидротехническое сооружение между водоёмами с различными уровнями воды, позволяющее переводить суда из одного водоёма в другой"@ru ;
    skos:inScheme gn:S ;
    skos:notation "S.SLCE" ;
    skos:prefLabel "шлюз"@bg,
        "sluice"@en,
        "sluse"@no,
        "шлюз"@ru,
        "sluss"@sv .

gn:S.SNTR a gn:Code ;
    skos:definition "a facility where victims of physical or mental disorders are treated"@en,
        "лечебно-профилактическое учреждение для лечения и отдыха"@ru ;
    skos:inScheme gn:S ;
    skos:notation "S.SNTR" ;
    skos:prefLabel "санаториум"@bg,
        "sanatorium"@en,
        "sanatorium"@no,
        "санаторий"@ru,
        "sanatorium"@sv .

gn:S.SPA a gn:Code ;
    skos:definition "a resort area usually developed around a medicinal spring"@en,
        "курорт с минеральным источником"@ru ;
    skos:inScheme gn:S ;
    skos:notation "S.SPA" ;
    skos:prefLabel "спа"@bg,
        "spa"@en,
        "spa"@no,
        "спа"@ru,
        "bad"@sv .

gn:S.SPLY a gn:Code ;
    skos:definition "a passage or outlet through which surplus water flows over, around or through a dam"@en,
        "водосброс, осуществляющийся путём свободного перелива воды через гребень плотины"@ru ;
    skos:inScheme gn:S ;
    skos:notation "S.SPLY" ;
    skos:prefLabel "преливник"@bg,
        "spillway"@en,
        "overløp"@no,
        "водослив"@ru,
        "dammavlopp"@sv .

gn:S.SQR a gn:Code ;
    skos:definition "a broad, open, public area near the center of a town or city"@en,
        "незастроенное, обрамлённое какими-л. зданиями, зелёными насаждениями место в пределах города или села, составляющее часть городского, сельского пространства"@ru ;
    skos:inScheme gn:S ;
    skos:notation "S.SQR" ;
    skos:prefLabel "площад"@bg,
        "square"@en,
        "plass"@no,
        "площадь"@ru,
        "torg"@sv .

gn:S.STBL a gn:Code ;
    skos:definition "a building for the shelter and feeding of farm animals, especially horses"@en,
        "помещение для содержания лошадей, обычно представляет собой постройку, разделённую на индивидуальные для каждой лошади секции, которые называются денниками"@ru ;
    skos:inScheme gn:S ;
    skos:notation "S.STBL" ;
    skos:prefLabel "обор"@bg,
        "stable"@en,
        "stall"@no,
        "конюшня"@ru,
        "stall"@sv .

gn:S.STDM a gn:Code ;
    skos:definition "a structure with an enclosure for athletic games with tiers of seats for spectators"@en,
        "комплексное спортивное сооружение со специально оборудованными площадками для состязаний, тренировок, вспомогательными помещениями и трибунами для зрителей"@ru ;
    skos:inScheme gn:S ;
    skos:notation "S.STDM" ;
    skos:prefLabel "стадион"@bg,
        "stadium"@en,
        "stadion"@no,
        "стадион"@ru,
        "stadium"@sv .

gn:S.STNB a gn:Code ;
    skos:definition "a scientific facility used as a base from which research is carried out or monitored"@en,
        "помещение, которое используется в качестве базы для проведения различных научных исследований"@ru ;
    skos:inScheme gn:S ;
    skos:notation "S.STNB" ;
    skos:prefLabel "научно иследователска база"@bg,
        "scientific research base"@en,
        "forskningsbase"@no,
        "научно-исследовательская база"@ru,
        "forskningsstation"@sv .

gn:S.STNC a gn:Code ;
    skos:definition "a facility from which the coast is guarded by armed vessels"@en,
        "пункт, с которого вооруженные корабли ведут охрану береговой линии"@ru ;
    skos:inScheme gn:S ;
    skos:notation "S.STNC" ;
    skos:prefLabel "станция на брегова охрана"@bg,
        "coast guard station"@en,
        "kystvaktstasjon"@no,
        "пост береговой охраны"@ru,
        "kustvaktsstation"@sv .

gn:S.STNE a gn:Code ;
    skos:definition "a facility for carrying out experiments"@en,
        "место проведения различного рода испытаний"@ru ;
    skos:inScheme gn:S ;
    skos:notation "S.STNE" ;
    skos:prefLabel "експериментална станция"@bg,
        "experiment station"@en,
        "eksperimentstasjon"@no,
        "испытательная станция"@ru,
        "experimentstation"@sv .

gn:S.STNF a gn:Code ;
    skos:definition "a collection of buildings and facilities for carrying out forest management"@en,
        "хозяйственные строения, в которых располагается управление лесным участком"@ru ;
    skos:inScheme gn:S ;
    skos:notation "S.STNF" ;
    skos:prefLabel "горска станция"@bg,
        "forest station"@en,
        "skogstasjon"@no,
        "лесничество"@ru,
        "skogsstation"@sv .

gn:S.STNI a gn:Code ;
    skos:definition "a station at which vehicles, goods, and people are inspected"@en,
        "место досмотра вещей и обыска людей"@ru ;
    skos:inScheme gn:S ;
    skos:notation "S.STNI" ;
    skos:prefLabel "инспекционна станция"@bg,
        "inspection station"@en,
        "inspeksjonsstasjon"@no,
        "контрольно-пропускной пункт"@ru,
        "inspektionsstation"@sv .

gn:S.STNM a gn:Code ;
    skos:definition "a station at which weather elements are recorded"@en,
        "учреждение, которое проводит регулярные наблюдения за состоянием атмосферы"@ru ;
    skos:inScheme gn:S ;
    skos:notation "S.STNM" ;
    skos:prefLabel "метереологична станция"@bg,
        "meteorological station"@en,
        "meteorologisk stasjon"@no,
        "метеорологическая станция"@ru,
        "meteorologisk station"@sv .

gn:S.STNR a gn:Code ;
    skos:definition "a facility for producing and transmitting information by radio waves"@en,
        "комплекс устройств для передачи информации посредством радиоволн и (или) её приёма"@ru ;
    skos:inScheme gn:S ;
    skos:notation "S.STNR" ;
    skos:prefLabel "радио станция"@bg,
        "radio station"@en,
        "radiostasjon"@no,
        "радиостанция"@ru,
        "radiostation"@sv .

gn:S.STNS a gn:Code ;
    skos:definition "a facility for tracking and communicating with orbiting satellites"@en,
        "космический аппарат, предназначенный для долговременного пребывания людей на околоземной орбите с целью проведения научных исследований в условиях космического пространства, разведки, наблюдений за поверхностью и атмосферой планеты, астрономических наблюдений, и т.п."@ru ;
    skos:inScheme gn:S ;
    skos:notation "S.STNS" ;
    skos:prefLabel "сателитна станция"@bg,
        "satellite station"@en,
        "satellittstasjon"@no,
        "орбитальная станция"@ru,
        "satellitstation"@sv .

gn:S.STNW a gn:Code ;
    skos:definition "a facility for butchering whales and processing train oil"@en,
        "место забоя китов"@ru ;
    skos:inScheme gn:S ;
    skos:notation "S.STNW" ;
    skos:prefLabel "китоловна станция"@bg,
        "whaling station"@en,
        "hvalfangststasjon"@no,
        "китобойная станция"@ru,
        "valstation"@sv .

gn:S.STPS a gn:Code ;
    skos:definition "stones or slabs placed for ease in ascending or descending a steep slope"@en,
        "пристройка перед входом в дом, состоящая из площадки и лестницы, иногда под навесом"@ru ;
    skos:inScheme gn:S ;
    skos:notation "S.STPS" ;
    skos:prefLabel "стъпало"@bg,
        "steps"@en,
        "trinn"@no,
        "крыльцо"@ru,
        "trappa"@sv .

gn:S.SWT a gn:Code ;
    skos:definition "facility for the processing of sewage and/or wastewater"@en,
        "комплекс инженерных сооружений в системе канализации населённого места или промышленного предприятия, предназначенный для очистки"@ru ;
    skos:inScheme gn:S ;
    skos:notation "S.SWT" ;
    skos:prefLabel "sewage treatment plant"@en,
        "очистное сооружение"@ru .

gn:S.THTR a gn:Code ;
    skos:definition "A building, room, or outdoor structure for the presentation of plays, films, or other dramatic performances"@en,
        "учреждение, организация, занимающиеся устройством представлений"@ru ;
    skos:inScheme gn:S ;
    skos:notation "S.THTR" ;
    skos:prefLabel "театър"@bg,
        "theater"@en,
        "teater"@no,
        "театр"@ru,
        "teater"@sv .

gn:S.TMB a gn:Code ;
    skos:definition "a structure for interring bodies"@en,
        "яма для погребения умершего"@ru ;
    skos:inScheme gn:S ;
    skos:notation "S.TMB" ;
    skos:prefLabel "гробница(и)"@bg,
        "tomb(s)"@en,
        "grav"@no,
        "могила"@ru,
        "grav(ar)"@sv .

gn:S.TMPL a gn:Code ;
    skos:definition "an edifice dedicated to religious worship"@en,
        "здание, предназначенное для совершения богослужений и религиозных обрядов"@ru ;
    skos:inScheme gn:S ;
    skos:notation "S.TMPL" ;
    skos:prefLabel "храм(ове)"@bg,
        "temple(s)"@en,
        "tempel"@no,
        "храм"@ru,
        "tempel"@sv .

gn:S.TNKD a gn:Code ;
    skos:definition "a small artificial pond used for immersing cattle in chemically treated water for disease control"@en,
        "искусственный водоем со специальным химическим раствором; в этот водоем опускают крупный рогатый скот для профилактики от опасных заболеваний"@ru ;
    skos:inScheme gn:S ;
    skos:notation "S.TNKD" ;
    skos:prefLabel "яма за третиране на животни"@bg,
        "cattle dipping tank"@en,
        "desinfeksjonsstasjon for kveg"@no,
        "макательная ванна для крупного рогатого скота"@ru,
        "cattle dipping tank"@sv .

gn:S.TOWR a gn:Code ;
    skos:definition "a high conspicuous structure, typically much higher than its diameter"@en,
        "высокое узкое архитектурное или инженерное сооружение (круглой, четырёхгранной или многогранной формы) различного назначения"@ru ;
    skos:inScheme gn:S ;
    skos:notation "S.TOWR" ;
    skos:prefLabel "кула"@bg,
        "tower"@en,
        "tårn"@no,
        "башня"@ru,
        "torn"@sv .

gn:S.TRANT a gn:Code ;
    skos:definition "facilities for the handling of vehicular freight and passengers"@en,
        "станция для перегрузки материалов с одного вида транспорта на другой и для пересадки пассажиров"@ru ;
    skos:inScheme gn:S ;
    skos:notation "S.TRANT" ;
    skos:prefLabel "transit terminal"@en,
        "перевалочная база/станция пересадки"@ru .

gn:S.TRIG a gn:Code ;
    skos:definition "a point on the earth whose position has been determined by triangulation"@en,
        "опорный геодезический пункт, созданный методом триангуляции (геодезия)"@ru ;
    skos:inScheme gn:S ;
    skos:notation "S.TRIG" ;
    skos:prefLabel "триангулачна точка"@bg,
        "triangulation station"@en,
        "trianguleringsstasjon"@no,
        "триангуляционный пост"@ru,
        "trianguleringsstation"@sv .

gn:S.TRMO a gn:Code ;
    skos:definition "a tank farm or loading facility at the end of an oil pipeline"@en,
        "нефтебаза или нефтеналивная станция в конце нефтепровода"@ru ;
    skos:inScheme gn:S ;
    skos:notation "S.TRMO" ;
    skos:prefLabel "нефтен терминал"@bg,
        "oil pipeline terminal"@en,
        "terminal for oljerørledning"@no,
        "конечный пункт нефтепровода"@ru,
        "oljepipelineterminal"@sv .

gn:S.TWO a gn:Code ;
    skos:definition "Temporary Work Offices"@en,
        "учреждение, осуществляющее посредничество между предпринимателями и наёмными работниками"@ru ;
    skos:inScheme gn:S ;
    skos:notation "S.TWO" ;
    skos:prefLabel "temp work office"@bg,
        "temp work office"@en,
        "temp work office"@no,
        "биржа труда"@ru,
        "Temp Work Office"@sv .

gn:S.UNIO a gn:Code ;
    owl:deprecated true ;
    skos:definition "Post Universitary Education Institutes (post graduate studies and highly specialised master programs) & MBA"@en ;
    skos:inScheme gn:S ;
    skos:notation "S.UNIO" ;
    skos:prefLabel "postgrad & MBA"@en .

gn:S.UNIP a gn:Code ;
    skos:definition "University Preparation Schools & Institutions"@en,
        "подготовительные курсы для поступления в высшее учебное заведение"@ru ;
    skos:inScheme gn:S ;
    skos:notation "S.UNIP" ;
    skos:prefLabel "university prep school"@bg,
        "university prep school"@en,
        "university prep school"@no,
        "подготовительные курсы"@ru,
        "University Prep School"@sv .

gn:S.UNIV a gn:Code ;
    skos:definition "An institution for higher learning with teaching and research facilities constituting a graduate school and professional schools that award master's degrees and doctorates and an undergraduate division that awards bachelor's degrees."@en,
        "высшее учебно-научное заведение с различными гуманитарными и естественно-математическими отделениями (факультетами)"@ru ;
    skos:inScheme gn:S ;
    skos:notation "S.UNIV" ;
    skos:prefLabel "университет"@bg,
        "university"@en,
        "universitet"@no,
        "университет"@ru,
        "universitet"@sv .

gn:S.USGE a gn:Code ;
    skos:definition "a facility operated by the United States Government in Panama"@en,
        "учреждение, которое находится под контролем правительства США в Панаме"@ru ;
    skos:inScheme gn:S ;
    skos:notation "S.USGE" ;
    skos:prefLabel "представителство на САЩ"@bg,
        "united states government establishment"@en,
        "anlegg tilhørende USA"@no,
        "представительство США в Панаме"@ru,
        "amerikansk regeringsbyggnad"@sv .

gn:S.VETF a gn:Code ;
    skos:definition "a building or camp at which veterinary services are available"@en,
        "больница, где лечат животных"@ru ;
    skos:inScheme gn:S ;
    skos:notation "S.VETF" ;
    skos:prefLabel "ветеринарна лечебница"@bg,
        "veterinary facility"@en,
        "veterinæranlegg"@no,
        "ветеринарная клиника"@ru,
        "veterinärklinik"@sv .

gn:S.WALL a gn:Code ;
    skos:definition "a thick masonry structure, usually enclosing a field or building, or forming the side of a structure"@en,
        "вертикальная часть здания, служащая для поддержания перекрытий и разделения помещения на части"@ru ;
    skos:inScheme gn:S ;
    skos:notation "S.WALL" ;
    skos:prefLabel "вал"@bg,
        "wall"@en,
        "mur"@no,
        "стена"@ru,
        "mur"@sv .

gn:S.WALLA a gn:Code ;
    skos:definition "the remains of a linear defensive stone structure"@en,
        "руины защитного сооружения, построенного из камня"@ru ;
    skos:inScheme gn:S ;
    skos:notation "S.WALLA" ;
    skos:prefLabel "античен вал"@bg,
        "ancient wall"@en,
        "fortidsmur"@no,
        "античная стена"@ru,
        "historisk damm"@sv .

gn:S.WEIR a gn:Code ;
    skos:definition "a small dam in a stream, designed to raise the water level or to divert stream flow through a desired channel"@en,
        "гидротехническое сооружение, перегораживающее водоток для подъёма воды в реке, создания водохранилища или электростанции"@ru ;
    skos:inScheme gn:S ;
    skos:notation "S.WEIR" ;
    skos:prefLabel "бент(ове)"@bg,
        "weir(s)"@en,
        "fiskedam"@no,
        "плотина"@ru,
        "damm, fördämning"@sv .

gn:S.WHRF a gn:Code ;
    skos:definition "a structure of open rather than solid construction along a shore or a bank which provides berthing for ships and cargo-handling facilities"@en,
        "специально оборудованное место, сооружение для причаливания и стоянки судов"@ru ;
    skos:inScheme gn:S ;
    skos:notation "S.WHRF" ;
    skos:prefLabel "пристан(и)"@bg,
        "wharf(-ves)"@en,
        "kai"@no,
        "пристань"@ru,
        "kaj, brygga"@sv .

gn:S.WRCK a gn:Code ;
    skos:definition "the site of the remains of a wrecked vessel"@en,
        "остатки кораблекрушения, выброшенные морем на берег"@ru ;
    skos:inScheme gn:S ;
    skos:notation "S.WRCK" ;
    skos:prefLabel "гробница за кораби"@bg,
        "wreck"@en,
        "vrak"@no,
        "обломки разбитого судна"@ru,
        "vrak"@sv .

gn:S.WTRW a gn:Code ;
    skos:definition "a facility for supplying potable water through a water source and a system of pumps and filtration beds"@en,
        "система наносов и очистных сооружений, сквозь которые проходит вода, используемая в дальнейшем для питья и технических целей"@ru ;
    skos:inScheme gn:S ;
    skos:notation "S.WTRW" ;
    skos:prefLabel "водопроводна станция"@bg,
        "waterworks"@en,
        "vannverk"@no,
        "водопроводная станция"@ru,
        "vattenverk, vattenkonst"@sv .

gn:S.ZNF a gn:Code ;
    skos:definition "an area, usually a section of a port, where goods may be received and shipped free of customs duty and of most customs regulations"@en,
        "территория, на которой не взимаются таможенные пошлины, налоги и сборы с пересекающих границу иностранных товаров"@ru ;
    skos:inScheme gn:S ;
    skos:notation "S.ZNF" ;
    skos:prefLabel "свободна търговска зона"@bg,
        "free trade zone"@en,
        "frihandelssone"@no,
        "зона свободной торговли"@ru,
        "frihandelszon"@sv .

gn:S.ZOO a gn:Code ;
    skos:definition "a zoological garden or park where wild animals are kept for exhibition"@en,
        "зоологический парк, где содержат диких животных с целью их демонстрации"@ru ;
    skos:inScheme gn:S ;
    skos:notation "S.ZOO" ;
    skos:prefLabel "зоопарк"@bg,
        "zoo"@en,
        "dyrehage"@no,
        "зоопарк"@ru,
        "zoo"@sv .

gn:T.ASPH a gn:Code ;
    skos:definition "a small basin containing naturally occurring asphalt"@en,
        "небольшой бассейн, который вместо воды заполнен природным асфальтом"@ru ;
    skos:inScheme gn:T ;
    skos:notation "T.ASPH" ;
    skos:prefLabel "асфалтово езеро"@bg,
        "asphalt lake"@en,
        "asfaltsjø"@no,
        "асфальтовое озеро"@ru,
        "asfaltssjö"@sv .

gn:T.ATOL a gn:Code ;
    skos:definition "a ring-shaped coral reef which has closely spaced islands on it encircling a lagoon"@en,
        "коралловый остров кольцеобразной формы с мелководной лагуной внутри (преимущественно в Индийском и Тихом океанах)"@ru ;
    skos:inScheme gn:T ;
    skos:notation "T.ATOL" ;
    skos:prefLabel "атол(и)"@bg,
        "atoll(s)"@en,
        "atoll"@no,
        "атолл"@ru,
        "atoll(er)"@sv .

gn:T.BAR a gn:Code ;
    skos:definition "a shallow ridge or mound of coarse unconsolidated material in a stream channel, at the mouth of a stream, estuary, or lagoon and in the wave-break zone along coasts"@en,
        "наносная мель у морских берегов (обычно в устье реки)"@ru ;
    skos:inScheme gn:T ;
    skos:notation "T.BAR" ;
    skos:prefLabel "нанос"@bg,
        "bar"@en,
        "bar"@no,
        "бар"@ru,
        "rev"@sv .

gn:T.BCH a gn:Code ;
    skos:definition "a shore zone of coarse unconsolidated sediment that extends from the low-water line to the highest reach of storm waves"@en,
        "отлогий намывной берег, удобный для купания и принятия солнечных ванн"@ru ;
    skos:inScheme gn:T ;
    skos:notation "T.BCH" ;
    skos:prefLabel "бряг"@bg,
        "beach"@en,
        "strand"@no,
        "пляж"@ru,
        "strand"@sv .

gn:T.BCHS a gn:Code ;
    skos:definition "a shore zone of coarse unconsolidated sediment that extends from the low-water line to the highest reach of storm waves"@en,
        "отлогие намывные берега, удобные для купания и принятия солнечных ванн"@ru ;
    skos:inScheme gn:T ;
    skos:notation "T.BCHS" ;
    skos:prefLabel "брегове"@bg,
        "beaches"@en,
        "strender"@no,
        "пляжи"@ru,
        "stränder"@sv .

gn:T.BDLD a gn:Code ;
    skos:definition "an area characterized by a maze of very closely spaced, deep, narrow, steep-sided ravines, and sharp crests and pinnacles"@en,
        "неплодородная эродированная сильнопересечённая местность"@ru ;
    skos:inScheme gn:T ;
    skos:notation "T.BDLD" ;
    skos:prefLabel "Необитаема зона"@bg,
        "badlands"@en,
        "steinørken"@no,
        "бесплодная земля"@ru,
        "ofruktbart land"@sv .

gn:T.BLDR a gn:Code ;
    skos:definition "a high altitude or high latitude bare, flat area covered with large angular rocks"@en,
        "равнинная местность, покрытая большими углообразными валунами"@ru ;
    skos:inScheme gn:T ;
    skos:notation "T.BLDR" ;
    skos:prefLabel "Скалиста зона"@bg,
        "boulder field"@en,
        "steinmark"@no,
        "завалуненное поле"@ru,
        "stenblocksfält"@sv .

gn:T.BLHL a gn:Code ;
    skos:definition "a hole in coastal rock through which sea water is forced by a rising tide or waves and spurted through an outlet into the air"@en,
        "a hole in coastal rock through which sea water is forced by a rising tide or waves and spurted through an outlet into the air"@ru ;
    skos:inScheme gn:T ;
    skos:notation "T.BLHL" ;
    skos:prefLabel "ноздра(и)"@bg,
        "blowhole(s)"@en,
        "luftehull"@no,
        "blowhole"@ru,
        "blowhole(s)"@sv .

gn:T.BLOW a gn:Code ;
    skos:definition "a small depression in sandy terrain, caused by wind erosion"@en,
        "небольшое углубление на песчаной местности, образовавшееся в результате эрозии"@ru ;
    skos:inScheme gn:T ;
    skos:notation "T.BLOW" ;
    skos:prefLabel "пукнатина(и)"@bg,
        "blowout(s)"@en,
        "utblåsning"@no,
        "развеянная дюна"@ru,
        "utvidgning(ar)"@sv .

gn:T.BNCH a gn:Code ;
    skos:definition "a long, narrow bedrock platform bounded by steeper slopes above and below, usually overlooking a waterbody"@en,
        "выдающаяся вперед часть горного массива (обычно над водой), имеющая вид ступени или террасы"@ru ;
    skos:inScheme gn:T ;
    skos:notation "T.BNCH" ;
    skos:prefLabel "банка"@bg,
        "bench"@en,
        "benk"@no,
        "выступ, имеющий вид ступени или террасы"@ru,
        "avsats"@sv .

gn:T.BUTE a gn:Code ;
    skos:definition "a small, isolated, usually flat-topped hill with steep sides"@en,
        "небольшая  возвышенность округлой или овальной формы с крутым склоном"@ru ;
    skos:inScheme gn:T ;
    skos:notation "T.BUTE" ;
    skos:prefLabel "Изолирана скала(и)"@bg,
        "butte(s)"@en,
        "høyde med bratte sider"@no,
        "крутой холм на равнине"@ru,
        "kulle"@sv .

gn:T.CAPE a gn:Code ;
    skos:definition "a land area, more prominent than a point, projecting into the sea and marking a notable change in coastal direction"@en,
        "часть суши, острым углом вдающаяся в водное пространство (море, озеро, реку)"@ru ;
    skos:inScheme gn:T ;
    skos:notation "T.CAPE" ;
    skos:prefLabel "нос"@bg,
        "cape"@en,
        "nes"@no,
        "мыс"@ru,
        "udde, kap"@sv .

gn:T.CFT a gn:Code ;
    skos:definition "a deep narrow slot, notch, or groove in a coastal cliff"@en,
        "узкое ущелье в горах"@ru ;
    skos:inScheme gn:T ;
    skos:notation "T.CFT" ;
    skos:prefLabel "цепнатина(и)"@bg,
        "cleft(s)"@en,
        "kløft"@no,
        "расщелина"@ru,
        "klyfta"@sv .

gn:T.CLDA a gn:Code ;
    skos:definition "a depression measuring kilometers across formed by the collapse of a volcanic mountain"@en,
        "котлообразная впадина с крутыми склонами и ровным дном, образовавшаяся вследствие провала вершины вулкана, а иногда и прилегающей к нему местности"@ru ;
    skos:inScheme gn:T ;
    skos:notation "T.CLDA" ;
    skos:prefLabel "Вулканично пропадане"@bg,
        "caldera"@en,
        "caldera"@no,
        "кальдера"@ru,
        "krater"@sv .

gn:T.CLF a gn:Code ;
    skos:definition "a high, steep to perpendicular slope overlooking a waterbody or lower area"@en,
        "отвесная скала"@ru ;
    skos:inScheme gn:T ;
    skos:notation "T.CLF" ;
    skos:prefLabel "урва(и)"@bg,
        "cliff(s)"@en,
        "klippe"@no,
        "утес"@ru,
        "brant klippa, stup"@sv .

gn:T.CNYN a gn:Code ;
    skos:definition "a deep, narrow valley with steep sides cutting into a plateau or mountainous area"@en,
        "глубокая речная долина с очень крутыми или отвесными склонами"@ru ;
    skos:inScheme gn:T ;
    skos:notation "T.CNYN" ;
    skos:prefLabel "каньон"@bg,
        "canyon"@en,
        "canyon"@no,
        "каньон"@ru,
        "kanjon, djup flodbädd"@sv .

gn:T.CONE a gn:Code ;
    skos:definition "a conical landform composed of mud or volcanic material"@en,
        "рельеф канонической формы, образованный из вулканогенного материала и покрытый грязью"@ru ;
    skos:inScheme gn:T ;
    skos:notation "T.CONE" ;
    skos:prefLabel "конус(и)"@bg,
        "cone(s)"@en,
        "kjegle"@no,
        "конус вулкана"@ru,
        "kon"@sv .

gn:T.CRDR a gn:Code ;
    skos:definition "a strip or area of land having significance as an access way"@en,
        "узкое длинное пространство, проход, ограниченные с обеих сторон"@ru ;
    skos:inScheme gn:T ;
    skos:notation "T.CRDR" ;
    skos:prefLabel "коридор"@bg,
        "corridor"@en,
        "korridor"@no,
        "коридор"@ru,
        "korridor"@sv .

gn:T.CRQ a gn:Code ;
    skos:definition "a bowl-like hollow partially surrounded by cliffs or steep slopes at the head of a glaciated valley"@en,
        "естественное чашеобразное углубление в привершинной части горы (обычно со скалистыми или покрытыми льдом, снегом стенами)"@ru ;
    skos:inScheme gn:T ;
    skos:notation "T.CRQ" ;
    skos:prefLabel "циркус"@bg,
        "cirque"@en,
        "dalgryte"@no,
        "цирк"@ru,
        "kitteldal"@sv .

gn:T.CRQS a gn:Code ;
    skos:definition "bowl-like hollows partially surrounded by cliffs or steep slopes at the head of a glaciated valley"@en,
        "естественные чашеобразные углубления в привершинной части горы (обычно со скалистыми или покрытыми льдом, снегом стенами)"@ru ;
    skos:inScheme gn:T ;
    skos:notation "T.CRQS" ;
    skos:prefLabel "циркуси"@bg,
        "cirques"@en,
        "dalgryter"@no,
        "цирки"@ru,
        "kitteldalar"@sv .

gn:T.CRTR a gn:Code ;
    skos:definition "a generally circular saucer or bowl-shaped depression caused by volcanic or meteorite explosive action"@en,
        "углубление на вершине вулкана, из которого при извержении выливается лава"@ru ;
    skos:inScheme gn:T ;
    skos:notation "T.CRTR" ;
    skos:prefLabel "кратер(и)"@bg,
        "crater(s)"@en,
        "krater"@no,
        "кратер"@ru,
        "krater"@sv .

gn:T.CUET a gn:Code ;
    skos:definition "an asymmetric ridge formed on tilted strata"@en,
        "наклонная равнина, круто обрезанная с одной стороны"@ru ;
    skos:inScheme gn:T ;
    skos:notation "T.CUET" ;
    skos:prefLabel "стръмен хълм(ове)"@bg,
        "cuesta(s)"@en,
        "cuesta"@no,
        "куэста"@ru,
        "backe"@sv .

gn:T.DLTA a gn:Code ;
    skos:definition "a flat plain formed by alluvial deposits at the mouth of a stream"@en,
        "устье большой реки с его разветвлениями на отдельные рукава и прилегающая к нему суша"@ru ;
    skos:inScheme gn:T ;
    skos:notation "T.DLTA" ;
    skos:prefLabel "делта"@bg,
        "delta"@en,
        "delta"@no,
        "дельта реки"@ru,
        "delta"@sv .

gn:T.DPR a gn:Code ;
    skos:definition "a low area surrounded by higher land and usually characterized by interior drainage"@en,
        "понижение земной поверхности в пределах суши, на дне океанов и морей"@ru ;
    skos:inScheme gn:T ;
    skos:notation "T.DPR" ;
    skos:prefLabel "депресия(и)"@bg,
        "depression(s)"@en,
        "fordypning"@no,
        "впадина"@ru,
        "depression(er)"@sv .

gn:T.DSRT a gn:Code ;
    skos:definition "a large area with little or no vegetation due to extreme environmental conditions"@en,
        "обширная засушливая область с небольшим количеством осадков, резкими колебаниями воздуха и почвы и скудной растительностью"@ru ;
    skos:inScheme gn:T ;
    skos:notation "T.DSRT" ;
    skos:prefLabel "пустина(и)"@bg,
        "desert"@en,
        "ørken"@no,
        "пустыня"@ru,
        "öken"@sv .

gn:T.DUNE a gn:Code ;
    skos:definition "a wave form, ridge or star shape feature composed of sand"@en,
        "песчаный холм или их группа, образованные ветром на слабо закреплённых растительностью песчаных массивах"@ru ;
    skos:inScheme gn:T ;
    skos:notation "T.DUNE" ;
    skos:prefLabel "дюня(и)"@bg,
        "dune(s)"@en,
        "sanddyne"@no,
        "дюна"@ru,
        "sanddyn(er)"@sv .

gn:T.DVD a gn:Code ;
    skos:definition "a line separating adjacent drainage basins"@en,
        "возвышенная местность между бассейнами рек, разделяющая их"@ru ;
    skos:inScheme gn:T ;
    skos:notation "T.DVD" ;
    skos:prefLabel "разделение"@bg,
        "divide"@en,
        "vannskille"@no,
        "водораздел"@ru,
        "vattendelare"@sv .

gn:T.ERG a gn:Code ;
    skos:definition "an extensive tract of shifting sand and sand dunes"@en,
        "тип пустынь с песчаной поверхностью"@ru ;
    skos:inScheme gn:T ;
    skos:notation "T.ERG" ;
    skos:prefLabel "пясъчна пустиня"@bg,
        "sandy desert"@en,
        "sandørken"@no,
        "песчаная пустыня"@ru,
        "sandöken"@sv .

gn:T.FAN a gn:Code ;
    skos:definition "a fan-shaped wedge of coarse alluvium with apex merging with a mountain stream bed and the fan spreading out at a low angle slope onto an adjacent plain"@en,
        "форма рельефа, имеющая вид слабовыпуклого полуконуса, образованного скоплением рыхлого обломочного материала (аллювия) в устьевой части временных водных потоков и небольших рек или при выходе их из гор на предгорные равнины или из ущелий в более широкую долину"@ru ;
    skos:inScheme gn:T ;
    skos:notation "T.FAN" ;
    skos:prefLabel "ветрило(а)"@bg,
        "fan(s)"@en,
        "avleiringsvifte"@no,
        "конус выноса"@ru,
        "fan(s)"@sv .

gn:T.FORD a gn:Code ;
    skos:definition "a shallow part of a stream which can be crossed on foot or by land vehicle"@en,
        "мелкое место во всю ширину реки, озера и т.п., удобное для перехода, переезда"@ru ;
    skos:inScheme gn:T ;
    skos:notation "T.FORD" ;
    skos:prefLabel "брод"@bg,
        "ford"@en,
        "vadested"@no,
        "брод"@ru,
        "vadställe"@sv .

gn:T.FSR a gn:Code ;
    skos:definition "a crack associated with volcanism"@en,
        "глубокая трещина, узкое ущелье в горной породе, в земле"@ru ;
    skos:inScheme gn:T ;
    skos:notation "T.FSR" ;
    skos:prefLabel "цепнатина"@bg,
        "fissure"@en,
        "revne"@no,
        "расселина"@ru,
        "klyfta, spricka"@sv .

gn:T.GAP a gn:Code ;
    skos:definition "a low place in a ridge, not used for transportation"@en,
        "крутой, глубокий обрыв, очень глубокая расселина, бездна"@ru ;
    skos:inScheme gn:T ;
    skos:notation "T.GAP" ;
    skos:prefLabel "клисура"@bg,
        "gap"@en,
        "kløft"@no,
        "пропасть"@ru,
        "gap, öppning, hål, klyfta"@sv .

gn:T.GRGE a gn:Code ;
    skos:definition "a short, narrow, steep-sided section of a stream valley"@en,
        "узкая крутосклонная долина (обычно в пределах горной страны), промытая рекой в твёрдых коренных породах"@ru ;
    skos:inScheme gn:T ;
    skos:notation "T.GRGE" ;
    skos:prefLabel "пролом(и)"@bg,
        "gorge(s)"@en,
        "juv"@no,
        "ущелье"@ru,
        "trång klyfta mellan berg"@sv .

gn:T.HDLD a gn:Code ;
    skos:definition "a high projection of land extending into a large body of water beyond the line of the coast"@en,
        "часть суши, острым углом вдающаяся в водное пространство (море, озеро, реку)"@ru ;
    skos:inScheme gn:T ;
    skos:notation "T.HDLD" ;
    skos:prefLabel "нос"@bg,
        "headland"@en,
        "pynt"@no,
        "возвышенный мыс"@ru,
        "halvö,udde"@sv .

gn:T.HLL a gn:Code ;
    skos:definition "a rounded elevation of limited extent rising above the surrounding land with local relief of less than 300m"@en,
        "небольшая отлогая горка, возвышенность округлой или овальной формы с пологими склонами"@ru ;
    skos:inScheme gn:T ;
    skos:notation "T.HLL" ;
    skos:prefLabel "възвишение"@bg,
        "hill"@en,
        "ås"@no,
        "холм"@ru,
        "kulle"@sv .

gn:T.HLLS a gn:Code ;
    skos:definition "rounded elevations of limited extent rising above the surrounding land with local relief of less than 300m"@en,
        "небольшие отлогие горки, возвышенности округлой или овальной формы с пологими склонами"@ru ;
    skos:inScheme gn:T ;
    skos:notation "T.HLLS" ;
    skos:prefLabel "възвишения"@bg,
        "hills"@en,
        "åser"@no,
        "холмы"@ru,
        "kullar"@sv .

gn:T.HMCK a gn:Code ;
    skos:definition "a patch of ground, distinct from and slightly above the surrounding plain or wetland. Often occurs in groups"@en,
        "ледяная глыба, образовавшаяся при сжатии льдов на северных морях и реках"@ru ;
    skos:inScheme gn:T ;
    skos:notation "T.HMCK" ;
    skos:prefLabel "хамак(и)"@bg,
        "hammock(s)"@en,
        "hammock (stykker av hevet land)"@no,
        "торос"@ru,
        "hammock"@sv .

gn:T.HMDA a gn:Code ;
    skos:definition "a relatively sand-free, high bedrock plateau in a hot desert, with or without a gravel veneer"@en,
        "тип пустыни, развитой на слабовыветренных коренных породах плато низкогорий и мелкосопочника, покрытых щебнем и галькой (поверхность К. п. почти лишена почвенно-растительного покрова, животный компонент типично пустынный)"@ru ;
    skos:inScheme gn:T ;
    skos:notation "T.HMDA" ;
    skos:prefLabel "пустинно плато"@bg,
        "rock desert"@en,
        "steinørken"@no,
        "каменистая пустыня"@ru,
        "klippöken"@sv .

gn:T.INTF a gn:Code ;
    skos:definition "a relatively undissected upland between adjacent stream valleys"@en,
        "местность, расположенная между двумя реками"@ru ;
    skos:inScheme gn:T ;
    skos:notation "T.INTF" ;
    skos:prefLabel "промеждутък"@bg,
        "interfluve"@en,
        "land mellom to elver"@no,
        "междуречье"@ru,
        "interfluve"@sv .

gn:T.ISL a gn:Code ;
    skos:definition "a tract of land, smaller than a continent, surrounded by water at high water"@en,
        "часть суши, со всех сторон окружённая водой"@ru ;
    skos:inScheme gn:T ;
    skos:notation "T.ISL" ;
    skos:prefLabel "остров"@bg,
        "island"@en,
        "øy"@no,
        "остров"@ru,
        "ö"@sv .

gn:T.ISLET a gn:Code ;
    skos:definition "small island, bigger than rock, smaller than island."@en ;
    skos:historyNote "Added in v3.0"@en ;
    skos:inScheme gn:T ;
    skos:notation "T.ISLET" ;
    skos:prefLabel "islet"@en .

gn:T.ISLF a gn:Code ;
    skos:definition "an island created by landfill or diking and filling in a wetland, bay, or lagoon"@en,
        "искусственный остров (для разработки морских месторождений нефти и газа)"@ru ;
    skos:inScheme gn:T ;
    skos:notation "T.ISLF" ;
    skos:prefLabel "искуствен остров"@bg,
        "artificial island"@en,
        "kunstig øy"@no,
        "искусственный остров"@ru,
        "artificiell ö"@sv .

gn:T.ISLM a gn:Code ;
    skos:definition "a mangrove swamp surrounded by a waterbody"@en,
        "мангровое болото, окруженное водой"@ru ;
    skos:inScheme gn:T ;
    skos:notation "T.ISLM" ;
    skos:prefLabel "мангров остров"@bg,
        "mangrove island"@en,
        "mangroveøy"@no,
        "мангровый остров"@ru,
        "mangrove ö"@sv .

gn:T.ISLS a gn:Code ;
    skos:definition "tracts of land, smaller than a continent, surrounded by water at high water"@en,
        "части суши, со всех сторон окружённые водой"@ru ;
    skos:inScheme gn:T ;
    skos:notation "T.ISLS" ;
    skos:prefLabel "острови"@bg,
        "islands"@en,
        "øyer"@no,
        "острова"@ru,
        "öar"@sv .

gn:T.ISLT a gn:Code ;
    skos:definition "a coastal island connected to the mainland by barrier beaches, levees or dikes"@en,
        "побережье острова, соединенное с материком посредством вырытого рва, траншеи или дамбы"@ru ;
    skos:inScheme gn:T ;
    skos:notation "T.ISLT" ;
    skos:prefLabel "остров свързан със сушата"@bg,
        "land-tied island"@en,
        "øy med landforbindelse"@no,
        "соединяющийся с материком остров"@ru,
        "halvö"@sv .

gn:T.ISLX a gn:Code ;
    skos:inScheme gn:T ;
    skos:notation "T.ISLX" ;
    skos:prefLabel "част от остров"@bg,
        "section of island"@en,
        "del av øy"@no,
        "участок острова"@ru,
        "del av ö"@sv .

gn:T.ISTH a gn:Code ;
    skos:definition "a narrow strip of land connecting two larger land masses and bordered by water"@en,
        "полоса суши, соединяющая два материка или материк с полуостровом и т.п., разделённые водой"@ru ;
    skos:inScheme gn:T ;
    skos:notation "T.ISTH" ;
    skos:prefLabel "провлак"@bg,
        "isthmus"@en,
        "landtunge"@no,
        "перешеек"@ru,
        "näs"@sv .

gn:T.KRST a gn:Code ;
    skos:definition "a distinctive landscape developed on soluble rock such as limestone characterized by sinkholes, caves, disappearing streams, and underground drainage"@en,
        "ландшафт, образованный деятельностью подземных вод на участках суши, поверхность которых сложена растворимыми горными породами: известняками, гипсом, каменной солью и др."@ru ;
    skos:inScheme gn:T ;
    skos:notation "T.KRST" ;
    skos:prefLabel "карст"@bg,
        "karst area"@en,
        "karstområde"@no,
        "карстовый район"@ru,
        "karstområde"@sv .

gn:T.LAVA a gn:Code ;
    skos:definition "an area of solidified lava"@en ;
    skos:inScheme gn:T ;
    skos:notation "T.LAVA" ;
    skos:prefLabel "зона с лава"@bg,
        "lava area"@en,
        "lavaområde"@no,
        "район застывшей лавы"@ru,
        "lavaområde"@sv .

gn:T.LEV a gn:Code ;
    skos:definition "a natural low embankment bordering a distributary or meandering stream; often built up artificially to control floods"@en,
        "гидротехническое сооружение, перегораживающее водоток для подъёма воды в реке, создания водохранилища или электростанции"@ru ;
    skos:inScheme gn:T ;
    skos:notation "T.LEV" ;
    skos:prefLabel "вал"@bg,
        "levee"@en,
        "demning"@no,
        "плотина"@ru,
        "skyddsvall"@sv .

gn:T.MESA a gn:Code ;
    skos:definition "a flat-topped, isolated elevation with steep slopes on all sides, less extensive than a plateau"@en,
        "обширная возвышенность с равнинной или холмистой поверхностью"@ru ;
    skos:inScheme gn:T ;
    skos:notation "T.MESA" ;
    skos:prefLabel "скалисто плато(а)"@bg,
        "mesa(s)"@en,
        "mesa"@no,
        "плоскогорье"@ru,
        "platå(er)"@sv .

gn:T.MND a gn:Code ;
    skos:definition "a low, isolated, rounded hill"@en,
        "холм, горка"@ru ;
    skos:inScheme gn:T ;
    skos:notation "T.MND" ;
    skos:prefLabel "могила(и)"@bg,
        "mound(s)"@en,
        "voll"@no,
        "бугор"@ru,
        "höjd(er)"@sv .

gn:T.MRN a gn:Code ;
    skos:definition "a mound, ridge, or other accumulation of glacial till"@en,
        "скопление обломков горных пород, образуемое на границе передвижения и таяния ледников"@ru ;
    skos:inScheme gn:T ;
    skos:notation "T.MRN" ;
    skos:prefLabel "морена"@bg,
        "moraine"@en,
        "morene"@no,
        "морена"@ru,
        "morän"@sv .

gn:T.MT a gn:Code ;
    skos:definition "an elevation standing high above the surrounding area with small summit area, steep slopes and local relief of 300m or more"@en,
        "Значительная возвышенность, поднимающаяся над окружающей местностью"@ru ;
    skos:inScheme gn:T ;
    skos:notation "T.MT" ;
    skos:prefLabel "планина"@bg,
        "mountain"@en,
        "fjell"@no,
        "гора"@ru,
        "berg"@sv .

gn:T.MTS a gn:Code ;
    skos:definition "a mountain range or a group of mountains or high ridges"@en,
        "значительные возвышенности, поднимающиеся над окружающей местностью"@ru ;
    skos:inScheme gn:T ;
    skos:notation "T.MTS" ;
    skos:prefLabel "планини"@bg,
        "mountains"@en,
        "fjell"@no,
        "горы"@ru,
        "berg"@sv .

gn:T.NKM a gn:Code ;
    skos:definition "a narrow strip of land between the two limbs of a meander loop at its narrowest point"@en,
        "узкий участок суши между двумя краями излучины реки; самая узкая часть меандра реки"@ru ;
    skos:inScheme gn:T ;
    skos:notation "T.NKM" ;
    skos:prefLabel "Извивка между меандри"@bg,
        "meander neck"@en,
        "meanderhals"@no,
        "шейка меандра"@ru,
        "meander neck"@sv .

gn:T.NTK a gn:Code ;
    skos:definition "a rock or mountain peak protruding through glacial ice"@en,
        "изолированный скалистый пик, горный гребень или холм, выступающий над ледниковой поверхностью"@ru ;
    skos:inScheme gn:T ;
    skos:notation "T.NTK" ;
    skos:prefLabel "Ледникова скала"@bg,
        "nunatak"@en,
        "nunatak"@no,
        "нунатак"@ru,
        "nunatak"@sv .

gn:T.NTKS a gn:Code ;
    skos:definition "rocks or mountain peaks protruding through glacial ice"@en,
        "изолированные скалистые пики, горные гребни или холмы, выступающие над ледниковой поверхностью"@ru ;
    skos:inScheme gn:T ;
    skos:notation "T.NTKS" ;
    skos:prefLabel "Ледникови скали"@bg,
        "nunataks"@en,
        "nunatakker"@no,
        "нунатаки"@ru,
        "nunataker"@sv .

gn:T.PAN a gn:Code ;
    skos:definition "a near-level shallow, natural depression or basin, usually containing an intermittent lake, pond, or pool"@en,
        "большое углубление, впадина в земной поверхности с покатым спуском со всех сторон"@ru ;
    skos:inScheme gn:T ;
    skos:notation "T.PAN" ;
    skos:prefLabel "котловина"@bg,
        "pan"@en,
        "aurhelle"@no,
        "котловина"@ru,
        "sänka"@sv .

gn:T.PANS a gn:Code ;
    skos:definition "a near-level shallow, natural depression or basin, usually containing an intermittent lake, pond, or pool"@en,
        "большие углубления, впадины в земной поверхности с покатым спуском со всех сторон"@ru ;
    skos:inScheme gn:T ;
    skos:notation "T.PANS" ;
    skos:prefLabel "котловини"@bg,
        "pans"@en,
        "aurheller"@no,
        "котловины"@ru,
        "sänkor"@sv .

gn:T.PASS a gn:Code ;
    skos:definition "a break in a mountain range or other high obstruction, used for transportation from one side to the other [See also gap]"@en,
        "ущелье, узкий, тесный проход между возвышенностями или водными преградами (в котором можно остановить противника)"@ru ;
    skos:inScheme gn:T ;
    skos:notation "T.PASS" ;
    skos:prefLabel "Дефиле"@bg,
        "pass"@en,
        "pass"@no,
        "дефиле"@ru,
        "bergspass, trång väg(passage)"@sv .

gn:T.PEN a gn:Code ;
    skos:definition "an elongate area of land projecting into a body of water and nearly surrounded by water"@en,
        "часть суши, с трёх сторон омываемая водой, а четвёртой стороной примыкающая к материку или острову"@ru ;
    skos:inScheme gn:T ;
    skos:notation "T.PEN" ;
    skos:prefLabel "полуостров"@bg,
        "peninsula"@en,
        "halvøy"@no,
        "полуостров"@ru,
        "halvö"@sv .

gn:T.PENX a gn:Code ;
    skos:inScheme gn:T ;
    skos:notation "T.PENX" ;
    skos:prefLabel "част от полуостров"@bg,
        "section of peninsula"@en,
        "del av halvøy"@no,
        "участок полуострова"@ru,
        "del av halvö"@sv .

gn:T.PK a gn:Code ;
    skos:definition "a pointed elevation atop a mountain, ridge, or other hypsographic feature"@en,
        "остроконечная горная вершина или высшая точка горной вершины вообще"@ru ;
    skos:inScheme gn:T ;
    skos:notation "T.PK" ;
    skos:prefLabel "връх"@bg,
        "peak"@en,
        "tind"@no,
        "пик"@ru,
        "topp"@sv .

gn:T.PKS a gn:Code ;
    skos:definition "pointed elevations atop a mountain, ridge, or other hypsographic features"@en,
        "остроконечные горные вершины"@ru ;
    skos:inScheme gn:T ;
    skos:notation "T.PKS" ;
    skos:prefLabel "върхове"@bg,
        "peaks"@en,
        "tinder"@no,
        "пики"@ru,
        "toppar"@sv .

gn:T.PLAT a gn:Code ;
    skos:definition "an elevated plain with steep slopes on one or more sides, and often with incised streams"@en,
        "возвышенная равнина, ограниченная чётко выраженными уступами, крутыми склонами"@ru ;
    skos:inScheme gn:T ;
    skos:notation "T.PLAT" ;
    skos:prefLabel "плато"@bg,
        "plateau"@en,
        "platå"@no,
        "плато"@ru,
        "platå"@sv .

gn:T.PLATX a gn:Code ;
    skos:inScheme gn:T ;
    skos:notation "T.PLATX" ;
    skos:prefLabel "част от плато"@bg,
        "section of plateau"@en,
        "del av platå"@no,
        "участок плато"@ru,
        "del av platå"@sv .

gn:T.PLDR a gn:Code ;
    skos:definition "an area reclaimed from the sea by diking and draining"@en,
        "осушенный участок моря или другого водоёма"@ru ;
    skos:inScheme gn:T ;
    skos:notation "T.PLDR" ;
    skos:prefLabel "Преградена с дига зона"@bg,
        "polder"@en,
        "polder"@no,
        "польдер"@ru,
        "invallat landområde"@sv .

gn:T.PLN a gn:Code ;
    skos:definition "an extensive area of comparatively level to gently undulating land, lacking surface irregularities, and usually adjacent to a higher area"@en,
        "обширный участок суши без значительных повышений и понижений поверхности"@ru ;
    skos:inScheme gn:T ;
    skos:notation "T.PLN" ;
    skos:prefLabel "поле(та)"@bg,
        "plain(s)"@en,
        "sletteland"@no,
        "равнина"@ru,
        "slätt(land)"@sv .

gn:T.PLNX a gn:Code ;
    skos:inScheme gn:T ;
    skos:notation "T.PLNX" ;
    skos:prefLabel "Част от поле"@bg,
        "section of plain"@en,
        "del av slette"@no,
        "участок равнины"@ru,
        "del av slättland"@sv .

gn:T.PROM a gn:Code ;
    skos:definition "a bluff or prominent hill overlooking or projecting into a lowland"@en,
        "выступ, мыс"@ru ;
    skos:inScheme gn:T ;
    skos:notation "T.PROM" ;
    skos:prefLabel "издатина(и)"@bg,
        "promontory(-ies)"@en,
        "tange"@no,
        "промонторий"@ru,
        "hög udde"@sv .

gn:T.PT a gn:Code ;
    skos:definition "a tapering piece of land projecting into a body of water, less prominent than a cape"@en,
        "длинная узкая отмель, идущая от берега, или низменный узкий мыс"@ru ;
    skos:inScheme gn:T ;
    skos:notation "T.PT" ;
    skos:prefLabel "Място"@bg,
        "point"@en,
        "odde"@no,
        "выступающая морская коса"@ru,
        "udde"@sv .

gn:T.PTS a gn:Code ;
    skos:definition "tapering pieces of land projecting into a body of water, less prominent than a cape"@en,
        "длинные узкие отмели, идущие от берега, или низменные узкие мысы"@ru ;
    skos:inScheme gn:T ;
    skos:notation "T.PTS" ;
    skos:prefLabel "Места"@bg,
        "points"@en,
        "odder"@no,
        "выступающие морские косы"@ru,
        "uddar"@sv .

gn:T.RDGB a gn:Code ;
    skos:definition "a ridge of sand just inland and parallel to the beach, usually in series"@en,
        "песчаная гряда, находящаяся на суше или идущая параллельно пляжу"@ru ;
    skos:inScheme gn:T ;
    skos:notation "T.RDGB" ;
    skos:prefLabel "Плажен хребет"@bg,
        "beach ridge"@en,
        "strandrygg"@no,
        "гребень косы"@ru,
        "bergskam"@sv .

gn:T.RDGE a gn:Code ;
    skos:definition "a long narrow elevation with steep sides, and a more or less continuous crest"@en,
        "ряд гор, тянущихся в одном направлении, горная цепь"@ru ;
    skos:inScheme gn:T ;
    skos:notation "T.RDGE" ;
    skos:prefLabel "хребет(и)"@bg,
        "ridge(s)"@en,
        "rygg"@no,
        "горный хребет"@ru,
        "rygg, kam, ås"@sv .

gn:T.REG a gn:Code ;
    skos:definition "a desert plain characterized by a surface veneer of gravel and stones"@en,
        "каменистая пустыня"@ru ;
    skos:inScheme gn:T ;
    skos:notation "T.REG" ;
    skos:prefLabel "камениста пустиня"@bg,
        "stony desert"@en,
        "steinørken"@no,
        "гаммада"@ru,
        "stenöken"@sv .

gn:T.RK a gn:Code ;
    skos:definition "a conspicuous, isolated rocky mass"@en,
        "каменная глыба, утёс с крутыми склонами и острыми выступами"@ru ;
    skos:inScheme gn:T ;
    skos:notation "T.RK" ;
    skos:prefLabel "скала"@bg,
        "rock"@en,
        "stein"@no,
        "скала"@ru,
        "klippa"@sv .

gn:T.RKFL a gn:Code ;
    skos:definition "an irregular mass of fallen rock at the base of a cliff or steep slope"@en,
        "камни, низвергающиеся с гор лавиной"@ru ;
    skos:inScheme gn:T ;
    skos:notation "T.RKFL" ;
    skos:prefLabel "Свлачище"@bg,
        "rockfall"@en,
        "steinras"@no,
        "камнепад"@ru,
        "ras"@sv .

gn:T.RKS a gn:Code ;
    skos:definition "conspicuous, isolated rocky masses"@en,
        "остроконечные горные вершины или высшие точки горной вершины вообще"@ru ;
    skos:inScheme gn:T ;
    skos:notation "T.RKS" ;
    skos:prefLabel "скали"@bg,
        "rocks"@en,
        "klipper"@no,
        "скалы"@ru,
        "klippor"@sv .

gn:T.SAND a gn:Code ;
    skos:definition "a tract of land covered with sand"@en,
        "территория, покрытая песками"@ru ;
    skos:inScheme gn:T ;
    skos:notation "T.SAND" ;
    skos:prefLabel "Пясъчна област"@bg,
        "sand area"@en,
        "sandområde"@no,
        "район песков"@ru,
        "sandområde"@sv .

gn:T.SBED a gn:Code ;
    skos:definition "a channel formerly containing the water of a stream"@en,
        "углубление в почве, по которому ранее текла вода"@ru ;
    skos:inScheme gn:T ;
    skos:notation "T.SBED" ;
    skos:prefLabel "Сухо легло на поток"@bg,
        "dry stream bed"@en,
        "tørt elveleie"@no,
        "высохшее речное русло"@ru,
        "uttorkad flodbädd"@sv .

gn:T.SCRP a gn:Code ;
    skos:definition "a long line of cliffs or steep slopes separating level surfaces above and below"@en,
        "покатая поверхность горы, холма и т.п.; склон"@ru ;
    skos:inScheme gn:T ;
    skos:notation "T.SCRP" ;
    skos:prefLabel "Насип"@bg,
        "escarpment"@en,
        "bratt skråning"@no,
        "откос"@ru,
        "brant sluttning"@sv .

gn:T.SDL a gn:Code ;
    skos:definition "a broad, open pass crossing a ridge or between hills or mountains"@en,
        "продолговатая впадина, понижение между вершинами горного хребта или возвышенности"@ru ;
    skos:inScheme gn:T ;
    skos:notation "T.SDL" ;
    skos:prefLabel "Седловина"@bg,
        "saddle"@en,
        "sal"@no,
        "седловина"@ru,
        "sadelformad bergsrygg"@sv .

gn:T.SHOR a gn:Code ;
    skos:definition "a narrow zone bordering a waterbody which covers and uncovers at high and low water, respectively"@en,
        "полоса земной поверхности по обе стороны береговой линии моря, озера, водохранилища"@ru ;
    skos:inScheme gn:T ;
    skos:notation "T.SHOR" ;
    skos:prefLabel "бряг"@bg,
        "shore"@en,
        "bredd"@no,
        "побережье"@ru,
        "kust, strand"@sv .

gn:T.SINK a gn:Code ;
    skos:definition "a small crater-shape depression in a karst area"@en,
        "отрицательная форма рельефа, замкнутая впадина чашеобразной, конической или другой формы, диаметром до 50 метров, глубиной до 15 (иногда до 200) метров"@ru ;
    skos:inScheme gn:T ;
    skos:notation "T.SINK" ;
    skos:prefLabel "Впадина"@bg,
        "sinkhole"@en,
        "jordfallshull"@no,
        "карстовая воронка"@ru,
        "sänka"@sv .

gn:T.SLID a gn:Code ;
    skos:definition "a mound of earth material, at the base of a slope and the associated scoured area"@en,
        "естественное или специально сооруженное возвышение для спуска на лыжах, санках и т.п."@ru ;
    skos:inScheme gn:T ;
    skos:notation "T.SLID" ;
    skos:prefLabel "Стръмнина"@bg,
        "slide"@en,
        "ras"@no,
        "горка"@ru,
        "kana"@sv .

gn:T.SLP a gn:Code ;
    skos:definition "a surface with a relatively uniform slope angle"@en,
        "наклонная поверхность, скат (горы, холма и т.п.)"@ru ;
    skos:inScheme gn:T ;
    skos:notation "T.SLP" ;
    skos:prefLabel "наклон(и)"@bg,
        "slope(s)"@en,
        "kontinentalskråning"@no,
        "склон"@ru,
        "sluttning"@sv .

gn:T.SPIT a gn:Code ;
    skos:definition "a narrow, straight or curved continuation of a beach into a waterbody"@en,
        "узкий и длинный мыс при слиянии двух рек; песчаная коса, намытая прибоем"@ru ;
    skos:inScheme gn:T ;
    skos:notation "T.SPIT" ;
    skos:prefLabel "Дълъг подводен бряг"@bg,
        "spit"@en,
        "tange"@no,
        "стрелка"@ru,
        "landtunga"@sv .

gn:T.SPUR a gn:Code ;
    skos:definition "a subordinate ridge projecting outward from a hill, mountain or other elevation"@en,
        "ответвление основной горной цепи"@ru ;
    skos:inScheme gn:T ;
    skos:notation "T.SPUR" ;
    skos:prefLabel "Издадена скала(и)"@bg,
        "spur(s)"@en,
        "utspring"@no,
        "отрог"@ru,
        "utlöpare"@sv .

gn:T.TAL a gn:Code ;
    skos:definition "a steep concave slope formed by an accumulation of loose rock fragments at the base of a cliff or steep slope"@en,
        "пологий спуск, покрытый обломками горных пород, осыпающимися в результате выветривания"@ru ;
    skos:inScheme gn:T ;
    skos:notation "T.TAL" ;
    skos:prefLabel "Склон"@bg,
        "talus slope"@en,
        "steinur"@no,
        "скат, покрытый осыпью"@ru,
        "stenrassluttning"@sv .

gn:T.TRGD a gn:Code ;
    skos:definition "a long wind-swept trough between parallel longitudinal dunes"@en,
        "понижение земной поверхности в пределах суши, на дне океанов и морей, расположенное между двумя дюнами"@ru ;
    skos:inScheme gn:T ;
    skos:notation "T.TRGD" ;
    skos:prefLabel "бразда(и) между дюни"@bg,
        "interdune trough(s)"@en,
        "dal mellom sanddyner"@no,
        "впадина между дюнами"@ru,
        "ränna mellan dyner"@sv .

gn:T.TRR a gn:Code ;
    skos:definition "a long, narrow alluvial platform bounded by steeper slopes above and below, usually overlooking a waterbody"@en,
        "горизонтальная или слегка наклонная площадка, образующая уступ на склоне местности, естественного происхождения или устроенная искусственно"@ru ;
    skos:inScheme gn:T ;
    skos:notation "T.TRR" ;
    skos:prefLabel "тераса"@bg,
        "terrace"@en,
        "terrasse"@no,
        "терраса"@ru,
        "terass"@sv .

gn:T.UPLD a gn:Code ;
    skos:definition "an extensive interior region of high land with low to moderate surface relief"@en,
        "обширная возвышенность с равнинной или холмистой поверхностью"@ru ;
    skos:inScheme gn:T ;
    skos:notation "T.UPLD" ;
    skos:prefLabel "низина"@bg,
        "upland"@en,
        "oppland"@no,
        "плоскогорье"@ru,
        "högland"@sv .

gn:T.VAL a gn:Code ;
    skos:definition "an elongated depression usually traversed by a stream"@en,
        "удлинённая впадина между гор или в холмистой местности; равнина вдоль речного русла"@ru ;
    skos:inScheme gn:T ;
    skos:notation "T.VAL" ;
    skos:prefLabel "долина"@bg,
        "valley"@en,
        "dal"@no,
        "долина"@ru,
        "dal"@sv .

gn:T.VALG a gn:Code ;
    skos:definition "a valley the floor of which is notably higher than the valley or shore to which it leads; most common in areas that have been glaciated"@en,
        "боковая долина, днище которой оканчивается выше днища главной долины"@ru ;
    skos:inScheme gn:T ;
    skos:notation "T.VALG" ;
    skos:prefLabel "Наклонена долина"@bg,
        "hanging valley"@en,
        "hengende dal"@no,
        "висячая долина"@ru,
        "hängdal"@sv .

gn:T.VALS a gn:Code ;
    skos:definition "elongated depressions usually traversed by a stream"@en,
        "удлинённые впадины между гор или в холмистой местности; равнины вдоль речного русла"@ru ;
    skos:inScheme gn:T ;
    skos:notation "T.VALS" ;
    skos:prefLabel "долини"@bg,
        "valleys"@en,
        "daler"@no,
        "долины"@ru,
        "dalar"@sv .

gn:T.VALX a gn:Code ;
    skos:inScheme gn:T ;
    skos:notation "T.VALX" ;
    skos:prefLabel "част от долина"@bg,
        "section of valley"@en,
        "del av dal"@no,
        "участок долины"@ru,
        "del av dal"@sv .

gn:T.VLC a gn:Code ;
    skos:definition "a conical elevation composed of volcanic materials with a crater at the top"@en,
        "конусообразная гора с кратером на вершине, через который из недр земли извергаются огонь, лава, пепел, горячие газы, пары воды и обломки горных пород"@ru ;
    skos:inScheme gn:T ;
    skos:notation "T.VLC" ;
    skos:prefLabel "вулкан"@bg,
        "volcano"@en,
        "vulkan"@no,
        "вулкан"@ru,
        "vulkan"@sv .

gn:U.APNU a gn:Code ;
    skos:definition "a gentle slope, with a generally smooth surface, particularly found around groups of islands and seamounts"@en,
        "прибрежная мелководная зона океана (с глубинами до 200 м); материковая отмель"@ru ;
    skos:inScheme gn:U ;
    skos:notation "U.APNU" ;
    skos:prefLabel "Козирка"@bg,
        "apron"@en,
        "slette"@no,
        "береговой шельф"@ru,
        "plattform"@sv .

gn:U.ARCU a gn:Code ;
    skos:definition "a low bulge around the southeastern end of the island of Hawaii"@en,
        "территория, пространство, границы которого имеют форму изогнутой линии (например, дуга на юго-востоке Гавайского хребта)"@ru ;
    skos:inScheme gn:U ;
    skos:notation "U.ARCU" ;
    skos:prefLabel "Арка"@bg,
        "arch"@en,
        "bue"@no,
        "дуга"@ru,
        "båge, valv"@sv .

gn:U.ARRU a gn:Code ;
    skos:definition "an area of subdued corrugations off Baja California"@en,
        "an area of subdued corrugations off Baja California"@ru ;
    skos:inScheme gn:U ;
    skos:notation "U.ARRU" ;
    skos:prefLabel "Нагъване"@bg,
        "arrugado"@en,
        "arrugado"@no,
        "arrugado"@ru,
        "veckig"@sv .

gn:U.BDLU a gn:Code ;
    skos:definition "a region adjacent to a continent, normally occupied by or bordering a shelf, that is highly irregular with depths well in excess of those typical of a shelf"@en,
        "невысокий порог, отделяющий геосинклиналь от океана"@ru ;
    skos:inScheme gn:U ;
    skos:notation "U.BDLU" ;
    skos:prefLabel "Гранична област"@bg,
        "borderland"@en,
        "grenseområde"@no,
        "бордерленд"@ru,
        "gränsland"@sv .

gn:U.BKSU a gn:Code ;
    skos:definition "elevations, typically located on a shelf, over which the depth of water is relatively shallow but sufficient for safe surface navigation"@en,
        "геологические образования, обязанные своим происхождением деятельности текучей воды; возвышенности на поверхности шельфа, не препятствующие судоходству"@ru ;
    skos:inScheme gn:U ;
    skos:notation "U.BKSU" ;
    skos:prefLabel "Крайбрежия"@bg,
        "banks"@en,
        "bredd"@no,
        "наносы"@ru,
        "strandsluttningar"@sv .

gn:U.BNCU a gn:Code ;
    owl:deprecated true ;
    skos:definition "a small terrace"@en ;
    skos:inScheme gn:U ;
    skos:notation "U.BNCU" ;
    skos:prefLabel "bench"@en .

gn:U.BNKU a gn:Code ;
    skos:definition "an elevation, typically located on a shelf, over which the depth of water is relatively shallow but sufficient for safe surface navigation"@en,
        "геологическое образование, обязанное своим происхождением деятельности текучей воды; возвышенность на поверхности шельфа, не препятствующее судоходству"@ru ;
    skos:inScheme gn:U ;
    skos:notation "U.BNKU" ;
    skos:prefLabel "Крайбрежие"@bg,
        "bank"@en,
        "bredd"@no,
        "нанос"@ru,
        "strandsluttning, vall"@sv .

gn:U.BSNU a gn:Code ;
    skos:definition "a depression more or less equidimensional in plan and of variable extent"@en,
        "понижение земной поверхности в пределах суши, на дне океанов и морей"@ru ;
    skos:inScheme gn:U ;
    skos:notation "U.BSNU" ;
    skos:prefLabel "басейн"@bg,
        "basin"@en,
        "basseng"@no,
        "впадина"@ru,
        "sänka, bassäng"@sv .

gn:U.CDAU a gn:Code ;
    skos:definition "an entire mountain system including the subordinate ranges, interior plateaus, and basins"@en,
        "горная цепь"@ru ;
    skos:inScheme gn:U ;
    skos:notation "U.CDAU" ;
    skos:prefLabel "кордилиери"@bg,
        "cordillera"@en,
        "fjellkjede"@no,
        "кордельера"@ru,
        "bergskedja"@sv .

gn:U.CNSU a gn:Code ;
    skos:definition "relatively narrow, deep depressions with steep sides, the bottom of which generally has a continuous slope"@en,
        "глубокие речные долины с очень крутыми или отвесными склонами"@ru ;
    skos:inScheme gn:U ;
    skos:notation "U.CNSU" ;
    skos:prefLabel "каньони"@bg,
        "canyons"@en,
        "canyoner"@no,
        "каньоны"@ru,
        "kanjoner"@sv .

gn:U.CNYU a gn:Code ;
    skos:definition "a relatively narrow, deep depression with steep sides, the bottom of which generally has a continuous slope"@en,
        "глубокая речная долина с очень крутыми или отвесными склонами"@ru ;
    skos:inScheme gn:U ;
    skos:notation "U.CNYU" ;
    skos:prefLabel "каньон"@bg,
        "canyon"@en,
        "canyon"@no,
        "каньон"@ru,
        "kanjon"@sv .

gn:U.CRSU a gn:Code ;
    skos:definition "a gentle slope rising from oceanic depths towards the foot of a continental slope"@en,
        "континентальное подножие, один из основных элементов подводной окраины материков; расположено между основанием материкового склона и внешней границей ложа океана"@ru ;
    skos:inScheme gn:U ;
    skos:notation "U.CRSU" ;
    skos:prefLabel "Континентална издатина"@bg,
        "continental rise"@en,
        "kontinentalstigning"@no,
        "материковое подножие"@ru,
        "kontinentalhöjning"@sv .

gn:U.DEPU a gn:Code ;
    skos:definition "a localized deep area within the confines of a larger feature, such as a trough, basin or trench"@en,
        "водная глубь, морская бездна; глубокий провал в болоте, топь"@ru ;
    skos:inScheme gn:U ;
    skos:notation "U.DEPU" ;
    skos:prefLabel "Бездна"@bg,
        "deep"@en,
        "dyp"@no,
        "пучина"@ru,
        "djup"@sv .

gn:U.EDGU a gn:Code ;
    skos:definition "a line along which there is a marked increase of slope at the outer margin of a continental shelf or island shelf"@en,
        "внешний край континентального шельфа"@ru ;
    skos:inScheme gn:U ;
    skos:notation "U.EDGU" ;
    skos:prefLabel "бряг"@bg,
        "shelf edge"@en,
        "kontinentalsokkelkant"@no,
        "бровка шельфа"@ru,
        "shelf edge"@sv .

gn:U.ESCU a gn:Code ;
    skos:definition "an elongated and comparatively steep slope separating flat or gently sloping areas"@en,
        "отвесная скала"@ru ;
    skos:inScheme gn:U ;
    skos:notation "U.ESCU" ;
    skos:prefLabel "Насип"@bg,
        "escarpment (or scarp)"@en,
        "bratt skråning"@no,
        "утес"@ru,
        "brant sluttning"@sv .

gn:U.FANU a gn:Code ;
    skos:definition "a relatively smooth feature normally sloping away from the lower termination of a canyon or canyon system"@en,
        "аккумулятивная форма рельефа, образованная скоплением обломочных пород, вынесенных горными реками на предгорную равнину или в более плоскую широкую долину, где происходит резкое уменьшение живой силы потока"@ru ;
    skos:inScheme gn:U ;
    skos:notation "U.FANU" ;
    skos:prefLabel "Вертрило"@bg,
        "fan"@en,
        "avleiringsvifte"@no,
        "конус выступа"@ru,
        "fan"@sv .

gn:U.FLTU a gn:Code ;
    skos:definition "a small level or nearly level area"@en,
        "равнина, расположенная не выше 200 м над уровнем моря; низменная территория, местность"@ru ;
    skos:inScheme gn:U ;
    skos:notation "U.FLTU" ;
    skos:prefLabel "Плитчина"@bg,
        "flat"@en,
        "flate"@no,
        "низменность"@ru,
        "flat"@sv .

gn:U.FRKU a gn:Code ;
    owl:deprecated true ;
    skos:definition "a branch of a canyon or valley"@en ;
    skos:inScheme gn:U ;
    skos:notation "U.FRKU" ;
    skos:prefLabel "fork"@en .

gn:U.FRSU a gn:Code ;
    owl:deprecated true ;
    skos:definition "a branch of a canyon or valley"@en ;
    skos:inScheme gn:U ;
    skos:notation "U.FRSU" ;
    skos:prefLabel "forks"@en .

gn:U.FRZU a gn:Code ;
    skos:definition "an extensive linear zone of irregular topography of the sea floor, characterized by steep-sided or asymmetrical ridges, troughs, or escarpments"@en,
        "система крупных разломов (сбросов) и грабенов (рифтов)"@ru ;
    skos:inScheme gn:U ;
    skos:notation "U.FRZU" ;
    skos:prefLabel "Зона на накъсване"@bg,
        "fracture zone"@en,
        "bruddsone"@no,
        "зона разломов земной коры"@ru,
        "fracture zone"@sv .

gn:U.FURU a gn:Code ;
    skos:definition "a closed, linear, narrow, shallow depression"@en,
        "длинная узкая впадина на дне океана или моря"@ru ;
    skos:inScheme gn:U ;
    skos:notation "U.FURU" ;
    skos:prefLabel "Улей"@bg,
        "furrow"@en,
        "fure"@no,
        "желоб"@ru,
        "spår"@sv .

gn:U.GAPU a gn:Code ;
    skos:definition "a narrow break in a ridge or rise"@en,
        "узкая крутосклонная долина (обычно в пределах горной страны), промытая рекой в твёрдых коренных породах"@ru ;
    skos:inScheme gn:U ;
    skos:notation "U.GAPU" ;
    skos:prefLabel "клисура"@bg,
        "gap"@en,
        "passasje"@no,
        "ущелье"@ru,
        "klyfta"@sv .

gn:U.GLYU a gn:Code ;
    skos:definition "a small valley-like feature"@en,
        "впадина в земле, промытая ливнем, образованная потоком воды"@ru ;
    skos:inScheme gn:U ;
    skos:notation "U.GLYU" ;
    skos:prefLabel "Дере"@bg,
        "gully"@en,
        "renne"@no,
        "промоина"@ru,
        "ravin"@sv .

gn:U.HLLU a gn:Code ;
    skos:definition "an elevation rising generally less than 500 meters"@en,
        "возвышенность, высота которой менее 500 метров"@ru ;
    skos:inScheme gn:U ;
    skos:notation "U.HLLU" ;
    skos:prefLabel "Стръмнина"@bg,
        "hill"@en,
        "ås"@no,
        "холм"@ru,
        "kulle"@sv .

gn:U.HLSU a gn:Code ;
    skos:definition "elevations rising generally less than 500 meters"@en,
        "возвышенности, высота которых менее 500 метров"@ru ;
    skos:inScheme gn:U ;
    skos:notation "U.HLSU" ;
    skos:prefLabel "Стръмнини"@bg,
        "hills"@en,
        "åser"@no,
        "холмы"@ru,
        "kullar"@sv .

gn:U.HOLU a gn:Code ;
    skos:definition "a small depression of the sea floor"@en,
        "понижение земной поверхности в пределах суши, на дне океанов и морей"@ru ;
    skos:inScheme gn:U ;
    skos:notation "U.HOLU" ;
    skos:prefLabel "Вдлъбнатина"@bg,
        "hole"@en,
        "hull"@no,
        "впадина"@ru,
        "hål"@sv .

gn:U.KNLU a gn:Code ;
    skos:definition "an elevation rising generally more than 500 meters and less than 1,000 meters and of limited extent across the summit"@en,
        "небольшая подводная возвышенность   округлой или овальной формы с пологими склонами"@ru ;
    skos:inScheme gn:U ;
    skos:notation "U.KNLU" ;
    skos:prefLabel "Хълм"@bg,
        "knoll"@en,
        "knaus"@no,
        "возвышение морского дна"@ru,
        "liten kulle"@sv .

gn:U.KNSU a gn:Code ;
    skos:definition "elevations rising generally more than 500 meters and less than 1,000 meters and of limited extent across the summits"@en,
        "небольшие подводные возвышенности округлой или овальной формы с пологими склонами"@ru ;
    skos:inScheme gn:U ;
    skos:notation "U.KNSU" ;
    skos:prefLabel "Хълмове"@bg,
        "knolls"@en,
        "knauser"@no,
        "возвышения морского дна"@ru,
        "små kullar"@sv .

gn:U.LDGU a gn:Code ;
    skos:definition "a rocky projection or outcrop, commonly linear and near shore"@en,
        "надводные или подводные скалистые возвышения морского дна, опасные для судоходства"@ru ;
    skos:inScheme gn:U ;
    skos:notation "U.LDGU" ;
    skos:prefLabel "тераса"@bg,
        "ledge"@en,
        "avsats"@no,
        "риф"@ru,
        "klippavsats"@sv .

gn:U.LEVU a gn:Code ;
    skos:definition "an embankment bordering a canyon, valley, or seachannel"@en,
        "искусственное земляное возвышение, ограждающее каньон, речную долину или морской канал"@ru ;
    skos:inScheme gn:U ;
    skos:notation "U.LEVU" ;
    skos:prefLabel "Стръмен бряг"@bg,
        "levee"@en,
        "demning"@no,
        "насыпь"@ru,
        "damm"@sv .

gn:U.MDVU a gn:Code ;
    owl:deprecated true ;
    skos:definition "the axial depression of the mid-oceanic ridge system"@en ;
    skos:inScheme gn:U ;
    skos:notation "U.MDVU" ;
    skos:prefLabel "median valley"@en .

gn:U.MESU a gn:Code ;
    skos:definition "an isolated, extensive, flat-topped elevation on the shelf, with relatively steep sides"@en,
        "гора с плоскими вершинами и более или менее крутыми, иногда ступенчатыми склонами"@ru ;
    skos:inScheme gn:U ;
    skos:notation "U.MESU" ;
    skos:prefLabel "Високо плато"@bg,
        "mesa"@en,
        "mesa"@no,
        "столовая гора"@ru,
        "högplatå"@sv .

gn:U.MNDU a gn:Code ;
    skos:definition "a low, isolated, rounded hill"@en,
        "низкий холмик округлой формы на месте погребения"@ru ;
    skos:inScheme gn:U ;
    skos:notation "U.MNDU" ;
    skos:prefLabel "Могила"@bg,
        "mound"@en,
        "voll"@no,
        "могильный холм"@ru,
        "gravkulle"@sv .

gn:U.MOTU a gn:Code ;
    skos:definition "an annular depression that may not be continuous, located at the base of many seamounts, islands, and other isolated elevations"@en,
        "длинное углубление, вырытое в земле"@ru ;
    skos:inScheme gn:U ;
    skos:notation "U.MOTU" ;
    skos:prefLabel "Ров"@bg,
        "moat"@en,
        "vollgrav"@no,
        "ров"@ru,
        "vallgrav"@sv .

gn:U.MTSU a gn:Code ;
    owl:deprecated true ;
    skos:definition "well-delineated subdivisions of a large and complex positive feature"@en ;
    skos:inScheme gn:U ;
    skos:notation "U.MTSU" ;
    skos:prefLabel "mountains"@en .

gn:U.MTU a gn:Code ;
    skos:definition "a well-delineated subdivision of a large and complex positive feature"@en,
        "значительная возвышенность, поднимающаяся над окружающей местностью"@ru ;
    skos:inScheme gn:U ;
    skos:notation "U.MTU" ;
    skos:prefLabel "планина"@bg,
        "mountain"@en,
        "fjell"@no,
        "гора"@ru,
        "berg"@sv .

gn:U.PKSU a gn:Code ;
    skos:definition "prominent elevations, part of a larger feature, either pointed or of very limited extent across the summit"@en,
        "остроконечные горные вершины или высшие точки горной вершины вообще"@ru ;
    skos:inScheme gn:U ;
    skos:notation "U.PKSU" ;
    skos:prefLabel "върхове"@bg,
        "peaks"@en,
        "topper"@no,
        "пики"@ru,
        "toppar"@sv .

gn:U.PKU a gn:Code ;
    skos:definition "a prominent elevation, part of a larger feature, either pointed or of very limited extent across the summit"@en,
        "остроконечная горная вершина или высшая точка горной вершины вообще"@ru ;
    skos:inScheme gn:U ;
    skos:notation "U.PKU" ;
    skos:prefLabel "връх"@bg,
        "peak"@en,
        "topp"@no,
        "пик"@ru,
        "topp"@sv .

gn:U.PLFU a gn:Code ;
    owl:deprecated true ;
    skos:definition "a flat or gently sloping underwater surface extending seaward from the shore"@en ;
    skos:inScheme gn:U ;
    skos:notation "U.PLFU" ;
    skos:prefLabel "platform"@en .

gn:U.PLNU a gn:Code ;
    skos:definition "a flat, gently sloping or nearly level region"@en,
        "участок дна моря, океана без резких колебаний высот"@ru ;
    skos:inScheme gn:U ;
    skos:notation "U.PLNU" ;
    skos:prefLabel "Поле"@bg,
        "plain"@en,
        "slette"@no,
        "равнина"@ru,
        "slätt(land)"@sv .

gn:U.PLTU a gn:Code ;
    skos:definition "a comparatively flat-topped feature of considerable extent, dropping off abruptly on one or more sides"@en,
        "возвышенная равнина, ограниченная чётко выраженными уступами, крутыми склонами"@ru ;
    skos:inScheme gn:U ;
    skos:notation "U.PLTU" ;
    skos:prefLabel "плато"@bg,
        "plateau"@en,
        "platå"@no,
        "плато"@ru,
        "platå"@sv .

gn:U.PNLU a gn:Code ;
    skos:definition "a high tower or spire-shaped pillar of rock or coral, alone or cresting a summit"@en,
        "остроконечная скала"@ru ;
    skos:inScheme gn:U ;
    skos:notation "U.PNLU" ;
    skos:prefLabel "Шпиц"@bg,
        "pinnacle"@en,
        "tind"@no,
        "шпиц"@ru,
        "klippa"@sv .

gn:U.PRVU a gn:Code ;
    skos:definition "a region identifiable by a group of similar physiographic features whose characteristics are markedly in contrast with surrounding areas"@en,
        "часть природной географической зоны в составе определенной физико-географической области; региональная единица физико-географического районирования. Физико-географические провинции выделяются по морфоструктурным особенностям рельефа и климату, а в горах - по характеру высотной поясности"@ru ;
    skos:inScheme gn:U ;
    skos:notation "U.PRVU" ;
    skos:prefLabel "Регион"@bg,
        "province"@en,
        "provins"@no,
        "провинция, физико-географическая"@ru,
        "provins"@sv .

gn:U.RAVU a gn:Code ;
    owl:deprecated true ;
    skos:definition "a small canyon"@en ;
    skos:inScheme gn:U ;
    skos:notation "U.RAVU" ;
    skos:prefLabel "ravine"@en .

gn:U.RDGU a gn:Code ;
    skos:definition "a long narrow elevation with steep sides"@en,
        "цепи невысоких гор"@ru ;
    skos:inScheme gn:U ;
    skos:notation "U.RDGU" ;
    skos:prefLabel "Гребен"@bg,
        "ridge"@en,
        "rygg"@no,
        "горный кряжи"@ru,
        "ås"@sv .

gn:U.RDSU a gn:Code ;
    skos:definition "long narrow elevations with steep sides"@en,
        "цепь невысоких гор"@ru ;
    skos:inScheme gn:U ;
    skos:notation "U.RDSU" ;
    skos:prefLabel "Гребени"@bg,
        "ridges"@en,
        "rygger"@no,
        "горный кряж"@ru,
        "åsar"@sv .

gn:U.RFSU a gn:Code ;
    skos:definition "surface-navigation hazards composed of consolidated material"@en,
        "надводные или подводные скалистые возвышения морского дна, опасные для судоходства"@ru ;
    skos:inScheme gn:U ;
    skos:notation "U.RFSU" ;
    skos:prefLabel "Рифове"@bg,
        "reefs"@en,
        "rev"@no,
        "рифы"@ru,
        "rev"@sv .

gn:U.RFU a gn:Code ;
    skos:definition "a surface-navigation hazard composed of consolidated material"@en,
        "надводные или подводные скалистые возвышения морского дна, опасные для судоходства"@ru ;
    skos:inScheme gn:U ;
    skos:notation "U.RFU" ;
    skos:prefLabel "Риф"@bg,
        "reef"@en,
        "rev"@no,
        "риф"@ru,
        "rev"@sv .

gn:U.RISU a gn:Code ;
    skos:definition "a broad elevation that rises gently, and generally smoothly, from the sea floor"@en,
        "участок морского дна,  возвышающийся над окружающим рельефом"@ru ;
    skos:inScheme gn:U ;
    skos:notation "U.RISU" ;
    skos:prefLabel "възвишение"@bg,
        "rise"@en,
        "stigning"@no,
        "небольшое возвышение морского дна"@ru,
        "höjd"@sv .

gn:U.RMPU a gn:Code ;
    owl:deprecated true ;
    skos:definition "a gentle slope connecting areas of different elevations"@en ;
    skos:inScheme gn:U ;
    skos:notation "U.RMPU" ;
    skos:prefLabel "ramp"@en .

gn:U.RNGU a gn:Code ;
    owl:deprecated true ;
    skos:definition "a series of associated ridges or seamounts"@en ;
    skos:inScheme gn:U ;
    skos:notation "U.RNGU" ;
    skos:prefLabel "range"@en .

gn:U.SCNU a gn:Code ;
    skos:definition "a continuously sloping, elongated depression commonly found in fans or plains and customarily bordered by levees on one or two sides"@en,
        "впадина на дне морского дна, с покатыми краями и защищенная с одной или двух сторон валом"@ru ;
    skos:inScheme gn:U ;
    skos:notation "U.SCNU" ;
    skos:prefLabel "Морски канал"@bg,
        "seachannel"@en,
        "sjøkanal"@no,
        "канал на дне океана"@ru,
        "havskanal"@sv .

gn:U.SCSU a gn:Code ;
    skos:definition "continuously sloping, elongated depressions commonly found in fans or plains and customarily bordered by levees on one or two sides"@en,
        "впадины на дне морского дна с пологими склонами, защищенные с одной или двух сторон валом"@ru ;
    skos:inScheme gn:U ;
    skos:notation "U.SCSU" ;
    skos:prefLabel "Морски канали"@bg,
        "seachannels"@en,
        "sjøkanaler"@no,
        "каналы на дне океана"@ru,
        "havskanaler"@sv .

gn:U.SDLU a gn:Code ;
    skos:definition "a low part, resembling in shape a saddle, in a ridge or between contiguous seamounts"@en,
        "продолговатая впадина, понижение между вершинами подводного горного хребта или возвышенности"@ru ;
    skos:inScheme gn:U ;
    skos:notation "U.SDLU" ;
    skos:prefLabel "Седловина"@bg,
        "saddle"@en,
        "sal"@no,
        "седловина подводной горной цепи"@ru,
        "sadelformad bergsrygg"@sv .

gn:U.SHFU a gn:Code ;
    skos:definition "a zone adjacent to a continent (or around an island) that extends from the low water line to a depth at which there is usually a marked increase of slope towards oceanic depths"@en,
        "прибрежная мелководная зона океана (с глубинами до 200 м); материковая отмель"@ru ;
    skos:inScheme gn:U ;
    skos:notation "U.SHFU" ;
    skos:prefLabel "шелф"@bg,
        "shelf"@en,
        "hylle"@no,
        "шельф"@ru,
        "sandrev, klippavsats"@sv .

gn:U.SHLU a gn:Code ;
    skos:definition "a surface-navigation hazard composed of unconsolidated material"@en,
        "участок (обычно прибрежный) реки, озера и т.п. с небольшой глубиной"@ru ;
    skos:inScheme gn:U ;
    skos:notation "U.SHLU" ;
    skos:prefLabel "Плитчина"@bg,
        "shoal"@en,
        "sandgrunne"@no,
        "мелководье"@ru,
        "grund, sandrev"@sv .

gn:U.SHSU a gn:Code ;
    skos:definition "hazards to surface navigation composed of unconsolidated material"@en,
        "участки (обычно прибрежные) реки, озера и т.п. с небольшой глубиной"@ru ;
    skos:inScheme gn:U ;
    skos:notation "U.SHSU" ;
    skos:prefLabel "Плитчини"@bg,
        "shoals"@en,
        "sandgrunner"@no,
        "мелководья"@ru,
        "sandbankar"@sv .

gn:U.SHVU a gn:Code ;
    skos:definition "a valley on the shelf, generally the shoreward extension of a canyon"@en,
        "относительно мелководная подводная равнина, прилегающая к берегам материков и генетически составляющая часть материковой платформы"@ru ;
    skos:inScheme gn:U ;
    skos:notation "U.SHVU" ;
    skos:prefLabel "Шелфова долина"@bg,
        "shelf valley"@en,
        "dal gjennom kontinentalhyllen"@no,
        "материковая отмель"@ru,
        "shelf valley"@sv .

gn:U.SILU a gn:Code ;
    skos:definition "the low part of a gap or saddle separating basins"@en,
        "каменистое поперечное возвышение дна реки, нарушающее плавность её течения и затрудняющее судоходство"@ru ;
    skos:inScheme gn:U ;
    skos:notation "U.SILU" ;
    skos:prefLabel "Интрузия"@bg,
        "sill"@en,
        "terskel"@no,
        "порог"@ru,
        "tröskel"@sv .

gn:U.SLPU a gn:Code ;
    skos:definition "the slope seaward from the shelf edge to the beginning of a continental rise or the point where there is a general reduction in slope"@en,
        "покатая поверхность горы, холма и т.п.; склон"@ru ;
    skos:inScheme gn:U ;
    skos:notation "U.SLPU" ;
    skos:prefLabel "скат"@bg,
        "slope"@en,
        "skråning"@no,
        "откос"@ru,
        "sluttning"@sv .

gn:U.SMSU a gn:Code ;
    skos:definition "elevations rising generally more than 1,000 meters and of limited extent across the summit"@en,
        "изолированные поднятия морского дна с относительной высотой более 500 м и четко выраженной конической или куполообразной одной или несколькими вершинами и крутыми склонами"@ru ;
    skos:inScheme gn:U ;
    skos:notation "U.SMSU" ;
    skos:prefLabel "Морски връх"@bg,
        "seamounts"@en,
        "undersjøiske fjell"@no,
        "подводные горы"@ru,
        "undervattensberg"@sv .

gn:U.SMU a gn:Code ;
    skos:definition "an elevation rising generally more than 1,000 meters and of limited extent across the summit"@en,
        "изолированное поднятие морского дна с относительной высотой более 500 м и четко выраженной конической или куполообразной одной или несколькими вершинами и крутыми склонами"@ru ;
    skos:inScheme gn:U ;
    skos:notation "U.SMU" ;
    skos:prefLabel "Морски върхове"@bg,
        "seamount"@en,
        "undersjøisk fjell"@no,
        "подводная гора"@ru,
        "undervattensberg"@sv .

gn:U.SPRU a gn:Code ;
    skos:definition "a subordinate elevation, ridge, or rise projecting outward from a larger feature"@en,
        "ряд гор, тянущихся в одном направлении, горная цепь"@ru ;
    skos:inScheme gn:U ;
    skos:notation "U.SPRU" ;
    skos:prefLabel "хребет"@bg,
        "spur"@en,
        "utspring"@no,
        "хребет"@ru,
        "utlöpare"@sv .

gn:U.TERU a gn:Code ;
    skos:definition "a relatively flat horizontal or gently inclined surface, sometimes long and narrow, which is bounded by a steeper ascending slope on one side and by a steep descending slope on the opposite side"@en,
        "горизонтальная или слегка наклонная площадка, образующая уступ на склоне местности, естественного происхождения или устроенная искусственно"@ru ;
    skos:inScheme gn:U ;
    skos:notation "U.TERU" ;
    skos:prefLabel "тераса"@bg,
        "terrace"@en,
        "terrasse"@no,
        "терраса"@ru,
        "terass"@sv .

gn:U.TMSU a gn:Code ;
    skos:definition "seamounts having a comparatively smooth, flat top"@en,
        "плосковершинные подводные вулканические горы, встречающиеся одиночно или группами"@ru ;
    skos:inScheme gn:U ;
    skos:notation "U.TMSU" ;
    skos:prefLabel "Плоски възвишения"@bg,
        "tablemounts (or guyots)"@en,
        "guyoter"@no,
        "гайоты"@ru,
        "undervattensberg"@sv .

gn:U.TMTU a gn:Code ;
    skos:definition "a seamount having a comparatively smooth, flat top"@en,
        "подводный плосковершинный вулкан"@ru ;
    skos:inScheme gn:U ;
    skos:notation "U.TMTU" ;
    skos:prefLabel "Плоско възвишение"@bg,
        "tablemount (or guyot)"@en,
        "guyot"@no,
        "гайот"@ru,
        "undervattensberg"@sv .

gn:U.TNGU a gn:Code ;
    skos:definition "an elongate (tongue-like) extension of a flat sea floor into an adjacent higher feature"@en,
        "длинная узкая отмель, идущая от берега, или низменный узкий мыс"@ru ;
    skos:inScheme gn:U ;
    skos:notation "U.TNGU" ;
    skos:prefLabel "нос"@bg,
        "tongue"@en,
        "landtunge"@no,
        "коса"@ru,
        "landtunga"@sv .

gn:U.TRGU a gn:Code ;
    skos:definition "a long depression of the sea floor characteristically flat bottomed and steep sided, and normally shallower than a trench"@en,
        "углубление с пологими склонами  на дне океанов и морей"@ru ;
    skos:inScheme gn:U ;
    skos:notation "U.TRGU" ;
    skos:prefLabel "падина"@bg,
        "trough"@en,
        "gjennomgang"@no,
        "впадина на дне океана с пологими склонами"@ru,
        "ränna"@sv .

gn:U.TRNU a gn:Code ;
    skos:definition "a long, narrow, characteristically very deep and asymmetrical depression of the sea floor, with relatively steep sides"@en,
        "углубление с крутыми склонами на дне океанов и морей"@ru ;
    skos:inScheme gn:U ;
    skos:notation "U.TRNU" ;
    skos:prefLabel "просека"@bg,
        "trench"@en,
        "renne"@no,
        "впадина на дне океана с крутыми склонами"@ru,
        "dike"@sv .

gn:U.VALU a gn:Code ;
    skos:definition "a relatively shallow, wide depression, the bottom of which usually has a continuous gradient"@en,
        "овраг с пологими склонами"@ru ;
    skos:inScheme gn:U ;
    skos:notation "U.VALU" ;
    skos:prefLabel "долина"@bg,
        "valley"@en,
        "dal"@no,
        "лощина"@ru,
        "dal"@sv .

gn:U.VLSU a gn:Code ;
    skos:definition "a relatively shallow, wide depression, the bottom of which usually has a continuous gradient"@en,
        "овраги с пологими склонами"@ru ;
    skos:inScheme gn:U ;
    skos:notation "U.VLSU" ;
    skos:prefLabel "долини"@bg,
        "valleys"@en,
        "daler"@no,
        "лощины"@ru,
        "dalar"@sv .

gn:V.BUSH a gn:Code ;
    skos:definition "a small clump of conspicuous bushes in an otherwise bare area"@en,
        "заросли куста"@ru ;
    skos:inScheme gn:V ;
    skos:notation "V.BUSH" ;
    skos:prefLabel "храст(и)"@bg,
        "bush(es)"@en,
        "busk"@no,
        "кустарник"@ru,
        "djungel"@sv .

gn:V.CULT a gn:Code ;
    skos:definition "an area under cultivation"@en,
        "площадь, предназначенная для возделывания многих с.-х. культур"@ru ;
    skos:inScheme gn:V ;
    skos:notation "V.CULT" ;
    skos:prefLabel "обработваеми площи"@bg,
        "cultivated area"@en,
        "dyrket mark"@no,
        "посевная площадь"@ru,
        "uppodlat område"@sv .

gn:V.FRST a gn:Code ;
    skos:definition "an area dominated by tree vegetation"@en,
        "множество дикорастущих деревьев, расположенных на большом пространстве; пространство, обильно поросшее деревьями"@ru ;
    skos:inScheme gn:V ;
    skos:notation "V.FRST" ;
    skos:prefLabel "гори"@bg,
        "forest(s)"@en,
        "skog"@no,
        "лес"@ru,
        "skog(ar)"@sv .

gn:V.FRSTF a gn:Code ;
    skos:definition "a forest fossilized by geologic processes and now exposed at the earth's surface"@en,
        "значительное скопление древесных окаменелостей на небольшом участке"@ru ;
    skos:inScheme gn:V ;
    skos:notation "V.FRSTF" ;
    skos:prefLabel "горски вкаменелости"@bg,
        "fossilized forest"@en,
        "forsteinet skog"@no,
        "окаменелый лес"@ru,
        "fossil skog"@sv .

gn:V.GRSLD a gn:Code ;
    skos:definition "an area dominated by grass vegetation"@en,
        "пространство земли, покрытое травянистой растительностью; сенокосное, пастбищное угодье"@ru ;
    skos:inScheme gn:V ;
    skos:notation "V.GRSLD" ;
    skos:prefLabel "ливади"@bg,
        "grassland"@en,
        "gresslette"@no,
        "луг"@ru,
        "grässlätt"@sv .

gn:V.GRVC a gn:Code ;
    skos:definition "a planting of coconut trees"@en,
        "большой участок земли, занятый кокосовыми деревьями"@ru ;
    skos:inScheme gn:V ;
    skos:notation "V.GRVC" ;
    skos:prefLabel "кокосови насаждения"@bg,
        "coconut grove"@en,
        "kokospalmelund"@no,
        "плантация кокосовых деревьев"@ru,
        "kokoslund"@sv .

gn:V.GRVO a gn:Code ;
    skos:definition "a planting of olive trees"@en,
        "большой участок земли, занятый оливковыми деревьями"@ru ;
    skos:inScheme gn:V ;
    skos:notation "V.GRVO" ;
    skos:prefLabel "маслинова плантация"@bg,
        "olive grove"@en,
        "olivenlund"@no,
        "плантация оливковых деревьев"@ru,
        "olivlund"@sv .

gn:V.GRVP a gn:Code ;
    skos:definition "a planting of palm trees"@en,
        "небольшой лесной участок, состоящий из пальмовых деревьев"@ru ;
    skos:inScheme gn:V ;
    skos:notation "V.GRVP" ;
    skos:prefLabel "палмова плантация"@bg,
        "palm grove"@en,
        "palmelund"@no,
        "пальмовая роща"@ru,
        "palmlund"@sv .

gn:V.GRVPN a gn:Code ;
    skos:definition "a planting of pine trees"@en,
        "небольшой лесной участок, состоящий из сосен"@ru ;
    skos:inScheme gn:V ;
    skos:notation "V.GRVPN" ;
    skos:prefLabel "иглолистни насаждения"@bg,
        "pine grove"@en,
        "furulund"@no,
        "сосновая роща"@ru,
        "furulund"@sv .

gn:V.HTH a gn:Code ;
    skos:definition "an upland moor or sandy area dominated by low shrubby vegetation including heather"@en,
        "вересковые пустоши, тип растительности, представленный вечнозелёными кустарниками и кустарничками, преимущественно семейства вересковых, имеющих жёсткие узкие листья"@ru ;
    skos:inScheme gn:V ;
    skos:notation "V.HTH" ;
    skos:prefLabel "пустош"@bg,
        "heath"@en,
        "hei"@no,
        "верещатник"@ru,
        "hed"@sv .

gn:V.MDW a gn:Code ;
    skos:definition "a small, poorly drained area dominated by grassy vegetation"@en,
        "небольшой луг, луг среди других угодий (лесных, пастбищных"@ru ;
    skos:inScheme gn:V ;
    skos:notation "V.MDW" ;
    skos:prefLabel "ливада"@bg,
        "meadow"@en,
        "eng"@no,
        "луговина"@ru,
        "äng"@sv .

gn:V.OCH a gn:Code ;
    skos:definition "a planting of fruit or nut trees"@en,
        "участок земли, на котором выращивают фруктовые деревья"@ru ;
    skos:inScheme gn:V ;
    skos:notation "V.OCH" ;
    skos:prefLabel "овощна градина(и)"@bg,
        "orchard(s)"@en,
        "frukthage"@no,
        "фруктовый сад"@ru,
        "fruktträdgård(ar)"@sv .

gn:V.SCRB a gn:Code ;
    skos:definition "an area of low trees, bushes, and shrubs stunted by some environmental limitation"@en,
        "густо разросшийся кустарник, массив трав, деревьев и т. п."@ru ;
    skos:inScheme gn:V ;
    skos:notation "V.SCRB" ;
    skos:prefLabel "храсти"@bg,
        "scrubland"@en,
        "krattskog"@no,
        "кустарниковая заросль"@ru,
        "buskterräng"@sv .

gn:V.TREE a gn:Code ;
    skos:definition "a conspicuous tree used as a landmark"@en,
        "дерево (известное благодаря чему-л.), являющееся  достопримечательностью"@ru ;
    skos:inScheme gn:V ;
    skos:notation "V.TREE" ;
    skos:prefLabel "дървета"@bg,
        "tree(s)"@en,
        "tre"@no,
        "дерево"@ru,
        "träd"@sv .

gn:V.TUND a gn:Code ;
    skos:definition "a marshy, treeless, high latitude plain, dominated by mosses, lichens, and low shrub vegetation under permafrost conditions"@en,
        "тип растительности высоких широт Северного полушария Земли, характеризующийся развитием мохового и лишайникового покровов, наличием низкорослых кустарников и т.п.; природная зона с таким типом растительности"@ru ;
    skos:inScheme gn:V ;
    skos:notation "V.TUND" ;
    skos:prefLabel "тундра"@bg,
        "tundra"@en,
        "tundra"@no,
        "тундра"@ru,
        "tundra"@sv .

gn:V.VIN a gn:Code ;
    skos:definition "a planting of grapevines"@en,
        "участок, засаженный виноградом; виноградная плантация"@ru ;
    skos:inScheme gn:V ;
    skos:notation "V.VIN" ;
    skos:prefLabel "лозя"@bg,
        "vineyard"@en,
        "vingård"@no,
        "виноградник"@ru,
        "vingård"@sv .

gn:V.VINS a gn:Code ;
    skos:definition "plantings of grapevines"@en,
        "виноградные плантации"@ru ;
    skos:inScheme gn:V ;
    skos:notation "V.VINS" ;
    skos:prefLabel "лозя"@bg,
        "vineyards"@en,
        "vingårder"@no,
        "виноградники"@ru,
        "vingårdar"@sv .

gn:childrenFeatures a owl:ObjectProperty ;
    rdfs:label "children features"@en ;
    rdfs:comment "Links to an RDF document containing the descriptions of children features"@en ;
    rdfs:domain gn:Feature ;
    rdfs:range gn:RDFData .

gn:colloquialName a owl:DatatypeProperty ;
    rdfs:label "colloquial name"@en ;
    rdfs:subPropertyOf gn:alternateName .

gn:historicalName a owl:DatatypeProperty ;
    rdfs:label "historical name"@en ;
    rdfs:subPropertyOf gn:alternateName .

gn:locatedIn a owl:ObjectProperty ;
    rdfs:label "located in"@en ;
    rdfs:comment "Indicates that the subject resource is located in the object feature"@en ;
    rdfs:range gn:Feature .

gn:locationMap a owl:ObjectProperty ;
    rdfs:label "map"@en ;
    rdfs:comment "A geonames map centered on the feature."@en ;
    rdfs:domain gn:Feature ;
    rdfs:range gn:Map .

gn:nearby a owl:ObjectProperty ;
    rdfs:label "nearby"@en ;
    rdfs:comment "A feature close to the reference feature"@en ;
    rdfs:domain gn:Feature ;
    rdfs:range gn:Feature .

gn:nearbyFeatures a owl:ObjectProperty ;
    rdfs:label "nearby features"@en ;
    rdfs:comment "Links to an RDF document containing the descriptions of nearby features"@en ;
    rdfs:domain gn:Feature ;
    rdfs:range gn:RDFData .

gn:neighbour a owl:ObjectProperty,
        owl:SymmetricProperty ;
    rdfs:label "neighbour"@en ;
    rdfs:comment "A feature sharing a common boarder with the reference feature"@en ;
    rdfs:domain gn:Feature ;
    rdfs:range gn:Feature .

gn:neighbouringFeatures a owl:ObjectProperty ;
    rdfs:label "neighbouring features"@en ;
    rdfs:comment "Links to an RDF document containing the descriptions of neighbouring features. Applies when the feature has definite boarders."@en ;
    rdfs:domain gn:Feature ;
    rdfs:range gn:RDFData .

gn:officialName a owl:DatatypeProperty ;
    rdfs:label "official name"@en ;
    rdfs:comment "A name in an official local language"@en ;
    rdfs:domain gn:Feature ;
    rdfs:subPropertyOf skos:prefLabel .

gn:parentCountry a owl:ObjectProperty ;
    rdfs:label "parent country"@en ;
    rdfs:domain gn:Feature ;
    rdfs:range [ a owl:Restriction ;
            owl:hasValue gn:A.PCLI ;
            owl:onProperty gn:featureCode ] ;
    rdfs:subPropertyOf gn:parentFeature .

gn:postalCode a owl:DatatypeProperty ;
    rdfs:label "postal code"@en ;
    rdfs:domain gn:Feature .

gn:shortName a owl:DatatypeProperty ;
    rdfs:label "short name"@en ;
    rdfs:domain gn:Feature ;
    rdfs:subPropertyOf gn:alternateName .

gn:wikipediaArticle a owl:ObjectProperty ;
    rdfs:label "wikipedia article"@en ;
    rdfs:comment "A Wikipedia article of which subject is the resource."@en ;
    rdfs:domain gn:Feature ;
    rdfs:range gn:WikipediaArticle .

geosparql:asGML a owl:DatatypeProperty ;
    rdfs:label "asGML"@en ;
    dc:contributor "Matthew Perry" ;
    dc:creator "OGC GeoSPARQL 1.0 Standard Working Group" ;
    dc:date "2011-06-16"^^xsd:date ;
    dc:description """      The GML serialization of a geometry
    """@en ;
    rdfs:comment """      The GML serialization of a geometry
    """@en ;
    rdfs:domain geosparql:Geometry ;
    rdfs:isDefinedBy <http://www.opengis.net/ont/geosparql>,
        <http://www.opengis.net/spec/geosparql/1.0> ;
    rdfs:range geosparql:gmlLiteral ;
    rdfs:subPropertyOf geosparql:hasSerialization ;
    skos:definition """      The GML serialization of a geometry
    """@en ;
    skos:prefLabel "asGML"@en .

geosparql:asWKT a owl:DatatypeProperty ;
    rdfs:label "asWKT"@en ;
    dc:contributor "Matthew Perry" ;
    dc:creator "OGC GeoSPARQL 1.0 Standard Working Group" ;
    dc:date "2011-06-16"^^xsd:date ;
    dc:description """      The WKT serialization of a geometry
    """@en ;
    rdfs:comment """      The WKT serialization of a geometry
    """@en ;
    rdfs:domain geosparql:Geometry ;
    rdfs:isDefinedBy <http://www.opengis.net/ont/geosparql>,
        <http://www.opengis.net/spec/geosparql/1.0> ;
    rdfs:range geosparql:wktLiteral ;
    rdfs:subPropertyOf geosparql:hasSerialization ;
    skos:definition """      The WKT serialization of a geometry
    """@en ;
    skos:prefLabel "asWKT"@en .

geosparql:coordinateDimension a owl:DatatypeProperty ;
    rdfs:label "coordinateDimension"@en ;
    dc:contributor "Matthew Perry" ;
    dc:creator "OGC GeoSPARQL 1.0 Standard Working Group" ;
    dc:date "2011-06-16"^^xsd:date ;
    dc:description """      The number of measurements or axes needed to describe the position of this
      geometry in a coordinate system.
    """@en ;
    rdfs:comment """      The number of measurements or axes needed to describe the position of this
      geometry in a coordinate system.
    """@en ;
    rdfs:domain geosparql:Geometry ;
    rdfs:isDefinedBy <http://www.opengis.net/ont/geosparql>,
        <http://www.opengis.net/spec/geosparql/1.0> ;
    rdfs:range xsd:integer ;
    skos:definition """      The number of measurements or axes needed to describe the position of this
      geometry in a coordinate system.
    """@en ;
    skos:prefLabel "coordinateDimension"@en .

geosparql:defaultGeometry a owl:ObjectProperty ;
    rdfs:label "defaultGeometry"@en ;
    dc:contributor "Matthew Perry" ;
    dc:creator "OGC GeoSPARQL 1.0 Standard Working Group" ;
    dc:date "2011-06-16"^^xsd:date ;
    dc:description """      The default geometry to be used in spatial calculations.
      It is Usually the most detailed geometry.
    """@en ;
    rdfs:comment """      The default geometry to be used in spatial calculations.
      It is Usually the most detailed geometry.
    """@en ;
    rdfs:domain geosparql:Feature ;
    rdfs:isDefinedBy <http://www.opengis.net/ont/geosparql>,
        <http://www.opengis.net/spec/geosparql/1.0> ;
    rdfs:range geosparql:Geometry ;
    rdfs:subPropertyOf geosparql:hasGeometry ;
    skos:definition """      The default geometry to be used in spatial calculations.
      It is Usually the most detailed geometry.
    """@en ;
    skos:prefLabel "defaultGeometry"@en .

geosparql:dimension a owl:DatatypeProperty ;
    rdfs:label "dimension"@en ;
    dc:contributor "Matthew Perry" ;
    dc:creator "OGC GeoSPARQL 1.0 Standard Working Group" ;
    dc:date "2011-06-16"^^xsd:date ;
    dc:description """      The topological dimension of this geometric object, which 
      must be less than or equal to the coordinate dimension. 
      In non-homogeneous collections, this will return the largest 
      topological dimension of the contained objects.
    """@en ;
    rdfs:comment """      The topological dimension of this geometric object, which 
      must be less than or equal to the coordinate dimension. 
      In non-homogeneous collections, this will return the largest 
      topological dimension of the contained objects.
    """@en ;
    rdfs:domain geosparql:Geometry ;
    rdfs:isDefinedBy <http://www.opengis.net/ont/geosparql>,
        <http://www.opengis.net/spec/geosparql/1.0> ;
    rdfs:range xsd:integer ;
    skos:definition """      The topological dimension of this geometric object, which 
      must be less than or equal to the coordinate dimension. 
      In non-homogeneous collections, this will return the largest 
      topological dimension of the contained objects.
    """@en ;
    skos:prefLabel "dimension"@en .

geosparql:ehContains a owl:ObjectProperty ;
    rdfs:label "contains"@en ;
    dc:contributor "Matthew Perry" ;
    dc:creator "OGC GeoSPARQL 1.0 Standard Working Group" ;
    dc:date "2011-06-16"^^xsd:date ;
    dc:description """      Exists if the subject SpatialObject spatially contains the 
      object SpatialObject. DE-9IM: T*TFF*FF*
    """@en ;
    rdfs:comment """      Exists if the subject SpatialObject spatially contains the 
      object SpatialObject. DE-9IM: T*TFF*FF*
    """@en ;
    rdfs:domain geosparql:SpatialObject ;
    rdfs:isDefinedBy <http://www.opengis.net/ont/geosparql>,
        <http://www.opengis.net/spec/geosparql/1.0> ;
    rdfs:range geosparql:SpatialObject ;
    skos:definition """      Exists if the subject SpatialObject spatially contains the 
      object SpatialObject. DE-9IM: T*TFF*FF*
    """@en ;
    skos:prefLabel "contains"@en .

geosparql:ehCoveredBy a owl:ObjectProperty ;
    rdfs:label "coveredBy"@en ;
    dc:contributor "Matthew Perry" ;
    dc:creator "OGC GeoSPARQL 1.0 Standard Working Group" ;
    dc:date "2011-06-16"^^xsd:date ;
    dc:description """      Exists if the subject SpatialObject is spatially covered 
      by the object SpatialObject. DE-9IM: TFF*TFT**
    """@en ;
    rdfs:comment """      Exists if the subject SpatialObject is spatially covered 
      by the object SpatialObject. DE-9IM: TFF*TFT**
    """@en ;
    rdfs:domain geosparql:SpatialObject ;
    rdfs:isDefinedBy <http://www.opengis.net/ont/geosparql>,
        <http://www.opengis.net/spec/geosparql/1.0> ;
    rdfs:range geosparql:SpatialObject ;
    skos:definition """      Exists if the subject SpatialObject is spatially covered 
      by the object SpatialObject. DE-9IM: TFF*TFT**
    """@en ;
    skos:prefLabel "coveredBy"@en .

geosparql:ehCovers a owl:ObjectProperty ;
    rdfs:label "covers"@en ;
    dc:contributor "Matthew Perry" ;
    dc:creator "OGC GeoSPARQL 1.0 Standard Working Group" ;
    dc:date "2011-06-16"^^xsd:date ;
    dc:description """      Exists if the subject SpatialObject spatially covers the 
      object SpatialObject. DE-9IM: T*TFT*FF*
    """@en ;
    rdfs:comment """      Exists if the subject SpatialObject spatially covers the 
      object SpatialObject. DE-9IM: T*TFT*FF*
    """@en ;
    rdfs:domain geosparql:SpatialObject ;
    rdfs:isDefinedBy <http://www.opengis.net/ont/geosparql>,
        <http://www.opengis.net/spec/geosparql/1.0> ;
    rdfs:range geosparql:SpatialObject ;
    skos:definition """      Exists if the subject SpatialObject spatially covers the 
      object SpatialObject. DE-9IM: T*TFT*FF*
    """@en ;
    skos:prefLabel "covers"@en .

geosparql:ehDisjoint a owl:ObjectProperty ;
    rdfs:label "disjoint"@en ;
    dc:contributor "Matthew Perry" ;
    dc:creator "OGC GeoSPARQL 1.0 Standard Working Group" ;
    dc:date "2011-06-16"^^xsd:date ;
    dc:description """      Exists if the subject SpatialObject is spatially disjoint
      from the object SpatialObject. DE-9IM: FF*FF****
    """@en ;
    rdfs:comment """      Exists if the subject SpatialObject is spatially disjoint
      from the object SpatialObject. DE-9IM: FF*FF****
    """@en ;
    rdfs:domain geosparql:SpatialObject ;
    rdfs:isDefinedBy <http://www.opengis.net/ont/geosparql>,
        <http://www.opengis.net/spec/geosparql/1.0> ;
    rdfs:range geosparql:SpatialObject ;
    skos:definition """      Exists if the subject SpatialObject is spatially disjoint
      from the object SpatialObject. DE-9IM: FF*FF****
    """@en ;
    skos:prefLabel "disjoint"@en .

geosparql:ehEquals a owl:ObjectProperty ;
    rdfs:label "equals"@en ;
    dc:contributor "Matthew Perry" ;
    dc:creator "OGC GeoSPARQL 1.0 Standard Working Group" ;
    dc:date "2011-06-16"^^xsd:date ;
    dc:description """      Exists if the subject SpatialObject spatially equals the 
      object SpatialObject. DE-9IM: TFFFTFFFT
    """@en ;
    rdfs:comment """      Exists if the subject SpatialObject spatially equals the 
      object SpatialObject. DE-9IM: TFFFTFFFT
    """@en ;
    rdfs:domain geosparql:SpatialObject ;
    rdfs:isDefinedBy <http://www.opengis.net/ont/geosparql>,
        <http://www.opengis.net/spec/geosparql/1.0> ;
    rdfs:range geosparql:SpatialObject ;
    skos:definition """      Exists if the subject SpatialObject spatially equals the 
      object SpatialObject. DE-9IM: TFFFTFFFT
    """@en ;
    skos:prefLabel "equals"@en .

geosparql:ehInside a owl:ObjectProperty ;
    rdfs:label "inside"@en ;
    dc:contributor "Matthew Perry" ;
    dc:creator "OGC GeoSPARQL 1.0 Standard Working Group" ;
    dc:date "2011-06-16"^^xsd:date ;
    dc:description """      Exists if the subject SpatialObject is spatially inside 
      the object SpatialObject. DE-9IM: TFF*FFT**
    """@en ;
    rdfs:comment """      Exists if the subject SpatialObject is spatially inside 
      the object SpatialObject. DE-9IM: TFF*FFT**
    """@en ;
    rdfs:domain geosparql:SpatialObject ;
    rdfs:isDefinedBy <http://www.opengis.net/ont/geosparql>,
        <http://www.opengis.net/spec/geosparql/1.0> ;
    rdfs:range geosparql:SpatialObject ;
    skos:definition """      Exists if the subject SpatialObject is spatially inside 
      the object SpatialObject. DE-9IM: TFF*FFT**
    """@en ;
    skos:prefLabel "inside"@en .

geosparql:ehMeet a owl:ObjectProperty ;
    rdfs:label "meet"@en ;
    dc:contributor "Matthew Perry" ;
    dc:creator "OGC GeoSPARQL 1.0 Standard Working Group" ;
    dc:date "2011-06-16"^^xsd:date ;
    dc:description """      Exists if the subject SpatialObject spatially meets the 
      object SpatialObject. 
      DE-9IM: FT******* ^ F**T***** ^ F***T****
    """@en ;
    rdfs:comment """      Exists if the subject SpatialObject spatially meets the 
      object SpatialObject. 
      DE-9IM: FT******* ^ F**T***** ^ F***T****
    """@en ;
    rdfs:domain geosparql:SpatialObject ;
    rdfs:isDefinedBy <http://www.opengis.net/ont/geosparql>,
        <http://www.opengis.net/spec/geosparql/1.0> ;
    rdfs:range geosparql:SpatialObject ;
    skos:definition """      Exists if the subject SpatialObject spatially meets the 
      object SpatialObject. 
      DE-9IM: FT******* ^ F**T***** ^ F***T****
    """@en ;
    skos:prefLabel "meet"@en .

geosparql:ehOverlap a owl:ObjectProperty ;
    rdfs:label "overlap"@en ;
    dc:contributor "Matthew Perry" ;
    dc:creator "OGC GeoSPARQL 1.0 Standard Working Group" ;
    dc:date "2011-06-16"^^xsd:date ;
    dc:description """      Exists if the subject SpatialObject spatially overlaps the 
      object SpatialObject. DE-9IM: T*T***T**
    """@en ;
    rdfs:comment """      Exists if the subject SpatialObject spatially overlaps the 
      object SpatialObject. DE-9IM: T*T***T**
    """@en ;
    rdfs:domain geosparql:SpatialObject ;
    rdfs:isDefinedBy <http://www.opengis.net/ont/geosparql>,
        <http://www.opengis.net/spec/geosparql/1.0> ;
    rdfs:range geosparql:SpatialObject ;
    skos:definition """      Exists if the subject SpatialObject spatially overlaps the 
      object SpatialObject. DE-9IM: T*T***T**
    """@en ;
    skos:prefLabel "overlap"@en .

geosparql:isEmpty a owl:DatatypeProperty ;
    rdfs:label "isEmpty"@en ;
    dc:contributor "Matthew Perry" ;
    dc:creator "OGC GeoSPARQL 1.0 Standard Working Group" ;
    dc:date "2011-06-16"^^xsd:date ;
    dc:description """      (true) if this geometric object is the empty Geometry. If 
      true, then this geometric object represents the empty point 
      set for the coordinate space.
    """@en ;
    rdfs:comment """      (true) if this geometric object is the empty Geometry. If 
      true, then this geometric object represents the empty point 
      set for the coordinate space.
    """@en ;
    rdfs:domain geosparql:Geometry ;
    rdfs:isDefinedBy <http://www.opengis.net/ont/geosparql>,
        <http://www.opengis.net/spec/geosparql/1.0> ;
    rdfs:range xsd:boolean ;
    skos:definition """      (true) if this geometric object is the empty Geometry. If 
      true, then this geometric object represents the empty point 
      set for the coordinate space.
    """@en ;
    skos:prefLabel "isEmpty"@en .

geosparql:isSimple a owl:DatatypeProperty ;
    rdfs:label "isSimple"@en ;
    dc:contributor "Matthew Perry" ;
    dc:creator "OGC GeoSPARQL 1.0 Standard Working Group" ;
    dc:date "2011-06-16"^^xsd:date ;
    dc:description """      (true) if this geometric object has no anomalous geometric 
      points, such as self intersection or self tangency.
    """@en ;
    rdfs:comment """      (true) if this geometric object has no anomalous geometric 
      points, such as self intersection or self tangency.
    """@en ;
    rdfs:domain geosparql:Geometry ;
    rdfs:isDefinedBy <http://www.opengis.net/ont/geosparql>,
        <http://www.opengis.net/spec/geosparql/1.0> ;
    rdfs:range xsd:boolean ;
    skos:definition """      (true) if this geometric object has no anomalous geometric 
      points, such as self intersection or self tangency.
    """@en ;
    skos:prefLabel "isSimple"@en .

geosparql:rcc8dc a owl:ObjectProperty ;
    rdfs:label "disconnected"@en ;
    dc:contributor "Matthew Perry" ;
    dc:creator "OGC GeoSPARQL 1.0 Standard Working Group" ;
    dc:date "2011-06-16"^^xsd:date ;
    dc:description """      Exists if the subject SpatialObject is spatially disjoint
      from the object SpatialObject. DE-9IM: FFTFFTTTT
    """@en ;
    rdfs:comment """      Exists if the subject SpatialObject is spatially disjoint
      from the object SpatialObject. DE-9IM: FFTFFTTTT
    """@en ;
    rdfs:domain geosparql:SpatialObject ;
    rdfs:isDefinedBy <http://www.opengis.net/ont/geosparql>,
        <http://www.opengis.net/spec/geosparql/1.0> ;
    rdfs:range geosparql:SpatialObject ;
    skos:definition """      Exists if the subject SpatialObject is spatially disjoint
      from the object SpatialObject. DE-9IM: FFTFFTTTT
    """@en ;
    skos:prefLabel "disconnected"@en .

geosparql:rcc8ec a owl:ObjectProperty ;
    rdfs:label "externally connected"@en ;
    dc:contributor "Matthew Perry" ;
    dc:creator "OGC GeoSPARQL 1.0 Standard Working Group" ;
    dc:date "2011-06-16"^^xsd:date ;
    dc:description """      Exists if the subject SpatialObject spatially meets the 
      object SpatialObject. DE-9IM: FFTFTTTTT
    """@en ;
    rdfs:comment """      Exists if the subject SpatialObject spatially meets the 
      object SpatialObject. DE-9IM: FFTFTTTTT
    """@en ;
    rdfs:domain geosparql:SpatialObject ;
    rdfs:isDefinedBy <http://www.opengis.net/ont/geosparql>,
        <http://www.opengis.net/spec/geosparql/1.0> ;
    rdfs:range geosparql:SpatialObject ;
    skos:definition """      Exists if the subject SpatialObject spatially meets the 
      object SpatialObject. DE-9IM: FFTFTTTTT
    """@en ;
    skos:prefLabel "externally connected"@en .

geosparql:rcc8eq a owl:ObjectProperty ;
    rdfs:label "equals"@en ;
    dc:contributor "Matthew Perry" ;
    dc:creator "OGC GeoSPARQL 1.0 Standard Working Group" ;
    dc:date "2011-06-16"^^xsd:date ;
    dc:description """      Exists if the subject SpatialObject spatially equals the 
      object SpatialObject. DE-9IM: TFFFTFFFT
    """@en ;
    rdfs:comment """      Exists if the subject SpatialObject spatially equals the 
      object SpatialObject. DE-9IM: TFFFTFFFT
    """@en ;
    rdfs:domain geosparql:SpatialObject ;
    rdfs:isDefinedBy <http://www.opengis.net/ont/geosparql>,
        <http://www.opengis.net/spec/geosparql/1.0> ;
    rdfs:range geosparql:SpatialObject ;
    skos:definition """      Exists if the subject SpatialObject spatially equals the 
      object SpatialObject. DE-9IM: TFFFTFFFT
    """@en ;
    skos:prefLabel "equals"@en .

geosparql:rcc8ntpp a owl:ObjectProperty ;
    rdfs:label "non-tangential proper part"@en ;
    dc:contributor "Matthew Perry" ;
    dc:creator "OGC GeoSPARQL 1.0 Standard Working Group" ;
    dc:date "2011-06-16"^^xsd:date ;
    dc:description """      Exists if the subject SpatialObject is spatially inside 
      the object SpatialObject. DE-9IM: TFFTFFTTT
    """@en ;
    rdfs:comment """      Exists if the subject SpatialObject is spatially inside 
      the object SpatialObject. DE-9IM: TFFTFFTTT
    """@en ;
    rdfs:domain geosparql:SpatialObject ;
    rdfs:isDefinedBy <http://www.opengis.net/ont/geosparql>,
        <http://www.opengis.net/spec/geosparql/1.0> ;
    rdfs:range geosparql:SpatialObject ;
    skos:definition """      Exists if the subject SpatialObject is spatially inside 
      the object SpatialObject. DE-9IM: TFFTFFTTT
    """@en ;
    skos:prefLabel "non-tangential proper part"@en .

geosparql:rcc8ntppi a owl:ObjectProperty ;
    rdfs:label "non-tangential proper part inverse"@en ;
    dc:contributor "Matthew Perry" ;
    dc:creator "OGC GeoSPARQL 1.0 Standard Working Group" ;
    dc:date "2011-06-16"^^xsd:date ;
    dc:description """      Exists if the subject SpatialObject spatially contains the 
      object SpatialObject. DE-9IM: TTTFFTFFT
    """@en ;
    rdfs:comment """      Exists if the subject SpatialObject spatially contains the 
      object SpatialObject. DE-9IM: TTTFFTFFT
    """@en ;
    rdfs:domain geosparql:SpatialObject ;
    rdfs:isDefinedBy <http://www.opengis.net/ont/geosparql>,
        <http://www.opengis.net/spec/geosparql/1.0> ;
    rdfs:range geosparql:SpatialObject ;
    skos:definition """      Exists if the subject SpatialObject spatially contains the 
      object SpatialObject. DE-9IM: TTTFFTFFT
    """@en ;
    skos:prefLabel "non-tangential proper part inverse"@en .

geosparql:rcc8po a owl:ObjectProperty ;
    rdfs:label "partially overlapping"@en ;
    dc:contributor "Matthew Perry" ;
    dc:creator "OGC GeoSPARQL 1.0 Standard Working Group" ;
    dc:date "2011-06-16"^^xsd:date ;
    dc:description """      Exists if the subject SpatialObject spatially overlaps the 
      object SpatialObject. DE-9IM: TTTTTTTTT
    """@en ;
    rdfs:comment """      Exists if the subject SpatialObject spatially overlaps the 
      object SpatialObject. DE-9IM: TTTTTTTTT
    """@en ;
    rdfs:domain geosparql:SpatialObject ;
    rdfs:isDefinedBy <http://www.opengis.net/ont/geosparql>,
        <http://www.opengis.net/spec/geosparql/1.0> ;
    rdfs:range geosparql:SpatialObject ;
    skos:definition """      Exists if the subject SpatialObject spatially overlaps the 
      object SpatialObject. DE-9IM: TTTTTTTTT
    """@en ;
    skos:prefLabel "partially overlapping"@en .

geosparql:rcc8tpp a owl:ObjectProperty ;
    rdfs:label "tangential proper part"@en ;
    dc:contributor "Matthew Perry" ;
    dc:creator "OGC GeoSPARQL 1.0 Standard Working Group" ;
    dc:date "2011-06-16"^^xsd:date ;
    dc:description """      Exists if the subject SpatialObject is spatially covered 
      by the object SpatialObject. DE-9IM: TFFTTFTTT
    """@en ;
    rdfs:comment """      Exists if the subject SpatialObject is spatially covered 
      by the object SpatialObject. DE-9IM: TFFTTFTTT
    """@en ;
    rdfs:domain geosparql:SpatialObject ;
    rdfs:isDefinedBy <http://www.opengis.net/ont/geosparql>,
        <http://www.opengis.net/spec/geosparql/1.0> ;
    rdfs:range geosparql:SpatialObject ;
    skos:definition """      Exists if the subject SpatialObject is spatially covered 
      by the object SpatialObject. DE-9IM: TFFTTFTTT
    """@en ;
    skos:prefLabel "tangential proper part"@en .

geosparql:rcc8tppi a owl:ObjectProperty ;
    rdfs:label "tangential proper part inverse"@en ;
    dc:contributor "Matthew Perry" ;
    dc:creator "OGC GeoSPARQL 1.0 Standard Working Group" ;
    dc:date "2011-06-16"^^xsd:date ;
    dc:description """      Exists if the subject SpatialObject spatially covers the 
      object SpatialObject. DE-9IM: TTTFTTFFT
    """@en ;
    rdfs:comment """      Exists if the subject SpatialObject spatially covers the 
      object SpatialObject. DE-9IM: TTTFTTFFT
    """@en ;
    rdfs:domain geosparql:SpatialObject ;
    rdfs:isDefinedBy <http://www.opengis.net/ont/geosparql>,
        <http://www.opengis.net/spec/geosparql/1.0> ;
    rdfs:range geosparql:SpatialObject ;
    skos:definition """      Exists if the subject SpatialObject spatially covers the 
      object SpatialObject. DE-9IM: TTTFTTFFT
    """@en ;
    skos:prefLabel "tangential proper part inverse"@en .

geosparql:sfContains a owl:ObjectProperty ;
    rdfs:label "contains"@en ;
    dc:contributor "Matthew Perry" ;
    dc:creator "OGC GeoSPARQL 1.0 Standard Working Group" ;
    dc:date "2011-06-16"^^xsd:date ;
    dc:description """      Exists if the subject SpatialObject spatially contains the 
      object SpatialObject. DE-9IM: T*****FF*
    """@en ;
    rdfs:comment """      Exists if the subject SpatialObject spatially contains the 
      object SpatialObject. DE-9IM: T*****FF*
    """@en ;
    rdfs:domain geosparql:SpatialObject ;
    rdfs:isDefinedBy <http://www.opengis.net/ont/geosparql>,
        <http://www.opengis.net/spec/geosparql/1.0> ;
    rdfs:range geosparql:SpatialObject ;
    skos:definition """      Exists if the subject SpatialObject spatially contains the 
      object SpatialObject. DE-9IM: T*****FF*
    """@en ;
    skos:prefLabel "contains"@en .

geosparql:sfCrosses a owl:ObjectProperty ;
    rdfs:label "crosses"@en ;
    dc:contributor "Matthew Perry" ;
    dc:creator "OGC GeoSPARQL 1.0 Standard Working Group" ;
    dc:date "2011-06-16"^^xsd:date ;
    dc:description """      Exists if the subject SpatialObject spatially crosses the 
      object SpatialObject. DE-9IM: T*T******
    """@en ;
    rdfs:comment """      Exists if the subject SpatialObject spatially crosses the 
      object SpatialObject. DE-9IM: T*T******
    """@en ;
    rdfs:domain geosparql:SpatialObject ;
    rdfs:isDefinedBy <http://www.opengis.net/ont/geosparql>,
        <http://www.opengis.net/spec/geosparql/1.0> ;
    rdfs:range geosparql:SpatialObject ;
    skos:definition """      Exists if the subject SpatialObject spatially crosses the 
      object SpatialObject. DE-9IM: T*T******
    """@en ;
    skos:prefLabel "crosses"@en .

geosparql:sfDisjoint a owl:ObjectProperty ;
    rdfs:label "disjoint"@en ;
    dc:contributor "Matthew Perry" ;
    dc:creator "OGC GeoSPARQL 1.0 Standard Working Group" ;
    dc:date "2011-06-16"^^xsd:date ;
    dc:description """      Exists if the subject SpatialObject is spatially disjoint 
      from the object SpatialObject. DE-9IM: FF*FF****
    """@en ;
    rdfs:comment """      Exists if the subject SpatialObject is spatially disjoint 
      from the object SpatialObject. DE-9IM: FF*FF****
    """@en ;
    rdfs:domain geosparql:SpatialObject ;
    rdfs:isDefinedBy <http://www.opengis.net/ont/geosparql>,
        <http://www.opengis.net/spec/geosparql/1.0> ;
    rdfs:range geosparql:SpatialObject ;
    skos:definition """      Exists if the subject SpatialObject is spatially disjoint 
      from the object SpatialObject. DE-9IM: FF*FF****
    """@en ;
    skos:prefLabel "disjoint"@en .

geosparql:sfEquals a owl:ObjectProperty ;
    rdfs:label "equals"@en ;
    dc:contributor "Matthew Perry" ;
    dc:creator "OGC GeoSPARQL 1.0 Standard Working Group" ;
    dc:date "2011-06-16"^^xsd:date ;
    dc:description """      Exists if the subject SpatialObject spatially equals the 
      object SpatialObject. DE-9IM: TFFFTFFFT
    """@en ;
    rdfs:comment """      Exists if the subject SpatialObject spatially equals the 
      object SpatialObject. DE-9IM: TFFFTFFFT
    """@en ;
    rdfs:domain geosparql:SpatialObject ;
    rdfs:isDefinedBy <http://www.opengis.net/ont/geosparql>,
        <http://www.opengis.net/spec/geosparql/1.0> ;
    rdfs:range geosparql:SpatialObject ;
    skos:definition """      Exists if the subject SpatialObject spatially equals the 
      object SpatialObject. DE-9IM: TFFFTFFFT
    """@en ;
    skos:prefLabel "equals"@en .

geosparql:sfIntersects a owl:ObjectProperty ;
    rdfs:label "intersects"@en ;
    dc:contributor "Matthew Perry" ;
    dc:creator "OGC GeoSPARQL 1.0 Standard Working Group" ;
    dc:date "2011-06-16"^^xsd:date ;
    dc:description """      Exists if the subject SpatialObject is not spatially disjoint 
      from the object SpatialObject.
      DE-9IM: T******** ^ *T******* ^ ***T***** ^ ****T**** 
    """@en ;
    rdfs:comment """      Exists if the subject SpatialObject is not spatially disjoint 
      from the object SpatialObject.
      DE-9IM: T******** ^ *T******* ^ ***T***** ^ ****T**** 
    """@en ;
    rdfs:domain geosparql:SpatialObject ;
    rdfs:isDefinedBy <http://www.opengis.net/ont/geosparql>,
        <http://www.opengis.net/spec/geosparql/1.0> ;
    rdfs:range geosparql:SpatialObject ;
    skos:definition """      Exists if the subject SpatialObject is not spatially disjoint 
      from the object SpatialObject.
      DE-9IM: T******** ^ *T******* ^ ***T***** ^ ****T**** 
    """@en ;
    skos:prefLabel "intersects"@en .

geosparql:sfOverlaps a owl:ObjectProperty ;
    rdfs:label "overlaps"@en ;
    dc:contributor "Matthew Perry" ;
    dc:creator "OGC GeoSPARQL 1.0 Standard Working Group" ;
    dc:date "2011-06-16"^^xsd:date ;
    dc:description """      Exists if the subject SpatialObject spatially overlaps the 
      object SpatialObject. DE-9IM: T*T***T** 
    """@en ;
    rdfs:comment """      Exists if the subject SpatialObject spatially overlaps the 
      object SpatialObject. DE-9IM: T*T***T** 
    """@en ;
    rdfs:domain geosparql:SpatialObject ;
    rdfs:isDefinedBy <http://www.opengis.net/ont/geosparql>,
        <http://www.opengis.net/spec/geosparql/1.0> ;
    rdfs:range geosparql:SpatialObject ;
    skos:definition """      Exists if the subject SpatialObject spatially overlaps the 
      object SpatialObject. DE-9IM: T*T***T** 
    """@en ;
    skos:prefLabel "overlaps"@en .

geosparql:sfTouches a owl:ObjectProperty ;
    rdfs:label "touches"@en ;
    dc:contributor "Matthew Perry" ;
    dc:creator "OGC GeoSPARQL 1.0 Standard Working Group" ;
    dc:date "2011-06-16"^^xsd:date ;
    dc:description """      Exists if the subject SpatialObject spatially touches the 
      object SpatialObject.
      DE-9IM: FT******* ^ F**T***** ^ F***T****
    """@en ;
    rdfs:comment """      Exists if the subject SpatialObject spatially touches the 
      object SpatialObject.
      DE-9IM: FT******* ^ F**T***** ^ F***T****
    """@en ;
    rdfs:domain geosparql:SpatialObject ;
    rdfs:isDefinedBy <http://www.opengis.net/ont/geosparql>,
        <http://www.opengis.net/spec/geosparql/1.0> ;
    rdfs:range geosparql:SpatialObject ;
    skos:definition """      Exists if the subject SpatialObject spatially touches the 
      object SpatialObject.
      DE-9IM: FT******* ^ F**T***** ^ F***T****
    """@en ;
    skos:prefLabel "touches"@en .

geosparql:sfWithin a owl:ObjectProperty ;
    rdfs:label "within"@en ;
    dc:contributor "Matthew Perry" ;
    dc:creator "OGC GeoSPARQL 1.0 Standard Working Group" ;
    dc:date "2011-06-16"^^xsd:date ;
    dc:description """      Exists if the subject SpatialObject is spatially within the 
      object SpatialObject. DE-9IM: T*F**F***
    """@en ;
    rdfs:comment """      Exists if the subject SpatialObject is spatially within the 
      object SpatialObject. DE-9IM: T*F**F***
    """@en ;
    rdfs:domain geosparql:SpatialObject ;
    rdfs:isDefinedBy <http://www.opengis.net/ont/geosparql>,
        <http://www.opengis.net/spec/geosparql/1.0> ;
    rdfs:range geosparql:SpatialObject ;
    skos:definition """      Exists if the subject SpatialObject is spatially within the 
      object SpatialObject. DE-9IM: T*F**F***
    """@en ;
    skos:prefLabel "within"@en .

geosparql:spatialDimension a owl:DatatypeProperty ;
    rdfs:label "spatialDimension"@en ;
    dc:contributor "Matthew Perry" ;
    dc:creator "OGC GeoSPARQL 1.0 Standard Working Group" ;
    dc:date "2011-06-16"^^xsd:date ;
    dc:description """      The number of measurements or axes needed to describe the spatial position of 
      this geometry in a coordinate system.
    """@en ;
    rdfs:comment """      The number of measurements or axes needed to describe the spatial position of 
      this geometry in a coordinate system.
    """@en ;
    rdfs:domain geosparql:Geometry ;
    rdfs:isDefinedBy <http://www.opengis.net/ont/geosparql>,
        <http://www.opengis.net/spec/geosparql/1.0> ;
    rdfs:range xsd:integer ;
    skos:definition """      The number of measurements or axes needed to describe the spatial position of 
      this geometry in a coordinate system.
    """@en ;
    skos:prefLabel "spatialDimension"@en .

rdf:HTML a rdfs:Datatype ;
    rdfs:label "HTML" ;
    rdfs:comment "The datatype of RDF literals storing fragments of HTML content" ;
    rdfs:isDefinedBy rdf: ;
    rdfs:seeAlso rdf11-concepts:section-html ;
    rdfs:subClassOf rdfs:Literal .

rdf:PlainLiteral a rdfs:Datatype ;
    rdfs:label "PlainLiteral" ;
    rdfs:comment "The class of plain (i.e. untyped) literal values, as used in RIF and OWL 2" ;
    rdfs:isDefinedBy rdf: ;
    rdfs:seeAlso <http://www.w3.org/TR/rdf-plain-literal/> ;
    rdfs:subClassOf rdfs:Literal .

rdf:XMLLiteral a rdfs:Datatype ;
    rdfs:label "XMLLiteral" ;
    rdfs:comment "The datatype of XML literal values." ;
    rdfs:isDefinedBy rdf: ;
    rdfs:subClassOf rdfs:Literal .

rdf:first a rdf:Property ;
    rdfs:label "first" ;
    rdfs:comment "The first item in the subject RDF list." ;
    rdfs:domain rdf:List ;
    rdfs:isDefinedBy rdf: ;
    rdfs:range rdfs:Resource .

rdf:langString a rdfs:Datatype ;
    rdfs:label "langString" ;
    rdfs:comment "The datatype of language-tagged string values" ;
    rdfs:isDefinedBy rdf: ;
    rdfs:seeAlso rdf11-concepts:section-Graph-Literal ;
    rdfs:subClassOf rdfs:Literal .

rdf:object a rdf:Property ;
    rdfs:label "object" ;
    rdfs:comment "The object of the subject RDF statement." ;
    rdfs:domain rdf:Statement ;
    rdfs:isDefinedBy rdf: ;
    rdfs:range rdfs:Resource .

rdf:predicate a rdf:Property ;
    rdfs:label "predicate" ;
    rdfs:comment "The predicate of the subject RDF statement." ;
    rdfs:domain rdf:Statement ;
    rdfs:isDefinedBy rdf: ;
    rdfs:range rdfs:Resource .

rdf:rest a rdf:Property ;
    rdfs:label "rest" ;
    rdfs:comment "The rest of the subject RDF list after the first item." ;
    rdfs:domain rdf:List ;
    rdfs:isDefinedBy rdf: ;
    rdfs:range rdf:List .

rdf:subject a rdf:Property ;
    rdfs:label "subject" ;
    rdfs:comment "The subject of the subject RDF statement." ;
    rdfs:domain rdf:Statement ;
    rdfs:isDefinedBy rdf: ;
    rdfs:range rdfs:Resource .

rdf:type a rdf:Property ;
    rdfs:label "type" ;
    rdfs:comment "The subject is an instance of a class." ;
    rdfs:domain rdfs:Resource ;
    rdfs:isDefinedBy rdf: ;
    rdfs:range rdfs:Class .

rdfs:comment a rdf:Property ;
    rdfs:label "comment" ;
    rdfs:comment "A description of the subject resource." ;
    rdfs:domain rdfs:Resource ;
    rdfs:isDefinedBy rdfs: ;
    rdfs:range rdfs:Literal .

rdfs:domain a rdf:Property ;
    rdfs:label "domain" ;
    rdfs:comment "A domain of the subject property." ;
    rdfs:domain rdf:Property ;
    rdfs:isDefinedBy rdfs: ;
    rdfs:range rdfs:Class .

rdfs:isDefinedBy a rdf:Property ;
    rdfs:label "isDefinedBy" ;
    rdfs:comment "The defininition of the subject resource." ;
    rdfs:domain rdfs:Resource ;
    rdfs:isDefinedBy rdfs: ;
    rdfs:range rdfs:Resource ;
    rdfs:subPropertyOf rdfs:seeAlso .

rdfs:member a rdf:Property ;
    rdfs:label "member" ;
    rdfs:comment "A member of the subject resource." ;
    rdfs:domain rdfs:Resource ;
    rdfs:isDefinedBy rdfs: ;
    rdfs:range rdfs:Resource .

rdfs:range a rdf:Property ;
    rdfs:label "range" ;
    rdfs:comment "A range of the subject property." ;
    rdfs:domain rdf:Property ;
    rdfs:isDefinedBy rdfs: ;
    rdfs:range rdfs:Class .

rdfs:subClassOf a rdf:Property ;
    rdfs:label "subClassOf" ;
    rdfs:comment "The subject is a subclass of a class." ;
    rdfs:domain rdfs:Class ;
    rdfs:isDefinedBy rdfs: ;
    rdfs:range rdfs:Class .

rdfs:subPropertyOf a rdf:Property ;
    rdfs:label "subPropertyOf" ;
    rdfs:comment "The subject is a subproperty of a property." ;
    rdfs:domain rdf:Property ;
    rdfs:isDefinedBy rdfs: ;
    rdfs:range rdf:Property .

owl:Nothing a owl:Class ;
    rdfs:label "Nothing" ;
    rdfs:comment "This is the empty class." ;
    rdfs:isDefinedBy owl: ;
    rdfs:subClassOf owl:Thing .

owl:allValuesFrom a rdf:Property ;
    rdfs:label "allValuesFrom" ;
    rdfs:comment "The property that determines the class that a universal property restriction refers to." ;
    rdfs:domain owl:Restriction ;
    rdfs:isDefinedBy owl: ;
    rdfs:range rdfs:Class .

owl:annotatedProperty a rdf:Property ;
    rdfs:label "annotatedProperty" ;
    rdfs:comment "The property that determines the predicate of an annotated axiom or annotated annotation." ;
    rdfs:domain rdfs:Resource ;
    rdfs:isDefinedBy owl: ;
    rdfs:range rdfs:Resource .

owl:annotatedSource a rdf:Property ;
    rdfs:label "annotatedSource" ;
    rdfs:comment "The property that determines the subject of an annotated axiom or annotated annotation." ;
    rdfs:domain rdfs:Resource ;
    rdfs:isDefinedBy owl: ;
    rdfs:range rdfs:Resource .

owl:annotatedTarget a rdf:Property ;
    rdfs:label "annotatedTarget" ;
    rdfs:comment "The property that determines the object of an annotated axiom or annotated annotation." ;
    rdfs:domain rdfs:Resource ;
    rdfs:isDefinedBy owl: ;
    rdfs:range rdfs:Resource .

owl:assertionProperty a rdf:Property ;
    rdfs:label "assertionProperty" ;
    rdfs:comment "The property that determines the predicate of a negative property assertion." ;
    rdfs:domain owl:NegativePropertyAssertion ;
    rdfs:isDefinedBy owl: ;
    rdfs:range rdf:Property .

owl:backwardCompatibleWith a owl:AnnotationProperty,
        owl:OntologyProperty ;
    rdfs:label "backwardCompatibleWith" ;
    rdfs:comment "The annotation property that indicates that a given ontology is backward compatible with another ontology." ;
    rdfs:domain owl:Ontology ;
    rdfs:isDefinedBy owl: ;
    rdfs:range owl:Ontology .

owl:bottomDataProperty a owl:DatatypeProperty ;
    rdfs:label "bottomDataProperty" ;
    rdfs:comment "The data property that does not relate any individual to any data value." ;
    rdfs:domain owl:Thing ;
    rdfs:isDefinedBy owl: ;
    rdfs:range rdfs:Literal .

owl:bottomObjectProperty a owl:ObjectProperty ;
    rdfs:label "bottomObjectProperty" ;
    rdfs:comment "The object property that does not relate any two individuals." ;
    rdfs:domain owl:Thing ;
    rdfs:isDefinedBy owl: ;
    rdfs:range owl:Thing .

owl:cardinality a rdf:Property ;
    rdfs:label "cardinality" ;
    rdfs:comment "The property that determines the cardinality of an exact cardinality restriction." ;
    rdfs:domain owl:Restriction ;
    rdfs:isDefinedBy owl: ;
    rdfs:range xsd:nonNegativeInteger .

owl:complementOf a rdf:Property ;
    rdfs:label "complementOf" ;
    rdfs:comment "The property that determines that a given class is the complement of another class." ;
    rdfs:domain owl:Class ;
    rdfs:isDefinedBy owl: ;
    rdfs:range owl:Class .

owl:datatypeComplementOf a rdf:Property ;
    rdfs:label "datatypeComplementOf" ;
    rdfs:comment "The property that determines that a given data range is the complement of another data range with respect to the data domain." ;
    rdfs:domain rdfs:Datatype ;
    rdfs:isDefinedBy owl: ;
    rdfs:range rdfs:Datatype .

owl:deprecated a owl:AnnotationProperty ;
    rdfs:label "deprecated" ;
    rdfs:comment "The annotation property that indicates that a given entity has been deprecated." ;
    rdfs:domain rdfs:Resource ;
    rdfs:isDefinedBy owl: ;
    rdfs:range rdfs:Resource .

owl:differentFrom a rdf:Property ;
    rdfs:label "differentFrom" ;
    rdfs:comment "The property that determines that two given individuals are different." ;
    rdfs:domain owl:Thing ;
    rdfs:isDefinedBy owl: ;
    rdfs:range owl:Thing .

owl:disjointUnionOf a rdf:Property ;
    rdfs:label "disjointUnionOf" ;
    rdfs:comment "The property that determines that a given class is equivalent to the disjoint union of a collection of other classes." ;
    rdfs:domain owl:Class ;
    rdfs:isDefinedBy owl: ;
    rdfs:range rdf:List .

owl:disjointWith a rdf:Property ;
    rdfs:label "disjointWith" ;
    rdfs:comment "The property that determines that two given classes are disjoint." ;
    rdfs:domain owl:Class ;
    rdfs:isDefinedBy owl: ;
    rdfs:range owl:Class .

owl:distinctMembers a rdf:Property ;
    rdfs:label "distinctMembers" ;
    rdfs:comment "The property that determines the collection of pairwise different individuals in a owl:AllDifferent axiom." ;
    rdfs:domain owl:AllDifferent ;
    rdfs:isDefinedBy owl: ;
    rdfs:range rdf:List .

owl:equivalentClass a rdf:Property ;
    rdfs:label "equivalentClass" ;
    rdfs:comment "The property that determines that two given classes are equivalent, and that is used to specify datatype definitions." ;
    rdfs:domain rdfs:Class ;
    rdfs:isDefinedBy owl: ;
    rdfs:range rdfs:Class .

owl:equivalentProperty a rdf:Property ;
    rdfs:label "equivalentProperty" ;
    rdfs:comment "The property that determines that two given properties are equivalent." ;
    rdfs:domain rdf:Property ;
    rdfs:isDefinedBy owl: ;
    rdfs:range rdf:Property .

owl:hasKey a rdf:Property ;
    rdfs:label "hasKey" ;
    rdfs:comment "The property that determines the collection of properties that jointly build a key." ;
    rdfs:domain owl:Class ;
    rdfs:isDefinedBy owl: ;
    rdfs:range rdf:List .

owl:hasSelf a rdf:Property ;
    rdfs:label "hasSelf" ;
    rdfs:comment "The property that determines the property that a self restriction refers to." ;
    rdfs:domain owl:Restriction ;
    rdfs:isDefinedBy owl: ;
    rdfs:range rdfs:Resource .

owl:hasValue a rdf:Property ;
    rdfs:label "hasValue" ;
    rdfs:comment "The property that determines the individual that a has-value restriction refers to." ;
    rdfs:domain owl:Restriction ;
    rdfs:isDefinedBy owl: ;
    rdfs:range rdfs:Resource .

owl:imports a owl:OntologyProperty ;
    rdfs:label "imports" ;
    rdfs:comment "The property that is used for importing other ontologies into a given ontology." ;
    rdfs:domain owl:Ontology ;
    rdfs:isDefinedBy owl: ;
    rdfs:range owl:Ontology .

owl:incompatibleWith a owl:AnnotationProperty,
        owl:OntologyProperty ;
    rdfs:label "incompatibleWith" ;
    rdfs:comment "The annotation property that indicates that a given ontology is incompatible with another ontology." ;
    rdfs:domain owl:Ontology ;
    rdfs:isDefinedBy owl: ;
    rdfs:range owl:Ontology .

owl:intersectionOf a rdf:Property ;
    rdfs:label "intersectionOf" ;
    rdfs:comment "The property that determines the collection of classes or data ranges that build an intersection." ;
    rdfs:domain rdfs:Class ;
    rdfs:isDefinedBy owl: ;
    rdfs:range rdf:List .

owl:inverseOf a rdf:Property ;
    rdfs:label "inverseOf" ;
    rdfs:comment "The property that determines that two given properties are inverse." ;
    rdfs:domain owl:ObjectProperty ;
    rdfs:isDefinedBy owl: ;
    rdfs:range owl:ObjectProperty .

owl:maxCardinality a rdf:Property ;
    rdfs:label "maxCardinality" ;
    rdfs:comment "The property that determines the cardinality of a maximum cardinality restriction." ;
    rdfs:domain owl:Restriction ;
    rdfs:isDefinedBy owl: ;
    rdfs:range xsd:nonNegativeInteger .

owl:maxQualifiedCardinality a rdf:Property ;
    rdfs:label "maxQualifiedCardinality" ;
    rdfs:comment "The property that determines the cardinality of a maximum qualified cardinality restriction." ;
    rdfs:domain owl:Restriction ;
    rdfs:isDefinedBy owl: ;
    rdfs:range xsd:nonNegativeInteger .

owl:members a rdf:Property ;
    rdfs:label "members" ;
    rdfs:comment "The property that determines the collection of members in either a owl:AllDifferent, owl:AllDisjointClasses or owl:AllDisjointProperties axiom." ;
    rdfs:domain rdfs:Resource ;
    rdfs:isDefinedBy owl: ;
    rdfs:range rdf:List .

owl:minCardinality a rdf:Property ;
    rdfs:label "minCardinality" ;
    rdfs:comment "The property that determines the cardinality of a minimum cardinality restriction." ;
    rdfs:domain owl:Restriction ;
    rdfs:isDefinedBy owl: ;
    rdfs:range xsd:nonNegativeInteger .

owl:minQualifiedCardinality a rdf:Property ;
    rdfs:label "minQualifiedCardinality" ;
    rdfs:comment "The property that determines the cardinality of a minimum qualified cardinality restriction." ;
    rdfs:domain owl:Restriction ;
    rdfs:isDefinedBy owl: ;
    rdfs:range xsd:nonNegativeInteger .

owl:onClass a rdf:Property ;
    rdfs:label "onClass" ;
    rdfs:comment "The property that determines the class that a qualified object cardinality restriction refers to." ;
    rdfs:domain owl:Restriction ;
    rdfs:isDefinedBy owl: ;
    rdfs:range owl:Class .

owl:onDataRange a rdf:Property ;
    rdfs:label "onDataRange" ;
    rdfs:comment "The property that determines the data range that a qualified data cardinality restriction refers to." ;
    rdfs:domain owl:Restriction ;
    rdfs:isDefinedBy owl: ;
    rdfs:range rdfs:Datatype .

owl:onDatatype a rdf:Property ;
    rdfs:label "onDatatype" ;
    rdfs:comment "The property that determines the datatype that a datatype restriction refers to." ;
    rdfs:domain rdfs:Datatype ;
    rdfs:isDefinedBy owl: ;
    rdfs:range rdfs:Datatype .

owl:onProperties a rdf:Property ;
    rdfs:label "onProperties" ;
    rdfs:comment "The property that determines the n-tuple of properties that a property restriction on an n-ary data range refers to." ;
    rdfs:domain owl:Restriction ;
    rdfs:isDefinedBy owl: ;
    rdfs:range rdf:List .

owl:onProperty a rdf:Property ;
    rdfs:label "onProperty" ;
    rdfs:comment "The property that determines the property that a property restriction refers to." ;
    rdfs:domain owl:Restriction ;
    rdfs:isDefinedBy owl: ;
    rdfs:range rdf:Property .

owl:oneOf a rdf:Property ;
    rdfs:label "oneOf" ;
    rdfs:comment "The property that determines the collection of individuals or data values that build an enumeration." ;
    rdfs:domain rdfs:Class ;
    rdfs:isDefinedBy owl: ;
    rdfs:range rdf:List .

owl:priorVersion a owl:AnnotationProperty,
        owl:OntologyProperty ;
    rdfs:label "priorVersion" ;
    rdfs:comment "The annotation property that indicates the predecessor ontology of a given ontology." ;
    rdfs:domain owl:Ontology ;
    rdfs:isDefinedBy owl: ;
    rdfs:range owl:Ontology .

owl:propertyChainAxiom a rdf:Property ;
    rdfs:label "propertyChainAxiom" ;
    rdfs:comment "The property that determines the n-tuple of properties that build a sub property chain of a given property." ;
    rdfs:domain owl:ObjectProperty ;
    rdfs:isDefinedBy owl: ;
    rdfs:range rdf:List .

owl:propertyDisjointWith a rdf:Property ;
    rdfs:label "propertyDisjointWith" ;
    rdfs:comment "The property that determines that two given properties are disjoint." ;
    rdfs:domain rdf:Property ;
    rdfs:isDefinedBy owl: ;
    rdfs:range rdf:Property .

owl:qualifiedCardinality a rdf:Property ;
    rdfs:label "qualifiedCardinality" ;
    rdfs:comment "The property that determines the cardinality of an exact qualified cardinality restriction." ;
    rdfs:domain owl:Restriction ;
    rdfs:isDefinedBy owl: ;
    rdfs:range xsd:nonNegativeInteger .

owl:sameAs a rdf:Property ;
    rdfs:label "sameAs" ;
    rdfs:comment "The property that determines that two given individuals are equal." ;
    rdfs:domain owl:Thing ;
    rdfs:isDefinedBy owl: ;
    rdfs:range owl:Thing .

owl:someValuesFrom a rdf:Property ;
    rdfs:label "someValuesFrom" ;
    rdfs:comment "The property that determines the class that an existential property restriction refers to." ;
    rdfs:domain owl:Restriction ;
    rdfs:isDefinedBy owl: ;
    rdfs:range rdfs:Class .

owl:sourceIndividual a rdf:Property ;
    rdfs:label "sourceIndividual" ;
    rdfs:comment "The property that determines the subject of a negative property assertion." ;
    rdfs:domain owl:NegativePropertyAssertion ;
    rdfs:isDefinedBy owl: ;
    rdfs:range owl:Thing .

owl:targetIndividual a rdf:Property ;
    rdfs:label "targetIndividual" ;
    rdfs:comment "The property that determines the object of a negative object property assertion." ;
    rdfs:domain owl:NegativePropertyAssertion ;
    rdfs:isDefinedBy owl: ;
    rdfs:range owl:Thing .

owl:targetValue a rdf:Property ;
    rdfs:label "targetValue" ;
    rdfs:comment "The property that determines the value of a negative data property assertion." ;
    rdfs:domain owl:NegativePropertyAssertion ;
    rdfs:isDefinedBy owl: ;
    rdfs:range rdfs:Literal .

owl:topDataProperty a owl:DatatypeProperty ;
    rdfs:label "topDataProperty" ;
    rdfs:comment "The data property that relates every individual to every data value." ;
    rdfs:domain owl:Thing ;
    rdfs:isDefinedBy owl: ;
    rdfs:range rdfs:Literal .

owl:topObjectProperty a owl:ObjectProperty ;
    rdfs:label "topObjectProperty" ;
    rdfs:comment "The object property that relates every two individuals." ;
    rdfs:domain owl:Thing ;
    rdfs:isDefinedBy owl: ;
    rdfs:range owl:Thing .

owl:unionOf a rdf:Property ;
    rdfs:label "unionOf" ;
    rdfs:comment "The property that determines the collection of classes or data ranges that build a union." ;
    rdfs:domain rdfs:Class ;
    rdfs:isDefinedBy owl: ;
    rdfs:range rdf:List .

owl:versionIRI a owl:OntologyProperty ;
    rdfs:label "versionIRI" ;
    rdfs:comment "The property that identifies the version IRI of an ontology." ;
    rdfs:domain owl:Ontology ;
    rdfs:isDefinedBy owl: ;
    rdfs:range owl:Ontology .

owl:versionInfo a owl:AnnotationProperty ;
    rdfs:label "versionInfo" ;
    rdfs:comment "The annotation property that provides version information for an ontology or another OWL construct." ;
    rdfs:domain rdfs:Resource ;
    rdfs:isDefinedBy owl: ;
    rdfs:range rdfs:Resource .

owl:withRestrictions a rdf:Property ;
    rdfs:label "withRestrictions" ;
    rdfs:comment "The property that determines the collection of facet-value pairs that define a datatype restriction." ;
    rdfs:domain rdfs:Datatype ;
    rdfs:isDefinedBy owl: ;
    rdfs:range rdf:List .

wgs84: rdfs:label "geo" ;
    dc:date "$Date: 2009/04/20 15:00:30 $" ;
    dc:description """A vocabulary for representing latitude, longitude and 
 altitude information in the WGS84 geodetic reference datum. 
 Version $Id: wgs84_pos.rdf,v 1.22 2009/04/20 15:00:30 timbl Exp $. See http://www.w3.org/2003/01/geo/ for more details.""" ;
    dc:title "WGS84 Geo Positioning: an RDF vocabulary" ;
    rdfs:comment """Recent changes to this namespace:
$Log: wgs84_pos.rdf,v $
Revision 1.22  2009/04/20 15:00:30  timbl
Remove the time bits which have been deal with elsewhere eg in iCal.

Revision 1.21  2009/04/20 12:52:47  timbl
try again

Revision 1.20  2009/04/20 12:42:11  timbl
Add Event (edited ages ago and never checked in), and location (following discussion http://chatlogs.planetrdf.com/swig/2009-04-20#T12-36-09)

Revision 1.19  2009/04/20 12:36:31  timbl
Add Event (edited ages ago and never checked in), and location (following discussion http://chatlogs.planetrdf.com/swig/2009-04-20#T12-36-09)

Revision 1.18  2006/02/01 22:01:04  danbri
Clarified that lat and long are decimal degrees, and that alt is decimal metres about local reference ellipsoid

Revision 1.17  2004/02/06 17:38:12  danbri
Fixed a bad commit screwup

Revision 1.15  2003/04/19 11:24:08  danbri
Fixed the typo even more.

Revision 1.14  2003/04/19 11:16:56  danbri
fixed a typo

Revision 1.13  2003/02/19 22:27:27  connolly
relaxed domain constraints on lat/long/alt from Point to SpatialThing

Revision 1.12  2003/01/12 01:41:41  danbri
Trying local copy of XSLT doc.

Revision 1.11  2003/01/12 01:20:18  danbri
added a link to morten's xslt rdfs viewer.

Revision 1.10  2003/01/11 18:56:49  danbri
Removed datatype range from lat and long properties, since they would
have required each occurance of the property to mention the datatype.

Revision 1.9  2003/01/11 11:41:31  danbri
Another typo; repaired rdfs:Property to rdf:Property x4

Revision 1.8  2003/01/11 11:05:02  danbri
Added an rdfs:range for each lat/long/alt property,
http://www.w3.org/2001/XMLSchema#float

Revision 1.7  2003/01/10 20:25:16  danbri
Longer rdfs:comment for Point, trying to be Earth-centric and neutral about
coordinate system(s) at the same time. Feedback welcomed.

Revision 1.6  2003/01/10 20:18:30  danbri
Added CVS log comments into the RDF/XML as an rdfs:comment property of the
vocabulary. Note that this is not common practice (but seems both harmless
and potentially useful).


revision 1.5
date: 2003/01/10 20:14:31;  author: danbri;  state: Exp;  lines: +16 -5
Updated schema:
Added a dc:date, added url for more info. Changed the rdfs:label of the
namespace from gp to geo. Added a class Point, set as the rdfs:domain of
each property. Added XML comment on the lat_long property suggesting that
we might not need it (based on #rdfig commentary from implementors).

revision 1.4
date: 2003/01/10 20:01:07;  author: danbri;  state: Exp;  lines: +6 -5
Fixed typo; several rdfs:about attributes are now rdf:about. Thanks to MortenF in
#rdfig for catching this error.

revision 1.3
date: 2003/01/10 11:59:03;  author: danbri;  state: Exp;  lines: +4 -3
fixed buglet in vocab, added more wgs links

revision 1.2
date: 2003/01/10 11:01:11;  author: danbri;  state: Exp;  lines: +4 -4
Removed alt from the as-a-flat-string property, and switched from
space separated to comma separated.

revision 1.1
date: 2003/01/10 10:53:23;  author: danbri;  state: Exp;
basic geo vocab
""" .

wgs84:alt a rdf:Property ;
    rdfs:label "altitude" ;
    rdfs:comment """The WGS84 altitude of a SpatialThing (decimal meters 
above the local reference ellipsoid).""" ;
    rdfs:domain wgs84:SpatialThing .

wgs84:lat_long a rdf:Property ;
    rdfs:label "lat/long" ;
    rdfs:comment "A comma-separated representation of a latitude, longitude coordinate." .

wgs84:location a rdf:Property ;
    rdfs:label "location" ;
    rdfs:comment """The relation between something and the point, 
 or other geometrical thing in space, where it is.  For example, the realtionship between
 a radio tower and a Point with a given lat and long.
 Or a relationship between a park and its outline as a closed arc of points, or a road and
 its location as a arc (a sequence of points).
 Clearly in practice there will be limit to the accuracy of any such statement, but one would expect
 an accuracy appropriate for the size of the object and uses such as mapping .
 """ ;
    rdfs:range wgs84:SpatialThing ;
    rdfs:subPropertyOf foaf:based_near .

<http://www.w3.org/2003/06/sw-vocab-status/ns> a owl:Ontology ;
    dc:contributor "Pierre-Yves Vandenbussche" ;
    dc:creator "Dan Brickley",
        "Leigh Dodds",
        "Libby Miller" ;
    dc:description "An RDF vocabulary for relating SW vocabulary terms to their status." ;
    dc:issued "2003-06-01"^^xsd:date ;
    dc:modified "2011-12-12"^^xsd:date ;
    dc:title "SemWeb Vocab Status ontology" ;
    vann:preferredNamespacePrefix "vs" ;
    vann:preferredNamespaceUri "http://www.w3.org/2003/06/sw-vocab-status/ns#" ;
    rdfs:comment "This vocabulary was created in the FOAF project, based on experience with FOAF, Dublin Core and other early RDF vocabularies. Deployment experience shows that changing namespace URIs is expensive and unrewarding, so this vocabulary provides terms to support in-place evolution of structured data vocabularies. By indicating status at the level of terms rather than vocabularies, dictionary-style, fine grained improvements become easier. Different organizations and parties can agree or disagree on the status of a vocabulary term; however the status published alongside the term may deserve special attention. Future work could include patterns for citing announcements and decisions, or using SKOS to decentralise the extension of the basic status levels."@en .

swvocab:moreinfo a rdf:Property ;
    rdfs:label "more info" ;
    rdfs:comment "more information about the status etc of a term, typically human oriented" ;
    rdfs:isDefinedBy swvocab: ;
    swvocab:term_status "unstable" .

swvocab:term_status a rdf:Property,
        owl:AnnotationProperty ;
    rdfs:label "term status" ;
    rdfs:comment "the status of a vocabulary term, expressed as a short symbolic string; known values include 'unstable','testing', 'stable' and 'archaic'" ;
    rdfs:isDefinedBy swvocab: ;
    swvocab:term_status "unstable" .

swvocab:userdocs a rdf:Property ;
    rdfs:label "user docs" ;
    rdfs:comment "human-oriented documentation, examples etc for use of this term" ;
    rdfs:isDefinedBy swvocab: ;
    swvocab:term_status "unstable" .

skos:changeNote a rdf:Property,
        owl:AnnotationProperty ;
    rdfs:label "change note"@en ;
    rdfs:isDefinedBy <http://www.w3.org/2004/02/skos/core> ;
    rdfs:subPropertyOf skos:note ;
    skos:definition "A note about a modification to a concept."@en .

skos:definition a rdf:Property,
        owl:AnnotationProperty ;
    rdfs:label "definition"@en ;
    rdfs:isDefinedBy <http://www.w3.org/2004/02/skos/core> ;
    rdfs:subPropertyOf skos:note ;
    skos:definition "A statement or formal explanation of the meaning of a concept."@en .

skos:editorialNote a rdf:Property,
        owl:AnnotationProperty ;
    rdfs:label "editorial note"@en ;
    rdfs:isDefinedBy <http://www.w3.org/2004/02/skos/core> ;
    rdfs:subPropertyOf skos:note ;
    skos:definition "A note for an editor, translator or maintainer of the vocabulary."@en .

skos:exactMatch a rdf:Property,
        owl:ObjectProperty,
        owl:SymmetricProperty,
        owl:TransitiveProperty ;
    rdfs:label "has exact match"@en ;
    rdfs:comment "skos:exactMatch is disjoint with each of the properties skos:broadMatch and skos:relatedMatch."@en ;
    rdfs:isDefinedBy <http://www.w3.org/2004/02/skos/core> ;
    rdfs:subPropertyOf skos:closeMatch ;
    skos:definition "skos:exactMatch is used to link two concepts, indicating a high degree of confidence that the concepts can be used interchangeably across a wide range of information retrieval applications. skos:exactMatch is a transitive property, and is a sub-property of skos:closeMatch."@en .

skos:example a rdf:Property,
        owl:AnnotationProperty ;
    rdfs:label "example"@en ;
    rdfs:isDefinedBy <http://www.w3.org/2004/02/skos/core> ;
    rdfs:subPropertyOf skos:note ;
    skos:definition "An example of the use of a concept."@en .

skos:hiddenLabel a rdf:Property,
        owl:AnnotationProperty ;
    rdfs:label "hidden label"@en ;
    rdfs:comment "The range of skos:hiddenLabel is the class of RDF plain literals."@en,
        "skos:prefLabel, skos:altLabel and skos:hiddenLabel are pairwise disjoint properties."@en ;
    rdfs:isDefinedBy <http://www.w3.org/2004/02/skos/core> ;
    rdfs:subPropertyOf rdfs:label ;
    skos:definition "A lexical label for a resource that should be hidden when generating visual displays of the resource, but should still be accessible to free text search operations."@en .

skos:historyNote a rdf:Property,
        owl:AnnotationProperty ;
    rdfs:label "history note"@en ;
    rdfs:isDefinedBy <http://www.w3.org/2004/02/skos/core> ;
    rdfs:subPropertyOf skos:note ;
    skos:definition "A note about the past state/use/meaning of a concept."@en .

skos:member a rdf:Property,
        owl:ObjectProperty ;
    rdfs:label "has member"@en ;
    rdfs:domain skos:Collection ;
    rdfs:isDefinedBy <http://www.w3.org/2004/02/skos/core> ;
    rdfs:range [ a owl:Class ;
            owl:unionOf ( skos:Concept skos:Collection ) ] ;
    skos:definition "Relates a collection to one of its members."@en .

skos:memberList a rdf:Property,
        owl:FunctionalProperty,
        owl:ObjectProperty ;
    rdfs:label "has member list"@en ;
    rdfs:comment """For any resource, every item in the list given as the value of the
      skos:memberList property is also a value of the skos:member property."""@en ;
    rdfs:domain skos:OrderedCollection ;
    rdfs:isDefinedBy <http://www.w3.org/2004/02/skos/core> ;
    rdfs:range rdf:List ;
    skos:definition "Relates an ordered collection to the RDF list containing its members."@en .

skos:notation a rdf:Property,
        owl:DatatypeProperty ;
    rdfs:label "notation"@en ;
    rdfs:comment "Used to store the values of feature codes"@en ;
    rdfs:isDefinedBy <http://www.w3.org/2004/02/skos/core> ;
    skos:definition "A notation, also known as classification code, is a string of characters such as \"T58.5\" or \"303.4833\" used to uniquely identify a concept within the scope of a given concept scheme."@en ;
    skos:scopeNote "By convention, skos:notation is used with a typed literal in the object position of the triple."@en .

skos:relatedMatch a rdf:Property,
        owl:ObjectProperty,
        owl:SymmetricProperty ;
    rdfs:label "has related match"@en ;
    rdfs:isDefinedBy <http://www.w3.org/2004/02/skos/core> ;
    rdfs:subPropertyOf skos:mappingRelation,
        skos:related ;
    skos:definition "skos:relatedMatch is used to state an associative mapping link between two conceptual resources in different concept schemes."@en .

skos:scopeNote a rdf:Property,
        owl:AnnotationProperty ;
    rdfs:label "scope note"@en ;
    rdfs:isDefinedBy <http://www.w3.org/2004/02/skos/core> ;
    rdfs:subPropertyOf skos:note ;
    skos:definition "A note that helps to clarify the meaning and/or the use of a concept."@en .

locn:address a rdf:Property ;
    rdfs:label "address"@en ;
    dcterms:identifier "locn:address" ;
    rdfs:comment "The locn:address property relationship associates any resource with the locn:Address class "@en ;
    rdfs:isDefinedBy <http://www.w3.org/ns/locn> ;
    rdfs:range locn:Address ;
    swvocab:term_status "testing"@en .

locn:addressArea a rdf:Property ;
    rdfs:label "address area"@en ;
    dcterms:identifier "locn:addressArea" ;
    rdfs:comment "The name or names of a geographic area or locality that groups a number of addressable objects for addressing purposes, without being an administrative unit. This would typically be part of a city, a neighbourhood or village. The domain of locn:addressArea is locn:Address."@en ;
    rdfs:domain locn:Address ;
    rdfs:isDefinedBy <http://www.w3.org/ns/locn> ;
    rdfs:range rdfs:Literal ;
    swvocab:term_status "testing"@en .

locn:addressId a rdf:Property ;
    rdfs:label "address ID"@en ;
    dcterms:identifier "locn:addressId" ;
    rdfs:comment "The concept of adding a globally unique identifier for each instance of an address is a crucial part of the INSPIRE data spec. The domain of locn:addressId is locn:Address."@en ;
    rdfs:domain locn:Address ;
    rdfs:isDefinedBy <http://www.w3.org/ns/locn> ;
    rdfs:range rdfs:Literal ;
    swvocab:term_status "unstable"@en .

locn:adminUnitL1 a rdf:Property ;
    rdfs:label "admin unit level 1"@en ;
    dcterms:identifier "locn:adminUnitL1" ;
    vann:usageNote "Best practice is to use the ISO 3166-1 code but if this is inappropriate for the context, country names should be provided in a consistent manner to reduce ambiguity. For example, either write 'United Kingdom' or 'UK' consistently throughout the data set and avoid mixing the two."@en ;
    rdfs:comment "The uppermost administrative unit for the address, almost always a country. The domain of locn:adminUnitL1 is locn:Address and the range is a literal, conceptually defined by the INSPIRE Geographical Name data type."@en ;
    rdfs:domain locn:Address ;
    rdfs:isDefinedBy <http://www.w3.org/ns/locn> ;
    swvocab:term_status "testing"@en .

locn:adminUnitL2 a rdf:Property ;
    rdfs:label "admin unit level 2"@en ;
    dcterms:identifier "locn:adminUnitL2" ;
    rdfs:comment "The region of the address, usually a county, state or other such area that typically encompasses several localities. The domain of  locn:adminUnitL2 is locn:Address and the range is a literal, conceptually defined by the INSPIRE Geographical Name data type."@en ;
    rdfs:domain locn:Address ;
    rdfs:isDefinedBy <http://www.w3.org/ns/locn> ;
    swvocab:term_status "testing"@en .

locn:fullAddress a rdf:Property ;
    rdfs:label "full address"@en ;
    dcterms:identifier "locn:fullAddress" ;
    rdfs:comment "The complete address written as a string, with or without formatting. The domain of locn:fullAddress is locn:Address."@en ;
    rdfs:domain locn:Address ;
    rdfs:isDefinedBy <http://www.w3.org/ns/locn> ;
    rdfs:range rdfs:Literal ;
    swvocab:term_status "testing"@en .

locn:geographicName a rdf:Property ;
    rdfs:label "geographic name"@en ;
    dcterms:identifier "locn:geographicName" ;
    rdfs:comment """
A geographic name is a proper noun applied to a spatial object. Taking the example used in the relevant INSPIRE data specification (page 18), the following are all valid geographic names for the Greek capital:
- Αθήνα (the Greek endonym written in the Greek script)
- Athína (the standard Romanisation of the endonym)
- Athens (the English language exonym)
For INSPIRE-conformant data, provide the metadata for the geographic name using a skos:Concept as a datatype.
"""@en ;
    rdfs:isDefinedBy <http://www.w3.org/ns/locn> ;
    swvocab:term_status "testing"@en ;
    powder-s:describedby <https://joinup.ec.europa.eu/node/55858> .

locn:geometry a rdf:Property ;
    rdfs:label "geometry"@en ;
    dcterms:identifier "locn:geometry" ;
    vann:example """
The following are examples of equivalent statements using different geometry encodings. In the examples, prefix gsp is used for namespace URI http://www.opengis.net/ont/geosparql#, whereas prefix sf is used for namespace URI http://www.opengis.net/ont/sf#.
- WKT (GeoSPARQL)
:Resource locn:geometry
  "<http://www.opengis.net/def/crs/OGC/1.3/CRS84> Point(-0.001475 51.477811)"^^gsp:wktLiteral .
- GML
:Resource locn:geometry
  "<gml:Point srsName='http://www.opengis.net/def/crs/OGC/1.3/CRS84'>
  <gml:coordinates>-0.001475, 51.477811</gml:coordinates></gml:Point>"^^gsp:gmlLiteral .
- RDF+WKT (GeoSPARQL)
:Resource locn:geometry
  [ a sf:Point; gsp:asWKT "<http://www.opengis.net/def/crs/OGC/1.3/CRS84> Point(-0.001475 51.477811)"^^gsp:wktLiteral ] .
- RDF+GML (GeoSPARQL)
:Resource locn:geometry
  [ a sf:Point; gsp:asGML
     "<gml:Point srsName='http://www.opengis.net/def/crs/OGC/1.3/CRS84'>
      <gml:coordinates>-0.001475, 51.477811</gml:coordinates></gml:Point>"^^gsp:gmlLiteral ] .
- RDF (WGS84 lat/long)
:Resource locn:geometry [ a geo:Point; geo:lat "51.477811"; geo:long "-0.001475" ] .
- RDF (schema.org)
:Resource locn:geometry [ a schema:GeoCoordinates; schema:latitude "51.477811"; schema:longitude "-0.001475" ] .
- geo URI
:Resource locn:geometry <geo:51.477811,-0.001475;u=0;crs=wgs84> .
- GeoHash URI
:Resource locn:geometry <http://geohash.org/gcpuzgnzvxkp> .
    """@en ;
    vann:usageNote """
Depending on how a geometry is encoded, the range of this property may be one of the following:
- a literal (e.g., WKT - string literal -, GML, KML - XML literal)
- a geometry class, as those defined in the OGC's GeoSPARQL specification, in the W3C's Basic Geo (WGS84 lat/long) vocabulary, and at schema.org;
- geocoded URIs, as geo or GeoHash URIs, treated as URI references.
For interoperability reasons, it is recommended using one of the following:
- Any geometry:
  - WKT, GML, and RDF+WKT/GML, as per the GeoSPARQL specification.
  - KML (Keyhole Markup Language) - note that KML supports the following geometries only: point, line string, linear ring, and polygon.
  - RDF as per the schema.org vocabulary (see classes schema:GeoCoordinates and schema:GeoShape).
- Points: one of the above, or:
  - RDF as per the W3C Basic Geo (WGS84 lat/long) vocabulary.
  - GeoHash URIs.
  - geo URIs.
    """@en ;
    rdfs:comment "Associates any resource with the corresponding geometry."@en ;
    rdfs:isDefinedBy <http://www.w3.org/ns/locn> ;
    rdfs:range locn:Geometry ;
    swvocab:term_status "testing"@en ;
    powder-s:describedby <https://joinup.ec.europa.eu/node/55858> .

locn:location a rdf:Property ;
    rdfs:label "location"@en ;
    dcterms:identifier "locn:location" ;
    rdfs:comment "The location property links any resource to the Location Class. Asserting the location relationship implies only that the domain has some connection to a Location in time or space. It does not imply that the resource is necessarily at that location at the time when the assertion is made."@en ;
    rdfs:isDefinedBy <http://www.w3.org/ns/locn> ;
    rdfs:range dcterms:Location ;
    swvocab:term_status "testing"@en .

locn:locatorDesignator a rdf:Property ;
    rdfs:label "locator designator"@en ;
    dcterms:identifier "locn:locatorDesignator" ;
    rdfs:comment """A number or a sequence of characters that uniquely identifies the locator within the relevant scope(s). The full identification of the locator could include one or more locator designators.
    """@en ;
    rdfs:isDefinedBy <http://www.w3.org/ns/locn> ;
    swvocab:term_status "testing"@en .

locn:locatorName a rdf:Property ;
    rdfs:label "locator name"@en ;
    dcterms:identifier "locn:locatorName" ;
    rdfs:comment """Proper noun(s) applied to the real world entity identified by the locator. The locator name could be the name of the property or complex, of the building or part of the building, or it could be the name of a room inside a building. 
    """@en ;
    rdfs:isDefinedBy <http://www.w3.org/ns/locn> ;
    swvocab:term_status "testing"@en .

locn:poBox a rdf:Property ;
    rdfs:label "PO box"@en ;
    dcterms:identifier "locn:poBox" ;
    rdfs:comment "The Post Office Box number. The domain of locn:poBox is locn:Address."@en ;
    rdfs:domain locn:Address ;
    rdfs:isDefinedBy <http://www.w3.org/ns/locn> ;
    rdfs:range rdfs:Literal ;
    swvocab:term_status "testing"@en .

locn:postCode a rdf:Property ;
    rdfs:label "post code"@en ;
    dcterms:identifier "locn:postCode" ;
    rdfs:comment "The post code (a.k.a postal code, zip code etc.). Post codes are common elements in many countries' postal address systems. The domain of locn:postCode is locn:Address."@en ;
    rdfs:domain locn:Address ;
    rdfs:isDefinedBy <http://www.w3.org/ns/locn> ;
    rdfs:range rdfs:Literal ;
    swvocab:term_status "testing"@en .

locn:postName a rdf:Property ;
    rdfs:label "post name"@en ;
    dcterms:identifier "locn:postName" ;
    rdfs:comment "The key postal division of the address, usually the city. (INSPIRE's definition is \"One or more names created and maintained for postal purposes to identify a subdivision of addresses and postal delivery points.\"). The domain of locn:postName is locn:Address."@en ;
    rdfs:domain locn:Address ;
    rdfs:isDefinedBy <http://www.w3.org/ns/locn> ;
    rdfs:range rdfs:Literal ;
    swvocab:term_status "testing"@en .

locn:thoroughfare a rdf:Property ;
    rdfs:label "thoroughfare"@en ;
    dcterms:identifier "locn:thoroughfare" ;
    rdfs:comment "An address component that represents the name of a passage or way through from one location to another. A thoroughfare is not necessarily a road, it might be a waterway or some other feature. The domain of locn:thoroughfare is locn:Address."@en ;
    rdfs:domain locn:Address ;
    rdfs:isDefinedBy <http://www.w3.org/ns/locn> ;
    rdfs:range rdfs:Literal ;
    swvocab:term_status "testing"@en .

foaf:account a rdf:Property,
        owl:ObjectProperty ;
    rdfs:label "account" ;
    rdfs:comment "Indicates an account held by this agent." ;
    rdfs:domain foaf:Agent ;
    rdfs:isDefinedBy foaf: ;
    rdfs:range foaf:OnlineAccount ;
    swvocab:term_status "testing" .

foaf:accountName a rdf:Property,
        owl:DatatypeProperty ;
    rdfs:label "account name" ;
    rdfs:comment "Indicates the name (identifier) associated with this online account." ;
    rdfs:domain foaf:OnlineAccount ;
    rdfs:isDefinedBy foaf: ;
    rdfs:range rdfs:Literal ;
    swvocab:term_status "testing" .

foaf:accountServiceHomepage a rdf:Property,
        owl:ObjectProperty ;
    rdfs:label "account service homepage" ;
    rdfs:comment "Indicates a homepage of the service provide for this online account." ;
    rdfs:domain foaf:OnlineAccount ;
    rdfs:isDefinedBy foaf: ;
    rdfs:range foaf:Document ;
    swvocab:term_status "testing" .

foaf:age a rdf:Property,
        owl:DatatypeProperty,
        owl:FunctionalProperty ;
    rdfs:label "age" ;
    rdfs:comment "The age in years of some agent." ;
    rdfs:domain foaf:Agent ;
    rdfs:isDefinedBy foaf: ;
    rdfs:range rdfs:Literal ;
    swvocab:term_status "unstable" .

foaf:aimChatID a rdf:Property,
        owl:DatatypeProperty,
        owl:InverseFunctionalProperty ;
    rdfs:label "AIM chat ID" ;
    rdfs:comment "An AIM chat ID" ;
    rdfs:domain foaf:Agent ;
    rdfs:isDefinedBy foaf: ;
    rdfs:range rdfs:Literal ;
    rdfs:subPropertyOf foaf:nick ;
    swvocab:term_status "testing" .

foaf:birthday a rdf:Property,
        owl:DatatypeProperty,
        owl:FunctionalProperty ;
    rdfs:label "birthday" ;
    rdfs:comment "The birthday of this Agent, represented in mm-dd string form, eg. '12-31'." ;
    rdfs:domain foaf:Agent ;
    rdfs:isDefinedBy foaf: ;
    rdfs:range rdfs:Literal ;
    swvocab:term_status "unstable" .

foaf:currentProject a rdf:Property,
        owl:ObjectProperty ;
    rdfs:label "current project" ;
    rdfs:comment "A current project this person works on." ;
    rdfs:domain foaf:Person ;
    rdfs:isDefinedBy foaf: ;
    rdfs:range owl:Thing ;
    swvocab:term_status "testing" .

foaf:dnaChecksum a rdf:Property,
        owl:DatatypeProperty ;
    rdfs:label "DNA checksum" ;
    rdfs:comment "A checksum for the DNA of some thing. Joke." ;
    rdfs:isDefinedBy foaf: ;
    rdfs:range rdfs:Literal ;
    swvocab:term_status "archaic" .

foaf:familyName a rdf:Property,
        owl:DatatypeProperty ;
    rdfs:label "familyName" ;
    rdfs:comment "The family name of some person." ;
    rdfs:domain foaf:Person ;
    rdfs:isDefinedBy foaf: ;
    rdfs:range rdfs:Literal ;
    swvocab:term_status "testing" .

foaf:family_name a rdf:Property,
        owl:DatatypeProperty ;
    rdfs:label "family_name" ;
    rdfs:comment "The family name of some person." ;
    rdfs:domain foaf:Person ;
    rdfs:isDefinedBy foaf: ;
    rdfs:range rdfs:Literal ;
    swvocab:term_status "archaic" .

foaf:firstName a rdf:Property,
        owl:DatatypeProperty ;
    rdfs:label "firstName" ;
    rdfs:comment "The first name of a person." ;
    rdfs:domain foaf:Person ;
    rdfs:isDefinedBy foaf: ;
    rdfs:range rdfs:Literal ;
    swvocab:term_status "testing" .

foaf:focus a rdf:Property,
        owl:ObjectProperty ;
    rdfs:label "focus" ;
    rdfs:comment "The underlying or 'focal' entity associated with some SKOS-described concept." ;
    rdfs:domain skos:Concept ;
    rdfs:isDefinedBy foaf: ;
    rdfs:range owl:Thing ;
    swvocab:term_status "testing" .

foaf:fundedBy a rdf:Property,
        owl:ObjectProperty ;
    rdfs:label "funded by" ;
    rdfs:comment "An organization funding a project or person." ;
    rdfs:domain owl:Thing ;
    rdfs:isDefinedBy foaf: ;
    rdfs:range owl:Thing ;
    swvocab:term_status "archaic" .

foaf:geekcode a rdf:Property,
        owl:DatatypeProperty ;
    rdfs:label "geekcode" ;
    rdfs:comment "A textual geekcode for this person, see http://www.geekcode.com/geek.html" ;
    rdfs:domain foaf:Person ;
    rdfs:isDefinedBy foaf: ;
    rdfs:range rdfs:Literal ;
    swvocab:term_status "archaic" .

foaf:gender a rdf:Property,
        owl:DatatypeProperty,
        owl:FunctionalProperty ;
    rdfs:label "gender" ;
    rdfs:comment "The gender of this Agent (typically but not necessarily 'male' or 'female')." ;
    rdfs:domain foaf:Agent ;
    rdfs:isDefinedBy foaf: ;
    rdfs:range rdfs:Literal ;
    swvocab:term_status "testing" .

foaf:givenName a rdf:Property,
        owl:DatatypeProperty ;
    rdfs:label "Given name" ;
    rdfs:comment "The given name of some person." ;
    rdfs:isDefinedBy foaf: ;
    swvocab:term_status "testing" .

foaf:givenname a rdf:Property,
        owl:DatatypeProperty ;
    rdfs:label "Given name" ;
    rdfs:comment "The given name of some person." ;
    rdfs:isDefinedBy foaf: ;
    swvocab:term_status "archaic" .

foaf:holdsAccount a rdf:Property,
        owl:ObjectProperty ;
    rdfs:label "account" ;
    rdfs:comment "Indicates an account held by this agent." ;
    rdfs:domain foaf:Agent ;
    rdfs:isDefinedBy foaf: ;
    rdfs:range foaf:OnlineAccount ;
    swvocab:term_status "archaic" .

foaf:homepage a rdf:Property,
        owl:InverseFunctionalProperty,
        owl:ObjectProperty ;
    rdfs:label "homepage" ;
    rdfs:comment "A homepage for some thing." ;
    rdfs:domain owl:Thing ;
    rdfs:isDefinedBy foaf: ;
    rdfs:range foaf:Document ;
    rdfs:subPropertyOf foaf:isPrimaryTopicOf,
        foaf:page ;
    swvocab:term_status "stable" .

foaf:icqChatID a rdf:Property,
        owl:DatatypeProperty,
        owl:InverseFunctionalProperty ;
    rdfs:label "ICQ chat ID" ;
    rdfs:comment "An ICQ chat ID" ;
    rdfs:domain foaf:Agent ;
    rdfs:isDefinedBy foaf: ;
    rdfs:range rdfs:Literal ;
    rdfs:subPropertyOf foaf:nick ;
    swvocab:term_status "testing" .

foaf:img a rdf:Property,
        owl:ObjectProperty ;
    rdfs:label "image" ;
    rdfs:comment "An image that can be used to represent some thing (ie. those depictions which are particularly representative of something, eg. one's photo on a homepage)." ;
    rdfs:domain foaf:Person ;
    rdfs:isDefinedBy foaf: ;
    rdfs:range foaf:Image ;
    rdfs:subPropertyOf foaf:depiction ;
    swvocab:term_status "testing" .

foaf:interest a rdf:Property,
        owl:ObjectProperty ;
    rdfs:label "interest" ;
    rdfs:comment "A page about a topic of interest to this person." ;
    rdfs:domain foaf:Agent ;
    rdfs:isDefinedBy foaf: ;
    rdfs:range foaf:Document ;
    swvocab:term_status "testing" .

foaf:jabberID a rdf:Property,
        owl:DatatypeProperty,
        owl:InverseFunctionalProperty ;
    rdfs:label "jabber ID" ;
    rdfs:comment "A jabber ID for something." ;
    rdfs:domain foaf:Agent ;
    rdfs:isDefinedBy foaf: ;
    rdfs:range rdfs:Literal ;
    swvocab:term_status "testing" .

foaf:knows a rdf:Property,
        owl:ObjectProperty ;
    rdfs:label "knows" ;
    rdfs:comment "A person known by this person (indicating some level of reciprocated interaction between the parties)." ;
    rdfs:domain foaf:Person ;
    rdfs:isDefinedBy foaf: ;
    rdfs:range foaf:Person ;
    swvocab:term_status "stable" .

foaf:lastName a rdf:Property,
        owl:DatatypeProperty ;
    rdfs:label "lastName" ;
    rdfs:comment "The last name of a person." ;
    rdfs:domain foaf:Person ;
    rdfs:isDefinedBy foaf: ;
    rdfs:range rdfs:Literal ;
    swvocab:term_status "testing" .

foaf:logo a rdf:Property,
        owl:InverseFunctionalProperty,
        owl:ObjectProperty ;
    rdfs:label "logo" ;
    rdfs:comment "A logo representing some thing." ;
    rdfs:domain owl:Thing ;
    rdfs:isDefinedBy foaf: ;
    rdfs:range owl:Thing ;
    swvocab:term_status "testing" .

foaf:mbox a rdf:Property,
        owl:InverseFunctionalProperty,
        owl:ObjectProperty ;
    rdfs:label "personal mailbox" ;
    rdfs:comment "A  personal mailbox, ie. an Internet mailbox associated with exactly one owner, the first owner of this mailbox. This is a 'static inverse functional property', in that  there is (across time and change) at most one individual that ever has any particular value for foaf:mbox." ;
    rdfs:domain foaf:Agent ;
    rdfs:isDefinedBy foaf: ;
    rdfs:range owl:Thing ;
    swvocab:term_status "stable" .

foaf:mbox_sha1sum a rdf:Property,
        owl:DatatypeProperty,
        owl:InverseFunctionalProperty ;
    rdfs:label "sha1sum of a personal mailbox URI name" ;
    rdfs:comment "The sha1sum of the URI of an Internet mailbox associated with exactly one owner, the  first owner of the mailbox." ;
    rdfs:domain foaf:Agent ;
    rdfs:isDefinedBy foaf: ;
    rdfs:range rdfs:Literal ;
    swvocab:term_status "testing" .

foaf:member a rdf:Property,
        owl:ObjectProperty ;
    rdfs:label "member" ;
    rdfs:comment "Indicates a member of a Group" ;
    rdfs:domain foaf:Group ;
    rdfs:isDefinedBy foaf: ;
    rdfs:range foaf:Agent ;
    swvocab:term_status "stable" .

foaf:membershipClass a rdf:Property,
        owl:AnnotationProperty ;
    rdfs:label "membershipClass" ;
    rdfs:comment "Indicates the class of individuals that are a member of a Group" ;
    rdfs:isDefinedBy foaf: ;
    swvocab:term_status "unstable" .

foaf:msnChatID a rdf:Property,
        owl:DatatypeProperty,
        owl:InverseFunctionalProperty ;
    rdfs:label "MSN chat ID" ;
    rdfs:comment "An MSN chat ID" ;
    rdfs:domain foaf:Agent ;
    rdfs:isDefinedBy foaf: ;
    rdfs:range rdfs:Literal ;
    rdfs:subPropertyOf foaf:nick ;
    swvocab:term_status "testing" .

foaf:myersBriggs a rdf:Property,
        owl:DatatypeProperty ;
    rdfs:label "myersBriggs" ;
    rdfs:comment "A Myers Briggs (MBTI) personality classification." ;
    rdfs:domain foaf:Person ;
    rdfs:isDefinedBy foaf: ;
    rdfs:range rdfs:Literal ;
    swvocab:term_status "testing" .

foaf:name a rdf:Property,
        owl:DatatypeProperty ;
    rdfs:label "name" ;
    rdfs:comment "A name for some thing." ;
    rdfs:domain owl:Thing ;
    rdfs:isDefinedBy foaf: ;
    rdfs:range rdfs:Literal ;
    rdfs:subPropertyOf rdfs:label ;
    swvocab:term_status "testing" .

foaf:openid a rdf:Property,
        owl:InverseFunctionalProperty,
        owl:ObjectProperty ;
    rdfs:label "openid" ;
    rdfs:comment "An OpenID for an Agent." ;
    rdfs:domain foaf:Agent ;
    rdfs:isDefinedBy foaf: ;
    rdfs:range foaf:Document ;
    rdfs:subPropertyOf foaf:isPrimaryTopicOf ;
    swvocab:term_status "testing" .

foaf:pastProject a rdf:Property,
        owl:ObjectProperty ;
    rdfs:label "past project" ;
    rdfs:comment "A project this person has previously worked on." ;
    rdfs:domain foaf:Person ;
    rdfs:isDefinedBy foaf: ;
    rdfs:range owl:Thing ;
    swvocab:term_status "testing" .

foaf:phone a rdf:Property,
        owl:ObjectProperty ;
    rdfs:label "phone" ;
    rdfs:comment "A phone,  specified using fully qualified tel: URI scheme (refs: http://www.w3.org/Addressing/schemes.html#tel)." ;
    rdfs:isDefinedBy foaf: ;
    swvocab:term_status "testing" .

foaf:plan a rdf:Property,
        owl:DatatypeProperty ;
    rdfs:label "plan" ;
    rdfs:comment "A .plan comment, in the tradition of finger and '.plan' files." ;
    rdfs:domain foaf:Person ;
    rdfs:isDefinedBy foaf: ;
    rdfs:range rdfs:Literal ;
    swvocab:term_status "testing" .

foaf:publications a rdf:Property,
        owl:ObjectProperty ;
    rdfs:label "publications" ;
    rdfs:comment "A link to the publications of this person." ;
    rdfs:domain foaf:Person ;
    rdfs:isDefinedBy foaf: ;
    rdfs:range foaf:Document ;
    swvocab:term_status "testing" .

foaf:schoolHomepage a rdf:Property,
        owl:ObjectProperty ;
    rdfs:label "schoolHomepage" ;
    rdfs:comment "A homepage of a school attended by the person." ;
    rdfs:domain foaf:Person ;
    rdfs:isDefinedBy foaf: ;
    rdfs:range foaf:Document ;
    swvocab:term_status "testing" .

foaf:sha1 a rdf:Property,
        owl:DatatypeProperty ;
    rdfs:label "sha1sum (hex)" ;
    rdfs:comment "A sha1sum hash, in hex." ;
    rdfs:domain foaf:Document ;
    rdfs:isDefinedBy foaf: ;
    swvocab:term_status "unstable" .

foaf:skypeID a rdf:Property,
        owl:DatatypeProperty ;
    rdfs:label "Skype ID" ;
    rdfs:comment "A Skype ID" ;
    rdfs:domain foaf:Agent ;
    rdfs:isDefinedBy foaf: ;
    rdfs:range rdfs:Literal ;
    rdfs:subPropertyOf foaf:nick ;
    swvocab:term_status "testing" .

foaf:status a rdf:Property,
        owl:DatatypeProperty ;
    rdfs:label "status" ;
    rdfs:comment "A string expressing what the user is happy for the general public (normally) to know about their current activity." ;
    rdfs:domain foaf:Agent ;
    rdfs:isDefinedBy foaf: ;
    rdfs:range rdfs:Literal ;
    swvocab:term_status "unstable" .

foaf:surname a rdf:Property,
        owl:DatatypeProperty ;
    rdfs:label "Surname" ;
    rdfs:comment "The surname of some person." ;
    rdfs:domain foaf:Person ;
    rdfs:isDefinedBy foaf: ;
    rdfs:range rdfs:Literal ;
    swvocab:term_status "archaic" .

foaf:theme a rdf:Property,
        owl:ObjectProperty ;
    rdfs:label "theme" ;
    rdfs:comment "A theme." ;
    rdfs:domain owl:Thing ;
    rdfs:isDefinedBy foaf: ;
    rdfs:range owl:Thing ;
    swvocab:term_status "archaic" .

foaf:thumbnail a rdf:Property,
        owl:ObjectProperty ;
    rdfs:label "thumbnail" ;
    rdfs:comment "A derived thumbnail image." ;
    rdfs:domain foaf:Image ;
    rdfs:isDefinedBy foaf: ;
    rdfs:range foaf:Image ;
    swvocab:term_status "testing" .

foaf:tipjar a rdf:Property,
        owl:ObjectProperty ;
    rdfs:label "tipjar" ;
    rdfs:comment "A tipjar document for this agent, describing means for payment and reward." ;
    rdfs:domain foaf:Agent ;
    rdfs:isDefinedBy foaf: ;
    rdfs:range foaf:Document ;
    rdfs:subPropertyOf foaf:page ;
    swvocab:term_status "testing" .

foaf:title a rdf:Property,
        owl:DatatypeProperty ;
    rdfs:label "title" ;
    rdfs:comment "Title (Mr, Mrs, Ms, Dr. etc)" ;
    rdfs:isDefinedBy foaf: ;
    swvocab:term_status "testing" .

foaf:topic_interest a rdf:Property,
        owl:ObjectProperty ;
    rdfs:label "topic_interest" ;
    rdfs:comment "A thing of interest to this person." ;
    rdfs:domain foaf:Agent ;
    rdfs:isDefinedBy foaf: ;
    rdfs:range owl:Thing ;
    swvocab:term_status "testing" .

foaf:weblog a rdf:Property,
        owl:InverseFunctionalProperty,
        owl:ObjectProperty ;
    rdfs:label "weblog" ;
    rdfs:comment "A weblog of some thing (whether person, group, company etc.)." ;
    rdfs:domain foaf:Agent ;
    rdfs:isDefinedBy foaf: ;
    rdfs:range foaf:Document ;
    rdfs:subPropertyOf foaf:page ;
    swvocab:term_status "stable" .

foaf:workInfoHomepage a rdf:Property,
        owl:ObjectProperty ;
    rdfs:label "work info homepage" ;
    rdfs:comment "A work info homepage of some person; a page about their work for some organization." ;
    rdfs:domain foaf:Person ;
    rdfs:isDefinedBy foaf: ;
    rdfs:range foaf:Document ;
    swvocab:term_status "testing" .

foaf:workplaceHomepage a rdf:Property,
        owl:ObjectProperty ;
    rdfs:label "workplace homepage" ;
    rdfs:comment "A workplace homepage of some person; the homepage of an organization they work for." ;
    rdfs:domain foaf:Person ;
    rdfs:isDefinedBy foaf: ;
    rdfs:range foaf:Document ;
    swvocab:term_status "testing" .

foaf:yahooChatID a rdf:Property,
        owl:DatatypeProperty,
        owl:InverseFunctionalProperty ;
    rdfs:label "Yahoo chat ID" ;
    rdfs:comment "A Yahoo chat ID" ;
    rdfs:domain foaf:Agent ;
    rdfs:isDefinedBy foaf: ;
    rdfs:range rdfs:Literal ;
    rdfs:subPropertyOf foaf:nick ;
    swvocab:term_status "testing" .

wot:assurance a owl:AnnotationProperty .

wot:src_assurance a owl:AnnotationProperty .

person:bernard-vatant a foaf:Person ;
    foaf:name "Bernard Vatant" ;
    foaf:page <http://blog.hubjects.com> ;
    foaf:workplaceHomepage <http://www.mondeca.com> .

resource:GeoNames a foaf:Organization ;
    ns4:dtm gn:Marc-Wick ;
    foaf:homepage <http://www.geonames.org> ;
    foaf:name "GeoNames" .

crmeh:EHE0009_ContextFind a owl:Class ;
    rdfs:label "Context Find"@en ;
    rdfs:comment "Finds are obviously physical objects; it may be that a particular find can be described in more detail as a man-made object, but not all finds are man-made hence the link to the more generic entity. The distinction between bulk finds and small finds present in the recording system does not appear to relate to the nature of finds themselves, rather to the practicalities of recording large numbers of objects hence, at this point, no distinction is made between bulk and small finds other than bulk finds have less information about them recorded"@en ;
    rdfs:isDefinedBy crmeh:CRMEH ;
    rdfs:subClassOf crm:E19_Physical_Object ;
    owl:sameAs crmeh:EHE0009 ;
    skos:notation "EHE0009" .

crmeh:EHE0018_ContextSample a owl:Class ;
    rdfs:label "Context Sample"@en ;
    rdfs:comment "A sample can be seen as some stuff removed from something"@en ;
    rdfs:isDefinedBy crmeh:CRMEH ;
    rdfs:subClassOf crm:E18_Physical_Thing ;
    owl:sameAs crmeh:EHE0018 ;
    skos:notation "EHE0018" .

crmeh:EHP3_occupied a owl:ObjectProperty ;
    rdfs:label "occupied"@en ;
    rdfs:comment "The Physical Stuff is located at the place defined by the Context. This property is a specialism of \"P53: has former or current location\", as it denotes the place the Context Stuff filled out when the Context was defined. It may be at other places before (e.g. geological pressures/ landdrift etc.) or after (removal as block)"@en ;
    rdfs:domain crmeh:EHE0008_ContextStuff ;
    rdfs:isDefinedBy crmeh:CRMEH ;
    rdfs:range crmeh:EHE0007_Context ;
    rdfs:subPropertyOf crm:P53_has_former_or_current_location ;
    owl:inverseOf crmeh:EHP3i_was_occupied_by ;
    owl:sameAs crmeh:EHP3 ;
    skos:notation "EHP3" .

crmeh:EHP3i_was_occupied_by a owl:ObjectProperty ;
    rdfs:label "was occupied by"@en ;
    rdfs:domain crmeh:EHE0007_Context ;
    rdfs:isDefinedBy crmeh:CRMEH ;
    rdfs:range crmeh:EHE0008_ContextStuff ;
    rdfs:subPropertyOf crm:P53i_is_former_or_current_location_of ;
    owl:inverseOf crmeh:EHP3_occupied ;
    owl:sameAs crmeh:EHP3i ;
    skos:notation "EHP3i" .

crmeh:EHP4_depicts a owl:ObjectProperty ;
    rdfs:label "depicts"@en ;
    rdfs:comment "Record photographs show arrangements of contexts at particular points during the excavation. Can also be general record shots of trenches or the excavation as a whole. Can also be of finds in situ"@en ;
    rdfs:domain crmeh:EHE2010_DepictionEvent ;
    rdfs:isDefinedBy crmeh:CRMEH ;
    rdfs:range crmeh:EHE0006_GroupStuff,
        crmeh:EHE0007_Context,
        crmeh:EHE0008_ContextStuff ;
    rdfs:subPropertyOf crm:P62_depicts ;
    owl:inverseOf crmeh:EHP4i_is_depicted_by ;
    owl:sameAs crmeh:EHP4 ;
    skos:notation "EHP4" .

crmeh:EHP4i_is_depicted_by a owl:ObjectProperty ;
    rdfs:label "is depicted by"@en ;
    rdfs:comment "A find can be drawn and photographed"@en ;
    rdfs:domain crmeh:EHE0006_GroupStuff,
        crmeh:EHE0007_Context,
        crmeh:EHE0008_ContextStuff ;
    rdfs:isDefinedBy crmeh:CRMEH ;
    rdfs:range crmeh:EHE2010_DepictionEvent ;
    rdfs:subPropertyOf crm:P62i_is_depicted_by ;
    owl:inverseOf crmeh:EHP4_depicts ;
    owl:sameAs crmeh:EHP4i ;
    skos:notation "EHP4i" .

dc:contributor a rdf:Property ;
    rdfs:label "Contributor"@en ;
    dcterms:description "Examples of a Contributor include a person, an organization, or a service. Typically, the name of a Contributor should be used to indicate the entity."@en ;
    dcterms:hasVersion history:contributor-006 ;
    dcterms:issued "1999-07-02"^^xsd:date ;
    dcterms:modified "2008-01-14"^^xsd:date ;
    rdfs:comment "An entity responsible for making contributions to the resource."@en ;
    rdfs:isDefinedBy dc: ;
    skos:note "A second property with the same name as this property has been declared in the dcterms: namespace (http://purl.org/dc/terms/).  See the Introduction to the document \"DCMI Metadata Terms\" (http://dublincore.org/documents/dcmi-terms/) for an explanation."@en .

dc:creator a rdf:Property ;
    rdfs:label "Creator"@en ;
    dcterms:description "Examples of a Creator include a person, an organization, or a service. Typically, the name of a Creator should be used to indicate the entity."@en ;
    dcterms:hasVersion history:creator-006 ;
    dcterms:issued "1999-07-02"^^xsd:date ;
    dcterms:modified "2008-01-14"^^xsd:date ;
    rdfs:comment "An entity primarily responsible for making the resource."@en ;
    rdfs:isDefinedBy dc: ;
    skos:note "A second property with the same name as this property has been declared in the dcterms: namespace (http://purl.org/dc/terms/).  See the Introduction to the document \"DCMI Metadata Terms\" (http://dublincore.org/documents/dcmi-terms/) for an explanation."@en .

dc:language a rdf:Property ;
    rdfs:label "Language"@en ;
    dcterms:description "Recommended best practice is to use a controlled vocabulary such as RFC 4646 [RFC4646]."@en ;
    dcterms:hasVersion history:language-007 ;
    dcterms:issued "1999-07-02"^^xsd:date ;
    dcterms:modified "2008-01-14"^^xsd:date ;
    rdfs:comment "A language of the resource."@en ;
    rdfs:isDefinedBy dc: ;
    rdfs:seeAlso <http://www.ietf.org/rfc/rfc4646.txt> ;
    skos:note "A second property with the same name as this property has been declared in the dcterms: namespace (http://purl.org/dc/terms/).  See the Introduction to the document \"DCMI Metadata Terms\" (http://dublincore.org/documents/dcmi-terms/) for an explanation."@en .

dc:publisher a rdf:Property ;
    rdfs:label "Publisher"@en ;
    dcterms:description "Examples of a Publisher include a person, an organization, or a service. Typically, the name of a Publisher should be used to indicate the entity."@en ;
    dcterms:hasVersion history:publisher-006 ;
    dcterms:issued "1999-07-02"^^xsd:date ;
    dcterms:modified "2008-01-14"^^xsd:date ;
    rdfs:comment "An entity responsible for making the resource available."@en ;
    rdfs:isDefinedBy dc: ;
    skos:note "A second property with the same name as this property has been declared in the dcterms: namespace (http://purl.org/dc/terms/).  See the Introduction to the document \"DCMI Metadata Terms\" (http://dublincore.org/documents/dcmi-terms/) for an explanation."@en .

dc:source a rdf:Property ;
    rdfs:label "Source"@en ;
    dcterms:description "The described resource may be derived from the related resource in whole or in part. Recommended best practice is to identify the related resource by means of a string conforming to a formal identification system."@en ;
    dcterms:hasVersion history:source-006 ;
    dcterms:issued "1999-07-02"^^xsd:date ;
    dcterms:modified "2008-01-14"^^xsd:date ;
    rdfs:comment "A related resource from which the described resource is derived."@en ;
    rdfs:isDefinedBy dc: ;
    skos:note "A second property with the same name as this property has been declared in the dcterms: namespace (http://purl.org/dc/terms/).  See the Introduction to the document \"DCMI Metadata Terms\" (http://dublincore.org/documents/dcmi-terms/) for an explanation."@en .

dc:subject a rdf:Property ;
    rdfs:label "Subject"@en ;
    dcterms:description "Typically, the subject will be represented using keywords, key phrases, or classification codes. Recommended best practice is to use a controlled vocabulary."@en ;
    dcterms:hasVersion history:subject-007 ;
    dcterms:issued "1999-07-02"^^xsd:date ;
    dcterms:modified "2012-06-14"^^xsd:date ;
    rdfs:comment "The topic of the resource."@en ;
    rdfs:isDefinedBy dc: ;
    skos:note "A second property with the same name as this property has been declared in the dcterms: namespace (http://purl.org/dc/terms/).  See the Introduction to the document \"DCMI Metadata Terms\" (http://dublincore.org/documents/dcmi-terms/) for an explanation."@en .

dc:type a rdf:Property ;
    rdfs:label "Type"@en ;
    dcterms:description "Recommended best practice is to use a controlled vocabulary such as the DCMI Type Vocabulary [DCMITYPE]. To describe the file format, physical medium, or dimensions of the resource, use the Format element."@en ;
    dcterms:hasVersion history:type-006 ;
    dcterms:issued "1999-07-02"^^xsd:date ;
    dcterms:modified "2008-01-14"^^xsd:date ;
    rdfs:comment "The nature or genre of the resource."@en ;
    rdfs:isDefinedBy dc: ;
    skos:note "A second property with the same name as this property has been declared in the dcterms: namespace (http://purl.org/dc/terms/).  See the Introduction to the document \"DCMI Metadata Terms\" (http://dublincore.org/documents/dcmi-terms/) for an explanation."@en .

dcterms:contributor a rdf:Property ;
    rdfs:label "Contributor"@en ;
    dcterms:description "Examples of a Contributor include a person, an organization, or a service."@en ;
    dcterms:hasVersion history:contributorT-001 ;
    dcterms:issued "2008-01-14"^^xsd:date ;
    dcterms:modified "2010-10-11"^^xsd:date ;
    rdfs:comment "An entity responsible for making contributions to the resource."@en ;
    rdfs:isDefinedBy dcterms: ;
    rdfs:range dcterms:Agent ;
    rdfs:subPropertyOf dc:contributor .

dcterms:creator a rdf:Property ;
    rdfs:label "Creator"@en ;
    dcterms:description "Examples of a Creator include a person, an organization, or a service."@en ;
    dcterms:hasVersion history:creatorT-002 ;
    dcterms:issued "2008-01-14"^^xsd:date ;
    dcterms:modified "2010-10-11"^^xsd:date ;
    rdfs:comment "An entity primarily responsible for making the resource."@en ;
    rdfs:isDefinedBy dcterms: ;
    rdfs:range dcterms:Agent ;
    rdfs:subPropertyOf dc:creator,
        dcterms:contributor ;
    owl:equivalentProperty foaf:maker .

dcterms:title a rdf:Property ;
    rdfs:label "Title"@en ;
    dcterms:hasVersion history:titleT-002 ;
    dcterms:issued "2008-01-14"^^xsd:date ;
    dcterms:modified "2010-10-11"^^xsd:date ;
    rdfs:comment "A name given to the resource."@en ;
    rdfs:isDefinedBy dcterms: ;
    rdfs:range rdfs:Literal ;
    rdfs:subPropertyOf dc:title .

crm:P105_right_held_by a rdf:Property ;
    rdfs:label "Rechte stehen zu"@de,
        "δικαίωμα κατέχεται από"@el,
        "right held by"@en,
        "droit détenu par"@fr,
        "são direitos de "@pt,
        "право принадлежит"@ru ;
    rdfs:comment """This property identifies the E39 Actor who holds the instances of E30 Right to an E72 Legal Object.
	It is a superproperty of P52 has current owner (is current owner of) because ownership is a right that is held on the owned object.
P105 right held by (has right on) is a shortcut of the fully developed path from E72 Legal Object through P104 is subject to (applies to), E30 Right, P75 possesses (is possessed by) to E39 Actor."""@en ;
    rdfs:domain crm:E72_Legal_Object ;
    rdfs:range crm:E39_Actor .

crm:P105i_has_right_on a rdf:Property ;
    rdfs:label "hat Rechte an"@de,
        "έχει δικαίωμα σε"@el,
        "has right on"@en,
        "détient un droit sur"@fr,
        "possui direitos sobre"@pt,
        "владеет правом на"@ru ;
    rdfs:domain crm:E39_Actor ;
    rdfs:range crm:E72_Legal_Object .

crm:P125_used_object_of_type a rdf:Property ;
    rdfs:label "benutzte Objekt des Typus"@de,
        "χρησιμοποίησε αντικείμενο τύπου"@el,
        "used object of type"@en,
        "a employé un objet du type"@fr,
        "usou objeto do tipo"@pt,
        "использовал объект типа"@ru ;
    rdfs:comment "This property defines the kind of objects used in an E7 Activity, when the specific instance is either unknown or not of interest, such as use of \"a hammer\"."@en ;
    rdfs:domain crm:E7_Activity ;
    rdfs:range crm:E55_Type .

crm:P125i_was_type_of_object_used_in a rdf:Property ;
    rdfs:label "Objekt des Typus ... wurde benutzt in"@de,
        "ήταν o τύπος αντικείμενου που χρησιμοποιήθηκε σε"@el,
        "was type of object used in"@en,
        "était le type d’objet employé par"@fr,
        "foi tipo do objeto usado em"@pt,
        "был типом объекта использованного в"@ru ;
    rdfs:domain crm:E55_Type ;
    rdfs:range crm:E7_Activity .

crm:P128_carries a rdf:Property ;
    rdfs:label "trägt"@de,
        "φέρει"@el,
        "carries"@en,
        "est le support de"@fr,
        "é o suporte de"@pt,
        "несет"@ru ;
    rdfs:comment """This property identifies an E73 Information Object carried by an instance of E24 Physical Man-Made Thing.
In general this would be an E84 Information Carrier P65 shows visual item (is shown by) is a specialisation of P128 carries (is carried by) which should be used for carrying visual items."""@en ;
    rdfs:domain crm:E24_Physical_Man-Made_Thing ;
    rdfs:range crm:E73_Information_Object ;
    rdfs:subPropertyOf crm:P130_shows_features_of .

crm:P128i_is_carried_by a rdf:Property ;
    rdfs:label "wird getragen von"@de,
        "φέρεται από"@el,
        "is carried by"@en,
        "a pour support"@fr,
        "é suportado por"@pt,
        "переносится посредством"@ru ;
    rdfs:domain crm:E73_Information_Object ;
    rdfs:range crm:E24_Physical_Man-Made_Thing ;
    rdfs:subPropertyOf crm:P130i_features_are_also_found_on .

crm:P2i_is_type_of a rdf:Property ;
    rdfs:label "ist Typus von"@de,
        "είναι ο τύπος του/της"@el,
        "is type of"@en,
        "est le type de"@fr,
        "é o tipo de"@pt,
        "является типом для"@ru ;
    rdfs:domain crm:E55_Type ;
    rdfs:range crm:E1_CRM_Entity .

crm:P46_is_composed_of a rdf:Property ;
    rdfs:label "ist zusammengesetzt aus"@de,
        "αποτελείται από"@el,
        "is composed of"@en,
        "est composée de"@fr,
        "é composto de"@pt,
        "составлен из"@ru ;
    rdfs:comment """This property allows instances of E18 Physical Thing to be analysed into component elements.
Component elements, since they are themselves instances of E18 Physical Thing, may be further analysed into sub-components, thereby creating a hierarchy of part decomposition. An instance of E18 Physical Thing may be shared between multiple wholes, for example two buildings may share a common wall.
This property is intended to describe specific components that are individually documented, rather than general aspects. Overall descriptions of the structure of an instance of E18 Physical Thing are captured by the P3 has note property.
The instances of E57 Materials of which an item of E18 Physical Thing is composed should be documented using P45 consists of (is incorporated in)."""@en ;
    rdfs:domain crm:E18_Physical_Thing ;
    rdfs:range crm:E18_Physical_Thing .

crm:P46i_forms_part_of a rdf:Property ;
    rdfs:label "bildet Teil von"@de,
        "αποτελεί μέρος του/της"@el,
        "forms part of"@en,
        "fait partie de"@fr,
        "faz parte de"@pt,
        "формирует часть"@ru ;
    rdfs:domain crm:E18_Physical_Thing ;
    rdfs:range crm:E18_Physical_Thing .

crm:P51_has_former_or_current_owner a rdf:Property ;
    rdfs:label "hat früheren oder derzeitigen Besitzer "@de,
        "έχει ή είχε ιδιοκτήτη"@el,
        "has former or current owner"@en,
        "est ou a été possédée par"@fr,
        "é ou foi propriedade de"@pt,
        "имеет бывшего или текущего владельца"@ru ;
    rdfs:comment """This property identifies the E39 Actor that is or has been the legal owner (i.e. title holder) of an instance of E18 Physical Thing at some time.
The distinction with P52 has current owner (is current owner of) is that P51 has former or current owner (is former or current owner of) does not indicate whether the specified owners are current. P51 has former or current owner (is former or current owner of) is a shortcut for the more detailed path from E18 Physical Thing through P24 transferred title of (changed ownership through), E8 Acquisition, P23 transferred title from (surrendered title through), or P22 transferred title to (acquired title through) to E39 Actor."""@en ;
    rdfs:domain crm:E18_Physical_Thing ;
    rdfs:range crm:E39_Actor .

crm:P51i_is_former_or_current_owner_of a rdf:Property ;
    rdfs:label "ist früherer oder derzeitiger Besitzer von"@de,
        "είναι ή ήταν ιδιοκτήτης του/της"@el,
        "is former or current owner of"@en,
        "est ou a été propriétaire de"@fr,
        "é ou foi proprietário de"@pt,
        "является бывшим или текущим владельцем для"@ru ;
    rdfs:domain crm:E39_Actor ;
    rdfs:range crm:E18_Physical_Thing .

crm:P62_depicts a rdf:Property ;
    rdfs:label "bildet ab"@de,
        "απεικονίζει"@el,
        "depicts"@en,
        "figure"@fr,
        "retrata"@pt,
        "описывает"@ru ;
    rdfs:comment """This property identifies something that is depicted by an instance of E24 Physical Man-Made Thing.
This property is a shortcut of the more fully developed path from E24 Physical Man-Made Thing through P65 shows visual item (is shown by), E36 Visual Item, P138 represents (has representation) to E1CRM Entity. P62.1 mode of depiction allows the nature of the depiction to be refined."""@en ;
    rdfs:domain crm:E24_Physical_Man-Made_Thing ;
    rdfs:range crm:E1_CRM_Entity .

crm:P62i_is_depicted_by a rdf:Property ;
    rdfs:label "wird abgebildet durch"@de,
        "απεικονίζεται σε"@el,
        "is depicted by"@en,
        "est figurée sur"@fr,
        "é retratada por"@pt,
        "описан посредством"@ru ;
    rdfs:domain crm:E1_CRM_Entity ;
    rdfs:range crm:E24_Physical_Man-Made_Thing .

crm:P94_has_created a rdf:Property ;
    rdfs:label "hat erschaffen"@de,
        "δημιούργησε"@el,
        "has created"@en,
        "a créé"@fr,
        "criou"@pt,
        "создал"@ru ;
    rdfs:comment """This property allows a conceptual E65 Creation to be linked to the E28 Conceptual Object created by it. 
It represents the act of conceiving the intellectual content of the E28 Conceptual Object. It does not represent the act of creating the first physical carrier of the E28 Conceptual Object. As an example, this is the composition of a poem, not its commitment to paper."""@en ;
    rdfs:domain crm:E65_Creation ;
    rdfs:range crm:E28_Conceptual_Object ;
    rdfs:subPropertyOf crm:P92_brought_into_existence .

crm:P94i_was_created_by a rdf:Property ;
    rdfs:label "wurde erschaffen durch"@de,
        "δημιουργήθηκε από"@el,
        "was created by"@en,
        "a été créé par"@fr,
        "foi criado por"@pt,
        "был создан посредством"@ru ;
    rdfs:domain crm:E28_Conceptual_Object ;
    rdfs:range crm:E65_Creation ;
    rdfs:subPropertyOf crm:P92i_was_brought_into_existence_by .

gn:A.ADM1 a gn:Code ;
    skos:definition "a primary administrative division of a country, such as a state in the United States"@en,
        "первоначальное политико-административное  деление, например, деление США на штаты"@ru ;
    skos:inScheme gn:A ;
    skos:notation "A.ADM1" ;
    skos:prefLabel "първостепенна административна единица"@bg,
        "first-order administrative division"@en,
        "primær administrativ inndeling"@no,
        "политико-административное деление первого порядка"@ru,
        "första ordningens administrativ avdelning"@sv .

gn:A.ADM2 a gn:Code ;
    skos:definition "a subdivision of a first-order administrative division"@en,
        "дальнейшее деление политико-административного деления первого порядка"@ru ;
    skos:inScheme gn:A ;
    skos:notation "A.ADM2" ;
    skos:prefLabel "второстепенна административна единица"@bg,
        "second-order administrative division"@en,
        "sekundær administrativ inndeling"@no,
        "политико-административное деление второго порядка"@ru,
        "andra ordningens administrativ avdelning"@sv .

gn:A.ADM3 a gn:Code ;
    skos:definition "a subdivision of a second-order administrative division"@en,
        "дальнейшее деление политико-административного деления второго порядка"@ru ;
    skos:inScheme gn:A ;
    skos:notation "A.ADM3" ;
    skos:prefLabel "третостепенна административна единица"@bg,
        "third-order administrative division"@en,
        "administrativ inndeling av tredje grad"@no,
        "политико-административное деление третьего порядка"@ru,
        "tredje ordningens administrativ avdelning"@sv .

gn:A.ADM4 a gn:Code ;
    skos:definition "a subdivision of a third-order administrative division"@en,
        "дальнейшее деление политико-административного деления третьего порядка"@ru ;
    skos:inScheme gn:A ;
    skos:notation "A.ADM4" ;
    skos:prefLabel "четвъртостепенна административна единица"@bg,
        "fourth-order administrative division"@en,
        "administrativ inndeling av fjerde grad"@no,
        "политико-административное деление четвертого порядка"@ru,
        "fjärde ordningens administrativ avdelning"@sv .

gn:A.PCLI a gn:Code ;
    skos:inScheme gn:A ;
    skos:notation "A.PCLI" ;
    skos:prefLabel "независимо политическо образувание"@bg,
        "independent political entity"@en,
        "uavhengig politisk enhet"@no,
        "независимое политическое образование"@ru,
        "oberoende politisk enhet"@sv .

gn:Map a owl:Class ;
    rdfs:label "Map"@en ;
    rdfs:comment "A Web page displaying a map"@en ;
    rdfs:subClassOf foaf:Document .

gn:Marc-Wick a foaf:Person ;
    foaf:name "Marc Wick" .

gn:WikipediaArticle a owl:Class ;
    rdfs:label "Wikipedia Article"@en ;
    rdfs:comment "A Wikipedia article"@en ;
    rdfs:subClassOf foaf:Document .

gn:countryCode a owl:DatatypeProperty ;
    rdfs:label "ISO country code"@en ;
    rdfs:comment "A two letters country code in the ISO 3166 list"@en,
        "The countryCode value for a Geoname Feature is equal to the countryCode value of the parentCountry value."@en ;
    rdfs:domain gn:Feature .

gn:featureClass a owl:ObjectProperty ;
    rdfs:label "feature class"@en ;
    rdfs:comment "The main category of the feature, as defined in geonames taxonomy."@en ;
    rdfs:domain gn:Feature ;
    rdfs:range gn:Class ;
    rdfs:subPropertyOf dcterms:type ;
    owl:propertyChainAxiom ( gn:featureCode skos:inScheme ) .

gn:geonamesID a owl:DatatypeProperty ;
    rdfs:label "geonames identifier"@en ;
    rdfs:subPropertyOf dcterms:identifier ;
    skos:historyNote "Added in version 3.1"@en .

gn:name a owl:DatatypeProperty ;
    rdfs:label "name"@en ;
    rdfs:comment "The main international name of a feature. The value has no xml:lang tag."@en ;
    rdfs:domain gn:Feature .

gn:parentADM1 a owl:ObjectProperty ;
    rdfs:label "level 1 administrative parent"@en ;
    rdfs:domain gn:Feature ;
    rdfs:range [ a owl:Restriction ;
            owl:hasValue gn:A.ADM1 ;
            owl:onProperty gn:featureCode ] ;
    rdfs:subPropertyOf gn:parentFeature .

gn:parentADM2 a owl:ObjectProperty ;
    rdfs:label "level 2 administrative parent"@en ;
    rdfs:domain gn:Feature ;
    rdfs:range [ a owl:Restriction ;
            owl:hasValue gn:A.ADM2 ;
            owl:onProperty gn:featureCode ] ;
    rdfs:subPropertyOf gn:parentFeature .

gn:parentADM3 a owl:ObjectProperty ;
    rdfs:label "level 3 administrative parent"@en ;
    rdfs:domain gn:Feature ;
    rdfs:range [ a owl:Restriction ;
            owl:hasValue gn:A.ADM3 ;
            owl:onProperty gn:featureCode ] ;
    rdfs:subPropertyOf gn:parentFeature .

gn:parentADM4 a owl:ObjectProperty ;
    rdfs:label "level 4 administrative parent"@en ;
    rdfs:domain gn:Feature ;
    rdfs:range [ a owl:Restriction ;
            owl:hasValue gn:A.ADM4 ;
            owl:onProperty gn:featureCode ] ;
    rdfs:subPropertyOf gn:parentFeature .

gn:population a owl:DatatypeProperty ;
    rdfs:label "population"@en ;
    rdfs:domain gn:Feature ;
    rdfs:range xsd:integer .

geosparql:gmlLiteral a rdfs:Datatype ;
    rdfs:label "GML Literal"@en ;
    dc:contributor "Matthew Perry" ;
    dc:creator "OGC GeoSPARQL 1.0 Standard Working Group" ;
    dc:date "2011-06-16"^^xsd:date ;
    dc:description """      A GML serialization of a geometry object.
    """@en ;
    rdfs:comment """      A GML serialization of a geometry object.
    """@en ;
    rdfs:isDefinedBy <http://www.opengis.net/ont/geosparql>,
        <http://www.opengis.net/spec/geosparql/1.0> ;
    skos:definition """      A GML serialization of a geometry object.
    """@en ;
    skos:prefLabel "GML Literal"@en .

geosparql:hasGeometry a owl:ObjectProperty ;
    rdfs:label "hasGeometry"@en ;
    dc:contributor "Matthew Perry" ;
    dc:creator "OGC GeoSPARQL 1.0 Standard Working Group" ;
    dc:date "2011-06-16"^^xsd:date ;
    dc:description """      A spatial representation for a given feature.
    """@en ;
    rdfs:comment """      A spatial representation for a given feature.
    """@en ;
    rdfs:domain geosparql:Feature ;
    rdfs:isDefinedBy <http://www.opengis.net/ont/geosparql>,
        <http://www.opengis.net/spec/geosparql/1.0> ;
    rdfs:range geosparql:Geometry ;
    skos:definition """      A spatial representation for a given feature.
    """@en ;
    skos:prefLabel "hasGeometry"@en .

geosparql:wktLiteral a rdfs:Datatype ;
    rdfs:label "Well-known Text Literal"@en ;
    dc:contributor "Matthew Perry" ;
    dc:creator "OGC GeoSPARQL 1.0 Standard Working Group" ;
    dc:date "2011-06-16"^^xsd:date ;
    dc:description """      A Well-known Text serialization of a geometry object.
    """@en ;
    rdfs:comment """      A Well-known Text serialization of a geometry object.
    """@en ;
    rdfs:isDefinedBy <http://www.opengis.net/ont/geosparql>,
        <http://www.opengis.net/spec/geosparql/1.0> ;
    skos:definition """      A Well-known Text serialization of a geometry object.
    """@en ;
    skos:prefLabel "Well-known Text Literal"@en .

rdfs:seeAlso a rdf:Property ;
    rdfs:label "seeAlso",
        "geographic identifier"@en ;
    dcterms:identifier "rdfs:seeAlso" ;
    vann:usageNote "Used in the ISA Programme Location Core Vocabulary to provide a URI that identifies the location. This should be expressed using the rdfs:seeAlso property unless the identifier is already the subject of the description. Examples include URIs from GeoNames.org and DBpedia such as http://dbpedia.org/resource/ISO_3166-2:XX where XX is the ISO 3166 two character code for a country."@en ;
    rdfs:comment "Further information about the subject resource.",
        "rdfs:seeAlso fully represents the ISA Programme Location Core Vocabulary concept of a geographic identifier."@en ;
    rdfs:domain rdfs:Resource ;
    rdfs:isDefinedBy rdfs: ;
    rdfs:range rdfs:Resource ;
    swvocab:term_status "unstable"@en .

<http://www.w3.org/2002/07/owl> a owl:Ontology ;
    dc:title "The OWL 2 Schema vocabulary (OWL 2)" ;
    rdfs:comment """\r
  This ontology partially describes the built-in classes and\r
  properties that together form the basis of the RDF/XML syntax of OWL 2.\r
  The content of this ontology is based on Tables 6.1 and 6.2\r
  in Section 6.4 of the OWL 2 RDF-Based Semantics specification,\r
  available at http://www.w3.org/TR/owl2-rdf-based-semantics/.\r
  Please note that those tables do not include the different annotations\r
  (labels, comments and rdfs:isDefinedBy links) used in this file.\r
  Also note that the descriptions provided in this ontology do not\r
  provide a complete and correct formal description of either the syntax\r
  or the semantics of the introduced terms (please see the OWL 2\r
  recommendations for the complete and normative specifications).\r
  Furthermore, the information provided by this ontology may be\r
  misleading if not used with care. This ontology SHOULD NOT be imported\r
  into OWL ontologies. Importing this file into an OWL 2 DL ontology\r
  will cause it to become an OWL 2 Full ontology and may have other,\r
  unexpected, consequences.\r
   """ ;
    rdfs:isDefinedBy <http://www.w3.org/TR/owl2-mapping-to-rdf/>,
        <http://www.w3.org/TR/owl2-rdf-based-semantics/>,
        <http://www.w3.org/TR/owl2-syntax/> ;
    rdfs:seeAlso owl2-rdf-based-semantics:table-axiomatic-classes,
        owl2-rdf-based-semantics:table-axiomatic-properties ;
    owl:imports <http://www.w3.org/2000/01/rdf-schema> ;
    owl:versionIRI <http://www.w3.org/2002/07/owl> ;
    owl:versionInfo "$Date: 2009/11/15 10:54:12 $" ;
    ns3:namespaceTransformation <http://dev.w3.org/cvsweb/2009/owl-grddl/owx2rdf.xsl> .

wgs84:lat a rdf:Property ;
    rdfs:label "latitude" ;
    rdfs:comment "The WGS84 latitude of a SpatialThing (decimal degrees)." ;
    rdfs:domain wgs84:SpatialThing .

wgs84:long a rdf:Property ;
    rdfs:label "longitude" ;
    rdfs:comment "The WGS84 longitude of a SpatialThing (decimal degrees)." ;
    rdfs:domain wgs84:SpatialThing .

skos:OrderedCollection a owl:Class ;
    rdfs:label "Ordered Collection"@en ;
    rdfs:isDefinedBy <http://www.w3.org/2004/02/skos/core> ;
    rdfs:subClassOf skos:Collection ;
    skos:definition "An ordered collection of concepts, where both the grouping and the ordering are meaningful."@en ;
    skos:scopeNote "Ordered collections can be used where you would like a set of concepts to be displayed in a specific order, and optionally under a 'node label'."@en .

skos:altLabel a rdf:Property,
        owl:AnnotationProperty ;
    rdfs:label "alternative label"@en ;
    rdfs:comment "The range of skos:altLabel is the class of RDF plain literals."@en,
        "skos:prefLabel, skos:altLabel and skos:hiddenLabel are pairwise disjoint properties."@en ;
    rdfs:isDefinedBy <http://www.w3.org/2004/02/skos/core> ;
    rdfs:subPropertyOf rdfs:label ;
    skos:definition "An alternative lexical label for a resource."@en ;
    skos:example "Acronyms, abbreviations, spelling variants, and irregular plural/singular forms may be included among the alternative labels for a concept. Mis-spelled terms are normally included as hidden labels (see skos:hiddenLabel)."@en .

skos:broadMatch a rdf:Property,
        owl:ObjectProperty ;
    rdfs:label "has broader match"@en ;
    rdfs:isDefinedBy <http://www.w3.org/2004/02/skos/core> ;
    rdfs:subPropertyOf skos:broader,
        skos:mappingRelation ;
    owl:inverseOf skos:narrowMatch ;
    skos:definition "skos:broadMatch is used to state a hierarchical mapping link between two conceptual resources in different concept schemes."@en .

skos:closeMatch a rdf:Property,
        owl:ObjectProperty,
        owl:SymmetricProperty ;
    rdfs:label "has close match"@en ;
    rdfs:isDefinedBy <http://www.w3.org/2004/02/skos/core> ;
    rdfs:subPropertyOf skos:mappingRelation ;
    skos:definition "skos:closeMatch is used to link two concepts that are sufficiently similar that they can be used interchangeably in some information retrieval applications. In order to avoid the possibility of \"compound errors\" when combining mappings across more than two concept schemes, skos:closeMatch is not declared to be a transitive property."@en .

skos:hasTopConcept a rdf:Property,
        owl:ObjectProperty ;
    rdfs:label "has top concept"@en ;
    rdfs:domain skos:ConceptScheme ;
    rdfs:isDefinedBy <http://www.w3.org/2004/02/skos/core> ;
    rdfs:range skos:Concept ;
    owl:inverseOf skos:topConceptOf ;
    skos:definition "Relates, by convention, a concept scheme to a concept which is topmost in the broader/narrower concept hierarchies for that scheme, providing an entry point to these hierarchies."@en .

skos:narrowMatch a rdf:Property,
        owl:ObjectProperty ;
    rdfs:label "has narrower match"@en ;
    rdfs:isDefinedBy <http://www.w3.org/2004/02/skos/core> ;
    rdfs:subPropertyOf skos:mappingRelation,
        skos:narrower ;
    owl:inverseOf skos:broadMatch ;
    skos:definition "skos:narrowMatch is used to state a hierarchical mapping link between two conceptual resources in different concept schemes."@en .

skos:prefLabel a rdf:Property,
        owl:AnnotationProperty,
        owl:DatatypeProperty ;
    rdfs:label "preferred label"@en ;
    rdfs:comment "A resource has no more than one value of skos:prefLabel per language tag, and no more than one value of skos:prefLabel without language tag."@en,
        "The range of skos:prefLabel is the class of RDF plain literals."@en,
        """skos:prefLabel, skos:altLabel and skos:hiddenLabel are pairwise
      disjoint properties."""@en ;
    rdfs:isDefinedBy <http://www.w3.org/2004/02/skos/core> ;
    rdfs:subPropertyOf rdfs:label ;
    skos:definition "The preferred lexical label for a resource, in a given language."@en .

skos:related a rdf:Property,
        owl:ObjectProperty,
        owl:SymmetricProperty ;
    rdfs:label "has related"@en ;
    rdfs:comment "skos:related is disjoint with skos:broaderTransitive"@en ;
    rdfs:isDefinedBy <http://www.w3.org/2004/02/skos/core> ;
    rdfs:subPropertyOf skos:semanticRelation ;
    skos:definition "Relates a concept to a concept with which there is an associative semantic relationship."@en .

skos:topConceptOf a rdf:Property,
        owl:ObjectProperty ;
    rdfs:label "is top concept in scheme"@en ;
    rdfs:domain skos:Concept ;
    rdfs:isDefinedBy <http://www.w3.org/2004/02/skos/core> ;
    rdfs:range skos:ConceptScheme ;
    rdfs:subPropertyOf skos:inScheme ;
    owl:inverseOf skos:hasTopConcept ;
    skos:definition "Relates a concept to the concept scheme that it is a top level concept of."@en .

<http://www.w3.org/ns/locn.html> rdfs:label "HTML version of the ISA Programme Location Core Vocabulary"@en ;
    dcat:mediaType "text/html"^^dcterms:IMT .

<http://www.w3.org/ns/locn.rdf> rdfs:label "RDF/XML version of the ISA Programme Location Core Vocabulary"@en ;
    dcterms:format data:RDF_XML ;
    dcat:mediaType "application/rdf+xml"^^dcterms:IMT .

<http://www.w3.org/ns/locn.svg> rdfs:label "Class and property diagram of the LOCN vocabulary" .

<http://www.w3.org/ns/locn.ttl> rdfs:label "Turtle version of the ISA Programme Location Core Vocabulary"@en ;
    dcterms:format data:Turtle ;
    dcat:mediaType "text/turtle"^^dcterms:IMT .

foaf:based_near a rdf:Property,
        owl:ObjectProperty ;
    rdfs:label "based near" ;
    rdfs:comment "A location that something is based near, for some broadly human notion of near." ;
    rdfs:domain wgs84:SpatialThing ;
    rdfs:isDefinedBy foaf: ;
    rdfs:range wgs84:SpatialThing ;
    swvocab:term_status "testing" .

foaf:depicts a rdf:Property,
        owl:ObjectProperty ;
    rdfs:label "depicts" ;
    rdfs:comment "A thing depicted in this representation." ;
    rdfs:domain foaf:Image ;
    rdfs:isDefinedBy foaf: ;
    rdfs:range owl:Thing ;
    owl:inverseOf foaf:depiction ;
    swvocab:term_status "testing" .

foaf:made a rdf:Property,
        owl:ObjectProperty ;
    rdfs:label "made" ;
    rdfs:comment "Something that was made by this agent." ;
    rdfs:domain foaf:Agent ;
    rdfs:isDefinedBy foaf: ;
    rdfs:range owl:Thing ;
    owl:inverseOf foaf:maker ;
    swvocab:term_status "stable" .

foaf:primaryTopic a rdf:Property,
        owl:FunctionalProperty,
        owl:ObjectProperty ;
    rdfs:label "primary topic" ;
    rdfs:comment "The primary topic of some page or document." ;
    rdfs:domain foaf:Document ;
    rdfs:isDefinedBy foaf: ;
    rdfs:range owl:Thing ;
    owl:inverseOf foaf:isPrimaryTopicOf ;
    swvocab:term_status "stable" .

foaf:topic a rdf:Property,
        owl:ObjectProperty ;
    rdfs:label "topic" ;
    rdfs:comment "A topic of some page or document." ;
    rdfs:domain foaf:Document ;
    rdfs:isDefinedBy foaf: ;
    rdfs:range owl:Thing ;
    owl:inverseOf foaf:page ;
    swvocab:term_status "testing" .

licence:isa-open-metadata-licence-v11 ns:attributionName "European Commission"@en ;
    ns:attributionURL eu: ;
    dcterms:title "ISA Open Metadata Licence v1.1" .

<https://joinup.ec.europa.eu/node/43160> dcterms:title "Process and Methodology for Developing Core Vocabularies" .

crmeh:EHE2010_DepictionEvent a owl:Class ;
    rdfs:label "Depiction Event"@en ;
    rdfs:comment "This describes the act of documenting Physical Stuff by images or drawings of visible physical features, eventually enriched by grid references. The resulting photo or drawing \"documents\" the depicted stuff"@en ;
    rdfs:isDefinedBy crmeh:CRMEH ;
    rdfs:subClassOf crm:E65_Creation ;
    owl:sameAs crmeh:EHE2010 ;
    skos:notation "EHE2010" .

dc:identifier a rdf:Property ;
    rdfs:label "Identifier"@en ;
    dcterms:description "Recommended best practice is to identify the resource by means of a string conforming to a formal identification system. "@en ;
    dcterms:hasVersion history:identifier-006 ;
    dcterms:issued "1999-07-02"^^xsd:date ;
    dcterms:modified "2008-01-14"^^xsd:date ;
    rdfs:comment "An unambiguous reference to the resource within a given context."@en ;
    rdfs:isDefinedBy dc: ;
    skos:note "A second property with the same name as this property has been declared in the dcterms: namespace (http://purl.org/dc/terms/).  See the Introduction to the document \"DCMI Metadata Terms\" (http://dublincore.org/documents/dcmi-terms/) for an explanation."@en .

dc:title a rdf:Property,
        owl:AnnotationProperty ;
    rdfs:label "Title"@en ;
    dcterms:hasVersion history:title-006 ;
    dcterms:issued "1999-07-02"^^xsd:date ;
    dcterms:modified "2008-01-14"^^xsd:date ;
    rdfs:comment "A name given to the resource."@en ;
    rdfs:isDefinedBy dc: ;
    skos:note "A second property with the same name as this property has been declared in the dcterms: namespace (http://purl.org/dc/terms/).  See the Introduction to the document \"DCMI Metadata Terms\" (http://dublincore.org/documents/dcmi-terms/) for an explanation."@en .

dcterms:audience a rdf:Property ;
    rdfs:label "Audience"@en ;
    dcterms:hasVersion history:audience-003 ;
    dcterms:issued "2001-05-21"^^xsd:date ;
    dcterms:modified "2008-01-14"^^xsd:date ;
    rdfs:comment "A class of entity for whom the resource is intended or useful."@en ;
    rdfs:isDefinedBy dcterms: ;
    rdfs:range dcterms:AgentClass .

dcterms:coverage a rdf:Property ;
    rdfs:label "Coverage"@en ;
    dcterms:description "Spatial topic and spatial applicability may be a named place or a location specified by its geographic coordinates. Temporal topic may be a named period, date, or date range. A jurisdiction may be a named administrative entity or a geographic place to which the resource applies. Recommended best practice is to use a controlled vocabulary such as the Thesaurus of Geographic Names [TGN]. Where appropriate, named places or time periods can be used in preference to numeric identifiers such as sets of coordinates or date ranges."@en ;
    dcterms:hasVersion history:coverageT-001 ;
    dcterms:issued "2008-01-14"^^xsd:date ;
    dcterms:modified "2008-01-14"^^xsd:date ;
    rdfs:comment "The spatial or temporal topic of the resource, the spatial applicability of the resource, or the jurisdiction under which the resource is relevant."@en ;
    rdfs:isDefinedBy dcterms: ;
    rdfs:range dcterms:LocationPeriodOrJurisdiction ;
    rdfs:subPropertyOf dc:coverage .

dcterms:description a rdf:Property ;
    rdfs:label "Description"@en ;
    dcterms:description "Description may include but is not limited to: an abstract, a table of contents, a graphical representation, or a free-text account of the resource."@en ;
    dcterms:hasVersion history:descriptionT-001 ;
    dcterms:issued "2008-01-14"^^xsd:date ;
    dcterms:modified "2008-01-14"^^xsd:date ;
    rdfs:comment "An account of the resource."@en ;
    rdfs:isDefinedBy dcterms: ;
    rdfs:subPropertyOf dc:description .

dcterms:format a rdf:Property ;
    rdfs:label "Format"@en ;
    dcterms:description "Examples of dimensions include size and duration. Recommended best practice is to use a controlled vocabulary such as the list of Internet Media Types [MIME]."@en ;
    dcterms:hasVersion history:formatT-001 ;
    dcterms:issued "2008-01-14"^^xsd:date ;
    dcterms:modified "2008-01-14"^^xsd:date ;
    rdfs:comment "The file format, physical medium, or dimensions of the resource."@en ;
    rdfs:isDefinedBy dcterms: ;
    rdfs:range dcterms:MediaTypeOrExtent ;
    rdfs:subPropertyOf dc:format .

dcterms:identifier a rdf:Property ;
    rdfs:label "Identifier"@en ;
    dcterms:description "Recommended best practice is to identify the resource by means of a string conforming to a formal identification system. "@en ;
    dcterms:hasVersion history:identifierT-001 ;
    dcterms:issued "2008-01-14"^^xsd:date ;
    dcterms:modified "2008-01-14"^^xsd:date ;
    rdfs:comment "An unambiguous reference to the resource within a given context."@en ;
    rdfs:isDefinedBy dcterms: ;
    rdfs:range rdfs:Literal ;
    rdfs:subPropertyOf dc:identifier .

dcterms:rights a rdf:Property ;
    rdfs:label "Rights"@en ;
    dcterms:description "Typically, rights information includes a statement about various property rights associated with the resource, including intellectual property rights."@en ;
    dcterms:hasVersion history:rightsT-001 ;
    dcterms:issued "2008-01-14"^^xsd:date ;
    dcterms:modified "2008-01-14"^^xsd:date ;
    rdfs:comment "Information about rights held in and over the resource."@en ;
    rdfs:isDefinedBy dcterms: ;
    rdfs:range dcterms:RightsStatement ;
    rdfs:subPropertyOf dc:rights .

dcterms:type a rdf:Property ;
    rdfs:label "Type"@en ;
    dcterms:description "Recommended best practice is to use a controlled vocabulary such as the DCMI Type Vocabulary [DCMITYPE]. To describe the file format, physical medium, or dimensions of the resource, use the Format element."@en ;
    dcterms:hasVersion history:typeT-001 ;
    dcterms:issued "2008-01-14"^^xsd:date ;
    dcterms:modified "2008-01-14"^^xsd:date ;
    rdfs:comment "The nature or genre of the resource."@en ;
    rdfs:isDefinedBy dcterms: ;
    rdfs:range rdfs:Class ;
    rdfs:subPropertyOf dc:type .

crm:P130_shows_features_of a rdf:Property ;
    rdfs:label "zeigt Merkmale von"@de,
        "παρουσιάζει χαρακτηριστικά του/της"@el,
        "shows features of"@en,
        "présente des caractéristiques de"@fr,
        "apresenta características de"@pt,
        "демонстрирует признаки"@ru ;
    rdfs:comment """This property generalises the notions of  "copy of" and "similar to" into a dynamic, asymmetric relationship, where the domain expresses the derivative, if such a direction can be established.
Otherwise, the relationship is symmetric. It is a short-cut of P15 was influenced by (influenced) in a creation or production, if such a reason for the similarity can be verified. Moreover it expresses similarity in cases that can be stated between two objects only, without historical knowledge about its reasons."""@en ;
    rdfs:domain crm:E70_Thing ;
    rdfs:range crm:E70_Thing .

crm:P130i_features_are_also_found_on a rdf:Property ;
    rdfs:label "Merkmale auch auf"@de,
        "χαρακτηριστικά του βρίσκονται επίσης σε"@el,
        "features are also found on"@en,
        "a des caractéristiques se trouvant aussi sur"@fr,
        "características são também encontradas em"@pt,
        "признаки также найдены на"@ru ;
    rdfs:domain crm:E70_Thing ;
    rdfs:range crm:E70_Thing .

crm:P2_has_type a rdf:Property ;
    rdfs:label "hat den Typus"@de,
        "έχει τύπο"@el,
        "has type"@en,
        "est de type"@fr,
        "é do tipo"@pt,
        "имеет тип"@ru ;
    rdfs:comment """This property allows sub typing of CRM entities - a form of specialisation – through the use of a terminological hierarchy, or thesaurus. 
The CRM is intended to focus on the high-level entities and relationships needed to describe data structures. Consequently, it does not specialise entities any further than is required for this immediate purpose. However, entities in the isA hierarchy of the CRM may by specialised into any number of sub entities, which can be defined in the E55 Type hierarchy. E51 Contact Point, for example, may be specialised into “e-mail address”, “telephone number”, “post office box”, “URL” etc. none of which figures explicitly in the CRM hierarchy. Sub typing obviously requires consistency between the meaning of the terms assigned and the more general intent of the CRM entity in question."""@en ;
    rdfs:domain crm:E1_CRM_Entity ;
    rdfs:range crm:E55_Type .

crm:P3_has_note a rdf:Property ;
    rdfs:label "hat Anmerkung"@de,
        "έχει επεξήγηση"@el,
        "has note"@en,
        "a pour note"@fr,
        "tem nota"@pt,
        "имеет примечание"@ru ;
    rdfs:comment """This property is a container for all informal descriptions about an object that have not been expressed in terms of CRM constructs. 
In particular it captures the characterisation of the item itself, its internal structures, appearance etc.
Like property P2 has type (is type of), this property is a consequence of the restricted focus of the CRM. The aim is not to capture, in a structured form, everything that can be said about an item; indeed, the CRM formalism is not regarded as sufficient to express everything that can be said. Good practice requires use of distinct note fields for different aspects of a characterisation. The P3.1 has type property of P3 has note allows differentiation of specific notes, e.g. “construction”, “decoration” etc. 
An item may have many notes, but a note is attached to a specific item."""@en ;
    rdfs:domain crm:E1_CRM_Entity ;
    rdfs:range rdfs:Literal .

crm:P49_has_former_or_current_keeper a rdf:Property ;
    rdfs:label "hat früheren oder derzeitigen Betreuer"@de,
        "είναι ή ήταν στην κατοχή του"@el,
        "has former or current keeper"@en,
        "est ou a été détenu par"@fr,
        "é ou foi guardada por"@pt,
        "имеет бывшего или текущего смотрителя"@ru ;
    rdfs:comment """This property identifies the E39 Actor or Actors who have or have had custody of an instance of E18 Physical Thing at some time. 
The distinction with P50 has current keeper (is current keeper of) is that P49 has former or current keeper (is former or current keeper of) leaves open the question as to whether the specified keepers are current. 
P49 has former or current keeper (is former or current keeper of) is a shortcut for the more detailed path from E18 Physical Thing through P30 transferred custody of (custody transferred through), E10 Transfer of Custody, P28 custody surrendered by (surrendered custody through) or P29 custody received by (received custody through) to E39 Actor."""@en ;
    rdfs:domain crm:E18_Physical_Thing ;
    rdfs:range crm:E39_Actor .

crm:P49i_is_former_or_current_keeper_of a rdf:Property ;
    rdfs:label "ist früherer oder derzeitiger Betreuer von"@de,
        "κατέχει ή κατείχε"@el,
        "is former or current keeper of"@en,
        "est ou a été détenteur de"@fr,
        "é ou foi guardador de"@pt,
        "является бывшим или текущим смотрителем для"@ru ;
    rdfs:domain crm:E39_Actor ;
    rdfs:range crm:E18_Physical_Thing .

crm:P53_has_former_or_current_location a rdf:Property ;
    rdfs:label "hat früheren oder derzeitigen Standort"@de,
        "βρίσκεται ή βρισκόταν σε"@el,
        "has former or current location"@en,
        "a ou a eu pour localisation"@fr,
        "é ou foi localizada em"@pt,
        "имеет текущее или бывшее местоположение"@ru ;
    rdfs:comment """This property allows an instance of E53 Place to be associated as the former or current location of an instance of E18 Physical Thing.
In the case of E19 Physical Objects, the property does not allow any indication of the Time-Span during which the Physical Object was located at this Place, nor if this is the current location.
In the case of immobile objects, the Place would normally correspond to the Place of creation.
P53 has former or current location (is former or current location of) is a shortcut. A more detailed representation can make use of the fully developed (i.e. indirect) path from E19 Physical Object through P25 moved (moved by), E9 Move, P26 moved to (was destination of) or P27 moved from (was origin of) to E53 Place."""@en ;
    rdfs:domain crm:E18_Physical_Thing ;
    rdfs:range crm:E53_Place .

crm:P53i_is_former_or_current_location_of a rdf:Property ;
    rdfs:label "ist früherer oder derzeitiger Standort von"@de,
        "είναι ή ήταν θέση του"@el,
        "is former or current location of"@en,
        "est ou a été localisation de"@fr,
        "é ou foi localização de"@pt,
        "является текущим или бывшим местоположением для"@ru ;
    rdfs:domain crm:E53_Place ;
    rdfs:range crm:E18_Physical_Thing .

crm:P7_took_place_at a rdf:Property ;
    rdfs:label "fand statt in"@de,
        "έλαβε χώρα σε"@el,
        "took place at"@en,
        "a eu lieu dans"@fr,
        "ocorreu em"@pt,
        "совершался на"@ru ;
    rdfs:comment """This property describes the spatial location of an instance of E4 Period. 
The related E53 Place should be seen as an approximation of the geographical area within which the phenomena that characterise the period in question occurred. P7took place at (witnessed) does not convey any meaning other than spatial positioning (generally on the surface of the earth).  For example, the period “R?volution fran?aise” can be said to have taken place in “France”, the “Victorian” period, may be said to have taken place in “Britain” and its colonies, as well as other parts of Europe and north America.
A period can take place at multiple locations."""@en ;
    rdfs:domain crm:E4_Period ;
    rdfs:range crm:E53_Place .

crm:P7i_witnessed a rdf:Property ;
    rdfs:label "bezeugte"@de,
        "υπήρξε τόπος του"@el,
        "witnessed"@en,
        "a été témoin de"@fr,
        "testemunhou"@pt,
        "был местом совершения"@ru ;
    rdfs:domain crm:E53_Place ;
    rdfs:range crm:E4_Period .

geosparql:hasSerialization a owl:DatatypeProperty ;
    rdfs:label "has serialization"@en ;
    dc:contributor "Matthew Perry" ;
    dc:creator "OGC GeoSPARQL 1.0 Standard Working Group" ;
    dc:date "2011-06-16"^^xsd:date ;
    dc:description """      Connects a geometry object with its text-based serialization.
    """@en ;
    rdfs:comment """      Connects a geometry object with its text-based serialization.
    """@en ;
    rdfs:domain geosparql:Geometry ;
    rdfs:isDefinedBy <http://www.opengis.net/ont/geosparql>,
        <http://www.opengis.net/spec/geosparql/1.0> ;
    rdfs:range rdfs:Literal ;
    skos:definition """      Connects a geometry object with its text-based serialization.
    """@en ;
    skos:prefLabel "has serialization"@en .

() a rdf:List ;
    rdfs:label "nil" ;
    rdfs:comment "The empty list, with no items in it. If the rest of a list is nil then the list has no more items in it." ;
    rdfs:isDefinedBy rdf: .

skos:broader a rdf:Property,
        owl:ObjectProperty ;
    rdfs:label "has broader"@en ;
    rdfs:comment "Broader concepts are typically rendered as parents in a concept hierarchy (tree)."@en ;
    rdfs:isDefinedBy <http://www.w3.org/2004/02/skos/core> ;
    rdfs:subPropertyOf skos:broaderTransitive ;
    owl:inverseOf skos:narrower ;
    skos:definition "Relates a concept to a concept that is more general in meaning."@en ;
    skos:scopeNote "By convention, skos:broader is only used to assert an immediate (i.e. direct) hierarchical link between two conceptual resources."@en .

skos:broaderTransitive a rdf:Property,
        owl:ObjectProperty,
        owl:TransitiveProperty ;
    rdfs:label "has broader transitive"@en ;
    rdfs:isDefinedBy <http://www.w3.org/2004/02/skos/core> ;
    rdfs:subPropertyOf skos:semanticRelation ;
    owl:inverseOf skos:narrowerTransitive ;
    skos:definition "skos:broaderTransitive is a transitive superproperty of skos:broader." ;
    skos:scopeNote "By convention, skos:broaderTransitive is not used to make assertions. Rather, the properties can be used to draw inferences about the transitive closure of the hierarchical relation, which is useful e.g. when implementing a simple query expansion algorithm in a search application."@en .

skos:inScheme a rdf:Property,
        owl:ObjectProperty ;
    rdfs:label "is in scheme"@en ;
    rdfs:isDefinedBy <http://www.w3.org/2004/02/skos/core> ;
    rdfs:range skos:ConceptScheme ;
    skos:definition "Relates a resource (for example a concept) to a concept scheme in which it is included."@en ;
    skos:scopeNote "A concept may be a member of more than one concept scheme."@en .

skos:narrower a rdf:Property,
        owl:ObjectProperty ;
    rdfs:label "has narrower"@en ;
    rdfs:comment "Narrower concepts are typically rendered as children in a concept hierarchy (tree)."@en ;
    rdfs:isDefinedBy <http://www.w3.org/2004/02/skos/core> ;
    rdfs:subPropertyOf skos:narrowerTransitive ;
    owl:inverseOf skos:broader ;
    skos:definition "Relates a concept to a concept that is more specific in meaning."@en ;
    skos:scopeNote "By convention, skos:broader is only used to assert an immediate (i.e. direct) hierarchical link between two conceptual resources."@en .

skos:narrowerTransitive a rdf:Property,
        owl:ObjectProperty,
        owl:TransitiveProperty ;
    rdfs:label "has narrower transitive"@en ;
    rdfs:isDefinedBy <http://www.w3.org/2004/02/skos/core> ;
    rdfs:subPropertyOf skos:semanticRelation ;
    owl:inverseOf skos:broaderTransitive ;
    skos:definition "skos:narrowerTransitive is a transitive superproperty of skos:narrower." ;
    skos:scopeNote "By convention, skos:narrowerTransitive is not used to make assertions. Rather, the properties can be used to draw inferences about the transitive closure of the hierarchical relation, which is useful e.g. when implementing a simple query expansion algorithm in a search application."@en .

foaf:depiction a rdf:Property,
        owl:ObjectProperty ;
    rdfs:label "depiction" ;
    rdfs:comment "A depiction of some thing." ;
    rdfs:domain owl:Thing ;
    rdfs:isDefinedBy foaf: ;
    rdfs:range foaf:Image ;
    owl:inverseOf foaf:depicts ;
    swvocab:term_status "testing" .

foaf:maker a rdf:Property,
        owl:ObjectProperty ;
    rdfs:label "maker" ;
    rdfs:comment "An agent that  made this thing." ;
    rdfs:domain owl:Thing ;
    rdfs:isDefinedBy foaf: ;
    rdfs:range foaf:Agent ;
    owl:equivalentProperty dcterms:creator ;
    owl:inverseOf foaf:made ;
    swvocab:term_status "stable" .

crmeh:EHE0006_GroupStuff a owl:Class ;
    rdfs:label "Group Stuff"@en ;
    rdfs:comment "The process of grouping draws together the stuff found in multiple contexts according to some commonality of observed properties. As such, by grouping together a collection of post-hole cuts to form a sub-group witnessing the creation of a post-built structure, we are defining a new feature that represents said structure. The grouped Context Stuff may only be a part of the overall structure the Group is intended to represent. As such, it may cover even a larger space than the constituent contexts (e.g. in some unexcavated areas)"@en ;
    rdfs:isDefinedBy crmeh:CRMEH ;
    rdfs:subClassOf crm:E18_Physical_Thing ;
    owl:sameAs crmeh:EHE0006 ;
    skos:notation "EHE0006" .

dc:coverage a rdf:Property ;
    rdfs:label "Coverage"@en ;
    dcterms:description "Spatial topic and spatial applicability may be a named place or a location specified by its geographic coordinates. Temporal topic may be a named period, date, or date range. A jurisdiction may be a named administrative entity or a geographic place to which the resource applies. Recommended best practice is to use a controlled vocabulary such as the Thesaurus of Geographic Names [TGN]. Where appropriate, named places or time periods can be used in preference to numeric identifiers such as sets of coordinates or date ranges."@en ;
    dcterms:hasVersion history:coverage-006 ;
    dcterms:issued "1999-07-02"^^xsd:date ;
    dcterms:modified "2008-01-14"^^xsd:date ;
    rdfs:comment "The spatial or temporal topic of the resource, the spatial applicability of the resource, or the jurisdiction under which the resource is relevant."@en ;
    rdfs:isDefinedBy dc: ;
    skos:note "A second property with the same name as this property has been declared in the dcterms: namespace (http://purl.org/dc/terms/).  See the Introduction to the document \"DCMI Metadata Terms\" (http://dublincore.org/documents/dcmi-terms/) for an explanation."@en .

dc:description a rdf:Property,
        owl:AnnotationProperty ;
    rdfs:label "Description"@en ;
    dcterms:description "Description may include but is not limited to: an abstract, a table of contents, a graphical representation, or a free-text account of the resource."@en ;
    dcterms:hasVersion history:description-006 ;
    dcterms:issued "1999-07-02"^^xsd:date ;
    dcterms:modified "2008-01-14"^^xsd:date ;
    rdfs:comment "An account of the resource."@en ;
    rdfs:isDefinedBy dc: ;
    skos:note "A second property with the same name as this property has been declared in the dcterms: namespace (http://purl.org/dc/terms/).  See the Introduction to the document \"DCMI Metadata Terms\" (http://dublincore.org/documents/dcmi-terms/) for an explanation."@en .

dc:format a rdf:Property ;
    rdfs:label "Format"@en ;
    dcterms:description "Examples of dimensions include size and duration. Recommended best practice is to use a controlled vocabulary such as the list of Internet Media Types [MIME]."@en ;
    dcterms:hasVersion history:format-007 ;
    dcterms:issued "1999-07-02"^^xsd:date ;
    dcterms:modified "2008-01-14"^^xsd:date ;
    rdfs:comment "The file format, physical medium, or dimensions of the resource."@en ;
    rdfs:isDefinedBy dc: ;
    skos:note "A second property with the same name as this property has been declared in the dcterms: namespace (http://purl.org/dc/terms/).  See the Introduction to the document \"DCMI Metadata Terms\" (http://dublincore.org/documents/dcmi-terms/) for an explanation."@en .

dc:rights a rdf:Property ;
    rdfs:label "Rights"@en ;
    dcterms:description "Typically, rights information includes a statement about various property rights associated with the resource, including intellectual property rights."@en ;
    dcterms:hasVersion history:rights-006 ;
    dcterms:issued "1999-07-02"^^xsd:date ;
    dcterms:modified "2008-01-14"^^xsd:date ;
    rdfs:comment "Information about rights held in and over the resource."@en ;
    rdfs:isDefinedBy dc: ;
    skos:note "A second property with the same name as this property has been declared in the dcterms: namespace (http://purl.org/dc/terms/).  See the Introduction to the document \"DCMI Metadata Terms\" (http://dublincore.org/documents/dcmi-terms/) for an explanation."@en .

crm:P140_assigned_attribute_to a rdf:Property ;
    rdfs:label "wies Merkmal zu"@de,
        "απέδωσε ιδιότητα σε"@el,
        "assigned attribute to"@en,
        "a affecté un attribut à"@fr,
        "atribuiu atributo para"@pt,
        "присвоил атрибут для"@ru ;
    rdfs:comment "This property indicates the item to which an attribute or relation is assigned. "@en ;
    rdfs:domain crm:E13_Attribute_Assignment ;
    rdfs:range crm:E1_CRM_Entity .

crm:P140i_was_attributed_by a rdf:Property ;
    rdfs:label "bekam Merkmal zugewiesen durch"@de,
        "χαρακτηρίστηκε από"@el,
        "was attributed by"@en,
        "a reçu un attribut par"@fr,
        "foi atribuído por"@pt,
        "получил атрибут посредством"@ru ;
    rdfs:domain crm:E1_CRM_Entity ;
    rdfs:range crm:E13_Attribute_Assignment .

crm:P16_used_specific_object a rdf:Property ;
    rdfs:label "benutzte das bestimmte Objekt"@de,
        "χρησιμοποίησε αντικείμενο"@el,
        "used specific object"@en,
        "a utilisé l'objet spécifique"@fr,
        "usou objeto específico"@pt,
        "использовал особый объект"@ru ;
    rdfs:comment """This property describes the use of material or immaterial things in a way essential to the performance or the outcome of an E7 Activity. 
This property typically applies to tools, instruments, moulds, raw materials and items embedded in a product. It implies that the presence of the object in question was a necessary condition for the action. For example, the activity of writing this text required the use of a computer. An immaterial thing can be used if at least one of its carriers is present. For example, the software tools on a computer.
Another example is the use of a particular name by a particular group of people over some span to identify a thing, such as a settlement. In this case, the physical carriers of this name are at least the people understanding its use."""@en ;
    rdfs:domain crm:E7_Activity ;
    rdfs:range crm:E70_Thing ;
    rdfs:subPropertyOf crm:P12_occurred_in_the_presence_of,
        crm:P15_was_influenced_by .

crm:P16i_was_used_for a rdf:Property ;
    rdfs:label "wurde benutzt für"@de,
        "χρησιμοποιήθηκε για"@el,
        "was used for"@en,
        "a été utilisé pour"@fr,
        "foi usado por"@pt,
        "был использован для"@ru ;
    rdfs:domain crm:E70_Thing ;
    rdfs:range crm:E7_Activity ;
    rdfs:subPropertyOf crm:P12i_was_present_at,
        crm:P15i_influenced .

crm:P31_has_modified a rdf:Property ;
    rdfs:label "veränderte"@de,
        "τροποποίησε"@el,
        "has modified"@en,
        "a modifié"@fr,
        "modificou"@pt,
        "изменил"@ru ;
    rdfs:comment """This property identifies the E24 Physical Man-Made Thing modified in an E11 Modification.
If a modification is applied to a non-man-made object, it is regarded as an E22 Man-Made Object from that time onwards. """@en ;
    rdfs:domain crm:E11_Modification ;
    rdfs:range crm:E24_Physical_Man-Made_Thing ;
    rdfs:subPropertyOf crm:P12_occurred_in_the_presence_of .

crm:P31i_was_modified_by a rdf:Property ;
    rdfs:label "wurde verändert durch"@de,
        "τροποποιήθηκε από"@el,
        "was modified by"@en,
        "a été modifié par"@fr,
        "foi modificada por"@pt,
        "был изменен посредством"@ru ;
    rdfs:domain crm:E24_Physical_Man-Made_Thing ;
    rdfs:range crm:E11_Modification ;
    rdfs:subPropertyOf crm:P12i_was_present_at .

gn:RDFData a owl:Class ;
    rdfs:label "RDF Data"@en ;
    rdfs:comment "A Document containing RDF description of one or several features."@en ;
    rdfs:subClassOf foaf:Document .

gn:alternateName a owl:DatatypeProperty ;
    rdfs:domain gn:Feature ;
    rdfs:subPropertyOf skos:altLabel .

geosparql:Feature a owl:Class ;
    rdfs:label "Feature"@en ;
    dc:contributor "Matthew Perry" ;
    dc:creator "OGC GeoSPARQL 1.0 Standard Working Group" ;
    dc:date "2011-06-16"^^xsd:date ;
    dc:description """      This class represents the top-level feature type. This class is 
      equivalent to GFI_Feature defined in ISO 19156:2011, and it is 
      superclass of all feature types.
    """@en ;
    rdfs:comment """      This class represents the top-level feature type. This class is 
      equivalent to GFI_Feature defined in ISO 19156:2011, and it is 
      superclass of all feature types.
    """@en ;
    rdfs:isDefinedBy <http://www.opengis.net/ont/geosparql>,
        <http://www.opengis.net/spec/geosparql/1.0> ;
    rdfs:subClassOf geosparql:SpatialObject ;
    owl:disjointWith geosparql:Geometry ;
    skos:definition """      This class represents the top-level feature type. This class is 
      equivalent to GFI_Feature defined in ISO 19156:2011, and it is 
      superclass of all feature types.
    """@en ;
    skos:prefLabel "Feature"@en .

skos:Collection a owl:Class ;
    rdfs:label "Collection"@en ;
    rdfs:isDefinedBy <http://www.w3.org/2004/02/skos/core> ;
    owl:disjointWith skos:Concept,
        skos:ConceptScheme ;
    skos:definition "A meaningful collection of concepts."@en ;
    skos:scopeNote "Labelled collections can be used where you would like a set of concepts to be displayed under a 'node label' in the hierarchy."@en .

foaf:isPrimaryTopicOf a rdf:Property,
        owl:InverseFunctionalProperty ;
    rdfs:label "is primary topic of" ;
    rdfs:comment "A document that this thing is the primary topic of." ;
    rdfs:domain owl:Thing ;
    rdfs:isDefinedBy foaf: ;
    rdfs:range foaf:Document ;
    rdfs:subPropertyOf foaf:page ;
    owl:inverseOf foaf:primaryTopic ;
    swvocab:term_status "stable" .

crmeh:EHE0007_Context a owl:Class ;
    rdfs:label "Context"@en ;
    rdfs:comment "This seems to be the best conceptual descriptor for what a context actually is. In this way, a cut is defined by a three-dimensional plane, a deposit or structure is described by a three-dimensional volume. A deposit or structure will also have some 'stuff' in the defined place i.e. the material that makes up the deposit or structure"@en ;
    rdfs:isDefinedBy crmeh:CRMEH ;
    rdfs:subClassOf crm:E53_Place ;
    owl:sameAs crmeh:EHE0007 ;
    skos:notation "EHE0007" .

crm:P14_carried_out_by a rdf:Property ;
    rdfs:label "wurde ausgeführt von"@de,
        "πραγματοποιήθηκε από"@el,
        "carried out by"@en,
        "réalisée par"@fr,
        "realizada por"@pt,
        "выполнялся"@ru ;
    rdfs:comment """This property describes the active participation of an E39 Actor in an E7 Activity. 
It implies causal or legal responsibility. The P14.1 in the role of property of the property allows the nature of an Actor’s participation to be specified."""@en ;
    rdfs:domain crm:E7_Activity ;
    rdfs:range crm:E39_Actor ;
    rdfs:subPropertyOf crm:P11_had_participant .

crm:P14i_performed a rdf:Property ;
    rdfs:label "führte aus"@de,
        "πραγματοποίησε"@el,
        "performed"@en,
        "a exécuté"@fr,
        "executou"@pt,
        "выполнял"@ru ;
    rdfs:domain crm:E39_Actor ;
    rdfs:range crm:E7_Activity ;
    rdfs:subPropertyOf crm:P11i_participated_in .

crm:P15_was_influenced_by a rdf:Property ;
    rdfs:label "wurde beeinflußt durch"@de,
        "επηρεάστηκε από"@el,
        "was influenced by"@en,
        "a été influencée par"@fr,
        "foi influenciado por "@pt,
        "находился под влиянием"@ru ;
    rdfs:comment """This is a high level property, which captures the relationship between an E7 Activity and anything that may have had some bearing upon it.
The property has more specific sub properties."""@en ;
    rdfs:domain crm:E7_Activity ;
    rdfs:range crm:E1_CRM_Entity .

crm:P15i_influenced a rdf:Property ;
    rdfs:label "beeinflußte"@de,
        "επηρέασε"@el,
        "influenced"@en,
        "a influencé"@fr,
        "influenciou"@pt,
        "оказал влияние на"@ru ;
    rdfs:domain crm:E1_CRM_Entity ;
    rdfs:range crm:E7_Activity .

crm:P93_took_out_of_existence a rdf:Property ;
    rdfs:label "beendete die Existenz von"@de,
        "αναίρεσε"@el,
        "took out of existence"@en,
        "a fait cesser d’exister"@fr,
        "cessou a existência de"@pt,
        "положил конец существованию"@ru ;
    rdfs:comment """This property allows an E64 End of Existence event to be linked to the E77 Persistent Item taken out of existence by it.
In the case of immaterial things, the E64 End of Existence is considered to take place with the destruction of the last physical carrier.
This allows an “end” to be attached to any Persistent Item being documented i.e. E70 Thing, E72 Legal Object, E39 Actor, E41 Appellation, E51 Contact Point and E55 Type. For many Persistent Items we know the maximum life-span and can infer, that they must have ended to exist. We assume in that case an End of Existence, which may be as unnoticeable as forgetting the secret knowledge by the last representative of some indigenous nation."""@en ;
    rdfs:domain crm:E64_End_of_Existence ;
    rdfs:range crm:E77_Persistent_Item ;
    rdfs:subPropertyOf crm:P12_occurred_in_the_presence_of .

crm:P93i_was_taken_out_of_existence_by a rdf:Property ;
    rdfs:label "wurde seiner Existenz beraubt durch"@de,
        "αναιρέθηκε από"@el,
        "was taken out of existence by"@en,
        "a cessé d’exister du fait de"@fr,
        "deixou de existir"@pt,
        "прекратил существование посредством"@ru ;
    rdfs:domain crm:E77_Persistent_Item ;
    rdfs:range crm:E64_End_of_Existence ;
    rdfs:subPropertyOf crm:P12i_was_present_at .

rdfs:label a rdf:Property ;
    rdfs:label "label" ;
    rdfs:comment "A human-readable name for the subject." ;
    rdfs:domain rdfs:Resource ;
    rdfs:isDefinedBy rdfs: ;
    rdfs:range rdfs:Literal .

skos:mappingRelation a rdf:Property,
        owl:ObjectProperty ;
    rdfs:label "is in mapping relation with"@en ;
    rdfs:comment "These concept mapping relations mirror semantic relations, and the data model defined below is similar (with the exception of skos:exactMatch) to the data model defined for semantic relations. A distinct vocabulary is provided for concept mapping relations, to provide a convenient way to differentiate links within a concept scheme from links between concept schemes. However, this pattern of usage is not a formal requirement of the SKOS data model, and relies on informal definitions of best practice."@en ;
    rdfs:isDefinedBy <http://www.w3.org/2004/02/skos/core> ;
    rdfs:subPropertyOf skos:semanticRelation ;
    skos:definition "Relates two concepts coming, by convention, from different schemes, and that have comparable meanings"@en .

skos:semanticRelation a rdf:Property,
        owl:ObjectProperty ;
    rdfs:label "is in semantic relation with"@en ;
    rdfs:domain skos:Concept ;
    rdfs:isDefinedBy <http://www.w3.org/2004/02/skos/core> ;
    rdfs:range skos:Concept ;
    skos:definition "Links a concept to a concept related by meaning."@en ;
    skos:scopeNote "This property should not be used directly, but as a super-property for all properties denoting a relationship of meaning between concepts."@en .

<https://joinup.ec.europa.eu/node/55858> dcterms:title "Core Vocabularies Specification" .

crm:P141_assigned a rdf:Property ;
    rdfs:label "wies zu"@de,
        "απέδωσε"@el,
        "assigned"@en,
        "a attribué"@fr,
        "atribuiu"@pt,
        "присвоил"@ru ;
    rdfs:comment "This property indicates the attribute that was assigned or the item that was related to the item denoted by a property P140 assigned attribute to in an Attribute assignment action."@en ;
    rdfs:domain crm:E13_Attribute_Assignment ;
    rdfs:range crm:E1_CRM_Entity .

crm:P141i_was_assigned_by a rdf:Property ;
    rdfs:label "wurde zugewiesen durch"@de,
        "αποδόθηκε από"@el,
        "was assigned by"@en,
        "a été attribué par"@fr,
        "foi atribuído por"@pt,
        "был присвоен посредством"@ru ;
    rdfs:domain crm:E1_CRM_Entity ;
    rdfs:range crm:E13_Attribute_Assignment .

crm:P67_refers_to a rdf:Property ;
    rdfs:label "verweist auf"@de,
        "αναφέρεται σε"@el,
        "refers to"@en,
        "fait référence à"@fr,
        "referencia"@pt,
        "ссылается на"@ru ;
    rdfs:comment "This property documents that an E89 Propositional Object makes a statement about an instance of E1 CRM Entity. P67 refers to (is referred to by) has the P67.1 has type link to an instance of E55 Type. This is intended to allow a more detailed description of the type of reference. This differs from P129 is about (is subject of), which describes the primary subject or subjects of the E89 Propositional Object."@en ;
    rdfs:domain crm:E89_Propositional_Object ;
    rdfs:range crm:E1_CRM_Entity .

crm:P67i_is_referred_to_by a rdf:Property ;
    rdfs:label "wird angeführt von"@de,
        "αναφέρεται από"@el,
        "is referred to by"@en,
        "est référencé par"@fr,
        "é referenciado por"@pt,
        "имеет ссылку на себя от"@ru ;
    rdfs:domain crm:E1_CRM_Entity ;
    rdfs:range crm:E89_Propositional_Object .

crm:P92_brought_into_existence a rdf:Property ;
    rdfs:label "brachte in Existenz"@de,
        "γέννησε"@el,
        "brought into existence"@en,
        "a fait exister"@fr,
        "trouxe à existência"@pt,
        "создал"@ru ;
    rdfs:comment """This property allows an E63 Beginning of Existence event to be linked to the E77 Persistent Item brought into existence by it.
It allows a “start” to be attached to any Persistent Item being documented i.e. E70 Thing, E72 Legal Object, E39 Actor, E41 Appellation, E51 Contact Point and E55 Type"""@en ;
    rdfs:domain crm:E63_Beginning_of_Existence ;
    rdfs:range crm:E77_Persistent_Item ;
    rdfs:subPropertyOf crm:P12_occurred_in_the_presence_of .

crm:P92i_was_brought_into_existence_by a rdf:Property ;
    rdfs:label "wurde in Existenz gebracht durch"@de,
        "γεννήθηκε από"@el,
        "was brought into existence by"@en,
        "a commencé à exister du fait de"@fr,
        "passou a existir por"@pt,
        "был создан посредством"@ru ;
    rdfs:domain crm:E77_Persistent_Item ;
    rdfs:range crm:E63_Beginning_of_Existence ;
    rdfs:subPropertyOf crm:P12i_was_present_at .

gn:parentFeature a owl:ObjectProperty,
        owl:TransitiveProperty ;
    rdfs:label "parent feature"@en ;
    rdfs:comment "A feature parent of the current one, in either administrative or physical subdivision."@en ;
    rdfs:domain gn:Feature ;
    rdfs:range gn:Feature .

rdf:value a rdf:Property ;
    rdfs:label "value" ;
    rdfs:comment "Idiomatic property used for structured values." ;
    rdfs:domain rdfs:Resource ;
    rdfs:isDefinedBy rdf: ;
    rdfs:range rdfs:Resource .

skos:ConceptScheme a owl:Class ;
    rdfs:label "Concept Scheme"@en ;
    rdfs:isDefinedBy <http://www.w3.org/2004/02/skos/core> ;
    owl:disjointWith skos:Concept ;
    skos:definition "A set of concepts, optionally including statements about semantic relationships between those concepts."@en ;
    skos:example "Thesauri, classification schemes, subject heading lists, taxonomies, 'folksonomies', and other types of controlled vocabulary are all examples of concept schemes. Concept schemes are also embedded in glossaries and terminologies."@en ;
    skos:scopeNote "A concept scheme may be defined to include concepts from different sources."@en .

foaf:nick a rdf:Property,
        owl:DatatypeProperty ;
    rdfs:label "nickname" ;
    rdfs:comment "A short informal nickname characterising an agent (includes login identifiers, IRC and other chat nicknames)." ;
    rdfs:isDefinedBy foaf: ;
    swvocab:term_status "testing" .

foaf:page a rdf:Property,
        owl:ObjectProperty ;
    rdfs:label "page" ;
    rdfs:comment "A page or document about this thing." ;
    rdfs:domain owl:Thing ;
    rdfs:isDefinedBy foaf: ;
    rdfs:range foaf:Document ;
    owl:inverseOf foaf:topic ;
    swvocab:term_status "stable" .

crmeh:EHE0008_ContextStuff a owl:Class ;
    rdfs:label "Context Stuff"@en ;
    rdfs:comment "If we see context as a definition of a place, then there also needs to be a physical presence of some material constellation in said place. The Context Stuff is created in this form by the Context Formation, and may be either destroyed by excavation or by later destructive investigation. It is regarded to exist as long as it preserves at least partially the geometric arrangement of particles it had at excavation time. See, e.g., the transfer of the Vasa ship to the museum built around it, and the later \"excavation\" of the inner hull"@en ;
    rdfs:isDefinedBy crmeh:CRMEH ;
    rdfs:subClassOf crm:E18_Physical_Thing ;
    owl:sameAs crmeh:EHE0008 ;
    skos:notation "EHE0008" .

crm:P1_is_identified_by a rdf:Property ;
    rdfs:label "wird bezeichnet als"@de,
        "αναγνωρίζεται ως"@el,
        "is identified by"@en,
        "est identifiée par"@fr,
        "é identificado por"@pt,
        "идентифицируется посредством"@ru ;
    rdfs:comment """This property describes the naming or identification of any real world item by a name or any other identifier. 
This property is intended for identifiers in general use, which form part of the world the model intends to describe, and not merely for internal database identifiers which are specific to a technical system, unless these latter also have a more general use outside the technical context. This property includes in particular identification by mathematical expressions such as coordinate systems used for the identification of instances of E53 Place. The property does not reveal anything about when, where and by whom this identifier was used. A more detailed representation can be made using the fully developed (i.e. indirect) path through E15 Identifier Assignment."""@en ;
    rdfs:domain crm:E1_CRM_Entity ;
    rdfs:range crm:E41_Appellation .

crm:P1i_identifies a rdf:Property ;
    rdfs:label "bezeichnet"@de,
        "είναι αναγνωριστικό"@el,
        "identifies"@en,
        "identifie"@fr,
        "identifica"@pt,
        "идентифицирует"@ru ;
    rdfs:domain crm:E41_Appellation ;
    rdfs:range crm:E1_CRM_Entity .

skos:note a rdf:Property,
        owl:AnnotationProperty ;
    rdfs:label "note"@en ;
    rdfs:isDefinedBy <http://www.w3.org/2004/02/skos/core> ;
    skos:definition "A general note, for any purpose."@en ;
    skos:scopeNote "This property may be used directly, or as a super-property for more specific note types."@en .

crm:P11_had_participant a rdf:Property ;
    rdfs:label "hatte Teilnehmer"@de,
        "είχε συμμέτοχο"@el,
        "had participant"@en,
        "a eu pour participant"@fr,
        "tem participante"@pt,
        "имел участника"@ru ;
    rdfs:comment """This property describes the active or passive participation of instances of E39 Actors in an E5 Event. 
It connects the life-line of the related E39 Actor with the E53 Place and E50 Date of the event. The property implies that the Actor was involved in the event but does not imply any causal relationship. The subject of a portrait can be said to have participated in the creation of the portrait."""@en ;
    rdfs:domain crm:E5_Event ;
    rdfs:range crm:E39_Actor ;
    rdfs:subPropertyOf crm:P12_occurred_in_the_presence_of .

crm:P11i_participated_in a rdf:Property ;
    rdfs:label "nahm Teil an"@de,
        "συμμετείχε σε"@el,
        "participated in"@en,
        "a participé à"@fr,
        "participa em"@pt,
        "участвовал в"@ru ;
    rdfs:domain crm:E39_Actor ;
    rdfs:range crm:E5_Event ;
    rdfs:subPropertyOf crm:P12i_was_present_at .

gn:featureCode a owl:ObjectProperty ;
    rdfs:label "feature code"@en ;
    rdfs:comment "Type of the feature, as defined in geonames taxonomy."@en ;
    rdfs:domain gn:Feature ;
    rdfs:range gn:Code ;
    rdfs:subPropertyOf dcterms:type .

dcterms:date a rdf:Property ;
    rdfs:label "Date"@en ;
    dcterms:description "Date may be used to express temporal information at any level of granularity.  Recommended best practice is to use an encoding scheme, such as the W3CDTF profile of ISO 8601 [W3CDTF]."@en ;
    dcterms:hasVersion history:dateT-001 ;
    dcterms:issued "2008-01-14"^^xsd:date ;
    dcterms:modified "2008-01-14"^^xsd:date ;
    rdfs:comment "A point or period of time associated with an event in the lifecycle of the resource."@en ;
    rdfs:isDefinedBy dcterms: ;
    rdfs:range rdfs:Literal ;
    rdfs:subPropertyOf dc:date .

crm:P12_occurred_in_the_presence_of a rdf:Property ;
    rdfs:label "fand statt im Beisein von"@de,
        "συνέβη παρουσία του/της"@el,
        "occurred in the presence of"@en,
        "est arrivé en présence de"@fr,
        "ocorreu na presença de"@pt,
        "появился в присутствии"@ru ;
    rdfs:comment """This property describes the active or passive presence of an E77 Persistent Item in an E5 Event without implying any specific role. 
It connects the history of a thing with the E53 Place and E50 Date of an event. For example, an object may be the desk, now in a museum on which a treaty was signed. The presence of an immaterial thing implies the presence of at least one of its carriers."""@en ;
    rdfs:domain crm:E5_Event ;
    rdfs:range crm:E77_Persistent_Item .

crm:P12i_was_present_at a rdf:Property ;
    rdfs:label "war anwesend bei"@de,
        "ήταν παρών/παρούσα/παρόν σε"@el,
        "was present at"@en,
        "était présent à"@fr,
        "estava presente no"@pt,
        "присутствовал при"@ru ;
    rdfs:domain crm:E77_Persistent_Item ;
    rdfs:range crm:E5_Event .

dc:date a rdf:Property,
        owl:AnnotationProperty ;
    rdfs:label "Date"@en ;
    dcterms:description "Date may be used to express temporal information at any level of granularity.  Recommended best practice is to use an encoding scheme, such as the W3CDTF profile of ISO 8601 [W3CDTF]."@en ;
    dcterms:hasVersion history:date-006 ;
    dcterms:issued "1999-07-02"^^xsd:date ;
    dcterms:modified "2008-01-14"^^xsd:date ;
    rdfs:comment "A point or period of time associated with an event in the lifecycle of the resource."@en ;
    rdfs:isDefinedBy dc: ;
    skos:note "A second property with the same name as this property has been declared in the dcterms: namespace (http://purl.org/dc/terms/).  See the Introduction to the document \"DCMI Metadata Terms\" (http://dublincore.org/documents/dcmi-terms/) for an explanation."@en .

gn:Class a owl:Class ;
    rdfs:label "Class"@en ;
    rdfs:comment "A class of features."@en ;
    rdfs:subClassOf skos:ConceptScheme .

skos:Concept a owl:Class ;
    rdfs:label "Concept",
        "Concept"@en ;
    rdfs:isDefinedBy <http://www.w3.org/2004/02/skos/core> ;
    skos:definition "An idea or notion; a unit of thought."@en .

geosparql:Geometry a owl:Class ;
    rdfs:label "Geometry"@en ;
    dc:contributor "Matthew Perry" ;
    dc:creator "OGC GeoSPARQL 1.0 Standard Working Group" ;
    dc:date "2011-06-16"^^xsd:date ;
    dc:description """      The class represents the top-level geometry type. This class is 
      equivalent to the UML class GM_Object defined in ISO 19107, and 
      it is superclass of all geometry types.
    """@en ;
    rdfs:comment """      The class represents the top-level geometry type. This class is 
      equivalent to the UML class GM_Object defined in ISO 19107, and 
      it is superclass of all geometry types.
    """@en ;
    rdfs:isDefinedBy <http://www.opengis.net/ont/geosparql>,
        <http://www.opengis.net/spec/geosparql/1.0> ;
    rdfs:subClassOf geosparql:SpatialObject ;
    owl:disjointWith geosparql:Feature ;
    skos:definition """      The class represents the top-level geometry type. This class is 
      equivalent to the UML class GM_Object defined in ISO 19107, and 
      it is superclass of all geometry types.
    """@en ;
    skos:prefLabel "Geometry"@en .

dc:relation a rdf:Property ;
    rdfs:label "Relation"@en ;
    dcterms:description "Recommended best practice is to identify the related resource by means of a string conforming to a formal identification system. "@en ;
    dcterms:hasVersion history:relation-006 ;
    dcterms:issued "1999-07-02"^^xsd:date ;
    dcterms:modified "2008-01-14"^^xsd:date ;
    rdfs:comment "A related resource."@en ;
    rdfs:isDefinedBy dc: ;
    skos:note "A second property with the same name as this property has been declared in the dcterms: namespace (http://purl.org/dc/terms/).  See the Introduction to the document \"DCMI Metadata Terms\" (http://dublincore.org/documents/dcmi-terms/) for an explanation."@en .

dcterms:relation a rdf:Property ;
    rdfs:label "Relation"@en ;
    dcterms:description "Recommended best practice is to identify the related resource by means of a string conforming to a formal identification system. "@en ;
    dcterms:hasVersion history:relationT-001 ;
    dcterms:issued "2008-01-14"^^xsd:date ;
    dcterms:modified "2008-01-14"^^xsd:date ;
    rdfs:comment "A related resource."@en ;
    rdfs:isDefinedBy dcterms: ;
    rdfs:subPropertyOf dc:relation ;
    skos:note "This term is intended to be used with non-literal values as defined in the DCMI Abstract Model (http://dublincore.org/documents/abstract-model/).  As of December 2007, the DCMI Usage Board is seeking a way to express this intention with a formal range declaration."@en .

dc: dcterms:modified "2012-06-14"^^xsd:date ;
    dcterms:publisher <http://purl.org/dc/aboutdcmi#DCMI> ;
    dcterms:title "Dublin Core Metadata Element Set, Version 1.1"@en .

rdfs: a owl:Ontology ;
    dc:title "The RDF Schema vocabulary (RDFS)" ;
    rdfs:seeAlso <http://www.w3.org/2000/01/rdf-schema-more> .

gn:P a gn:Class ;
    rdfs:comment "city, village,..."@en .

gn:V a gn:Class ;
    rdfs:comment "forest, heath, ..."@en .

<http://www.w3.org/ns/locn> a voaf:Vocabulary,
        owl:Ontology ;
    rdfs:label "ISA Programme Location Core Vocabulary"@en ;
    ns:attributionName "European Commission"@en ;
    ns:attributionURL eu: ;
    dcterms:abstract "The ISA Programme Location Core Vocabulary provides a minimum set of classes and properties for describing any place in terms of its name, address or geometry. The vocabulary is specifically designed to aid the publication of data that is interoperable with EU INSPIRE Directive. It is closely integrated with the Business and Person Core Vocabularies of the EU ISA Programme, now available in W3C space as, respectively, the Registered Organization vocabulary and ISA Person Core Vocabulary."@en ;
    dcterms:conformsTo <https://joinup.ec.europa.eu/node/43160> ;
    dcterms:hasFormat <http://www.w3.org/ns/locn.html>,
        <http://www.w3.org/ns/locn.rdf>,
        <http://www.w3.org/ns/locn.ttl> ;
    dcterms:issued "2013-11-25"^^xsd:date ;
    dcterms:license licence:isa-open-metadata-licence-v11 ;
    dcterms:mediator [ foaf:homepage <http://www.w3.org/community/locadd/> ;
            foaf:mbox <mailto:public-locadd@w3.org> ;
            foaf:name "Locations and Addresses Community Group" ] ;
    dcterms:modified "2015-03-23"^^xsd:date ;
    dcterms:rights "Copyright © European Union, 2012-2015."@en ;
    dcterms:title "ISA Programme Location Core Vocabulary"@en ;
    vann:changes """
2015-03-23: Updates in the namespace document and in the RDF/XML and Turtle schemas:
- Fixed copyright notice.
- Added class and property diagram.
- Updated GeoSPARQL (a) namespace URIs  and (b) datatype names in the examples of property locn:geometry, based on version 1.0 of the GeoSPARQL specification, and added a note in the examples.
  - prefix ogc (http://www.opengis.net/rdf#) replaced with gsp (http://www.opengis.net/ont/geosparql#) and sf (http://www.opengis.net/ont/sf#)
  - ogc:WKTLiteral → gsp:wktLiteral
  - ogc:GMLLiteral → gsp:gmlLiteral
- Added namespace declarations for all namespace prefixes used in LOCN namespace document, even though they are not used in class/property definitions.
- Corrected the endonym of the Greek capital written in the Greek script in the definition of class locn:geographicName (Aθnνa → Αθήνα).
- Fixed links and typos, minor revisions made to the textual descriptions.
2013-12-21: (PhilA) Update in RDF/XML and Turtle schemas:
- Updated voaf namespace.
- Corrected links to different distributions of the schema.
- Removed xml:base and used http://www/w3/org/ns/locn as the schema URI cf. original which used the namespace URI (with the final # character).
2013-11-25: Changes since final draft version released by the EU ISA Programme Core Vocabularies Working Group (Location Task Force)
- Revised usage note of class locn:Geometry. The text describing its recommended usage has been moved to usage note of property locn:geometry.
- Dropped domain/range restriction for locn:geographicName.
- Dropped domain/range restriction for locn:locatorDesignator. Free text definition updated accordingly.
- Dropped domain/range restriction for locn:locatorName. Free text definition updated accordingly.
- Corrected free text definition of property locn:geometry (its domain is "any resource", and not a "location").
- Revised usage note of property locn:geometry to include text about recommended usage, formerly included in the usage note of class locn:Geometry.
- Revised usage note and examples of property locn:geometry to include support to geocoded URIs (e.g., geo URIs, GeoHash URIs).
- Added term status. All terms have been set to "testing", with the exception of class locn:Geometry and properties rdfs:seeAlso (geographic identifier) and locn:addressId.
- Renamed subject in Turtle examples (ex:a → :Resource).
- Fixed links and typos, minor revisions made to the textual descriptions.
    """@en ;
    vann:preferredNamespacePrefix "locn" ;
    vann:preferredNamespaceUri "http://www.w3.org/ns/locn#"^^xsd:anyURI ;
    voaf:classNumber "3"^^xsd:nonNegativeInteger ;
    voaf:propertyNumber "16"^^xsd:nonNegativeInteger ;
    voaf:reliesOn dcterms:,
        rdfs: ;
    rdfs:comment "This is a new version of the final draft published by the European Commission in May 2012, revised according to the results of the ISA Core Location Pilot (see Section Change History for the list of changes). It is currently under the control of the Locations and Addresses Community Group, but is not under active development or review. Comments and queries should be sent to that group via public-locadd@w3.org. Terms defined here may be deprecated by that or future groups but will not disappear or their definition change."@en ;
    ns2:editor [ org:affiliation [ foaf:homepage jrc: ;
                    foaf:name "European Commission - Joint Research Centre (JRC)"@en ] ;
            foaf:name "Michael Lutz" ],
        [ org:affiliation [ foaf:homepage <http://www.w3.org/> ;
                    foaf:name "W3C/ERCIM" ] ;
            rdfs:seeAlso <http://philarcher.org/foaf.rdf#me> ;
            foaf:homepage <http://philarcher.org/> ;
            foaf:name "Phil Archer" ],
        [ org:affiliation [ foaf:homepage jrc: ;
                    foaf:name "European Commission - Joint Research Centre (JRC)"@en ] ;
            rdfs:seeAlso <http://andrea-perego.name/foaf/#me> ;
            foaf:homepage <http://about.me/andrea.perego> ;
            foaf:name "Andrea Perego" ] ;
    owl:versionInfo "First version in w3.org/ns space"@en ;
    powder-s:describedby <https://joinup.ec.europa.eu/node/55858> ;
    foaf:depiction <http://www.w3.org/ns/locn.svg> ;
    foaf:maker [ foaf:homepage <https://joinup.ec.europa.eu/node/42444> ;
            foaf:name "EU ISA Programme Core Vocabularies Working Group (Location Task Force)" ] .

rdf: a owl:Ontology ;
    dc:description "This is the RDF Schema for the RDF vocabulary terms in the RDF Namespace, defined in RDF 1.1 Concepts." ;
    dc:title "The RDF Concepts Vocabulary (RDF)" .

gn:A a gn:Class ;
    rdfs:comment "country, state, region ..."@en .

gn:R a gn:Class ;
    rdfs:comment "road, railroad, ..."@en .

gn:Feature a owl:Class ;
    rdfs:label "Feature"@en ;
    rdfs:comment "A geographical feature"@en ;
    rdfs:subClassOf org:Place,
        wgs84:SpatialThing ;
    owl:equivalentClass <http://geovocab.org/spatial#Feature>,
        <http://www.mindswap.org/2003/owl/geo/geoFeatures20040307.owl#GeographicFeature> ;
    skos:historyNote "Modified in version 3.1 : The cardinality constraints on feature code, feature class are relaxed on this class, and put on the specific subclass Geonames Feature. This class and attached properties can therefore be used for features not necessarily identified in the Geoanmes data base"@en .

<http://www.w3.org/2004/02/skos/core> a owl:Ontology ;
    dcterms:contributor "Dave Beckett",
        "Nikki Rogers",
        "Participants in W3C's Semantic Web Deployment Working Group." ;
    dcterms:creator "Alistair Miles",
        "Sean Bechhofer" ;
    dcterms:description "An RDF vocabulary for describing the basic structure and content of concept schemes such as thesauri, classification schemes, subject heading lists, taxonomies, 'folksonomies', other types of controlled vocabulary, and also concept schemes embedded in glossaries and terminologies."@en ;
    dcterms:title "SKOS Vocabulary"@en ;
    rdfs:seeAlso <http://www.w3.org/TR/skos-reference/> .

owl:Thing a owl:Class ;
    rdfs:label "Thing" ;
    rdfs:comment "The class of OWL individuals." ;
    rdfs:isDefinedBy owl: .

<http://www.opengis.net/ont/geosparql> a owl:Ontology ;
    dc:creator "Open Geospatial Consortium" ;
    dc:date "2012-04-30"^^xsd:date ;
    dc:description "An RDF/OWL vocabulary for representing spatial information" ;
    dc:source <http://www.opengis.net/doc/IS/geosparql/1.0>,
        "OGC GeoSPARQL – A Geographic Query Language for RDF Data OGC 11-052r5" ;
    rdfs:seeAlso <http://www.opengis.net/def/function/ogc-geosparql/1.0>,
        <http://www.opengis.net/def/rule/ogc-geosparql/1.0>,
        <http://www.opengis.net/doc/IS/geosparql/1.0> ;
    owl:imports dc:,
        <http://www.opengis.net/ont/gml>,
        <http://www.opengis.net/ont/sf>,
        <http://www.w3.org/2004/02/skos/core> ;
    owl:versionInfo "OGC GeoSPARQL 1.0" .

gn:L a gn:Class ;
    rdfs:comment "parks,area, ..."@en .

geosparql:SpatialObject a owl:Class ;
    rdfs:label "SpatialObject"@en ;
    dc:contributor "Matthew Perry" ;
    dc:creator "OGC GeoSPARQL 1.0 Standard Working Group" ;
    dc:date "2011-06-16"^^xsd:date ;
    dc:description """      The class spatial-object represents everything that can have 
      a spatial representation. It is superclass of feature and geometry.
    """@en ;
    rdfs:comment """      The class spatial-object represents everything that can have 
      a spatial representation. It is superclass of feature and geometry.
    """@en ;
    rdfs:isDefinedBy <http://www.opengis.net/ont/geosparql>,
        <http://www.opengis.net/spec/geosparql/1.0> ;
    skos:definition """      The class spatial-object represents everything that can have 
      a spatial representation. It is superclass of feature and geometry.
    """@en ;
    skos:prefLabel "SpatialObject"@en .

gn:U a gn:Class ;
    rdfs:comment "undersea"@en .

foaf: a owl:Ontology ;
    dc:description "The Friend of a Friend (FOAF) RDF vocabulary, described using W3C RDF Schema and the Web Ontology Language." ;
    dc:title "Friend of a Friend (FOAF) vocabulary" .

gn:T a gn:Class ;
    rdfs:comment "mountain, hill, rock, ..."@en .

dcterms: dcterms:modified "2012-06-14"^^xsd:date ;
    dcterms:publisher <http://purl.org/dc/aboutdcmi#DCMI> ;
    dcterms:title "DCMI Metadata Terms - other"@en .

gn:H a gn:Class ;
    rdfs:comment "stream, lake, ..."@en .

crmeh:CRMEH a owl:Ontology ;
    rdfs:label "CRMEH"@en ;
    dcterms:created "2007-04-17"@en ;
    dcterms:creator "Ceri Binding, University of South Wales"@en ;
    dcterms:description "English Heritage extensions to CIDOC CRM v5.0.4 expressed in RDF, for the archaeology domain"@en ;
    dcterms:language "en"@en ;
    dcterms:modified "2014-10-29"@en ;
    dcterms:requires <http://www.cidoc-crm.org/rdfs/cidoc_crm_v5.0.4_official_release.rdfs> ;
    dcterms:title "CRMEH"@en ;
    rdfs:comment """English Heritage extensions to CIDOC CRM expressed in RDF, for the archaeology domain. Naming and numbering; identifiers UIDs assigned according to the following scheme:
EHE0xxx – objects and places, concepts representing real-world entities
EHE1xxx – events in the past
EHE2xxx – events in the present
UIDs have been assigned initially using an alphabetised list of entities. Where additional entities have been inserted into the model, they have been assigned UIDs from the end of the appropriate numbering sequence with existing UIDs retained: No renumbering of existing entities should occur. To this end, the number allocation blocks comprise 999 UIDs in each sequence to allow room for expansion.
Naming convention follows broadly OO principles in that names are formed according to the relationships an object participates in. Core entities are named using natural language names that are easily understood eg Group, Context or Find. Associated entities are then named accordingly. For example, if we take a Group, an event relating to this group would be referred to as a GroupEvent. The record of such an event taking place would be a GroupEventRecord and an associated note would be referred to as a GroupEventRecordNote. If this note was classified by type the classification would be a GroupEventRecordNoteType. Similarly, if we take a Find (referred to as a ContextFind in the model in order to reinforce the idea that all finds originate from a context, even if the context is unknown), then we can see that it was produced as part of a ContextFindProductionEvent which took place at a ContextFindProductionEventLocation."""@en ;
    owl:imports <http://www.cidoc-crm.org/rdfs/cidoc_crm_v5.0.4_official_release.rdfs> ;
    owl:versionInfo "20141029"@en .

gn:S a gn:Class ;
    rdfs:comment "spot, building, farm, ..."@en .

gn:Code a owl:Class ;
    rdfs:label "Code"@en ;
    rdfs:comment "A feature code."@en ;
    rdfs:subClassOf skos:Concept .

